<?xml version="1.0"?><rdf:RDF 	xmlns:rdf="http://www.w3.org/1999/02/22-rdf-syntax-ns#" 	xmlns:skos="http://www.w3.org/2004/02/skos/core#" 	xmlns:dc="http://purl.org/dc/terms/" 	xmlns:foaf="http://xmlns.com/foaf/0.1/" 	xmlns:cito="http://purl.org/net/cito/"> <skos:Concept rdf:about="http://www.cognitiveatlas.org/id/trm_4a3fd79d09b6d"> <dc:identifier>trm_4a3fd79d09b6d</dc:identifier>
		<dc:Title>Cognitive Atlas : Lexicon : backward masking</dc:Title>
		<dc:Description>RDF output for 'backward masking'</dc:Description>
		<dc:Type>InteractiveResource</dc:Type>
		<dc:Publisher>Cognitive Atlas</dc:Publisher>
		<dc:Creator>Cognitive Atlas RDF Generator</dc:Creator>
		<dc:Contributor>Brenda Gregory</dc:Contributor>
		<dc:Date>2011-04-28 16:12:37</dc:Date>
		<dc:Format>text/rdf</dc:Format>
		<dc:Language>en</dc:Language>
		<skos:editorialNote>Generated by testgenall.php on Thu Mar 29 10:24:07 PDT 2012.</skos:editorialNote>
		<skos:historyNote>Revision 3: 2 previous definitions.</skos:historyNote>
		<skos:changeNote>See http://www.cognitiveatlas.org/id/trm_4a3fd79d09b6d for complete revision history.</skos:changeNote>
		<skos:scopeNote>http://www.w3.org/2004/02/skos/core#Concept</skos:scopeNote>
		<skos:Note>SKOS properties defined in http://www.w3.org/TR/skos-primer/#secrel</skos:Note>
		<skos:inScheme rdf:resource="http://www.cognitiveatlas.org/tasks/"/>
		<skos:definition>a phenomenon wherein presenting one stimulus (a &#34;mask&#34; or &#34;masking stimulus&#34;) immediately after another brief (≤ 50 ms) &#34;target&#34; stimulus leads to a failure to consciously perceive the first stimulus.</skos:definition>
		<skos:prefLabel>backward masking</skos:prefLabel>
		<skos:altLabel></skos:altLabel>
</skos:Concept><skos:Concept rdf:about="http://www.cognitiveatlas.org/id/trm_4a3fd79d0b3d7"> <dc:identifier>trm_4a3fd79d0b3d7</dc:identifier>
		<dc:Title>Cognitive Atlas : Lexicon : trace conditioning</dc:Title>
		<dc:Description>RDF output for 'trace conditioning'</dc:Description>
		<dc:Type>InteractiveResource</dc:Type>
		<dc:Publisher>Cognitive Atlas</dc:Publisher>
		<dc:Creator>Cognitive Atlas RDF Generator</dc:Creator>
		<dc:Contributor>Brenda Gregory</dc:Contributor>
		<dc:Date>2011-04-29 10:51:16</dc:Date>
		<dc:Format>text/rdf</dc:Format>
		<dc:Language>en</dc:Language>
		<skos:editorialNote>Generated by testgenall.php on Thu Mar 29 10:24:07 PDT 2012.</skos:editorialNote>
		<skos:historyNote>Revision 3: 2 previous definitions.</skos:historyNote>
		<skos:changeNote>See http://www.cognitiveatlas.org/id/trm_4a3fd79d0b3d7 for complete revision history.</skos:changeNote>
		<skos:scopeNote>http://www.w3.org/2004/02/skos/core#Concept</skos:scopeNote>
		<skos:Note>SKOS properties defined in http://www.w3.org/TR/skos-primer/#secrel</skos:Note>
		<skos:inScheme rdf:resource="http://www.cognitiveatlas.org/tasks/"/>
		<skos:definition>a form of classical conditioning in which the presentation of the conditioned stimulus and the unconditioned stimulus is separated in time by an interstimulus interval.</skos:definition>
		<skos:prefLabel>trace conditioning</skos:prefLabel>
		<skos:altLabel></skos:altLabel>
		<cito:citesForInformation rdf:resource="http://www.cognitiveatlas.org/citation/id/cit_4dbaf9ccb868b"/>
</skos:Concept><skos:Concept rdf:about="http://www.cognitiveatlas.org/id/trm_4af89b3a925ca"> <dc:identifier>trm_4af89b3a925ca</dc:identifier>
		<dc:Title>Cognitive Atlas : Lexicon : Vandenberg & Kuse Tasks</dc:Title>
		<dc:Description>RDF output for 'Vandenberg & Kuse Tasks'</dc:Description>
		<dc:Type>InteractiveResource</dc:Type>
		<dc:Publisher>Cognitive Atlas</dc:Publisher>
		<dc:Creator>Cognitive Atlas RDF Generator</dc:Creator>
		<dc:Contributor>Christian Battista</dc:Contributor>
		<dc:Date>2009-11-09 14:44:10</dc:Date>
		<dc:Format>text/rdf</dc:Format>
		<dc:Language>en</dc:Language>
		<skos:editorialNote>Generated by testgenall.php on Thu Mar 29 10:24:07 PDT 2012.</skos:editorialNote>
		<skos:historyNote>No previous definition revisions.</skos:historyNote>
		<skos:changeNote>This is the first and only definition provided.</skos:changeNote>
		<skos:scopeNote>http://www.w3.org/2004/02/skos/core#Concept</skos:scopeNote>
		<skos:Note>SKOS properties defined in http://www.w3.org/TR/skos-primer/#secrel</skos:Note>
		<skos:inScheme rdf:resource="http://www.cognitiveatlas.org/tasks/"/>
		<skos:definition>Paper and pencil Test of mental rotation ability.  Participants must are presented with four 3-D block figures and must select 2 from the group which match a reference figure.  This test is administered under time contraints.  A male advantage is typically seen on this type of task, as measured by test accuracy.</skos:definition>
		<skos:prefLabel>Vandenberg & Kuse Tasks</skos:prefLabel>
		<skos:altLabel></skos:altLabel>
		<skos:related rdf:resource="http://www.cognitiveatlas.org/id/trm_4c8990810541d"/>
		<skos:related rdf:resource="http://www.cognitiveatlas.org/id/trm_4a3fd79d0b1a6"/>
		<skos:related rdf:resource="http://www.cognitiveatlas.org/id/trm_4a3fd79d0b1a6"/>
		<skos:related rdf:resource="http://www.cognitiveatlas.org/id/trm_4a3fd79d0a914"/>
		<skos:example>Mental Rotation Task is a broader synonym of Vandenberg & Kuse Tasks</skos:example>
		<skos:example>spatial ability is measured by the contrast of average time of men minus average time of women trials in the Vandenberg & Kuse Tasks</skos:example>
		<skos:example>spatial ability is measured by the contrast of areas of activation during task minus baseline trials in the Vandenberg & Kuse Tasks</skos:example>
		<skos:example>mental rotation is measured by the contrast of participant&#39;s time minus average time trials in the Vandenberg & Kuse Tasks</skos:example>
		<cito:citesForInformation rdf:resource="http://www.cognitiveatlas.org/citation/id/cit_4af89b79c6709"/>
		<cito:citesForInformation rdf:resource="http://www.cognitiveatlas.org/citation/id/cit_4dffde6cdeade"/>
		<cito:citesForInformation rdf:resource="http://www.cognitiveatlas.org/citation/id/cit_4dffde9649276"/>
</skos:Concept><skos:Concept rdf:about="http://www.cognitiveatlas.org/id/trm_4b1968619b00b"> <dc:identifier>trm_4b1968619b00b</dc:identifier>
		<dc:Title>Cognitive Atlas : Lexicon : Color-word Stroop Task</dc:Title>
		<dc:Description>RDF output for 'Color-word Stroop Task'</dc:Description>
		<dc:Type>InteractiveResource</dc:Type>
		<dc:Publisher>Cognitive Atlas</dc:Publisher>
		<dc:Creator>Cognitive Atlas RDF Generator</dc:Creator>
		<dc:Contributor>Russ Poldrack</dc:Contributor>
		<dc:Date>2012-01-28 12:02:06</dc:Date>
		<dc:Format>text/rdf</dc:Format>
		<dc:Language>en</dc:Language>
		<skos:editorialNote>Generated by testgenall.php on Thu Mar 29 10:24:07 PDT 2012.</skos:editorialNote>
		<skos:historyNote>Revision 4: 3 previous definitions.</skos:historyNote>
		<skos:changeNote>See http://www.cognitiveatlas.org/id/trm_4b1968619b00b for complete revision history.</skos:changeNote>
		<skos:scopeNote>http://www.w3.org/2004/02/skos/core#Concept</skos:scopeNote>
		<skos:Note>SKOS properties defined in http://www.w3.org/TR/skos-primer/#secrel</skos:Note>
		<skos:inScheme rdf:resource="http://www.cognitiveatlas.org/tasks/"/>
		<skos:definition>A task in which single words (including names of colors) are presented in colored ink, and the subject is asked to name the color of the ink as quickly as possible. The ink color may either match or conflict with the color name. Accuracy and response time are measured.</skos:definition>
		<skos:prefLabel>Color-word Stroop Task</skos:prefLabel>
		<skos:altLabel>Stroop color-word task, Stroop color-word interference task, Stroop color naming task</skos:altLabel>
		<skos:related rdf:resource="http://www.cognitiveatlas.org/id/trm_4a3fd79d0af66"/>
		<skos:related rdf:resource="http://www.cognitiveatlas.org/id/trm_4a3fd79d0af66"/>
		<skos:related rdf:resource="http://www.cognitiveatlas.org/id/trm_4a3fd79d0af66"/>
		<skos:related rdf:resource="http://www.cognitiveatlas.org/id/trm_4a3fd79d0a038"/>
		<skos:related rdf:resource="http://www.cognitiveatlas.org/id/tsk_4a57abb949e27"/>
		<skos:related rdf:resource="http://www.cognitiveatlas.org/id/tsk_4a57abb949e27"/>
		<skos:example>Color-word Stroop Task is descended from Stroop task</skos:example>
		<skos:example>Color-word Stroop Task is a narrower synonym of Stroop task</skos:example>
		<skos:example>response inhibition is measured by the contrast of Incongruent trials in the Color-word Stroop Task</skos:example>
		<skos:example>response inhibition is measured by the contrast of Incongruent - Congruent trials in the Color-word Stroop Task</skos:example>
		<skos:example>response inhibition is measured by the contrast of Incongruent - Neutral trials in the Color-word Stroop Task</skos:example>
		<skos:example>decision making is measured by the contrast of  trials in the Color-word Stroop Task</skos:example>
		<cito:citesForInformation rdf:resource="http://www.cognitiveatlas.org/citation/id/cit_4b1968a44c363"/>
		<cito:citesForInformation rdf:resource="http://www.cognitiveatlas.org/citation/id/cit_4de7ba5e5f0ff"/>
</skos:Concept><skos:Concept rdf:about="http://www.cognitiveatlas.org/id/trm_4b4a537644d76"> <dc:identifier>trm_4b4a537644d76</dc:identifier>
		<dc:Title>Cognitive Atlas : Lexicon : Continuous Performance Task</dc:Title>
		<dc:Description>RDF output for 'Continuous Performance Task'</dc:Description>
		<dc:Type>InteractiveResource</dc:Type>
		<dc:Publisher>Cognitive Atlas</dc:Publisher>
		<dc:Creator>Cognitive Atlas RDF Generator</dc:Creator>
		<dc:Contributor>Russ Poldrack</dc:Contributor>
		<dc:Date>2011-08-10 07:27:22</dc:Date>
		<dc:Format>text/rdf</dc:Format>
		<dc:Language>en</dc:Language>
		<skos:editorialNote>Generated by testgenall.php on Thu Mar 29 10:24:07 PDT 2012.</skos:editorialNote>
		<skos:historyNote>Revision 2: 1 previous definitions.</skos:historyNote>
		<skos:changeNote>See http://www.cognitiveatlas.org/id/trm_4b4a537644d76 for complete revision history.</skos:changeNote>
		<skos:scopeNote>http://www.w3.org/2004/02/skos/core#Concept</skos:scopeNote>
		<skos:Note>SKOS properties defined in http://www.w3.org/TR/skos-primer/#secrel</skos:Note>
		<skos:inScheme rdf:resource="http://www.cognitiveatlas.org/tasks/"/>
		<skos:definition>A task in which subjects are presented with a stream of letters, and must respond to one of the letters and refrain from responding to any other letters.</skos:definition>
		<skos:prefLabel>Continuous Performance Task</skos:prefLabel>
		<skos:altLabel>CPT</skos:altLabel>
		<skos:related rdf:resource="http://www.cognitiveatlas.org/id/tsk_4a57abb949bcd"/>
		<skos:related rdf:resource="http://www.cognitiveatlas.org/id/trm_4c40d22c8a69d"/>
		<skos:related rdf:resource="http://www.cognitiveatlas.org/id/trm_4a3fd79d0b5ef"/>
		<skos:example>n-back task is descended from Continuous Performance Task</skos:example>
		<skos:example> is an exact synonym of Continuous Performance Task</skos:example>
		<skos:example>attentional focusing is measured by the contrast of Target trials in the Continuous Performance Task</skos:example>
		<cito:citesForInformation rdf:resource="http://www.cognitiveatlas.org/citation/id/cit_4b50c39646c37"/>
		<cito:citesForInformation rdf:resource="http://www.cognitiveatlas.org/citation/id/cit_4de7c16c78382"/>
		<cito:citesForInformation rdf:resource="http://www.cognitiveatlas.org/citation/id/cit_4de7c139bf72e"/>
</skos:Concept><skos:Concept rdf:about="http://www.cognitiveatlas.org/id/trm_4b65e5e2ab3ca"> <dc:identifier>trm_4b65e5e2ab3ca</dc:identifier>
		<dc:Title>Cognitive Atlas : Lexicon : word-picture verification task</dc:Title>
		<dc:Description>RDF output for 'word-picture verification task'</dc:Description>
		<dc:Type>InteractiveResource</dc:Type>
		<dc:Publisher>Cognitive Atlas</dc:Publisher>
		<dc:Creator>Cognitive Atlas RDF Generator</dc:Creator>
		<dc:Contributor>Joseph Devlin</dc:Contributor>
		<dc:Date>2010-01-31 12:19:46</dc:Date>
		<dc:Format>text/rdf</dc:Format>
		<dc:Language>en</dc:Language>
		<skos:editorialNote>Generated by testgenall.php on Thu Mar 29 10:24:07 PDT 2012.</skos:editorialNote>
		<skos:historyNote>No previous definition revisions.</skos:historyNote>
		<skos:changeNote>This is the first and only definition provided.</skos:changeNote>
		<skos:scopeNote>http://www.w3.org/2004/02/skos/core#Concept</skos:scopeNote>
		<skos:Note>SKOS properties defined in http://www.w3.org/TR/skos-primer/#secrel</skos:Note>
		<skos:inScheme rdf:resource="http://www.cognitiveatlas.org/tasks/"/>
		<skos:definition>is an experimental paradigm where a picture of an object is presented along with either an auditory or written word and participants indicate whether the word and the picture refer to the same concept.  It is typically used as a test of semantic memory integrity.</skos:definition>
		<skos:prefLabel>word-picture verification task</skos:prefLabel>
		<skos:altLabel></skos:altLabel>
		<skos:related rdf:resource="http://www.cognitiveatlas.org/id/trm_4a3fd79d0b077"/>
		<skos:related rdf:resource="http://www.cognitiveatlas.org/id/trm_4a3fd79d0b87a"/>
		<skos:example>semantic knowledge is measured by the contrast of accuracy of participant minus average accuracy of controls trials in the word-picture verification task</skos:example>
		<skos:example>semantic processing is measured by the contrast of response time to non-matching minus response time to matching trials in the word-picture verification task</skos:example>
		<cito:citesForInformation rdf:resource="http://www.cognitiveatlas.org/citation/id/cit_4e0255eb69f10"/>
		<cito:citesForInformation rdf:resource="http://www.cognitiveatlas.org/citation/id/cit_4e02566db5a5c"/>
</skos:Concept><skos:Concept rdf:about="http://www.cognitiveatlas.org/id/trm_4b7497a289534"> <dc:identifier>trm_4b7497a289534</dc:identifier>
		<dc:Title>Cognitive Atlas : Lexicon : Block Design Test</dc:Title>
		<dc:Description>RDF output for 'Block Design Test'</dc:Description>
		<dc:Type>InteractiveResource</dc:Type>
		<dc:Publisher>Cognitive Atlas</dc:Publisher>
		<dc:Creator>Cognitive Atlas RDF Generator</dc:Creator>
		<dc:Contributor>Deanna Lau</dc:Contributor>
		<dc:Date>2010-02-11 15:49:54</dc:Date>
		<dc:Format>text/rdf</dc:Format>
		<dc:Language>en</dc:Language>
		<skos:editorialNote>Generated by testgenall.php on Thu Mar 29 10:24:07 PDT 2012.</skos:editorialNote>
		<skos:historyNote>No previous definition revisions.</skos:historyNote>
		<skos:changeNote>This is the first and only definition provided.</skos:changeNote>
		<skos:scopeNote>http://www.w3.org/2004/02/skos/core#Concept</skos:scopeNote>
		<skos:Note>SKOS properties defined in http://www.w3.org/TR/skos-primer/#secrel</skos:Note>
		<skos:inScheme rdf:resource="http://www.cognitiveatlas.org/tasks/"/>
		<skos:definition>The Block Design is a subtest of Perceptual Reasoning index of the Wechsler Adult Intelligence Scale IV. The Block Design test measures spatial perception, visual abstract processing, and problem solving.</skos:definition>
		<skos:prefLabel>Block Design Test</skos:prefLabel>
		<skos:altLabel></skos:altLabel>
		<skos:related rdf:resource="http://www.cognitiveatlas.org/id/trm_4b82c75498408"/>
		<skos:related rdf:resource="http://www.cognitiveatlas.org/id/tsk_4a57abb949f12"/>
		<skos:example>Block Design Test is descended from Wechsler Adult Intelligence Scale - Revised</skos:example>
		<skos:example>Central Coherence is measured by the contrast of Unsegmented blocks trials in the Block Design Test</skos:example>
		<cito:citesForInformation rdf:resource="http://www.cognitiveatlas.org/citation/id/cit_4de680a224fcb"/>
		<cito:citesForInformation rdf:resource="http://www.cognitiveatlas.org/citation/id/cit_4de6814c280be"/>
		<cito:citesForInformation rdf:resource="http://www.cognitiveatlas.org/citation/id/cit_4de68240df295"/>
</skos:Concept><skos:Concept rdf:about="http://www.cognitiveatlas.org/id/trm_4b749b8829eee"> <dc:identifier>trm_4b749b8829eee</dc:identifier>
		<dc:Title>Cognitive Atlas : Lexicon : Embedded Figures Test</dc:Title>
		<dc:Description>RDF output for 'Embedded Figures Test'</dc:Description>
		<dc:Type>InteractiveResource</dc:Type>
		<dc:Publisher>Cognitive Atlas</dc:Publisher>
		<dc:Creator>Cognitive Atlas RDF Generator</dc:Creator>
		<dc:Contributor>Deanna Lau</dc:Contributor>
		<dc:Date>2010-02-11 16:06:32</dc:Date>
		<dc:Format>text/rdf</dc:Format>
		<dc:Language>en</dc:Language>
		<skos:editorialNote>Generated by testgenall.php on Thu Mar 29 10:24:07 PDT 2012.</skos:editorialNote>
		<skos:historyNote>No previous definition revisions.</skos:historyNote>
		<skos:changeNote>This is the first and only definition provided.</skos:changeNote>
		<skos:scopeNote>http://www.w3.org/2004/02/skos/core#Concept</skos:scopeNote>
		<skos:Note>SKOS properties defined in http://www.w3.org/TR/skos-primer/#secrel</skos:Note>
		<skos:inScheme rdf:resource="http://www.cognitiveatlas.org/tasks/"/>
		<skos:definition>In the embedded Figures Test, the research participant is shown a complex background figure and asked to describe it. After this, the participant is shown a target (such as the outline of a triangle) and asked to locate the target amid the background figure.</skos:definition>
		<skos:prefLabel>Embedded Figures Test</skos:prefLabel>
		<skos:altLabel></skos:altLabel>
		<skos:related rdf:resource="http://www.cognitiveatlas.org/id/trm_4b82c75498408"/>
		<skos:related rdf:resource="http://www.cognitiveatlas.org/id/trm_4b82c75498408"/>
		<skos:related rdf:resource="http://www.cognitiveatlas.org/id/trm_4a3fd79d0a81b"/>
		<skos:related rdf:resource="http://www.cognitiveatlas.org/id/trm_4a3fd79d0a81b"/>
		<skos:related rdf:resource="http://www.cognitiveatlas.org/id/trm_4a3fd79d0b507"/>
		<skos:related rdf:resource="http://www.cognitiveatlas.org/id/trm_4a3fd79d0b507"/>
		<skos:example>Central Coherence is measured by the contrast of Segmented blocks trials in the Embedded Figures Test</skos:example>
		<skos:example>Central Coherence is measured by the contrast of Unsegmented blocks trials in the Embedded Figures Test</skos:example>
		<skos:example>logical reasoning is measured by the contrast of Segmented blocks trials in the Embedded Figures Test</skos:example>
		<skos:example>logical reasoning is measured by the contrast of Unsegmented blocks trials in the Embedded Figures Test</skos:example>
		<skos:example>visuospatial sketch pad is measured by the contrast of Segmented blocks trials in the Embedded Figures Test</skos:example>
		<skos:example>visuospatial sketch pad is measured by the contrast of Unsegmented blocks trials in the Embedded Figures Test</skos:example>
		<cito:citesForInformation rdf:resource="http://www.cognitiveatlas.org/citation/id/cit_4de9659d6844b"/>
		<cito:citesForInformation rdf:resource="http://www.cognitiveatlas.org/citation/id/cit_4de9667a84427"/>
</skos:Concept><skos:Concept rdf:about="http://www.cognitiveatlas.org/id/trm_4b75ea4ddd896"> <dc:identifier>trm_4b75ea4ddd896</dc:identifier>
		<dc:Title>Cognitive Atlas : Lexicon : Same-Different Task</dc:Title>
		<dc:Description>RDF output for 'Same-Different Task'</dc:Description>
		<dc:Type>InteractiveResource</dc:Type>
		<dc:Publisher>Cognitive Atlas</dc:Publisher>
		<dc:Creator>Cognitive Atlas RDF Generator</dc:Creator>
		<dc:Contributor>Russ Poldrack</dc:Contributor>
		<dc:Date>2012-01-28 07:49:44</dc:Date>
		<dc:Format>text/rdf</dc:Format>
		<dc:Language>en</dc:Language>
		<skos:editorialNote>Generated by testgenall.php on Thu Mar 29 10:24:07 PDT 2012.</skos:editorialNote>
		<skos:historyNote>Revision 2: 1 previous definitions.</skos:historyNote>
		<skos:changeNote>See http://www.cognitiveatlas.org/id/trm_4b75ea4ddd896 for complete revision history.</skos:changeNote>
		<skos:scopeNote>http://www.w3.org/2004/02/skos/core#Concept</skos:scopeNote>
		<skos:Note>SKOS properties defined in http://www.w3.org/TR/skos-primer/#secrel</skos:Note>
		<skos:inScheme rdf:resource="http://www.cognitiveatlas.org/tasks/"/>
		<skos:definition>A task which assesses shifting attention. In the computerized version of this task, three spaceships appear on a screen and the participant must determine if the spaceships are all different or all the same. The spaceships can differ in color, size, or shape type. There are three levels of difficulty.  In the first level, the spaceships must all be identical to be considered the same. In the second level of difficulty, the spaceships are considered the same even if they only share two qualities, and in the third difficulty level, the spaceships only need to share one quality to be considered the same. Auditory feedback is given after each response notifying the child whether their answer was correct. </skos:definition>
		<skos:prefLabel>Same-Different Task</skos:prefLabel>
		<skos:altLabel>same-different matching task</skos:altLabel>
		<skos:related rdf:resource="http://www.cognitiveatlas.org/id/trm_4a3fd79d0b607"/>
		<skos:related rdf:resource="http://www.cognitiveatlas.org/id/trm_4a3fd79d0a723"/>
		<skos:related rdf:resource="http://www.cognitiveatlas.org/id/trm_4a3fd79d0b4cd"/>
		<skos:example>set shifting is measured by the contrast of Accuracy on level 3 minus accuracy on level 1 trials in the Same-Different Task</skos:example>
		<skos:example>judgment is measured by the contrast of Overall accuracy of participant minus average accuracy trials in the Same-Different Task</skos:example>
		<skos:example>visual search is measured by the contrast of Overall accuracy of participant minus average accuracy trials in the Same-Different Task</skos:example>
		<cito:citesForInformation rdf:resource="http://www.cognitiveatlas.org/citation/id/cit_4dfa41d36bda6"/>
		<cito:citesForInformation rdf:resource="http://www.cognitiveatlas.org/citation/id/cit_4dfa425ea3b91"/>
</skos:Concept><skos:Concept rdf:about="http://www.cognitiveatlas.org/id/trm_4b843655d5d75"> <dc:identifier>trm_4b843655d5d75</dc:identifier>
		<dc:Title>Cognitive Atlas : Lexicon : Chimeric Animal Stroop Task</dc:Title>
		<dc:Description>RDF output for 'Chimeric Animal Stroop Task'</dc:Description>
		<dc:Type>InteractiveResource</dc:Type>
		<dc:Publisher>Cognitive Atlas</dc:Publisher>
		<dc:Creator>Cognitive Atlas RDF Generator</dc:Creator>
		<dc:Contributor>Deanna Lau</dc:Contributor>
		<dc:Date>2010-02-23 12:11:01</dc:Date>
		<dc:Format>text/rdf</dc:Format>
		<dc:Language>en</dc:Language>
		<skos:editorialNote>Generated by testgenall.php on Thu Mar 29 10:24:07 PDT 2012.</skos:editorialNote>
		<skos:historyNote>No previous definition revisions.</skos:historyNote>
		<skos:changeNote>This is the first and only definition provided.</skos:changeNote>
		<skos:scopeNote>http://www.w3.org/2004/02/skos/core#Concept</skos:scopeNote>
		<skos:Note>SKOS properties defined in http://www.w3.org/TR/skos-primer/#secrel</skos:Note>
		<skos:inScheme rdf:resource="http://www.cognitiveatlas.org/tasks/"/>
		<skos:definition>A task in which participants are shown pictures of chimeric animals (such as a duck&#39;s head attached to a cow&#39;s body) and asked to name animal that the head belongs to while ignoring the identity of the body, or vice versa.  </skos:definition>
		<skos:prefLabel>Chimeric Animal Stroop Task</skos:prefLabel>
		<skos:altLabel></skos:altLabel>
		<skos:related rdf:resource="http://www.cognitiveatlas.org/id/trm_4a3fd79d0a6ad"/>
		<skos:related rdf:resource="http://www.cognitiveatlas.org/id/tsk_4a57abb949e27"/>
		<skos:example>Chimeric Animal Stroop Task is descended from Stroop task</skos:example>
		<skos:example>interference is measured by the contrast of Incongruent trials in the Chimeric Animal Stroop Task</skos:example>
		<cito:citesForInformation rdf:resource="http://www.cognitiveatlas.org/citation/id/cit_4de6bb4540504"/>
</skos:Concept><skos:Concept rdf:about="http://www.cognitiveatlas.org/id/trm_4b86c2e871b14"> <dc:identifier>trm_4b86c2e871b14</dc:identifier>
		<dc:Title>Cognitive Atlas : Lexicon : Rapid Automatized Naming Test</dc:Title>
		<dc:Description>RDF output for 'Rapid Automatized Naming Test'</dc:Description>
		<dc:Type>InteractiveResource</dc:Type>
		<dc:Publisher>Cognitive Atlas</dc:Publisher>
		<dc:Creator>Cognitive Atlas RDF Generator</dc:Creator>
		<dc:Contributor>Russ Poldrack</dc:Contributor>
		<dc:Date>2011-08-10 07:32:03</dc:Date>
		<dc:Format>text/rdf</dc:Format>
		<dc:Language>en</dc:Language>
		<skos:editorialNote>Generated by testgenall.php on Thu Mar 29 10:24:07 PDT 2012.</skos:editorialNote>
		<skos:historyNote>Revision 3: 2 previous definitions.</skos:historyNote>
		<skos:changeNote>See http://www.cognitiveatlas.org/id/trm_4b86c2e871b14 for complete revision history.</skos:changeNote>
		<skos:scopeNote>http://www.w3.org/2004/02/skos/core#Concept</skos:scopeNote>
		<skos:Note>SKOS properties defined in http://www.w3.org/TR/skos-primer/#secrel</skos:Note>
		<skos:inScheme rdf:resource="http://www.cognitiveatlas.org/tasks/"/>
		<skos:definition>&#34;Participants are required to name, as rapidly as possible, items presented visually on a chart. Each chart contains five rows of 10 stimuli from a category of five items. Categories include colors, lowercase letters, digits, and common objects. The tests are scored for total number of errors and time in seconds taken to complete each chart.&#34; - (Meyer, Wood, Hart, &amp; Felton 1998)</skos:definition>
		<skos:prefLabel>Rapid Automatized Naming Test</skos:prefLabel>
		<skos:altLabel>RAN</skos:altLabel>
		<skos:related rdf:resource="http://www.cognitiveatlas.org/id/trm_4a3fd79d0ac87"/>
		<skos:related rdf:resource="http://www.cognitiveatlas.org/id/trm_4a3fd79d0b80f"/>
		<skos:related rdf:resource="http://www.cognitiveatlas.org/id/trm_4a3fd79d0ba6c"/>
		<skos:example>phonological encoding is measured by the contrast of standard deviation from the mean time trials in the Rapid Automatized Naming Test</skos:example>
		<skos:example>lexical access is measured by the contrast of standard deviation from the mean time trials in the Rapid Automatized Naming Test</skos:example>
		<skos:example>working memory retrieval is measured by the contrast of standard deviation from the mean time trials in the Rapid Automatized Naming Test</skos:example>
		<cito:citesForInformation rdf:resource="http://www.cognitiveatlas.org/citation/id/cit_4df91145b0ba1"/>
		<cito:citesForInformation rdf:resource="http://www.cognitiveatlas.org/citation/id/cit_4df914b66445d"/>
</skos:Concept><skos:Concept rdf:about="http://www.cognitiveatlas.org/id/trm_4b86c473a7166"> <dc:identifier>trm_4b86c473a7166</dc:identifier>
		<dc:Title>Cognitive Atlas : Lexicon : Underlining Test</dc:Title>
		<dc:Description>RDF output for 'Underlining Test'</dc:Description>
		<dc:Type>InteractiveResource</dc:Type>
		<dc:Publisher>Cognitive Atlas</dc:Publisher>
		<dc:Creator>Cognitive Atlas RDF Generator</dc:Creator>
		<dc:Contributor>Deanna Lau</dc:Contributor>
		<dc:Date>2010-02-25 10:41:55</dc:Date>
		<dc:Format>text/rdf</dc:Format>
		<dc:Language>en</dc:Language>
		<skos:editorialNote>Generated by testgenall.php on Thu Mar 29 10:24:07 PDT 2012.</skos:editorialNote>
		<skos:historyNote>No previous definition revisions.</skos:historyNote>
		<skos:changeNote>This is the first and only definition provided.</skos:changeNote>
		<skos:scopeNote>http://www.w3.org/2004/02/skos/core#Concept</skos:scopeNote>
		<skos:Note>SKOS properties defined in http://www.w3.org/TR/skos-primer/#secrel</skos:Note>
		<skos:inScheme rdf:resource="http://www.cognitiveatlas.org/tasks/"/>
		<skos:definition>This test involves finding and underlining stimuli that are among other stimuli.  There are four conditions of the test: finding and underlining letters among other letters, drawings among other drawings, real words among nonsense letter strings, and then specific nonsense words among others.  </skos:definition>
		<skos:prefLabel>Underlining Test</skos:prefLabel>
		<skos:altLabel></skos:altLabel>
		<skos:related rdf:resource="http://www.cognitiveatlas.org/id/trm_4a3fd79d0b4cd"/>
		<skos:related rdf:resource="http://www.cognitiveatlas.org/id/trm_4a3fd79d09cae"/>
		<skos:related rdf:resource="http://www.cognitiveatlas.org/id/trm_4aae62e4ad209"/>
		<skos:related rdf:resource="http://www.cognitiveatlas.org/id/trm_4a3fd79d0a431"/>
		<skos:example>visual search is measured by the contrast of # correct minus # incorrect/30 or 60 seconds trials in the Underlining Test</skos:example>
		<skos:example>chunking is measured by the contrast of Unspaced Four-Letter Word trials in the Underlining Test</skos:example>
		<skos:example>cognitive control is measured by the contrast of # correct minus # incorrect/30 or 60 seconds trials in the Underlining Test</skos:example>
		<skos:example>goal maintenance is measured by the contrast of # correct minus # incorrect/30 or 60 seconds trials in the Underlining Test</skos:example>
		<cito:citesForInformation rdf:resource="http://www.cognitiveatlas.org/citation/id/cit_4dffd3c8a71f1"/>
		<cito:citesForInformation rdf:resource="http://www.cognitiveatlas.org/citation/id/cit_4dffd5afb9aab"/>
</skos:Concept><skos:Concept rdf:about="http://www.cognitiveatlas.org/id/trm_4b86c55f3d5df"> <dc:identifier>trm_4b86c55f3d5df</dc:identifier>
		<dc:Title>Cognitive Atlas : Lexicon : WISC-R Mazes</dc:Title>
		<dc:Description>RDF output for 'WISC-R Mazes'</dc:Description>
		<dc:Type>InteractiveResource</dc:Type>
		<dc:Publisher>Cognitive Atlas</dc:Publisher>
		<dc:Creator>Cognitive Atlas RDF Generator</dc:Creator>
		<dc:Contributor>Deanna Lau</dc:Contributor>
		<dc:Date>2010-02-25 10:45:51</dc:Date>
		<dc:Format>text/rdf</dc:Format>
		<dc:Language>en</dc:Language>
		<skos:editorialNote>Generated by testgenall.php on Thu Mar 29 10:24:07 PDT 2012.</skos:editorialNote>
		<skos:historyNote>No previous definition revisions.</skos:historyNote>
		<skos:changeNote>This is the first and only definition provided.</skos:changeNote>
		<skos:scopeNote>http://www.w3.org/2004/02/skos/core#Concept</skos:scopeNote>
		<skos:Note>SKOS properties defined in http://www.w3.org/TR/skos-primer/#secrel</skos:Note>
		<skos:inScheme rdf:resource="http://www.cognitiveatlas.org/tasks/"/>
		<skos:definition>This task involves completing a series of increasingly complex mazes.  </skos:definition>
		<skos:prefLabel>WISC-R Mazes</skos:prefLabel>
		<skos:altLabel></skos:altLabel>
		<skos:related rdf:resource="http://www.cognitiveatlas.org/id/trm_4a3fd79d0a252"/>
		<skos:related rdf:resource="http://www.cognitiveatlas.org/id/trm_4a3fd79d0b1a6"/>
		<skos:related rdf:resource="http://www.cognitiveatlas.org/id/trm_4a3fd79d0b5ef"/>
		<skos:related rdf:resource="http://www.cognitiveatlas.org/id/trm_4a3fd79d09de4"/>
		<skos:related rdf:resource="http://www.cognitiveatlas.org/id/trm_4da87fdd7820e"/>
		<skos:example>WISC-R Mazes is an exact synonym of Porteus maze test</skos:example>
		<skos:example>executive function is measured by the contrast of participant score minus average score trials in the WISC-R Mazes</skos:example>
		<skos:example>spatial ability is measured by the contrast of participant score minus average score trials in the WISC-R Mazes</skos:example>
		<skos:example>attentional focusing is measured by the contrast of participant score minus average score trials in the WISC-R Mazes</skos:example>
		<skos:example>conceptual planning is measured by the contrast of participant score minus average score trials in the WISC-R Mazes</skos:example>
		<cito:citesForInformation rdf:resource="http://www.cognitiveatlas.org/citation/id/cit_4e02118f13539"/>
		<cito:citesForInformation rdf:resource="http://www.cognitiveatlas.org/citation/id/cit_4e021813ae10f"/>
</skos:Concept><skos:Concept rdf:about="http://www.cognitiveatlas.org/id/trm_4b86dbcd8ff78"> <dc:identifier>trm_4b86dbcd8ff78</dc:identifier>
		<dc:Title>Cognitive Atlas : Lexicon : Rapid Serial Object Transformation</dc:Title>
		<dc:Description>RDF output for 'Rapid Serial Object Transformation'</dc:Description>
		<dc:Type>InteractiveResource</dc:Type>
		<dc:Publisher>Cognitive Atlas</dc:Publisher>
		<dc:Creator>Cognitive Atlas RDF Generator</dc:Creator>
		<dc:Contributor>Deanna Lau</dc:Contributor>
		<dc:Date>2010-02-25 12:21:33</dc:Date>
		<dc:Format>text/rdf</dc:Format>
		<dc:Language>en</dc:Language>
		<skos:editorialNote>Generated by testgenall.php on Thu Mar 29 10:24:07 PDT 2012.</skos:editorialNote>
		<skos:historyNote>No previous definition revisions.</skos:historyNote>
		<skos:changeNote>This is the first and only definition provided.</skos:changeNote>
		<skos:scopeNote>http://www.w3.org/2004/02/skos/core#Concept</skos:scopeNote>
		<skos:Note>SKOS properties defined in http://www.w3.org/TR/skos-primer/#secrel</skos:Note>
		<skos:inScheme rdf:resource="http://www.cognitiveatlas.org/tasks/"/>
		<skos:definition>A task where two sets of differently colored superimposed patterns of dots rotate in opposite directions.  The participant is asked to pay attention to on set of dots.  One of the sets of dots will then move across the screen and the participant must say which direction the dots are moving.  </skos:definition>
		<skos:prefLabel>Rapid Serial Object Transformation</skos:prefLabel>
		<skos:altLabel></skos:altLabel>
		<skos:related rdf:resource="http://www.cognitiveatlas.org/id/trm_4a3fd79d0b46f"/>
		<skos:related rdf:resource="http://www.cognitiveatlas.org/id/trm_4a3fd79d0b46f"/>
		<skos:related rdf:resource="http://www.cognitiveatlas.org/id/trm_4a3fd79d0a116"/>
		<skos:related rdf:resource="http://www.cognitiveatlas.org/id/trm_4a3fd79d0a116"/>
		<skos:related rdf:resource="http://www.cognitiveatlas.org/id/trm_4a3fd79d0b5fb"/>
		<skos:related rdf:resource="http://www.cognitiveatlas.org/id/trm_4a3fd79d0b5fb"/>
		<skos:example>visual attention is measured by the contrast of ERP strength minus baseline trials in the Rapid Serial Object Transformation</skos:example>
		<skos:example>visual attention is measured by the contrast of accuracy of participant minus average accuracy of controls trials in the Rapid Serial Object Transformation</skos:example>
		<skos:example>divided attention is measured by the contrast of ERP strength minus baseline trials in the Rapid Serial Object Transformation</skos:example>
		<skos:example>divided attention is measured by the contrast of accuracy during task minus accuracy of some baseline test (e.g. only one pattern) trials in the Rapid Serial Object Transformation</skos:example>
		<skos:example>attention shifting is measured by the contrast of ERP strength minus baseline trials in the Rapid Serial Object Transformation</skos:example>
		<skos:example>attention shifting is measured by the contrast of accuracy during task minus accuracy of some baseline test (e.g. only one pattern) trials in the Rapid Serial Object Transformation</skos:example>
		<cito:citesForInformation rdf:resource="http://www.cognitiveatlas.org/citation/id/cit_4df91b1fdf56d"/>
		<cito:citesForInformation rdf:resource="http://www.cognitiveatlas.org/citation/id/cit_4df91d265cb10"/>
</skos:Concept><skos:Concept rdf:about="http://www.cognitiveatlas.org/id/trm_4b94affc43245"> <dc:identifier>trm_4b94affc43245</dc:identifier>
		<dc:Title>Cognitive Atlas : Lexicon : Wechsler Abbreviated Scale of Intelligence</dc:Title>
		<dc:Description>RDF output for 'Wechsler Abbreviated Scale of Intelligence'</dc:Description>
		<dc:Type>InteractiveResource</dc:Type>
		<dc:Publisher>Cognitive Atlas</dc:Publisher>
		<dc:Creator>Cognitive Atlas RDF Generator</dc:Creator>
		<dc:Contributor>Carinna Torgerson</dc:Contributor>
		<dc:Date>2011-06-21 15:10:30</dc:Date>
		<dc:Format>text/rdf</dc:Format>
		<dc:Language>en</dc:Language>
		<skos:editorialNote>Generated by testgenall.php on Thu Mar 29 10:24:07 PDT 2012.</skos:editorialNote>
		<skos:historyNote>Revision 2: 1 previous definitions.</skos:historyNote>
		<skos:changeNote>See http://www.cognitiveatlas.org/id/trm_4b94affc43245 for complete revision history.</skos:changeNote>
		<skos:scopeNote>http://www.w3.org/2004/02/skos/core#Concept</skos:scopeNote>
		<skos:Note>SKOS properties defined in http://www.w3.org/TR/skos-primer/#secrel</skos:Note>
		<skos:inScheme rdf:resource="http://www.cognitiveatlas.org/tasks/"/>
		<skos:definition>The WASI meets the demand for a reliable, brief measure of intellectual ability in clinical, educational and research settings for ages 6 to 89 years. With parallel forms of WAIS-IIIUK and WISC-IIIUK subtests, it offers the clinician a means of reducing practice effects on repeat testing. It yields traditional verbal, performance and full scale IQ scores and is linked to the WISC-IIIUK and WAIS-IIIUK. The WASI allows you to choose whether to use the four or two subtest format.</skos:definition>
		<skos:prefLabel>Wechsler Abbreviated Scale of Intelligence</skos:prefLabel>
		<skos:altLabel></skos:altLabel>
		<skos:related rdf:resource="http://www.cognitiveatlas.org/id/trm_4a3fd79d0b1a6"/>
		<skos:related rdf:resource="http://www.cognitiveatlas.org/id/trm_4a3fd79d0b44c"/>
		<skos:related rdf:resource="http://www.cognitiveatlas.org/id/trm_4a3fd79d0b077"/>
		<skos:related rdf:resource="http://www.cognitiveatlas.org/id/trm_4a3fd79d0a81b"/>
		<skos:related rdf:resource="http://www.cognitiveatlas.org/id/trm_4a3fd79d09f64"/>
		<skos:related rdf:resource="http://www.cognitiveatlas.org/id/trm_4a3fd79d0a375"/>
		<skos:related rdf:resource="http://www.cognitiveatlas.org/id/trm_4a3fd79d09d35"/>
		<skos:related rdf:resource="http://www.cognitiveatlas.org/id/tsk_4a57abb949f12"/>
		<skos:example>Wechsler Abbreviated Scale of Intelligence is descended from Wechsler Adult Intelligence Scale - Revised</skos:example>
		<skos:example>spatial ability is measured by the contrast of Block Design trials in the Wechsler Abbreviated Scale of Intelligence</skos:example>
		<skos:example>verbal fluency is measured by the contrast of Vocabulary trials in the Wechsler Abbreviated Scale of Intelligence</skos:example>
		<skos:example>semantic knowledge is measured by the contrast of Similarities trials in the Wechsler Abbreviated Scale of Intelligence</skos:example>
		<skos:example>logical reasoning is measured by the contrast of Matrix Reasoning trials in the Wechsler Abbreviated Scale of Intelligence</skos:example>
		<skos:example>crystallized intelligence is measured by the contrast of Block Design trials in the Wechsler Abbreviated Scale of Intelligence</skos:example>
		<skos:example>fluid intelligence is measured by the contrast of Matrix Reasoning trials in the Wechsler Abbreviated Scale of Intelligence</skos:example>
		<skos:example>cognitive development is measured by the contrast of participant IQ minus average IQ trials in the Wechsler Abbreviated Scale of Intelligence</skos:example>
		<cito:citesForInformation rdf:resource="http://www.cognitiveatlas.org/citation/id/cit_4e01178801f3a"/>
		<cito:citesForInformation rdf:resource="http://www.cognitiveatlas.org/citation/id/cit_4e011c63d5874"/>
</skos:Concept><skos:Concept rdf:about="http://www.cognitiveatlas.org/id/trm_4b94b12bf0eb2"> <dc:identifier>trm_4b94b12bf0eb2</dc:identifier>
		<dc:Title>Cognitive Atlas : Lexicon : Wechsler Memory Scale Fourth Edition</dc:Title>
		<dc:Description>RDF output for 'Wechsler Memory Scale Fourth Edition'</dc:Description>
		<dc:Type>InteractiveResource</dc:Type>
		<dc:Publisher>Cognitive Atlas</dc:Publisher>
		<dc:Creator>Cognitive Atlas RDF Generator</dc:Creator>
		<dc:Contributor>Nolan Nichols</dc:Contributor>
		<dc:Date>2010-03-08 00:11:23</dc:Date>
		<dc:Format>text/rdf</dc:Format>
		<dc:Language>en</dc:Language>
		<skos:editorialNote>Generated by testgenall.php on Thu Mar 29 10:24:07 PDT 2012.</skos:editorialNote>
		<skos:historyNote>No previous definition revisions.</skos:historyNote>
		<skos:changeNote>This is the first and only definition provided.</skos:changeNote>
		<skos:scopeNote>http://www.w3.org/2004/02/skos/core#Concept</skos:scopeNote>
		<skos:Note>SKOS properties defined in http://www.w3.org/TR/skos-primer/#secrel</skos:Note>
		<skos:inScheme rdf:resource="http://www.cognitiveatlas.org/tasks/"/>
		<skos:definition>Areas of Assessment

Updated Test Structure

The WMS-IV has had significant changes to the overall test structure. Based on feedback from customers, we are introducing four new subtests and modifying three existing subtests.

4 subtests were added:

    * Spatial Addition
    * Symbol Span
    * Design Memory
    * General Cognitive Screener

3 subtests retained with modifications:

    * Logical Memory
      Although the stories remain the same as seen in WMS-III for ages 16-69 years old, the repetition trial for Story B has been dropped to increase the consistency with previous editions. For the older age range of 65-90 years old, a new story was developed with content more relevant. The story is shorter and repeated once to enable adequate floor through age 90. You can obtain immediate versus delay and recognition versus delay contrast scores.
    * Verbal Paired Associates
      It now includes a combination of difficult and easy items. For the younger age group (16-69 years) there are 14 items of which 10 are hard. For the older age group (65-90 years), there are 10 items of which six are hard. Delayed Free Recall Trial has been added while Recognition Trial has increased its level of difficulty. You can obtain immediate versus delay and recognition versus delay contrast scores.
    * Visual Reproduction
      While following the same structure and format as seen in WMS-III, there have been a few changes to the subtest. Recognition Trial has been shortened and scoring has been improved. Based on Munro Cullum’s research, scoring is easier and faster than previously experienced and emphasizes recall with less focus on drawing accuracy. You can obtain immediate versus delay and recognition versus delay contrast scores.

8 subtests were eliminated:

    * Information &amp; Orientation
    * Spatial Span
    * Mental Control
    * Faces
    * Digit Span
    * Family Pictures
    * Letter Number
    * Word List (CVLT-II can be entered int</skos:definition>
		<skos:prefLabel>Wechsler Memory Scale Fourth Edition</skos:prefLabel>
		<skos:altLabel></skos:altLabel>
		<skos:related rdf:resource="http://www.cognitiveatlas.org/id/trm_4a3fd79d0b457"/>
		<skos:related rdf:resource="http://www.cognitiveatlas.org/id/trm_4a3fd79d0b457"/>
		<skos:related rdf:resource="http://www.cognitiveatlas.org/id/trm_4a3fd79d09aa7"/>
		<skos:related rdf:resource="http://www.cognitiveatlas.org/id/trm_4a3fd79d0b507"/>
		<skos:related rdf:resource="http://www.cognitiveatlas.org/id/trm_4a3fd79d0b507"/>
		<skos:related rdf:resource="http://www.cognitiveatlas.org/id/trm_4a3fd79d0afa0"/>
		<skos:related rdf:resource="http://www.cognitiveatlas.org/id/trm_4a3fd79d0af7d"/>
		<skos:related rdf:resource="http://www.cognitiveatlas.org/id/tsk_4a57abb949f12"/>
		<skos:example>Wechsler Memory Scale Fourth Edition is descended from Wechsler Adult Intelligence Scale - Revised</skos:example>
		<skos:example>verbal memory is measured by the contrast of Vocabulary trials in the Wechsler Memory Scale Fourth Edition</skos:example>
		<skos:example>verbal memory is measured by the contrast of Verbal Paired Associates trials in the Wechsler Memory Scale Fourth Edition</skos:example>
		<skos:example>auditory memory is measured by the contrast of Symbol Span trials in the Wechsler Memory Scale Fourth Edition</skos:example>
		<skos:example>visuospatial sketch pad is measured by the contrast of Visual Reproduction trials in the Wechsler Memory Scale Fourth Edition</skos:example>
		<skos:example>visuospatial sketch pad is measured by the contrast of Spatial Addition trials in the Wechsler Memory Scale Fourth Edition</skos:example>
		<skos:example>retrieval cue is measured by the contrast of Verbal Paired Associates trials in the Wechsler Memory Scale Fourth Edition</skos:example>
		<skos:example>retention is measured by the contrast of immediate score minus delayed score trials in the Wechsler Memory Scale Fourth Edition</skos:example>
		<cito:citesForInformation rdf:resource="http://www.cognitiveatlas.org/citation/id/cit_4e0130fb32bb2"/>
		<cito:citesForInformation rdf:resource="http://www.cognitiveatlas.org/citation/id/cit_4e012d85aad12"/>
		<cito:citesForInformation rdf:resource="http://www.cognitiveatlas.org/citation/id/cit_4e0131b7f019b"/>
</skos:Concept><skos:Concept rdf:about="http://www.cognitiveatlas.org/id/trm_4b9568b2865c2"> <dc:identifier>trm_4b9568b2865c2</dc:identifier>
		<dc:Title>Cognitive Atlas : Lexicon : MicroCog</dc:Title>
		<dc:Description>RDF output for 'MicroCog'</dc:Description>
		<dc:Type>InteractiveResource</dc:Type>
		<dc:Publisher>Cognitive Atlas</dc:Publisher>
		<dc:Creator>Cognitive Atlas RDF Generator</dc:Creator>
		<dc:Contributor>Nolan Nichols</dc:Contributor>
		<dc:Date>2010-03-08 13:14:26</dc:Date>
		<dc:Format>text/rdf</dc:Format>
		<dc:Language>en</dc:Language>
		<skos:editorialNote>Generated by testgenall.php on Thu Mar 29 10:24:07 PDT 2012.</skos:editorialNote>
		<skos:historyNote>No previous definition revisions.</skos:historyNote>
		<skos:changeNote>This is the first and only definition provided.</skos:changeNote>
		<skos:scopeNote>http://www.w3.org/2004/02/skos/core#Concept</skos:scopeNote>
		<skos:Note>SKOS properties defined in http://www.w3.org/TR/skos-primer/#secrel</skos:Note>
		<skos:inScheme rdf:resource="http://www.cognitiveatlas.org/tasks/"/>
		<skos:definition>Overview

The first automated neuropsychological battery developed for clinical practice-fast, reliable, extremely efficient

Target specific concerns of cognitive impairment in adults with the updated MicroCog™: Assessment of Cognitive Functioning Windows® Edition (MicroCog™ for Windows®). This version includes significant enhancements and is optimized for Windows®.

Content
This computer administered battery tests individuals with 18 subtests that contribute to summary scores for nine interrelated cognitive areas:
• Attention/Mental Control
• Memory
• Spatial Processing
• Reasoning/Calculation
• Reaction Time
• Information Processing Accuracy
• Information Processing Speed
• Cognitive Functioning
• Cognitive Proficiency

Efficient Screener or Diagnostic Instrument
• Flexible-allows you to choose which subtests to administer
• Provides differential diagnosis across a wide population

Two Forms
• Standard Form (60 to 90 minutes)
• Short Form (30 to 45 minutes)

User Friendly
Most examinees can complete the test quickly and with minimal assistance after a brief orientation by a testing assistant.

Test-Retest, Store Data
MicroCog for Windows® stores test data and is proven effective in testretest situations to monitor a patient&#39;s ongoing cognitive status. A report is automatically provided at the end of each administration.

Other Features and Benefits
• For a broad age range (18-89 years)
• Fast administration time (30 to 90 minutes)
• Results do not vary across cultural differences
• Does not require computer literacy or Internet access (PC-based)
• Report credits embedded in software application (separate use counter not required)

Special Uses
• Screening for dementia or Alzheimer&#39;s
• Determining driving fitness
• Evaluating airline pilots (approved by Federal Aviation Administration for re-certification)
• Testing neurological function of athletes-pre- and post</skos:definition>
		<skos:prefLabel>MicroCog</skos:prefLabel>
		<skos:altLabel></skos:altLabel>
		<skos:related rdf:resource="http://www.cognitiveatlas.org/id/trm_4a3fd79d0b5ef"/>
		<skos:related rdf:resource="http://www.cognitiveatlas.org/id/trm_4a3fd79d0b1a6"/>
		<skos:related rdf:resource="http://www.cognitiveatlas.org/id/trm_4a3fd79d0aec1"/>
		<skos:related rdf:resource="http://www.cognitiveatlas.org/id/trm_4a3fd79d0adf4"/>
		<skos:related rdf:resource="http://www.cognitiveatlas.org/id/trm_4aae62e4ad209"/>
		<skos:example>attentional focusing is measured by the contrast of subject score minus population-matched average score trials in the MicroCog</skos:example>
		<skos:example>spatial ability is measured by the contrast of subject score minus population-matched average score trials in the MicroCog</skos:example>
		<skos:example>reasoning is measured by the contrast of subject score minus population-matched average score trials in the MicroCog</skos:example>
		<skos:example>processing capacity is measured by the contrast of subject score minus population-matched average score trials in the MicroCog</skos:example>
		<skos:example>cognitive control is measured by the contrast of subject score minus population-matched average score trials in the MicroCog</skos:example>
		<cito:citesForInformation rdf:resource="http://www.cognitiveatlas.org/citation/id/cit_4df26828bb610"/>
		<cito:citesForInformation rdf:resource="http://www.cognitiveatlas.org/citation/id/cit_4df26852b47fb"/>
		<cito:citesForInformation rdf:resource="http://www.cognitiveatlas.org/citation/id/cit_4df2693407bcd"/>
</skos:Concept><skos:Concept rdf:about="http://www.cognitiveatlas.org/id/trm_4c3e0a9576c3b"> <dc:identifier>trm_4c3e0a9576c3b</dc:identifier>
		<dc:Title>Cognitive Atlas : Lexicon : letter number sequencing</dc:Title>
		<dc:Description>RDF output for 'letter number sequencing'</dc:Description>
		<dc:Type>InteractiveResource</dc:Type>
		<dc:Publisher>Cognitive Atlas</dc:Publisher>
		<dc:Creator>Cognitive Atlas RDF Generator</dc:Creator>
		<dc:Contributor>Russ Poldrack</dc:Contributor>
		<dc:Date>2011-08-10 07:30:02</dc:Date>
		<dc:Format>text/rdf</dc:Format>
		<dc:Language>en</dc:Language>
		<skos:editorialNote>Generated by testgenall.php on Thu Mar 29 10:24:07 PDT 2012.</skos:editorialNote>
		<skos:historyNote>Revision 2: 1 previous definitions.</skos:historyNote>
		<skos:changeNote>See http://www.cognitiveatlas.org/id/trm_4c3e0a9576c3b for complete revision history.</skos:changeNote>
		<skos:scopeNote>http://www.w3.org/2004/02/skos/core#Concept</skos:scopeNote>
		<skos:Note>SKOS properties defined in http://www.w3.org/TR/skos-primer/#secrel</skos:Note>
		<skos:inScheme rdf:resource="http://www.cognitiveatlas.org/tasks/"/>
		<skos:definition>a task that requires the reordering of an initially unordered set of letters and numbers</skos:definition>
		<skos:prefLabel>letter number sequencing</skos:prefLabel>
		<skos:altLabel>letter-number sequencing</skos:altLabel>
		<skos:related rdf:resource="http://www.cognitiveatlas.org/id/trm_4a3fd79d09b04"/>
		<skos:related rdf:resource="http://www.cognitiveatlas.org/id/trm_4a3fd79d0a116"/>
		<skos:related rdf:resource="http://www.cognitiveatlas.org/id/trm_4a3fd79d0b5a7"/>
		<skos:related rdf:resource="http://www.cognitiveatlas.org/id/tsk_4a57abb949f12"/>
		<skos:example>letter number sequencing is descended from Wechsler Adult Intelligence Scale - Revised</skos:example>
		<skos:example>auditory working memory is measured by the contrast of longest correct sequence of controls minus longest correct sequence of subject trials in the letter number sequencing</skos:example>
		<skos:example>divided attention is measured by the contrast of longest correct sequence of controls minus longest correct sequence of subject trials in the letter number sequencing</skos:example>
		<skos:example>working memory is measured by the contrast of  trials in the letter number sequencing</skos:example>
		<cito:citesForInformation rdf:resource="http://www.cognitiveatlas.org/citation/id/cit_4df1494498003"/>
		<cito:citesForInformation rdf:resource="http://www.cognitiveatlas.org/citation/id/cit_4df1582d37ad2"/>
		<cito:citesForInformation rdf:resource="http://www.cognitiveatlas.org/citation/id/cit_4df159cc74d27"/>
</skos:Concept><skos:Concept rdf:about="http://www.cognitiveatlas.org/id/trm_4c3e0add96550"> <dc:identifier>trm_4c3e0add96550</dc:identifier>
		<dc:Title>Cognitive Atlas : Lexicon : oculomotor delayed response</dc:Title>
		<dc:Description>RDF output for 'oculomotor delayed response'</dc:Description>
		<dc:Type>InteractiveResource</dc:Type>
		<dc:Publisher>Cognitive Atlas</dc:Publisher>
		<dc:Creator>Cognitive Atlas RDF Generator</dc:Creator>
		<dc:Contributor>Russ Poldrack</dc:Contributor>
		<dc:Date>2010-07-14 12:07:09</dc:Date>
		<dc:Format>text/rdf</dc:Format>
		<dc:Language>en</dc:Language>
		<skos:editorialNote>Generated by testgenall.php on Thu Mar 29 10:24:07 PDT 2012.</skos:editorialNote>
		<skos:historyNote>No previous definition revisions.</skos:historyNote>
		<skos:changeNote>This is the first and only definition provided.</skos:changeNote>
		<skos:scopeNote>http://www.w3.org/2004/02/skos/core#Concept</skos:scopeNote>
		<skos:Note>SKOS properties defined in http://www.w3.org/TR/skos-primer/#secrel</skos:Note>
		<skos:inScheme rdf:resource="http://www.cognitiveatlas.org/tasks/"/>
		<skos:definition>a task that requires an eye movement to be made to a cued location after a delay</skos:definition>
		<skos:prefLabel>oculomotor delayed response</skos:prefLabel>
		<skos:altLabel></skos:altLabel>
		<skos:related rdf:resource="http://www.cognitiveatlas.org/id/trm_4a3fd79d0b4d8"/>
		<skos:related rdf:resource="http://www.cognitiveatlas.org/id/trm_4a3fd79d0a972"/>
		<skos:example>visual working memory is measured by the contrast of sensory modality trials in the oculomotor delayed response</skos:example>
		<skos:example>motor control is measured by the contrast of sensory modality trials in the oculomotor delayed response</skos:example>
		<cito:citesForInformation rdf:resource="http://www.cognitiveatlas.org/citation/id/cit_4c9974facbe21"/>
		<cito:citesForInformation rdf:resource="http://www.cognitiveatlas.org/citation/id/cit_4df6673e5e8f6"/>
		<cito:citesForInformation rdf:resource="http://www.cognitiveatlas.org/citation/id/cit_4df667a52ae21"/>
</skos:Concept><skos:Concept rdf:about="http://www.cognitiveatlas.org/id/trm_4c40d10cd776e"> <dc:identifier>trm_4c40d10cd776e</dc:identifier>
		<dc:Title>Cognitive Atlas : Lexicon : operation span task</dc:Title>
		<dc:Description>RDF output for 'operation span task'</dc:Description>
		<dc:Type>InteractiveResource</dc:Type>
		<dc:Publisher>Cognitive Atlas</dc:Publisher>
		<dc:Creator>Cognitive Atlas RDF Generator</dc:Creator>
		<dc:Contributor>Russ Poldrack</dc:Contributor>
		<dc:Date>2010-07-16 14:37:16</dc:Date>
		<dc:Format>text/rdf</dc:Format>
		<dc:Language>en</dc:Language>
		<skos:editorialNote>Generated by testgenall.php on Thu Mar 29 10:24:07 PDT 2012.</skos:editorialNote>
		<skos:historyNote>No previous definition revisions.</skos:historyNote>
		<skos:changeNote>This is the first and only definition provided.</skos:changeNote>
		<skos:scopeNote>http://www.w3.org/2004/02/skos/core#Concept</skos:scopeNote>
		<skos:Note>SKOS properties defined in http://www.w3.org/TR/skos-primer/#secrel</skos:Note>
		<skos:inScheme rdf:resource="http://www.cognitiveatlas.org/tasks/"/>
		<skos:definition>A task in which subjects are asked to perform a simple mathematical verification (e.g., 4/2 +1 = 3) and then read a word, with a recall test following some number of those verify/read pairs.  The maximum number of words that can be recalled is the &#34;operation span&#34;.</skos:definition>
		<skos:prefLabel>operation span task</skos:prefLabel>
		<skos:altLabel></skos:altLabel>
		<skos:related rdf:resource="http://www.cognitiveatlas.org/id/trm_4a3fd79d0b5ef"/>
		<skos:related rdf:resource="http://www.cognitiveatlas.org/id/trm_4a3fd79d0b5a7"/>
		<skos:related rdf:resource="http://www.cognitiveatlas.org/id/trm_4c40d1d16071e"/>
		<skos:related rdf:resource="http://www.cognitiveatlas.org/id/trm_4c40d168898db"/>
		<skos:example>operation span task is related to listening span task</skos:example>
		<skos:example>operation span task is related to reading span task</skos:example>
		<skos:example>attentional focusing is measured by the contrast of operation span of participant minus average operation span of controls trials in the operation span task</skos:example>
		<skos:example>working memory is measured by the contrast of operation span of participant minus average operation span of controls trials in the operation span task</skos:example>
		<cito:citesForInformation rdf:resource="http://www.cognitiveatlas.org/citation/id/cit_4df68009ba53f"/>
		<cito:citesForInformation rdf:resource="http://www.cognitiveatlas.org/citation/id/cit_4df680680e574"/>
</skos:Concept><skos:Concept rdf:about="http://www.cognitiveatlas.org/id/trm_4c40d168898db"> <dc:identifier>trm_4c40d168898db</dc:identifier>
		<dc:Title>Cognitive Atlas : Lexicon : reading span task</dc:Title>
		<dc:Description>RDF output for 'reading span task'</dc:Description>
		<dc:Type>InteractiveResource</dc:Type>
		<dc:Publisher>Cognitive Atlas</dc:Publisher>
		<dc:Creator>Cognitive Atlas RDF Generator</dc:Creator>
		<dc:Contributor>Russ Poldrack</dc:Contributor>
		<dc:Date>2010-07-16 14:38:48</dc:Date>
		<dc:Format>text/rdf</dc:Format>
		<dc:Language>en</dc:Language>
		<skos:editorialNote>Generated by testgenall.php on Thu Mar 29 10:24:07 PDT 2012.</skos:editorialNote>
		<skos:historyNote>No previous definition revisions.</skos:historyNote>
		<skos:changeNote>This is the first and only definition provided.</skos:changeNote>
		<skos:scopeNote>http://www.w3.org/2004/02/skos/core#Concept</skos:scopeNote>
		<skos:Note>SKOS properties defined in http://www.w3.org/TR/skos-primer/#secrel</skos:Note>
		<skos:inScheme rdf:resource="http://www.cognitiveatlas.org/tasks/"/>
		<skos:definition>A task that requires participants to read series of unconnected sentences aloud and to remember the final word of each sentence of a series (grouped according to the total number of sentences). With each sentence presented on a card, participants were cued to recall the memorized end-of-sentence words in their original order by a blank card at the end of a series. The number of sentences of a series was incrementally increased until a participant&#39;s reading span, or the maximum number of final words correctly recalled, was found. (From http://en.wikipedia.org/wiki/Reading_span_task)</skos:definition>
		<skos:prefLabel>reading span task</skos:prefLabel>
		<skos:altLabel></skos:altLabel>
		<skos:related rdf:resource="http://www.cognitiveatlas.org/id/trm_4c40d10cd776e"/>
		<skos:related rdf:resource="http://www.cognitiveatlas.org/id/trm_4a3fd79d0b507"/>
		<skos:related rdf:resource="http://www.cognitiveatlas.org/id/trm_4a3fd79d0b89e"/>
		<skos:related rdf:resource="http://www.cognitiveatlas.org/id/trm_4c40d1d16071e"/>
		<skos:example>reading span task is related to listening span task</skos:example>
		<skos:example>operation span task is related to reading span task</skos:example>
		<skos:example>visuospatial sketch pad is measured by the contrast of reading span of participant minus average reading span of controls trials in the reading span task</skos:example>
		<skos:example>sentence processing is measured by the contrast of reading span of participant minus average reading span of controls trials in the reading span task</skos:example>
		<cito:citesForInformation rdf:resource="http://www.cognitiveatlas.org/citation/id/cit_4df926830ddfb"/>
		<cito:citesForInformation rdf:resource="http://www.cognitiveatlas.org/citation/id/cit_4df9284aa3755"/>
		<cito:citesForInformation rdf:resource="http://www.cognitiveatlas.org/citation/id/cit_4df92881d4a85"/>
</skos:Concept><skos:Concept rdf:about="http://www.cognitiveatlas.org/id/trm_4c40d1d16071e"> <dc:identifier>trm_4c40d1d16071e</dc:identifier>
		<dc:Title>Cognitive Atlas : Lexicon : listening span task</dc:Title>
		<dc:Description>RDF output for 'listening span task'</dc:Description>
		<dc:Type>InteractiveResource</dc:Type>
		<dc:Publisher>Cognitive Atlas</dc:Publisher>
		<dc:Creator>Cognitive Atlas RDF Generator</dc:Creator>
		<dc:Contributor>Russ Poldrack</dc:Contributor>
		<dc:Date>2010-07-16 14:40:33</dc:Date>
		<dc:Format>text/rdf</dc:Format>
		<dc:Language>en</dc:Language>
		<skos:editorialNote>Generated by testgenall.php on Thu Mar 29 10:24:07 PDT 2012.</skos:editorialNote>
		<skos:historyNote>No previous definition revisions.</skos:historyNote>
		<skos:changeNote>This is the first and only definition provided.</skos:changeNote>
		<skos:scopeNote>http://www.w3.org/2004/02/skos/core#Concept</skos:scopeNote>
		<skos:Note>SKOS properties defined in http://www.w3.org/TR/skos-primer/#secrel</skos:Note>
		<skos:inScheme rdf:resource="http://www.cognitiveatlas.org/tasks/"/>
		<skos:definition>A task in which subjects must listen to a set of sentences and remember the last word in the sentence.  The number of words that can be recalled is the &#34;listening span.&#34; </skos:definition>
		<skos:prefLabel>listening span task</skos:prefLabel>
		<skos:altLabel></skos:altLabel>
		<skos:related rdf:resource="http://www.cognitiveatlas.org/id/trm_4a3fd79d0971e"/>
		<skos:related rdf:resource="http://www.cognitiveatlas.org/id/trm_4a3fd79d09b04"/>
		<skos:related rdf:resource="http://www.cognitiveatlas.org/id/trm_4c40d10cd776e"/>
		<skos:related rdf:resource="http://www.cognitiveatlas.org/id/trm_4c40d168898db"/>
		<skos:related rdf:resource="http://www.cognitiveatlas.org/id/tsk_4a57abb949d69"/>
		<skos:example>listening span task is a broader synonym of Salthouse and Babcock Listening Span task </skos:example>
		<skos:example>acoustic processing is measured by the contrast of size of subject sentence set minus average size of sentence set of control subjects trials in the listening span task</skos:example>
		<skos:example>auditory working memory is measured by the contrast of size of subject sentence set minus average size of sentence set of control subjects trials in the listening span task</skos:example>
		<skos:example>operation span task is related to listening span task</skos:example>
		<skos:example>reading span task is related to listening span task</skos:example>
		<cito:citesForInformation rdf:resource="http://www.cognitiveatlas.org/citation/id/cit_4df24dddcbfec"/>
		<cito:citesForInformation rdf:resource="http://www.cognitiveatlas.org/citation/id/cit_4df24d9db3458"/>
</skos:Concept><skos:Concept rdf:about="http://www.cognitiveatlas.org/id/trm_4c40d2a93ea15"> <dc:identifier>trm_4c40d2a93ea15</dc:identifier>
		<dc:Title>Cognitive Atlas : Lexicon : AX-CPT task</dc:Title>
		<dc:Description>RDF output for 'AX-CPT task'</dc:Description>
		<dc:Type>InteractiveResource</dc:Type>
		<dc:Publisher>Cognitive Atlas</dc:Publisher>
		<dc:Creator>Cognitive Atlas RDF Generator</dc:Creator>
		<dc:Contributor>Russ Poldrack</dc:Contributor>
		<dc:Date>2010-07-16 14:44:09</dc:Date>
		<dc:Format>text/rdf</dc:Format>
		<dc:Language>en</dc:Language>
		<skos:editorialNote>Generated by testgenall.php on Thu Mar 29 10:24:07 PDT 2012.</skos:editorialNote>
		<skos:historyNote>No previous definition revisions.</skos:historyNote>
		<skos:changeNote>This is the first and only definition provided.</skos:changeNote>
		<skos:scopeNote>http://www.w3.org/2004/02/skos/core#Concept</skos:scopeNote>
		<skos:Note>SKOS properties defined in http://www.w3.org/TR/skos-primer/#secrel</skos:Note>
		<skos:inScheme rdf:resource="http://www.cognitiveatlas.org/tasks/"/>
		<skos:definition>A version of the continuous performance task in which subjects are told to make one response for the letter X when it was preceded by the letter A, and another response for all other stimuli.</skos:definition>
		<skos:prefLabel>AX-CPT task</skos:prefLabel>
		<skos:altLabel></skos:altLabel>
		<skos:related rdf:resource="http://www.cognitiveatlas.org/id/trm_4a3fd79d0b311"/>
		<skos:related rdf:resource="http://www.cognitiveatlas.org/id/trm_4aae62e4ad209"/>
		<skos:related rdf:resource="http://www.cognitiveatlas.org/id/trm_4c40d22c8a69d"/>
		<skos:example>AX-CPT task is a narrower synonym of </skos:example>
		<skos:example>sustained attention is measured by the contrast of  trials in the AX-CPT task</skos:example>
		<skos:example>cognitive control is measured by the contrast of  trials in the AX-CPT task</skos:example>
		<cito:citesForInformation rdf:resource="http://www.cognitiveatlas.org/citation/id/cit_4c995f00bcff7"/>
</skos:Concept><skos:Concept rdf:about="http://www.cognitiveatlas.org/id/trm_4c40d325977f0"> <dc:identifier>trm_4c40d325977f0</dc:identifier>
		<dc:Title>Cognitive Atlas : Lexicon : self-ordered pointing task</dc:Title>
		<dc:Description>RDF output for 'self-ordered pointing task'</dc:Description>
		<dc:Type>InteractiveResource</dc:Type>
		<dc:Publisher>Cognitive Atlas</dc:Publisher>
		<dc:Creator>Cognitive Atlas RDF Generator</dc:Creator>
		<dc:Contributor>Russ Poldrack</dc:Contributor>
		<dc:Date>2010-07-16 14:46:13</dc:Date>
		<dc:Format>text/rdf</dc:Format>
		<dc:Language>en</dc:Language>
		<skos:editorialNote>Generated by testgenall.php on Thu Mar 29 10:24:07 PDT 2012.</skos:editorialNote>
		<skos:historyNote>No previous definition revisions.</skos:historyNote>
		<skos:changeNote>This is the first and only definition provided.</skos:changeNote>
		<skos:scopeNote>http://www.w3.org/2004/02/skos/core#Concept</skos:scopeNote>
		<skos:Note>SKOS properties defined in http://www.w3.org/TR/skos-primer/#secrel</skos:Note>
		<skos:inScheme rdf:resource="http://www.cognitiveatlas.org/tasks/"/>
		<skos:definition>A task in which a set of stimuli is presented, and subjects must point to one stimulus at a time, without ever pointing at the same stimulus twice.</skos:definition>
		<skos:prefLabel>self-ordered pointing task</skos:prefLabel>
		<skos:altLabel></skos:altLabel>
		<skos:related rdf:resource="http://www.cognitiveatlas.org/id/trm_4a3fd79d0a246"/>
		<skos:related rdf:resource="http://www.cognitiveatlas.org/id/trm_4a3fd79d09d64"/>
		<skos:related rdf:resource="http://www.cognitiveatlas.org/id/trm_4a3fd79d0abaa"/>
		<skos:related rdf:resource="http://www.cognitiveatlas.org/id/trm_4a3fd79d0adf4"/>
		<skos:example>executive control is measured by the contrast of accuracy of participant minus average accuracy of controls trials in the self-ordered pointing task</skos:example>
		<skos:example>cognitive load is measured by the contrast of accuracy of participant minus average accuracy of controls trials in the self-ordered pointing task</skos:example>
		<skos:example>perceptual identification is measured by the contrast of accuracy of participant minus average accuracy of controls trials in the self-ordered pointing task</skos:example>
		<skos:example>processing capacity is measured by the contrast of accuracy of participant minus average accuracy of controls trials in the self-ordered pointing task</skos:example>
		<cito:citesForInformation rdf:resource="http://www.cognitiveatlas.org/citation/id/cit_4dfa4ec4c2f17"/>
		<cito:citesForInformation rdf:resource="http://www.cognitiveatlas.org/citation/id/cit_4dfa4f4b46a28"/>
		<cito:citesForInformation rdf:resource="http://www.cognitiveatlas.org/citation/id/cit_4dfa5075657c3"/>
</skos:Concept><skos:Concept rdf:about="http://www.cognitiveatlas.org/id/trm_4c40d4054f38b"> <dc:identifier>trm_4c40d4054f38b</dc:identifier>
		<dc:Title>Cognitive Atlas : Lexicon : keep-track task</dc:Title>
		<dc:Description>RDF output for 'keep-track task'</dc:Description>
		<dc:Type>InteractiveResource</dc:Type>
		<dc:Publisher>Cognitive Atlas</dc:Publisher>
		<dc:Creator>Cognitive Atlas RDF Generator</dc:Creator>
		<dc:Contributor>Russ Poldrack</dc:Contributor>
		<dc:Date>2010-07-16 14:49:57</dc:Date>
		<dc:Format>text/rdf</dc:Format>
		<dc:Language>en</dc:Language>
		<skos:editorialNote>Generated by testgenall.php on Thu Mar 29 10:24:07 PDT 2012.</skos:editorialNote>
		<skos:historyNote>No previous definition revisions.</skos:historyNote>
		<skos:changeNote>This is the first and only definition provided.</skos:changeNote>
		<skos:scopeNote>http://www.w3.org/2004/02/skos/core#Concept</skos:scopeNote>
		<skos:Note>SKOS properties defined in http://www.w3.org/TR/skos-primer/#secrel</skos:Note>
		<skos:inScheme rdf:resource="http://www.cognitiveatlas.org/tasks/"/>
		<skos:definition>A task in which subjects are first shown a set of categories to keep track of for a particular trial (e.g., animals, colors, and countries).  They are then presented with words (including words from each category), and must remember the last word that was presented from each of the categories and recall those words at the end of the trial.  </skos:definition>
		<skos:prefLabel>keep-track task</skos:prefLabel>
		<skos:altLabel></skos:altLabel>
		<skos:related rdf:resource="http://www.cognitiveatlas.org/id/trm_4a3fd79d0b5a7"/>
		<skos:related rdf:resource="http://www.cognitiveatlas.org/id/trm_4c3e05903e4bb"/>
		<skos:related rdf:resource="http://www.cognitiveatlas.org/id/trm_4a3fd79d09d64"/>
		<skos:example>working memory is measured by the contrast of accuracy of subject minus average accuracy of controls trials in the keep-track task</skos:example>
		<skos:example>updating is measured by the contrast of accuracy of subject minus average accuracy of controls trials in the keep-track task</skos:example>
		<skos:example>cognitive load is measured by the contrast of accuracy of subject minus average accuracy of controls trials in the keep-track task</skos:example>
		<cito:citesForInformation rdf:resource="http://www.cognitiveatlas.org/citation/id/cit_4c40d41a2ebf1"/>
		<cito:citesForInformation rdf:resource="http://www.cognitiveatlas.org/citation/id/cit_4df139dd0ea2b"/>
		<cito:citesForInformation rdf:resource="http://www.cognitiveatlas.org/citation/id/cit_4df13a5ce83cf"/>
		<cito:citesForInformation rdf:resource="http://www.cognitiveatlas.org/citation/id/cit_4df13a75366ab"/>
</skos:Concept><skos:Concept rdf:about="http://www.cognitiveatlas.org/id/trm_4c8989e1f3df7"> <dc:identifier>trm_4c8989e1f3df7</dc:identifier>
		<dc:Title>Cognitive Atlas : Lexicon : Acupuncture Task</dc:Title>
		<dc:Description>RDF output for 'Acupuncture Task'</dc:Description>
		<dc:Type>InteractiveResource</dc:Type>
		<dc:Publisher>Cognitive Atlas</dc:Publisher>
		<dc:Creator>Cognitive Atlas RDF Generator</dc:Creator>
		<dc:Contributor>Brenda Gregory</dc:Contributor>
		<dc:Date>2011-04-28 12:08:19</dc:Date>
		<dc:Format>text/rdf</dc:Format>
		<dc:Language>en</dc:Language>
		<skos:editorialNote>Generated by testgenall.php on Thu Mar 29 10:24:07 PDT 2012.</skos:editorialNote>
		<skos:historyNote>Revision 2: 1 previous definitions.</skos:historyNote>
		<skos:changeNote>See http://www.cognitiveatlas.org/id/trm_4c8989e1f3df7 for complete revision history.</skos:changeNote>
		<skos:scopeNote>http://www.w3.org/2004/02/skos/core#Concept</skos:scopeNote>
		<skos:Note>SKOS properties defined in http://www.w3.org/TR/skos-primer/#secrel</skos:Note>
		<skos:inScheme rdf:resource="http://www.cognitiveatlas.org/tasks/"/>
		<skos:definition>subjects are stimulated with Chinese acupuncture.</skos:definition>
		<skos:prefLabel>Acupuncture Task</skos:prefLabel>
		<skos:altLabel></skos:altLabel>
		<skos:related rdf:resource="http://www.cognitiveatlas.org/id/trm_4b65259eeee34"/>
		<skos:related rdf:resource="http://www.cognitiveatlas.org/id/trm_4a3fd79d0a22f"/>
		<skos:example>pain is measured by the contrast of pain at baseling minus pain during acupunture trials in the Acupuncture Task</skos:example>
		<skos:example>excitation is measured by the contrast of areas of activation during task minus baseline trials in the Acupuncture Task</skos:example>
		<cito:citesForInformation rdf:resource="http://www.cognitiveatlas.org/citation/id/cit_4e038181420d2"/>
		<cito:citesForInformation rdf:resource="http://www.cognitiveatlas.org/citation/id/cit_4e0381d7b178a"/>
		<cito:citesForInformation rdf:resource="http://www.cognitiveatlas.org/citation/id/cit_4e0382d2a6cc1"/>
</skos:Concept><skos:Concept rdf:about="http://www.cognitiveatlas.org/id/trm_4c898a20eb254"> <dc:identifier>trm_4c898a20eb254</dc:identifier>
		<dc:Title>Cognitive Atlas : Lexicon : Braille Reading Task</dc:Title>
		<dc:Description>RDF output for 'Braille Reading Task'</dc:Description>
		<dc:Type>InteractiveResource</dc:Type>
		<dc:Publisher>Cognitive Atlas</dc:Publisher>
		<dc:Creator>Cognitive Atlas RDF Generator</dc:Creator>
		<dc:Contributor>Brenda Gregory</dc:Contributor>
		<dc:Date>2011-04-28 12:07:50</dc:Date>
		<dc:Format>text/rdf</dc:Format>
		<dc:Language>en</dc:Language>
		<skos:editorialNote>Generated by testgenall.php on Thu Mar 29 10:24:07 PDT 2012.</skos:editorialNote>
		<skos:historyNote>Revision 2: 1 previous definitions.</skos:historyNote>
		<skos:changeNote>See http://www.cognitiveatlas.org/id/trm_4c898a20eb254 for complete revision history.</skos:changeNote>
		<skos:scopeNote>http://www.w3.org/2004/02/skos/core#Concept</skos:scopeNote>
		<skos:Note>SKOS properties defined in http://www.w3.org/TR/skos-primer/#secrel</skos:Note>
		<skos:inScheme rdf:resource="http://www.cognitiveatlas.org/tasks/"/>
		<skos:definition>Blind subjects read Braille words with their finger(s).</skos:definition>
		<skos:prefLabel>Braille Reading Task</skos:prefLabel>
		<skos:altLabel></skos:altLabel>
		<skos:related rdf:resource="http://www.cognitiveatlas.org/id/trm_4a3fd79d0aeb6"/>
		<skos:related rdf:resource="http://www.cognitiveatlas.org/id/trm_4a3fd79d0abb6"/>
		<skos:related rdf:resource="http://www.cognitiveatlas.org/id/trm_4a3fd79d0b802"/>
		<skos:example>reading is measured by the contrast of areas of activation while reading words or sentences minus reading control dots trials in the Braille Reading Task</skos:example>
		<skos:example>perceptual learning is measured by the contrast of areas of activation of early blind minus areas of activation of late blind trials in the Braille Reading Task</skos:example>
		<skos:example>language processing is measured by the contrast of areas of activation while reading words or sentences minus reading control dots trials in the Braille Reading Task</skos:example>
		<cito:citesForInformation rdf:resource="http://www.cognitiveatlas.org/citation/id/cit_4e038ec4905b8"/>
		<cito:citesForInformation rdf:resource="http://www.cognitiveatlas.org/citation/id/cit_4e03913cdccdb"/>
		<cito:citesForInformation rdf:resource="http://www.cognitiveatlas.org/citation/id/cit_4e0394c089c6c"/>
</skos:Concept><skos:Concept rdf:about="http://www.cognitiveatlas.org/id/trm_4c898a680e424"> <dc:identifier>trm_4c898a680e424</dc:identifier>
		<dc:Title>Cognitive Atlas : Lexicon : Breath-Holding</dc:Title>
		<dc:Description>RDF output for 'Breath-Holding'</dc:Description>
		<dc:Type>InteractiveResource</dc:Type>
		<dc:Publisher>Cognitive Atlas</dc:Publisher>
		<dc:Creator>Cognitive Atlas RDF Generator</dc:Creator>
		<dc:Contributor>Carinna Torgerson</dc:Contributor>
		<dc:Date>2011-06-01 12:58:21</dc:Date>
		<dc:Format>text/rdf</dc:Format>
		<dc:Language>en</dc:Language>
		<skos:editorialNote>Generated by testgenall.php on Thu Mar 29 10:24:07 PDT 2012.</skos:editorialNote>
		<skos:historyNote>Revision 3: 2 previous definitions.</skos:historyNote>
		<skos:changeNote>See http://www.cognitiveatlas.org/id/trm_4c898a680e424 for complete revision history.</skos:changeNote>
		<skos:scopeNote>http://www.w3.org/2004/02/skos/core#Concept</skos:scopeNote>
		<skos:Note>SKOS properties defined in http://www.w3.org/TR/skos-primer/#secrel</skos:Note>
		<skos:inScheme rdf:resource="http://www.cognitiveatlas.org/tasks/"/>
		<skos:definition>Subjects hold their breath as examiner measures mean blood flow velocity divided by time to find the breath-holding index (BHI). Measures cerebral hemodynamic auto-regulation.</skos:definition>
		<skos:prefLabel>Breath-Holding</skos:prefLabel>
		<skos:altLabel></skos:altLabel>
		<cito:citesForInformation rdf:resource="http://www.cognitiveatlas.org/citation/id/cit_4de69a7c6da49"/>
		<cito:citesForInformation rdf:resource="http://www.cognitiveatlas.org/citation/id/cit_4de69c53b79e1"/>
</skos:Concept><skos:Concept rdf:about="http://www.cognitiveatlas.org/id/trm_4c898a8fd3afb"> <dc:identifier>trm_4c898a8fd3afb</dc:identifier>
		<dc:Title>Cognitive Atlas : Lexicon : Chewing/Swallowing</dc:Title>
		<dc:Description>RDF output for 'Chewing/Swallowing'</dc:Description>
		<dc:Type>InteractiveResource</dc:Type>
		<dc:Publisher>Cognitive Atlas</dc:Publisher>
		<dc:Creator>Cognitive Atlas RDF Generator</dc:Creator>
		<dc:Contributor>Brenda Gregory</dc:Contributor>
		<dc:Date>2011-04-27 15:50:29</dc:Date>
		<dc:Format>text/rdf</dc:Format>
		<dc:Language>en</dc:Language>
		<skos:editorialNote>Generated by testgenall.php on Thu Mar 29 10:24:07 PDT 2012.</skos:editorialNote>
		<skos:historyNote>Revision 2: 1 previous definitions.</skos:historyNote>
		<skos:changeNote>See http://www.cognitiveatlas.org/id/trm_4c898a8fd3afb for complete revision history.</skos:changeNote>
		<skos:scopeNote>http://www.w3.org/2004/02/skos/core#Concept</skos:scopeNote>
		<skos:Note>SKOS properties defined in http://www.w3.org/TR/skos-primer/#secrel</skos:Note>
		<skos:inScheme rdf:resource="http://www.cognitiveatlas.org/tasks/"/>
		<skos:definition>Subjects chew an oral stimulus that is not food (e.g., gum) or swallow their own saliva.  If the oral stimulus is food or liquid that is swallowed, then the correct paradigm class is Eating/Drinking.</skos:definition>
		<skos:prefLabel>Chewing/Swallowing</skos:prefLabel>
		<skos:altLabel></skos:altLabel>
		<skos:related rdf:resource="http://www.cognitiveatlas.org/id/trm_4a3fd79d0a972"/>
		<skos:example>motor control is measured by the contrast of areas of activation during task minus baseline trials in the Chewing/Swallowing</skos:example>
		<cito:citesForInformation rdf:resource="http://www.cognitiveatlas.org/citation/id/cit_4de95d166bed4"/>
		<cito:citesForInformation rdf:resource="http://www.cognitiveatlas.org/citation/id/cit_4e03974bb3add"/>
		<cito:citesForInformation rdf:resource="http://www.cognitiveatlas.org/citation/id/cit_4e0398f59c895"/>
		<cito:citesForInformation rdf:resource="http://www.cognitiveatlas.org/citation/id/cit_4e0398ff79de3"/>
</skos:Concept><skos:Concept rdf:about="http://www.cognitiveatlas.org/id/trm_4c898acd1f28e"> <dc:identifier>trm_4c898acd1f28e</dc:identifier>
		<dc:Title>Cognitive Atlas : Lexicon : Classical Conditioning</dc:Title>
		<dc:Description>RDF output for 'Classical Conditioning'</dc:Description>
		<dc:Type>InteractiveResource</dc:Type>
		<dc:Publisher>Cognitive Atlas</dc:Publisher>
		<dc:Creator>Cognitive Atlas RDF Generator</dc:Creator>
		<dc:Contributor>Carinna Torgerson</dc:Contributor>
		<dc:Date>2011-06-01 16:14:39</dc:Date>
		<dc:Format>text/rdf</dc:Format>
		<dc:Language>en</dc:Language>
		<skos:editorialNote>Generated by testgenall.php on Thu Mar 29 10:24:07 PDT 2012.</skos:editorialNote>
		<skos:historyNote>Revision 3: 2 previous definitions.</skos:historyNote>
		<skos:changeNote>See http://www.cognitiveatlas.org/id/trm_4c898acd1f28e for complete revision history.</skos:changeNote>
		<skos:scopeNote>http://www.w3.org/2004/02/skos/core#Concept</skos:scopeNote>
		<skos:Note>SKOS properties defined in http://www.w3.org/TR/skos-primer/#secrel</skos:Note>
		<skos:inScheme rdf:resource="http://www.cognitiveatlas.org/tasks/"/>
		<skos:definition>Subjects are presented with paired stimuli in an attempt to study associative learning or get a subject to react to the conditioned stimulus in the same manner as the unconditioned stimulus, demonstrating a learned association between the two.</skos:definition>
		<skos:prefLabel>Classical Conditioning</skos:prefLabel>
		<skos:altLabel></skos:altLabel>
		<skos:related rdf:resource="http://www.cognitiveatlas.org/id/trm_4a3fd79d098c9"/>
		<skos:related rdf:resource="http://www.cognitiveatlas.org/id/trm_4a3fd79d0ab70"/>
		<skos:related rdf:resource="http://www.cognitiveatlas.org/id/trm_4a3fd79d0ab70"/>
		<skos:related rdf:resource="http://www.cognitiveatlas.org/id/trm_4a3fd79d0ab70"/>
		<skos:related rdf:resource="http://www.cognitiveatlas.org/id/trm_4a3fd79d0ab70"/>
		<skos:related rdf:resource="http://www.cognitiveatlas.org/id/trm_4a3fd79d0a637"/>
		<skos:related rdf:resource="http://www.cognitiveatlas.org/id/trm_4a3fd79d09b28"/>
		<skos:related rdf:resource="http://www.cognitiveatlas.org/id/trm_4a3fd79d09b28"/>
		<skos:related rdf:resource="http://www.cognitiveatlas.org/id/trm_4a3fd79d09b28"/>
		<skos:example>association learning is measured by the contrast of conditioned response trials in the Classical Conditioning</skos:example>
		<skos:example>pavlovian conditioning is measured by the contrast of conditioned stimulus trials in the Classical Conditioning</skos:example>
		<skos:example>pavlovian conditioning is measured by the contrast of unconditioned stimulus trials in the Classical Conditioning</skos:example>
		<skos:example>pavlovian conditioning is measured by the contrast of unconditioned response trials in the Classical Conditioning</skos:example>
		<skos:example>pavlovian conditioning is measured by the contrast of conditioned response trials in the Classical Conditioning</skos:example>
		<skos:example>instinct is measured by the contrast of unconditioned stimulus trials in the Classical Conditioning</skos:example>
		<skos:example>automaticity is measured by the contrast of unconditioned stimulus trials in the Classical Conditioning</skos:example>
		<skos:example>automaticity is measured by the contrast of unconditioned response trials in the Classical Conditioning</skos:example>
		<skos:example>automaticity is measured by the contrast of conditioned response trials in the Classical Conditioning</skos:example>
		<cito:citesForInformation rdf:resource="http://www.cognitiveatlas.org/citation/id/cit_4de6cb32edf13"/>
		<cito:citesForInformation rdf:resource="http://www.cognitiveatlas.org/citation/id/cit_4de6cbabc885d"/>
		<cito:citesForInformation rdf:resource="http://www.cognitiveatlas.org/citation/id/cit_4de6cc590c7ea"/>
</skos:Concept><skos:Concept rdf:about="http://www.cognitiveatlas.org/id/trm_4c898b02722d2"> <dc:identifier>trm_4c898b02722d2</dc:identifier>
		<dc:Title>Cognitive Atlas : Lexicon : Counting/Calculation</dc:Title>
		<dc:Description>RDF output for 'Counting/Calculation'</dc:Description>
		<dc:Type>InteractiveResource</dc:Type>
		<dc:Publisher>Cognitive Atlas</dc:Publisher>
		<dc:Creator>Cognitive Atlas RDF Generator</dc:Creator>
		<dc:Contributor>Brenda Gregory</dc:Contributor>
		<dc:Date>2011-04-27 15:46:15</dc:Date>
		<dc:Format>text/rdf</dc:Format>
		<dc:Language>en</dc:Language>
		<skos:editorialNote>Generated by testgenall.php on Thu Mar 29 10:24:07 PDT 2012.</skos:editorialNote>
		<skos:historyNote>Revision 2: 1 previous definitions.</skos:historyNote>
		<skos:changeNote>See http://www.cognitiveatlas.org/id/trm_4c898b02722d2 for complete revision history.</skos:changeNote>
		<skos:scopeNote>http://www.w3.org/2004/02/skos/core#Concept</skos:scopeNote>
		<skos:Note>SKOS properties defined in http://www.w3.org/TR/skos-primer/#secrel</skos:Note>
		<skos:inScheme rdf:resource="http://www.cognitiveatlas.org/tasks/"/>
		<skos:definition>Subjects count, add, subtract, multiply, or divide various stimuli (numbers, bars, dots, etc).</skos:definition>
		<skos:prefLabel>Counting/Calculation</skos:prefLabel>
		<skos:altLabel></skos:altLabel>
		<cito:citesForInformation rdf:resource="http://www.cognitiveatlas.org/citation/id/cit_4de7c9250d6a4"/>
		<cito:citesForInformation rdf:resource="http://www.cognitiveatlas.org/citation/id/cit_4de7ccf4107f0"/>
		<cito:citesForInformation rdf:resource="http://www.cognitiveatlas.org/citation/id/cit_4de7ce1dbd04d"/>
</skos:Concept><skos:Concept rdf:about="http://www.cognitiveatlas.org/id/trm_4c898b29660b0"> <dc:identifier>trm_4c898b29660b0</dc:identifier>
		<dc:Title>Cognitive Atlas : Lexicon : Cued Explicit Recognition</dc:Title>
		<dc:Description>RDF output for 'Cued Explicit Recognition'</dc:Description>
		<dc:Type>InteractiveResource</dc:Type>
		<dc:Publisher>Cognitive Atlas</dc:Publisher>
		<dc:Creator>Cognitive Atlas RDF Generator</dc:Creator>
		<dc:Contributor>Brenda Gregory</dc:Contributor>
		<dc:Date>2011-04-27 15:45:43</dc:Date>
		<dc:Format>text/rdf</dc:Format>
		<dc:Language>en</dc:Language>
		<skos:editorialNote>Generated by testgenall.php on Thu Mar 29 10:24:07 PDT 2012.</skos:editorialNote>
		<skos:historyNote>Revision 2: 1 previous definitions.</skos:historyNote>
		<skos:changeNote>See http://www.cognitiveatlas.org/id/trm_4c898b29660b0 for complete revision history.</skos:changeNote>
		<skos:scopeNote>http://www.w3.org/2004/02/skos/core#Concept</skos:scopeNote>
		<skos:Note>SKOS properties defined in http://www.w3.org/TR/skos-primer/#secrel</skos:Note>
		<skos:inScheme rdf:resource="http://www.cognitiveatlas.org/tasks/"/>
		<skos:definition>Subjects view a list of items (words, pictures, sounds, or abstract patterns) prior to scanning.  During scanning, probe words are presented and subject recall if the words are familiar or unfamiliar.</skos:definition>
		<skos:prefLabel>Cued Explicit Recognition</skos:prefLabel>
		<skos:altLabel></skos:altLabel>
		<skos:related rdf:resource="http://www.cognitiveatlas.org/id/trm_4a3fd79d0b58f"/>
		<skos:related rdf:resource="http://www.cognitiveatlas.org/id/trm_4a3fd79d0b908"/>
		<skos:related rdf:resource="http://www.cognitiveatlas.org/id/tsk_4a57abb9499c7"/>
		<skos:related rdf:resource="http://www.cognitiveatlas.org/id/trm_4b4a5ddfb90d0"/>
		<skos:example>Cued Explicit Recognition is related to continuous recognition paradigm</skos:example>
		<skos:example>Cued Explicit Recognition is a narrower synonym of </skos:example>
		<skos:example>word recognition is measured by the contrast of hit rate (number of correct recognitions) trials in the Cued Explicit Recognition</skos:example>
		<skos:example>forgetting is measured by the contrast of miss rate (number of items subject failed to recognize) trials in the Cued Explicit Recognition</skos:example>
		<cito:citesForInformation rdf:resource="http://www.cognitiveatlas.org/citation/id/cit_4de7d0dee02b1"/>
		<cito:citesForInformation rdf:resource="http://www.cognitiveatlas.org/citation/id/cit_4de7d120be9c2"/>
</skos:Concept><skos:Concept rdf:about="http://www.cognitiveatlas.org/id/trm_4c898b4b463aa"> <dc:identifier>trm_4c898b4b463aa</dc:identifier>
		<dc:Title>Cognitive Atlas : Lexicon : Deception Task</dc:Title>
		<dc:Description>RDF output for 'Deception Task'</dc:Description>
		<dc:Type>InteractiveResource</dc:Type>
		<dc:Publisher>Cognitive Atlas</dc:Publisher>
		<dc:Creator>Cognitive Atlas RDF Generator</dc:Creator>
		<dc:Contributor>Brenda Gregory</dc:Contributor>
		<dc:Date>2011-04-27 15:45:13</dc:Date>
		<dc:Format>text/rdf</dc:Format>
		<dc:Language>en</dc:Language>
		<skos:editorialNote>Generated by testgenall.php on Thu Mar 29 10:24:07 PDT 2012.</skos:editorialNote>
		<skos:historyNote>Revision 2: 1 previous definitions.</skos:historyNote>
		<skos:changeNote>See http://www.cognitiveatlas.org/id/trm_4c898b4b463aa for complete revision history.</skos:changeNote>
		<skos:scopeNote>http://www.w3.org/2004/02/skos/core#Concept</skos:scopeNote>
		<skos:Note>SKOS properties defined in http://www.w3.org/TR/skos-primer/#secrel</skos:Note>
		<skos:inScheme rdf:resource="http://www.cognitiveatlas.org/tasks/"/>
		<skos:definition>Subjects are asked to perform a task and either lie or be truthful in their responses.</skos:definition>
		<skos:prefLabel>Deception Task</skos:prefLabel>
		<skos:altLabel></skos:altLabel>
		<skos:related rdf:resource="http://www.cognitiveatlas.org/id/trm_4a3fd79d0b392"/>
		<skos:related rdf:resource="http://www.cognitiveatlas.org/id/trm_4a3fd79d0b392"/>
		<skos:related rdf:resource="http://www.cognitiveatlas.org/id/trm_4a3fd79d0a02c"/>
		<skos:example>theory of mind is measured by the contrast of object occlusion and misinformation scores trials in the Deception Task</skos:example>
		<skos:example>theory of mind is measured by the contrast of accuracy trials in the Deception Task</skos:example>
		<skos:example>deception is measured by the contrast of hider trials in the Deception Task</skos:example>
		<cito:citesForInformation rdf:resource="http://www.cognitiveatlas.org/citation/id/cit_4de7db8fec7a0"/>
		<cito:citesForInformation rdf:resource="http://www.cognitiveatlas.org/citation/id/cit_4de7db976e852"/>
		<cito:citesForInformation rdf:resource="http://www.cognitiveatlas.org/citation/id/cit_4de7dea05cb2d"/>
</skos:Concept><skos:Concept rdf:about="http://www.cognitiveatlas.org/id/trm_4c898b8c2d071"> <dc:identifier>trm_4c898b8c2d071</dc:identifier>
		<dc:Title>Cognitive Atlas : Lexicon : Deductive Reasoning Task</dc:Title>
		<dc:Description>RDF output for 'Deductive Reasoning Task'</dc:Description>
		<dc:Type>InteractiveResource</dc:Type>
		<dc:Publisher>Cognitive Atlas</dc:Publisher>
		<dc:Creator>Cognitive Atlas RDF Generator</dc:Creator>
		<dc:Contributor>Carinna Torgerson</dc:Contributor>
		<dc:Date>2011-06-02 12:27:28</dc:Date>
		<dc:Format>text/rdf</dc:Format>
		<dc:Language>en</dc:Language>
		<skos:editorialNote>Generated by testgenall.php on Thu Mar 29 10:24:07 PDT 2012.</skos:editorialNote>
		<skos:historyNote>Revision 3: 2 previous definitions.</skos:historyNote>
		<skos:changeNote>See http://www.cognitiveatlas.org/id/trm_4c898b8c2d071 for complete revision history.</skos:changeNote>
		<skos:scopeNote>http://www.w3.org/2004/02/skos/core#Concept</skos:scopeNote>
		<skos:Note>SKOS properties defined in http://www.w3.org/TR/skos-primer/#secrel</skos:Note>
		<skos:inScheme rdf:resource="http://www.cognitiveatlas.org/tasks/"/>
		<skos:definition>Participants generate or evaluate conclusions based on given or well-known premises.</skos:definition>
		<skos:prefLabel>Deductive Reasoning Task</skos:prefLabel>
		<skos:altLabel></skos:altLabel>
		<skos:related rdf:resource="http://www.cognitiveatlas.org/id/trm_4a3fd79d09ece"/>
		<skos:related rdf:resource="http://www.cognitiveatlas.org/id/trm_4a3fd79d0a80f"/>
		<skos:related rdf:resource="http://www.cognitiveatlas.org/id/trm_4a3fd79d0a80f"/>
		<skos:related rdf:resource="http://www.cognitiveatlas.org/id/trm_4a3fd79d0a81b"/>
		<skos:related rdf:resource="http://www.cognitiveatlas.org/id/trm_4a3fd79d0a81b"/>
		<skos:related rdf:resource="http://www.cognitiveatlas.org/id/trm_4a3fd79d0a827"/>
		<skos:related rdf:resource="http://www.cognitiveatlas.org/id/trm_4a3fd79d0a827"/>
		<skos:related rdf:resource="http://www.cognitiveatlas.org/id/trm_4a3fd79d09e07"/>
		<skos:related rdf:resource="http://www.cognitiveatlas.org/id/trm_4a3fd79d0a072"/>
		<skos:related rdf:resource="http://www.cognitiveatlas.org/id/trm_4a3fd79d0a072"/>
		<skos:related rdf:resource="http://www.cognitiveatlas.org/id/trm_4a3fd79d0aec1"/>
		<skos:related rdf:resource="http://www.cognitiveatlas.org/id/trm_4a3fd79d0aec1"/>
		<skos:example>convergent thinking is measured by the contrast of valid trials in the Deductive Reasoning Task</skos:example>
		<skos:example>logic is measured by the contrast of valid trials in the Deductive Reasoning Task</skos:example>
		<skos:example>logic is measured by the contrast of invalid trials in the Deductive Reasoning Task</skos:example>
		<skos:example>logical reasoning is measured by the contrast of valid trials in the Deductive Reasoning Task</skos:example>
		<skos:example>logical reasoning is measured by the contrast of invalid trials in the Deductive Reasoning Task</skos:example>
		<skos:example> is measured by Deductive Reasoning Task</skos:example>
		<skos:example> is measured by Deductive Reasoning Task</skos:example>
		<skos:example>conditional reasoning is measured by the contrast of valid trials in the Deductive Reasoning Task</skos:example>
		<skos:example>deductive reasoning is measured by the contrast of valid trials in the Deductive Reasoning Task</skos:example>
		<skos:example>deductive reasoning is measured by the contrast of invalid trials in the Deductive Reasoning Task</skos:example>
		<skos:example>reasoning is measured by the contrast of valid trials in the Deductive Reasoning Task</skos:example>
		<skos:example>reasoning is measured by the contrast of invalid trials in the Deductive Reasoning Task</skos:example>
		<cito:citesForInformation rdf:resource="http://www.cognitiveatlas.org/citation/id/cit_4de7e35975765"/>
		<cito:citesForInformation rdf:resource="http://www.cognitiveatlas.org/citation/id/cit_4de7e5ab750f3"/>
</skos:Concept><skos:Concept rdf:about="http://www.cognitiveatlas.org/id/trm_4c898bbab4fd4"> <dc:identifier>trm_4c898bbab4fd4</dc:identifier>
		<dc:Title>Cognitive Atlas : Lexicon : Divided Auditory Attention</dc:Title>
		<dc:Description>RDF output for 'Divided Auditory Attention'</dc:Description>
		<dc:Type>InteractiveResource</dc:Type>
		<dc:Publisher>Cognitive Atlas</dc:Publisher>
		<dc:Creator>Cognitive Atlas RDF Generator</dc:Creator>
		<dc:Contributor>Russ Poldrack</dc:Contributor>
		<dc:Date>2012-01-28 07:34:08</dc:Date>
		<dc:Format>text/rdf</dc:Format>
		<dc:Language>en</dc:Language>
		<skos:editorialNote>Generated by testgenall.php on Thu Mar 29 10:24:07 PDT 2012.</skos:editorialNote>
		<skos:historyNote>Revision 3: 2 previous definitions.</skos:historyNote>
		<skos:changeNote>See http://www.cognitiveatlas.org/id/trm_4c898bbab4fd4 for complete revision history.</skos:changeNote>
		<skos:scopeNote>http://www.w3.org/2004/02/skos/core#Concept</skos:scopeNote>
		<skos:Note>SKOS properties defined in http://www.w3.org/TR/skos-primer/#secrel</skos:Note>
		<skos:inScheme rdf:resource="http://www.cognitiveatlas.org/tasks/"/>
		<skos:definition>During the performance of an unrelated task, subjects simultaneously respond to auditory stimuli (tone or word discrimination, with or without distractors).   Also often co-coded with Tone Monitor/Discrimination.</skos:definition>
		<skos:prefLabel>Divided Auditory Attention</skos:prefLabel>
		<skos:altLabel>divided attention test</skos:altLabel>
		<skos:related rdf:resource="http://www.cognitiveatlas.org/id/trm_4a3fd79d0a252"/>
		<skos:related rdf:resource="http://www.cognitiveatlas.org/id/trm_4a3fd79d0a246"/>
		<skos:related rdf:resource="http://www.cognitiveatlas.org/id/trm_4a3fd79d09a10"/>
		<skos:related rdf:resource="http://www.cognitiveatlas.org/id/trm_4a3fd79d09713"/>
		<skos:example>executive function is measured by the contrast of response time and accuracy trials in the Divided Auditory Attention</skos:example>
		<skos:example>executive control is measured by the contrast of response time and accuracy trials in the Divided Auditory Attention</skos:example>
		<skos:example>auditory attention is measured by the contrast of response time and accuracy trials in the Divided Auditory Attention</skos:example>
		<skos:example>acoustic phonetic processing is measured by the contrast of response time and accuracy trials in the Divided Auditory Attention</skos:example>
</skos:Concept><skos:Concept rdf:about="http://www.cognitiveatlas.org/id/trm_4c898be57fcbc"> <dc:identifier>trm_4c898be57fcbc</dc:identifier>
		<dc:Title>Cognitive Atlas : Lexicon : Drawing</dc:Title>
		<dc:Description>RDF output for 'Drawing'</dc:Description>
		<dc:Type>InteractiveResource</dc:Type>
		<dc:Publisher>Cognitive Atlas</dc:Publisher>
		<dc:Creator>Cognitive Atlas RDF Generator</dc:Creator>
		<dc:Contributor>Brenda Gregory</dc:Contributor>
		<dc:Date>2011-04-27 15:42:01</dc:Date>
		<dc:Format>text/rdf</dc:Format>
		<dc:Language>en</dc:Language>
		<skos:editorialNote>Generated by testgenall.php on Thu Mar 29 10:24:07 PDT 2012.</skos:editorialNote>
		<skos:historyNote>Revision 2: 1 previous definitions.</skos:historyNote>
		<skos:changeNote>See http://www.cognitiveatlas.org/id/trm_4c898be57fcbc for complete revision history.</skos:changeNote>
		<skos:scopeNote>http://www.w3.org/2004/02/skos/core#Concept</skos:scopeNote>
		<skos:Note>SKOS properties defined in http://www.w3.org/TR/skos-primer/#secrel</skos:Note>
		<skos:inScheme rdf:resource="http://www.cognitiveatlas.org/tasks/"/>
		<skos:definition>Subjects draw lines, circles, or drawings using a pen or stylus.</skos:definition>
		<skos:prefLabel>Drawing</skos:prefLabel>
		<skos:altLabel></skos:altLabel>
		<skos:related rdf:resource="http://www.cognitiveatlas.org/id/trm_4a3fd79d0a972"/>
		<skos:related rdf:resource="http://www.cognitiveatlas.org/id/trm_4a3fd79d0b4b5"/>
		<skos:example>motor control is measured by the contrast of overall similarity to intended picture trials in the Drawing</skos:example>
		<skos:example>visual perception is measured by the contrast of overall similarity to intended picture trials in the Drawing</skos:example>
		<cito:citesForInformation rdf:resource="http://www.cognitiveatlas.org/citation/id/cit_4de945dfc30cd"/>
		<cito:citesForInformation rdf:resource="http://www.cognitiveatlas.org/citation/id/cit_4de9461b6796c"/>
		<cito:citesForInformation rdf:resource="http://www.cognitiveatlas.org/citation/id/cit_4de94660f1003"/>
</skos:Concept><skos:Concept rdf:about="http://www.cognitiveatlas.org/id/trm_4c898c0786246"> <dc:identifier>trm_4c898c0786246</dc:identifier>
		<dc:Title>Cognitive Atlas : Lexicon : Eating/Drinking</dc:Title>
		<dc:Description>RDF output for 'Eating/Drinking'</dc:Description>
		<dc:Type>InteractiveResource</dc:Type>
		<dc:Publisher>Cognitive Atlas</dc:Publisher>
		<dc:Creator>Cognitive Atlas RDF Generator</dc:Creator>
		<dc:Contributor>Brenda Gregory</dc:Contributor>
		<dc:Date>2011-04-27 15:41:28</dc:Date>
		<dc:Format>text/rdf</dc:Format>
		<dc:Language>en</dc:Language>
		<skos:editorialNote>Generated by testgenall.php on Thu Mar 29 10:24:07 PDT 2012.</skos:editorialNote>
		<skos:historyNote>Revision 2: 1 previous definitions.</skos:historyNote>
		<skos:changeNote>See http://www.cognitiveatlas.org/id/trm_4c898c0786246 for complete revision history.</skos:changeNote>
		<skos:scopeNote>http://www.w3.org/2004/02/skos/core#Concept</skos:scopeNote>
		<skos:Note>SKOS properties defined in http://www.w3.org/TR/skos-primer/#secrel</skos:Note>
		<skos:inScheme rdf:resource="http://www.cognitiveatlas.org/tasks/"/>
		<skos:definition>Subjects eat food (e.g., chocolate) or drink liquids (e.g., juice).</skos:definition>
		<skos:prefLabel>Eating/Drinking</skos:prefLabel>
		<skos:altLabel></skos:altLabel>
		<skos:related rdf:resource="http://www.cognitiveatlas.org/id/trm_4aae62e4ad209"/>
		<skos:related rdf:resource="http://www.cognitiveatlas.org/id/trm_4a3fd79d0b05e"/>
		<skos:example>cognitive control is measured by the contrast of amount consumed trials in the Eating/Drinking</skos:example>
		<skos:example>self monitoring is measured by the contrast of amount consumed trials in the Eating/Drinking</skos:example>
		<cito:citesForInformation rdf:resource="http://www.cognitiveatlas.org/citation/id/cit_4de95b9715bd7"/>
		<cito:citesForInformation rdf:resource="http://www.cognitiveatlas.org/citation/id/cit_4de95c52de732"/>
</skos:Concept><skos:Concept rdf:about="http://www.cognitiveatlas.org/id/trm_4c898c33ee5f8"> <dc:identifier>trm_4c898c33ee5f8</dc:identifier>
		<dc:Title>Cognitive Atlas : Lexicon : Encoding Task</dc:Title>
		<dc:Description>RDF output for 'Encoding Task'</dc:Description>
		<dc:Type>InteractiveResource</dc:Type>
		<dc:Publisher>Cognitive Atlas</dc:Publisher>
		<dc:Creator>Cognitive Atlas RDF Generator</dc:Creator>
		<dc:Contributor>Brenda Gregory</dc:Contributor>
		<dc:Date>2010-09-09 18:38:59</dc:Date>
		<dc:Format>text/rdf</dc:Format>
		<dc:Language>en</dc:Language>
		<skos:editorialNote>Generated by testgenall.php on Thu Mar 29 10:24:07 PDT 2012.</skos:editorialNote>
		<skos:historyNote>No previous definition revisions.</skos:historyNote>
		<skos:changeNote>This is the first and only definition provided.</skos:changeNote>
		<skos:scopeNote>http://www.w3.org/2004/02/skos/core#Concept</skos:scopeNote>
		<skos:Note>SKOS properties defined in http://www.w3.org/TR/skos-primer/#secrel</skos:Note>
		<skos:inScheme rdf:resource="http://www.cognitiveatlas.org/tasks/"/>
		<skos:definition>Subjects view stimuli (words, pictures, letters) and are instructed to memorize them.</skos:definition>
		<skos:prefLabel>Encoding Task</skos:prefLabel>
		<skos:altLabel></skos:altLabel>
		<skos:related rdf:resource="http://www.cognitiveatlas.org/id/trm_4a3fd79d09707"/>
		<skos:related rdf:resource="http://www.cognitiveatlas.org/id/trm_4a3fd79d09a3d"/>
		<skos:related rdf:resource="http://www.cognitiveatlas.org/id/trm_4a3fd79d09a49"/>
		<skos:related rdf:resource="http://www.cognitiveatlas.org/id/trm_4a3fd79d0a15c"/>
		<skos:related rdf:resource="http://www.cognitiveatlas.org/id/trm_4a3fd79d0b8e5"/>
		<skos:related rdf:resource="http://www.cognitiveatlas.org/id/trm_4a3fd79d0b756"/>
		<skos:related rdf:resource="http://www.cognitiveatlas.org/id/trm_4a3fd79d0a7d4"/>
		<skos:related rdf:resource="http://www.cognitiveatlas.org/id/trm_4a3fd79d0ac87"/>
		<skos:related rdf:resource="http://www.cognitiveatlas.org/id/trm_4a3fd79d098a6"/>
		<skos:related rdf:resource="http://www.cognitiveatlas.org/id/trm_4a3fd79d0b8d9"/>
		<skos:example>acoustic encoding is measured by the contrast of # items remembered with encoding task - number remembered without trials in the Encoding Task</skos:example>
		<skos:example>auditory coding is measured by the contrast of # items remembered with encoding task - number remembered without trials in the Encoding Task</skos:example>
		<skos:example>auditory encoding is measured by the contrast of # items remembered with encoding task - number remembered without trials in the Encoding Task</skos:example>
		<skos:example>effortful processing is measured by the contrast of # items remembered with encoding task - number remembered without trials in the Encoding Task</skos:example>
		<skos:example>encoding is measured by the contrast of # items remembered with encoding task - number remembered without trials in the Encoding Task</skos:example>
		<skos:example>grammatical encoding is measured by the contrast of # items remembered with encoding task - number remembered without trials in the Encoding Task</skos:example>
		<skos:example>lexical encoding is measured by the contrast of # items remembered with encoding task - number remembered without trials in the Encoding Task</skos:example>
		<skos:example>phonological encoding is measured by the contrast of # items remembered with encoding task - number remembered without trials in the Encoding Task</skos:example>
		<skos:example>articulatory rehearsal is measured by the contrast of # items remembered with encoding task - number remembered without trials in the Encoding Task</skos:example>
		<skos:example>elaborative rehearsal is measured by the contrast of # items remembered with encoding task - number remembered without trials in the Encoding Task</skos:example>
		<cito:citesForInformation rdf:resource="http://www.cognitiveatlas.org/citation/id/cit_4de9676c85e39"/>
		<cito:citesForInformation rdf:resource="http://www.cognitiveatlas.org/citation/id/cit_4de96a66cba15"/>
</skos:Concept><skos:Concept rdf:about="http://www.cognitiveatlas.org/id/trm_4c898c8bf1b4f"> <dc:identifier>trm_4c898c8bf1b4f</dc:identifier>
		<dc:Title>Cognitive Atlas : Lexicon : Episodic Recall</dc:Title>
		<dc:Description>RDF output for 'Episodic Recall'</dc:Description>
		<dc:Type>InteractiveResource</dc:Type>
		<dc:Publisher>Cognitive Atlas</dc:Publisher>
		<dc:Creator>Cognitive Atlas RDF Generator</dc:Creator>
		<dc:Contributor>Brenda Gregory</dc:Contributor>
		<dc:Date>2011-04-27 15:40:36</dc:Date>
		<dc:Format>text/rdf</dc:Format>
		<dc:Language>en</dc:Language>
		<skos:editorialNote>Generated by testgenall.php on Thu Mar 29 10:24:07 PDT 2012.</skos:editorialNote>
		<skos:historyNote>Revision 2: 1 previous definitions.</skos:historyNote>
		<skos:changeNote>See http://www.cognitiveatlas.org/id/trm_4c898c8bf1b4f for complete revision history.</skos:changeNote>
		<skos:scopeNote>http://www.w3.org/2004/02/skos/core#Concept</skos:scopeNote>
		<skos:Note>SKOS properties defined in http://www.w3.org/TR/skos-primer/#secrel</skos:Note>
		<skos:inScheme rdf:resource="http://www.cognitiveatlas.org/tasks/"/>
		<skos:definition>Subjects recall items from episodic memory (autobiographical history, long-term event memories).  This class is commonly used in generating a type of emotion linked to a specific memory.  This class does NOT include tasks which probe semantic memory (memory of facts or concepts) in which subjects are asked to recall stimuli that were memorized prior to scanning - those are coded as Cued Explicit Recognition.</skos:definition>
		<skos:prefLabel>Episodic Recall</skos:prefLabel>
		<skos:altLabel></skos:altLabel>
		<skos:related rdf:resource="http://www.cognitiveatlas.org/id/trm_4a3fd79d0a1f4"/>
		<skos:related rdf:resource="http://www.cognitiveatlas.org/id/trm_4a3fd79d09b1c"/>
		<skos:example>episodic memory is measured by the contrast of number of correct identifications trials in the Episodic Recall</skos:example>
		<skos:example>autobiographical recall is measured by the contrast of number of correct identifications trials in the Episodic Recall</skos:example>
		<cito:citesForInformation rdf:resource="http://www.cognitiveatlas.org/citation/id/cit_4de96b805dd7d"/>
		<cito:citesForInformation rdf:resource="http://www.cognitiveatlas.org/citation/id/cit_4de96cb32187e"/>
</skos:Concept><skos:Concept rdf:about="http://www.cognitiveatlas.org/id/trm_4c898cb4ada49"> <dc:identifier>trm_4c898cb4ada49</dc:identifier>
		<dc:Title>Cognitive Atlas : Lexicon : Face Monitor/Discrimination</dc:Title>
		<dc:Description>RDF output for 'Face Monitor/Discrimination'</dc:Description>
		<dc:Type>InteractiveResource</dc:Type>
		<dc:Publisher>Cognitive Atlas</dc:Publisher>
		<dc:Creator>Cognitive Atlas RDF Generator</dc:Creator>
		<dc:Contributor>Brenda Gregory</dc:Contributor>
		<dc:Date>2011-04-27 15:39:58</dc:Date>
		<dc:Format>text/rdf</dc:Format>
		<dc:Language>en</dc:Language>
		<skos:editorialNote>Generated by testgenall.php on Thu Mar 29 10:24:07 PDT 2012.</skos:editorialNote>
		<skos:historyNote>Revision 2: 1 previous definitions.</skos:historyNote>
		<skos:changeNote>See http://www.cognitiveatlas.org/id/trm_4c898cb4ada49 for complete revision history.</skos:changeNote>
		<skos:scopeNote>http://www.w3.org/2004/02/skos/core#Concept</skos:scopeNote>
		<skos:Note>SKOS properties defined in http://www.w3.org/TR/skos-primer/#secrel</skos:Note>
		<skos:inScheme rdf:resource="http://www.cognitiveatlas.org/tasks/"/>
		<skos:definition>Subjects are presented with human faces and are instructed to view them passively or discriminate according to their order, gender, location, emotion, or appearance.  If the subjects view the faces passively, then the experiment is NOT co-coded with Passive Viewing.</skos:definition>
		<skos:prefLabel>Face Monitor/Discrimination</skos:prefLabel>
		<skos:altLabel></skos:altLabel>
		<cito:citesForInformation rdf:resource="http://www.cognitiveatlas.org/citation/id/cit_4ded0b038fa4f"/>
</skos:Concept><skos:Concept rdf:about="http://www.cognitiveatlas.org/id/trm_4c898da401420"> <dc:identifier>trm_4c898da401420</dc:identifier>
		<dc:Title>Cognitive Atlas : Lexicon : Film Viewing</dc:Title>
		<dc:Description>RDF output for 'Film Viewing'</dc:Description>
		<dc:Type>InteractiveResource</dc:Type>
		<dc:Publisher>Cognitive Atlas</dc:Publisher>
		<dc:Creator>Cognitive Atlas RDF Generator</dc:Creator>
		<dc:Contributor>Brenda Gregory</dc:Contributor>
		<dc:Date>2011-04-27 15:39:31</dc:Date>
		<dc:Format>text/rdf</dc:Format>
		<dc:Language>en</dc:Language>
		<skos:editorialNote>Generated by testgenall.php on Thu Mar 29 10:24:07 PDT 2012.</skos:editorialNote>
		<skos:historyNote>Revision 2: 1 previous definitions.</skos:historyNote>
		<skos:changeNote>See http://www.cognitiveatlas.org/id/trm_4c898da401420 for complete revision history.</skos:changeNote>
		<skos:scopeNote>http://www.w3.org/2004/02/skos/core#Concept</skos:scopeNote>
		<skos:Note>SKOS properties defined in http://www.w3.org/TR/skos-primer/#secrel</skos:Note>
		<skos:inScheme rdf:resource="http://www.cognitiveatlas.org/tasks/"/>
		<skos:definition>Subjects view movie or film clips passively or are required to make a discrimination when the clip is over.</skos:definition>
		<skos:prefLabel>Film Viewing</skos:prefLabel>
		<skos:altLabel></skos:altLabel>
		<cito:citesForInformation rdf:resource="http://www.cognitiveatlas.org/citation/id/cit_4ded210380450"/>
		<cito:citesForInformation rdf:resource="http://www.cognitiveatlas.org/citation/id/cit_4ded21b26bd98"/>
		<cito:citesForInformation rdf:resource="http://www.cognitiveatlas.org/citation/id/cit_4ded21f250d0a"/>
</skos:Concept><skos:Concept rdf:about="http://www.cognitiveatlas.org/id/trm_4c898f079d05e"> <dc:identifier>trm_4c898f079d05e</dc:identifier>
		<dc:Title>Cognitive Atlas : Lexicon : Finger Tapping Task</dc:Title>
		<dc:Description>RDF output for 'Finger Tapping Task'</dc:Description>
		<dc:Type>InteractiveResource</dc:Type>
		<dc:Publisher>Cognitive Atlas</dc:Publisher>
		<dc:Creator>Cognitive Atlas RDF Generator</dc:Creator>
		<dc:Contributor>Brenda Gregory</dc:Contributor>
		<dc:Date>2011-04-27 15:39:02</dc:Date>
		<dc:Format>text/rdf</dc:Format>
		<dc:Language>en</dc:Language>
		<skos:editorialNote>Generated by testgenall.php on Thu Mar 29 10:24:07 PDT 2012.</skos:editorialNote>
		<skos:historyNote>Revision 2: 1 previous definitions.</skos:historyNote>
		<skos:changeNote>See http://www.cognitiveatlas.org/id/trm_4c898f079d05e for complete revision history.</skos:changeNote>
		<skos:scopeNote>http://www.w3.org/2004/02/skos/core#Concept</skos:scopeNote>
		<skos:Note>SKOS properties defined in http://www.w3.org/TR/skos-primer/#secrel</skos:Note>
		<skos:inScheme rdf:resource="http://www.cognitiveatlas.org/tasks/"/>
		<skos:definition>Subjects tap their fingers according to a visual, auditory, or no cue.</skos:definition>
		<skos:prefLabel>Finger Tapping Task</skos:prefLabel>
		<skos:altLabel></skos:altLabel>
		<skos:related rdf:resource="http://www.cognitiveatlas.org/id/trm_4a3fd79d0a972"/>
		<skos:related rdf:resource="http://www.cognitiveatlas.org/id/trm_4a3fd79d0a972"/>
		<skos:related rdf:resource="http://www.cognitiveatlas.org/id/trm_4a3fd79d0afc3"/>
		<skos:related rdf:resource="http://www.cognitiveatlas.org/id/trm_4a3fd79d0a9a1"/>
		<skos:related rdf:resource="http://www.cognitiveatlas.org/id/trm_4a3fd79d0a9a1"/>
		<skos:example>motor control is measured by the contrast of % rhythm maintainance trials in the Finger Tapping Task</skos:example>
		<skos:example>motor control is measured by the contrast of tap speed trials in the Finger Tapping Task</skos:example>
		<skos:example>rhythm is measured by the contrast of % rhythm maintainance trials in the Finger Tapping Task</skos:example>
		<skos:example>motor planning is measured by the contrast of % rhythm maintainance trials in the Finger Tapping Task</skos:example>
		<skos:example>motor planning is measured by the contrast of tap speed trials in the Finger Tapping Task</skos:example>
		<cito:citesForInformation rdf:resource="http://www.cognitiveatlas.org/citation/id/cit_4ded24f51cbfe"/>
		<cito:citesForInformation rdf:resource="http://www.cognitiveatlas.org/citation/id/cit_4ded266c7ec7a"/>
		<cito:citesForInformation rdf:resource="http://www.cognitiveatlas.org/citation/id/cit_4ded2a5caaa84"/>
</skos:Concept><skos:Concept rdf:about="http://www.cognitiveatlas.org/id/trm_4c898f72228f3"> <dc:identifier>trm_4c898f72228f3</dc:identifier>
		<dc:Title>Cognitive Atlas : Lexicon : Fixation Task</dc:Title>
		<dc:Description>RDF output for 'Fixation Task'</dc:Description>
		<dc:Type>InteractiveResource</dc:Type>
		<dc:Publisher>Cognitive Atlas</dc:Publisher>
		<dc:Creator>Cognitive Atlas RDF Generator</dc:Creator>
		<dc:Contributor>Brenda Gregory</dc:Contributor>
		<dc:Date>2011-04-27 15:50:02</dc:Date>
		<dc:Format>text/rdf</dc:Format>
		<dc:Language>en</dc:Language>
		<skos:editorialNote>Generated by testgenall.php on Thu Mar 29 10:24:07 PDT 2012.</skos:editorialNote>
		<skos:historyNote>Revision 2: 1 previous definitions.</skos:historyNote>
		<skos:changeNote>See http://www.cognitiveatlas.org/id/trm_4c898f72228f3 for complete revision history.</skos:changeNote>
		<skos:scopeNote>http://www.w3.org/2004/02/skos/core#Concept</skos:scopeNote>
		<skos:Note>SKOS properties defined in http://www.w3.org/TR/skos-primer/#secrel</skos:Note>
		<skos:inScheme rdf:resource="http://www.cognitiveatlas.org/tasks/"/>
		<skos:definition>Subjects fixate on a visual target.</skos:definition>
		<skos:prefLabel>Fixation Task</skos:prefLabel>
		<skos:altLabel></skos:altLabel>
		<skos:related rdf:resource="http://www.cognitiveatlas.org/id/trm_4a3fd79d0b5e3"/>
		<skos:related rdf:resource="http://www.cognitiveatlas.org/id/trm_4a3fd79d0a3d2"/>
		<skos:related rdf:resource="http://www.cognitiveatlas.org/id/trm_4a3fd79d0b46f"/>
		<skos:related rdf:resource="http://www.cognitiveatlas.org/id/trm_4a3fd79d0b5ef"/>
		<skos:related rdf:resource="http://www.cognitiveatlas.org/id/trm_4a3fd79d0a38d"/>
		<skos:example>attention span is measured by the contrast of fixation time below maximum degree of eye movement trials in the Fixation Task</skos:example>
		<skos:example>gaze is measured by the contrast of degree of eye movement trials in the Fixation Task</skos:example>
		<skos:example>visual attention is measured by the contrast of degree of eye movement trials in the Fixation Task</skos:example>
		<skos:example>attentional focusing is measured by the contrast of fixation time below maximum degree of eye movement trials in the Fixation Task</skos:example>
		<skos:example>focused attention is measured by the contrast of fixation time below maximum degree of eye movement trials in the Fixation Task</skos:example>
		<cito:citesForInformation rdf:resource="http://www.cognitiveatlas.org/citation/id/cit_4ded3987ad7d8"/>
		<cito:citesForInformation rdf:resource="http://www.cognitiveatlas.org/citation/id/cit_4ded39a505d17"/>
</skos:Concept><skos:Concept rdf:about="http://www.cognitiveatlas.org/id/trm_4c898f8f297ac"> <dc:identifier>trm_4c898f8f297ac</dc:identifier>
		<dc:Title>Cognitive Atlas : Lexicon : Flashing Checkerboard</dc:Title>
		<dc:Description>RDF output for 'Flashing Checkerboard'</dc:Description>
		<dc:Type>InteractiveResource</dc:Type>
		<dc:Publisher>Cognitive Atlas</dc:Publisher>
		<dc:Creator>Cognitive Atlas RDF Generator</dc:Creator>
		<dc:Contributor>Brenda Gregory</dc:Contributor>
		<dc:Date>2011-04-27 15:37:14</dc:Date>
		<dc:Format>text/rdf</dc:Format>
		<dc:Language>en</dc:Language>
		<skos:editorialNote>Generated by testgenall.php on Thu Mar 29 10:24:07 PDT 2012.</skos:editorialNote>
		<skos:historyNote>Revision 2: 1 previous definitions.</skos:historyNote>
		<skos:changeNote>See http://www.cognitiveatlas.org/id/trm_4c898f8f297ac for complete revision history.</skos:changeNote>
		<skos:scopeNote>http://www.w3.org/2004/02/skos/core#Concept</skos:scopeNote>
		<skos:Note>SKOS properties defined in http://www.w3.org/TR/skos-primer/#secrel</skos:Note>
		<skos:inScheme rdf:resource="http://www.cognitiveatlas.org/tasks/"/>
		<skos:definition>Subjects view a flashing checkerboard.</skos:definition>
		<skos:prefLabel>Flashing Checkerboard</skos:prefLabel>
		<skos:altLabel></skos:altLabel>
		<cito:citesForInformation rdf:resource="http://www.cognitiveatlas.org/citation/id/cit_4ded3d4c05798"/>
		<cito:citesForInformation rdf:resource="http://www.cognitiveatlas.org/citation/id/cit_4ded3e2ad4374"/>
</skos:Concept><skos:Concept rdf:about="http://www.cognitiveatlas.org/id/trm_4c898fad429ed"> <dc:identifier>trm_4c898fad429ed</dc:identifier>
		<dc:Title>Cognitive Atlas : Lexicon : Flexion/Extension</dc:Title>
		<dc:Description>RDF output for 'Flexion/Extension'</dc:Description>
		<dc:Type>InteractiveResource</dc:Type>
		<dc:Publisher>Cognitive Atlas</dc:Publisher>
		<dc:Creator>Cognitive Atlas RDF Generator</dc:Creator>
		<dc:Contributor>Brenda Gregory</dc:Contributor>
		<dc:Date>2011-04-27 15:35:49</dc:Date>
		<dc:Format>text/rdf</dc:Format>
		<dc:Language>en</dc:Language>
		<skos:editorialNote>Generated by testgenall.php on Thu Mar 29 10:24:07 PDT 2012.</skos:editorialNote>
		<skos:historyNote>Revision 2: 1 previous definitions.</skos:historyNote>
		<skos:changeNote>See http://www.cognitiveatlas.org/id/trm_4c898fad429ed for complete revision history.</skos:changeNote>
		<skos:scopeNote>http://www.w3.org/2004/02/skos/core#Concept</skos:scopeNote>
		<skos:Note>SKOS properties defined in http://www.w3.org/TR/skos-primer/#secrel</skos:Note>
		<skos:inScheme rdf:resource="http://www.cognitiveatlas.org/tasks/"/>
		<skos:definition>Subjects move (flex and extend) their hands, arms, legs, feet, lips, tongue, etc.</skos:definition>
		<skos:prefLabel>Flexion/Extension</skos:prefLabel>
		<skos:altLabel></skos:altLabel>
		<skos:related rdf:resource="http://www.cognitiveatlas.org/id/trm_4a3fd79d0a972"/>
		<skos:example>motor control is measured by the contrast of average degrees of movement minus participant degrees of movement trials in the Flexion/Extension</skos:example>
		<cito:citesForInformation rdf:resource="http://www.cognitiveatlas.org/citation/id/cit_4e03ab99e1b02"/>
		<cito:citesForInformation rdf:resource="http://www.cognitiveatlas.org/citation/id/cit_4e03ae8ed5655"/>
</skos:Concept><skos:Concept rdf:about="http://www.cognitiveatlas.org/id/trm_4c898fc6722f4"> <dc:identifier>trm_4c898fc6722f4</dc:identifier>
		<dc:Title>Cognitive Atlas : Lexicon : Free Word List Recall</dc:Title>
		<dc:Description>RDF output for 'Free Word List Recall'</dc:Description>
		<dc:Type>InteractiveResource</dc:Type>
		<dc:Publisher>Cognitive Atlas</dc:Publisher>
		<dc:Creator>Cognitive Atlas RDF Generator</dc:Creator>
		<dc:Contributor>Brenda Gregory</dc:Contributor>
		<dc:Date>2011-04-27 15:35:17</dc:Date>
		<dc:Format>text/rdf</dc:Format>
		<dc:Language>en</dc:Language>
		<skos:editorialNote>Generated by testgenall.php on Thu Mar 29 10:24:07 PDT 2012.</skos:editorialNote>
		<skos:historyNote>Revision 2: 1 previous definitions.</skos:historyNote>
		<skos:changeNote>See http://www.cognitiveatlas.org/id/trm_4c898fc6722f4 for complete revision history.</skos:changeNote>
		<skos:scopeNote>http://www.w3.org/2004/02/skos/core#Concept</skos:scopeNote>
		<skos:Note>SKOS properties defined in http://www.w3.org/TR/skos-primer/#secrel</skos:Note>
		<skos:inScheme rdf:resource="http://www.cognitiveatlas.org/tasks/"/>
		<skos:definition>Subjects view a list of words and after a delay are asked to freely recall the words presented.</skos:definition>
		<skos:prefLabel>Free Word List Recall</skos:prefLabel>
		<skos:altLabel></skos:altLabel>
		<skos:related rdf:resource="http://www.cognitiveatlas.org/id/trm_4a3fd79d09cae"/>
		<skos:related rdf:resource="http://www.cognitiveatlas.org/id/trm_4a3fd79d0a1ae"/>
		<skos:related rdf:resource="http://www.cognitiveatlas.org/id/trm_4a3fd79d0b5a7"/>
		<skos:related rdf:resource="http://www.cognitiveatlas.org/id/trm_4a3fd79d0b5a7"/>
		<skos:example>chunking is measured by the contrast of category list trials in the Free Word List Recall</skos:example>
		<skos:example>emotional memory is measured by the contrast of emotion manipulation trials in the Free Word List Recall</skos:example>
		<skos:example>working memory is measured by the contrast of emotion manipulation trials in the Free Word List Recall</skos:example>
		<skos:example>working memory is measured by the contrast of category list trials in the Free Word List Recall</skos:example>
		<cito:citesForInformation rdf:resource="http://www.cognitiveatlas.org/citation/id/cit_4ded49d3ccb06"/>
		<cito:citesForInformation rdf:resource="http://www.cognitiveatlas.org/citation/id/cit_4ded4a820253d"/>
		<cito:citesForInformation rdf:resource="http://www.cognitiveatlas.org/citation/id/cit_4ded4cd6790d6"/>
</skos:Concept><skos:Concept rdf:about="http://www.cognitiveatlas.org/id/trm_4c898ff0bea97"> <dc:identifier>trm_4c898ff0bea97</dc:identifier>
		<dc:Title>Cognitive Atlas : Lexicon : Grasping Task</dc:Title>
		<dc:Description>RDF output for 'Grasping Task'</dc:Description>
		<dc:Type>InteractiveResource</dc:Type>
		<dc:Publisher>Cognitive Atlas</dc:Publisher>
		<dc:Creator>Cognitive Atlas RDF Generator</dc:Creator>
		<dc:Contributor>Brenda Gregory</dc:Contributor>
		<dc:Date>2011-04-27 15:34:50</dc:Date>
		<dc:Format>text/rdf</dc:Format>
		<dc:Language>en</dc:Language>
		<skos:editorialNote>Generated by testgenall.php on Thu Mar 29 10:24:07 PDT 2012.</skos:editorialNote>
		<skos:historyNote>Revision 2: 1 previous definitions.</skos:historyNote>
		<skos:changeNote>See http://www.cognitiveatlas.org/id/trm_4c898ff0bea97 for complete revision history.</skos:changeNote>
		<skos:scopeNote>http://www.w3.org/2004/02/skos/core#Concept</skos:scopeNote>
		<skos:Note>SKOS properties defined in http://www.w3.org/TR/skos-primer/#secrel</skos:Note>
		<skos:inScheme rdf:resource="http://www.cognitiveatlas.org/tasks/"/>
		<skos:definition>Subjects grasped or gripped a presented stimulus with their hand or mimicked grasping one that was not physically presented (i.e., was imaginary or presented as a picture or video).</skos:definition>
		<skos:prefLabel>Grasping Task</skos:prefLabel>
		<skos:altLabel></skos:altLabel>
		<skos:related rdf:resource="http://www.cognitiveatlas.org/id/trm_4a3fd79d0a9a1"/>
		<skos:related rdf:resource="http://www.cognitiveatlas.org/id/trm_4a3fd79d0a972"/>
		<skos:example>motor planning is measured by the contrast of response time trials in the Grasping Task</skos:example>
		<skos:example>motor control is measured by the contrast of kinematics trials in the Grasping Task</skos:example>
		<cito:citesForInformation rdf:resource="http://www.cognitiveatlas.org/citation/id/cit_4ded4f12303ba"/>
		<cito:citesForInformation rdf:resource="http://www.cognitiveatlas.org/citation/id/cit_4ded50957217b"/>
</skos:Concept><skos:Concept rdf:about="http://www.cognitiveatlas.org/id/trm_4c899005b11d5"> <dc:identifier>trm_4c899005b11d5</dc:identifier>
		<dc:Title>Cognitive Atlas : Lexicon : Imagined Movement</dc:Title>
		<dc:Description>RDF output for 'Imagined Movement'</dc:Description>
		<dc:Type>InteractiveResource</dc:Type>
		<dc:Publisher>Cognitive Atlas</dc:Publisher>
		<dc:Creator>Cognitive Atlas RDF Generator</dc:Creator>
		<dc:Contributor>Brenda Gregory</dc:Contributor>
		<dc:Date>2011-04-27 15:34:21</dc:Date>
		<dc:Format>text/rdf</dc:Format>
		<dc:Language>en</dc:Language>
		<skos:editorialNote>Generated by testgenall.php on Thu Mar 29 10:24:07 PDT 2012.</skos:editorialNote>
		<skos:historyNote>Revision 2: 1 previous definitions.</skos:historyNote>
		<skos:changeNote>See http://www.cognitiveatlas.org/id/trm_4c899005b11d5 for complete revision history.</skos:changeNote>
		<skos:scopeNote>http://www.w3.org/2004/02/skos/core#Concept</skos:scopeNote>
		<skos:Note>SKOS properties defined in http://www.w3.org/TR/skos-primer/#secrel</skos:Note>
		<skos:inScheme rdf:resource="http://www.cognitiveatlas.org/tasks/"/>
		<skos:definition>Subjects imagine performing some movement (e.g., finger tapping, reaching).</skos:definition>
		<skos:prefLabel>Imagined Movement</skos:prefLabel>
		<skos:altLabel></skos:altLabel>
		<skos:related rdf:resource="http://www.cognitiveatlas.org/id/trm_4a3fd79d09d4d"/>
		<skos:related rdf:resource="http://www.cognitiveatlas.org/id/trm_4a3fd79d0a504"/>
		<skos:related rdf:resource="http://www.cognitiveatlas.org/id/trm_4a3fd79d0a9a1"/>
		<skos:example>cognitive effort is measured by the contrast of real task effort minus imagined task effort trials in the Imagined Movement</skos:example>
		<skos:example>imageability is measured by the contrast of real task time minus imagined task time trials in the Imagined Movement</skos:example>
		<skos:example>motor planning is measured by the contrast of real task areas of activation minus imagined task areas of activation trials in the Imagined Movement</skos:example>
		<cito:citesForInformation rdf:resource="http://www.cognitiveatlas.org/citation/id/cit_4ded64ca43d85"/>
		<cito:citesForInformation rdf:resource="http://www.cognitiveatlas.org/citation/id/cit_4ded6591af1c4"/>
		<cito:citesForInformation rdf:resource="http://www.cognitiveatlas.org/citation/id/cit_4dee507055993"/>
</skos:Concept><skos:Concept rdf:about="http://www.cognitiveatlas.org/id/trm_4c89903149aeb"> <dc:identifier>trm_4c89903149aeb</dc:identifier>
		<dc:Title>Cognitive Atlas : Lexicon : Imagined Objects/Scenes</dc:Title>
		<dc:Description>RDF output for 'Imagined Objects/Scenes'</dc:Description>
		<dc:Type>InteractiveResource</dc:Type>
		<dc:Publisher>Cognitive Atlas</dc:Publisher>
		<dc:Creator>Cognitive Atlas RDF Generator</dc:Creator>
		<dc:Contributor>Brenda Gregory</dc:Contributor>
		<dc:Date>2011-04-27 14:07:59</dc:Date>
		<dc:Format>text/rdf</dc:Format>
		<dc:Language>en</dc:Language>
		<skos:editorialNote>Generated by testgenall.php on Thu Mar 29 10:24:07 PDT 2012.</skos:editorialNote>
		<skos:historyNote>Revision 2: 1 previous definitions.</skos:historyNote>
		<skos:changeNote>See http://www.cognitiveatlas.org/id/trm_4c89903149aeb for complete revision history.</skos:changeNote>
		<skos:scopeNote>http://www.w3.org/2004/02/skos/core#Concept</skos:scopeNote>
		<skos:Note>SKOS properties defined in http://www.w3.org/TR/skos-primer/#secrel</skos:Note>
		<skos:inScheme rdf:resource="http://www.cognitiveatlas.org/tasks/"/>
		<skos:definition>Subject generate vivid images of objects, places, concepts, hypothetical events (not in their past), or the completion of tasks.</skos:definition>
		<skos:prefLabel>Imagined Objects/Scenes</skos:prefLabel>
		<skos:altLabel></skos:altLabel>
		<skos:related rdf:resource="http://www.cognitiveatlas.org/id/trm_4a3fd79d09d35"/>
		<skos:related rdf:resource="http://www.cognitiveatlas.org/id/trm_4a3fd79d0a908"/>
		<skos:example>cognitive development is measured by the contrast of physical representation of imagined object trials in the Imagined Objects/Scenes</skos:example>
		<skos:example>mental representation is measured by the contrast of real visual areas of activation minus imagined task areas of activation trials in the Imagined Objects/Scenes</skos:example>
		<cito:citesForInformation rdf:resource="http://www.cognitiveatlas.org/citation/id/cit_4dee531f3d1d2"/>
		<cito:citesForInformation rdf:resource="http://www.cognitiveatlas.org/citation/id/cit_4dee58e9e6249"/>
</skos:Concept><skos:Concept rdf:about="http://www.cognitiveatlas.org/id/trm_4c8990480ad0f"> <dc:identifier>trm_4c8990480ad0f</dc:identifier>
		<dc:Title>Cognitive Atlas : Lexicon : Isometric Force</dc:Title>
		<dc:Description>RDF output for 'Isometric Force'</dc:Description>
		<dc:Type>InteractiveResource</dc:Type>
		<dc:Publisher>Cognitive Atlas</dc:Publisher>
		<dc:Creator>Cognitive Atlas RDF Generator</dc:Creator>
		<dc:Contributor>Brenda Gregory</dc:Contributor>
		<dc:Date>2011-04-27 14:07:22</dc:Date>
		<dc:Format>text/rdf</dc:Format>
		<dc:Language>en</dc:Language>
		<skos:editorialNote>Generated by testgenall.php on Thu Mar 29 10:24:07 PDT 2012.</skos:editorialNote>
		<skos:historyNote>Revision 2: 1 previous definitions.</skos:historyNote>
		<skos:changeNote>See http://www.cognitiveatlas.org/id/trm_4c8990480ad0f for complete revision history.</skos:changeNote>
		<skos:scopeNote>http://www.w3.org/2004/02/skos/core#Concept</skos:scopeNote>
		<skos:Note>SKOS properties defined in http://www.w3.org/TR/skos-primer/#secrel</skos:Note>
		<skos:inScheme rdf:resource="http://www.cognitiveatlas.org/tasks/"/>
		<skos:definition>Subjects use their hands or fingers to apply isometric force or complete a precision grip task.</skos:definition>
		<skos:prefLabel>Isometric Force</skos:prefLabel>
		<skos:altLabel></skos:altLabel>
		<skos:related rdf:resource="http://www.cognitiveatlas.org/id/trm_4a3fd79d0a972"/>
		<skos:related rdf:resource="http://www.cognitiveatlas.org/id/trm_4d7fc7c13b3c0"/>
		<skos:example>motor control is measured by the contrast of MVC minus baseline trials in the Isometric Force</skos:example>
		<skos:example> is measured by Isometric Force</skos:example>
		<cito:citesForInformation rdf:resource="http://www.cognitiveatlas.org/citation/id/cit_4df1170745145"/>
		<cito:citesForInformation rdf:resource="http://www.cognitiveatlas.org/citation/id/cit_4df118cd39510"/>
		<cito:citesForInformation rdf:resource="http://www.cognitiveatlas.org/citation/id/cit_4df118dbecd68"/>
</skos:Concept><skos:Concept rdf:about="http://www.cognitiveatlas.org/id/trm_4c8990810541d"> <dc:identifier>trm_4c8990810541d</dc:identifier>
		<dc:Title>Cognitive Atlas : Lexicon : Mental Rotation Task</dc:Title>
		<dc:Description>RDF output for 'Mental Rotation Task'</dc:Description>
		<dc:Type>InteractiveResource</dc:Type>
		<dc:Publisher>Cognitive Atlas</dc:Publisher>
		<dc:Creator>Cognitive Atlas RDF Generator</dc:Creator>
		<dc:Contributor>Brenda Gregory</dc:Contributor>
		<dc:Date>2011-04-27 14:06:49</dc:Date>
		<dc:Format>text/rdf</dc:Format>
		<dc:Language>en</dc:Language>
		<skos:editorialNote>Generated by testgenall.php on Thu Mar 29 10:24:07 PDT 2012.</skos:editorialNote>
		<skos:historyNote>Revision 2: 1 previous definitions.</skos:historyNote>
		<skos:changeNote>See http://www.cognitiveatlas.org/id/trm_4c8990810541d for complete revision history.</skos:changeNote>
		<skos:scopeNote>http://www.w3.org/2004/02/skos/core#Concept</skos:scopeNote>
		<skos:Note>SKOS properties defined in http://www.w3.org/TR/skos-primer/#secrel</skos:Note>
		<skos:inScheme rdf:resource="http://www.cognitiveatlas.org/tasks/"/>
		<skos:definition>Subjects view rotated letters, numbers, or objects (2D or 3D) and indicate if they are in their normal or mirror orientation; includes variations, but all tasks include mental rotation of stimuli.</skos:definition>
		<skos:prefLabel>Mental Rotation Task</skos:prefLabel>
		<skos:altLabel></skos:altLabel>
		<skos:related rdf:resource="http://www.cognitiveatlas.org/id/trm_4a3fd79d0a914"/>
		<skos:related rdf:resource="http://www.cognitiveatlas.org/id/trm_4a3fd79d0b1a6"/>
		<skos:related rdf:resource="http://www.cognitiveatlas.org/id/trm_4a3fd79d0b1a6"/>
		<skos:related rdf:resource="http://www.cognitiveatlas.org/id/trm_4af89b3a925ca"/>
		<skos:example>Mental Rotation Task is a broader synonym of Vandenberg & Kuse Tasks</skos:example>
		<skos:example>mental rotation is measured by the contrast of areas of activation during task minus baseline trials in the Mental Rotation Task</skos:example>
		<skos:example>spatial ability is measured by the contrast of average male score minus average female score trials in the Mental Rotation Task</skos:example>
		<skos:example>spatial ability is measured by the contrast of areas of activation during task minus baseline trials in the Mental Rotation Task</skos:example>
		<cito:citesForInformation rdf:resource="http://www.cognitiveatlas.org/citation/id/cit_4df2640e52fc0"/>
		<cito:citesForInformation rdf:resource="http://www.cognitiveatlas.org/citation/id/cit_4df26542d6fa4"/>
		<cito:citesForInformation rdf:resource="http://www.cognitiveatlas.org/citation/id/cit_4df265bceb313"/>
</skos:Concept><skos:Concept rdf:about="http://www.cognitiveatlas.org/id/trm_4c89909cc1f33"> <dc:identifier>trm_4c89909cc1f33</dc:identifier>
		<dc:Title>Cognitive Atlas : Lexicon : Micturition Task</dc:Title>
		<dc:Description>RDF output for 'Micturition Task'</dc:Description>
		<dc:Type>InteractiveResource</dc:Type>
		<dc:Publisher>Cognitive Atlas</dc:Publisher>
		<dc:Creator>Cognitive Atlas RDF Generator</dc:Creator>
		<dc:Contributor>Carinna Torgerson</dc:Contributor>
		<dc:Date>2011-06-10 14:14:20</dc:Date>
		<dc:Format>text/rdf</dc:Format>
		<dc:Language>en</dc:Language>
		<skos:editorialNote>Generated by testgenall.php on Thu Mar 29 10:24:07 PDT 2012.</skos:editorialNote>
		<skos:historyNote>Revision 3: 2 previous definitions.</skos:historyNote>
		<skos:changeNote>See http://www.cognitiveatlas.org/id/trm_4c89909cc1f33 for complete revision history.</skos:changeNote>
		<skos:scopeNote>http://www.w3.org/2004/02/skos/core#Concept</skos:scopeNote>
		<skos:Note>SKOS properties defined in http://www.w3.org/TR/skos-primer/#secrel</skos:Note>
		<skos:inScheme rdf:resource="http://www.cognitiveatlas.org/tasks/"/>
		<skos:definition>Subjects think about voiding urine, provide urine samples, or keep a micturition diary.</skos:definition>
		<skos:prefLabel>Micturition Task</skos:prefLabel>
		<skos:altLabel></skos:altLabel>
		<cito:citesForInformation rdf:resource="http://www.cognitiveatlas.org/citation/id/cit_4df28348481c8"/>
		<cito:citesForInformation rdf:resource="http://www.cognitiveatlas.org/citation/id/cit_4df28a235e3ea"/>
</skos:Concept><skos:Concept rdf:about="http://www.cognitiveatlas.org/id/trm_4c8990b07a037"> <dc:identifier>trm_4c8990b07a037</dc:identifier>
		<dc:Title>Cognitive Atlas : Lexicon : Music Comprehension/Production</dc:Title>
		<dc:Description>RDF output for 'Music Comprehension/Production'</dc:Description>
		<dc:Type>InteractiveResource</dc:Type>
		<dc:Publisher>Cognitive Atlas</dc:Publisher>
		<dc:Creator>Cognitive Atlas RDF Generator</dc:Creator>
		<dc:Contributor>Brenda Gregory</dc:Contributor>
		<dc:Date>2011-04-27 14:01:56</dc:Date>
		<dc:Format>text/rdf</dc:Format>
		<dc:Language>en</dc:Language>
		<skos:editorialNote>Generated by testgenall.php on Thu Mar 29 10:24:07 PDT 2012.</skos:editorialNote>
		<skos:historyNote>Revision 2: 1 previous definitions.</skos:historyNote>
		<skos:changeNote>See http://www.cognitiveatlas.org/id/trm_4c8990b07a037 for complete revision history.</skos:changeNote>
		<skos:scopeNote>http://www.w3.org/2004/02/skos/core#Concept</skos:scopeNote>
		<skos:Note>SKOS properties defined in http://www.w3.org/TR/skos-primer/#secrel</skos:Note>
		<skos:inScheme rdf:resource="http://www.cognitiveatlas.org/tasks/"/>
		<skos:definition>Subjects listen to music passively or are asked to sing overtly.</skos:definition>
		<skos:prefLabel>Music Comprehension/Production</skos:prefLabel>
		<skos:altLabel></skos:altLabel>
		<skos:related rdf:resource="http://www.cognitiveatlas.org/id/trm_4a3fd79d0989a"/>
		<skos:related rdf:resource="http://www.cognitiveatlas.org/id/trm_4a3fd79d0989a"/>
		<skos:related rdf:resource="http://www.cognitiveatlas.org/id/trm_4a3fd79d09b04"/>
		<skos:related rdf:resource="http://www.cognitiveatlas.org/id/trm_4a3fd79d0a6dc"/>
		<skos:related rdf:resource="http://www.cognitiveatlas.org/id/trm_4a3fd79d0afc3"/>
		<skos:example>articulatory planning is measured by the contrast of Production trials in the Music Comprehension/Production</skos:example>
		<skos:example>articulatory planning is measured by the contrast of accuracy of subject minus average accuracy of controls trials in the Music Comprehension/Production</skos:example>
		<skos:example>auditory working memory is measured by the contrast of accuracy of subject minus average accuracy of controls trials in the Music Comprehension/Production</skos:example>
		<skos:example>intonation is measured by the contrast of accuracy of subject minus average accuracy of controls trials in the Music Comprehension/Production</skos:example>
		<skos:example>rhythm is measured by the contrast of accuracy of subject minus average accuracy of controls trials in the Music Comprehension/Production</skos:example>
		<cito:citesForInformation rdf:resource="http://www.cognitiveatlas.org/citation/id/cit_4df29588eab25"/>
		<cito:citesForInformation rdf:resource="http://www.cognitiveatlas.org/citation/id/cit_4df296306eec0"/>
		<cito:citesForInformation rdf:resource="http://www.cognitiveatlas.org/citation/id/cit_4df29760dee51"/>
		<cito:citesForInformation rdf:resource="http://www.cognitiveatlas.org/citation/id/cit_4df29999d911d"/>
</skos:Concept><skos:Concept rdf:about="http://www.cognitiveatlas.org/id/trm_4c8990c87035d"> <dc:identifier>trm_4c8990c87035d</dc:identifier>
		<dc:Title>Cognitive Atlas : Lexicon : Naming (Covert)</dc:Title>
		<dc:Description>RDF output for 'Naming (Covert)'</dc:Description>
		<dc:Type>InteractiveResource</dc:Type>
		<dc:Publisher>Cognitive Atlas</dc:Publisher>
		<dc:Creator>Cognitive Atlas RDF Generator</dc:Creator>
		<dc:Contributor>Brenda Gregory</dc:Contributor>
		<dc:Date>2011-04-27 14:01:14</dc:Date>
		<dc:Format>text/rdf</dc:Format>
		<dc:Language>en</dc:Language>
		<skos:editorialNote>Generated by testgenall.php on Thu Mar 29 10:24:07 PDT 2012.</skos:editorialNote>
		<skos:historyNote>Revision 2: 1 previous definitions.</skos:historyNote>
		<skos:changeNote>See http://www.cognitiveatlas.org/id/trm_4c8990c87035d for complete revision history.</skos:changeNote>
		<skos:scopeNote>http://www.w3.org/2004/02/skos/core#Concept</skos:scopeNote>
		<skos:Note>SKOS properties defined in http://www.w3.org/TR/skos-primer/#secrel</skos:Note>
		<skos:inScheme rdf:resource="http://www.cognitiveatlas.org/tasks/"/>
		<skos:definition>Subjects view objects (pictures, line drawings, etc.) and name them silently.</skos:definition>
		<skos:prefLabel>Naming (Covert)</skos:prefLabel>
		<skos:altLabel></skos:altLabel>
		<skos:related rdf:resource="http://www.cognitiveatlas.org/id/trm_4a3fd79d0b077"/>
		<skos:related rdf:resource="http://www.cognitiveatlas.org/id/trm_4a3fd79d0b80f"/>
		<skos:related rdf:resource="http://www.cognitiveatlas.org/id/trm_4c8990e187dc7"/>
		<skos:example>semantic knowledge is measured by the contrast of areas of activation during task minus baseline trials in the Naming (Covert)</skos:example>
		<skos:example>lexical access is measured by the contrast of areas of activation during task minus baseline trials in the Naming (Covert)</skos:example>
		<skos:example>Naming (Overt) is related to Naming (Covert)</skos:example>
		<cito:citesForInformation rdf:resource="http://www.cognitiveatlas.org/citation/id/cit_4e03b605d042a"/>
		<cito:citesForInformation rdf:resource="http://www.cognitiveatlas.org/citation/id/cit_4e03b6a5a0645"/>
</skos:Concept><skos:Concept rdf:about="http://www.cognitiveatlas.org/id/trm_4c8990e187dc7"> <dc:identifier>trm_4c8990e187dc7</dc:identifier>
		<dc:Title>Cognitive Atlas : Lexicon : Naming (Overt)</dc:Title>
		<dc:Description>RDF output for 'Naming (Overt)'</dc:Description>
		<dc:Type>InteractiveResource</dc:Type>
		<dc:Publisher>Cognitive Atlas</dc:Publisher>
		<dc:Creator>Cognitive Atlas RDF Generator</dc:Creator>
		<dc:Contributor>Russ Poldrack</dc:Contributor>
		<dc:Date>2012-01-28 07:32:13</dc:Date>
		<dc:Format>text/rdf</dc:Format>
		<dc:Language>en</dc:Language>
		<skos:editorialNote>Generated by testgenall.php on Thu Mar 29 10:24:07 PDT 2012.</skos:editorialNote>
		<skos:historyNote>Revision 3: 2 previous definitions.</skos:historyNote>
		<skos:changeNote>See http://www.cognitiveatlas.org/id/trm_4c8990e187dc7 for complete revision history.</skos:changeNote>
		<skos:scopeNote>http://www.w3.org/2004/02/skos/core#Concept</skos:scopeNote>
		<skos:Note>SKOS properties defined in http://www.w3.org/TR/skos-primer/#secrel</skos:Note>
		<skos:inScheme rdf:resource="http://www.cognitiveatlas.org/tasks/"/>
		<skos:definition>Subjects view objects (pictures, line drawings, etc.)  and name them aloud.</skos:definition>
		<skos:prefLabel>Naming (Overt)</skos:prefLabel>
		<skos:altLabel>overt naming task, reading aloud task</skos:altLabel>
		<skos:related rdf:resource="http://www.cognitiveatlas.org/id/trm_4a3fd79d0b077"/>
		<skos:related rdf:resource="http://www.cognitiveatlas.org/id/trm_4a3fd79d0b80f"/>
		<skos:related rdf:resource="http://www.cognitiveatlas.org/id/trm_4a3fd79d0b44c"/>
		<skos:related rdf:resource="http://www.cognitiveatlas.org/id/trm_4a3fd79d0a9dc"/>
		<skos:related rdf:resource="http://www.cognitiveatlas.org/id/trm_4c8990c87035d"/>
		<skos:example>Naming (Overt) is related to Naming (Covert)</skos:example>
		<skos:example>semantic knowledge is measured by the contrast of areas of activation during task minus baseline trials in the Naming (Overt)</skos:example>
		<skos:example>lexical access is measured by the contrast of areas of activation during task minus baseline trials in the Naming (Overt)</skos:example>
		<skos:example>verbal fluency is measured by the contrast of accuracy of participant minus average accuracy of controls trials in the Naming (Overt)</skos:example>
		<skos:example>naming is measured by the contrast of  trials in the Naming (Overt)</skos:example>
		<cito:citesForInformation rdf:resource="http://www.cognitiveatlas.org/citation/id/cit_4e03b8a08daef"/>
		<cito:citesForInformation rdf:resource="http://www.cognitiveatlas.org/citation/id/cit_4e03b8e52443f"/>
</skos:Concept><skos:Concept rdf:about="http://www.cognitiveatlas.org/id/trm_4c8990f59266f"> <dc:identifier>trm_4c8990f59266f</dc:identifier>
		<dc:Title>Cognitive Atlas : Lexicon : Non-Painful Electrical Stimulation</dc:Title>
		<dc:Description>RDF output for 'Non-Painful Electrical Stimulation'</dc:Description>
		<dc:Type>InteractiveResource</dc:Type>
		<dc:Publisher>Cognitive Atlas</dc:Publisher>
		<dc:Creator>Cognitive Atlas RDF Generator</dc:Creator>
		<dc:Contributor>Brenda Gregory</dc:Contributor>
		<dc:Date>2011-04-27 14:11:03</dc:Date>
		<dc:Format>text/rdf</dc:Format>
		<dc:Language>en</dc:Language>
		<skos:editorialNote>Generated by testgenall.php on Thu Mar 29 10:24:07 PDT 2012.</skos:editorialNote>
		<skos:historyNote>Revision 2: 1 previous definitions.</skos:historyNote>
		<skos:changeNote>See http://www.cognitiveatlas.org/id/trm_4c8990f59266f for complete revision history.</skos:changeNote>
		<skos:scopeNote>http://www.w3.org/2004/02/skos/core#Concept</skos:scopeNote>
		<skos:Note>SKOS properties defined in http://www.w3.org/TR/skos-primer/#secrel</skos:Note>
		<skos:inScheme rdf:resource="http://www.cognitiveatlas.org/tasks/"/>
		<skos:definition>Subjects are electrically stimulated at a non-painful threshold.</skos:definition>
		<skos:prefLabel>Non-Painful Electrical Stimulation</skos:prefLabel>
		<skos:altLabel></skos:altLabel>
		<skos:related rdf:resource="http://www.cognitiveatlas.org/id/trm_4a3fd79d0b160"/>
		<skos:related rdf:resource="http://www.cognitiveatlas.org/id/trm_4c89910b7f8bc"/>
		<skos:example>somatosensation is measured by the contrast of average rating of sensation minus subject rating of sensation  trials in the Non-Painful Electrical Stimulation</skos:example>
		<skos:example>Non-Painful Thermal Stimulation is related to Non-Painful Electrical Stimulation</skos:example>
		<cito:citesForInformation rdf:resource="http://www.cognitiveatlas.org/citation/id/cit_4df2a29270c5a"/>
		<cito:citesForInformation rdf:resource="http://www.cognitiveatlas.org/citation/id/cit_4df2a2bd69110"/>
</skos:Concept><skos:Concept rdf:about="http://www.cognitiveatlas.org/id/trm_4c89910b7f8bc"> <dc:identifier>trm_4c89910b7f8bc</dc:identifier>
		<dc:Title>Cognitive Atlas : Lexicon : Non-Painful Thermal Stimulation</dc:Title>
		<dc:Description>RDF output for 'Non-Painful Thermal Stimulation'</dc:Description>
		<dc:Type>InteractiveResource</dc:Type>
		<dc:Publisher>Cognitive Atlas</dc:Publisher>
		<dc:Creator>Cognitive Atlas RDF Generator</dc:Creator>
		<dc:Contributor>Brenda Gregory</dc:Contributor>
		<dc:Date>2011-04-27 14:11:36</dc:Date>
		<dc:Format>text/rdf</dc:Format>
		<dc:Language>en</dc:Language>
		<skos:editorialNote>Generated by testgenall.php on Thu Mar 29 10:24:07 PDT 2012.</skos:editorialNote>
		<skos:historyNote>Revision 2: 1 previous definitions.</skos:historyNote>
		<skos:changeNote>See http://www.cognitiveatlas.org/id/trm_4c89910b7f8bc for complete revision history.</skos:changeNote>
		<skos:scopeNote>http://www.w3.org/2004/02/skos/core#Concept</skos:scopeNote>
		<skos:Note>SKOS properties defined in http://www.w3.org/TR/skos-primer/#secrel</skos:Note>
		<skos:inScheme rdf:resource="http://www.cognitiveatlas.org/tasks/"/>
		<skos:definition>Subjects experience thermal stimulation (heat) at a non-painful threshold.</skos:definition>
		<skos:prefLabel>Non-Painful Thermal Stimulation</skos:prefLabel>
		<skos:altLabel></skos:altLabel>
		<skos:related rdf:resource="http://www.cognitiveatlas.org/id/trm_4a3fd79d0b39d"/>
		<skos:related rdf:resource="http://www.cognitiveatlas.org/id/trm_4a3fd79d0b39d"/>
		<skos:related rdf:resource="http://www.cognitiveatlas.org/id/trm_4a3fd79d0b160"/>
		<skos:related rdf:resource="http://www.cognitiveatlas.org/id/trm_4a3fd79d0b160"/>
		<skos:related rdf:resource="http://www.cognitiveatlas.org/id/trm_4c8990f59266f"/>
		<skos:example>Non-Painful Thermal Stimulation is related to Non-Painful Electrical Stimulation</skos:example>
		<skos:example>thermosensation is measured by the contrast of rating of sensation minus baseline trials in the Non-Painful Thermal Stimulation</skos:example>
		<skos:example>thermosensation is measured by the contrast of average rating of sensation minus subject rating of sensation trials in the Non-Painful Thermal Stimulation</skos:example>
		<skos:example>somatosensation is measured by the contrast of areas of activation during task minus baseline trials in the Non-Painful Thermal Stimulation</skos:example>
		<skos:example>somatosensation is measured by the contrast of rating of sensation minus baseline trials in the Non-Painful Thermal Stimulation</skos:example>
		<cito:citesForInformation rdf:resource="http://www.cognitiveatlas.org/citation/id/cit_4df2a4f26e696"/>
		<cito:citesForInformation rdf:resource="http://www.cognitiveatlas.org/citation/id/cit_4df2a58e17389"/>
</skos:Concept><skos:Concept rdf:about="http://www.cognitiveatlas.org/id/trm_4c89912c79030"> <dc:identifier>trm_4c89912c79030</dc:identifier>
		<dc:Title>Cognitive Atlas : Lexicon : Olfactory Monitor/Discrimination</dc:Title>
		<dc:Description>RDF output for 'Olfactory Monitor/Discrimination'</dc:Description>
		<dc:Type>InteractiveResource</dc:Type>
		<dc:Publisher>Cognitive Atlas</dc:Publisher>
		<dc:Creator>Cognitive Atlas RDF Generator</dc:Creator>
		<dc:Contributor>Brenda Gregory</dc:Contributor>
		<dc:Date>2011-04-27 14:10:26</dc:Date>
		<dc:Format>text/rdf</dc:Format>
		<dc:Language>en</dc:Language>
		<skos:editorialNote>Generated by testgenall.php on Thu Mar 29 10:24:07 PDT 2012.</skos:editorialNote>
		<skos:historyNote>Revision 2: 1 previous definitions.</skos:historyNote>
		<skos:changeNote>See http://www.cognitiveatlas.org/id/trm_4c89912c79030 for complete revision history.</skos:changeNote>
		<skos:scopeNote>http://www.w3.org/2004/02/skos/core#Concept</skos:scopeNote>
		<skos:Note>SKOS properties defined in http://www.w3.org/TR/skos-primer/#secrel</skos:Note>
		<skos:inScheme rdf:resource="http://www.cognitiveatlas.org/tasks/"/>
		<skos:definition>Subjects are presented with odors and are instructed to smell them passively or to discriminate according to some feature (pleasant/unpleasant, strong/weak, same/different, etc.).</skos:definition>
		<skos:prefLabel>Olfactory Monitor/Discrimination</skos:prefLabel>
		<skos:altLabel></skos:altLabel>
		<skos:related rdf:resource="http://www.cognitiveatlas.org/id/trm_4a3fd79d0aac8"/>
		<skos:example>olfactory perception is measured by the contrast of average accuracy of controls minus accuracy of participant trials in the Olfactory Monitor/Discrimination</skos:example>
		<cito:citesForInformation rdf:resource="http://www.cognitiveatlas.org/citation/id/cit_4df67bf2e5c6e"/>
		<cito:citesForInformation rdf:resource="http://www.cognitiveatlas.org/citation/id/cit_4df67ccdb54d7"/>
</skos:Concept><skos:Concept rdf:about="http://www.cognitiveatlas.org/id/trm_4c89913f80802"> <dc:identifier>trm_4c89913f80802</dc:identifier>
		<dc:Title>Cognitive Atlas : Lexicon : Orthographic Discrimination</dc:Title>
		<dc:Description>RDF output for 'Orthographic Discrimination'</dc:Description>
		<dc:Type>InteractiveResource</dc:Type>
		<dc:Publisher>Cognitive Atlas</dc:Publisher>
		<dc:Creator>Cognitive Atlas RDF Generator</dc:Creator>
		<dc:Contributor>Brenda Gregory</dc:Contributor>
		<dc:Date>2011-04-27 14:09:45</dc:Date>
		<dc:Format>text/rdf</dc:Format>
		<dc:Language>en</dc:Language>
		<skos:editorialNote>Generated by testgenall.php on Thu Mar 29 10:24:07 PDT 2012.</skos:editorialNote>
		<skos:historyNote>Revision 2: 1 previous definitions.</skos:historyNote>
		<skos:changeNote>See http://www.cognitiveatlas.org/id/trm_4c89913f80802 for complete revision history.</skos:changeNote>
		<skos:scopeNote>http://www.w3.org/2004/02/skos/core#Concept</skos:scopeNote>
		<skos:Note>SKOS properties defined in http://www.w3.org/TR/skos-primer/#secrel</skos:Note>
		<skos:inScheme rdf:resource="http://www.cognitiveatlas.org/tasks/"/>
		<skos:definition>Subjects view letters and discriminate according to some feature (uppercase/lowercase, alphabetic order, same/different spelling of words, vowel/consonant, font size, etc.).</skos:definition>
		<skos:prefLabel>Orthographic Discrimination</skos:prefLabel>
		<skos:altLabel></skos:altLabel>
		<skos:related rdf:resource="http://www.cognitiveatlas.org/id/trm_4a3fd79d0a398"/>
		<skos:related rdf:resource="http://www.cognitiveatlas.org/id/trm_4a3fd79d0b4d8"/>
		<skos:related rdf:resource="http://www.cognitiveatlas.org/id/trm_4a3fd79d0b4b5"/>
		<skos:example>form perception is measured by the contrast of average accuracy of controls minus accuracy of participant trials in the Orthographic Discrimination</skos:example>
		<skos:example>visual working memory is measured by the contrast of average accuracy of controls minus accuracy of participant trials in the Orthographic Discrimination</skos:example>
		<skos:example>visual perception is measured by the contrast of average accuracy of controls minus accuracy of participant trials in the Orthographic Discrimination</skos:example>
		<cito:citesForInformation rdf:resource="http://www.cognitiveatlas.org/citation/id/cit_4df685705601c"/>
		<cito:citesForInformation rdf:resource="http://www.cognitiveatlas.org/citation/id/cit_4df685a7276bf"/>
</skos:Concept><skos:Concept rdf:about="http://www.cognitiveatlas.org/id/trm_4c8991c5beb0a"> <dc:identifier>trm_4c8991c5beb0a</dc:identifier>
		<dc:Title>Cognitive Atlas : Lexicon : Pain Monitor/Discrimination Task</dc:Title>
		<dc:Description>RDF output for 'Pain Monitor/Discrimination Task'</dc:Description>
		<dc:Type>InteractiveResource</dc:Type>
		<dc:Publisher>Cognitive Atlas</dc:Publisher>
		<dc:Creator>Cognitive Atlas RDF Generator</dc:Creator>
		<dc:Contributor>Russ Poldrack</dc:Contributor>
		<dc:Date>2012-01-28 08:02:42</dc:Date>
		<dc:Format>text/rdf</dc:Format>
		<dc:Language>en</dc:Language>
		<skos:editorialNote>Generated by testgenall.php on Thu Mar 29 10:24:07 PDT 2012.</skos:editorialNote>
		<skos:historyNote>Revision 4: 3 previous definitions.</skos:historyNote>
		<skos:changeNote>See http://www.cognitiveatlas.org/id/trm_4c8991c5beb0a for complete revision history.</skos:changeNote>
		<skos:scopeNote>http://www.w3.org/2004/02/skos/core#Concept</skos:scopeNote>
		<skos:Note>SKOS properties defined in http://www.w3.org/TR/skos-primer/#secrel</skos:Note>
		<skos:inScheme rdf:resource="http://www.cognitiveatlas.org/tasks/"/>
		<skos:definition>Subjects experience thermal or electrical stimulation at a painful threshold.</skos:definition>
		<skos:prefLabel>Pain Monitor/Discrimination Task</skos:prefLabel>
		<skos:altLabel>pain judgment task</skos:altLabel>
		<skos:related rdf:resource="http://www.cognitiveatlas.org/id/trm_4a3fd79d0b160"/>
		<skos:related rdf:resource="http://www.cognitiveatlas.org/id/trm_4a3fd79d0b160"/>
		<skos:example>somatosensation is measured by the contrast of areas of activation during task minus baseline trials in the Pain Monitor/Discrimination Task</skos:example>
		<skos:example>somatosensation is measured by the contrast of subject rating during task minus subject baseline rating trials in the Pain Monitor/Discrimination Task</skos:example>
		<cito:citesForInformation rdf:resource="http://www.cognitiveatlas.org/citation/id/cit_4df687ee627dc"/>
</skos:Concept><skos:Concept rdf:about="http://www.cognitiveatlas.org/id/trm_4c8991e6e8597"> <dc:identifier>trm_4c8991e6e8597</dc:identifier>
		<dc:Title>Cognitive Atlas : Lexicon : Paired Associate Recall</dc:Title>
		<dc:Description>RDF output for 'Paired Associate Recall'</dc:Description>
		<dc:Type>InteractiveResource</dc:Type>
		<dc:Publisher>Cognitive Atlas</dc:Publisher>
		<dc:Creator>Cognitive Atlas RDF Generator</dc:Creator>
		<dc:Contributor>Brenda Gregory</dc:Contributor>
		<dc:Date>2011-04-27 14:08:41</dc:Date>
		<dc:Format>text/rdf</dc:Format>
		<dc:Language>en</dc:Language>
		<skos:editorialNote>Generated by testgenall.php on Thu Mar 29 10:24:07 PDT 2012.</skos:editorialNote>
		<skos:historyNote>Revision 2: 1 previous definitions.</skos:historyNote>
		<skos:changeNote>See http://www.cognitiveatlas.org/id/trm_4c8991e6e8597 for complete revision history.</skos:changeNote>
		<skos:scopeNote>http://www.w3.org/2004/02/skos/core#Concept</skos:scopeNote>
		<skos:Note>SKOS properties defined in http://www.w3.org/TR/skos-primer/#secrel</skos:Note>
		<skos:inScheme rdf:resource="http://www.cognitiveatlas.org/tasks/"/>
		<skos:definition>Subjects are shown paired stimuli prior to the task.  During the task, subjects are shown a single stimuli and are asked to recall the associated pair.  Stimuli may be words, faces, objects, etc.</skos:definition>
		<skos:prefLabel>Paired Associate Recall</skos:prefLabel>
		<skos:altLabel></skos:altLabel>
		<skos:related rdf:resource="http://www.cognitiveatlas.org/id/trm_4a3fd79d0b08f"/>
		<skos:related rdf:resource="http://www.cognitiveatlas.org/id/trm_4a3fd79d098c9"/>
		<skos:example>semantic working memory is measured by the contrast of accuracy of participant minus average accuracy of controls trials in the Paired Associate Recall</skos:example>
		<skos:example>association learning is measured by the contrast of accuracy of participant minus average accuracy of controls trials in the Paired Associate Recall</skos:example>
		<cito:citesForInformation rdf:resource="http://www.cognitiveatlas.org/citation/id/cit_4df68cbf988f6"/>
		<cito:citesForInformation rdf:resource="http://www.cognitiveatlas.org/citation/id/cit_4df68dd003e32"/>
</skos:Concept><skos:Concept rdf:about="http://www.cognitiveatlas.org/id/trm_4c8991fadfe01"> <dc:identifier>trm_4c8991fadfe01</dc:identifier>
		<dc:Title>Cognitive Atlas : Lexicon : Passive Listening</dc:Title>
		<dc:Description>RDF output for 'Passive Listening'</dc:Description>
		<dc:Type>InteractiveResource</dc:Type>
		<dc:Publisher>Cognitive Atlas</dc:Publisher>
		<dc:Creator>Cognitive Atlas RDF Generator</dc:Creator>
		<dc:Contributor>Brenda Gregory</dc:Contributor>
		<dc:Date>2011-04-27 14:06:12</dc:Date>
		<dc:Format>text/rdf</dc:Format>
		<dc:Language>en</dc:Language>
		<skos:editorialNote>Generated by testgenall.php on Thu Mar 29 10:24:07 PDT 2012.</skos:editorialNote>
		<skos:historyNote>Revision 2: 1 previous definitions.</skos:historyNote>
		<skos:changeNote>See http://www.cognitiveatlas.org/id/trm_4c8991fadfe01 for complete revision history.</skos:changeNote>
		<skos:scopeNote>http://www.w3.org/2004/02/skos/core#Concept</skos:scopeNote>
		<skos:Note>SKOS properties defined in http://www.w3.org/TR/skos-primer/#secrel</skos:Note>
		<skos:inScheme rdf:resource="http://www.cognitiveatlas.org/tasks/"/>
		<skos:definition>Subjects listen to various auditory stimuli and make no response.  Stimuli include speech (words, sentences), noise, tones, etc.  If the stimulus is tones, then the experiment is co-coded with Tone Monitor/Discrimination.</skos:definition>
		<skos:prefLabel>Passive Listening</skos:prefLabel>
		<skos:altLabel></skos:altLabel>
		<skos:related rdf:resource="http://www.cognitiveatlas.org/id/trm_4a3fd79d0995e"/>
		<skos:related rdf:resource="http://www.cognitiveatlas.org/id/trm_4a3fd79d0995e"/>
		<skos:related rdf:resource="http://www.cognitiveatlas.org/id/trm_4a3fd79d0971e"/>
		<skos:related rdf:resource="http://www.cognitiveatlas.org/id/trm_4a3fd79d0971e"/>
		<skos:related rdf:resource="http://www.cognitiveatlas.org/id/trm_4c8a84825c4e4"/>
		<skos:example>audition is measured by the contrast of areas of activation during task minus baseline trials in the Passive Listening</skos:example>
		<skos:example>audition is measured by the contrast of BOLD activity during task minus baseline trials in the Passive Listening</skos:example>
		<skos:example>acoustic processing is measured by the contrast of areas of activation during task minus baseline trials in the Passive Listening</skos:example>
		<skos:example>acoustic processing is measured by the contrast of BOLD activity during task minus baseline trials in the Passive Listening</skos:example>
		<skos:example>Tone Monitor/Discrimination is related to Passive Listening</skos:example>
		<cito:citesForInformation rdf:resource="http://www.cognitiveatlas.org/citation/id/cit_4df69a05abcdf"/>
		<cito:citesForInformation rdf:resource="http://www.cognitiveatlas.org/citation/id/cit_4df69a462da8f"/>
		<cito:citesForInformation rdf:resource="http://www.cognitiveatlas.org/citation/id/cit_4df69a7fcd8a1"/>
</skos:Concept><skos:Concept rdf:about="http://www.cognitiveatlas.org/id/trm_4c899211a965c"> <dc:identifier>trm_4c899211a965c</dc:identifier>
		<dc:Title>Cognitive Atlas : Lexicon : Passive Viewing</dc:Title>
		<dc:Description>RDF output for 'Passive Viewing'</dc:Description>
		<dc:Type>InteractiveResource</dc:Type>
		<dc:Publisher>Cognitive Atlas</dc:Publisher>
		<dc:Creator>Cognitive Atlas RDF Generator</dc:Creator>
		<dc:Contributor>Brenda Gregory</dc:Contributor>
		<dc:Date>2011-04-27 14:05:32</dc:Date>
		<dc:Format>text/rdf</dc:Format>
		<dc:Language>en</dc:Language>
		<skos:editorialNote>Generated by testgenall.php on Thu Mar 29 10:24:07 PDT 2012.</skos:editorialNote>
		<skos:historyNote>Revision 2: 1 previous definitions.</skos:historyNote>
		<skos:changeNote>See http://www.cognitiveatlas.org/id/trm_4c899211a965c for complete revision history.</skos:changeNote>
		<skos:scopeNote>http://www.w3.org/2004/02/skos/core#Concept</skos:scopeNote>
		<skos:Note>SKOS properties defined in http://www.w3.org/TR/skos-primer/#secrel</skos:Note>
		<skos:inScheme rdf:resource="http://www.cognitiveatlas.org/tasks/"/>
		<skos:definition>Subjects view various visual stimuli and make no response.  Stimuli include houses, faces, objects, fractals, letter strings, line drawings, complex scenes, etc. If the presented stimuli were faces, the experiments are co-coded with Face Monitor/Discrimination.  But if the presented stimuli are words, the experiments are NOT coded as Passive Viewing but rather as Reading (Covert).</skos:definition>
		<skos:prefLabel>Passive Viewing</skos:prefLabel>
		<skos:altLabel></skos:altLabel>
		<skos:related rdf:resource="http://www.cognitiveatlas.org/id/trm_4a3fd79d0b4b5"/>
		<skos:related rdf:resource="http://www.cognitiveatlas.org/id/trm_4a3fd79d0b4b5"/>
		<skos:example>visual perception is measured by the contrast of areas of activation during task minus baseline trials in the Passive Viewing</skos:example>
		<skos:example>visual perception is measured by the contrast of BOLD activity during task minus baseline trials in the Passive Viewing</skos:example>
		<cito:citesForInformation rdf:resource="http://www.cognitiveatlas.org/citation/id/cit_4df69bc1e8b17"/>
		<cito:citesForInformation rdf:resource="http://www.cognitiveatlas.org/citation/id/cit_4df69c4ab40a5"/>
</skos:Concept><skos:Concept rdf:about="http://www.cognitiveatlas.org/id/trm_4c89922cb6402"> <dc:identifier>trm_4c89922cb6402</dc:identifier>
		<dc:Title>Cognitive Atlas : Lexicon : Phonological Discrimination</dc:Title>
		<dc:Description>RDF output for 'Phonological Discrimination'</dc:Description>
		<dc:Type>InteractiveResource</dc:Type>
		<dc:Publisher>Cognitive Atlas</dc:Publisher>
		<dc:Creator>Cognitive Atlas RDF Generator</dc:Creator>
		<dc:Contributor>Russ Poldrack</dc:Contributor>
		<dc:Date>2012-01-28 07:55:55</dc:Date>
		<dc:Format>text/rdf</dc:Format>
		<dc:Language>en</dc:Language>
		<skos:editorialNote>Generated by testgenall.php on Thu Mar 29 10:24:07 PDT 2012.</skos:editorialNote>
		<skos:historyNote>Revision 3: 2 previous definitions.</skos:historyNote>
		<skos:changeNote>See http://www.cognitiveatlas.org/id/trm_4c89922cb6402 for complete revision history.</skos:changeNote>
		<skos:scopeNote>http://www.w3.org/2004/02/skos/core#Concept</skos:scopeNote>
		<skos:Note>SKOS properties defined in http://www.w3.org/TR/skos-primer/#secrel</skos:Note>
		<skos:inScheme rdf:resource="http://www.cognitiveatlas.org/tasks/"/>
		<skos:definition>Subjects view or listen to phonemes, syllables, or words and discriminate according to some feature of their sounds (rhyming, number of syllables, homophones, etc.).</skos:definition>
		<skos:prefLabel>Phonological Discrimination</skos:prefLabel>
		<skos:altLabel>phonological decision task</skos:altLabel>
		<skos:related rdf:resource="http://www.cognitiveatlas.org/id/trm_4a3fd79d09713"/>
		<skos:related rdf:resource="http://www.cognitiveatlas.org/id/trm_4a3fd79d0b238"/>
		<skos:related rdf:resource="http://www.cognitiveatlas.org/id/trm_4a3fd79d0b247"/>
		<skos:example>acoustic phonetic processing is measured by the contrast of accuracy of participant minus average accuracy of controls trials in the Phonological Discrimination</skos:example>
		<skos:example>speech processing is measured by the contrast of accuracy of participant minus average accuracy of controls trials in the Phonological Discrimination</skos:example>
		<skos:example>speech production is measured by the contrast of accuracy of participant minus average accuracy of controls trials in the Phonological Discrimination</skos:example>
		<cito:citesForInformation rdf:resource="http://www.cognitiveatlas.org/citation/id/cit_4df6a1763f297"/>
		<cito:citesForInformation rdf:resource="http://www.cognitiveatlas.org/citation/id/cit_4df6a2981317a"/>
</skos:Concept><skos:Concept rdf:about="http://www.cognitiveatlas.org/id/trm_4c89924414c69"> <dc:identifier>trm_4c89924414c69</dc:identifier>
		<dc:Title>Cognitive Atlas : Lexicon : Pitch Monitor/Discrimination</dc:Title>
		<dc:Description>RDF output for 'Pitch Monitor/Discrimination'</dc:Description>
		<dc:Type>InteractiveResource</dc:Type>
		<dc:Publisher>Cognitive Atlas</dc:Publisher>
		<dc:Creator>Cognitive Atlas RDF Generator</dc:Creator>
		<dc:Contributor>Russ Poldrack</dc:Contributor>
		<dc:Date>2012-01-28 07:07:58</dc:Date>
		<dc:Format>text/rdf</dc:Format>
		<dc:Language>en</dc:Language>
		<skos:editorialNote>Generated by testgenall.php on Thu Mar 29 10:24:07 PDT 2012.</skos:editorialNote>
		<skos:historyNote>Revision 3: 2 previous definitions.</skos:historyNote>
		<skos:changeNote>See http://www.cognitiveatlas.org/id/trm_4c89924414c69 for complete revision history.</skos:changeNote>
		<skos:scopeNote>http://www.w3.org/2004/02/skos/core#Concept</skos:scopeNote>
		<skos:Note>SKOS properties defined in http://www.w3.org/TR/skos-primer/#secrel</skos:Note>
		<skos:inScheme rdf:resource="http://www.cognitiveatlas.org/tasks/"/>
		<skos:definition>Subjects are presented with various stimuli (human speech and non-speech vocalizations, animal vocalization, mechanical noise, etc.) and are instructed to listen to them passively (also co-coded with Passive Listening), or discriminate based on pitch (pleasant/unpleasant, same/different, duration, familiar/unfamiliar, male/female).</skos:definition>
		<skos:prefLabel>Pitch Monitor/Discrimination</skos:prefLabel>
		<skos:altLabel>pitch discrimination task</skos:altLabel>
		<skos:related rdf:resource="http://www.cognitiveatlas.org/id/trm_4a3fd79d09713"/>
		<skos:related rdf:resource="http://www.cognitiveatlas.org/id/trm_4c8a84825c4e4"/>
		<skos:example>acoustic phonetic processing is measured by the contrast of accuracy of participant minus average accuracy of controls trials in the Pitch Monitor/Discrimination</skos:example>
		<skos:example>Tone Monitor/Discrimination is an exact synonym of Pitch Monitor/Discrimination</skos:example>
		<cito:citesForInformation rdf:resource="http://www.cognitiveatlas.org/citation/id/cit_4df7abf9d8f2d"/>
		<cito:citesForInformation rdf:resource="http://www.cognitiveatlas.org/citation/id/cit_4df7b76fb3126"/>
</skos:Concept><skos:Concept rdf:about="http://www.cognitiveatlas.org/id/trm_4c89926767870"> <dc:identifier>trm_4c89926767870</dc:identifier>
		<dc:Title>Cognitive Atlas : Lexicon : Pointing</dc:Title>
		<dc:Description>RDF output for 'Pointing'</dc:Description>
		<dc:Type>InteractiveResource</dc:Type>
		<dc:Publisher>Cognitive Atlas</dc:Publisher>
		<dc:Creator>Cognitive Atlas RDF Generator</dc:Creator>
		<dc:Contributor>Brenda Gregory</dc:Contributor>
		<dc:Date>2011-04-27 14:03:44</dc:Date>
		<dc:Format>text/rdf</dc:Format>
		<dc:Language>en</dc:Language>
		<skos:editorialNote>Generated by testgenall.php on Thu Mar 29 10:24:07 PDT 2012.</skos:editorialNote>
		<skos:historyNote>Revision 2: 1 previous definitions.</skos:historyNote>
		<skos:changeNote>See http://www.cognitiveatlas.org/id/trm_4c89926767870 for complete revision history.</skos:changeNote>
		<skos:scopeNote>http://www.w3.org/2004/02/skos/core#Concept</skos:scopeNote>
		<skos:Note>SKOS properties defined in http://www.w3.org/TR/skos-primer/#secrel</skos:Note>
		<skos:inScheme rdf:resource="http://www.cognitiveatlas.org/tasks/"/>
		<skos:definition>Subjects look and point at a target (e.g., cursor with their arm, hand, finger, or shoulder.</skos:definition>
		<skos:prefLabel>Pointing</skos:prefLabel>
		<skos:altLabel></skos:altLabel>
		<skos:related rdf:resource="http://www.cognitiveatlas.org/id/trm_4a3fd79d0a9a1"/>
		<skos:related rdf:resource="http://www.cognitiveatlas.org/id/trm_4a3fd79d0b1a6"/>
		<skos:related rdf:resource="http://www.cognitiveatlas.org/id/trm_4b75ed06c917d"/>
		<skos:related rdf:resource="http://www.cognitiveatlas.org/id/trm_4a3fd79d0a72e"/>
		<skos:example>motor planning is measured by the contrast of standard deviation of error trials in the Pointing</skos:example>
		<skos:example>spatial ability is measured by the contrast of standard deviation of error trials in the Pointing</skos:example>
		<skos:example>Joint Attention is measured by the contrast of standard deviation of error trials in the Pointing</skos:example>
		<skos:example>kinaesthetic representation is measured by the contrast of standard deviation of error trials in the Pointing</skos:example>
		<cito:citesForInformation rdf:resource="http://www.cognitiveatlas.org/citation/id/cit_4df7bcf4a87cd"/>
		<cito:citesForInformation rdf:resource="http://www.cognitiveatlas.org/citation/id/cit_4df7bdb501ff1"/>
		<cito:citesForInformation rdf:resource="http://www.cognitiveatlas.org/citation/id/cit_4df7bf865d315"/>
</skos:Concept><skos:Concept rdf:about="http://www.cognitiveatlas.org/id/trm_4c8a82ba8a538"> <dc:identifier>trm_4c8a82ba8a538</dc:identifier>
		<dc:Title>Cognitive Atlas : Lexicon : Reading (Covert)</dc:Title>
		<dc:Description>RDF output for 'Reading (Covert)'</dc:Description>
		<dc:Type>InteractiveResource</dc:Type>
		<dc:Publisher>Cognitive Atlas</dc:Publisher>
		<dc:Creator>Cognitive Atlas RDF Generator</dc:Creator>
		<dc:Contributor>Russ Poldrack</dc:Contributor>
		<dc:Date>2012-01-28 08:12:17</dc:Date>
		<dc:Format>text/rdf</dc:Format>
		<dc:Language>en</dc:Language>
		<skos:editorialNote>Generated by testgenall.php on Thu Mar 29 10:24:07 PDT 2012.</skos:editorialNote>
		<skos:historyNote>Revision 4: 3 previous definitions.</skos:historyNote>
		<skos:changeNote>See http://www.cognitiveatlas.org/id/trm_4c8a82ba8a538 for complete revision history.</skos:changeNote>
		<skos:scopeNote>http://www.w3.org/2004/02/skos/core#Concept</skos:scopeNote>
		<skos:Note>SKOS properties defined in http://www.w3.org/TR/skos-primer/#secrel</skos:Note>
		<skos:inScheme rdf:resource="http://www.cognitiveatlas.org/tasks/"/>
		<skos:definition>Subjects view words, pseudo-words,  Asian characters, phrases, or sentences and read them silently.</skos:definition>
		<skos:prefLabel>Reading (Covert)</skos:prefLabel>
		<skos:altLabel>covert reading task, silent reading task, silent production task</skos:altLabel>
		<skos:related rdf:resource="http://www.cognitiveatlas.org/id/trm_4c8a82eeaa58f"/>
		<skos:example>Reading (Covert) is related to Reading (Overt)</skos:example>
</skos:Concept><skos:Concept rdf:about="http://www.cognitiveatlas.org/id/trm_4c8a82eeaa58f"> <dc:identifier>trm_4c8a82eeaa58f</dc:identifier>
		<dc:Title>Cognitive Atlas : Lexicon : Reading (Overt)</dc:Title>
		<dc:Description>RDF output for 'Reading (Overt)'</dc:Description>
		<dc:Type>InteractiveResource</dc:Type>
		<dc:Publisher>Cognitive Atlas</dc:Publisher>
		<dc:Creator>Cognitive Atlas RDF Generator</dc:Creator>
		<dc:Contributor>Brenda Gregory</dc:Contributor>
		<dc:Date>2011-04-26 14:20:27</dc:Date>
		<dc:Format>text/rdf</dc:Format>
		<dc:Language>en</dc:Language>
		<skos:editorialNote>Generated by testgenall.php on Thu Mar 29 10:24:07 PDT 2012.</skos:editorialNote>
		<skos:historyNote>Revision 2: 1 previous definitions.</skos:historyNote>
		<skos:changeNote>See http://www.cognitiveatlas.org/id/trm_4c8a82eeaa58f for complete revision history.</skos:changeNote>
		<skos:scopeNote>http://www.w3.org/2004/02/skos/core#Concept</skos:scopeNote>
		<skos:Note>SKOS properties defined in http://www.w3.org/TR/skos-primer/#secrel</skos:Note>
		<skos:inScheme rdf:resource="http://www.cognitiveatlas.org/tasks/"/>
		<skos:definition>Subjects view words, pseudo-words, Asian characters, phrases, or sentences and read them aloud.</skos:definition>
		<skos:prefLabel>Reading (Overt)</skos:prefLabel>
		<skos:altLabel></skos:altLabel>
		<skos:related rdf:resource="http://www.cognitiveatlas.org/id/trm_4c8a82ba8a538"/>
		<skos:example>Reading (Covert) is related to Reading (Overt)</skos:example>
</skos:Concept><skos:Concept rdf:about="http://www.cognitiveatlas.org/id/trm_4c8a830dec136"> <dc:identifier>trm_4c8a830dec136</dc:identifier>
		<dc:Title>Cognitive Atlas : Lexicon : Recitation/Repetition (Covert)</dc:Title>
		<dc:Description>RDF output for 'Recitation/Repetition (Covert)'</dc:Description>
		<dc:Type>InteractiveResource</dc:Type>
		<dc:Publisher>Cognitive Atlas</dc:Publisher>
		<dc:Creator>Cognitive Atlas RDF Generator</dc:Creator>
		<dc:Contributor>Brenda Gregory</dc:Contributor>
		<dc:Date>2011-04-26 14:20:07</dc:Date>
		<dc:Format>text/rdf</dc:Format>
		<dc:Language>en</dc:Language>
		<skos:editorialNote>Generated by testgenall.php on Thu Mar 29 10:24:07 PDT 2012.</skos:editorialNote>
		<skos:historyNote>Revision 2: 1 previous definitions.</skos:historyNote>
		<skos:changeNote>See http://www.cognitiveatlas.org/id/trm_4c8a830dec136 for complete revision history.</skos:changeNote>
		<skos:scopeNote>http://www.w3.org/2004/02/skos/core#Concept</skos:scopeNote>
		<skos:Note>SKOS properties defined in http://www.w3.org/TR/skos-primer/#secrel</skos:Note>
		<skos:inScheme rdf:resource="http://www.cognitiveatlas.org/tasks/"/>
		<skos:definition>Subjects silently repeat or recite phonemes, words, or well-known text (nursery rhymes, Pledge of Allegiance, months of the year, etc.).</skos:definition>
		<skos:prefLabel>Recitation/Repetition (Covert)</skos:prefLabel>
		<skos:altLabel></skos:altLabel>
		<skos:related rdf:resource="http://www.cognitiveatlas.org/id/trm_4a3fd79d098a6"/>
		<skos:related rdf:resource="http://www.cognitiveatlas.org/id/trm_4a3fd79d098a6"/>
		<skos:related rdf:resource="http://www.cognitiveatlas.org/id/trm_4a3fd79d0ba0d"/>
		<skos:example>articulatory rehearsal is measured by the contrast of areas of activation during task minus baseline trials in the Recitation/Repetition (Covert)</skos:example>
		<skos:example>articulatory rehearsal is measured by the contrast of BOLD activity during task minus baseline trials in the Recitation/Repetition (Covert)</skos:example>
		<skos:example>active maintenance is measured by the contrast of areas of activation during task minus baseline trials in the Recitation/Repetition (Covert)</skos:example>
		<cito:citesForInformation rdf:resource="http://www.cognitiveatlas.org/citation/id/cit_4e0261fcd005a"/>
		<cito:citesForInformation rdf:resource="http://www.cognitiveatlas.org/citation/id/cit_4e0262f1a2d08"/>
</skos:Concept><skos:Concept rdf:about="http://www.cognitiveatlas.org/id/trm_4c8a8329cb8ff"> <dc:identifier>trm_4c8a8329cb8ff</dc:identifier>
		<dc:Title>Cognitive Atlas : Lexicon : Recitation/Repetition (Overt)</dc:Title>
		<dc:Description>RDF output for 'Recitation/Repetition (Overt)'</dc:Description>
		<dc:Type>InteractiveResource</dc:Type>
		<dc:Publisher>Cognitive Atlas</dc:Publisher>
		<dc:Creator>Cognitive Atlas RDF Generator</dc:Creator>
		<dc:Contributor>Brenda Gregory</dc:Contributor>
		<dc:Date>2011-04-26 14:19:47</dc:Date>
		<dc:Format>text/rdf</dc:Format>
		<dc:Language>en</dc:Language>
		<skos:editorialNote>Generated by testgenall.php on Thu Mar 29 10:24:07 PDT 2012.</skos:editorialNote>
		<skos:historyNote>Revision 2: 1 previous definitions.</skos:historyNote>
		<skos:changeNote>See http://www.cognitiveatlas.org/id/trm_4c8a8329cb8ff for complete revision history.</skos:changeNote>
		<skos:scopeNote>http://www.w3.org/2004/02/skos/core#Concept</skos:scopeNote>
		<skos:Note>SKOS properties defined in http://www.w3.org/TR/skos-primer/#secrel</skos:Note>
		<skos:inScheme rdf:resource="http://www.cognitiveatlas.org/tasks/"/>
		<skos:definition>Subjects repeat or recite phonemes, words, or well-known text (nursery rhymes, Pledge of Allegiance, months of the year, etc.) aloud.</skos:definition>
		<skos:prefLabel>Recitation/Repetition (Overt)</skos:prefLabel>
		<skos:altLabel></skos:altLabel>
		<skos:related rdf:resource="http://www.cognitiveatlas.org/id/trm_4a3fd79d0b247"/>
		<skos:related rdf:resource="http://www.cognitiveatlas.org/id/trm_4a3fd79d0ba0d"/>
		<skos:related rdf:resource="http://www.cognitiveatlas.org/id/trm_4a3fd79d098a6"/>
		<skos:related rdf:resource="http://www.cognitiveatlas.org/id/trm_4a3fd79d098a6"/>
		<skos:example>speech production is measured by the contrast of areas of activation during covert minus areas of activation during overt trials in the Recitation/Repetition (Overt)</skos:example>
		<skos:example>active maintenance is measured by the contrast of areas of activation during task minus baseline trials in the Recitation/Repetition (Overt)</skos:example>
		<skos:example>articulatory rehearsal is measured by the contrast of areas of activation during task minus baseline trials in the Recitation/Repetition (Overt)</skos:example>
		<skos:example>articulatory rehearsal is measured by the contrast of BOLD activity during task minus baseline trials in the Recitation/Repetition (Overt)</skos:example>
		<cito:citesForInformation rdf:resource="http://www.cognitiveatlas.org/citation/id/cit_4e026560317f2"/>
		<cito:citesForInformation rdf:resource="http://www.cognitiveatlas.org/citation/id/cit_4e0267038b61b"/>
</skos:Concept><skos:Concept rdf:about="http://www.cognitiveatlas.org/id/trm_4c8a834779883"> <dc:identifier>trm_4c8a834779883</dc:identifier>
		<dc:Title>Cognitive Atlas : Lexicon : Rest</dc:Title>
		<dc:Description>RDF output for 'Rest'</dc:Description>
		<dc:Type>InteractiveResource</dc:Type>
		<dc:Publisher>Cognitive Atlas</dc:Publisher>
		<dc:Creator>Cognitive Atlas RDF Generator</dc:Creator>
		<dc:Contributor>Carinna Torgerson</dc:Contributor>
		<dc:Date>2011-06-15 15:28:40</dc:Date>
		<dc:Format>text/rdf</dc:Format>
		<dc:Language>en</dc:Language>
		<skos:editorialNote>Generated by testgenall.php on Thu Mar 29 10:24:07 PDT 2012.</skos:editorialNote>
		<skos:historyNote>Revision 3: 2 previous definitions.</skos:historyNote>
		<skos:changeNote>See http://www.cognitiveatlas.org/id/trm_4c8a834779883 for complete revision history.</skos:changeNote>
		<skos:scopeNote>http://www.w3.org/2004/02/skos/core#Concept</skos:scopeNote>
		<skos:Note>SKOS properties defined in http://www.w3.org/TR/skos-primer/#secrel</skos:Note>
		<skos:inScheme rdf:resource="http://www.cognitiveatlas.org/tasks/"/>
		<skos:definition>Subjects rest passively with their eyes open or closed. Often used as a baseline for comparison for other tasks.</skos:definition>
		<skos:prefLabel>Rest</skos:prefLabel>
		<skos:altLabel></skos:altLabel>
		<cito:citesForInformation rdf:resource="http://www.cognitiveatlas.org/citation/id/cit_4df932d053971"/>
		<cito:citesForInformation rdf:resource="http://www.cognitiveatlas.org/citation/id/cit_4df9330b7fdea"/>
</skos:Concept><skos:Concept rdf:about="http://www.cognitiveatlas.org/id/trm_4c8a8388de5ea"> <dc:identifier>trm_4c8a8388de5ea</dc:identifier>
		<dc:Title>Cognitive Atlas : Lexicon : Reward Task</dc:Title>
		<dc:Description>RDF output for 'Reward Task'</dc:Description>
		<dc:Type>InteractiveResource</dc:Type>
		<dc:Publisher>Cognitive Atlas</dc:Publisher>
		<dc:Creator>Cognitive Atlas RDF Generator</dc:Creator>
		<dc:Contributor>Carinna Torgerson</dc:Contributor>
		<dc:Date>2011-04-26 14:19:10</dc:Date>
		<dc:Format>text/rdf</dc:Format>
		<dc:Language>en</dc:Language>
		<skos:editorialNote>Generated by testgenall.php on Thu Mar 29 10:24:07 PDT 2012.</skos:editorialNote>
		<skos:historyNote>Revision 2: 1 previous definitions.</skos:historyNote>
		<skos:changeNote>See http://www.cognitiveatlas.org/id/trm_4c8a8388de5ea for complete revision history.</skos:changeNote>
		<skos:scopeNote>http://www.w3.org/2004/02/skos/core#Concept</skos:scopeNote>
		<skos:Note>SKOS properties defined in http://www.w3.org/TR/skos-primer/#secrel</skos:Note>
		<skos:inScheme rdf:resource="http://www.cognitiveatlas.org/tasks/"/>
		<skos:definition>Disambiguation</skos:definition>
		<skos:prefLabel>Reward Task</skos:prefLabel>
		<skos:altLabel></skos:altLabel>
		<skos:related rdf:resource="http://www.cognitiveatlas.org/id/tsk_4a57abb949d4e"/>
		<skos:example>reversal learning task is a narrower synonym of Reward Task</skos:example>
		<cito:citesForInformation rdf:resource="http://www.cognitiveatlas.org/citation/id/cit_4dfa31ffb8d52"/>
		<cito:citesForInformation rdf:resource="http://www.cognitiveatlas.org/citation/id/cit_4dfa327108202"/>
		<cito:citesForInformation rdf:resource="http://www.cognitiveatlas.org/citation/id/cit_4dfa349bebbb4"/>
</skos:Concept><skos:Concept rdf:about="http://www.cognitiveatlas.org/id/trm_4c8a83cac75f5"> <dc:identifier>trm_4c8a83cac75f5</dc:identifier>
		<dc:Title>Cognitive Atlas : Lexicon : Sequence Recall/Learning</dc:Title>
		<dc:Description>RDF output for 'Sequence Recall/Learning'</dc:Description>
		<dc:Type>InteractiveResource</dc:Type>
		<dc:Publisher>Cognitive Atlas</dc:Publisher>
		<dc:Creator>Cognitive Atlas RDF Generator</dc:Creator>
		<dc:Contributor>Brenda Gregory</dc:Contributor>
		<dc:Date>2011-04-26 14:18:50</dc:Date>
		<dc:Format>text/rdf</dc:Format>
		<dc:Language>en</dc:Language>
		<skos:editorialNote>Generated by testgenall.php on Thu Mar 29 10:24:07 PDT 2012.</skos:editorialNote>
		<skos:historyNote>Revision 2: 1 previous definitions.</skos:historyNote>
		<skos:changeNote>See http://www.cognitiveatlas.org/id/trm_4c8a83cac75f5 for complete revision history.</skos:changeNote>
		<skos:scopeNote>http://www.w3.org/2004/02/skos/core#Concept</skos:scopeNote>
		<skos:Note>SKOS properties defined in http://www.w3.org/TR/skos-primer/#secrel</skos:Note>
		<skos:inScheme rdf:resource="http://www.cognitiveatlas.org/tasks/"/>
		<skos:definition>Subjects learn and/or perform a complex sequence of finger tapping, button pressing, pointing/clicking, or various other motor responses.</skos:definition>
		<skos:prefLabel>Sequence Recall/Learning</skos:prefLabel>
		<skos:altLabel></skos:altLabel>
		<skos:related rdf:resource="http://www.cognitiveatlas.org/id/trm_4a3fd79d0a995"/>
		<skos:related rdf:resource="http://www.cognitiveatlas.org/id/trm_4a3fd79d0addc"/>
		<skos:related rdf:resource="http://www.cognitiveatlas.org/id/trm_4a3fd79d0addc"/>
		<skos:example>motor learning is measured by the contrast of accuracy with learning minus accuracy without learning/practice trials in the Sequence Recall/Learning</skos:example>
		<skos:example>procedural memory is measured by the contrast of accuracy with learning minus accuracy without learning/practice trials in the Sequence Recall/Learning</skos:example>
		<skos:example>procedural memory is measured by the contrast of accuracy of participant minus average accuracy of controls trials in the Sequence Recall/Learning</skos:example>
		<cito:citesForInformation rdf:resource="http://www.cognitiveatlas.org/citation/id/cit_4dfa79cfb619e"/>
		<cito:citesForInformation rdf:resource="http://www.cognitiveatlas.org/citation/id/cit_4dfa7a9c86986"/>
		<cito:citesForInformation rdf:resource="http://www.cognitiveatlas.org/citation/id/cit_4dfa7b536c9f3"/>
</skos:Concept><skos:Concept rdf:about="http://www.cognitiveatlas.org/id/trm_4c8a83f27ac55"> <dc:identifier>trm_4c8a83f27ac55</dc:identifier>
		<dc:Title>Cognitive Atlas : Lexicon : Spatial/Location Discrimination</dc:Title>
		<dc:Description>RDF output for 'Spatial/Location Discrimination'</dc:Description>
		<dc:Type>InteractiveResource</dc:Type>
		<dc:Publisher>Cognitive Atlas</dc:Publisher>
		<dc:Creator>Cognitive Atlas RDF Generator</dc:Creator>
		<dc:Contributor>Brenda Gregory</dc:Contributor>
		<dc:Date>2011-04-26 14:18:31</dc:Date>
		<dc:Format>text/rdf</dc:Format>
		<dc:Language>en</dc:Language>
		<skos:editorialNote>Generated by testgenall.php on Thu Mar 29 10:24:07 PDT 2012.</skos:editorialNote>
		<skos:historyNote>Revision 2: 1 previous definitions.</skos:historyNote>
		<skos:changeNote>See http://www.cognitiveatlas.org/id/trm_4c8a83f27ac55 for complete revision history.</skos:changeNote>
		<skos:scopeNote>http://www.w3.org/2004/02/skos/core#Concept</skos:scopeNote>
		<skos:Note>SKOS properties defined in http://www.w3.org/TR/skos-primer/#secrel</skos:Note>
		<skos:inScheme rdf:resource="http://www.cognitiveatlas.org/tasks/"/>
		<skos:definition>Subjects view shapes or other stimuli (letters, pictures, numbers, or arrows) and discriminate according to their location, orientation, or size.</skos:definition>
		<skos:prefLabel>Spatial/Location Discrimination</skos:prefLabel>
		<skos:altLabel></skos:altLabel>
		<skos:related rdf:resource="http://www.cognitiveatlas.org/id/trm_4a3fd79d0b1a6"/>
		<skos:example>spatial ability is measured by the contrast of accuracy of participant minus average accuracy of controls trials in the Spatial/Location Discrimination</skos:example>
		<cito:citesForInformation rdf:resource="http://www.cognitiveatlas.org/citation/id/cit_4e037969ab377"/>
		<cito:citesForInformation rdf:resource="http://www.cognitiveatlas.org/citation/id/cit_4e037a4b6cf79"/>
</skos:Concept><skos:Concept rdf:about="http://www.cognitiveatlas.org/id/trm_4c8a840d6f969"> <dc:identifier>trm_4c8a840d6f969</dc:identifier>
		<dc:Title>Cognitive Atlas : Lexicon : Subjective Emotional Picture Discrimination</dc:Title>
		<dc:Description>RDF output for 'Subjective Emotional Picture Discrimination'</dc:Description>
		<dc:Type>InteractiveResource</dc:Type>
		<dc:Publisher>Cognitive Atlas</dc:Publisher>
		<dc:Creator>Cognitive Atlas RDF Generator</dc:Creator>
		<dc:Contributor>Brenda Gregory</dc:Contributor>
		<dc:Date>2011-04-26 14:18:08</dc:Date>
		<dc:Format>text/rdf</dc:Format>
		<dc:Language>en</dc:Language>
		<skos:editorialNote>Generated by testgenall.php on Thu Mar 29 10:24:07 PDT 2012.</skos:editorialNote>
		<skos:historyNote>Revision 2: 1 previous definitions.</skos:historyNote>
		<skos:changeNote>See http://www.cognitiveatlas.org/id/trm_4c8a840d6f969 for complete revision history.</skos:changeNote>
		<skos:scopeNote>http://www.w3.org/2004/02/skos/core#Concept</skos:scopeNote>
		<skos:Note>SKOS properties defined in http://www.w3.org/TR/skos-primer/#secrel</skos:Note>
		<skos:inScheme rdf:resource="http://www.cognitiveatlas.org/tasks/"/>
		<skos:definition>Subjects view pictures and are instructed to respond to emotional pictures, to indicate which pictures are pleasant/unpleasant or funny/not funny, or rate the valence of emotional pictures.</skos:definition>
		<skos:prefLabel>Subjective Emotional Picture Discrimination</skos:prefLabel>
		<skos:altLabel></skos:altLabel>
		<skos:related rdf:resource="http://www.cognitiveatlas.org/id/trm_4a3fd79d0b65a"/>
		<skos:related rdf:resource="http://www.cognitiveatlas.org/id/tsk_4a57abb949aca"/>
		<skos:example>Subjective Emotional Picture Discrimination is a broader synonym of International Affective Picture System</skos:example>
		<skos:example>emotion perception is measured by the contrast of emotional rating to picture stimuli minus emotional rating to neutral baseline picture trials in the Subjective Emotional Picture Discrimination</skos:example>
		<cito:citesForInformation rdf:resource="http://www.cognitiveatlas.org/citation/id/cit_4dfbd113c54b9"/>
</skos:Concept><skos:Concept rdf:about="http://www.cognitiveatlas.org/id/trm_4c8a842512a33"> <dc:identifier>trm_4c8a842512a33</dc:identifier>
		<dc:Title>Cognitive Atlas : Lexicon : Syntactic Discrimination</dc:Title>
		<dc:Description>RDF output for 'Syntactic Discrimination'</dc:Description>
		<dc:Type>InteractiveResource</dc:Type>
		<dc:Publisher>Cognitive Atlas</dc:Publisher>
		<dc:Creator>Cognitive Atlas RDF Generator</dc:Creator>
		<dc:Contributor>Brenda Gregory</dc:Contributor>
		<dc:Date>2011-04-26 14:17:49</dc:Date>
		<dc:Format>text/rdf</dc:Format>
		<dc:Language>en</dc:Language>
		<skos:editorialNote>Generated by testgenall.php on Thu Mar 29 10:24:07 PDT 2012.</skos:editorialNote>
		<skos:historyNote>Revision 2: 1 previous definitions.</skos:historyNote>
		<skos:changeNote>See http://www.cognitiveatlas.org/id/trm_4c8a842512a33 for complete revision history.</skos:changeNote>
		<skos:scopeNote>http://www.w3.org/2004/02/skos/core#Concept</skos:scopeNote>
		<skos:Note>SKOS properties defined in http://www.w3.org/TR/skos-primer/#secrel</skos:Note>
		<skos:inScheme rdf:resource="http://www.cognitiveatlas.org/tasks/"/>
		<skos:definition>Subjects viewed grammatically correct and incorrect sentences and discriminate according to their grammar.  This class also includes morphosyntactic tasks such as gender discrimination of words.</skos:definition>
		<skos:prefLabel>Syntactic Discrimination</skos:prefLabel>
		<skos:altLabel></skos:altLabel>
		<skos:related rdf:resource="http://www.cognitiveatlas.org/id/trm_4a3fd79d0b340"/>
		<skos:related rdf:resource="http://www.cognitiveatlas.org/id/trm_4a3fd79d0b37a"/>
		<skos:related rdf:resource="http://www.cognitiveatlas.org/id/trm_4a3fd79d0b37a"/>
		<skos:related rdf:resource="http://www.cognitiveatlas.org/id/tsk_4a57abb949e7c"/>
		<skos:example>Syntactic Discrimination is related to syntactic acceptability judgement task</skos:example>
		<skos:example>syntactic parsing is measured by the contrast of accuracy of participant minus average accuracy of controls trials in the Syntactic Discrimination</skos:example>
		<skos:example>text comprehension is measured by the contrast of accuracy of participant minus average accuracy of controls trials in the Syntactic Discrimination</skos:example>
		<skos:example>text comprehension is measured by the contrast of response time to implausible sentences minus response time to plausible sentences trials in the Syntactic Discrimination</skos:example>
		<cito:citesForInformation rdf:resource="http://www.cognitiveatlas.org/citation/id/cit_4dff7f48ced10"/>
		<cito:citesForInformation rdf:resource="http://www.cognitiveatlas.org/citation/id/cit_4dff7f62138b4"/>
</skos:Concept><skos:Concept rdf:about="http://www.cognitiveatlas.org/id/trm_4c8a843d8d352"> <dc:identifier>trm_4c8a843d8d352</dc:identifier>
		<dc:Title>Cognitive Atlas : Lexicon : Tactile Monitor/Discrimination</dc:Title>
		<dc:Description>RDF output for 'Tactile Monitor/Discrimination'</dc:Description>
		<dc:Type>InteractiveResource</dc:Type>
		<dc:Publisher>Cognitive Atlas</dc:Publisher>
		<dc:Creator>Cognitive Atlas RDF Generator</dc:Creator>
		<dc:Contributor>Brenda Gregory</dc:Contributor>
		<dc:Date>2011-04-26 14:17:27</dc:Date>
		<dc:Format>text/rdf</dc:Format>
		<dc:Language>en</dc:Language>
		<skos:editorialNote>Generated by testgenall.php on Thu Mar 29 10:24:07 PDT 2012.</skos:editorialNote>
		<skos:historyNote>Revision 2: 1 previous definitions.</skos:historyNote>
		<skos:changeNote>See http://www.cognitiveatlas.org/id/trm_4c8a843d8d352 for complete revision history.</skos:changeNote>
		<skos:scopeNote>http://www.w3.org/2004/02/skos/core#Concept</skos:scopeNote>
		<skos:Note>SKOS properties defined in http://www.w3.org/TR/skos-primer/#secrel</skos:Note>
		<skos:inScheme rdf:resource="http://www.cognitiveatlas.org/tasks/"/>
		<skos:definition>Subjects experience tactile/somatosensory stimulation and are asked to attend passively or discriminate according to some feature (shape, texture, same/different, frequency of presentation,  etc.)  Also includes: subjects are presented with 3-dimensional objects and are asked to manipulate them in their hands and probe their features.</skos:definition>
		<skos:prefLabel>Tactile Monitor/Discrimination</skos:prefLabel>
		<skos:altLabel></skos:altLabel>
		<skos:related rdf:resource="http://www.cognitiveatlas.org/id/trm_4a3fd79d0a61f"/>
		<skos:related rdf:resource="http://www.cognitiveatlas.org/id/trm_4a3fd79d0b16c"/>
		<skos:related rdf:resource="http://www.cognitiveatlas.org/id/trm_4c8a84afdd863"/>
		<skos:example>inhibition of return is measured by the contrast of response time to second stimulus minus response time to first stimulus trials in the Tactile Monitor/Discrimination</skos:example>
		<skos:example> is measured by Tactile Monitor/Discrimination</skos:example>
		<skos:example>Vibrotactile Monitor/Discrimination is related to Tactile Monitor/Discrimination</skos:example>
		<cito:citesForInformation rdf:resource="http://www.cognitiveatlas.org/citation/id/cit_4dff846ab4ee4"/>
		<cito:citesForInformation rdf:resource="http://www.cognitiveatlas.org/citation/id/cit_4dff84c800f7b"/>
</skos:Concept><skos:Concept rdf:about="http://www.cognitiveatlas.org/id/trm_4c8a8467304e2"> <dc:identifier>trm_4c8a8467304e2</dc:identifier>
		<dc:Title>Cognitive Atlas : Lexicon : Theory of Mind Task</dc:Title>
		<dc:Description>RDF output for 'Theory of Mind Task'</dc:Description>
		<dc:Type>InteractiveResource</dc:Type>
		<dc:Publisher>Cognitive Atlas</dc:Publisher>
		<dc:Creator>Cognitive Atlas RDF Generator</dc:Creator>
		<dc:Contributor>Russ Poldrack</dc:Contributor>
		<dc:Date>2012-01-28 12:09:56</dc:Date>
		<dc:Format>text/rdf</dc:Format>
		<dc:Language>en</dc:Language>
		<skos:editorialNote>Generated by testgenall.php on Thu Mar 29 10:24:07 PDT 2012.</skos:editorialNote>
		<skos:historyNote>Revision 3: 2 previous definitions.</skos:historyNote>
		<skos:changeNote>See http://www.cognitiveatlas.org/id/trm_4c8a8467304e2 for complete revision history.</skos:changeNote>
		<skos:scopeNote>http://www.w3.org/2004/02/skos/core#Concept</skos:scopeNote>
		<skos:Note>SKOS properties defined in http://www.w3.org/TR/skos-primer/#secrel</skos:Note>
		<skos:inScheme rdf:resource="http://www.cognitiveatlas.org/tasks/"/>
		<skos:definition>Subjects are asked to perform a task involving the understanding of another&#39;s personal beliefs and feelings or forming hypotheses regarding the mental states of others.</skos:definition>
		<skos:prefLabel>Theory of Mind Task</skos:prefLabel>
		<skos:altLabel>TOM task</skos:altLabel>
		<skos:related rdf:resource="http://www.cognitiveatlas.org/id/trm_4a3fd79d0b392"/>
		<skos:related rdf:resource="http://www.cognitiveatlas.org/id/trm_4a3fd79d0b67d"/>
		<skos:related rdf:resource="http://www.cognitiveatlas.org/id/trm_4a3fd79d0a1a2"/>
		<skos:example>theory of mind is measured by the contrast of average score minus participant&#39;s score trials in the Theory of Mind Task</skos:example>
		<skos:example>empathy is measured by the contrast of average score minus participant&#39;s score trials in the Theory of Mind Task</skos:example>
		<skos:example>emotional intelligence is measured by the contrast of average score minus participant&#39;s score trials in the Theory of Mind Task</skos:example>
		<cito:citesForInformation rdf:resource="http://www.cognitiveatlas.org/citation/id/cit_4dffaad9dbd99"/>
		<cito:citesForInformation rdf:resource="http://www.cognitiveatlas.org/citation/id/cit_4dffac4b23cf5"/>
</skos:Concept><skos:Concept rdf:about="http://www.cognitiveatlas.org/id/trm_4c8a84825c4e4"> <dc:identifier>trm_4c8a84825c4e4</dc:identifier>
		<dc:Title>Cognitive Atlas : Lexicon : Tone Monitor/Discrimination</dc:Title>
		<dc:Description>RDF output for 'Tone Monitor/Discrimination'</dc:Description>
		<dc:Type>InteractiveResource</dc:Type>
		<dc:Publisher>Cognitive Atlas</dc:Publisher>
		<dc:Creator>Cognitive Atlas RDF Generator</dc:Creator>
		<dc:Contributor>Russ Poldrack</dc:Contributor>
		<dc:Date>2012-01-28 08:07:56</dc:Date>
		<dc:Format>text/rdf</dc:Format>
		<dc:Language>en</dc:Language>
		<skos:editorialNote>Generated by testgenall.php on Thu Mar 29 10:24:07 PDT 2012.</skos:editorialNote>
		<skos:historyNote>Revision 3: 2 previous definitions.</skos:historyNote>
		<skos:changeNote>See http://www.cognitiveatlas.org/id/trm_4c8a84825c4e4 for complete revision history.</skos:changeNote>
		<skos:scopeNote>http://www.w3.org/2004/02/skos/core#Concept</skos:scopeNote>
		<skos:Note>SKOS properties defined in http://www.w3.org/TR/skos-primer/#secrel</skos:Note>
		<skos:inScheme rdf:resource="http://www.cognitiveatlas.org/tasks/"/>
		<skos:definition>Subjects are presented with tones and are instructed to listen to them passively (also coded as Passive Listening) or discriminate according to their order, timing, pitch, frequency, or amplitude.</skos:definition>
		<skos:prefLabel>Tone Monitor/Discrimination</skos:prefLabel>
		<skos:altLabel>tone discrimination task, tone monitoring task</skos:altLabel>
		<skos:related rdf:resource="http://www.cognitiveatlas.org/id/trm_4a3fd79d09713"/>
		<skos:related rdf:resource="http://www.cognitiveatlas.org/id/trm_4c89924414c69"/>
		<skos:related rdf:resource="http://www.cognitiveatlas.org/id/trm_4c8991fadfe01"/>
		<skos:example>Tone Monitor/Discrimination is an exact synonym of Pitch Monitor/Discrimination</skos:example>
		<skos:example>Tone Monitor/Discrimination is related to Passive Listening</skos:example>
		<skos:example>acoustic phonetic processing is measured by the contrast of accuracy of participant minus average accuracy of controls trials in the Tone Monitor/Discrimination</skos:example>
		<cito:citesForInformation rdf:resource="http://www.cognitiveatlas.org/citation/id/cit_4dffb636bfd17"/>
		<cito:citesForInformation rdf:resource="http://www.cognitiveatlas.org/citation/id/cit_4dffb6f23f50f"/>
</skos:Concept><skos:Concept rdf:about="http://www.cognitiveatlas.org/id/trm_4c8a84afdd863"> <dc:identifier>trm_4c8a84afdd863</dc:identifier>
		<dc:Title>Cognitive Atlas : Lexicon : Vibrotactile Monitor/Discrimination</dc:Title>
		<dc:Description>RDF output for 'Vibrotactile Monitor/Discrimination'</dc:Description>
		<dc:Type>InteractiveResource</dc:Type>
		<dc:Publisher>Cognitive Atlas</dc:Publisher>
		<dc:Creator>Cognitive Atlas RDF Generator</dc:Creator>
		<dc:Contributor>Brenda Gregory</dc:Contributor>
		<dc:Date>2011-04-26 14:16:12</dc:Date>
		<dc:Format>text/rdf</dc:Format>
		<dc:Language>en</dc:Language>
		<skos:editorialNote>Generated by testgenall.php on Thu Mar 29 10:24:07 PDT 2012.</skos:editorialNote>
		<skos:historyNote>Revision 2: 1 previous definitions.</skos:historyNote>
		<skos:changeNote>See http://www.cognitiveatlas.org/id/trm_4c8a84afdd863 for complete revision history.</skos:changeNote>
		<skos:scopeNote>http://www.w3.org/2004/02/skos/core#Concept</skos:scopeNote>
		<skos:Note>SKOS properties defined in http://www.w3.org/TR/skos-primer/#secrel</skos:Note>
		<skos:inScheme rdf:resource="http://www.cognitiveatlas.org/tasks/"/>
		<skos:definition>Subjects experience vibrotactile stimulation to the hand, finger, arm, toe, or lip.</skos:definition>
		<skos:prefLabel>Vibrotactile Monitor/Discrimination</skos:prefLabel>
		<skos:altLabel></skos:altLabel>
		<skos:related rdf:resource="http://www.cognitiveatlas.org/id/trm_4a3fd79d0b16c"/>
		<skos:related rdf:resource="http://www.cognitiveatlas.org/id/trm_4a3fd79d0b1a6"/>
		<skos:related rdf:resource="http://www.cognitiveatlas.org/id/trm_4c8a843d8d352"/>
		<skos:example>Vibrotactile Monitor/Discrimination is related to Tactile Monitor/Discrimination</skos:example>
		<skos:example> is measured by Vibrotactile Monitor/Discrimination</skos:example>
		<skos:example>spatial ability is measured by the contrast of accuracy of participant minus average accuracy of controls trials in the Vibrotactile Monitor/Discrimination</skos:example>
		<cito:citesForInformation rdf:resource="http://www.cognitiveatlas.org/citation/id/cit_4e00c6e49f184"/>
		<cito:citesForInformation rdf:resource="http://www.cognitiveatlas.org/citation/id/cit_4e00c964c3a26"/>
		<cito:citesForInformation rdf:resource="http://www.cognitiveatlas.org/citation/id/cit_4e00cb18c7ec1"/>
</skos:Concept><skos:Concept rdf:about="http://www.cognitiveatlas.org/id/trm_4c8a84d4c4157"> <dc:identifier>trm_4c8a84d4c4157</dc:identifier>
		<dc:Title>Cognitive Atlas : Lexicon : Video Games</dc:Title>
		<dc:Description>RDF output for 'Video Games'</dc:Description>
		<dc:Type>InteractiveResource</dc:Type>
		<dc:Publisher>Cognitive Atlas</dc:Publisher>
		<dc:Creator>Cognitive Atlas RDF Generator</dc:Creator>
		<dc:Contributor>Brenda Gregory</dc:Contributor>
		<dc:Date>2011-04-26 14:15:53</dc:Date>
		<dc:Format>text/rdf</dc:Format>
		<dc:Language>en</dc:Language>
		<skos:editorialNote>Generated by testgenall.php on Thu Mar 29 10:24:07 PDT 2012.</skos:editorialNote>
		<skos:historyNote>Revision 2: 1 previous definitions.</skos:historyNote>
		<skos:changeNote>See http://www.cognitiveatlas.org/id/trm_4c8a84d4c4157 for complete revision history.</skos:changeNote>
		<skos:scopeNote>http://www.w3.org/2004/02/skos/core#Concept</skos:scopeNote>
		<skos:Note>SKOS properties defined in http://www.w3.org/TR/skos-primer/#secrel</skos:Note>
		<skos:inScheme rdf:resource="http://www.cognitiveatlas.org/tasks/"/>
		<skos:definition>Subjects play video games.</skos:definition>
		<skos:prefLabel>Video Games</skos:prefLabel>
		<skos:altLabel></skos:altLabel>
		<cito:citesForInformation rdf:resource="http://www.cognitiveatlas.org/citation/id/cit_4e00d0212dd04"/>
		<cito:citesForInformation rdf:resource="http://www.cognitiveatlas.org/citation/id/cit_4e00d17e95e3f"/>
		<cito:citesForInformation rdf:resource="http://www.cognitiveatlas.org/citation/id/cit_4e00d5ce35eca"/>
</skos:Concept><skos:Concept rdf:about="http://www.cognitiveatlas.org/id/trm_4c8a84f20dde2"> <dc:identifier>trm_4c8a84f20dde2</dc:identifier>
		<dc:Title>Cognitive Atlas : Lexicon : Visual Distractor/Visual Attention</dc:Title>
		<dc:Description>RDF output for 'Visual Distractor/Visual Attention'</dc:Description>
		<dc:Type>InteractiveResource</dc:Type>
		<dc:Publisher>Cognitive Atlas</dc:Publisher>
		<dc:Creator>Cognitive Atlas RDF Generator</dc:Creator>
		<dc:Contributor>Brenda Gregory</dc:Contributor>
		<dc:Date>2011-04-26 14:14:54</dc:Date>
		<dc:Format>text/rdf</dc:Format>
		<dc:Language>en</dc:Language>
		<skos:editorialNote>Generated by testgenall.php on Thu Mar 29 10:24:07 PDT 2012.</skos:editorialNote>
		<skos:historyNote>Revision 2: 1 previous definitions.</skos:historyNote>
		<skos:changeNote>See http://www.cognitiveatlas.org/id/trm_4c8a84f20dde2 for complete revision history.</skos:changeNote>
		<skos:scopeNote>http://www.w3.org/2004/02/skos/core#Concept</skos:scopeNote>
		<skos:Note>SKOS properties defined in http://www.w3.org/TR/skos-primer/#secrel</skos:Note>
		<skos:inScheme rdf:resource="http://www.cognitiveatlas.org/tasks/"/>
		<skos:definition>This category is a catch-all for visuoattention paradigms.  Examples include:  subjects press a button when a visual target (letters, bars, circles, asterisks, LEDs, etc) appears; subjects detect changes in luminance, shape, or color of visual stimuli; subjects fixate on a central stimuli while ignoring peripheral distractors.  Also includes cued, attention shift, and divided attention paradigms.</skos:definition>
		<skos:prefLabel>Visual Distractor/Visual Attention</skos:prefLabel>
		<skos:altLabel></skos:altLabel>
		<skos:related rdf:resource="http://www.cognitiveatlas.org/id/trm_4a3fd79d0b46f"/>
		<skos:related rdf:resource="http://www.cognitiveatlas.org/id/trm_4a3fd79d0b4d8"/>
		<skos:related rdf:resource="http://www.cognitiveatlas.org/id/trm_4a3fd79d0b5fb"/>
		<skos:related rdf:resource="http://www.cognitiveatlas.org/id/trm_4a3fd79d0b4cd"/>
		<skos:example>visual attention is measured by the contrast of reaction time after some manipulation minus reaction time at baseline trials in the Visual Distractor/Visual Attention</skos:example>
		<skos:example>visual working memory is measured by the contrast of d&#39; (difference between correct identifications and false alarms) trials in the Visual Distractor/Visual Attention</skos:example>
		<skos:example>attention shifting is measured by the contrast of reaction time after some manipulation minus reaction time at baseline trials in the Visual Distractor/Visual Attention</skos:example>
		<skos:example>visual search is measured by the contrast of path of eye movements trials in the Visual Distractor/Visual Attention</skos:example>
		<cito:citesForInformation rdf:resource="http://www.cognitiveatlas.org/citation/id/cit_4e00e71b3a52b"/>
		<cito:citesForInformation rdf:resource="http://www.cognitiveatlas.org/citation/id/cit_4e00fc527b219"/>
		<cito:citesForInformation rdf:resource="http://www.cognitiveatlas.org/citation/id/cit_4e00fe06b6513"/>
</skos:Concept><skos:Concept rdf:about="http://www.cognitiveatlas.org/id/trm_4c8a85534241d"> <dc:identifier>trm_4c8a85534241d</dc:identifier>
		<dc:Title>Cognitive Atlas : Lexicon : Visual Pursuit/Tracking</dc:Title>
		<dc:Description>RDF output for 'Visual Pursuit/Tracking'</dc:Description>
		<dc:Type>InteractiveResource</dc:Type>
		<dc:Publisher>Cognitive Atlas</dc:Publisher>
		<dc:Creator>Cognitive Atlas RDF Generator</dc:Creator>
		<dc:Contributor>Russ Poldrack</dc:Contributor>
		<dc:Date>2012-01-28 07:50:54</dc:Date>
		<dc:Format>text/rdf</dc:Format>
		<dc:Language>en</dc:Language>
		<skos:editorialNote>Generated by testgenall.php on Thu Mar 29 10:24:07 PDT 2012.</skos:editorialNote>
		<skos:historyNote>Revision 3: 2 previous definitions.</skos:historyNote>
		<skos:changeNote>See http://www.cognitiveatlas.org/id/trm_4c8a85534241d for complete revision history.</skos:changeNote>
		<skos:scopeNote>http://www.w3.org/2004/02/skos/core#Concept</skos:scopeNote>
		<skos:Note>SKOS properties defined in http://www.w3.org/TR/skos-primer/#secrel</skos:Note>
		<skos:inScheme rdf:resource="http://www.cognitiveatlas.org/tasks/"/>
		<skos:definition>Subjects view a moving target(s) and track its movement across the screen.  Frequently, stimuli are moving dots.</skos:definition>
		<skos:prefLabel>Visual Pursuit/Tracking</skos:prefLabel>
		<skos:altLabel>tracking task</skos:altLabel>
		<skos:related rdf:resource="http://www.cognitiveatlas.org/id/trm_4a3fd79d0b4cd"/>
		<skos:related rdf:resource="http://www.cognitiveatlas.org/id/trm_4a3fd79d0b46f"/>
		<skos:related rdf:resource="http://www.cognitiveatlas.org/id/trm_4a3fd79d0b043"/>
		<skos:example>visual search is measured by the contrast of path of eye movements trials in the Visual Pursuit/Tracking</skos:example>
		<skos:example>visual attention is measured by the contrast of d&#39; (difference between correct identifications and false alarms) trials in the Visual Pursuit/Tracking</skos:example>
		<skos:example>selective attention is measured by the contrast of path of eye movements trials in the Visual Pursuit/Tracking</skos:example>
		<cito:citesForInformation rdf:resource="http://www.cognitiveatlas.org/citation/id/cit_4e0101d4ab56d"/>
		<cito:citesForInformation rdf:resource="http://www.cognitiveatlas.org/citation/id/cit_4e0103182e4c8"/>
</skos:Concept><skos:Concept rdf:about="http://www.cognitiveatlas.org/id/trm_4c8a8575d1e55"> <dc:identifier>trm_4c8a8575d1e55</dc:identifier>
		<dc:Title>Cognitive Atlas : Lexicon : Whistling</dc:Title>
		<dc:Description>RDF output for 'Whistling'</dc:Description>
		<dc:Type>InteractiveResource</dc:Type>
		<dc:Publisher>Cognitive Atlas</dc:Publisher>
		<dc:Creator>Cognitive Atlas RDF Generator</dc:Creator>
		<dc:Contributor>Brenda Gregory</dc:Contributor>
		<dc:Date>2011-04-26 14:14:09</dc:Date>
		<dc:Format>text/rdf</dc:Format>
		<dc:Language>en</dc:Language>
		<skos:editorialNote>Generated by testgenall.php on Thu Mar 29 10:24:07 PDT 2012.</skos:editorialNote>
		<skos:historyNote>Revision 2: 1 previous definitions.</skos:historyNote>
		<skos:changeNote>See http://www.cognitiveatlas.org/id/trm_4c8a8575d1e55 for complete revision history.</skos:changeNote>
		<skos:scopeNote>http://www.w3.org/2004/02/skos/core#Concept</skos:scopeNote>
		<skos:Note>SKOS properties defined in http://www.w3.org/TR/skos-primer/#secrel</skos:Note>
		<skos:inScheme rdf:resource="http://www.cognitiveatlas.org/tasks/"/>
		<skos:definition>Subjects whistle.</skos:definition>
		<skos:prefLabel>Whistling</skos:prefLabel>
		<skos:altLabel></skos:altLabel>
		<skos:related rdf:resource="http://www.cognitiveatlas.org/id/trm_4a3fd79d0a97e"/>
		<skos:example>motor execution is measured by the contrast of response time of subject minus response time of controls trials in the Whistling</skos:example>
		<cito:citesForInformation rdf:resource="http://www.cognitiveatlas.org/citation/id/cit_4e017ad71f8a4"/>
</skos:Concept><skos:Concept rdf:about="http://www.cognitiveatlas.org/id/trm_4c8a858da803d"> <dc:identifier>trm_4c8a858da803d</dc:identifier>
		<dc:Title>Cognitive Atlas : Lexicon : Word Stem Completion (Covert)</dc:Title>
		<dc:Description>RDF output for 'Word Stem Completion (Covert)'</dc:Description>
		<dc:Type>InteractiveResource</dc:Type>
		<dc:Publisher>Cognitive Atlas</dc:Publisher>
		<dc:Creator>Cognitive Atlas RDF Generator</dc:Creator>
		<dc:Contributor>Brenda Gregory</dc:Contributor>
		<dc:Date>2011-04-26 14:13:49</dc:Date>
		<dc:Format>text/rdf</dc:Format>
		<dc:Language>en</dc:Language>
		<skos:editorialNote>Generated by testgenall.php on Thu Mar 29 10:24:07 PDT 2012.</skos:editorialNote>
		<skos:historyNote>Revision 2: 1 previous definitions.</skos:historyNote>
		<skos:changeNote>See http://www.cognitiveatlas.org/id/trm_4c8a858da803d for complete revision history.</skos:changeNote>
		<skos:scopeNote>http://www.w3.org/2004/02/skos/core#Concept</skos:scopeNote>
		<skos:Note>SKOS properties defined in http://www.w3.org/TR/skos-primer/#secrel</skos:Note>
		<skos:inScheme rdf:resource="http://www.cognitiveatlas.org/tasks/"/>
		<skos:definition>Subjects view word stems and silently generate a word that completes the stem.</skos:definition>
		<skos:prefLabel>Word Stem Completion (Covert)</skos:prefLabel>
		<skos:altLabel></skos:altLabel>
		<skos:related rdf:resource="http://www.cognitiveatlas.org/id/trm_4a3fd79d0b80f"/>
		<skos:related rdf:resource="http://www.cognitiveatlas.org/id/trm_4a3fd79d0b44c"/>
		<skos:related rdf:resource="http://www.cognitiveatlas.org/id/trm_4c8a85a4564b2"/>
		<skos:example>lexical access is measured by the contrast of areas of activation during task minus baseline trials in the Word Stem Completion (Covert)</skos:example>
		<skos:example>verbal fluency is measured by the contrast of ERP strength minus baseline trials in the Word Stem Completion (Covert)</skos:example>
		<skos:example>Word Stem Completion (Overt) is related to Word Stem Completion (Covert)</skos:example>
		<cito:citesForInformation rdf:resource="http://www.cognitiveatlas.org/citation/id/cit_4e0243238bcb6"/>
		<cito:citesForInformation rdf:resource="http://www.cognitiveatlas.org/citation/id/cit_4e0244825eaa9"/>
		<cito:citesForInformation rdf:resource="http://www.cognitiveatlas.org/citation/id/cit_4e02541b3f03c"/>
</skos:Concept><skos:Concept rdf:about="http://www.cognitiveatlas.org/id/trm_4c8a85a4564b2"> <dc:identifier>trm_4c8a85a4564b2</dc:identifier>
		<dc:Title>Cognitive Atlas : Lexicon : Word Stem Completion (Overt)</dc:Title>
		<dc:Description>RDF output for 'Word Stem Completion (Overt)'</dc:Description>
		<dc:Type>InteractiveResource</dc:Type>
		<dc:Publisher>Cognitive Atlas</dc:Publisher>
		<dc:Creator>Cognitive Atlas RDF Generator</dc:Creator>
		<dc:Contributor>Russ Poldrack</dc:Contributor>
		<dc:Date>2012-01-28 12:07:05</dc:Date>
		<dc:Format>text/rdf</dc:Format>
		<dc:Language>en</dc:Language>
		<skos:editorialNote>Generated by testgenall.php on Thu Mar 29 10:24:07 PDT 2012.</skos:editorialNote>
		<skos:historyNote>Revision 3: 2 previous definitions.</skos:historyNote>
		<skos:changeNote>See http://www.cognitiveatlas.org/id/trm_4c8a85a4564b2 for complete revision history.</skos:changeNote>
		<skos:scopeNote>http://www.w3.org/2004/02/skos/core#Concept</skos:scopeNote>
		<skos:Note>SKOS properties defined in http://www.w3.org/TR/skos-primer/#secrel</skos:Note>
		<skos:inScheme rdf:resource="http://www.cognitiveatlas.org/tasks/"/>
		<skos:definition>Subjects view word stems and overtly generate a word that completes the stem.</skos:definition>
		<skos:prefLabel>Word Stem Completion (Overt)</skos:prefLabel>
		<skos:altLabel>word stem completion task</skos:altLabel>
		<skos:related rdf:resource="http://www.cognitiveatlas.org/id/trm_4a3fd79d0b44c"/>
		<skos:related rdf:resource="http://www.cognitiveatlas.org/id/trm_4a3fd79d0b80f"/>
		<skos:related rdf:resource="http://www.cognitiveatlas.org/id/trm_4a3fd79d0b247"/>
		<skos:related rdf:resource="http://www.cognitiveatlas.org/id/trm_4c8a858da803d"/>
		<skos:example>Word Stem Completion (Overt) is related to Word Stem Completion (Covert)</skos:example>
		<skos:example>verbal fluency is measured by the contrast of ERP strength minus baseline trials in the Word Stem Completion (Overt)</skos:example>
		<skos:example>lexical access is measured by the contrast of areas of activation during covert minus areas of activation during overt trials in the Word Stem Completion (Overt)</skos:example>
		<skos:example>speech production is measured by the contrast of areas of activation during covert minus areas of activation during overt trials in the Word Stem Completion (Overt)</skos:example>
		<cito:citesForInformation rdf:resource="http://www.cognitiveatlas.org/citation/id/cit_4e02524f9af58"/>
		<cito:citesForInformation rdf:resource="http://www.cognitiveatlas.org/citation/id/cit_4e0253b199160"/>
		<cito:citesForInformation rdf:resource="http://www.cognitiveatlas.org/citation/id/cit_4e02541b3f03c"/>
</skos:Concept><skos:Concept rdf:about="http://www.cognitiveatlas.org/id/trm_4c8a85c5c75eb"> <dc:identifier>trm_4c8a85c5c75eb</dc:identifier>
		<dc:Title>Cognitive Atlas : Lexicon : Writing Task</dc:Title>
		<dc:Description>RDF output for 'Writing Task'</dc:Description>
		<dc:Type>InteractiveResource</dc:Type>
		<dc:Publisher>Cognitive Atlas</dc:Publisher>
		<dc:Creator>Cognitive Atlas RDF Generator</dc:Creator>
		<dc:Contributor>Brenda Gregory</dc:Contributor>
		<dc:Date>2011-04-19 13:56:38</dc:Date>
		<dc:Format>text/rdf</dc:Format>
		<dc:Language>en</dc:Language>
		<skos:editorialNote>Generated by testgenall.php on Thu Mar 29 10:24:07 PDT 2012.</skos:editorialNote>
		<skos:historyNote>Revision 2: 1 previous definitions.</skos:historyNote>
		<skos:changeNote>See http://www.cognitiveatlas.org/id/trm_4c8a85c5c75eb for complete revision history.</skos:changeNote>
		<skos:scopeNote>http://www.w3.org/2004/02/skos/core#Concept</skos:scopeNote>
		<skos:Note>SKOS properties defined in http://www.w3.org/TR/skos-primer/#secrel</skos:Note>
		<skos:inScheme rdf:resource="http://www.cognitiveatlas.org/tasks/"/>
		<skos:definition>Subjects write letters or words with a pen, stylus, or their finger.</skos:definition>
		<skos:prefLabel>Writing Task</skos:prefLabel>
		<skos:altLabel></skos:altLabel>
		<skos:related rdf:resource="http://www.cognitiveatlas.org/id/trm_4a3fd79d0b2b4"/>
		<skos:related rdf:resource="http://www.cognitiveatlas.org/id/trm_4a3fd79d0a972"/>
		<skos:related rdf:resource="http://www.cognitiveatlas.org/id/trm_4a3fd79d0a972"/>
		<skos:related rdf:resource="http://www.cognitiveatlas.org/id/trm_4a3fd79d0a7d4"/>
		<skos:example>sublexical route is measured by the contrast of accuracy of participant minus average accuracy of controls trials in the Writing Task</skos:example>
		<skos:example>motor control is measured by the contrast of pressure exerted by participant minus average pressure trials in the Writing Task</skos:example>
		<skos:example>motor control is measured by the contrast of accuracy of participant minus average accuracy of controls trials in the Writing Task</skos:example>
		<skos:example>lexical encoding is measured by the contrast of accuracy of participant minus average accuracy of controls trials in the Writing Task</skos:example>
		<cito:citesForInformation rdf:resource="http://www.cognitiveatlas.org/citation/id/cit_4e0259989a9cd"/>
		<cito:citesForInformation rdf:resource="http://www.cognitiveatlas.org/citation/id/cit_4e025b0623ef1"/>
		<cito:citesForInformation rdf:resource="http://www.cognitiveatlas.org/citation/id/cit_4e025d3fa039f"/>
</skos:Concept><skos:Concept rdf:about="http://www.cognitiveatlas.org/id/trm_4cacee4a1d875"> <dc:identifier>trm_4cacee4a1d875</dc:identifier>
		<dc:Title>Cognitive Atlas : Lexicon : Mixed gambles task</dc:Title>
		<dc:Description>RDF output for 'Mixed gambles task'</dc:Description>
		<dc:Type>InteractiveResource</dc:Type>
		<dc:Publisher>Cognitive Atlas</dc:Publisher>
		<dc:Creator>Cognitive Atlas RDF Generator</dc:Creator>
		<dc:Contributor>Russ Poldrack</dc:Contributor>
		<dc:Date>2010-10-06 14:46:50</dc:Date>
		<dc:Format>text/rdf</dc:Format>
		<dc:Language>en</dc:Language>
		<skos:editorialNote>Generated by testgenall.php on Thu Mar 29 10:24:07 PDT 2012.</skos:editorialNote>
		<skos:historyNote>No previous definition revisions.</skos:historyNote>
		<skos:changeNote>This is the first and only definition provided.</skos:changeNote>
		<skos:scopeNote>http://www.w3.org/2004/02/skos/core#Concept</skos:scopeNote>
		<skos:Note>SKOS properties defined in http://www.w3.org/TR/skos-primer/#secrel</skos:Note>
		<skos:inScheme rdf:resource="http://www.cognitiveatlas.org/tasks/"/>
		<skos:definition>Subjects are presented with gambles in which they have a 50% chance of gaining some amount of money and a 50% chance of losing some other amount of money.  The subject decides whether or not they would accept the gamble.  The amount of the potential gain and loss are varied across trials.  Gambles are not resolved during performance of the task; after the end of the task, some gambles are chosen at random and played for real money if they were accepted. </skos:definition>
		<skos:prefLabel>Mixed gambles task</skos:prefLabel>
		<skos:altLabel></skos:altLabel>
		<skos:related rdf:resource="http://www.cognitiveatlas.org/id/trm_4a3fd79d0b64e"/>
		<skos:related rdf:resource="http://www.cognitiveatlas.org/id/trm_4a3fd79d09e07"/>
		<skos:example>risk seeking is measured by the contrast of number of choices with greater chance of loss than gain minus number of choices with greater chance of gain than loss trials in the Mixed gambles task</skos:example>
		<skos:example>conditional reasoning is measured by the contrast of Loss aversion trials in the Mixed gambles task</skos:example>
		<cito:citesForInformation rdf:resource="http://www.cognitiveatlas.org/citation/id/cit_4cacee5971d20"/>
		<cito:citesForInformation rdf:resource="http://www.cognitiveatlas.org/citation/id/cit_4df293f690a9a"/>
		<cito:citesForInformation rdf:resource="http://www.cognitiveatlas.org/citation/id/cit_4e9c8838b529c"/>
</skos:Concept><skos:Concept rdf:about="http://www.cognitiveatlas.org/id/trm_4cacf22a22d80"> <dc:identifier>trm_4cacf22a22d80</dc:identifier>
		<dc:Title>Cognitive Atlas : Lexicon : Probabilistic classification task</dc:Title>
		<dc:Description>RDF output for 'Probabilistic classification task'</dc:Description>
		<dc:Type>InteractiveResource</dc:Type>
		<dc:Publisher>Cognitive Atlas</dc:Publisher>
		<dc:Creator>Cognitive Atlas RDF Generator</dc:Creator>
		<dc:Contributor>Russ Poldrack</dc:Contributor>
		<dc:Date>2012-01-28 07:45:04</dc:Date>
		<dc:Format>text/rdf</dc:Format>
		<dc:Language>en</dc:Language>
		<skos:editorialNote>Generated by testgenall.php on Thu Mar 29 10:24:07 PDT 2012.</skos:editorialNote>
		<skos:historyNote>Revision 2: 1 previous definitions.</skos:historyNote>
		<skos:changeNote>See http://www.cognitiveatlas.org/id/trm_4cacf22a22d80 for complete revision history.</skos:changeNote>
		<skos:scopeNote>http://www.w3.org/2004/02/skos/core#Concept</skos:scopeNote>
		<skos:Note>SKOS properties defined in http://www.w3.org/TR/skos-primer/#secrel</skos:Note>
		<skos:inScheme rdf:resource="http://www.cognitiveatlas.org/tasks/"/>
		<skos:definition>Subjects are presented with a set of stimuli and must classify those stimuli into one of two categories. In a common version known as the &#34;weather prediction task&#34; the stimuli are cards with geometric shapes on them and the outcomes are rainy versus sunny weather.  The feedback is probabilistic, and performance is measured by the proportion of statistically optimal responses.</skos:definition>
		<skos:prefLabel>Probabilistic classification task</skos:prefLabel>
		<skos:altLabel>probabilistic classification learning task, weather prediction task</skos:altLabel>
		<skos:related rdf:resource="http://www.cognitiveatlas.org/id/trm_4a3fd79d0a585"/>
		<skos:example> is measured by Probabilistic classification task</skos:example>
		<cito:citesForInformation rdf:resource="http://www.cognitiveatlas.org/citation/id/cit_4cacf245b81ba"/>
		<cito:citesForInformation rdf:resource="http://www.cognitiveatlas.org/citation/id/cit_4df8eaad6e2b2"/>
</skos:Concept><skos:Concept rdf:about="http://www.cognitiveatlas.org/id/trm_4cacf3fbc503b"> <dc:identifier>trm_4cacf3fbc503b</dc:identifier>
		<dc:Title>Cognitive Atlas : Lexicon : Conditional stop signal task</dc:Title>
		<dc:Description>RDF output for 'Conditional stop signal task'</dc:Description>
		<dc:Type>InteractiveResource</dc:Type>
		<dc:Publisher>Cognitive Atlas</dc:Publisher>
		<dc:Creator>Cognitive Atlas RDF Generator</dc:Creator>
		<dc:Contributor>Russ Poldrack</dc:Contributor>
		<dc:Date>2010-10-06 15:11:07</dc:Date>
		<dc:Format>text/rdf</dc:Format>
		<dc:Language>en</dc:Language>
		<skos:editorialNote>Generated by testgenall.php on Thu Mar 29 10:24:07 PDT 2012.</skos:editorialNote>
		<skos:historyNote>No previous definition revisions.</skos:historyNote>
		<skos:changeNote>This is the first and only definition provided.</skos:changeNote>
		<skos:scopeNote>http://www.w3.org/2004/02/skos/core#Concept</skos:scopeNote>
		<skos:Note>SKOS properties defined in http://www.w3.org/TR/skos-primer/#secrel</skos:Note>
		<skos:inScheme rdf:resource="http://www.cognitiveatlas.org/tasks/"/>
		<skos:definition>A task in which an external stimulus signals the participant to interrupt an already-initiated motor response, but only for a subset of possible responses.  </skos:definition>
		<skos:prefLabel>Conditional stop signal task</skos:prefLabel>
		<skos:altLabel></skos:altLabel>
		<skos:related rdf:resource="http://www.cognitiveatlas.org/id/trm_4a3fd79d0a613"/>
		<skos:related rdf:resource="http://www.cognitiveatlas.org/id/trm_4a3fd79d0af66"/>
		<skos:example>inhibition is measured by the contrast of Stop-critical trial trials in the Conditional stop signal task</skos:example>
		<skos:example>response inhibition is measured by the contrast of Stop-critical trial trials in the Conditional stop signal task</skos:example>
		<cito:citesForInformation rdf:resource="http://www.cognitiveatlas.org/citation/id/cit_4cacf48576093"/>
		<cito:citesForInformation rdf:resource="http://www.cognitiveatlas.org/citation/id/cit_4de7becce685e"/>
		<cito:citesForInformation rdf:resource="http://www.cognitiveatlas.org/citation/id/cit_4cacf48576093"/>
		<cito:citesForInformation rdf:resource="http://www.cognitiveatlas.org/citation/id/cit_4de7bf28e2457"/>
</skos:Concept><skos:Concept rdf:about="http://www.cognitiveatlas.org/id/tsk_4a57abb94981d"> <dc:identifier>tsk_4a57abb94981d</dc:identifier>
		<dc:Title>Cognitive Atlas : Lexicon : Action imitation task</dc:Title>
		<dc:Description>RDF output for 'Action imitation task'</dc:Description>
		<dc:Type>InteractiveResource</dc:Type>
		<dc:Publisher>Cognitive Atlas</dc:Publisher>
		<dc:Creator>Cognitive Atlas RDF Generator</dc:Creator>
		<dc:Contributor>Antonia Hamilton</dc:Contributor>
		<dc:Date>2010-04-27 08:37:35</dc:Date>
		<dc:Format>text/rdf</dc:Format>
		<dc:Language>en</dc:Language>
		<skos:editorialNote>Generated by testgenall.php on Thu Mar 29 10:24:07 PDT 2012.</skos:editorialNote>
		<skos:historyNote>Revision 2: 1 previous definitions.</skos:historyNote>
		<skos:changeNote>See http://www.cognitiveatlas.org/id/tsk_4a57abb94981d for complete revision history.</skos:changeNote>
		<skos:scopeNote>http://www.w3.org/2004/02/skos/core#Concept</skos:scopeNote>
		<skos:Note>SKOS properties defined in http://www.w3.org/TR/skos-primer/#secrel</skos:Note>
		<skos:inScheme rdf:resource="http://www.cognitiveatlas.org/tasks/"/>
		<skos:definition>A task in which a participant sees another person perform an action and later performs the same action him/herself.  Imitation can be immediate or delayed.  It can be instructed or elicited implicitly (without the participant&#39;s conscious awareness).  The actions imitated can be familar/meaningful actions or unfamilar/meaningless actions.</skos:definition>
		<skos:prefLabel>Action imitation task</skos:prefLabel>
		<skos:altLabel></skos:altLabel>
		<skos:related rdf:resource="http://www.cognitiveatlas.org/id/trm_4a3fd79d0addc"/>
		<skos:related rdf:resource="http://www.cognitiveatlas.org/id/trm_4a3fd79d0a972"/>
		<skos:related rdf:resource="http://www.cognitiveatlas.org/id/trm_4a3fd79d0b08f"/>
		<skos:example>procedural memory is measured by the contrast of immediate accuracy minus delayed accuracy trials in the Action imitation task</skos:example>
		<skos:example>motor control is measured by the contrast of standard deviation from the mean accuracy score trials in the Action imitation task</skos:example>
		<skos:example>semantic working memory is measured by the contrast of accuracy for meaningful actions minus accuracy for meaningless actions trials in the Action imitation task</skos:example>
		<cito:citesForInformation rdf:resource="http://www.cognitiveatlas.org/citation/id/cit_4de538b33bb4f"/>
		<cito:citesForInformation rdf:resource="http://www.cognitiveatlas.org/citation/id/cit_4de539c965bec"/>
		<cito:citesForInformation rdf:resource="http://www.cognitiveatlas.org/citation/id/cit_4de539ea4f537"/>
</skos:Concept><skos:Concept rdf:about="http://www.cognitiveatlas.org/id/tsk_4a57abb949846"> <dc:identifier>tsk_4a57abb949846</dc:identifier>
		<dc:Title>Cognitive Atlas : Lexicon : Action observation task</dc:Title>
		<dc:Description>RDF output for 'Action observation task'</dc:Description>
		<dc:Type>InteractiveResource</dc:Type>
		<dc:Publisher>Cognitive Atlas</dc:Publisher>
		<dc:Creator>Cognitive Atlas RDF Generator</dc:Creator>
		<dc:Contributor>Carinna Torgerson</dc:Contributor>
		<dc:Date>2011-05-31 15:54:08</dc:Date>
		<dc:Format>text/rdf</dc:Format>
		<dc:Language>en</dc:Language>
		<skos:editorialNote>Generated by testgenall.php on Thu Mar 29 10:24:07 PDT 2012.</skos:editorialNote>
		<skos:historyNote>Revision 4: 3 previous definitions.</skos:historyNote>
		<skos:changeNote>See http://www.cognitiveatlas.org/id/tsk_4a57abb949846 for complete revision history.</skos:changeNote>
		<skos:scopeNote>http://www.w3.org/2004/02/skos/core#Concept</skos:scopeNote>
		<skos:Note>SKOS properties defined in http://www.w3.org/TR/skos-primer/#secrel</skos:Note>
		<skos:inScheme rdf:resource="http://www.cognitiveatlas.org/tasks/"/>
		<skos:definition>Subjects view images of actions in order to learn the action themselves. </skos:definition>
		<skos:prefLabel>Action observation task</skos:prefLabel>
		<skos:altLabel></skos:altLabel>
		<skos:related rdf:resource="http://www.cognitiveatlas.org/id/trm_4a3fd79d0addc"/>
		<skos:example>procedural memory is measured by the contrast of standard deviation from the mean accuracy score trials in the Action observation task</skos:example>
		<cito:citesForInformation rdf:resource="http://www.cognitiveatlas.org/citation/id/cit_4de54d5ebe6b8"/>
		<cito:citesForInformation rdf:resource="http://www.cognitiveatlas.org/citation/id/cit_4de54f7dc7893"/>
		<cito:citesForInformation rdf:resource="http://www.cognitiveatlas.org/citation/id/cit_4de550d699f55"/>
</skos:Concept><skos:Concept rdf:about="http://www.cognitiveatlas.org/id/tsk_4a57abb949858"> <dc:identifier>tsk_4a57abb949858</dc:identifier>
		<dc:Title>Cognitive Atlas : Lexicon : Adult Attachment Interview</dc:Title>
		<dc:Description>RDF output for 'Adult Attachment Interview'</dc:Description>
		<dc:Type>InteractiveResource</dc:Type>
		<dc:Publisher>Cognitive Atlas</dc:Publisher>
		<dc:Creator>Cognitive Atlas RDF Generator</dc:Creator>
		<dc:Contributor>Corey White</dc:Contributor>
		<dc:Date>2011-08-15 10:52:30</dc:Date>
		<dc:Format>text/rdf</dc:Format>
		<dc:Language>en</dc:Language>
		<skos:editorialNote>Generated by testgenall.php on Thu Mar 29 10:24:07 PDT 2012.</skos:editorialNote>
		<skos:historyNote>Revision 4: 3 previous definitions.</skos:historyNote>
		<skos:changeNote>See http://www.cognitiveatlas.org/id/tsk_4a57abb949858 for complete revision history.</skos:changeNote>
		<skos:scopeNote>http://www.w3.org/2004/02/skos/core#Concept</skos:scopeNote>
		<skos:Note>SKOS properties defined in http://www.w3.org/TR/skos-primer/#secrel</skos:Note>
		<skos:inScheme rdf:resource="http://www.cognitiveatlas.org/tasks/"/>
		<skos:definition>Standardized interview used to assess developmental and attachment history.  </skos:definition>
		<skos:prefLabel>Adult Attachment Interview</skos:prefLabel>
		<skos:altLabel></skos:altLabel>
		<cito:citesForInformation rdf:resource="http://www.cognitiveatlas.org/citation/id/cit_4de556688b4f4"/>
		<cito:citesForInformation rdf:resource="http://www.cognitiveatlas.org/citation/id/cit_4de55832c02cd"/>
		<cito:citesForInformation rdf:resource="http://www.cognitiveatlas.org/citation/id/cit_4de558973ecc8"/>
</skos:Concept><skos:Concept rdf:about="http://www.cognitiveatlas.org/id/tsk_4a57abb949869"> <dc:identifier>tsk_4a57abb949869</dc:identifier>
		<dc:Title>Cognitive Atlas : Lexicon : Antisaccade/prosaccade task</dc:Title>
		<dc:Description>RDF output for 'Antisaccade/prosaccade task'</dc:Description>
		<dc:Type>InteractiveResource</dc:Type>
		<dc:Publisher>Cognitive Atlas</dc:Publisher>
		<dc:Creator>Cognitive Atlas RDF Generator</dc:Creator>
		<dc:Contributor>Russ Poldrack</dc:Contributor>
		<dc:Date>2012-01-28 07:28:36</dc:Date>
		<dc:Format>text/rdf</dc:Format>
		<dc:Language>en</dc:Language>
		<skos:editorialNote>Generated by testgenall.php on Thu Mar 29 10:24:07 PDT 2012.</skos:editorialNote>
		<skos:historyNote>Revision 5: 4 previous definitions.</skos:historyNote>
		<skos:changeNote>See http://www.cognitiveatlas.org/id/tsk_4a57abb949869 for complete revision history.</skos:changeNote>
		<skos:scopeNote>http://www.w3.org/2004/02/skos/core#Concept</skos:scopeNote>
		<skos:Note>SKOS properties defined in http://www.w3.org/TR/skos-primer/#secrel</skos:Note>
		<skos:inScheme rdf:resource="http://www.cognitiveatlas.org/tasks/"/>
		<skos:definition>Subjects view a fixation point and a visual target is presented.  Subjects are instructed to make a saccade away from the target (antisaccade) or to the target (prosaccade).</skos:definition>
		<skos:prefLabel>Antisaccade/prosaccade task</skos:prefLabel>
		<skos:altLabel>antisaccade task</skos:altLabel>
		<skos:related rdf:resource="http://www.cognitiveatlas.org/id/trm_4a3fd79d0a246"/>
		<skos:example>executive control is measured by the contrast of  trials in the Antisaccade/prosaccade task</skos:example>
		<cito:citesForInformation rdf:resource="http://www.cognitiveatlas.org/citation/id/cit_4de55a73e5d36"/>
		<cito:citesForInformation rdf:resource="http://www.cognitiveatlas.org/citation/id/cit_4de55c07b5a3b"/>
</skos:Concept><skos:Concept rdf:about="http://www.cognitiveatlas.org/id/tsk_4a57abb949879"> <dc:identifier>tsk_4a57abb949879</dc:identifier>
		<dc:Title>Cognitive Atlas : Lexicon : attentional blink task</dc:Title>
		<dc:Description>RDF output for 'attentional blink task'</dc:Description>
		<dc:Type>InteractiveResource</dc:Type>
		<dc:Publisher>Cognitive Atlas</dc:Publisher>
		<dc:Creator>Cognitive Atlas RDF Generator</dc:Creator>
		<dc:Contributor>Carinna Torgerson</dc:Contributor>
		<dc:Date>2011-05-31 14:27:57</dc:Date>
		<dc:Format>text/rdf</dc:Format>
		<dc:Language>en</dc:Language>
		<skos:editorialNote>Generated by testgenall.php on Thu Mar 29 10:24:07 PDT 2012.</skos:editorialNote>
		<skos:historyNote>Revision 2: 1 previous definitions.</skos:historyNote>
		<skos:changeNote>See http://www.cognitiveatlas.org/id/tsk_4a57abb949879 for complete revision history.</skos:changeNote>
		<skos:scopeNote>http://www.w3.org/2004/02/skos/core#Concept</skos:scopeNote>
		<skos:Note>SKOS properties defined in http://www.w3.org/TR/skos-primer/#secrel</skos:Note>
		<skos:inScheme rdf:resource="http://www.cognitiveatlas.org/tasks/"/>
		<skos:definition>attentional processing of a first stimulus interferes with and/or delays the allocation of attention to a second stimulus if the second is presented before the processing of the first has been completed.</skos:definition>
		<skos:prefLabel>attentional blink task</skos:prefLabel>
		<skos:altLabel></skos:altLabel>
		<skos:related rdf:resource="http://www.cognitiveatlas.org/id/trm_4a3fd79d0a61f"/>
		<skos:example>inhibition of return is measured by the contrast of magnitude of response to second stimulus trials in the attentional blink task</skos:example>
		<cito:citesForInformation rdf:resource="http://www.cognitiveatlas.org/citation/id/cit_4de55d7a4b8b5"/>
		<cito:citesForInformation rdf:resource="http://www.cognitiveatlas.org/citation/id/cit_4de560080b812"/>
		<cito:citesForInformation rdf:resource="http://www.cognitiveatlas.org/citation/id/cit_4de560e975f67"/>
</skos:Concept><skos:Concept rdf:about="http://www.cognitiveatlas.org/id/tsk_4a57abb949889"> <dc:identifier>tsk_4a57abb949889</dc:identifier>
		<dc:Title>Cognitive Atlas : Lexicon : audio-visual target-detection task</dc:Title>
		<dc:Description>RDF output for 'audio-visual target-detection task'</dc:Description>
		<dc:Type>InteractiveResource</dc:Type>
		<dc:Publisher>Cognitive Atlas</dc:Publisher>
		<dc:Creator>Cognitive Atlas RDF Generator</dc:Creator>
		<dc:Contributor>Carinna Torgerson</dc:Contributor>
		<dc:Date>2011-06-23 11:47:10</dc:Date>
		<dc:Format>text/rdf</dc:Format>
		<dc:Language>en</dc:Language>
		<skos:editorialNote>Generated by testgenall.php on Thu Mar 29 10:24:07 PDT 2012.</skos:editorialNote>
		<skos:historyNote>Revision 2: 1 previous definitions.</skos:historyNote>
		<skos:changeNote>See http://www.cognitiveatlas.org/id/tsk_4a57abb949889 for complete revision history.</skos:changeNote>
		<skos:scopeNote>http://www.w3.org/2004/02/skos/core#Concept</skos:scopeNote>
		<skos:Note>SKOS properties defined in http://www.w3.org/TR/skos-primer/#secrel</skos:Note>
		<skos:inScheme rdf:resource="http://www.cognitiveatlas.org/tasks/"/>
		<skos:definition>This task pairs auditory and visual stimuli. Participants are asked to indicate when the paired stimuli are presented in synchrony, or to identify the locations of the stimuli among distracting visual and auditory information.</skos:definition>
		<skos:prefLabel>audio-visual target-detection task</skos:prefLabel>
		<skos:altLabel></skos:altLabel>
		<skos:related rdf:resource="http://www.cognitiveatlas.org/id/trm_4a3fd79d09e1e"/>
		<skos:related rdf:resource="http://www.cognitiveatlas.org/id/trm_4a3fd79d0b0c8"/>
		<skos:related rdf:resource="http://www.cognitiveatlas.org/id/trm_4a3fd79d0b043"/>
		<skos:related rdf:resource="http://www.cognitiveatlas.org/id/trm_4a3fd79d09953"/>
		<skos:example>conjunction search is measured by the contrast of reaction time (to detect target) to one stimulus minus reaction time to paired stimuli trials in the audio-visual target-detection task</skos:example>
		<skos:example>serial search is measured by the contrast of reaction time of participant minus average reaction time of controls trials in the audio-visual target-detection task</skos:example>
		<skos:example>selective attention is measured by the contrast of accuracy without distractors minus accuracy with distractors trials in the audio-visual target-detection task</skos:example>
		<skos:example>audiovisual perception is measured by the contrast of reaction time (to detect target) to one stimulus minus reaction time to paired stimuli trials in the audio-visual target-detection task</skos:example>
		<cito:citesForInformation rdf:resource="http://www.cognitiveatlas.org/citation/id/cit_4e03850620f63"/>
		<cito:citesForInformation rdf:resource="http://www.cognitiveatlas.org/citation/id/cit_4e0386596d735"/>
		<cito:citesForInformation rdf:resource="http://www.cognitiveatlas.org/citation/id/cit_4e038a746da54"/>
</skos:Concept><skos:Concept rdf:about="http://www.cognitiveatlas.org/id/tsk_4a57abb94989b"> <dc:identifier>tsk_4a57abb94989b</dc:identifier>
		<dc:Title>Cognitive Atlas : Lexicon : Backward digit span task</dc:Title>
		<dc:Description>RDF output for 'Backward digit span task'</dc:Description>
		<dc:Type>InteractiveResource</dc:Type>
		<dc:Publisher>Cognitive Atlas</dc:Publisher>
		<dc:Creator>Cognitive Atlas RDF Generator</dc:Creator>
		<dc:Contributor>Brenda Gregory</dc:Contributor>
		<dc:Date>2011-05-16 13:18:25</dc:Date>
		<dc:Format>text/rdf</dc:Format>
		<dc:Language>en</dc:Language>
		<skos:editorialNote>Generated by testgenall.php on Thu Mar 29 10:24:07 PDT 2012.</skos:editorialNote>
		<skos:historyNote>Revision 3: 2 previous definitions.</skos:historyNote>
		<skos:changeNote>See http://www.cognitiveatlas.org/id/tsk_4a57abb94989b for complete revision history.</skos:changeNote>
		<skos:scopeNote>http://www.w3.org/2004/02/skos/core#Concept</skos:scopeNote>
		<skos:Note>SKOS properties defined in http://www.w3.org/TR/skos-primer/#secrel</skos:Note>
		<skos:inScheme rdf:resource="http://www.cognitiveatlas.org/tasks/"/>
		<skos:definition>a test used to measure working memory, attention, concentration, and mental control.  In a typical test of memory span, a list of random numbers or letters is read out loud or presented on a computer screen at the rate of one per second. The test begins with two to three numbers, increasing until the person commits errors. At the end of a sequence, the person being tested is asked to recall the items in reverse of the presented order.</skos:definition>
		<skos:prefLabel>Backward digit span task</skos:prefLabel>
		<skos:altLabel></skos:altLabel>
		<skos:related rdf:resource="http://www.cognitiveatlas.org/id/tsk_4a57abb949f12"/>
		<skos:related rdf:resource="http://www.cognitiveatlas.org/id/tsk_4a57abb949a0d"/>
		<skos:related rdf:resource="http://www.cognitiveatlas.org/id/tsk_4a57abb949a85"/>
		<skos:example>Backward digit span task is related to Wechsler Adult Intelligence Scale - Revised</skos:example>
		<skos:example>Backward digit span task is descended from Digit span task</skos:example>
		<skos:example>Backward digit span task is an exact synonym of Forward digit span task</skos:example>
		<cito:citesForInformation rdf:resource="http://www.cognitiveatlas.org/citation/id/cit_4de575709967d"/>
</skos:Concept><skos:Concept rdf:about="http://www.cognitiveatlas.org/id/tsk_4a57abb9498ab"> <dc:identifier>tsk_4a57abb9498ab</dc:identifier>
		<dc:Title>Cognitive Atlas : Lexicon : Behavioral Rating Inventory of Executive Function</dc:Title>
		<dc:Description>RDF output for 'Behavioral Rating Inventory of Executive Function'</dc:Description>
		<dc:Type>InteractiveResource</dc:Type>
		<dc:Publisher>Cognitive Atlas</dc:Publisher>
		<dc:Creator>Cognitive Atlas RDF Generator</dc:Creator>
		<dc:Contributor>Brenda Gregory</dc:Contributor>
		<dc:Date>2011-04-28 17:22:32</dc:Date>
		<dc:Format>text/rdf</dc:Format>
		<dc:Language>en</dc:Language>
		<skos:editorialNote>Generated by testgenall.php on Thu Mar 29 10:24:07 PDT 2012.</skos:editorialNote>
		<skos:historyNote>Revision 5: 4 previous definitions.</skos:historyNote>
		<skos:changeNote>See http://www.cognitiveatlas.org/id/tsk_4a57abb9498ab for complete revision history.</skos:changeNote>
		<skos:scopeNote>http://www.w3.org/2004/02/skos/core#Concept</skos:scopeNote>
		<skos:Note>SKOS properties defined in http://www.w3.org/TR/skos-primer/#secrel</skos:Note>
		<skos:inScheme rdf:resource="http://www.cognitiveatlas.org/tasks/"/>
		<skos:definition>used for evaluating and planning treatment strategies for a wide spectrum of developmental and acquired neurological conditions, including learning disabilities, low birth weight, ADHD, Tourette&#39;s disorder, Traumatic Brain Injury, and Autism; consists of 8 non-overlapping clinical scales that form two broader indexes: Behavior Regulation (three scales) and Metacognition (five scales). A Global Executive Composite score is also produced; completed by parents and teachers, is suitable for children as young as 5 years old.</skos:definition>
		<skos:prefLabel>Behavioral Rating Inventory of Executive Function</skos:prefLabel>
		<skos:altLabel></skos:altLabel>
		<skos:related rdf:resource="http://www.cognitiveatlas.org/id/trm_4a3fd79d0a252"/>
		<skos:related rdf:resource="http://www.cognitiveatlas.org/id/trm_4a3fd79d0a252"/>
		<skos:example>executive function is measured by the contrast of Negativity Scale trials in the Behavioral Rating Inventory of Executive Function</skos:example>
		<skos:example>executive function is measured by the contrast of Inconsistency Scale trials in the Behavioral Rating Inventory of Executive Function</skos:example>
		<cito:citesForInformation rdf:resource="http://www.cognitiveatlas.org/citation/id/cit_4de57dbb23ab8"/>
		<cito:citesForInformation rdf:resource="http://www.cognitiveatlas.org/citation/id/cit_4de5816f70873"/>
		<cito:citesForInformation rdf:resource="http://www.cognitiveatlas.org/citation/id/cit_4de581a4dcac0"/>
</skos:Concept><skos:Concept rdf:about="http://www.cognitiveatlas.org/id/tsk_4a57abb9498bc"> <dc:identifier>tsk_4a57abb9498bc</dc:identifier>
		<dc:Title>Cognitive Atlas : Lexicon : Benton Facial Recognition Test</dc:Title>
		<dc:Description>RDF output for 'Benton Facial Recognition Test'</dc:Description>
		<dc:Type>InteractiveResource</dc:Type>
		<dc:Publisher>Cognitive Atlas</dc:Publisher>
		<dc:Creator>Cognitive Atlas RDF Generator</dc:Creator>
		<dc:Contributor>Brenda Gregory</dc:Contributor>
		<dc:Date>2010-04-29 08:07:35</dc:Date>
		<dc:Format>text/rdf</dc:Format>
		<dc:Language>en</dc:Language>
		<skos:editorialNote>Generated by testgenall.php on Thu Mar 29 10:24:07 PDT 2012.</skos:editorialNote>
		<skos:historyNote>Revision 2: 1 previous definitions.</skos:historyNote>
		<skos:changeNote>See http://www.cognitiveatlas.org/id/tsk_4a57abb9498bc for complete revision history.</skos:changeNote>
		<skos:scopeNote>http://www.w3.org/2004/02/skos/core#Concept</skos:scopeNote>
		<skos:Note>SKOS properties defined in http://www.w3.org/TR/skos-primer/#secrel</skos:Note>
		<skos:inScheme rdf:resource="http://www.cognitiveatlas.org/tasks/"/>
		<skos:definition>A tool used to assess deficits in facial recognition.</skos:definition>
		<skos:prefLabel>Benton Facial Recognition Test</skos:prefLabel>
		<skos:altLabel></skos:altLabel>
		<cito:citesForInformation rdf:resource="http://www.cognitiveatlas.org/citation/id/cit_4de5835057136"/>
		<cito:citesForInformation rdf:resource="http://www.cognitiveatlas.org/citation/id/cit_4de5851834e44"/>
</skos:Concept><skos:Concept rdf:about="http://www.cognitiveatlas.org/id/tsk_4a57abb9498ce"> <dc:identifier>tsk_4a57abb9498ce</dc:identifier>
		<dc:Title>Cognitive Atlas : Lexicon : Birmingham Object Recognition Battery</dc:Title>
		<dc:Description>RDF output for 'Birmingham Object Recognition Battery'</dc:Description>
		<dc:Type>InteractiveResource</dc:Type>
		<dc:Publisher>Cognitive Atlas</dc:Publisher>
		<dc:Creator>Cognitive Atlas RDF Generator</dc:Creator>
		<dc:Contributor>Brenda Gregory</dc:Contributor>
		<dc:Date>2011-04-19 13:54:34</dc:Date>
		<dc:Format>text/rdf</dc:Format>
		<dc:Language>en</dc:Language>
		<skos:editorialNote>Generated by testgenall.php on Thu Mar 29 10:24:07 PDT 2012.</skos:editorialNote>
		<skos:historyNote>Revision 3: 2 previous definitions.</skos:historyNote>
		<skos:changeNote>See http://www.cognitiveatlas.org/id/tsk_4a57abb9498ce for complete revision history.</skos:changeNote>
		<skos:scopeNote>http://www.w3.org/2004/02/skos/core#Concept</skos:scopeNote>
		<skos:Note>SKOS properties defined in http://www.w3.org/TR/skos-primer/#secrel</skos:Note>
		<skos:inScheme rdf:resource="http://www.cognitiveatlas.org/tasks/"/>
		<skos:definition>a set of standardized procedures for assessing neuropsychological disorders of visual object recognition which includes tests to assess low-level aspects of visual perception (using same-different matching of basic perceptual features, such as orientation, length, position and object size), intermediate visual processes (e.g., matching objects different in viewpoint), access to stored perceptual knowledge about objects (object decision), access to semantic knowledge (function and associative matches) and access to names from object (picture naming).</skos:definition>
		<skos:prefLabel>Birmingham Object Recognition Battery</skos:prefLabel>
		<skos:altLabel></skos:altLabel>
		<skos:related rdf:resource="http://www.cognitiveatlas.org/id/trm_4a3fd79d0a533"/>
		<skos:related rdf:resource="http://www.cognitiveatlas.org/id/trm_4a3fd79d0b4b5"/>
		<skos:related rdf:resource="http://www.cognitiveatlas.org/id/trm_4a3fd79d0b4b5"/>
		<skos:related rdf:resource="http://www.cognitiveatlas.org/id/trm_4a3fd79d0b4a9"/>
		<skos:related rdf:resource="http://www.cognitiveatlas.org/id/trm_4a3fd79d0a398"/>
		<skos:related rdf:resource="http://www.cognitiveatlas.org/id/trm_4a3fd79d0a398"/>
		<skos:related rdf:resource="http://www.cognitiveatlas.org/id/trm_4a3fd79d0a398"/>
		<skos:related rdf:resource="http://www.cognitiveatlas.org/id/trm_4a3fd79d0a398"/>
		<skos:related rdf:resource="http://www.cognitiveatlas.org/id/trm_4a3fd79d0a398"/>
		<skos:related rdf:resource="http://www.cognitiveatlas.org/id/trm_4a3fd79d0a398"/>
		<skos:related rdf:resource="http://www.cognitiveatlas.org/id/trm_4a3fd79d0a398"/>
		<skos:example>implicit memory is measured by the contrast of object decision trials in the Birmingham Object Recognition Battery</skos:example>
		<skos:example>visual perception is measured by the contrast of copying test trials in the Birmingham Object Recognition Battery</skos:example>
		<skos:example>visual perception is measured by the contrast of overlapping figures test trials in the Birmingham Object Recognition Battery</skos:example>
		<skos:example>visual object recognition is measured by the contrast of picture naming trials in the Birmingham Object Recognition Battery</skos:example>
		<skos:example>form perception is measured by the contrast of size match trials in the Birmingham Object Recognition Battery</skos:example>
		<skos:example>form perception is measured by the contrast of length match trials in the Birmingham Object Recognition Battery</skos:example>
		<skos:example>form perception is measured by the contrast of orientation match trials in the Birmingham Object Recognition Battery</skos:example>
		<skos:example>form perception is measured by the contrast of position gap match trials in the Birmingham Object Recognition Battery</skos:example>
		<skos:example>form perception is measured by the contrast of overlapping figures test trials in the Birmingham Object Recognition Battery</skos:example>
		<skos:example>form perception is measured by the contrast of minimal feature match trials in the Birmingham Object Recognition Battery</skos:example>
		<skos:example>form perception is measured by the contrast of foreshortened match trials in the Birmingham Object Recognition Battery</skos:example>
		<cito:citesForInformation rdf:resource="http://www.cognitiveatlas.org/citation/id/cit_4de672a871c2b"/>
		<cito:citesForInformation rdf:resource="http://www.cognitiveatlas.org/citation/id/cit_4de67a6a537ec"/>
</skos:Concept><skos:Concept rdf:about="http://www.cognitiveatlas.org/id/tsk_4a57abb9498df"> <dc:identifier>tsk_4a57abb9498df</dc:identifier>
		<dc:Title>Cognitive Atlas : Lexicon : Block Tapping Test</dc:Title>
		<dc:Description>RDF output for 'Block Tapping Test'</dc:Description>
		<dc:Type>InteractiveResource</dc:Type>
		<dc:Publisher>Cognitive Atlas</dc:Publisher>
		<dc:Creator>Cognitive Atlas RDF Generator</dc:Creator>
		<dc:Contributor>Carinna Torgerson</dc:Contributor>
		<dc:Date>2011-06-01 11:43:29</dc:Date>
		<dc:Format>text/rdf</dc:Format>
		<dc:Language>en</dc:Language>
		<skos:editorialNote>Generated by testgenall.php on Thu Mar 29 10:24:07 PDT 2012.</skos:editorialNote>
		<skos:historyNote>Revision 5: 4 previous definitions.</skos:historyNote>
		<skos:changeNote>See http://www.cognitiveatlas.org/id/tsk_4a57abb9498df for complete revision history.</skos:changeNote>
		<skos:scopeNote>http://www.w3.org/2004/02/skos/core#Concept</skos:scopeNote>
		<skos:Note>SKOS properties defined in http://www.w3.org/TR/skos-primer/#secrel</skos:Note>
		<skos:inScheme rdf:resource="http://www.cognitiveatlas.org/tasks/"/>
		<skos:definition>tool used for assessment of visual short-term memory and implicit visual-spatial learning. An examiner taps a series of blocks and the subject must repeat in the correct sequential order. If the sequence is correct, the examiner adds another tap to the next sequence.</skos:definition>
		<skos:prefLabel>Block Tapping Test</skos:prefLabel>
		<skos:altLabel></skos:altLabel>
		<skos:related rdf:resource="http://www.cognitiveatlas.org/id/trm_4a3fd79d0b4d8"/>
		<skos:related rdf:resource="http://www.cognitiveatlas.org/id/trm_4da881dace79c"/>
		<skos:example>Block Tapping Test is descended from Corsi Blocks</skos:example>
		<skos:example>visual working memory is measured by the contrast of percent correct (number of correct sequences/number of total sequences) trials in the Block Tapping Test</skos:example>
		<cito:citesForInformation rdf:resource="http://www.cognitiveatlas.org/citation/id/cit_4de68558af17d"/>
		<cito:citesForInformation rdf:resource="http://www.cognitiveatlas.org/citation/id/cit_4de688a847c71"/>
		<cito:citesForInformation rdf:resource="http://www.cognitiveatlas.org/citation/id/cit_4de688f69b2cc"/>
</skos:Concept><skos:Concept rdf:about="http://www.cognitiveatlas.org/id/tsk_4a57abb9498ef"> <dc:identifier>tsk_4a57abb9498ef</dc:identifier>
		<dc:Title>Cognitive Atlas : Lexicon : Boston Naming Test</dc:Title>
		<dc:Description>RDF output for 'Boston Naming Test'</dc:Description>
		<dc:Type>InteractiveResource</dc:Type>
		<dc:Publisher>Cognitive Atlas</dc:Publisher>
		<dc:Creator>Cognitive Atlas RDF Generator</dc:Creator>
		<dc:Contributor>Brenda Gregory</dc:Contributor>
		<dc:Date>2011-04-28 12:19:45</dc:Date>
		<dc:Format>text/rdf</dc:Format>
		<dc:Language>en</dc:Language>
		<skos:editorialNote>Generated by testgenall.php on Thu Mar 29 10:24:07 PDT 2012.</skos:editorialNote>
		<skos:historyNote>Revision 3: 2 previous definitions.</skos:historyNote>
		<skos:changeNote>See http://www.cognitiveatlas.org/id/tsk_4a57abb9498ef for complete revision history.</skos:changeNote>
		<skos:scopeNote>http://www.w3.org/2004/02/skos/core#Concept</skos:scopeNote>
		<skos:Note>SKOS properties defined in http://www.w3.org/TR/skos-primer/#secrel</skos:Note>
		<skos:inScheme rdf:resource="http://www.cognitiveatlas.org/tasks/"/>
		<skos:definition>assesses the ability to name pictures of objects through spontaneous responses and need for various types of cueing, inferences can be drawn regarding language facility and possible localization of cerebral damage.</skos:definition>
		<skos:prefLabel>Boston Naming Test</skos:prefLabel>
		<skos:altLabel></skos:altLabel>
		<skos:related rdf:resource="http://www.cognitiveatlas.org/id/trm_4a3fd79d0a7e0"/>
		<skos:related rdf:resource="http://www.cognitiveatlas.org/id/trm_4a3fd79d0b80f"/>
		<skos:example>lexical retrieval is measured by the contrast of percent correct (number of correct responses/number of total pictures) trials in the Boston Naming Test</skos:example>
		<skos:example>lexical access is measured by the contrast of percent correct (number of correct responses/number of total pictures) trials in the Boston Naming Test</skos:example>
		<cito:citesForInformation rdf:resource="http://www.cognitiveatlas.org/citation/id/cit_4de68d6f15aa1"/>
		<cito:citesForInformation rdf:resource="http://www.cognitiveatlas.org/citation/id/cit_4de68dd700a49"/>
		<cito:citesForInformation rdf:resource="http://www.cognitiveatlas.org/citation/id/cit_4de68e47e2dd6"/>
</skos:Concept><skos:Concept rdf:about="http://www.cognitiveatlas.org/id/tsk_4a57abb949900"> <dc:identifier>tsk_4a57abb949900</dc:identifier>
		<dc:Title>Cognitive Atlas : Lexicon : California Verbal Learning Test-II</dc:Title>
		<dc:Description>RDF output for 'California Verbal Learning Test-II'</dc:Description>
		<dc:Type>InteractiveResource</dc:Type>
		<dc:Publisher>Cognitive Atlas</dc:Publisher>
		<dc:Creator>Cognitive Atlas RDF Generator</dc:Creator>
		<dc:Contributor>Brenda Gregory</dc:Contributor>
		<dc:Date>2011-05-18 14:05:42</dc:Date>
		<dc:Format>text/rdf</dc:Format>
		<dc:Language>en</dc:Language>
		<skos:editorialNote>Generated by testgenall.php on Thu Mar 29 10:24:07 PDT 2012.</skos:editorialNote>
		<skos:historyNote>Revision 3: 2 previous definitions.</skos:historyNote>
		<skos:changeNote>See http://www.cognitiveatlas.org/id/tsk_4a57abb949900 for complete revision history.</skos:changeNote>
		<skos:scopeNote>http://www.w3.org/2004/02/skos/core#Concept</skos:scopeNote>
		<skos:Note>SKOS properties defined in http://www.w3.org/TR/skos-primer/#secrel</skos:Note>
		<skos:inScheme rdf:resource="http://www.cognitiveatlas.org/tasks/"/>
		<skos:definition>A comprehensive and detailed assessment of verbal learning and memory available for older adolescents and adults. In addition to recall and recognition scores, it measures encoding strategies, learning rates, error types, and other process data.</skos:definition>
		<skos:prefLabel>California Verbal Learning Test-II</skos:prefLabel>
		<skos:altLabel></skos:altLabel>
		<skos:related rdf:resource="http://www.cognitiveatlas.org/id/trm_4a3fd79d09cae"/>
		<skos:related rdf:resource="http://www.cognitiveatlas.org/id/trm_4a3fd79d09cae"/>
		<skos:related rdf:resource="http://www.cognitiveatlas.org/id/trm_4a3fd79d0ba01"/>
		<skos:related rdf:resource="http://www.cognitiveatlas.org/id/trm_4a3fd79d0ba01"/>
		<skos:related rdf:resource="http://www.cognitiveatlas.org/id/trm_4a3fd79d0ba01"/>
		<skos:related rdf:resource="http://www.cognitiveatlas.org/id/trm_4a3fd79d0ba01"/>
		<skos:related rdf:resource="http://www.cognitiveatlas.org/id/trm_4a3fd79d0afab"/>
		<skos:related rdf:resource="http://www.cognitiveatlas.org/id/trm_4a3fd79d0ba6c"/>
		<skos:example>chunking is measured by the contrast of immediate recall trials in the California Verbal Learning Test-II</skos:example>
		<skos:example>chunking is measured by the contrast of long recall trials in the California Verbal Learning Test-II</skos:example>
		<skos:example>memory retrieval is measured by the contrast of immediate recall trials in the California Verbal Learning Test-II</skos:example>
		<skos:example>memory retrieval is measured by the contrast of interference trials in the California Verbal Learning Test-II</skos:example>
		<skos:example>memory retrieval is measured by the contrast of long recall trials in the California Verbal Learning Test-II</skos:example>
		<skos:example>memory retrieval is measured by the contrast of recognition trial trials in the California Verbal Learning Test-II</skos:example>
		<skos:example>retroactive interference is measured by the contrast of interference trials in the California Verbal Learning Test-II</skos:example>
		<skos:example>working memory retrieval is measured by the contrast of immediate recall trials in the California Verbal Learning Test-II</skos:example>
		<cito:citesForInformation rdf:resource="http://www.cognitiveatlas.org/citation/id/cit_4de69e5b88fc9"/>
		<cito:citesForInformation rdf:resource="http://www.cognitiveatlas.org/citation/id/cit_4de69f3e615d3"/>
</skos:Concept><skos:Concept rdf:about="http://www.cognitiveatlas.org/id/tsk_4a57abb949912"> <dc:identifier>tsk_4a57abb949912</dc:identifier>
		<dc:Title>Cognitive Atlas : Lexicon : Cambridge Face Memory Test</dc:Title>
		<dc:Description>RDF output for 'Cambridge Face Memory Test'</dc:Description>
		<dc:Type>InteractiveResource</dc:Type>
		<dc:Publisher>Cognitive Atlas</dc:Publisher>
		<dc:Creator>Cognitive Atlas RDF Generator</dc:Creator>
		<dc:Contributor>Carinna Torgerson</dc:Contributor>
		<dc:Date>2011-06-01 14:13:24</dc:Date>
		<dc:Format>text/rdf</dc:Format>
		<dc:Language>en</dc:Language>
		<skos:editorialNote>Generated by testgenall.php on Thu Mar 29 10:24:07 PDT 2012.</skos:editorialNote>
		<skos:historyNote>Revision 2: 1 previous definitions.</skos:historyNote>
		<skos:changeNote>See http://www.cognitiveatlas.org/id/tsk_4a57abb949912 for complete revision history.</skos:changeNote>
		<skos:scopeNote>http://www.w3.org/2004/02/skos/core#Concept</skos:scopeNote>
		<skos:Note>SKOS properties defined in http://www.w3.org/TR/skos-primer/#secrel</skos:Note>
		<skos:inScheme rdf:resource="http://www.cognitiveatlas.org/tasks/"/>
		<skos:definition>a test with high reliability and validity that assesses the ability to learn and then recognize six new faces.</skos:definition>
		<skos:prefLabel>Cambridge Face Memory Test</skos:prefLabel>
		<skos:altLabel></skos:altLabel>
		<skos:related rdf:resource="http://www.cognitiveatlas.org/id/trm_4a3fd79d0a30c"/>
		<skos:related rdf:resource="http://www.cognitiveatlas.org/id/trm_4a3fd79d0a30c"/>
		<skos:related rdf:resource="http://www.cognitiveatlas.org/id/trm_4a3fd79d0a30c"/>
		<skos:example>face recognition is measured by the contrast of same images trials in the Cambridge Face Memory Test</skos:example>
		<skos:example>face recognition is measured by the contrast of novel images trials in the Cambridge Face Memory Test</skos:example>
		<skos:example>face recognition is measured by the contrast of novel images with noise trials in the Cambridge Face Memory Test</skos:example>
		<cito:citesForInformation rdf:resource="http://www.cognitiveatlas.org/citation/id/cit_4de6ae747d7df"/>
		<cito:citesForInformation rdf:resource="http://www.cognitiveatlas.org/citation/id/cit_4de6ae8530714"/>
		<cito:citesForInformation rdf:resource="http://www.cognitiveatlas.org/citation/id/cit_4de6aec3e8c37"/>
</skos:Concept><skos:Concept rdf:about="http://www.cognitiveatlas.org/id/tsk_4a57abb949923"> <dc:identifier>tsk_4a57abb949923</dc:identifier>
		<dc:Title>Cognitive Atlas : Lexicon : category fluency test</dc:Title>
		<dc:Description>RDF output for 'category fluency test'</dc:Description>
		<dc:Type>InteractiveResource</dc:Type>
		<dc:Publisher>Cognitive Atlas</dc:Publisher>
		<dc:Creator>Cognitive Atlas RDF Generator</dc:Creator>
		<dc:Contributor>Brenda Gregory</dc:Contributor>
		<dc:Date>2011-04-19 13:52:08</dc:Date>
		<dc:Format>text/rdf</dc:Format>
		<dc:Language>en</dc:Language>
		<skos:editorialNote>Generated by testgenall.php on Thu Mar 29 10:24:07 PDT 2012.</skos:editorialNote>
		<skos:historyNote>Revision 3: 2 previous definitions.</skos:historyNote>
		<skos:changeNote>See http://www.cognitiveatlas.org/id/tsk_4a57abb949923 for complete revision history.</skos:changeNote>
		<skos:scopeNote>http://www.w3.org/2004/02/skos/core#Concept</skos:scopeNote>
		<skos:Note>SKOS properties defined in http://www.w3.org/TR/skos-primer/#secrel</skos:Note>
		<skos:inScheme rdf:resource="http://www.cognitiveatlas.org/tasks/"/>
		<skos:definition>a psychological test in which participants have to say as many words as possible from a category in a given time (usually 60 seconds), this category can be semantic, such as animals or fruits, or phonemic, such as words that begin with letter p.</skos:definition>
		<skos:prefLabel>category fluency test</skos:prefLabel>
		<skos:altLabel></skos:altLabel>
		<skos:related rdf:resource="http://www.cognitiveatlas.org/id/trm_4a3fd79d0b077"/>
		<skos:related rdf:resource="http://www.cognitiveatlas.org/id/trm_4a3fd79d0b083"/>
		<skos:related rdf:resource="http://www.cognitiveatlas.org/id/trm_4a3fd79d0b87a"/>
		<skos:example>semantic knowledge is measured by the contrast of total correct responses for all categories trials in the category fluency test</skos:example>
		<skos:example>semantic memory is measured by the contrast of total correct responses for all categories trials in the category fluency test</skos:example>
		<skos:example>semantic processing is measured by the contrast of total correct responses for all categories trials in the category fluency test</skos:example>
		<cito:citesForInformation rdf:resource="http://www.cognitiveatlas.org/citation/id/cit_4de6b8980e553"/>
		<cito:citesForInformation rdf:resource="http://www.cognitiveatlas.org/citation/id/cit_4de6b8cfaa710"/>
		<cito:citesForInformation rdf:resource="http://www.cognitiveatlas.org/citation/id/cit_4de6b9186135d"/>
</skos:Concept><skos:Concept rdf:about="http://www.cognitiveatlas.org/id/tsk_4a57abb949934"> <dc:identifier>tsk_4a57abb949934</dc:identifier>
		<dc:Title>Cognitive Atlas : Lexicon : choice reaction time task</dc:Title>
		<dc:Description>RDF output for 'choice reaction time task'</dc:Description>
		<dc:Type>InteractiveResource</dc:Type>
		<dc:Publisher>Cognitive Atlas</dc:Publisher>
		<dc:Creator>Cognitive Atlas RDF Generator</dc:Creator>
		<dc:Contributor>Natalie Picchetti</dc:Contributor>
		<dc:Date>2011-04-15 12:04:24</dc:Date>
		<dc:Format>text/rdf</dc:Format>
		<dc:Language>en</dc:Language>
		<skos:editorialNote>Generated by testgenall.php on Thu Mar 29 10:24:07 PDT 2012.</skos:editorialNote>
		<skos:historyNote>Revision 3: 2 previous definitions.</skos:historyNote>
		<skos:changeNote>See http://www.cognitiveatlas.org/id/tsk_4a57abb949934 for complete revision history.</skos:changeNote>
		<skos:scopeNote>http://www.w3.org/2004/02/skos/core#Concept</skos:scopeNote>
		<skos:Note>SKOS properties defined in http://www.w3.org/TR/skos-primer/#secrel</skos:Note>
		<skos:inScheme rdf:resource="http://www.cognitiveatlas.org/tasks/"/>
		<skos:definition>Choice reaction time tasks require distinct responses for each possible class of stimulus. For example, the subject might be asked to press one button if a red light appears and a different button if a yellow light appears.</skos:definition>
		<skos:prefLabel>choice reaction time task</skos:prefLabel>
		<skos:altLabel></skos:altLabel>
		<skos:related rdf:resource="http://www.cognitiveatlas.org/id/trm_4a3fd79d0af71"/>
		<skos:related rdf:resource="http://www.cognitiveatlas.org/id/trm_4a3fd79d0af66"/>
		<skos:related rdf:resource="http://www.cognitiveatlas.org/id/trm_4a3fd79d0b61f"/>
		<skos:related rdf:resource="http://www.cognitiveatlas.org/id/trm_4a3fd79d0b61f"/>
		<skos:related rdf:resource="http://www.cognitiveatlas.org/id/trm_4a3fd79d0b61f"/>
		<skos:related rdf:resource="http://www.cognitiveatlas.org/id/trm_4a3fd79d0b61f"/>
		<skos:related rdf:resource="http://www.cognitiveatlas.org/id/trm_4a3fd79d09c8c"/>
		<skos:related rdf:resource="http://www.cognitiveatlas.org/id/trm_4a3fd79d09c8c"/>
		<skos:related rdf:resource="http://www.cognitiveatlas.org/id/trm_4a3fd79d09c8c"/>
		<skos:related rdf:resource="http://www.cognitiveatlas.org/id/trm_4a3fd79d09c8c"/>
		<skos:example>response selection is measured by the contrast of stimulus trials in the choice reaction time task</skos:example>
		<skos:example>response inhibition is measured by the contrast of non-stimulus trials in the choice reaction time task</skos:example>
		<skos:example>decision is measured by the contrast of stimulus trials in the choice reaction time task</skos:example>
		<skos:example>decision is measured by the contrast of non-stimulus trials in the choice reaction time task</skos:example>
		<skos:example>decision is measured by the contrast of right hand trials in the choice reaction time task</skos:example>
		<skos:example>decision is measured by the contrast of left hand trials in the choice reaction time task</skos:example>
		<skos:example>choice is measured by the contrast of stimulus trials in the choice reaction time task</skos:example>
		<skos:example>choice is measured by the contrast of non-stimulus trials in the choice reaction time task</skos:example>
		<skos:example>choice is measured by the contrast of right hand trials in the choice reaction time task</skos:example>
		<skos:example>choice is measured by the contrast of left hand trials in the choice reaction time task</skos:example>
		<cito:citesForInformation rdf:resource="http://www.cognitiveatlas.org/citation/id/cit_4de6be81bb92a"/>
		<cito:citesForInformation rdf:resource="http://www.cognitiveatlas.org/citation/id/cit_4de6c044a5928"/>
		<cito:citesForInformation rdf:resource="http://www.cognitiveatlas.org/citation/id/cit_4de6c0f7c1bec"/>
</skos:Concept><skos:Concept rdf:about="http://www.cognitiveatlas.org/id/tsk_4a57abb9499a8"> <dc:identifier>tsk_4a57abb9499a8</dc:identifier>
		<dc:Title>Cognitive Atlas : Lexicon : Clinical Evaluation of Language Fundamentals-3</dc:Title>
		<dc:Description>RDF output for 'Clinical Evaluation of Language Fundamentals-3'</dc:Description>
		<dc:Type>InteractiveResource</dc:Type>
		<dc:Publisher>Cognitive Atlas</dc:Publisher>
		<dc:Creator>Cognitive Atlas RDF Generator</dc:Creator>
		<dc:Contributor>Brenda Gregory</dc:Contributor>
		<dc:Date>2011-05-10 15:00:36</dc:Date>
		<dc:Format>text/rdf</dc:Format>
		<dc:Language>en</dc:Language>
		<skos:editorialNote>Generated by testgenall.php on Thu Mar 29 10:24:07 PDT 2012.</skos:editorialNote>
		<skos:historyNote>Revision 3: 2 previous definitions.</skos:historyNote>
		<skos:changeNote>See http://www.cognitiveatlas.org/id/tsk_4a57abb9499a8 for complete revision history.</skos:changeNote>
		<skos:scopeNote>http://www.w3.org/2004/02/skos/core#Concept</skos:scopeNote>
		<skos:Note>SKOS properties defined in http://www.w3.org/TR/skos-primer/#secrel</skos:Note>
		<skos:inScheme rdf:resource="http://www.cognitiveatlas.org/tasks/"/>
		<skos:definition>3rd edition of an assessment used to evaluate the nature and extent of language difficulties in school children and adolescents.</skos:definition>
		<skos:prefLabel>Clinical Evaluation of Language Fundamentals-3</skos:prefLabel>
		<skos:altLabel></skos:altLabel>
		<skos:related rdf:resource="http://www.cognitiveatlas.org/id/trm_4a3fd79d0b340"/>
		<skos:related rdf:resource="http://www.cognitiveatlas.org/id/trm_4a3fd79d0b340"/>
		<skos:related rdf:resource="http://www.cognitiveatlas.org/id/trm_4a3fd79d0b340"/>
		<skos:related rdf:resource="http://www.cognitiveatlas.org/id/trm_4a3fd79d0a775"/>
		<skos:related rdf:resource="http://www.cognitiveatlas.org/id/trm_4a3fd79d0a775"/>
		<skos:related rdf:resource="http://www.cognitiveatlas.org/id/trm_4a3fd79d0a7f8"/>
		<skos:related rdf:resource="http://www.cognitiveatlas.org/id/trm_4a3fd79d0a7f8"/>
		<skos:related rdf:resource="http://www.cognitiveatlas.org/id/trm_4a3fd79d0a7f8"/>
		<skos:related rdf:resource="http://www.cognitiveatlas.org/id/trm_4a3fd79d0a7f8"/>
		<skos:related rdf:resource="http://www.cognitiveatlas.org/id/trm_4a3fd79d0a7f8"/>
		<skos:related rdf:resource="http://www.cognitiveatlas.org/id/trm_4a3fd79d0b06b"/>
		<skos:related rdf:resource="http://www.cognitiveatlas.org/id/trm_4a3fd79d0b892"/>
		<skos:related rdf:resource="http://www.cognitiveatlas.org/id/trm_4a3fd79d0b892"/>
		<skos:related rdf:resource="http://www.cognitiveatlas.org/id/trm_4a3fd79d0b56b"/>
		<skos:related rdf:resource="http://www.cognitiveatlas.org/id/trm_4a3fd79d0b1f7"/>
		<skos:example>syntactic parsing is measured by the contrast of formulating sentences subtest trials in the Clinical Evaluation of Language Fundamentals-3</skos:example>
		<skos:example>syntactic parsing is measured by the contrast of sentence structure subtest trials in the Clinical Evaluation of Language Fundamentals-3</skos:example>
		<skos:example>syntactic parsing is measured by the contrast of sentence assembly subtest trials in the Clinical Evaluation of Language Fundamentals-3</skos:example>
		<skos:example>language comprehension is measured by the contrast of concepts and directions subtest trials in the Clinical Evaluation of Language Fundamentals-3</skos:example>
		<skos:example>language comprehension is measured by the contrast of semantic relationships subtest trials in the Clinical Evaluation of Language Fundamentals-3</skos:example>
		<skos:example>linguistic competence is measured by the contrast of formulating sentences subtest trials in the Clinical Evaluation of Language Fundamentals-3</skos:example>
		<skos:example>linguistic competence is measured by the contrast of sentence structure subtest trials in the Clinical Evaluation of Language Fundamentals-3</skos:example>
		<skos:example>linguistic competence is measured by the contrast of word classes subtest trials in the Clinical Evaluation of Language Fundamentals-3</skos:example>
		<skos:example>linguistic competence is measured by the contrast of word structure subtest trials in the Clinical Evaluation of Language Fundamentals-3</skos:example>
		<skos:example>linguistic competence is measured by the contrast of sentence assembly subtest trials in the Clinical Evaluation of Language Fundamentals-3</skos:example>
		<skos:example>semantic category is measured by the contrast of semantic relationships subtest trials in the Clinical Evaluation of Language Fundamentals-3</skos:example>
		<skos:example>sentence comprehension is measured by the contrast of sentence structure subtest trials in the Clinical Evaluation of Language Fundamentals-3</skos:example>
		<skos:example>sentence comprehension is measured by the contrast of sentence assembly subtest trials in the Clinical Evaluation of Language Fundamentals-3</skos:example>
		<skos:example>word order is measured by the contrast of sentence structure subtest trials in the Clinical Evaluation of Language Fundamentals-3</skos:example>
		<skos:example>speech perception is measured by the contrast of concepts and directions subtest trials in the Clinical Evaluation of Language Fundamentals-3</skos:example>
		<cito:citesForInformation rdf:resource="http://www.cognitiveatlas.org/citation/id/cit_4de6d36356597"/>
		<cito:citesForInformation rdf:resource="http://www.cognitiveatlas.org/citation/id/cit_4de6d481e3982"/>
</skos:Concept><skos:Concept rdf:about="http://www.cognitiveatlas.org/id/tsk_4a57abb9499b8"> <dc:identifier>tsk_4a57abb9499b8</dc:identifier>
		<dc:Title>Cognitive Atlas : Lexicon : color-discrimination task</dc:Title>
		<dc:Description>RDF output for 'color-discrimination task'</dc:Description>
		<dc:Type>InteractiveResource</dc:Type>
		<dc:Publisher>Cognitive Atlas</dc:Publisher>
		<dc:Creator>Cognitive Atlas RDF Generator</dc:Creator>
		<dc:Contributor>Russ Poldrack</dc:Contributor>
		<dc:Date>2012-01-28 11:27:07</dc:Date>
		<dc:Format>text/rdf</dc:Format>
		<dc:Language>en</dc:Language>
		<skos:editorialNote>Generated by testgenall.php on Thu Mar 29 10:24:07 PDT 2012.</skos:editorialNote>
		<skos:historyNote>Revision 4: 3 previous definitions.</skos:historyNote>
		<skos:changeNote>See http://www.cognitiveatlas.org/id/tsk_4a57abb9499b8 for complete revision history.</skos:changeNote>
		<skos:scopeNote>http://www.w3.org/2004/02/skos/core#Concept</skos:scopeNote>
		<skos:Note>SKOS properties defined in http://www.w3.org/TR/skos-primer/#secrel</skos:Note>
		<skos:inScheme rdf:resource="http://www.cognitiveatlas.org/tasks/"/>
		<skos:definition>is a behavioral task where a subject is to make specific responses when presented with particular colors.  The responses to the various colors are then evaluated to see if the subject was able to discern between different colors.    </skos:definition>
		<skos:prefLabel>color-discrimination task</skos:prefLabel>
		<skos:altLabel></skos:altLabel>
		<skos:related rdf:resource="http://www.cognitiveatlas.org/id/trm_4a3fd79d09d93"/>
		<skos:example>color perception is measured by the contrast of accuracy trials in the color-discrimination task</skos:example>
		<cito:citesForInformation rdf:resource="http://www.cognitiveatlas.org/citation/id/cit_4de7b6b2401d2"/>
		<cito:citesForInformation rdf:resource="http://www.cognitiveatlas.org/citation/id/cit_4de7b9f69e8ed"/>
</skos:Concept><skos:Concept rdf:about="http://www.cognitiveatlas.org/id/tsk_4a57abb9499c7"> <dc:identifier>tsk_4a57abb9499c7</dc:identifier>
		<dc:Title>Cognitive Atlas : Lexicon : continuous recognition paradigm</dc:Title>
		<dc:Description>RDF output for 'continuous recognition paradigm'</dc:Description>
		<dc:Type>InteractiveResource</dc:Type>
		<dc:Publisher>Cognitive Atlas</dc:Publisher>
		<dc:Creator>Cognitive Atlas RDF Generator</dc:Creator>
		<dc:Contributor>Brenda Gregory</dc:Contributor>
		<dc:Date>2011-04-19 12:06:22</dc:Date>
		<dc:Format>text/rdf</dc:Format>
		<dc:Language>en</dc:Language>
		<skos:editorialNote>Generated by testgenall.php on Thu Mar 29 10:24:07 PDT 2012.</skos:editorialNote>
		<skos:historyNote>Revision 3: 2 previous definitions.</skos:historyNote>
		<skos:changeNote>See http://www.cognitiveatlas.org/id/tsk_4a57abb9499c7 for complete revision history.</skos:changeNote>
		<skos:scopeNote>http://www.w3.org/2004/02/skos/core#Concept</skos:scopeNote>
		<skos:Note>SKOS properties defined in http://www.w3.org/TR/skos-primer/#secrel</skos:Note>
		<skos:inScheme rdf:resource="http://www.cognitiveatlas.org/tasks/"/>
		<skos:definition>In the continuous recognition paradigm, study and test phases are not separate entities, but rather, items are continuously presented and the participant is instructed to respond to an item as &#34;old&#34; if it has been seen before (generally presented a second time) in this continual stream of item presentation. Items that were correctly called &#34;old&#34; are the subsequently remembered trials, and items that were &#34;missed&#34; (not called old upon second presentation) make up the subsequently forgotten trials. </skos:definition>
		<skos:prefLabel>continuous recognition paradigm</skos:prefLabel>
		<skos:altLabel></skos:altLabel>
		<skos:related rdf:resource="http://www.cognitiveatlas.org/id/trm_4a3fd79d0b58f"/>
		<skos:related rdf:resource="http://www.cognitiveatlas.org/id/trm_4a3fd79d0a323"/>
		<skos:related rdf:resource="http://www.cognitiveatlas.org/id/trm_4a3fd79d0b908"/>
		<skos:related rdf:resource="http://www.cognitiveatlas.org/id/trm_4c898b29660b0"/>
		<skos:example>word recognition is measured by the contrast of number of correct identifications trials in the continuous recognition paradigm</skos:example>
		<skos:example>false memory is measured by the contrast of number of false positives trials in the continuous recognition paradigm</skos:example>
		<skos:example>forgetting is measured by the contrast of number of false negatives (missed words) trials in the continuous recognition paradigm</skos:example>
		<skos:example>Cued Explicit Recognition is related to continuous recognition paradigm</skos:example>
		<cito:citesForInformation rdf:resource="http://www.cognitiveatlas.org/citation/id/cit_4de7c4d6b3c33"/>
		<cito:citesForInformation rdf:resource="http://www.cognitiveatlas.org/citation/id/cit_4de7c838e4fbd"/>
</skos:Concept><skos:Concept rdf:about="http://www.cognitiveatlas.org/id/tsk_4a57abb9499d5"> <dc:identifier>tsk_4a57abb9499d5</dc:identifier>
		<dc:Title>Cognitive Atlas : Lexicon : Cups task</dc:Title>
		<dc:Description>RDF output for 'Cups task'</dc:Description>
		<dc:Type>InteractiveResource</dc:Type>
		<dc:Publisher>Cognitive Atlas</dc:Publisher>
		<dc:Creator>Cognitive Atlas RDF Generator</dc:Creator>
		<dc:Contributor>Russ Poldrack</dc:Contributor>
		<dc:Date>2011-08-10 07:39:24</dc:Date>
		<dc:Format>text/rdf</dc:Format>
		<dc:Language>en</dc:Language>
		<skos:editorialNote>Generated by testgenall.php on Thu Mar 29 10:24:07 PDT 2012.</skos:editorialNote>
		<skos:historyNote>Revision 6: 5 previous definitions.</skos:historyNote>
		<skos:changeNote>See http://www.cognitiveatlas.org/id/tsk_4a57abb9499d5 for complete revision history.</skos:changeNote>
		<skos:scopeNote>http://www.w3.org/2004/02/skos/core#Concept</skos:scopeNote>
		<skos:Note>SKOS properties defined in http://www.w3.org/TR/skos-primer/#secrel</skos:Note>
		<skos:inScheme rdf:resource="http://www.cognitiveatlas.org/tasks/"/>
		<skos:definition>On each trial, participants choose between a risky and safe option. Each trial involves either gains or losses. The options are presented as a choice of cups. The risky option involves two to five cups, one containing a gain (loss) of $2, $3 or $5, and the others containing $0. If the latter option is selected, the payoff from one cup is selected at random. The safe cup offers a sure gain (loss) $1.</skos:definition>
		<skos:prefLabel>Cups task</skos:prefLabel>
		<skos:altLabel></skos:altLabel>
		<skos:related rdf:resource="http://www.cognitiveatlas.org/id/trm_4a3fd79d0b64e"/>
		<skos:related rdf:resource="http://www.cognitiveatlas.org/id/trm_4a3fd79d0afcf"/>
		<skos:related rdf:resource="http://www.cognitiveatlas.org/id/trm_4b6525253c63f"/>
		<skos:related rdf:resource="http://www.cognitiveatlas.org/id/trm_4d5599f8ed1bf"/>
		<skos:example>risk seeking is measured by the contrast of number or value of rewards times probability of reward trials in the Cups task</skos:example>
		<skos:example>risk is measured by the contrast of probability of highest reward trials in the Cups task</skos:example>
		<skos:example>reward is measured by the contrast of money earned trials in the Cups task</skos:example>
		<skos:example> is an exact synonym of Cups task</skos:example>
		<cito:citesForInformation rdf:resource="http://www.cognitiveatlas.org/citation/id/cit_4d559a46899b6"/>
		<cito:citesForInformation rdf:resource="http://www.cognitiveatlas.org/citation/id/cit_4d559a784a767"/>
</skos:Concept><skos:Concept rdf:about="http://www.cognitiveatlas.org/id/tsk_4a57abb9499e3"> <dc:identifier>tsk_4a57abb9499e3</dc:identifier>
		<dc:Title>Cognitive Atlas : Lexicon : delayed match to sample task</dc:Title>
		<dc:Description>RDF output for 'delayed match to sample task'</dc:Description>
		<dc:Type>InteractiveResource</dc:Type>
		<dc:Publisher>Cognitive Atlas</dc:Publisher>
		<dc:Creator>Cognitive Atlas RDF Generator</dc:Creator>
		<dc:Contributor>Russ Poldrack</dc:Contributor>
		<dc:Date>2012-01-28 07:41:16</dc:Date>
		<dc:Format>text/rdf</dc:Format>
		<dc:Language>en</dc:Language>
		<skos:editorialNote>Generated by testgenall.php on Thu Mar 29 10:24:07 PDT 2012.</skos:editorialNote>
		<skos:historyNote>Revision 5: 4 previous definitions.</skos:historyNote>
		<skos:changeNote>See http://www.cognitiveatlas.org/id/tsk_4a57abb9499e3 for complete revision history.</skos:changeNote>
		<skos:scopeNote>http://www.w3.org/2004/02/skos/core#Concept</skos:scopeNote>
		<skos:Note>SKOS properties defined in http://www.w3.org/TR/skos-primer/#secrel</skos:Note>
		<skos:inScheme rdf:resource="http://www.cognitiveatlas.org/tasks/"/>
		<skos:definition>Subjects view an item(s). After a brief delay a probe item is presented and subjects are asked to recall if the probe item was presented before the delay (during encoding). Stimuli can be words, pictures, or abstract patterns. </skos:definition>
		<skos:prefLabel>delayed match to sample task</skos:prefLabel>
		<skos:altLabel>dms task, delayed matching to sample task</skos:altLabel>
		<skos:related rdf:resource="http://www.cognitiveatlas.org/id/trm_4a3fd79d0ba0d"/>
		<skos:related rdf:resource="http://www.cognitiveatlas.org/id/trm_4a3fd79d0a431"/>
		<skos:related rdf:resource="http://www.cognitiveatlas.org/id/trm_4a3fd79d0b92c"/>
		<skos:related rdf:resource="http://www.cognitiveatlas.org/id/trm_4a3fd79d0ba6c"/>
		<skos:related rdf:resource="http://www.cognitiveatlas.org/id/trm_4a3fd79d0b5a7"/>
		<skos:related rdf:resource="http://www.cognitiveatlas.org/id/tsk_4a57abb949e0c"/>
		<skos:example>delayed match to sample task is a broader synonym of Sternberg delayed recognition task</skos:example>
		<skos:example>active maintenance is measured by the contrast of reaction time to correct stimuli trials in the delayed match to sample task</skos:example>
		<skos:example>goal maintenance is measured by the contrast of reaction time to correct stimuli trials in the delayed match to sample task</skos:example>
		<skos:example>memory decay is measured by the contrast of reaction time to correct stimuli trials in the delayed match to sample task</skos:example>
		<skos:example>working memory retrieval is measured by the contrast of reaction time to correct stimuli trials in the delayed match to sample task</skos:example>
		<skos:example>working memory is measured by the contrast of reaction time to correct stimuli trials in the delayed match to sample task</skos:example>
		<cito:citesForInformation rdf:resource="http://www.cognitiveatlas.org/citation/id/cit_4de90c3072da3"/>
		<cito:citesForInformation rdf:resource="http://www.cognitiveatlas.org/citation/id/cit_4de90e59e864b"/>
</skos:Concept><skos:Concept rdf:about="http://www.cognitiveatlas.org/id/tsk_4a57abb9499f1"> <dc:identifier>tsk_4a57abb9499f1</dc:identifier>
		<dc:Title>Cognitive Atlas : Lexicon : delayed nonmatch to sample task</dc:Title>
		<dc:Description>RDF output for 'delayed nonmatch to sample task'</dc:Description>
		<dc:Type>InteractiveResource</dc:Type>
		<dc:Publisher>Cognitive Atlas</dc:Publisher>
		<dc:Creator>Cognitive Atlas RDF Generator</dc:Creator>
		<dc:Contributor>Russ Poldrack</dc:Contributor>
		<dc:Date>2012-01-28 07:41:37</dc:Date>
		<dc:Format>text/rdf</dc:Format>
		<dc:Language>en</dc:Language>
		<skos:editorialNote>Generated by testgenall.php on Thu Mar 29 10:24:07 PDT 2012.</skos:editorialNote>
		<skos:historyNote>Revision 2: 1 previous definitions.</skos:historyNote>
		<skos:changeNote>See http://www.cognitiveatlas.org/id/tsk_4a57abb9499f1 for complete revision history.</skos:changeNote>
		<skos:scopeNote>http://www.w3.org/2004/02/skos/core#Concept</skos:scopeNote>
		<skos:Note>SKOS properties defined in http://www.w3.org/TR/skos-primer/#secrel</skos:Note>
		<skos:inScheme rdf:resource="http://www.cognitiveatlas.org/tasks/"/>
		<skos:definition>A task in which an target is presented and then removed from view. This target must be maintained in working memory for a delay, after which it is presented with non-target(s). The participant&#39;s task is to identify the non-target.</skos:definition>
		<skos:prefLabel>delayed nonmatch to sample task</skos:prefLabel>
		<skos:altLabel>DNMS task, delayed nonmatching to sample task</skos:altLabel>
		<skos:related rdf:resource="http://www.cognitiveatlas.org/id/trm_4a3fd79d0b5a7"/>
		<skos:related rdf:resource="http://www.cognitiveatlas.org/id/trm_4a3fd79d0b5a7"/>
		<skos:related rdf:resource="http://www.cognitiveatlas.org/id/trm_4a3fd79d0b92c"/>
		<skos:related rdf:resource="http://www.cognitiveatlas.org/id/trm_4a3fd79d0b5a7"/>
		<skos:related rdf:resource="http://www.cognitiveatlas.org/id/trm_4a3fd79d0a04f"/>
		<skos:example>working memory is measured by the contrast of delay trials in the delayed nonmatch to sample task</skos:example>
		<skos:example>working memory is measured by the contrast of delay minus no delay trials in the delayed nonmatch to sample task</skos:example>
		<skos:example>memory decay is measured by the contrast of delay minus no delay trials in the delayed nonmatch to sample task</skos:example>
		<skos:example>working memory is measured by the contrast of delay minus no delay trials in the delayed nonmatch to sample task</skos:example>
		<skos:example>declarative memory is measured by the contrast of  trials in the delayed nonmatch to sample task</skos:example>
		<cito:citesForInformation rdf:resource="http://www.cognitiveatlas.org/citation/id/cit_4de91383320ad"/>
		<cito:citesForInformation rdf:resource="http://www.cognitiveatlas.org/citation/id/cit_4de913bd78e06"/>
</skos:Concept><skos:Concept rdf:about="http://www.cognitiveatlas.org/id/tsk_4a57abb9499ff"> <dc:identifier>tsk_4a57abb9499ff</dc:identifier>
		<dc:Title>Cognitive Atlas : Lexicon : delayed recall test</dc:Title>
		<dc:Description>RDF output for 'delayed recall test'</dc:Description>
		<dc:Type>InteractiveResource</dc:Type>
		<dc:Publisher>Cognitive Atlas</dc:Publisher>
		<dc:Creator>Cognitive Atlas RDF Generator</dc:Creator>
		<dc:Contributor>Agatha Lenartowicz</dc:Contributor>
		<dc:Date>2009-07-10 14:06:33</dc:Date>
		<dc:Format>text/rdf</dc:Format>
		<dc:Language>en</dc:Language>
		<skos:editorialNote>Generated by testgenall.php on Thu Mar 29 10:24:07 PDT 2012.</skos:editorialNote>
		<skos:historyNote>No previous definition revisions.</skos:historyNote>
		<skos:changeNote>This is the first and only definition provided.</skos:changeNote>
		<skos:scopeNote>http://www.w3.org/2004/02/skos/core#Concept</skos:scopeNote>
		<skos:Note>SKOS properties defined in http://www.w3.org/TR/skos-primer/#secrel</skos:Note>
		<skos:inScheme rdf:resource="http://www.cognitiveatlas.org/tasks/"/>
		<skos:definition>A task in which participants are given information to remember (list of words or paragraph) and which they are asked to reproduce after some span of time.</skos:definition>
		<skos:prefLabel>delayed recall test</skos:prefLabel>
		<skos:altLabel></skos:altLabel>
		<skos:related rdf:resource="http://www.cognitiveatlas.org/id/trm_4a3fd79d0ba01"/>
		<skos:related rdf:resource="http://www.cognitiveatlas.org/id/trm_4a3fd79d0a833"/>
		<skos:related rdf:resource="http://www.cognitiveatlas.org/id/trm_4a3fd79d0a1f4"/>
		<skos:example>memory retrieval is measured by the contrast of d&#39; trials in the delayed recall test</skos:example>
		<skos:example>long term memory is measured by the contrast of d&#39; trials in the delayed recall test</skos:example>
		<skos:example>episodic memory is measured by the contrast of number of correctly recalled items trials in the delayed recall test</skos:example>
		<cito:citesForInformation rdf:resource="http://www.cognitiveatlas.org/citation/id/cit_4de916aca4c94"/>
		<cito:citesForInformation rdf:resource="http://www.cognitiveatlas.org/citation/id/cit_4de9177761ed9"/>
</skos:Concept><skos:Concept rdf:about="http://www.cognitiveatlas.org/id/tsk_4a57abb949a0d"> <dc:identifier>tsk_4a57abb949a0d</dc:identifier>
		<dc:Title>Cognitive Atlas : Lexicon : Digit span task</dc:Title>
		<dc:Description>RDF output for 'Digit span task'</dc:Description>
		<dc:Type>InteractiveResource</dc:Type>
		<dc:Publisher>Cognitive Atlas</dc:Publisher>
		<dc:Creator>Cognitive Atlas RDF Generator</dc:Creator>
		<dc:Contributor>Agatha Lenartowicz</dc:Contributor>
		<dc:Date>2009-07-10 14:06:33</dc:Date>
		<dc:Format>text/rdf</dc:Format>
		<dc:Language>en</dc:Language>
		<skos:editorialNote>Generated by testgenall.php on Thu Mar 29 10:24:07 PDT 2012.</skos:editorialNote>
		<skos:historyNote>No previous definition revisions.</skos:historyNote>
		<skos:changeNote>This is the first and only definition provided.</skos:changeNote>
		<skos:scopeNote>http://www.w3.org/2004/02/skos/core#Concept</skos:scopeNote>
		<skos:Note>SKOS properties defined in http://www.w3.org/TR/skos-primer/#secrel</skos:Note>
		<skos:inScheme rdf:resource="http://www.cognitiveatlas.org/tasks/"/>
		<skos:definition>A task in which participants are presented with sequentially presented digits and are then asked to recall the items. The number of digits that can be correctly recalled provides an estimate of working memory capacity.</skos:definition>
		<skos:prefLabel>Digit span task</skos:prefLabel>
		<skos:altLabel></skos:altLabel>
		<skos:related rdf:resource="http://www.cognitiveatlas.org/id/trm_4a3fd79d0a252"/>
		<skos:related rdf:resource="http://www.cognitiveatlas.org/id/trm_4a3fd79d0ac9e"/>
		<skos:related rdf:resource="http://www.cognitiveatlas.org/id/tsk_4a57abb94989b"/>
		<skos:related rdf:resource="http://www.cognitiveatlas.org/id/tsk_4a57abb949a85"/>
		<skos:related rdf:resource="http://www.cognitiveatlas.org/id/trm_4a3fd79d0b5a7"/>
		<skos:related rdf:resource="http://www.cognitiveatlas.org/id/trm_4a3fd79d0b5a7"/>
		<skos:related rdf:resource="http://www.cognitiveatlas.org/id/tsk_4a57abb949de3"/>
		<skos:example>executive function is measured by the contrast of backward trials in the Digit span task</skos:example>
		<skos:example>phonological working memory is measured by the contrast of forward trials in the Digit span task</skos:example>
		<skos:example>Backward digit span task is descended from Digit span task</skos:example>
		<skos:example>Forward digit span task is descended from Digit span task</skos:example>
		<skos:example>working memory is measured by the contrast of forward trials in the Digit span task</skos:example>
		<skos:example>working memory is measured by the contrast of backward trials in the Digit span task</skos:example>
		<skos:example>Span/Supra-Span Test is related to Digit span task</skos:example>
		<cito:citesForInformation rdf:resource="http://www.cognitiveatlas.org/citation/id/cit_4de923c052e03"/>
		<cito:citesForInformation rdf:resource="http://www.cognitiveatlas.org/citation/id/cit_4de9247400a43"/>
		<cito:citesForInformation rdf:resource="http://www.cognitiveatlas.org/citation/id/cit_4de925a401795"/>
</skos:Concept><skos:Concept rdf:about="http://www.cognitiveatlas.org/id/tsk_4a57abb949a25"> <dc:identifier>tsk_4a57abb949a25</dc:identifier>
		<dc:Title>Cognitive Atlas : Lexicon : Digit/Symbol Coding test</dc:Title>
		<dc:Description>RDF output for 'Digit/Symbol Coding test'</dc:Description>
		<dc:Type>InteractiveResource</dc:Type>
		<dc:Publisher>Cognitive Atlas</dc:Publisher>
		<dc:Creator>Cognitive Atlas RDF Generator</dc:Creator>
		<dc:Contributor>Natalie Picchetti</dc:Contributor>
		<dc:Date>2011-04-19 13:20:28</dc:Date>
		<dc:Format>text/rdf</dc:Format>
		<dc:Language>en</dc:Language>
		<skos:editorialNote>Generated by testgenall.php on Thu Mar 29 10:24:07 PDT 2012.</skos:editorialNote>
		<skos:historyNote>Revision 3: 2 previous definitions.</skos:historyNote>
		<skos:changeNote>See http://www.cognitiveatlas.org/id/tsk_4a57abb949a25 for complete revision history.</skos:changeNote>
		<skos:scopeNote>http://www.w3.org/2004/02/skos/core#Concept</skos:scopeNote>
		<skos:Note>SKOS properties defined in http://www.w3.org/TR/skos-primer/#secrel</skos:Note>
		<skos:inScheme rdf:resource="http://www.cognitiveatlas.org/tasks/"/>
		<skos:definition>a neuropsychological test sensitive to brain damage, dementia, age and depression; consists of (e.g. nine) digit-symbol pairs (e.g. 1/-,2/┴ ... 7/Λ,8/X,9/=) followed by a list of digits. Under each digit the subject should write down the corresponding symbol as fast as possible. The number of correct symbols within the allowed time (e.g. 90 or 120 sec) is measured.</skos:definition>
		<skos:prefLabel>Digit/Symbol Coding test</skos:prefLabel>
		<skos:altLabel></skos:altLabel>
		<skos:related rdf:resource="http://www.cognitiveatlas.org/id/trm_4a3fd79d0a972"/>
		<skos:related rdf:resource="http://www.cognitiveatlas.org/id/trm_4a3fd79d0b5a7"/>
		<skos:related rdf:resource="http://www.cognitiveatlas.org/id/trm_4a3fd79d0b8c1"/>
		<skos:related rdf:resource="http://www.cognitiveatlas.org/id/trm_4a3fd79d0b8c1"/>
		<skos:related rdf:resource="http://www.cognitiveatlas.org/id/trm_4a3fd79d0ba01"/>
		<skos:related rdf:resource="http://www.cognitiveatlas.org/id/tsk_4a57abb949e44"/>
		<skos:related rdf:resource="http://www.cognitiveatlas.org/id/tsk_4a57abb949f12"/>
		<skos:example>Digit/Symbol Coding test is descended from Wechsler Adult Intelligence Scale - Revised</skos:example>
		<skos:example>motor control is measured by the contrast of digit/symbol coding - symbol copy trials in the Digit/Symbol Coding test</skos:example>
		<skos:example>working memory is measured by the contrast of immediate memory copy trials in the Digit/Symbol Coding test</skos:example>
		<skos:example>active retrieval is measured by the contrast of immediate memory copy trials in the Digit/Symbol Coding test</skos:example>
		<skos:example>active retrieval is measured by the contrast of general memory copy trials in the Digit/Symbol Coding test</skos:example>
		<skos:example>memory retrieval is measured by the contrast of general memory copy trials in the Digit/Symbol Coding test</skos:example>
		<skos:example>symbol-digit substitution is an exact synonym of Digit/Symbol Coding test</skos:example>
		<cito:citesForInformation rdf:resource="http://www.cognitiveatlas.org/citation/id/cit_4de927e5da6b5"/>
		<cito:citesForInformation rdf:resource="http://www.cognitiveatlas.org/citation/id/cit_4de92a7fb8ecc"/>
</skos:Concept><skos:Concept rdf:about="http://www.cognitiveatlas.org/id/tsk_4a57abb949a33"> <dc:identifier>tsk_4a57abb949a33</dc:identifier>
		<dc:Title>Cognitive Atlas : Lexicon : Doors and People Test</dc:Title>
		<dc:Description>RDF output for 'Doors and People Test'</dc:Description>
		<dc:Type>InteractiveResource</dc:Type>
		<dc:Publisher>Cognitive Atlas</dc:Publisher>
		<dc:Creator>Cognitive Atlas RDF Generator</dc:Creator>
		<dc:Contributor>Brenda Gregory</dc:Contributor>
		<dc:Date>2011-05-16 13:29:43</dc:Date>
		<dc:Format>text/rdf</dc:Format>
		<dc:Language>en</dc:Language>
		<skos:editorialNote>Generated by testgenall.php on Thu Mar 29 10:24:07 PDT 2012.</skos:editorialNote>
		<skos:historyNote>Revision 3: 2 previous definitions.</skos:historyNote>
		<skos:changeNote>See http://www.cognitiveatlas.org/id/tsk_4a57abb949a33 for complete revision history.</skos:changeNote>
		<skos:scopeNote>http://www.w3.org/2004/02/skos/core#Concept</skos:scopeNote>
		<skos:Note>SKOS properties defined in http://www.w3.org/TR/skos-primer/#secrel</skos:Note>
		<skos:inScheme rdf:resource="http://www.cognitiveatlas.org/tasks/"/>
		<skos:definition>Doors and People is a test of long-term memory. It yields a single age-scaled overall score which can be ‘unpacked’ to give separate measures of visual and verbal memory, recall and recognition, and forgetting.</skos:definition>
		<skos:prefLabel>Doors and People Test</skos:prefLabel>
		<skos:altLabel></skos:altLabel>
		<skos:related rdf:resource="http://www.cognitiveatlas.org/id/trm_4a3fd79d0b0f7"/>
		<skos:related rdf:resource="http://www.cognitiveatlas.org/id/trm_4a3fd79d0b0f7"/>
		<skos:related rdf:resource="http://www.cognitiveatlas.org/id/trm_4a3fd79d0b0f7"/>
		<skos:related rdf:resource="http://www.cognitiveatlas.org/id/trm_4a3fd79d0b0f7"/>
		<skos:related rdf:resource="http://www.cognitiveatlas.org/id/trm_4a3fd79d0a4f9"/>
		<skos:related rdf:resource="http://www.cognitiveatlas.org/id/trm_4a3fd79d0a4f9"/>
		<skos:related rdf:resource="http://www.cognitiveatlas.org/id/trm_4a3fd79d0b95b"/>
		<skos:related rdf:resource="http://www.cognitiveatlas.org/id/trm_4a3fd79d0b95b"/>
		<skos:related rdf:resource="http://www.cognitiveatlas.org/id/trm_4a3fd79d0b95b"/>
		<skos:related rdf:resource="http://www.cognitiveatlas.org/id/trm_4a3fd79d0b95b"/>
		<skos:related rdf:resource="http://www.cognitiveatlas.org/id/trm_4a3fd79d0b967"/>
		<skos:example>short term memory is measured by the contrast of verbal recall (people test) trials in the Doors and People Test</skos:example>
		<skos:example>short term memory is measured by the contrast of visual recognition (doors test) trials in the Doors and People Test</skos:example>
		<skos:example>short term memory is measured by the contrast of visual recall (shapes test) trials in the Doors and People Test</skos:example>
		<skos:example>short term memory is measured by the contrast of verbal recognition (names test) trials in the Doors and People Test</skos:example>
		<skos:example>iconic memory is measured by the contrast of visual recognition (doors test) trials in the Doors and People Test</skos:example>
		<skos:example>iconic memory is measured by the contrast of visual recall (shapes test) trials in the Doors and People Test</skos:example>
		<skos:example>recall is measured by the contrast of verbal recall (people test) trials in the Doors and People Test</skos:example>
		<skos:example>recall is measured by the contrast of visual recognition (doors test) trials in the Doors and People Test</skos:example>
		<skos:example>recall is measured by the contrast of visual recall (shapes test) trials in the Doors and People Test</skos:example>
		<skos:example>recall is measured by the contrast of verbal recognition (names test) trials in the Doors and People Test</skos:example>
		<skos:example>recognition is measured by the contrast of  trials in the Doors and People Test</skos:example>
		<cito:citesForInformation rdf:resource="http://www.cognitiveatlas.org/citation/id/cit_4de93edaee646"/>
		<cito:citesForInformation rdf:resource="http://www.cognitiveatlas.org/citation/id/cit_4de93eebd4580"/>
</skos:Concept><skos:Concept rdf:about="http://www.cognitiveatlas.org/id/tsk_4a57abb949a41"> <dc:identifier>tsk_4a57abb949a41</dc:identifier>
		<dc:Title>Cognitive Atlas : Lexicon : Edinburgh Handedness Inventory</dc:Title>
		<dc:Description>RDF output for 'Edinburgh Handedness Inventory'</dc:Description>
		<dc:Type>InteractiveResource</dc:Type>
		<dc:Publisher>Cognitive Atlas</dc:Publisher>
		<dc:Creator>Cognitive Atlas RDF Generator</dc:Creator>
		<dc:Contributor>Carinna Torgerson</dc:Contributor>
		<dc:Date>2011-06-03 15:37:06</dc:Date>
		<dc:Format>text/rdf</dc:Format>
		<dc:Language>en</dc:Language>
		<skos:editorialNote>Generated by testgenall.php on Thu Mar 29 10:24:07 PDT 2012.</skos:editorialNote>
		<skos:historyNote>Revision 4: 3 previous definitions.</skos:historyNote>
		<skos:changeNote>See http://www.cognitiveatlas.org/id/tsk_4a57abb949a41 for complete revision history.</skos:changeNote>
		<skos:scopeNote>http://www.w3.org/2004/02/skos/core#Concept</skos:scopeNote>
		<skos:Note>SKOS properties defined in http://www.w3.org/TR/skos-primer/#secrel</skos:Note>
		<skos:inScheme rdf:resource="http://www.cognitiveatlas.org/tasks/"/>
		<skos:definition>a measurement scale used to assess the dominance of a person&#39;s right or left hand in everyday activities. It consists of a questionnaire with 10 activities listed (writing, drawing, throwing, using scissors, using a toothbrush, using a knife without a fork, using a spoon, the upper hand when using a broom, striking a match, and opening the lid of a box). Participants must indicate which hand they would use, and the strength of this preference (strong, less strong, indifferent).</skos:definition>
		<skos:prefLabel>Edinburgh Handedness Inventory</skos:prefLabel>
		<skos:altLabel></skos:altLabel>
		<skos:related rdf:resource="http://www.cognitiveatlas.org/id/trm_4a3fd79d0a972"/>
		<skos:example>motor control is measured by the contrast of sum of strength scores x sum of items per hand trials in the Edinburgh Handedness Inventory</skos:example>
		<cito:citesForInformation rdf:resource="http://www.cognitiveatlas.org/citation/id/cit_4de960c6f2de9"/>
		<cito:citesForInformation rdf:resource="http://www.cognitiveatlas.org/citation/id/cit_4de960eae240d"/>
		<cito:citesForInformation rdf:resource="http://www.cognitiveatlas.org/citation/id/cit_4de964cc5ca4e"/>
</skos:Concept><skos:Concept rdf:about="http://www.cognitiveatlas.org/id/tsk_4a57abb949a4f"> <dc:identifier>tsk_4a57abb949a4f</dc:identifier>
		<dc:Title>Cognitive Atlas : Lexicon : Eriksen flanker task</dc:Title>
		<dc:Description>RDF output for 'Eriksen flanker task'</dc:Description>
		<dc:Type>InteractiveResource</dc:Type>
		<dc:Publisher>Cognitive Atlas</dc:Publisher>
		<dc:Creator>Cognitive Atlas RDF Generator</dc:Creator>
		<dc:Contributor>Russ Poldrack</dc:Contributor>
		<dc:Date>2012-01-28 08:16:14</dc:Date>
		<dc:Format>text/rdf</dc:Format>
		<dc:Language>en</dc:Language>
		<skos:editorialNote>Generated by testgenall.php on Thu Mar 29 10:24:07 PDT 2012.</skos:editorialNote>
		<skos:historyNote>Revision 2: 1 previous definitions.</skos:historyNote>
		<skos:changeNote>See http://www.cognitiveatlas.org/id/tsk_4a57abb949a4f for complete revision history.</skos:changeNote>
		<skos:scopeNote>http://www.w3.org/2004/02/skos/core#Concept</skos:scopeNote>
		<skos:Note>SKOS properties defined in http://www.w3.org/TR/skos-primer/#secrel</skos:Note>
		<skos:inScheme rdf:resource="http://www.cognitiveatlas.org/tasks/"/>
		<skos:definition>A task in which participants view stimuli (typically arrows) presented one at a time and to which they must make a simple lexical response. These stimuli are surrounded by either distracting or facilitating items. Distracting items are typically associated with an opposite response (&#34;incongruent&#34; = pointing in opposite direction to target stimulus), whereas facilitating items are typically associated with the same response as the target stimulus (&#34;congruent&#34; = pointing in the same direction as the target stimulus).</skos:definition>
		<skos:prefLabel>Eriksen flanker task</skos:prefLabel>
		<skos:altLabel>flanker task</skos:altLabel>
		<skos:related rdf:resource="http://www.cognitiveatlas.org/id/trm_4a3fd79d0a613"/>
		<skos:related rdf:resource="http://www.cognitiveatlas.org/id/trm_4a3fd79d0a252"/>
		<skos:related rdf:resource="http://www.cognitiveatlas.org/id/trm_4a3fd79d0b5ef"/>
		<skos:example>inhibition is measured by the contrast of incongruent response time - congruent response time trials in the Eriksen flanker task</skos:example>
		<skos:example>executive function is measured by the contrast of incongruent response time - congruent response time trials in the Eriksen flanker task</skos:example>
		<skos:example>attentional focusing is measured by the contrast of  trials in the Eriksen flanker task</skos:example>
		<cito:citesForInformation rdf:resource="http://www.cognitiveatlas.org/citation/id/cit_4decff805f5d3"/>
		<cito:citesForInformation rdf:resource="http://www.cognitiveatlas.org/citation/id/cit_4ded00170b7f2"/>
		<cito:citesForInformation rdf:resource="http://www.cognitiveatlas.org/citation/id/cit_4ded002c8ae1c"/>
</skos:Concept><skos:Concept rdf:about="http://www.cognitiveatlas.org/id/tsk_4a57abb949a5d"> <dc:identifier>tsk_4a57abb949a5d</dc:identifier>
		<dc:Title>Cognitive Atlas : Lexicon : Extradimensional shift task</dc:Title>
		<dc:Description>RDF output for 'Extradimensional shift task'</dc:Description>
		<dc:Type>InteractiveResource</dc:Type>
		<dc:Publisher>Cognitive Atlas</dc:Publisher>
		<dc:Creator>Cognitive Atlas RDF Generator</dc:Creator>
		<dc:Contributor>Agatha Lenartowicz</dc:Contributor>
		<dc:Date>2009-07-10 14:06:33</dc:Date>
		<dc:Format>text/rdf</dc:Format>
		<dc:Language>en</dc:Language>
		<skos:editorialNote>Generated by testgenall.php on Thu Mar 29 10:24:07 PDT 2012.</skos:editorialNote>
		<skos:historyNote>No previous definition revisions.</skos:historyNote>
		<skos:changeNote>This is the first and only definition provided.</skos:changeNote>
		<skos:scopeNote>http://www.w3.org/2004/02/skos/core#Concept</skos:scopeNote>
		<skos:Note>SKOS properties defined in http://www.w3.org/TR/skos-primer/#secrel</skos:Note>
		<skos:inScheme rdf:resource="http://www.cognitiveatlas.org/tasks/"/>
		<skos:definition>A task in which multiple (typically two) stimuli are presented simultaneously and the subject must select the stimulus that matches the currently relevant rule. The relevant rule alternates or &#34;shifts&#34; among multiple (typically two) rules. The rule represents the relevant task &#34;dimension&#34;. The stimulus-response mappings are unique and constant within each possible rule dimension.</skos:definition>
		<skos:prefLabel>Extradimensional shift task</skos:prefLabel>
		<skos:altLabel></skos:altLabel>
		<skos:related rdf:resource="http://www.cognitiveatlas.org/id/trm_4a3fd79d0ab65"/>
		<skos:related rdf:resource="http://www.cognitiveatlas.org/id/trm_4a3fd79d0b5fb"/>
		<skos:related rdf:resource="http://www.cognitiveatlas.org/id/tsk_4a57abb949ad7"/>
		<skos:related rdf:resource="http://www.cognitiveatlas.org/id/trm_4a3fd79d0b5fb"/>
		<skos:related rdf:resource="http://www.cognitiveatlas.org/id/trm_4a3fd79d0ab65"/>
		<skos:related rdf:resource="http://www.cognitiveatlas.org/id/tsk_4a57abb949dad"/>
		<skos:related rdf:resource="http://www.cognitiveatlas.org/id/trm_4a3fd79d0b607"/>
		<skos:example>pattern recognition is measured by the contrast of average number of trials per pattern change trials in the Extradimensional shift task</skos:example>
		<skos:example>attention shifting is measured by the contrast of average number of trials per pattern change trials in the Extradimensional shift task</skos:example>
		<skos:example>Intradimensional shift task is related to Extradimensional shift task</skos:example>
		<skos:example>attention shifting is measured by the contrast of accuracy of subject minus average accuracy of controls trials in the Extradimensional shift task</skos:example>
		<skos:example>pattern recognition is measured by the contrast of accuracy of subject minus average accuracy of controls trials in the Extradimensional shift task</skos:example>
		<skos:example>Set-shifting task is a broader synonym of Extradimensional shift task</skos:example>
		<skos:example>set shifting is measured by the contrast of accuracy of subject minus average accuracy of controls trials in the Extradimensional shift task</skos:example>
		<cito:citesForInformation rdf:resource="http://www.cognitiveatlas.org/citation/id/cit_4ded02531ead1"/>
		<cito:citesForInformation rdf:resource="http://www.cognitiveatlas.org/citation/id/cit_4ded02d39297e"/>
		<cito:citesForInformation rdf:resource="http://www.cognitiveatlas.org/citation/id/cit_4ded0357be770"/>
</skos:Concept><skos:Concept rdf:about="http://www.cognitiveatlas.org/id/tsk_4a57abb949a6a"> <dc:identifier>tsk_4a57abb949a6a</dc:identifier>
		<dc:Title>Cognitive Atlas : Lexicon : face n-back task</dc:Title>
		<dc:Description>RDF output for 'face n-back task'</dc:Description>
		<dc:Type>InteractiveResource</dc:Type>
		<dc:Publisher>Cognitive Atlas</dc:Publisher>
		<dc:Creator>Cognitive Atlas RDF Generator</dc:Creator>
		<dc:Contributor>Carinna Torgerson</dc:Contributor>
		<dc:Date>2011-06-06 10:39:51</dc:Date>
		<dc:Format>text/rdf</dc:Format>
		<dc:Language>en</dc:Language>
		<skos:editorialNote>Generated by testgenall.php on Thu Mar 29 10:24:08 PDT 2012.</skos:editorialNote>
		<skos:historyNote>Revision 3: 2 previous definitions.</skos:historyNote>
		<skos:changeNote>See http://www.cognitiveatlas.org/id/tsk_4a57abb949a6a for complete revision history.</skos:changeNote>
		<skos:scopeNote>http://www.w3.org/2004/02/skos/core#Concept</skos:scopeNote>
		<skos:Note>SKOS properties defined in http://www.w3.org/TR/skos-primer/#secrel</skos:Note>
		<skos:inScheme rdf:resource="http://www.cognitiveatlas.org/tasks/"/>
		<skos:definition>Task in which face stimuli are presented one at a time in a continuous stream, and the objective is to detect when the current face matches the face presented n previously (1,2, or 3 faces before).</skos:definition>
		<skos:prefLabel>face n-back task</skos:prefLabel>
		<skos:altLabel></skos:altLabel>
		<skos:related rdf:resource="http://www.cognitiveatlas.org/id/trm_4a3fd79d0b65a"/>
		<skos:related rdf:resource="http://www.cognitiveatlas.org/id/trm_4a3fd79d0a30c"/>
		<skos:related rdf:resource="http://www.cognitiveatlas.org/id/trm_4a3fd79d0a300"/>
		<skos:related rdf:resource="http://www.cognitiveatlas.org/id/trm_4a3fd79d0b08f"/>
		<skos:related rdf:resource="http://www.cognitiveatlas.org/id/trm_4a3fd79d0b4d8"/>
		<skos:related rdf:resource="http://www.cognitiveatlas.org/id/trm_4a3fd79d0b4d8"/>
		<skos:related rdf:resource="http://www.cognitiveatlas.org/id/trm_4a3fd79d0b5a7"/>
		<skos:related rdf:resource="http://www.cognitiveatlas.org/id/trm_4a3fd79d0b5a7"/>
		<skos:related rdf:resource="http://www.cognitiveatlas.org/id/trm_4a3fd79d0ba6c"/>
		<skos:related rdf:resource="http://www.cognitiveatlas.org/id/trm_4a3fd79d0ba6c"/>
		<skos:related rdf:resource="http://www.cognitiveatlas.org/id/tsk_4a57abb949bcd"/>
		<skos:related rdf:resource="http://www.cognitiveatlas.org/id/tsk_4a57abb949df1"/>
		<skos:related rdf:resource="http://www.cognitiveatlas.org/id/tsk_4a57abb949b1c"/>
		<skos:example>face n-back task is descended from n-back task</skos:example>
		<skos:example>face n-back task is related to spatial n-back task</skos:example>
		<skos:example>face n-back task is related to letter n-back task</skos:example>
		<skos:example>emotion perception is measured by the contrast of emotion detection trials in the face n-back task</skos:example>
		<skos:example>face recognition is measured by the contrast of identity detection trials in the face n-back task</skos:example>
		<skos:example>face perception is measured by the contrast of identity detection trials in the face n-back task</skos:example>
		<skos:example>semantic working memory is measured by the contrast of emotion detection trials in the face n-back task</skos:example>
		<skos:example>visual working memory is measured by the contrast of emotion detection trials in the face n-back task</skos:example>
		<skos:example>visual working memory is measured by the contrast of identity detection trials in the face n-back task</skos:example>
		<skos:example>working memory is measured by the contrast of emotion detection trials in the face n-back task</skos:example>
		<skos:example>working memory is measured by the contrast of identity detection trials in the face n-back task</skos:example>
		<skos:example>working memory retrieval is measured by the contrast of emotion detection trials in the face n-back task</skos:example>
		<skos:example>working memory retrieval is measured by the contrast of identity detection trials in the face n-back task</skos:example>
		<cito:citesForInformation rdf:resource="http://www.cognitiveatlas.org/citation/id/cit_4ded0c34d377f"/>
		<cito:citesForInformation rdf:resource="http://www.cognitiveatlas.org/citation/id/cit_4ded116d8ddff"/>
		<cito:citesForInformation rdf:resource="http://www.cognitiveatlas.org/citation/id/cit_4ded12df97519"/>
</skos:Concept><skos:Concept rdf:about="http://www.cognitiveatlas.org/id/tsk_4a57abb949a78"> <dc:identifier>tsk_4a57abb949a78</dc:identifier>
		<dc:Title>Cognitive Atlas : Lexicon : Fagerstrom Test for Nicotine Dependence</dc:Title>
		<dc:Description>RDF output for 'Fagerstrom Test for Nicotine Dependence'</dc:Description>
		<dc:Type>InteractiveResource</dc:Type>
		<dc:Publisher>Cognitive Atlas</dc:Publisher>
		<dc:Creator>Cognitive Atlas RDF Generator</dc:Creator>
		<dc:Contributor>Brenda Gregory</dc:Contributor>
		<dc:Date>2011-04-28 17:27:56</dc:Date>
		<dc:Format>text/rdf</dc:Format>
		<dc:Language>en</dc:Language>
		<skos:editorialNote>Generated by testgenall.php on Thu Mar 29 10:24:08 PDT 2012.</skos:editorialNote>
		<skos:historyNote>Revision 3: 2 previous definitions.</skos:historyNote>
		<skos:changeNote>See http://www.cognitiveatlas.org/id/tsk_4a57abb949a78 for complete revision history.</skos:changeNote>
		<skos:scopeNote>http://www.w3.org/2004/02/skos/core#Concept</skos:scopeNote>
		<skos:Note>SKOS properties defined in http://www.w3.org/TR/skos-primer/#secrel</skos:Note>
		<skos:inScheme rdf:resource="http://www.cognitiveatlas.org/tasks/"/>
		<skos:definition>a standard instrument for assessing the intensity of physical addiction to nicotine.</skos:definition>
		<skos:prefLabel>Fagerstrom Test for Nicotine Dependence</skos:prefLabel>
		<skos:altLabel></skos:altLabel>
		<skos:related rdf:resource="http://www.cognitiveatlas.org/id/tsk_4a57abb949eb3"/>
		<skos:example>Tobacco Craving Questionnaire is related to Fagerstrom Test for Nicotine Dependence</skos:example>
		<cito:citesForInformation rdf:resource="http://www.cognitiveatlas.org/citation/id/cit_4ded1500b344e"/>
		<cito:citesForInformation rdf:resource="http://www.cognitiveatlas.org/citation/id/cit_4ded1e256fbe7"/>
		<cito:citesForInformation rdf:resource="http://www.cognitiveatlas.org/citation/id/cit_4ded1ed9369d8"/>
		<cito:citesForInformation rdf:resource="http://www.cognitiveatlas.org/citation/id/cit_4ded1f253ee49"/>
</skos:Concept><skos:Concept rdf:about="http://www.cognitiveatlas.org/id/tsk_4a57abb949a85"> <dc:identifier>tsk_4a57abb949a85</dc:identifier>
		<dc:Title>Cognitive Atlas : Lexicon : Forward digit span task</dc:Title>
		<dc:Description>RDF output for 'Forward digit span task'</dc:Description>
		<dc:Type>InteractiveResource</dc:Type>
		<dc:Publisher>Cognitive Atlas</dc:Publisher>
		<dc:Creator>Cognitive Atlas RDF Generator</dc:Creator>
		<dc:Contributor>Brenda Gregory</dc:Contributor>
		<dc:Date>2010-03-25 15:52:06</dc:Date>
		<dc:Format>text/rdf</dc:Format>
		<dc:Language>en</dc:Language>
		<skos:editorialNote>Generated by testgenall.php on Thu Mar 29 10:24:08 PDT 2012.</skos:editorialNote>
		<skos:historyNote>Revision 2: 1 previous definitions.</skos:historyNote>
		<skos:changeNote>See http://www.cognitiveatlas.org/id/tsk_4a57abb949a85 for complete revision history.</skos:changeNote>
		<skos:scopeNote>http://www.w3.org/2004/02/skos/core#Concept</skos:scopeNote>
		<skos:Note>SKOS properties defined in http://www.w3.org/TR/skos-primer/#secrel</skos:Note>
		<skos:inScheme rdf:resource="http://www.cognitiveatlas.org/tasks/"/>
		<skos:definition>A method of short-term memory measurement in which a person listens to someone say a series of single-digit numbers and must repeat them back in the same order they were given.</skos:definition>
		<skos:prefLabel>Forward digit span task</skos:prefLabel>
		<skos:altLabel></skos:altLabel>
		<skos:related rdf:resource="http://www.cognitiveatlas.org/id/tsk_4a57abb94989b"/>
		<skos:related rdf:resource="http://www.cognitiveatlas.org/id/trm_4a3fd79d0ac9e"/>
		<skos:related rdf:resource="http://www.cognitiveatlas.org/id/trm_4a3fd79d0b5a7"/>
		<skos:related rdf:resource="http://www.cognitiveatlas.org/id/tsk_4a57abb949a0d"/>
		<skos:example>Forward digit span task is descended from Digit span task</skos:example>
		<skos:example>Backward digit span task is an exact synonym of Forward digit span task</skos:example>
		<skos:example>phonological working memory is measured by the contrast of length of longest correct sequence trials in the Forward digit span task</skos:example>
		<skos:example>working memory is measured by the contrast of length of longest correct sequence trials in the Forward digit span task</skos:example>
		<cito:citesForInformation rdf:resource="http://www.cognitiveatlas.org/citation/id/cit_4de575709967d"/>
</skos:Concept><skos:Concept rdf:about="http://www.cognitiveatlas.org/id/tsk_4a57abb949a93"> <dc:identifier>tsk_4a57abb949a93</dc:identifier>
		<dc:Title>Cognitive Atlas : Lexicon : Go/no-go task</dc:Title>
		<dc:Description>RDF output for 'Go/no-go task'</dc:Description>
		<dc:Type>InteractiveResource</dc:Type>
		<dc:Publisher>Cognitive Atlas</dc:Publisher>
		<dc:Creator>Cognitive Atlas RDF Generator</dc:Creator>
		<dc:Contributor>Russ Poldrack</dc:Contributor>
		<dc:Date>2012-01-28 08:09:20</dc:Date>
		<dc:Format>text/rdf</dc:Format>
		<dc:Language>en</dc:Language>
		<skos:editorialNote>Generated by testgenall.php on Thu Mar 29 10:24:08 PDT 2012.</skos:editorialNote>
		<skos:historyNote>Revision 2: 1 previous definitions.</skos:historyNote>
		<skos:changeNote>See http://www.cognitiveatlas.org/id/tsk_4a57abb949a93 for complete revision history.</skos:changeNote>
		<skos:scopeNote>http://www.w3.org/2004/02/skos/core#Concept</skos:scopeNote>
		<skos:Note>SKOS properties defined in http://www.w3.org/TR/skos-primer/#secrel</skos:Note>
		<skos:inScheme rdf:resource="http://www.cognitiveatlas.org/tasks/"/>
		<skos:definition>A task in which stimuli are presented in a continuous stream and participants perform a binary decision on each stimulus. One of the outcomes requires participants to make a motor response (go), whereas the other requires participants to withhold a response (no-go). Accuracy and reaction time are measured for each event. Go events typically occur with higher frequency than no-go events. </skos:definition>
		<skos:prefLabel>Go/no-go task</skos:prefLabel>
		<skos:altLabel>go/nogo task</skos:altLabel>
		<skos:related rdf:resource="http://www.cognitiveatlas.org/id/trm_4a3fd79d0af66"/>
		<skos:related rdf:resource="http://www.cognitiveatlas.org/id/trm_4b7c270940f9d"/>
		<skos:related rdf:resource="http://www.cognitiveatlas.org/id/trm_4a3fd79d0a613"/>
		<skos:example>response inhibition is measured by the contrast of Stop trial trials in the Go/no-go task</skos:example>
		<skos:example>behavioral inhibition (cognitive) is measured by the contrast of stop minus go trials in the Go/no-go task</skos:example>
		<skos:example>inhibition is measured by the contrast of Stop trial trials in the Go/no-go task</skos:example>
		<cito:citesForInformation rdf:resource="http://www.cognitiveatlas.org/citation/id/cit_4ded4d890aeb6"/>
		<cito:citesForInformation rdf:resource="http://www.cognitiveatlas.org/citation/id/cit_4ded4db7342f2"/>
		<cito:citesForInformation rdf:resource="http://www.cognitiveatlas.org/citation/id/cit_4ded4defe2990"/>
</skos:Concept><skos:Concept rdf:about="http://www.cognitiveatlas.org/id/tsk_4a57abb949aa1"> <dc:identifier>tsk_4a57abb949aa1</dc:identifier>
		<dc:Title>Cognitive Atlas : Lexicon : Gray Oral Reading Test - 4</dc:Title>
		<dc:Description>RDF output for 'Gray Oral Reading Test - 4'</dc:Description>
		<dc:Type>InteractiveResource</dc:Type>
		<dc:Publisher>Cognitive Atlas</dc:Publisher>
		<dc:Creator>Cognitive Atlas RDF Generator</dc:Creator>
		<dc:Contributor>Brenda Gregory</dc:Contributor>
		<dc:Date>2011-05-16 11:23:19</dc:Date>
		<dc:Format>text/rdf</dc:Format>
		<dc:Language>en</dc:Language>
		<skos:editorialNote>Generated by testgenall.php on Thu Mar 29 10:24:08 PDT 2012.</skos:editorialNote>
		<skos:historyNote>Revision 4: 3 previous definitions.</skos:historyNote>
		<skos:changeNote>See http://www.cognitiveatlas.org/id/tsk_4a57abb949aa1 for complete revision history.</skos:changeNote>
		<skos:scopeNote>http://www.w3.org/2004/02/skos/core#Concept</skos:scopeNote>
		<skos:Note>SKOS properties defined in http://www.w3.org/TR/skos-primer/#secrel</skos:Note>
		<skos:inScheme rdf:resource="http://www.cognitiveatlas.org/tasks/"/>
		<skos:definition>measures growth in oral reading and aids in the diagnosis of oral reading difficulties. Five scores provide information on oral reading skills in terms of: Rate, accuracy, fluency, comprehension, overall reading ability, and comprehension. The test consists of two parallel forms, each containing 14 developmentally sequenced reading passages with five comprehension questions following each passage.</skos:definition>
		<skos:prefLabel>Gray Oral Reading Test - 4</skos:prefLabel>
		<skos:altLabel></skos:altLabel>
		<skos:related rdf:resource="http://www.cognitiveatlas.org/id/trm_4a3fd79d0aeb6"/>
		<skos:related rdf:resource="http://www.cognitiveatlas.org/id/trm_4a3fd79d09bbf"/>
		<skos:related rdf:resource="http://www.cognitiveatlas.org/id/trm_4a3fd79d0a775"/>
		<skos:example>reading is measured by the contrast of sum of rate, accuracy, fluency, and comprehension scaled scores trials in the Gray Oral Reading Test - 4</skos:example>
		<skos:example>binocular vision is measured by the contrast of sum of rate, accuracy, fluency, and comprehension scaled scores trials in the Gray Oral Reading Test - 4</skos:example>
		<skos:example>language comprehension is measured by the contrast of sum of rate, accuracy, fluency, and comprehension scaled scores trials in the Gray Oral Reading Test - 4</skos:example>
		<cito:citesForInformation rdf:resource="http://www.cognitiveatlas.org/citation/id/cit_4ded57332dc2d"/>
		<cito:citesForInformation rdf:resource="http://www.cognitiveatlas.org/citation/id/cit_4ded57b5106eb"/>
</skos:Concept><skos:Concept rdf:about="http://www.cognitiveatlas.org/id/tsk_4a57abb949aae"> <dc:identifier>tsk_4a57abb949aae</dc:identifier>
		<dc:Title>Cognitive Atlas : Lexicon : Hooper Visual Organization Test</dc:Title>
		<dc:Description>RDF output for 'Hooper Visual Organization Test'</dc:Description>
		<dc:Type>InteractiveResource</dc:Type>
		<dc:Publisher>Cognitive Atlas</dc:Publisher>
		<dc:Creator>Cognitive Atlas RDF Generator</dc:Creator>
		<dc:Contributor>Naomi Kenner</dc:Contributor>
		<dc:Date>2009-07-10 14:06:33</dc:Date>
		<dc:Format>text/rdf</dc:Format>
		<dc:Language>en</dc:Language>
		<skos:editorialNote>Generated by testgenall.php on Thu Mar 29 10:24:08 PDT 2012.</skos:editorialNote>
		<skos:historyNote>No previous definition revisions.</skos:historyNote>
		<skos:changeNote>This is the first and only definition provided.</skos:changeNote>
		<skos:scopeNote>http://www.w3.org/2004/02/skos/core#Concept</skos:scopeNote>
		<skos:Note>SKOS properties defined in http://www.w3.org/TR/skos-primer/#secrel</skos:Note>
		<skos:inScheme rdf:resource="http://www.cognitiveatlas.org/tasks/"/>
		<skos:definition>a neuropsychological test of visual spatial ability that presents participants with a line drawing of a common object that has been broken into fragments, and asks participants to name what the object would be if reassembled.</skos:definition>
		<skos:prefLabel>Hooper Visual Organization Test</skos:prefLabel>
		<skos:altLabel></skos:altLabel>
		<skos:related rdf:resource="http://www.cognitiveatlas.org/id/trm_4b82c75498408"/>
		<skos:related rdf:resource="http://www.cognitiveatlas.org/id/trm_4a3fd79d0aaa4"/>
		<skos:related rdf:resource="http://www.cognitiveatlas.org/id/trm_4a3fd79d0b4a9"/>
		<skos:related rdf:resource="http://www.cognitiveatlas.org/id/trm_4a3fd79d0b9ad"/>
		<skos:example>Central Coherence is measured by the contrast of accuracy trials in the Hooper Visual Organization Test</skos:example>
		<skos:example>object perception is measured by the contrast of accuracy trials in the Hooper Visual Organization Test</skos:example>
		<skos:example>visual object recognition is measured by the contrast of accuracy trials in the Hooper Visual Organization Test</skos:example>
		<skos:example>feature detection is measured by the contrast of accuracy trials in the Hooper Visual Organization Test</skos:example>
		<cito:citesForInformation rdf:resource="http://www.cognitiveatlas.org/citation/id/cit_4ded5aa586b91"/>
		<cito:citesForInformation rdf:resource="http://www.cognitiveatlas.org/citation/id/cit_4ded60908fe9f"/>
</skos:Concept><skos:Concept rdf:about="http://www.cognitiveatlas.org/id/tsk_4a57abb949abc"> <dc:identifier>tsk_4a57abb949abc</dc:identifier>
		<dc:Title>Cognitive Atlas : Lexicon : immediate recall test</dc:Title>
		<dc:Description>RDF output for 'immediate recall test'</dc:Description>
		<dc:Type>InteractiveResource</dc:Type>
		<dc:Publisher>Cognitive Atlas</dc:Publisher>
		<dc:Creator>Cognitive Atlas RDF Generator</dc:Creator>
		<dc:Contributor>Natalie Picchetti</dc:Contributor>
		<dc:Date>2011-03-04 12:55:55</dc:Date>
		<dc:Format>text/rdf</dc:Format>
		<dc:Language>en</dc:Language>
		<skos:editorialNote>Generated by testgenall.php on Thu Mar 29 10:24:08 PDT 2012.</skos:editorialNote>
		<skos:historyNote>Revision 2: 1 previous definitions.</skos:historyNote>
		<skos:changeNote>See http://www.cognitiveatlas.org/id/tsk_4a57abb949abc for complete revision history.</skos:changeNote>
		<skos:scopeNote>http://www.w3.org/2004/02/skos/core#Concept</skos:scopeNote>
		<skos:Note>SKOS properties defined in http://www.w3.org/TR/skos-primer/#secrel</skos:Note>
		<skos:inScheme rdf:resource="http://www.cognitiveatlas.org/tasks/"/>
		<skos:definition>involves presenting a subject with material that is to be memorized.  Once the material is removed the subject is to immediately demonstrate everything that they remember from the material.

</skos:definition>
		<skos:prefLabel>immediate recall test</skos:prefLabel>
		<skos:altLabel></skos:altLabel>
		<skos:related rdf:resource="http://www.cognitiveatlas.org/id/trm_4a3fd79d0b5a7"/>
		<skos:related rdf:resource="http://www.cognitiveatlas.org/id/trm_4a3fd79d0ba6c"/>
		<skos:related rdf:resource="http://www.cognitiveatlas.org/id/trm_4a3fd79d0a04f"/>
		<skos:related rdf:resource="http://www.cognitiveatlas.org/id/trm_4da63357e4999"/>
		<skos:example>immediate recall test is descended from Wechsler Memory Scale (revised)</skos:example>
		<skos:example>working memory is measured by the contrast of number or percentage of words remembered trials in the immediate recall test</skos:example>
		<skos:example>working memory retrieval is measured by the contrast of number or percentage of words remembered trials in the immediate recall test</skos:example>
		<skos:example>declarative memory is measured by the contrast of number or percentage of words remembered trials in the immediate recall test</skos:example>
		<cito:citesForInformation rdf:resource="http://www.cognitiveatlas.org/citation/id/cit_4dee5e76d4914"/>
		<cito:citesForInformation rdf:resource="http://www.cognitiveatlas.org/citation/id/cit_4dee5f971af95"/>
		<cito:citesForInformation rdf:resource="http://www.cognitiveatlas.org/citation/id/cit_4dee6011c4cdc"/>
</skos:Concept><skos:Concept rdf:about="http://www.cognitiveatlas.org/id/tsk_4a57abb949aca"> <dc:identifier>tsk_4a57abb949aca</dc:identifier>
		<dc:Title>Cognitive Atlas : Lexicon : International Affective Picture System</dc:Title>
		<dc:Description>RDF output for 'International Affective Picture System'</dc:Description>
		<dc:Type>InteractiveResource</dc:Type>
		<dc:Publisher>Cognitive Atlas</dc:Publisher>
		<dc:Creator>Cognitive Atlas RDF Generator</dc:Creator>
		<dc:Contributor>Brenda Gregory</dc:Contributor>
		<dc:Date>2011-05-10 14:46:45</dc:Date>
		<dc:Format>text/rdf</dc:Format>
		<dc:Language>en</dc:Language>
		<skos:editorialNote>Generated by testgenall.php on Thu Mar 29 10:24:08 PDT 2012.</skos:editorialNote>
		<skos:historyNote>Revision 3: 2 previous definitions.</skos:historyNote>
		<skos:changeNote>See http://www.cognitiveatlas.org/id/tsk_4a57abb949aca for complete revision history.</skos:changeNote>
		<skos:scopeNote>http://www.w3.org/2004/02/skos/core#Concept</skos:scopeNote>
		<skos:Note>SKOS properties defined in http://www.w3.org/TR/skos-primer/#secrel</skos:Note>
		<skos:inScheme rdf:resource="http://www.cognitiveatlas.org/tasks/"/>
		<skos:definition>a database of photographs used in emotion research.</skos:definition>
		<skos:prefLabel>International Affective Picture System</skos:prefLabel>
		<skos:altLabel></skos:altLabel>
		<skos:related rdf:resource="http://www.cognitiveatlas.org/id/trm_4a3fd79d0b65a"/>
		<skos:related rdf:resource="http://www.cognitiveatlas.org/id/trm_4c8a840d6f969"/>
		<skos:example>emotion perception is measured by the contrast of arousal in response to picture minus baseline arousal trials in the International Affective Picture System</skos:example>
		<skos:example>Subjective Emotional Picture Discrimination is a broader synonym of International Affective Picture System</skos:example>
		<cito:citesForInformation rdf:resource="http://www.cognitiveatlas.org/citation/id/cit_4dee84ea9e443"/>
		<cito:citesForInformation rdf:resource="http://www.cognitiveatlas.org/citation/id/cit_4deeb0ea55189"/>
		<cito:citesForInformation rdf:resource="http://www.cognitiveatlas.org/citation/id/cit_4deeb25602cb2"/>
</skos:Concept><skos:Concept rdf:about="http://www.cognitiveatlas.org/id/tsk_4a57abb949ad7"> <dc:identifier>tsk_4a57abb949ad7</dc:identifier>
		<dc:Title>Cognitive Atlas : Lexicon : Intradimensional shift task</dc:Title>
		<dc:Description>RDF output for 'Intradimensional shift task'</dc:Description>
		<dc:Type>InteractiveResource</dc:Type>
		<dc:Publisher>Cognitive Atlas</dc:Publisher>
		<dc:Creator>Cognitive Atlas RDF Generator</dc:Creator>
		<dc:Contributor>Agatha Lenartowicz</dc:Contributor>
		<dc:Date>2009-07-10 14:06:33</dc:Date>
		<dc:Format>text/rdf</dc:Format>
		<dc:Language>en</dc:Language>
		<skos:editorialNote>Generated by testgenall.php on Thu Mar 29 10:24:08 PDT 2012.</skos:editorialNote>
		<skos:historyNote>No previous definition revisions.</skos:historyNote>
		<skos:changeNote>This is the first and only definition provided.</skos:changeNote>
		<skos:scopeNote>http://www.w3.org/2004/02/skos/core#Concept</skos:scopeNote>
		<skos:Note>SKOS properties defined in http://www.w3.org/TR/skos-primer/#secrel</skos:Note>
		<skos:inScheme rdf:resource="http://www.cognitiveatlas.org/tasks/"/>
		<skos:definition>A task in which multiple (typically two) stimuli are presented simultaneously and the subject must select the stimulus that matches the currently relevant rule. The rule represents the relevant task &#34;dimension&#34;. The stimulus-response mappings within this dimension alternate or &#34;shift&#34; among multiple (typically two) alternatives. </skos:definition>
		<skos:prefLabel>Intradimensional shift task</skos:prefLabel>
		<skos:altLabel></skos:altLabel>
		<skos:related rdf:resource="http://www.cognitiveatlas.org/id/trm_4a3fd79d0ab65"/>
		<skos:related rdf:resource="http://www.cognitiveatlas.org/id/trm_4a3fd79d0b5fb"/>
		<skos:related rdf:resource="http://www.cognitiveatlas.org/id/tsk_4a57abb949dad"/>
		<skos:related rdf:resource="http://www.cognitiveatlas.org/id/trm_4a3fd79d0b607"/>
		<skos:related rdf:resource="http://www.cognitiveatlas.org/id/tsk_4a57abb949a5d"/>
		<skos:related rdf:resource="http://www.cognitiveatlas.org/id/tsk_4a57abb949f21"/>
		<skos:example>Intradimensional shift task is related to Extradimensional shift task</skos:example>
		<skos:example>Intradimensional shift task is a broader synonym of Wisconsin Card Sorting test</skos:example>
		<skos:example>pattern recognition is measured by the contrast of accuracy of subject minus average accuracy of controls trials in the Intradimensional shift task</skos:example>
		<skos:example>attention shifting is measured by the contrast of accuracy of subject minus average accuracy of controls trials in the Intradimensional shift task</skos:example>
		<skos:example>Set-shifting task is a broader synonym of Intradimensional shift task</skos:example>
		<skos:example>set shifting is measured by the contrast of accuracy of subject minus average accuracy of controls trials in the Intradimensional shift task</skos:example>
		<cito:citesForInformation rdf:resource="http://www.cognitiveatlas.org/citation/id/cit_4ded02531ead1"/>
		<cito:citesForInformation rdf:resource="http://www.cognitiveatlas.org/citation/id/cit_4df107788dc80"/>
		<cito:citesForInformation rdf:resource="http://www.cognitiveatlas.org/citation/id/cit_4df1081c042e8"/>
</skos:Concept><skos:Concept rdf:about="http://www.cognitiveatlas.org/id/tsk_4a57abb949ae5"> <dc:identifier>tsk_4a57abb949ae5</dc:identifier>
		<dc:Title>Cognitive Atlas : Lexicon : Iowa Gambling Task</dc:Title>
		<dc:Description>RDF output for 'Iowa Gambling Task'</dc:Description>
		<dc:Type>InteractiveResource</dc:Type>
		<dc:Publisher>Cognitive Atlas</dc:Publisher>
		<dc:Creator>Cognitive Atlas RDF Generator</dc:Creator>
		<dc:Contributor>Tom Schonberg</dc:Contributor>
		<dc:Date>2011-02-11 12:25:41</dc:Date>
		<dc:Format>text/rdf</dc:Format>
		<dc:Language>en</dc:Language>
		<skos:editorialNote>Generated by testgenall.php on Thu Mar 29 10:24:08 PDT 2012.</skos:editorialNote>
		<skos:historyNote>Revision 3: 2 previous definitions.</skos:historyNote>
		<skos:changeNote>See http://www.cognitiveatlas.org/id/tsk_4a57abb949ae5 for complete revision history.</skos:changeNote>
		<skos:scopeNote>http://www.w3.org/2004/02/skos/core#Concept</skos:scopeNote>
		<skos:Note>SKOS properties defined in http://www.w3.org/TR/skos-primer/#secrel</skos:Note>
		<skos:inScheme rdf:resource="http://www.cognitiveatlas.org/tasks/"/>
		<skos:definition>a widely used experiment in the areas of cognition &amp; emotion that was originally developed to assist in detecting decision-making impairment in patients with prefrontal cortex damage; a computerized experiment that is carried out in real time and resembles real-world contingencies. The task allows participants to select cards from four decks displayed on-screen. Participants are instructed that the selection of each card will result in winning or losing money. The objective is to attempt to win as much money as possible. (from http://iowagamblingtask.com/)

On each trial, participants select a card from one of four decks; two ‘bad’ decks offer a higher reward on most trials but also higher possible loss and lower overall expected value, whereas two ‘good’ decks offer a lower reward on most trials but lower possible loss and higher expected value. Participants learn the nature of the decks through trial-and- error. In some versions of the task, the probabilities are not stationary.</skos:definition>
		<skos:prefLabel>Iowa Gambling Task</skos:prefLabel>
		<skos:altLabel></skos:altLabel>
		<skos:related rdf:resource="http://www.cognitiveatlas.org/id/trm_4d54b2cc0f943"/>
		<skos:related rdf:resource="http://www.cognitiveatlas.org/id/trm_4a3fd79d0b64e"/>
		<skos:related rdf:resource="http://www.cognitiveatlas.org/id/trm_4d55a2bbcfdff"/>
		<skos:example>Iowa Gambling Task is a narrower synonym of Choice task between risky and non-risky options</skos:example>
		<skos:example>Cambridge Gambling Task is related to Iowa Gambling Task</skos:example>
		<skos:example>risk seeking is measured by the contrast of accuracy of subject minus average accuracy of controls trials in the Iowa Gambling Task</skos:example>
		<cito:citesForInformation rdf:resource="http://www.cognitiveatlas.org/citation/id/cit_4d559af0468e0"/>
		<cito:citesForInformation rdf:resource="http://www.cognitiveatlas.org/citation/id/cit_4d559b7391b2f"/>
		<cito:citesForInformation rdf:resource="http://www.cognitiveatlas.org/citation/id/cit_4df10ba550665"/>
</skos:Concept><skos:Concept rdf:about="http://www.cognitiveatlas.org/id/tsk_4a57abb949af3"> <dc:identifier>tsk_4a57abb949af3</dc:identifier>
		<dc:Title>Cognitive Atlas : Lexicon : Ishihara plates for color blindness</dc:Title>
		<dc:Description>RDF output for 'Ishihara plates for color blindness'</dc:Description>
		<dc:Type>InteractiveResource</dc:Type>
		<dc:Publisher>Cognitive Atlas</dc:Publisher>
		<dc:Creator>Cognitive Atlas RDF Generator</dc:Creator>
		<dc:Contributor>Brenda Gregory</dc:Contributor>
		<dc:Date>2011-04-28 16:07:09</dc:Date>
		<dc:Format>text/rdf</dc:Format>
		<dc:Language>en</dc:Language>
		<skos:editorialNote>Generated by testgenall.php on Thu Mar 29 10:24:08 PDT 2012.</skos:editorialNote>
		<skos:historyNote>Revision 3: 2 previous definitions.</skos:historyNote>
		<skos:changeNote>See http://www.cognitiveatlas.org/id/tsk_4a57abb949af3 for complete revision history.</skos:changeNote>
		<skos:scopeNote>http://www.w3.org/2004/02/skos/core#Concept</skos:scopeNote>
		<skos:Note>SKOS properties defined in http://www.w3.org/TR/skos-primer/#secrel</skos:Note>
		<skos:inScheme rdf:resource="http://www.cognitiveatlas.org/tasks/"/>
		<skos:definition>a test for red-green color deficiencies that consists of a number of colored plates, called Ishihara plates, each of which contain a circle of dots appearing randomized in color and size. Within the pattern are dots which form a number visible to those with normal color vision and invisible, or difficult to see, for those with a red-green color vision defect.</skos:definition>
		<skos:prefLabel>Ishihara plates for color blindness</skos:prefLabel>
		<skos:altLabel></skos:altLabel>
		<skos:related rdf:resource="http://www.cognitiveatlas.org/id/trm_4a3fd79d09d93"/>
		<skos:example>color perception is measured by the contrast of number of plates read correctly by controls with normal color vision minus number of plates read correctly by subject trials in the Ishihara plates for color blindness</skos:example>
		<cito:citesForInformation rdf:resource="http://www.cognitiveatlas.org/citation/id/cit_4df114bf31698"/>
		<cito:citesForInformation rdf:resource="http://www.cognitiveatlas.org/citation/id/cit_4df11508648d7"/>
</skos:Concept><skos:Concept rdf:about="http://www.cognitiveatlas.org/id/tsk_4a57abb949b00"> <dc:identifier>tsk_4a57abb949b00</dc:identifier>
		<dc:Title>Cognitive Atlas : Lexicon : Kanizsa figures</dc:Title>
		<dc:Description>RDF output for 'Kanizsa figures'</dc:Description>
		<dc:Type>InteractiveResource</dc:Type>
		<dc:Publisher>Cognitive Atlas</dc:Publisher>
		<dc:Creator>Cognitive Atlas RDF Generator</dc:Creator>
		<dc:Contributor>Brenda Gregory</dc:Contributor>
		<dc:Date>2011-05-16 15:44:40</dc:Date>
		<dc:Format>text/rdf</dc:Format>
		<dc:Language>en</dc:Language>
		<skos:editorialNote>Generated by testgenall.php on Thu Mar 29 10:24:08 PDT 2012.</skos:editorialNote>
		<skos:historyNote>Revision 3: 2 previous definitions.</skos:historyNote>
		<skos:changeNote>See http://www.cognitiveatlas.org/id/tsk_4a57abb949b00 for complete revision history.</skos:changeNote>
		<skos:scopeNote>http://www.w3.org/2004/02/skos/core#Concept</skos:scopeNote>
		<skos:Note>SKOS properties defined in http://www.w3.org/TR/skos-primer/#secrel</skos:Note>
		<skos:inScheme rdf:resource="http://www.cognitiveatlas.org/tasks/"/>
		<skos:definition>An ambiguous figure in which the illusory contour of a square (or triangle) appears in the middle of four (or three) truncated solid squares (or circles). It is an illustration of the perceptual ability to make sense of an incomplete figure by creating a &#39;whole&#39; image from the separate elements (Gestalt organization).</skos:definition>
		<skos:prefLabel>Kanizsa figures</skos:prefLabel>
		<skos:altLabel></skos:altLabel>
		<skos:related rdf:resource="http://www.cognitiveatlas.org/id/trm_4a3fd79d0b1a6"/>
		<skos:related rdf:resource="http://www.cognitiveatlas.org/id/trm_4a3fd79d0ab88"/>
		<skos:related rdf:resource="http://www.cognitiveatlas.org/id/trm_4a3fd79d0b9c5"/>
		<skos:related rdf:resource="http://www.cognitiveatlas.org/id/trm_4a3fd79d0b9c5"/>
		<skos:example>spatial ability is measured by the contrast of accuracy of participant minus average accuracy of controls trials in the Kanizsa figures</skos:example>
		<skos:example>perceptual binding is measured by the contrast of reaction time to figures minus reaction time to Kanizsa figures trials in the Kanizsa figures</skos:example>
		<skos:example> is measured by Kanizsa figures</skos:example>
		<skos:example> is measured by Kanizsa figures</skos:example>
		<cito:citesForInformation rdf:resource="http://www.cognitiveatlas.org/citation/id/cit_4df12ffac3c10"/>
		<cito:citesForInformation rdf:resource="http://www.cognitiveatlas.org/citation/id/cit_4df1318cdbaf1"/>
		<cito:citesForInformation rdf:resource="http://www.cognitiveatlas.org/citation/id/cit_4df131e0b8a48"/>
		<cito:citesForInformation rdf:resource="http://www.cognitiveatlas.org/citation/id/cit_4df132ea6863d"/>
</skos:Concept><skos:Concept rdf:about="http://www.cognitiveatlas.org/id/tsk_4a57abb949b0e"> <dc:identifier>tsk_4a57abb949b0e</dc:identifier>
		<dc:Title>Cognitive Atlas : Lexicon : letter fluency test </dc:Title>
		<dc:Description>RDF output for 'letter fluency test '</dc:Description>
		<dc:Type>InteractiveResource</dc:Type>
		<dc:Publisher>Cognitive Atlas</dc:Publisher>
		<dc:Creator>Cognitive Atlas RDF Generator</dc:Creator>
		<dc:Contributor>Natalie Picchetti</dc:Contributor>
		<dc:Date>2011-04-18 11:42:37</dc:Date>
		<dc:Format>text/rdf</dc:Format>
		<dc:Language>en</dc:Language>
		<skos:editorialNote>Generated by testgenall.php on Thu Mar 29 10:24:08 PDT 2012.</skos:editorialNote>
		<skos:historyNote>Revision 3: 2 previous definitions.</skos:historyNote>
		<skos:changeNote>See http://www.cognitiveatlas.org/id/tsk_4a57abb949b0e for complete revision history.</skos:changeNote>
		<skos:scopeNote>http://www.w3.org/2004/02/skos/core#Concept</skos:scopeNote>
		<skos:Note>SKOS properties defined in http://www.w3.org/TR/skos-primer/#secrel</skos:Note>
		<skos:inScheme rdf:resource="http://www.cognitiveatlas.org/tasks/"/>
		<skos:definition>is a test that requires generation of words cued with a specific letter and depends on phonemic abilities.
</skos:definition>
		<skos:prefLabel>letter fluency test </skos:prefLabel>
		<skos:altLabel></skos:altLabel>
		<skos:related rdf:resource="http://www.cognitiveatlas.org/id/trm_4a3fd79d0b802"/>
		<skos:related rdf:resource="http://www.cognitiveatlas.org/id/trm_4a3fd79d0a833"/>
		<skos:example>language processing is measured by the contrast of standard deviation from the mean population score in the language of the participant trials in the letter fluency test </skos:example>
		<skos:example>long term memory is measured by the contrast of standard deviation from the mean population score in the language of the participant trials in the letter fluency test </skos:example>
		<cito:citesForInformation rdf:resource="http://www.cognitiveatlas.org/citation/id/cit_4dac85c619a65"/>
</skos:Concept><skos:Concept rdf:about="http://www.cognitiveatlas.org/id/tsk_4a57abb949b1c"> <dc:identifier>tsk_4a57abb949b1c</dc:identifier>
		<dc:Title>Cognitive Atlas : Lexicon : letter n-back task</dc:Title>
		<dc:Description>RDF output for 'letter n-back task'</dc:Description>
		<dc:Type>InteractiveResource</dc:Type>
		<dc:Publisher>Cognitive Atlas</dc:Publisher>
		<dc:Creator>Cognitive Atlas RDF Generator</dc:Creator>
		<dc:Contributor>Agatha Lenartowicz</dc:Contributor>
		<dc:Date>2009-07-10 14:06:33</dc:Date>
		<dc:Format>text/rdf</dc:Format>
		<dc:Language>en</dc:Language>
		<skos:editorialNote>Generated by testgenall.php on Thu Mar 29 10:24:08 PDT 2012.</skos:editorialNote>
		<skos:historyNote>No previous definition revisions.</skos:historyNote>
		<skos:changeNote>This is the first and only definition provided.</skos:changeNote>
		<skos:scopeNote>http://www.w3.org/2004/02/skos/core#Concept</skos:scopeNote>
		<skos:Note>SKOS properties defined in http://www.w3.org/TR/skos-primer/#secrel</skos:Note>
		<skos:inScheme rdf:resource="http://www.cognitiveatlas.org/tasks/"/>
		<skos:definition>A task in which participants view a continuous stream of letter stimuli. The object of the task is to identify letter repetitions that occur n-trials preceding to the current stimulus.</skos:definition>
		<skos:prefLabel>letter n-back task</skos:prefLabel>
		<skos:altLabel></skos:altLabel>
		<skos:related rdf:resource="http://www.cognitiveatlas.org/id/tsk_4a57abb949a6a"/>
		<skos:related rdf:resource="http://www.cognitiveatlas.org/id/trm_4a3fd79d0ac9e"/>
		<skos:related rdf:resource="http://www.cognitiveatlas.org/id/tsk_4a57abb949bcd"/>
		<skos:example>letter n-back task is descended from n-back task</skos:example>
		<skos:example>face n-back task is related to letter n-back task</skos:example>
		<skos:example>phonological working memory is measured by the contrast of 3-back minus 0-back trials in the letter n-back task</skos:example>
		<cito:citesForInformation rdf:resource="http://www.cognitiveatlas.org/citation/id/cit_4e08f4c466c94"/>
</skos:Concept><skos:Concept rdf:about="http://www.cognitiveatlas.org/id/tsk_4a57abb949b2b"> <dc:identifier>tsk_4a57abb949b2b</dc:identifier>
		<dc:Title>Cognitive Atlas : Lexicon : Letter naming task</dc:Title>
		<dc:Description>RDF output for 'Letter naming task'</dc:Description>
		<dc:Type>InteractiveResource</dc:Type>
		<dc:Publisher>Cognitive Atlas</dc:Publisher>
		<dc:Creator>Cognitive Atlas RDF Generator</dc:Creator>
		<dc:Contributor>Russ Poldrack</dc:Contributor>
		<dc:Date>2012-01-28 08:28:24</dc:Date>
		<dc:Format>text/rdf</dc:Format>
		<dc:Language>en</dc:Language>
		<skos:editorialNote>Generated by testgenall.php on Thu Mar 29 10:24:08 PDT 2012.</skos:editorialNote>
		<skos:historyNote>Revision 3: 2 previous definitions.</skos:historyNote>
		<skos:changeNote>See http://www.cognitiveatlas.org/id/tsk_4a57abb949b2b for complete revision history.</skos:changeNote>
		<skos:scopeNote>http://www.w3.org/2004/02/skos/core#Concept</skos:scopeNote>
		<skos:Note>SKOS properties defined in http://www.w3.org/TR/skos-primer/#secrel</skos:Note>
		<skos:inScheme rdf:resource="http://www.cognitiveatlas.org/tasks/"/>
		<skos:definition>Participants are presented with letters and asked to give the name for each letter as it appears or as the researcher points to it.</skos:definition>
		<skos:prefLabel>Letter naming task</skos:prefLabel>
		<skos:altLabel>character naming task</skos:altLabel>
		<skos:related rdf:resource="http://www.cognitiveatlas.org/id/trm_4a3fd79d0a781"/>
		<skos:related rdf:resource="http://www.cognitiveatlas.org/id/trm_4a3fd79d09d35"/>
		<skos:example>language learning is measured by the contrast of accuracy of participant minus average accuracy of age-matched controls trials in the Letter naming task</skos:example>
		<skos:example>cognitive development is measured by the contrast of accuracy of participant minus average accuracy of age-matched controls trials in the Letter naming task</skos:example>
		<cito:citesForInformation rdf:resource="http://www.cognitiveatlas.org/citation/id/cit_4df14501ad200"/>
		<cito:citesForInformation rdf:resource="http://www.cognitiveatlas.org/citation/id/cit_4df14513864d2"/>
</skos:Concept><skos:Concept rdf:about="http://www.cognitiveatlas.org/id/tsk_4a57abb949b38"> <dc:identifier>tsk_4a57abb949b38</dc:identifier>
		<dc:Title>Cognitive Atlas : Lexicon : Lexical decision task</dc:Title>
		<dc:Description>RDF output for 'Lexical decision task'</dc:Description>
		<dc:Type>InteractiveResource</dc:Type>
		<dc:Publisher>Cognitive Atlas</dc:Publisher>
		<dc:Creator>Cognitive Atlas RDF Generator</dc:Creator>
		<dc:Contributor>Russ Poldrack</dc:Contributor>
		<dc:Date>2012-01-28 08:10:42</dc:Date>
		<dc:Format>text/rdf</dc:Format>
		<dc:Language>en</dc:Language>
		<skos:editorialNote>Generated by testgenall.php on Thu Mar 29 10:24:08 PDT 2012.</skos:editorialNote>
		<skos:historyNote>Revision 4: 3 previous definitions.</skos:historyNote>
		<skos:changeNote>See http://www.cognitiveatlas.org/id/tsk_4a57abb949b38 for complete revision history.</skos:changeNote>
		<skos:scopeNote>http://www.w3.org/2004/02/skos/core#Concept</skos:scopeNote>
		<skos:Note>SKOS properties defined in http://www.w3.org/TR/skos-primer/#secrel</skos:Note>
		<skos:inScheme rdf:resource="http://www.cognitiveatlas.org/tasks/"/>
		<skos:definition>a procedure used in many psychology and psycholinguistics experiments; the basic procedure involves measuring how quickly people classify stimuli as words or nonwords.  Subjects are presented, either visually or auditorily, with a mixture of words and pseudowords (nonsense strings that respect the phonotactic rules of a language, like trud in English). Their task is to indicate, usually with a button-press, whether the presented stimulus is a word or not.</skos:definition>
		<skos:prefLabel>Lexical decision task</skos:prefLabel>
		<skos:altLabel>word/nonword task</skos:altLabel>
		<skos:related rdf:resource="http://www.cognitiveatlas.org/id/trm_4a3fd79d0b80f"/>
		<skos:related rdf:resource="http://www.cognitiveatlas.org/id/trm_4a3fd79d0ba01"/>
		<skos:related rdf:resource="http://www.cognitiveatlas.org/id/trm_4a3fd79d0ba01"/>
		<skos:example>lexical access is measured by the contrast of Words - Pseudowords trials in the Lexical decision task</skos:example>
		<skos:example>memory retrieval is measured by the contrast of Words - Pseudowords trials in the Lexical decision task</skos:example>
		<skos:example>memory retrieval is measured by the contrast of Words - Consonant letter strings trials in the Lexical decision task</skos:example>
		<cito:citesForInformation rdf:resource="http://www.cognitiveatlas.org/citation/id/cit_4df245d4391f1"/>
		<cito:citesForInformation rdf:resource="http://www.cognitiveatlas.org/citation/id/cit_4df24785e5610"/>
</skos:Concept><skos:Concept rdf:about="http://www.cognitiveatlas.org/id/tsk_4a57abb949b46"> <dc:identifier>tsk_4a57abb949b46</dc:identifier>
		<dc:Title>Cognitive Atlas : Lexicon : matching pennies game </dc:Title>
		<dc:Description>RDF output for 'matching pennies game '</dc:Description>
		<dc:Type>InteractiveResource</dc:Type>
		<dc:Publisher>Cognitive Atlas</dc:Publisher>
		<dc:Creator>Cognitive Atlas RDF Generator</dc:Creator>
		<dc:Contributor>Russ Poldrack</dc:Contributor>
		<dc:Date>2012-01-28 11:32:14</dc:Date>
		<dc:Format>text/rdf</dc:Format>
		<dc:Language>en</dc:Language>
		<skos:editorialNote>Generated by testgenall.php on Thu Mar 29 10:24:08 PDT 2012.</skos:editorialNote>
		<skos:historyNote>Revision 4: 3 previous definitions.</skos:historyNote>
		<skos:changeNote>See http://www.cognitiveatlas.org/id/tsk_4a57abb949b46 for complete revision history.</skos:changeNote>
		<skos:scopeNote>http://www.w3.org/2004/02/skos/core#Concept</skos:scopeNote>
		<skos:Note>SKOS properties defined in http://www.w3.org/TR/skos-primer/#secrel</skos:Note>
		<skos:inScheme rdf:resource="http://www.cognitiveatlas.org/tasks/"/>
		<skos:definition>The game is played between two players, Player A and Player B. Each player has a penny and must secretly turn the penny to heads or tails. The players then reveal their choices simultaneously. If the pennies match (both heads or both tails), Player A receives one dollar from Player B (+1 for A, -1 for B). If the pennies do not match (one heads and one tails), Player B receives one dollar from Player A (-1 for A, +1 for B). This is an example of a zero-sum game, where one player&#39;s gain is exactly equal to the other player&#39;s loss.</skos:definition>
		<skos:prefLabel>matching pennies game </skos:prefLabel>
		<skos:altLabel>matching pennies task</skos:altLabel>
		<skos:related rdf:resource="http://www.cognitiveatlas.org/id/trm_4a3fd79d09e07"/>
		<skos:related rdf:resource="http://www.cognitiveatlas.org/id/trm_4a3fd79d0a81b"/>
		<skos:example>conditional reasoning is measured by the contrast of participant&#39;s responses vs. Nash equilibrium equation trials in the matching pennies game </skos:example>
		<skos:example>logical reasoning is measured by the contrast of participant&#39;s responses vs. Nash equilibrium equation trials in the matching pennies game </skos:example>
		<cito:citesForInformation rdf:resource="http://www.cognitiveatlas.org/citation/id/cit_4df2513bdd820"/>
		<cito:citesForInformation rdf:resource="http://www.cognitiveatlas.org/citation/id/cit_4e03b0e78ad83"/>
		<cito:citesForInformation rdf:resource="http://www.cognitiveatlas.org/citation/id/cit_4e03b24948722"/>
</skos:Concept><skos:Concept rdf:about="http://www.cognitiveatlas.org/id/tsk_4a57abb949b54"> <dc:identifier>tsk_4a57abb949b54</dc:identifier>
		<dc:Title>Cognitive Atlas : Lexicon : Maudsley Obsessive Compulsive Inventory</dc:Title>
		<dc:Description>RDF output for 'Maudsley Obsessive Compulsive Inventory'</dc:Description>
		<dc:Type>InteractiveResource</dc:Type>
		<dc:Publisher>Cognitive Atlas</dc:Publisher>
		<dc:Creator>Cognitive Atlas RDF Generator</dc:Creator>
		<dc:Contributor>Carinna Torgerson</dc:Contributor>
		<dc:Date>2011-06-10 11:05:03</dc:Date>
		<dc:Format>text/rdf</dc:Format>
		<dc:Language>en</dc:Language>
		<skos:editorialNote>Generated by testgenall.php on Thu Mar 29 10:24:08 PDT 2012.</skos:editorialNote>
		<skos:historyNote>Revision 4: 3 previous definitions.</skos:historyNote>
		<skos:changeNote>See http://www.cognitiveatlas.org/id/tsk_4a57abb949b54 for complete revision history.</skos:changeNote>
		<skos:scopeNote>http://www.w3.org/2004/02/skos/core#Concept</skos:scopeNote>
		<skos:Note>SKOS properties defined in http://www.w3.org/TR/skos-primer/#secrel</skos:Note>
		<skos:inScheme rdf:resource="http://www.cognitiveatlas.org/tasks/"/>
		<skos:definition>assess obsessive-compulsive symptoms in the areas of contamination fears and washing behaviors, checking, slowness, and doubting using 30 dichotomously scored (true/false) items, with each pathological response receiving a score of 1. </skos:definition>
		<skos:prefLabel>Maudsley Obsessive Compulsive Inventory</skos:prefLabel>
		<skos:altLabel></skos:altLabel>
		<skos:related rdf:resource="http://www.cognitiveatlas.org/id/trm_4a3fd79d09eb6"/>
		<skos:related rdf:resource="http://www.cognitiveatlas.org/id/trm_4a3fd79d0b05e"/>
		<skos:example>conventionality is measured by the contrast of subject score minus average normal score trials in the Maudsley Obsessive Compulsive Inventory</skos:example>
		<skos:example>self monitoring is measured by the contrast of subject score minus average normal score trials in the Maudsley Obsessive Compulsive Inventory</skos:example>
		<cito:citesForInformation rdf:resource="http://www.cognitiveatlas.org/citation/id/cit_4df25d595b92e"/>
		<cito:citesForInformation rdf:resource="http://www.cognitiveatlas.org/citation/id/cit_4df25edcae6b5"/>
</skos:Concept><skos:Concept rdf:about="http://www.cognitiveatlas.org/id/tsk_4a57abb949bb1"> <dc:identifier>tsk_4a57abb949bb1</dc:identifier>
		<dc:Title>Cognitive Atlas : Lexicon : Mini Mental State Examination</dc:Title>
		<dc:Description>RDF output for 'Mini Mental State Examination'</dc:Description>
		<dc:Type>InteractiveResource</dc:Type>
		<dc:Publisher>Cognitive Atlas</dc:Publisher>
		<dc:Creator>Cognitive Atlas RDF Generator</dc:Creator>
		<dc:Contributor>Tom Schonberg</dc:Contributor>
		<dc:Date>2010-03-11 08:36:33</dc:Date>
		<dc:Format>text/rdf</dc:Format>
		<dc:Language>en</dc:Language>
		<skos:editorialNote>Generated by testgenall.php on Thu Mar 29 10:24:08 PDT 2012.</skos:editorialNote>
		<skos:historyNote>Revision 2: 1 previous definitions.</skos:historyNote>
		<skos:changeNote>See http://www.cognitiveatlas.org/id/tsk_4a57abb949bb1 for complete revision history.</skos:changeNote>
		<skos:scopeNote>http://www.w3.org/2004/02/skos/core#Concept</skos:scopeNote>
		<skos:Note>SKOS properties defined in http://www.w3.org/TR/skos-primer/#secrel</skos:Note>
		<skos:inScheme rdf:resource="http://www.cognitiveatlas.org/tasks/"/>
		<skos:definition>The mini-mental state examination (MMSE) or Folstein test is a brief 30-point questionnaire test that is used to screen for cognitive impairment. It is commonly used in medicine to screen for dementia. It is also used to estimate the severity of cognitive impairment at a given point in time and to follow the course of cognitive changes in an individual over time, thus making it an effective way to document an individual&#39;s response to treatment.</skos:definition>
		<skos:prefLabel>Mini Mental State Examination</skos:prefLabel>
		<skos:altLabel></skos:altLabel>
		<skos:related rdf:resource="http://www.cognitiveatlas.org/id/trm_4aae62e4ad209"/>
		<skos:example>cognitive control is measured by the contrast of participant score minus average score trials in the Mini Mental State Examination</skos:example>
		<cito:citesForInformation rdf:resource="http://www.cognitiveatlas.org/citation/id/cit_4df28c4e797c3"/>
		<cito:citesForInformation rdf:resource="http://www.cognitiveatlas.org/citation/id/cit_4df28c65937eb"/>
</skos:Concept><skos:Concept rdf:about="http://www.cognitiveatlas.org/id/tsk_4a57abb949bbf"> <dc:identifier>tsk_4a57abb949bbf</dc:identifier>
		<dc:Title>Cognitive Atlas : Lexicon : motor sequencing task</dc:Title>
		<dc:Description>RDF output for 'motor sequencing task'</dc:Description>
		<dc:Type>InteractiveResource</dc:Type>
		<dc:Publisher>Cognitive Atlas</dc:Publisher>
		<dc:Creator>Cognitive Atlas RDF Generator</dc:Creator>
		<dc:Contributor>Carinna Torgerson</dc:Contributor>
		<dc:Date>2011-06-10 14:40:57</dc:Date>
		<dc:Format>text/rdf</dc:Format>
		<dc:Language>en</dc:Language>
		<skos:editorialNote>Generated by testgenall.php on Thu Mar 29 10:24:08 PDT 2012.</skos:editorialNote>
		<skos:historyNote>Revision 2: 1 previous definitions.</skos:historyNote>
		<skos:changeNote>See http://www.cognitiveatlas.org/id/tsk_4a57abb949bbf for complete revision history.</skos:changeNote>
		<skos:scopeNote>http://www.w3.org/2004/02/skos/core#Concept</skos:scopeNote>
		<skos:Note>SKOS properties defined in http://www.w3.org/TR/skos-primer/#secrel</skos:Note>
		<skos:inScheme rdf:resource="http://www.cognitiveatlas.org/tasks/"/>
		<skos:definition>Participants perform several motoric tasks in a specific sequence/order.</skos:definition>
		<skos:prefLabel>motor sequencing task</skos:prefLabel>
		<skos:altLabel></skos:altLabel>
		<skos:related rdf:resource="http://www.cognitiveatlas.org/id/trm_4a3fd79d0addc"/>
		<skos:related rdf:resource="http://www.cognitiveatlas.org/id/trm_4a3fd79d0addc"/>
		<skos:related rdf:resource="http://www.cognitiveatlas.org/id/trm_4a3fd79d0a972"/>
		<skos:related rdf:resource="http://www.cognitiveatlas.org/id/trm_4a3fd79d0b0bd"/>
		<skos:example>procedural memory is measured by the contrast of accuracy of participant minus average accuracy of controls trials in the motor sequencing task</skos:example>
		<skos:example>procedural memory is measured by the contrast of longest correct sequence of controls minus longest correct sequence of subject trials in the motor sequencing task</skos:example>
		<skos:example>motor control is measured by the contrast of accuracy of participant minus average accuracy of controls trials in the motor sequencing task</skos:example>
		<skos:example>serial processing is measured by the contrast of accuracy of participant minus average accuracy of controls trials in the motor sequencing task</skos:example>
		<cito:citesForInformation rdf:resource="http://www.cognitiveatlas.org/citation/id/cit_4df2913e55edf"/>
		<cito:citesForInformation rdf:resource="http://www.cognitiveatlas.org/citation/id/cit_4df2914d941c6"/>
</skos:Concept><skos:Concept rdf:about="http://www.cognitiveatlas.org/id/tsk_4a57abb949bcd"> <dc:identifier>tsk_4a57abb949bcd</dc:identifier>
		<dc:Title>Cognitive Atlas : Lexicon : n-back task</dc:Title>
		<dc:Description>RDF output for 'n-back task'</dc:Description>
		<dc:Type>InteractiveResource</dc:Type>
		<dc:Publisher>Cognitive Atlas</dc:Publisher>
		<dc:Creator>Cognitive Atlas RDF Generator</dc:Creator>
		<dc:Contributor>Russ Poldrack</dc:Contributor>
		<dc:Date>2012-01-28 07:31:26</dc:Date>
		<dc:Format>text/rdf</dc:Format>
		<dc:Language>en</dc:Language>
		<skos:editorialNote>Generated by testgenall.php on Thu Mar 29 10:24:08 PDT 2012.</skos:editorialNote>
		<skos:historyNote>Revision 2: 1 previous definitions.</skos:historyNote>
		<skos:changeNote>See http://www.cognitiveatlas.org/id/tsk_4a57abb949bcd for complete revision history.</skos:changeNote>
		<skos:scopeNote>http://www.w3.org/2004/02/skos/core#Concept</skos:scopeNote>
		<skos:Note>SKOS properties defined in http://www.w3.org/TR/skos-primer/#secrel</skos:Note>
		<skos:inScheme rdf:resource="http://www.cognitiveatlas.org/tasks/"/>
		<skos:definition>A task in which items (e.g., letters) are presented one at a time and participants must identify each item that repeats relative to the item that occurred &#34;n&#34; items before its onset.</skos:definition>
		<skos:prefLabel>n-back task</skos:prefLabel>
		<skos:altLabel>1-back task, 2-back task, 3-back task</skos:altLabel>
		<skos:related rdf:resource="http://www.cognitiveatlas.org/id/trm_4a3fd79d0b5a7"/>
		<skos:related rdf:resource="http://www.cognitiveatlas.org/id/trm_4a3fd79d0b5a7"/>
		<skos:related rdf:resource="http://www.cognitiveatlas.org/id/trm_4a3fd79d0b5a7"/>
		<skos:related rdf:resource="http://www.cognitiveatlas.org/id/trm_4a3fd79d0b5a7"/>
		<skos:related rdf:resource="http://www.cognitiveatlas.org/id/tsk_4a57abb949b1c"/>
		<skos:related rdf:resource="http://www.cognitiveatlas.org/id/tsk_4a57abb949a6a"/>
		<skos:related rdf:resource="http://www.cognitiveatlas.org/id/tsk_4a57abb949df1"/>
		<skos:related rdf:resource="http://www.cognitiveatlas.org/id/trm_4a3fd79d0990e"/>
		<skos:related rdf:resource="http://www.cognitiveatlas.org/id/trm_4b4a537644d76"/>
		<skos:example>n-back task is descended from Continuous Performance Task</skos:example>
		<skos:example>working memory is measured by the contrast of 1-back trials in the n-back task</skos:example>
		<skos:example>working memory is measured by the contrast of 2-back trials in the n-back task</skos:example>
		<skos:example>working memory is measured by the contrast of 3-back trials in the n-back task</skos:example>
		<skos:example>working memory is measured by the contrast of 3-back minus 1-back trials in the n-back task</skos:example>
		<skos:example>letter n-back task is descended from n-back task</skos:example>
		<skos:example>face n-back task is descended from n-back task</skos:example>
		<skos:example>spatial n-back task is descended from n-back task</skos:example>
		<skos:example>attention capacity is measured by the contrast of  trials in the n-back task</skos:example>
		<cito:citesForInformation rdf:resource="http://www.cognitiveatlas.org/citation/id/cit_4b4a52cc53998"/>
</skos:Concept><skos:Concept rdf:about="http://www.cognitiveatlas.org/id/tsk_4a57abb949bdb"> <dc:identifier>tsk_4a57abb949bdb</dc:identifier>
		<dc:Title>Cognitive Atlas : Lexicon : nine-hole peg test</dc:Title>
		<dc:Description>RDF output for 'nine-hole peg test'</dc:Description>
		<dc:Type>InteractiveResource</dc:Type>
		<dc:Publisher>Cognitive Atlas</dc:Publisher>
		<dc:Creator>Cognitive Atlas RDF Generator</dc:Creator>
		<dc:Contributor>Brenda Gregory</dc:Contributor>
		<dc:Date>2011-05-03 13:58:07</dc:Date>
		<dc:Format>text/rdf</dc:Format>
		<dc:Language>en</dc:Language>
		<skos:editorialNote>Generated by testgenall.php on Thu Mar 29 10:24:08 PDT 2012.</skos:editorialNote>
		<skos:historyNote>Revision 3: 2 previous definitions.</skos:historyNote>
		<skos:changeNote>See http://www.cognitiveatlas.org/id/tsk_4a57abb949bdb for complete revision history.</skos:changeNote>
		<skos:scopeNote>http://www.w3.org/2004/02/skos/core#Concept</skos:scopeNote>
		<skos:Note>SKOS properties defined in http://www.w3.org/TR/skos-primer/#secrel</skos:Note>
		<skos:inScheme rdf:resource="http://www.cognitiveatlas.org/tasks/"/>
		<skos:definition>a timed test of fine motor coordination; the test involves the subject placing 9 dowels in 9 holes. Subjects are scored on the amount of time it takes to place and remove all 9 pegs.</skos:definition>
		<skos:prefLabel>nine-hole peg test</skos:prefLabel>
		<skos:altLabel></skos:altLabel>
		<skos:related rdf:resource="http://www.cognitiveatlas.org/id/trm_4a3fd79d0aa8d"/>
		<skos:related rdf:resource="http://www.cognitiveatlas.org/id/trm_4a3fd79d0a97e"/>
		<skos:example>object manipulation is measured by the contrast of standard deviation from the mean score trials in the nine-hole peg test</skos:example>
		<skos:example>motor execution is measured by the contrast of standard deviation from the mean score trials in the nine-hole peg test</skos:example>
		<cito:citesForInformation rdf:resource="http://www.cognitiveatlas.org/citation/id/cit_4df29eab0576a"/>
		<cito:citesForInformation rdf:resource="http://www.cognitiveatlas.org/citation/id/cit_4df29eeb080d5"/>
</skos:Concept><skos:Concept rdf:about="http://www.cognitiveatlas.org/id/tsk_4a57abb949be9"> <dc:identifier>tsk_4a57abb949be9</dc:identifier>
		<dc:Title>Cognitive Atlas : Lexicon : object-discrimination task</dc:Title>
		<dc:Description>RDF output for 'object-discrimination task'</dc:Description>
		<dc:Type>InteractiveResource</dc:Type>
		<dc:Publisher>Cognitive Atlas</dc:Publisher>
		<dc:Creator>Cognitive Atlas RDF Generator</dc:Creator>
		<dc:Contributor>Carinna Torgerson</dc:Contributor>
		<dc:Date>2011-06-13 12:23:01</dc:Date>
		<dc:Format>text/rdf</dc:Format>
		<dc:Language>en</dc:Language>
		<skos:editorialNote>Generated by testgenall.php on Thu Mar 29 10:24:08 PDT 2012.</skos:editorialNote>
		<skos:historyNote>Revision 2: 1 previous definitions.</skos:historyNote>
		<skos:changeNote>See http://www.cognitiveatlas.org/id/tsk_4a57abb949be9 for complete revision history.</skos:changeNote>
		<skos:scopeNote>http://www.w3.org/2004/02/skos/core#Concept</skos:scopeNote>
		<skos:Note>SKOS properties defined in http://www.w3.org/TR/skos-primer/#secrel</skos:Note>
		<skos:inScheme rdf:resource="http://www.cognitiveatlas.org/tasks/"/>
		<skos:definition>Participants are shown pairs or sets of objects. Experimenters then try to discern whether the participant is able to discriminate between the objects. This can be done by having subjects match identical objects to each other, having certain objects become associated with rewards and measuring accuracy, or measuring time spent observing novel objects compared to time spent observing previously seen objects.</skos:definition>
		<skos:prefLabel>object-discrimination task</skos:prefLabel>
		<skos:altLabel></skos:altLabel>
		<skos:related rdf:resource="http://www.cognitiveatlas.org/id/trm_4a3fd79d0aaa4"/>
		<skos:related rdf:resource="http://www.cognitiveatlas.org/id/trm_4a3fd79d0aaa4"/>
		<skos:related rdf:resource="http://www.cognitiveatlas.org/id/trm_4a3fd79d0b4d8"/>
		<skos:related rdf:resource="http://www.cognitiveatlas.org/id/trm_4a3fd79d0b4d8"/>
		<skos:example>object perception is measured by the contrast of d&#39; (difference between correct identifications and false alarms) trials in the object-discrimination task</skos:example>
		<skos:example>object perception is measured by the contrast of accuracy of participant minus average accuracy of controls trials in the object-discrimination task</skos:example>
		<skos:example>visual working memory is measured by the contrast of d&#39; (difference between correct identifications and false alarms) trials in the object-discrimination task</skos:example>
		<skos:example>visual working memory is measured by the contrast of accuracy of participant minus average accuracy of controls trials in the object-discrimination task</skos:example>
		<cito:citesForInformation rdf:resource="http://www.cognitiveatlas.org/citation/id/cit_4df65f9b1b64d"/>
		<cito:citesForInformation rdf:resource="http://www.cognitiveatlas.org/citation/id/cit_4df661ab51a8e"/>
		<cito:citesForInformation rdf:resource="http://www.cognitiveatlas.org/citation/id/cit_4df6641e6fe17"/>
</skos:Concept><skos:Concept rdf:about="http://www.cognitiveatlas.org/id/tsk_4a57abb949bf6"> <dc:identifier>tsk_4a57abb949bf6</dc:identifier>
		<dc:Title>Cognitive Atlas : Lexicon : oddball task</dc:Title>
		<dc:Description>RDF output for 'oddball task'</dc:Description>
		<dc:Type>InteractiveResource</dc:Type>
		<dc:Publisher>Cognitive Atlas</dc:Publisher>
		<dc:Creator>Cognitive Atlas RDF Generator</dc:Creator>
		<dc:Contributor>Agatha Lenartowicz</dc:Contributor>
		<dc:Date>2009-07-10 14:06:33</dc:Date>
		<dc:Format>text/rdf</dc:Format>
		<dc:Language>en</dc:Language>
		<skos:editorialNote>Generated by testgenall.php on Thu Mar 29 10:24:08 PDT 2012.</skos:editorialNote>
		<skos:historyNote>No previous definition revisions.</skos:historyNote>
		<skos:changeNote>This is the first and only definition provided.</skos:changeNote>
		<skos:scopeNote>http://www.w3.org/2004/02/skos/core#Concept</skos:scopeNote>
		<skos:Note>SKOS properties defined in http://www.w3.org/TR/skos-primer/#secrel</skos:Note>
		<skos:inScheme rdf:resource="http://www.cognitiveatlas.org/tasks/"/>
		<skos:definition>A task in which stimuli are presented in a continuous stream and participants must detect the presence of an oddball stimulus. The oddball is a stimulus that occurs infrequently relative to all other stimuli, and has distinct characteristics (e.g., a different tone among auditory stimuli).</skos:definition>
		<skos:prefLabel>oddball task</skos:prefLabel>
		<skos:altLabel></skos:altLabel>
		<skos:related rdf:resource="http://www.cognitiveatlas.org/id/trm_4a3fd79d0990e"/>
		<skos:related rdf:resource="http://www.cognitiveatlas.org/id/trm_4a3fd79d09a10"/>
		<skos:related rdf:resource="http://www.cognitiveatlas.org/id/trm_4a3fd79d09a10"/>
		<skos:example>attention capacity is measured by the contrast of accuracy of participant minus average accuracy of controls trials in the oddball task</skos:example>
		<skos:example>auditory attention is measured by the contrast of ERP strength minus baseline trials in the oddball task</skos:example>
		<skos:example>auditory attention is measured by the contrast of areas of activation during task minus baseline trials in the oddball task</skos:example>
		<cito:citesForInformation rdf:resource="http://www.cognitiveatlas.org/citation/id/cit_4df6693e9a252"/>
		<cito:citesForInformation rdf:resource="http://www.cognitiveatlas.org/citation/id/cit_4df66a8c48455"/>
</skos:Concept><skos:Concept rdf:about="http://www.cognitiveatlas.org/id/tsk_4a57abb949c04"> <dc:identifier>tsk_4a57abb949c04</dc:identifier>
		<dc:Title>Cognitive Atlas : Lexicon : Pantomime Task</dc:Title>
		<dc:Description>RDF output for 'Pantomime Task'</dc:Description>
		<dc:Type>InteractiveResource</dc:Type>
		<dc:Publisher>Cognitive Atlas</dc:Publisher>
		<dc:Creator>Cognitive Atlas RDF Generator</dc:Creator>
		<dc:Contributor>Natalie Picchetti</dc:Contributor>
		<dc:Date>2011-02-28 12:42:09</dc:Date>
		<dc:Format>text/rdf</dc:Format>
		<dc:Language>en</dc:Language>
		<skos:editorialNote>Generated by testgenall.php on Thu Mar 29 10:24:08 PDT 2012.</skos:editorialNote>
		<skos:historyNote>Revision 2: 1 previous definitions.</skos:historyNote>
		<skos:changeNote>See http://www.cognitiveatlas.org/id/tsk_4a57abb949c04 for complete revision history.</skos:changeNote>
		<skos:scopeNote>http://www.w3.org/2004/02/skos/core#Concept</skos:scopeNote>
		<skos:Note>SKOS properties defined in http://www.w3.org/TR/skos-primer/#secrel</skos:Note>
		<skos:inScheme rdf:resource="http://www.cognitiveatlas.org/tasks/"/>
		<skos:definition>is when a subject is asked to explain an emotion or how an object is used by only gesturing with their hands and not using speech.  </skos:definition>
		<skos:prefLabel>Pantomime Task</skos:prefLabel>
		<skos:altLabel></skos:altLabel>
		<skos:related rdf:resource="http://www.cognitiveatlas.org/id/trm_4a3fd79d0a972"/>
		<skos:related rdf:resource="http://www.cognitiveatlas.org/id/trm_4a3fd79d0a72e"/>
		<skos:example>motor control is measured by the contrast of subject&#39;s pantomime ability compared to controls trials in the Pantomime Task</skos:example>
		<skos:example>kinaesthetic representation is measured by the contrast of subject&#39;s pantomime ability compared to controls trials in the Pantomime Task</skos:example>
		<cito:citesForInformation rdf:resource="http://www.cognitiveatlas.org/citation/id/cit_4df693bd8d433"/>
		<cito:citesForInformation rdf:resource="http://www.cognitiveatlas.org/citation/id/cit_4df694dc1f3c3"/>
		<cito:citesForInformation rdf:resource="http://www.cognitiveatlas.org/citation/id/cit_4df696ea5d317"/>
</skos:Concept><skos:Concept rdf:about="http://www.cognitiveatlas.org/id/tsk_4a57abb949ce9"> <dc:identifier>tsk_4a57abb949ce9</dc:identifier>
		<dc:Title>Cognitive Atlas : Lexicon : Parrott Scale</dc:Title>
		<dc:Description>RDF output for 'Parrott Scale'</dc:Description>
		<dc:Type>InteractiveResource</dc:Type>
		<dc:Publisher>Cognitive Atlas</dc:Publisher>
		<dc:Creator>Cognitive Atlas RDF Generator</dc:Creator>
		<dc:Contributor>System Administrator</dc:Contributor>
		<dc:Date>2009-07-10 14:06:33</dc:Date>
		<dc:Format>text/rdf</dc:Format>
		<dc:Language>en</dc:Language>
		<skos:editorialNote>Generated by testgenall.php on Thu Mar 29 10:24:08 PDT 2012.</skos:editorialNote>
		<skos:historyNote>No previous definition revisions.</skos:historyNote>
		<skos:changeNote>This is the first and only definition provided.</skos:changeNote>
		<skos:scopeNote>http://www.w3.org/2004/02/skos/core#Concept</skos:scopeNote>
		<skos:Note>SKOS properties defined in http://www.w3.org/TR/skos-primer/#secrel</skos:Note>
		<skos:inScheme rdf:resource="http://www.cognitiveatlas.org/tasks/"/>
		<skos:definition>No definition submitted yet</skos:definition>
		<skos:prefLabel>Parrott Scale</skos:prefLabel>
		<skos:altLabel></skos:altLabel>
		<cito:citesForInformation rdf:resource="http://www.cognitiveatlas.org/citation/id/cit_4e02769be854b"/>
</skos:Concept><skos:Concept rdf:about="http://www.cognitiveatlas.org/id/tsk_4a57abb949cfb"> <dc:identifier>tsk_4a57abb949cfb</dc:identifier>
		<dc:Title>Cognitive Atlas : Lexicon : picture naming task</dc:Title>
		<dc:Description>RDF output for 'picture naming task'</dc:Description>
		<dc:Type>InteractiveResource</dc:Type>
		<dc:Publisher>Cognitive Atlas</dc:Publisher>
		<dc:Creator>Cognitive Atlas RDF Generator</dc:Creator>
		<dc:Contributor>Carinna Torgerson</dc:Contributor>
		<dc:Date>2011-06-13 17:12:08</dc:Date>
		<dc:Format>text/rdf</dc:Format>
		<dc:Language>en</dc:Language>
		<skos:editorialNote>Generated by testgenall.php on Thu Mar 29 10:24:08 PDT 2012.</skos:editorialNote>
		<skos:historyNote>Revision 2: 1 previous definitions.</skos:historyNote>
		<skos:changeNote>See http://www.cognitiveatlas.org/id/tsk_4a57abb949cfb for complete revision history.</skos:changeNote>
		<skos:scopeNote>http://www.w3.org/2004/02/skos/core#Concept</skos:scopeNote>
		<skos:Note>SKOS properties defined in http://www.w3.org/TR/skos-primer/#secrel</skos:Note>
		<skos:inScheme rdf:resource="http://www.cognitiveatlas.org/tasks/"/>
		<skos:definition>participants are shown pictures of objects and asked to identify the item.</skos:definition>
		<skos:prefLabel>picture naming task</skos:prefLabel>
		<skos:altLabel></skos:altLabel>
		<skos:related rdf:resource="http://www.cognitiveatlas.org/id/trm_4a3fd79d0aab0"/>
		<skos:related rdf:resource="http://www.cognitiveatlas.org/id/trm_4a3fd79d0b4a9"/>
		<skos:related rdf:resource="http://www.cognitiveatlas.org/id/trm_4a3fd79d0b083"/>
		<skos:example>object recognition is measured by the contrast of accuracy of participant minus average accuracy of age-matched controls trials in the picture naming task</skos:example>
		<skos:example>visual object recognition is measured by the contrast of accuracy of participant minus average accuracy of age-matched controls trials in the picture naming task</skos:example>
		<skos:example>semantic memory is measured by the contrast of accuracy of participant minus average accuracy of age-matched controls trials in the picture naming task</skos:example>
		<cito:citesForInformation rdf:resource="http://www.cognitiveatlas.org/citation/id/cit_4df6a462e2cf6"/>
		<cito:citesForInformation rdf:resource="http://www.cognitiveatlas.org/citation/id/cit_4df6a698b3885"/>
</skos:Concept><skos:Concept rdf:about="http://www.cognitiveatlas.org/id/tsk_4a57abb949d09"> <dc:identifier>tsk_4a57abb949d09</dc:identifier>
		<dc:Title>Cognitive Atlas : Lexicon : Positive and Negative Affect Scale</dc:Title>
		<dc:Description>RDF output for 'Positive and Negative Affect Scale'</dc:Description>
		<dc:Type>InteractiveResource</dc:Type>
		<dc:Publisher>Cognitive Atlas</dc:Publisher>
		<dc:Creator>Cognitive Atlas RDF Generator</dc:Creator>
		<dc:Contributor>Carinna Torgerson</dc:Contributor>
		<dc:Date>2011-06-22 15:46:49</dc:Date>
		<dc:Format>text/rdf</dc:Format>
		<dc:Language>en</dc:Language>
		<skos:editorialNote>Generated by testgenall.php on Thu Mar 29 10:24:08 PDT 2012.</skos:editorialNote>
		<skos:historyNote>Revision 2: 1 previous definitions.</skos:historyNote>
		<skos:changeNote>See http://www.cognitiveatlas.org/id/tsk_4a57abb949d09 for complete revision history.</skos:changeNote>
		<skos:scopeNote>http://www.w3.org/2004/02/skos/core#Concept</skos:scopeNote>
		<skos:Note>SKOS properties defined in http://www.w3.org/TR/skos-primer/#secrel</skos:Note>
		<skos:inScheme rdf:resource="http://www.cognitiveatlas.org/tasks/"/>
		<skos:definition>A psychometric scale to measure positive and negative affects in individuals, and both as states and traits. Positive affect questions assess to what extent the participant is attentive, interested, alert, excited, enthusiastic, inspired, proud, determined, strong and active. Negative affect questions assess to what extent the participant is distressed, upset, hostile, irritable, scared, afraid, ashamed, guilty, nervous, and jittery. Participants answer questions on a Likert scale where 0=very, 1=slightly or not at all, 2=a little, 3=moderately, 4=quite a bit, and 5=very much. The questionnaire asks whether participants have felt these traits &#34;during the past few weeks&#34; (trait) and &#34;during the past few days&#34; (state).</skos:definition>
		<skos:prefLabel>Positive and Negative Affect Scale</skos:prefLabel>
		<skos:altLabel></skos:altLabel>
		<skos:related rdf:resource="http://www.cognitiveatlas.org/id/trm_4a3fd79d0a95a"/>
		<skos:related rdf:resource="http://www.cognitiveatlas.org/id/trm_4a3fd79d0b6ad"/>
		<skos:related rdf:resource="http://www.cognitiveatlas.org/id/trm_4a3fd79d0b014"/>
		<skos:example>mood is measured by the contrast of State Affect trials in the Positive and Negative Affect Scale</skos:example>
		<skos:example>happiness is measured by the contrast of standard deviation from the mean score trials in the Positive and Negative Affect Scale</skos:example>
		<skos:example>sadness is measured by the contrast of standard deviation from the mean score trials in the Positive and Negative Affect Scale</skos:example>
		<cito:citesForInformation rdf:resource="http://www.cognitiveatlas.org/citation/id/cit_4df7cda442d0f"/>
		<cito:citesForInformation rdf:resource="http://www.cognitiveatlas.org/citation/id/cit_4df7cf146311a"/>
		<cito:citesForInformation rdf:resource="http://www.cognitiveatlas.org/citation/id/cit_4e026f26b3fbe"/>
</skos:Concept><skos:Concept rdf:about="http://www.cognitiveatlas.org/id/tsk_4a57abb949d17"> <dc:identifier>tsk_4a57abb949d17</dc:identifier>
		<dc:Title>Cognitive Atlas : Lexicon : Posner cueing task</dc:Title>
		<dc:Description>RDF output for 'Posner cueing task'</dc:Description>
		<dc:Type>InteractiveResource</dc:Type>
		<dc:Publisher>Cognitive Atlas</dc:Publisher>
		<dc:Creator>Cognitive Atlas RDF Generator</dc:Creator>
		<dc:Contributor>Brenda Gregory</dc:Contributor>
		<dc:Date>2011-04-19 12:09:45</dc:Date>
		<dc:Format>text/rdf</dc:Format>
		<dc:Language>en</dc:Language>
		<skos:editorialNote>Generated by testgenall.php on Thu Mar 29 10:24:08 PDT 2012.</skos:editorialNote>
		<skos:historyNote>Revision 3: 2 previous definitions.</skos:historyNote>
		<skos:changeNote>See http://www.cognitiveatlas.org/id/tsk_4a57abb949d17 for complete revision history.</skos:changeNote>
		<skos:scopeNote>http://www.w3.org/2004/02/skos/core#Concept</skos:scopeNote>
		<skos:Note>SKOS properties defined in http://www.w3.org/TR/skos-primer/#secrel</skos:Note>
		<skos:inScheme rdf:resource="http://www.cognitiveatlas.org/tasks/"/>
		<skos:definition>Subjects view two stimuli (boxes, letters, etc.) and are cued by an arrow to attend to one of the stimuli.  Subjects then discriminate and respond (e.g., press a button when one of the boxes is filled with a diagonal cross, or press the left button for an &#34;X&#34; and the right button for an &#34;O&#34;). </skos:definition>
		<skos:prefLabel>Posner cueing task</skos:prefLabel>
		<skos:altLabel></skos:altLabel>
		<skos:related rdf:resource="http://www.cognitiveatlas.org/id/trm_4a3fd79d0b5ef"/>
		<skos:related rdf:resource="http://www.cognitiveatlas.org/id/trm_4a3fd79d0b5fb"/>
		<skos:related rdf:resource="http://www.cognitiveatlas.org/id/trm_4a3fd79d0a700"/>
		<skos:related rdf:resource="http://www.cognitiveatlas.org/id/trm_4a3fd79d0a700"/>
		<skos:related rdf:resource="http://www.cognitiveatlas.org/id/trm_4a3fd79d0ad41"/>
		<skos:related rdf:resource="http://www.cognitiveatlas.org/id/trm_4a3fd79d0ad41"/>
		<skos:example>attentional focusing is measured by the contrast of congruent response time - uncued response time trials in the Posner cueing task</skos:example>
		<skos:example>attention shifting is measured by the contrast of incongruent response time - congruent response time trials in the Posner cueing task</skos:example>
		<skos:example>involuntary attention is measured by the contrast of incongruent response time - congruent response time trials in the Posner cueing task</skos:example>
		<skos:example>involuntary attention is measured by the contrast of congruent response time - uncued response time trials in the Posner cueing task</skos:example>
		<skos:example>preattentive processing is measured by the contrast of incongruent response time - congruent response time trials in the Posner cueing task</skos:example>
		<skos:example>preattentive processing is measured by the contrast of congruent response time - uncued response time trials in the Posner cueing task</skos:example>
		<cito:citesForInformation rdf:resource="http://www.cognitiveatlas.org/citation/id/cit_4df8df56116bc"/>
		<cito:citesForInformation rdf:resource="http://www.cognitiveatlas.org/citation/id/cit_4df8dfa7b9a85"/>
</skos:Concept><skos:Concept rdf:about="http://www.cognitiveatlas.org/id/tsk_4a57abb949d25"> <dc:identifier>tsk_4a57abb949d25</dc:identifier>
		<dc:Title>Cognitive Atlas : Lexicon : Pseudoword naming task</dc:Title>
		<dc:Description>RDF output for 'Pseudoword naming task'</dc:Description>
		<dc:Type>InteractiveResource</dc:Type>
		<dc:Publisher>Cognitive Atlas</dc:Publisher>
		<dc:Creator>Cognitive Atlas RDF Generator</dc:Creator>
		<dc:Contributor>Russ Poldrack</dc:Contributor>
		<dc:Date>2012-01-28 07:26:45</dc:Date>
		<dc:Format>text/rdf</dc:Format>
		<dc:Language>en</dc:Language>
		<skos:editorialNote>Generated by testgenall.php on Thu Mar 29 10:24:08 PDT 2012.</skos:editorialNote>
		<skos:historyNote>Revision 3: 2 previous definitions.</skos:historyNote>
		<skos:changeNote>See http://www.cognitiveatlas.org/id/tsk_4a57abb949d25 for complete revision history.</skos:changeNote>
		<skos:scopeNote>http://www.w3.org/2004/02/skos/core#Concept</skos:scopeNote>
		<skos:Note>SKOS properties defined in http://www.w3.org/TR/skos-primer/#secrel</skos:Note>
		<skos:inScheme rdf:resource="http://www.cognitiveatlas.org/tasks/"/>
		<skos:definition>Participants are presented (usually one at a time, rather than in list form) with words and pseudowords, which are strings of letters that have no meaning in the language but are still pronounceable and asked to read aloud what they see. In pseudoword choice or decision tasks, they are asked to identify whether the items are words or not.</skos:definition>
		<skos:prefLabel>Pseudoword naming task</skos:prefLabel>
		<skos:altLabel>pseudoword reading task</skos:altLabel>
		<skos:related rdf:resource="http://www.cognitiveatlas.org/id/trm_4a3fd79d0b832"/>
		<skos:related rdf:resource="http://www.cognitiveatlas.org/id/trm_4a3fd79d0b826"/>
		<skos:related rdf:resource="http://www.cognitiveatlas.org/id/trm_4a3fd79d0b802"/>
		<skos:related rdf:resource="http://www.cognitiveatlas.org/id/trm_4a3fd79d0b802"/>
		<skos:example>morphological processing is measured by the contrast of Response time to morphologically non-decomposable pseudowords minus response time to morphologically decomposable psuedowords trials in the Pseudoword naming task</skos:example>
		<skos:example>lexical processing is measured by the contrast of response time to pseudowords minus response time to words trials in the Pseudoword naming task</skos:example>
		<skos:example>language processing is measured by the contrast of Response time to morphologically non-decomposable pseudowords minus response time to morphologically decomposable psuedowords trials in the Pseudoword naming task</skos:example>
		<skos:example>language processing is measured by the contrast of response time to pseudowords minus response time to words trials in the Pseudoword naming task</skos:example>
		<cito:citesForInformation rdf:resource="http://www.cognitiveatlas.org/citation/id/cit_4df8f763d6cce"/>
		<cito:citesForInformation rdf:resource="http://www.cognitiveatlas.org/citation/id/cit_4df8f886475cc"/>
		<cito:citesForInformation rdf:resource="http://www.cognitiveatlas.org/citation/id/cit_4df8f9a7a4e06"/>
</skos:Concept><skos:Concept rdf:about="http://www.cognitiveatlas.org/id/tsk_4a57abb949d32"> <dc:identifier>tsk_4a57abb949d32</dc:identifier>
		<dc:Title>Cognitive Atlas : Lexicon : pyramids and palm trees task</dc:Title>
		<dc:Description>RDF output for 'pyramids and palm trees task'</dc:Description>
		<dc:Type>InteractiveResource</dc:Type>
		<dc:Publisher>Cognitive Atlas</dc:Publisher>
		<dc:Creator>Cognitive Atlas RDF Generator</dc:Creator>
		<dc:Contributor>Russ Poldrack</dc:Contributor>
		<dc:Date>2012-01-28 12:08:21</dc:Date>
		<dc:Format>text/rdf</dc:Format>
		<dc:Language>en</dc:Language>
		<skos:editorialNote>Generated by testgenall.php on Thu Mar 29 10:24:08 PDT 2012.</skos:editorialNote>
		<skos:historyNote>Revision 5: 4 previous definitions.</skos:historyNote>
		<skos:changeNote>See http://www.cognitiveatlas.org/id/tsk_4a57abb949d32 for complete revision history.</skos:changeNote>
		<skos:scopeNote>http://www.w3.org/2004/02/skos/core#Concept</skos:scopeNote>
		<skos:Note>SKOS properties defined in http://www.w3.org/TR/skos-primer/#secrel</skos:Note>
		<skos:inScheme rdf:resource="http://www.cognitiveatlas.org/tasks/"/>
		<skos:definition>a semantic memory test that presents one word or picture above two others. The participant is then asked to identify which of the bottom items best matches the top item. Semantic memory is necessary for the identification of the analogies, which link conceptually two perceptually, and functionally distinct entities.</skos:definition>
		<skos:prefLabel>pyramids and palm trees task</skos:prefLabel>
		<skos:altLabel>palmtrees and pyramids task</skos:altLabel>
		<skos:related rdf:resource="http://www.cognitiveatlas.org/id/trm_4a3fd79d0b083"/>
		<skos:related rdf:resource="http://www.cognitiveatlas.org/id/trm_4a3fd79d0b083"/>
		<skos:related rdf:resource="http://www.cognitiveatlas.org/id/tsk_4a57abb949d92"/>
		<skos:example>semantic memory is measured by the contrast of accuracy of participant minus average accuracy of controls trials in the pyramids and palm trees task</skos:example>
		<skos:example>semantic memory is measured by the contrast of accuracy during task minus accuracy of some baseline test (like matching) trials in the pyramids and palm trees task</skos:example>
		<skos:example>semantic association task is a broader synonym of pyramids and palm trees task</skos:example>
		<cito:citesForInformation rdf:resource="http://www.cognitiveatlas.org/citation/id/cit_4dbaf245b2a5f"/>
		<cito:citesForInformation rdf:resource="http://www.cognitiveatlas.org/citation/id/cit_4df8ffca4dd99"/>
</skos:Concept><skos:Concept rdf:about="http://www.cognitiveatlas.org/id/tsk_4a57abb949d40"> <dc:identifier>tsk_4a57abb949d40</dc:identifier>
		<dc:Title>Cognitive Atlas : Lexicon : recognition memory test</dc:Title>
		<dc:Description>RDF output for 'recognition memory test'</dc:Description>
		<dc:Type>InteractiveResource</dc:Type>
		<dc:Publisher>Cognitive Atlas</dc:Publisher>
		<dc:Creator>Cognitive Atlas RDF Generator</dc:Creator>
		<dc:Contributor>Matt Craddock</dc:Contributor>
		<dc:Date>2011-10-03 05:51:10</dc:Date>
		<dc:Format>text/rdf</dc:Format>
		<dc:Language>en</dc:Language>
		<skos:editorialNote>Generated by testgenall.php on Thu Mar 29 10:24:08 PDT 2012.</skos:editorialNote>
		<skos:historyNote>Revision 3: 2 previous definitions.</skos:historyNote>
		<skos:changeNote>See http://www.cognitiveatlas.org/id/tsk_4a57abb949d40 for complete revision history.</skos:changeNote>
		<skos:scopeNote>http://www.w3.org/2004/02/skos/core#Concept</skos:scopeNote>
		<skos:Note>SKOS properties defined in http://www.w3.org/TR/skos-primer/#secrel</skos:Note>
		<skos:inScheme rdf:resource="http://www.cognitiveatlas.org/tasks/"/>
		<skos:definition>In a recognition memory test, a participant is presented with some or all of a set of &#34;old&#34; stimuli that were encoded earlier, as well as several &#34;new&#34; stimuli that were not previously presented. The participant&#39;s task is to indicate whether each stimulus is old or new. Responses in recognition memory tests are commonly sorted into four classes: Hits (&#34;old&#34; response to an old stimulus), Misses (&#34;new&#34; response to an old stimulus), False Alarms (&#34;old&#34; response to a new stimulus), and Correct Rejections (&#34;new&#34; response to a new stimulus). By comparing the percentage of responses that fall into each of these classes, the experimenter can assess both a participant&#39;s ability to discriminate between old and new stimuli, and his or her tendency to provide a particular response regardless of the type of stimulus presented. In many recognition memory tests, each old/new judgment is followed by a prompt asking participants to indicate either how confident they are in that old/new judgment, or what type of subjective experience was elicited by the stimulus being judged (e.g., was the old/new judgment accompanied by a vivid recollection of the encoding experience). This additional information can be used to generate and test more precise hypotheses about how recognition memory decisions are made.</skos:definition>
		<skos:prefLabel>recognition memory test</skos:prefLabel>
		<skos:altLabel>old-new recognition</skos:altLabel>
		<skos:related rdf:resource="http://www.cognitiveatlas.org/id/trm_4a3fd79d0ba6c"/>
		<skos:related rdf:resource="http://www.cognitiveatlas.org/id/trm_4b4a5ddfb90d0"/>
		<skos:related rdf:resource="http://www.cognitiveatlas.org/id/trm_4a3fd79d0a281"/>
		<skos:example>working memory retrieval is measured by the contrast of d&#39; (difference between correct identifications and false alarms) trials in the recognition memory test</skos:example>
		<skos:example> is related to recognition memory test</skos:example>
		<skos:example>explicit memory is measured by the contrast of  trials in the recognition memory test</skos:example>
		<cito:citesForInformation rdf:resource="http://www.cognitiveatlas.org/citation/id/cit_4df92bed4ead0"/>
		<cito:citesForInformation rdf:resource="http://www.cognitiveatlas.org/citation/id/cit_4df92e7490cf5"/>
</skos:Concept><skos:Concept rdf:about="http://www.cognitiveatlas.org/id/tsk_4a57abb949d4e"> <dc:identifier>tsk_4a57abb949d4e</dc:identifier>
		<dc:Title>Cognitive Atlas : Lexicon : reversal learning task</dc:Title>
		<dc:Description>RDF output for 'reversal learning task'</dc:Description>
		<dc:Type>InteractiveResource</dc:Type>
		<dc:Publisher>Cognitive Atlas</dc:Publisher>
		<dc:Creator>Cognitive Atlas RDF Generator</dc:Creator>
		<dc:Contributor>Carinna Torgerson</dc:Contributor>
		<dc:Date>2011-06-15 15:44:50</dc:Date>
		<dc:Format>text/rdf</dc:Format>
		<dc:Language>en</dc:Language>
		<skos:editorialNote>Generated by testgenall.php on Thu Mar 29 10:24:08 PDT 2012.</skos:editorialNote>
		<skos:historyNote>Revision 2: 1 previous definitions.</skos:historyNote>
		<skos:changeNote>See http://www.cognitiveatlas.org/id/tsk_4a57abb949d4e for complete revision history.</skos:changeNote>
		<skos:scopeNote>http://www.w3.org/2004/02/skos/core#Concept</skos:scopeNote>
		<skos:Note>SKOS properties defined in http://www.w3.org/TR/skos-primer/#secrel</skos:Note>
		<skos:inScheme rdf:resource="http://www.cognitiveatlas.org/tasks/"/>
		<skos:definition>&#34;Reversal learning involves the adaptation of behavior according to changes in stimulus–reward contingencies [...] [Reversal learning]is exemplified by visual discrimination tasks where subjects must learn to respond according to the opposite, previously irrelevant, stimulus–reward pairing.&#34; - (Clark, Cools, &amp; Robbins 2004)</skos:definition>
		<skos:prefLabel>reversal learning task</skos:prefLabel>
		<skos:altLabel></skos:altLabel>
		<skos:related rdf:resource="http://www.cognitiveatlas.org/id/trm_4a3fd79d09810"/>
		<skos:related rdf:resource="http://www.cognitiveatlas.org/id/trm_4a3fd79d0a64e"/>
		<skos:related rdf:resource="http://www.cognitiveatlas.org/id/trm_4a3fd79d0a585"/>
		<skos:related rdf:resource="http://www.cognitiveatlas.org/id/trm_4c8a8388de5ea"/>
		<skos:example>reversal learning task is a narrower synonym of Reward Task</skos:example>
		<skos:example>analogical reasoning is measured by the contrast of standard deviation from the mean accuracy score trials in the reversal learning task</skos:example>
		<skos:example>instrumental learning is measured by the contrast of gains minus losses trials in the reversal learning task</skos:example>
		<skos:example> is measured by reversal learning task</skos:example>
		<cito:citesForInformation rdf:resource="http://www.cognitiveatlas.org/citation/id/cit_4df935600837d"/>
		<cito:citesForInformation rdf:resource="http://www.cognitiveatlas.org/citation/id/cit_4df936686738e"/>
		<cito:citesForInformation rdf:resource="http://www.cognitiveatlas.org/citation/id/cit_4df939590cac6"/>
</skos:Concept><skos:Concept rdf:about="http://www.cognitiveatlas.org/id/tsk_4a57abb949d5b"> <dc:identifier>tsk_4a57abb949d5b</dc:identifier>
		<dc:Title>Cognitive Atlas : Lexicon : Risky Gains task</dc:Title>
		<dc:Description>RDF output for 'Risky Gains task'</dc:Description>
		<dc:Type>InteractiveResource</dc:Type>
		<dc:Publisher>Cognitive Atlas</dc:Publisher>
		<dc:Creator>Cognitive Atlas RDF Generator</dc:Creator>
		<dc:Contributor>Brenda Gregory</dc:Contributor>
		<dc:Date>2011-04-19 12:05:46</dc:Date>
		<dc:Format>text/rdf</dc:Format>
		<dc:Language>en</dc:Language>
		<skos:editorialNote>Generated by testgenall.php on Thu Mar 29 10:24:08 PDT 2012.</skos:editorialNote>
		<skos:historyNote>Revision 3: 2 previous definitions.</skos:historyNote>
		<skos:changeNote>See http://www.cognitiveatlas.org/id/tsk_4a57abb949d5b for complete revision history.</skos:changeNote>
		<skos:scopeNote>http://www.w3.org/2004/02/skos/core#Concept</skos:scopeNote>
		<skos:Note>SKOS properties defined in http://www.w3.org/TR/skos-primer/#secrel</skos:Note>
		<skos:inScheme rdf:resource="http://www.cognitiveatlas.org/tasks/"/>
		<skos:definition>Subjects are presented with a sequence of three numbers in ascending order (20, 40, and 80).  Each number is displayed onscreen for one second and, if the subject presses a button while that number is displayed, he/she receives that number of points along with immediate positive visual and auditory feedback.  When a 40 or 80 appears, however, there is a chance that it will appear in an alternate color, along with immediate negative feedback signaling a loss of 40 or 80 points, respectively.  When this occurs, the trial ends immediately (i.e. the subject may not make a response). </skos:definition>
		<skos:prefLabel>Risky Gains task</skos:prefLabel>
		<skos:altLabel></skos:altLabel>
		<skos:related rdf:resource="http://www.cognitiveatlas.org/id/trm_4a3fd79d0b64e"/>
		<skos:related rdf:resource="http://www.cognitiveatlas.org/id/trm_4d55a2bbcfdff"/>
		<skos:related rdf:resource="http://www.cognitiveatlas.org/id/trm_4d559bcd67c18"/>
		<skos:example>Risky Gains task is a narrower synonym of Choice task between risky and non-risky options</skos:example>
		<skos:example>Risky Gains task is related to Balloon Analogue Risk Task (BART)</skos:example>
		<skos:example>risk seeking is measured by the contrast of frequency of selecting the safe choice (20) minus frequency of selecting risky choices (40 and 80) trials in the Risky Gains task</skos:example>
		<cito:citesForInformation rdf:resource="http://www.cognitiveatlas.org/citation/id/cit_4d55937f7d27c"/>
		<cito:citesForInformation rdf:resource="http://www.cognitiveatlas.org/citation/id/cit_4dfa39dc35f8c"/>
</skos:Concept><skos:Concept rdf:about="http://www.cognitiveatlas.org/id/tsk_4a57abb949d69"> <dc:identifier>tsk_4a57abb949d69</dc:identifier>
		<dc:Title>Cognitive Atlas : Lexicon : Salthouse and Babcock Listening Span task </dc:Title>
		<dc:Description>RDF output for 'Salthouse and Babcock Listening Span task '</dc:Description>
		<dc:Type>InteractiveResource</dc:Type>
		<dc:Publisher>Cognitive Atlas</dc:Publisher>
		<dc:Creator>Cognitive Atlas RDF Generator</dc:Creator>
		<dc:Contributor>Carinna Torgerson</dc:Contributor>
		<dc:Date>2011-06-16 10:27:27</dc:Date>
		<dc:Format>text/rdf</dc:Format>
		<dc:Language>en</dc:Language>
		<skos:editorialNote>Generated by testgenall.php on Thu Mar 29 10:24:08 PDT 2012.</skos:editorialNote>
		<skos:historyNote>Revision 2: 1 previous definitions.</skos:historyNote>
		<skos:changeNote>See http://www.cognitiveatlas.org/id/tsk_4a57abb949d69 for complete revision history.</skos:changeNote>
		<skos:scopeNote>http://www.w3.org/2004/02/skos/core#Concept</skos:scopeNote>
		<skos:Note>SKOS properties defined in http://www.w3.org/TR/skos-primer/#secrel</skos:Note>
		<skos:inScheme rdf:resource="http://www.cognitiveatlas.org/tasks/"/>
		<skos:definition>Participants listen to an experimenter read a set of sentences. The participant must simultaneously respond to comprehension questions, and record or remember the last word of each sentence. The measure of &#34;listening span&#34; is then the number of correct words recalled.</skos:definition>
		<skos:prefLabel>Salthouse and Babcock Listening Span task </skos:prefLabel>
		<skos:altLabel></skos:altLabel>
		<skos:related rdf:resource="http://www.cognitiveatlas.org/id/trm_4c40d1d16071e"/>
		<skos:related rdf:resource="http://www.cognitiveatlas.org/id/trm_4a3fd79d0a116"/>
		<skos:related rdf:resource="http://www.cognitiveatlas.org/id/trm_4a3fd79d0a116"/>
		<skos:related rdf:resource="http://www.cognitiveatlas.org/id/trm_4a3fd79d0b892"/>
		<skos:related rdf:resource="http://www.cognitiveatlas.org/id/trm_4a3fd79d09b04"/>
		<skos:related rdf:resource="http://www.cognitiveatlas.org/id/trm_4a3fd79d09b04"/>
		<skos:related rdf:resource="http://www.cognitiveatlas.org/id/trm_4a3fd79d0971e"/>
		<skos:example>listening span task is a broader synonym of Salthouse and Babcock Listening Span task </skos:example>
		<skos:example>divided attention is measured by the contrast of listening span with comprehension questions minus listening span without trials in the Salthouse and Babcock Listening Span task </skos:example>
		<skos:example>divided attention is measured by the contrast of listening comprehension with listening span task minus listening comprehension without trials in the Salthouse and Babcock Listening Span task </skos:example>
		<skos:example>sentence comprehension is measured by the contrast of listening comprehension of participant minus average listening comprehension trials in the Salthouse and Babcock Listening Span task </skos:example>
		<skos:example>auditory working memory is measured by the contrast of listening span of participant minus average listening span trials in the Salthouse and Babcock Listening Span task </skos:example>
		<skos:example>auditory working memory is measured by the contrast of listening comprehension of participant minus average listening comprehension trials in the Salthouse and Babcock Listening Span task </skos:example>
		<skos:example>acoustic processing is measured by the contrast of listening comprehension of participant minus average listening comprehension trials in the Salthouse and Babcock Listening Span task </skos:example>
		<cito:citesForInformation rdf:resource="http://www.cognitiveatlas.org/citation/id/cit_4dfa3d944a118"/>
</skos:Concept><skos:Concept rdf:about="http://www.cognitiveatlas.org/id/tsk_4a57abb949d76"> <dc:identifier>tsk_4a57abb949d76</dc:identifier>
		<dc:Title>Cognitive Atlas : Lexicon : selective attention task</dc:Title>
		<dc:Description>RDF output for 'selective attention task'</dc:Description>
		<dc:Type>InteractiveResource</dc:Type>
		<dc:Publisher>Cognitive Atlas</dc:Publisher>
		<dc:Creator>Cognitive Atlas RDF Generator</dc:Creator>
		<dc:Contributor>Natalie Picchetti</dc:Contributor>
		<dc:Date>2011-05-18 15:32:32</dc:Date>
		<dc:Format>text/rdf</dc:Format>
		<dc:Language>en</dc:Language>
		<skos:editorialNote>Generated by testgenall.php on Thu Mar 29 10:24:08 PDT 2012.</skos:editorialNote>
		<skos:historyNote>Revision 5: 4 previous definitions.</skos:historyNote>
		<skos:changeNote>See http://www.cognitiveatlas.org/id/tsk_4a57abb949d76 for complete revision history.</skos:changeNote>
		<skos:scopeNote>http://www.w3.org/2004/02/skos/core#Concept</skos:scopeNote>
		<skos:Note>SKOS properties defined in http://www.w3.org/TR/skos-primer/#secrel</skos:Note>
		<skos:inScheme rdf:resource="http://www.cognitiveatlas.org/tasks/"/>
		<skos:definition>involves a participant to attend to a specific stimuli in the presence of competing stimuli.</skos:definition>
		<skos:prefLabel>selective attention task</skos:prefLabel>
		<skos:altLabel></skos:altLabel>
		<skos:related rdf:resource="http://www.cognitiveatlas.org/id/trm_4a3fd79d0a116"/>
		<skos:related rdf:resource="http://www.cognitiveatlas.org/id/trm_4a3fd79d0a116"/>
		<skos:related rdf:resource="http://www.cognitiveatlas.org/id/trm_4a3fd79d0a613"/>
		<skos:related rdf:resource="http://www.cognitiveatlas.org/id/trm_4a3fd79d0a613"/>
		<skos:related rdf:resource="http://www.cognitiveatlas.org/id/tsk_4a57abb949e27"/>
		<skos:example>selective attention task is a broader synonym of Stroop task</skos:example>
		<skos:example>divided attention is measured by the contrast of response time with competing stimuli minus response time with a single stimuli or congruent stimuli trials in the selective attention task</skos:example>
		<skos:example>divided attention is measured by the contrast of accuracy with a single stimuli or congruent stimuli minus accuracy with competing stimuli  trials in the selective attention task</skos:example>
		<skos:example>inhibition is measured by the contrast of response time with competing stimuli minus response time with a single stimuli or congruent stimuli trials in the selective attention task</skos:example>
		<skos:example>inhibition is measured by the contrast of accuracy with a single stimuli or congruent stimuli minus accuracy with competing stimuli  trials in the selective attention task</skos:example>
		<cito:citesForInformation rdf:resource="http://www.cognitiveatlas.org/citation/id/cit_4dfa469b10290"/>
		<cito:citesForInformation rdf:resource="http://www.cognitiveatlas.org/citation/id/cit_4dfa4c5702657"/>
		<cito:citesForInformation rdf:resource="http://www.cognitiveatlas.org/citation/id/cit_4dfa4ceb27d43"/>
</skos:Concept><skos:Concept rdf:about="http://www.cognitiveatlas.org/id/tsk_4a57abb949d84"> <dc:identifier>tsk_4a57abb949d84</dc:identifier>
		<dc:Title>Cognitive Atlas : Lexicon : semantic anomaly judgement task</dc:Title>
		<dc:Description>RDF output for 'semantic anomaly judgement task'</dc:Description>
		<dc:Type>InteractiveResource</dc:Type>
		<dc:Publisher>Cognitive Atlas</dc:Publisher>
		<dc:Creator>Cognitive Atlas RDF Generator</dc:Creator>
		<dc:Contributor>Carinna Torgerson</dc:Contributor>
		<dc:Date>2011-06-16 13:46:08</dc:Date>
		<dc:Format>text/rdf</dc:Format>
		<dc:Language>en</dc:Language>
		<skos:editorialNote>Generated by testgenall.php on Thu Mar 29 10:24:08 PDT 2012.</skos:editorialNote>
		<skos:historyNote>Revision 3: 2 previous definitions.</skos:historyNote>
		<skos:changeNote>See http://www.cognitiveatlas.org/id/tsk_4a57abb949d84 for complete revision history.</skos:changeNote>
		<skos:scopeNote>http://www.w3.org/2004/02/skos/core#Concept</skos:scopeNote>
		<skos:Note>SKOS properties defined in http://www.w3.org/TR/skos-primer/#secrel</skos:Note>
		<skos:inScheme rdf:resource="http://www.cognitiveatlas.org/tasks/"/>
		<skos:definition>Participants read or listen to sentences, then judge whether the sentence is plausible and makes sense semantically, or is implausible. Sentences may be structurally and gramatically correct, but the verb and noun are incompatible. Often, the structure or length of sentences varies to assess the role of working memory in any resulting deficit. </skos:definition>
		<skos:prefLabel>semantic anomaly judgement task</skos:prefLabel>
		<skos:altLabel></skos:altLabel>
		<skos:related rdf:resource="http://www.cognitiveatlas.org/id/trm_4a3fd79d0ac9e"/>
		<skos:related rdf:resource="http://www.cognitiveatlas.org/id/trm_4a3fd79d0b892"/>
		<skos:related rdf:resource="http://www.cognitiveatlas.org/id/trm_4a3fd79d0b87a"/>
		<skos:related rdf:resource="http://www.cognitiveatlas.org/id/trm_4a3fd79d0b87a"/>
		<skos:related rdf:resource="http://www.cognitiveatlas.org/id/trm_4a3fd79d0b340"/>
		<skos:example>phonological working memory is measured by the contrast of accuracy on semantically anomalous sentences minus accuracy on semantically correct sentences trials in the semantic anomaly judgement task</skos:example>
		<skos:example>sentence comprehension is measured by the contrast of d&#39; (difference between correct identifications and false alarms) trials in the semantic anomaly judgement task</skos:example>
		<skos:example>semantic processing is measured by the contrast of d&#39; (difference between correct identifications and false alarms) trials in the semantic anomaly judgement task</skos:example>
		<skos:example>semantic processing is measured by the contrast of accuracy on semantically anomalous sentences minus accuracy on semantically correct sentences trials in the semantic anomaly judgement task</skos:example>
		<skos:example>syntactic parsing is measured by the contrast of d&#39; (difference between correct identifications and false alarms) trials in the semantic anomaly judgement task</skos:example>
		<cito:citesForInformation rdf:resource="http://www.cognitiveatlas.org/citation/id/cit_4dfa617dc1de5"/>
		<cito:citesForInformation rdf:resource="http://www.cognitiveatlas.org/citation/id/cit_4dfa6925a6cd8"/>
</skos:Concept><skos:Concept rdf:about="http://www.cognitiveatlas.org/id/tsk_4a57abb949d92"> <dc:identifier>tsk_4a57abb949d92</dc:identifier>
		<dc:Title>Cognitive Atlas : Lexicon : semantic association task</dc:Title>
		<dc:Description>RDF output for 'semantic association task'</dc:Description>
		<dc:Type>InteractiveResource</dc:Type>
		<dc:Publisher>Cognitive Atlas</dc:Publisher>
		<dc:Creator>Cognitive Atlas RDF Generator</dc:Creator>
		<dc:Contributor>Russ Poldrack</dc:Contributor>
		<dc:Date>2012-01-28 07:34:55</dc:Date>
		<dc:Format>text/rdf</dc:Format>
		<dc:Language>en</dc:Language>
		<skos:editorialNote>Generated by testgenall.php on Thu Mar 29 10:24:08 PDT 2012.</skos:editorialNote>
		<skos:historyNote>Revision 3: 2 previous definitions.</skos:historyNote>
		<skos:changeNote>See http://www.cognitiveatlas.org/id/tsk_4a57abb949d92 for complete revision history.</skos:changeNote>
		<skos:scopeNote>http://www.w3.org/2004/02/skos/core#Concept</skos:scopeNote>
		<skos:Note>SKOS properties defined in http://www.w3.org/TR/skos-primer/#secrel</skos:Note>
		<skos:inScheme rdf:resource="http://www.cognitiveatlas.org/tasks/"/>
		<skos:definition>Participants are shown pairs of words or pictures and asked to identify if the items are semantically related.</skos:definition>
		<skos:prefLabel>semantic association task</skos:prefLabel>
		<skos:altLabel>semantic association judgment task</skos:altLabel>
		<skos:related rdf:resource="http://www.cognitiveatlas.org/id/trm_4a3fd79d0b87a"/>
		<skos:related rdf:resource="http://www.cognitiveatlas.org/id/trm_4a3fd79d0b26d"/>
		<skos:related rdf:resource="http://www.cognitiveatlas.org/id/tsk_4a57abb949d32"/>
		<skos:example>semantic association task is a broader synonym of pyramids and palm trees task</skos:example>
		<skos:example>semantic processing is measured by the contrast of accuracy of participant minus average accuracy of controls trials in the semantic association task</skos:example>
		<skos:example>spreading activation is measured by the contrast of ERP for related stimuli minus ERP for unrelated stimuli trials in the semantic association task</skos:example>
		<cito:citesForInformation rdf:resource="http://www.cognitiveatlas.org/citation/id/cit_4dfa6e830012d"/>
		<cito:citesForInformation rdf:resource="http://www.cognitiveatlas.org/citation/id/cit_4dfa6f8fb453c"/>
		<cito:citesForInformation rdf:resource="http://www.cognitiveatlas.org/citation/id/cit_4dfa71a07c7d3"/>
</skos:Concept><skos:Concept rdf:about="http://www.cognitiveatlas.org/id/tsk_4a57abb949d9f"> <dc:identifier>tsk_4a57abb949d9f</dc:identifier>
		<dc:Title>Cognitive Atlas : Lexicon : sentence completion test</dc:Title>
		<dc:Description>RDF output for 'sentence completion test'</dc:Description>
		<dc:Type>InteractiveResource</dc:Type>
		<dc:Publisher>Cognitive Atlas</dc:Publisher>
		<dc:Creator>Cognitive Atlas RDF Generator</dc:Creator>
		<dc:Contributor>Carinna Torgerson</dc:Contributor>
		<dc:Date>2011-06-27 13:45:49</dc:Date>
		<dc:Format>text/rdf</dc:Format>
		<dc:Language>en</dc:Language>
		<skos:editorialNote>Generated by testgenall.php on Thu Mar 29 10:24:08 PDT 2012.</skos:editorialNote>
		<skos:historyNote>Revision 4: 3 previous definitions.</skos:historyNote>
		<skos:changeNote>See http://www.cognitiveatlas.org/id/tsk_4a57abb949d9f for complete revision history.</skos:changeNote>
		<skos:scopeNote>http://www.w3.org/2004/02/skos/core#Concept</skos:scopeNote>
		<skos:Note>SKOS properties defined in http://www.w3.org/TR/skos-primer/#secrel</skos:Note>
		<skos:inScheme rdf:resource="http://www.cognitiveatlas.org/tasks/"/>
		<skos:definition>a test that provides respondents with beginnings of sentences, referred to as “stems,” and respondents then complete the sentences in ways that are meaningful to them. The responses are believed to provide indications of attitudes, beliefs, motivations, or other mental states. In a common version of this test, the Hayling Sentence Completion Test, a second condition is added, in which participants must complete the sentence with a word that makes no sense, requiring them to inhibit the semantically activated information.</skos:definition>
		<skos:prefLabel>sentence completion test</skos:prefLabel>
		<skos:altLabel></skos:altLabel>
		<skos:related rdf:resource="http://www.cognitiveatlas.org/id/trm_4da88c904862b"/>
		<skos:example>sentence completion test is a broader synonym of Hayling Sentence Completion Test</skos:example>
		<cito:citesForInformation rdf:resource="http://www.cognitiveatlas.org/citation/id/cit_4dfa763d3dc3a"/>
		<cito:citesForInformation rdf:resource="http://www.cognitiveatlas.org/citation/id/cit_4e08eff992b51"/>
		<cito:citesForInformation rdf:resource="http://www.cognitiveatlas.org/citation/id/cit_4e08f0cdb596c"/>
</skos:Concept><skos:Concept rdf:about="http://www.cognitiveatlas.org/id/tsk_4a57abb949dad"> <dc:identifier>tsk_4a57abb949dad</dc:identifier>
		<dc:Title>Cognitive Atlas : Lexicon : Set-shifting task</dc:Title>
		<dc:Description>RDF output for 'Set-shifting task'</dc:Description>
		<dc:Type>InteractiveResource</dc:Type>
		<dc:Publisher>Cognitive Atlas</dc:Publisher>
		<dc:Creator>Cognitive Atlas RDF Generator</dc:Creator>
		<dc:Contributor>Agatha Lenartowicz</dc:Contributor>
		<dc:Date>2009-07-30 17:14:34</dc:Date>
		<dc:Format>text/rdf</dc:Format>
		<dc:Language>en</dc:Language>
		<skos:editorialNote>Generated by testgenall.php on Thu Mar 29 10:24:08 PDT 2012.</skos:editorialNote>
		<skos:historyNote>No previous definition revisions.</skos:historyNote>
		<skos:changeNote>This is the first and only definition provided.</skos:changeNote>
		<skos:scopeNote>http://www.w3.org/2004/02/skos/core#Concept</skos:scopeNote>
		<skos:Note>SKOS properties defined in http://www.w3.org/TR/skos-primer/#secrel</skos:Note>
		<skos:inScheme rdf:resource="http://www.cognitiveatlas.org/tasks/"/>
		<skos:definition>A task in which participants alternate between two or more judgments typically regarding the same set of stimuli. Accuracy and reaction time are measured for each judgment.</skos:definition>
		<skos:prefLabel>Set-shifting task</skos:prefLabel>
		<skos:altLabel></skos:altLabel>
		<skos:related rdf:resource="http://www.cognitiveatlas.org/id/trm_4a3fd79d0ad9f"/>
		<skos:related rdf:resource="http://www.cognitiveatlas.org/id/trm_4a3fd79d0b613"/>
		<skos:related rdf:resource="http://www.cognitiveatlas.org/id/trm_4a3fd79d0b613"/>
		<skos:related rdf:resource="http://www.cognitiveatlas.org/id/trm_4a3fd79d0a431"/>
		<skos:related rdf:resource="http://www.cognitiveatlas.org/id/trm_4a3fd79d0b607"/>
		<skos:related rdf:resource="http://www.cognitiveatlas.org/id/trm_4a3fd79d0b5d7"/>
		<skos:related rdf:resource="http://www.cognitiveatlas.org/id/tsk_4a57abb949e8a"/>
		<skos:related rdf:resource="http://www.cognitiveatlas.org/id/tsk_4a57abb949f21"/>
		<skos:related rdf:resource="http://www.cognitiveatlas.org/id/tsk_4a57abb949a5d"/>
		<skos:related rdf:resource="http://www.cognitiveatlas.org/id/tsk_4a57abb949ad7"/>
		<skos:example>Set-shifting task is a broader synonym of Wisconsin Card Sorting test</skos:example>
		<skos:example>Set-shifting task is a broader synonym of Extradimensional shift task</skos:example>
		<skos:example>Set-shifting task is a broader synonym of Intradimensional shift task</skos:example>
		<skos:example> is measured by Set-shifting task</skos:example>
		<skos:example>task switching is measured by the contrast of accuracy of participant minus average accuracy of controls trials in the Set-shifting task</skos:example>
		<skos:example>task switching is measured by the contrast of perservative errors minus nonperservative errors trials in the Set-shifting task</skos:example>
		<skos:example>goal maintenance is measured by the contrast of accuracy of participant minus average accuracy of controls trials in the Set-shifting task</skos:example>
		<skos:example>set shifting is measured by the contrast of accuracy of participant minus average accuracy of controls trials in the Set-shifting task</skos:example>
		<skos:example>attention shift is measured by the contrast of accuracy of participant minus average accuracy of controls trials in the Set-shifting task</skos:example>
		<skos:example>task-switching  is related to Set-shifting task</skos:example>
		<cito:citesForInformation rdf:resource="http://www.cognitiveatlas.org/citation/id/cit_4dfa8004f1e80"/>
		<cito:citesForInformation rdf:resource="http://www.cognitiveatlas.org/citation/id/cit_4dfa8109612c3"/>
</skos:Concept><skos:Concept rdf:about="http://www.cognitiveatlas.org/id/tsk_4a57abb949dbb"> <dc:identifier>tsk_4a57abb949dbb</dc:identifier>
		<dc:Title>Cognitive Atlas : Lexicon : Simon task</dc:Title>
		<dc:Description>RDF output for 'Simon task'</dc:Description>
		<dc:Type>InteractiveResource</dc:Type>
		<dc:Publisher>Cognitive Atlas</dc:Publisher>
		<dc:Creator>Cognitive Atlas RDF Generator</dc:Creator>
		<dc:Contributor>Brenda Gregory</dc:Contributor>
		<dc:Date>2011-04-19 12:07:28</dc:Date>
		<dc:Format>text/rdf</dc:Format>
		<dc:Language>en</dc:Language>
		<skos:editorialNote>Generated by testgenall.php on Thu Mar 29 10:24:08 PDT 2012.</skos:editorialNote>
		<skos:historyNote>Revision 3: 2 previous definitions.</skos:historyNote>
		<skos:changeNote>See http://www.cognitiveatlas.org/id/tsk_4a57abb949dbb for complete revision history.</skos:changeNote>
		<skos:scopeNote>http://www.w3.org/2004/02/skos/core#Concept</skos:scopeNote>
		<skos:Note>SKOS properties defined in http://www.w3.org/TR/skos-primer/#secrel</skos:Note>
		<skos:inScheme rdf:resource="http://www.cognitiveatlas.org/tasks/"/>
		<skos:definition>Subjects view arrows presented in the right or left visual field that were pointing to the left or right.  Subjects respond via button press as to the direction of the arrow.  In incongruent stimuli, left-pointing arrows are seen on the right side, and vice versa. </skos:definition>
		<skos:prefLabel>Simon task</skos:prefLabel>
		<skos:altLabel></skos:altLabel>
		<skos:related rdf:resource="http://www.cognitiveatlas.org/id/trm_4a3fd79d0af66"/>
		<skos:related rdf:resource="http://www.cognitiveatlas.org/id/trm_4a3fd79d0a9a1"/>
		<skos:example>response inhibition is measured by the contrast of incongruent response time - congruent response time trials in the Simon task</skos:example>
		<skos:example>motor planning is measured by the contrast of accuracy to congruent cues minus accuracy to incongruent cues trials in the Simon task</skos:example>
		<cito:citesForInformation rdf:resource="http://www.cognitiveatlas.org/citation/id/cit_4dfa87d55075d"/>
		<cito:citesForInformation rdf:resource="http://www.cognitiveatlas.org/citation/id/cit_4dfa8bc1d4088"/>
</skos:Concept><skos:Concept rdf:about="http://www.cognitiveatlas.org/id/tsk_4a57abb949dc8"> <dc:identifier>tsk_4a57abb949dc8</dc:identifier>
		<dc:Title>Cognitive Atlas : Lexicon : simple reaction time task</dc:Title>
		<dc:Description>RDF output for 'simple reaction time task'</dc:Description>
		<dc:Type>InteractiveResource</dc:Type>
		<dc:Publisher>Cognitive Atlas</dc:Publisher>
		<dc:Creator>Cognitive Atlas RDF Generator</dc:Creator>
		<dc:Contributor>Brenda Gregory</dc:Contributor>
		<dc:Date>2011-04-29 16:14:21</dc:Date>
		<dc:Format>text/rdf</dc:Format>
		<dc:Language>en</dc:Language>
		<skos:editorialNote>Generated by testgenall.php on Thu Mar 29 10:24:08 PDT 2012.</skos:editorialNote>
		<skos:historyNote>Revision 3: 2 previous definitions.</skos:historyNote>
		<skos:changeNote>See http://www.cognitiveatlas.org/id/tsk_4a57abb949dc8 for complete revision history.</skos:changeNote>
		<skos:scopeNote>http://www.w3.org/2004/02/skos/core#Concept</skos:scopeNote>
		<skos:Note>SKOS properties defined in http://www.w3.org/TR/skos-primer/#secrel</skos:Note>
		<skos:inScheme rdf:resource="http://www.cognitiveatlas.org/tasks/"/>
		<skos:definition>task that assesses the ability of the subject to respond to an external cue and retrieve a reward.</skos:definition>
		<skos:prefLabel>simple reaction time task</skos:prefLabel>
		<skos:altLabel></skos:altLabel>
		<skos:related rdf:resource="http://www.cognitiveatlas.org/id/trm_4a3fd79d0a972"/>
		<skos:example>motor control is measured by the contrast of reaction time of participant minus average reaction time of controls trials in the simple reaction time task</skos:example>
		<cito:citesForInformation rdf:resource="http://www.cognitiveatlas.org/citation/id/cit_4dfa8e7314757"/>
		<cito:citesForInformation rdf:resource="http://www.cognitiveatlas.org/citation/id/cit_4dfa907a5d7bb"/>
</skos:Concept><skos:Concept rdf:about="http://www.cognitiveatlas.org/id/tsk_4a57abb949dd6"> <dc:identifier>tsk_4a57abb949dd6</dc:identifier>
		<dc:Title>Cognitive Atlas : Lexicon : source memory test</dc:Title>
		<dc:Description>RDF output for 'source memory test'</dc:Description>
		<dc:Type>InteractiveResource</dc:Type>
		<dc:Publisher>Cognitive Atlas</dc:Publisher>
		<dc:Creator>Cognitive Atlas RDF Generator</dc:Creator>
		<dc:Contributor>Carinna Torgerson</dc:Contributor>
		<dc:Date>2011-06-16 16:41:32</dc:Date>
		<dc:Format>text/rdf</dc:Format>
		<dc:Language>en</dc:Language>
		<skos:editorialNote>Generated by testgenall.php on Thu Mar 29 10:24:08 PDT 2012.</skos:editorialNote>
		<skos:historyNote>Revision 2: 1 previous definitions.</skos:historyNote>
		<skos:changeNote>See http://www.cognitiveatlas.org/id/tsk_4a57abb949dd6 for complete revision history.</skos:changeNote>
		<skos:scopeNote>http://www.w3.org/2004/02/skos/core#Concept</skos:scopeNote>
		<skos:Note>SKOS properties defined in http://www.w3.org/TR/skos-primer/#secrel</skos:Note>
		<skos:inScheme rdf:resource="http://www.cognitiveatlas.org/tasks/"/>
		<skos:definition>Participants are shown a list or series of items (words, pictures, objects). Later, when shown an item, they are asked whether it has was shown to them before, and if they respond affirmatively, they are asked a question about the source of the item. The source question could be what the spatial location of the item was, what color it appeared in, or which list or set it belonged to.</skos:definition>
		<skos:prefLabel>source memory test</skos:prefLabel>
		<skos:altLabel></skos:altLabel>
		<skos:related rdf:resource="http://www.cognitiveatlas.org/id/trm_4a3fd79d0b18f"/>
		<skos:related rdf:resource="http://www.cognitiveatlas.org/id/trm_4a3fd79d0b18f"/>
		<skos:related rdf:resource="http://www.cognitiveatlas.org/id/trm_4a3fd79d09e87"/>
		<skos:related rdf:resource="http://www.cognitiveatlas.org/id/trm_4a3fd79d0b49e"/>
		<skos:related rdf:resource="http://www.cognitiveatlas.org/id/trm_4a3fd79d0b1d5"/>
		<skos:example>source memory is measured by the contrast of d&#39; (difference between correct identifications and false alarms) trials in the source memory test</skos:example>
		<skos:example>source memory is measured by the contrast of accuracy of recognition minus accuracy of source identification trials in the source memory test</skos:example>
		<skos:example>context memory is measured by the contrast of accuracy of recognition minus accuracy of source identification trials in the source memory test</skos:example>
		<skos:example>visual memory is measured by the contrast of accuracy of recognition minus accuracy of source identification trials in the source memory test</skos:example>
		<skos:example>spatial memory is measured by the contrast of accuracy of recognition minus accuracy of source identification trials in the source memory test</skos:example>
		<cito:citesForInformation rdf:resource="http://www.cognitiveatlas.org/citation/id/cit_4dfa9394d15a1"/>
		<cito:citesForInformation rdf:resource="http://www.cognitiveatlas.org/citation/id/cit_4dfa93ff7f8f2"/>
</skos:Concept><skos:Concept rdf:about="http://www.cognitiveatlas.org/id/tsk_4a57abb949de3"> <dc:identifier>tsk_4a57abb949de3</dc:identifier>
		<dc:Title>Cognitive Atlas : Lexicon : Span/Supra-Span Test</dc:Title>
		<dc:Description>RDF output for 'Span/Supra-Span Test'</dc:Description>
		<dc:Type>InteractiveResource</dc:Type>
		<dc:Publisher>Cognitive Atlas</dc:Publisher>
		<dc:Creator>Cognitive Atlas RDF Generator</dc:Creator>
		<dc:Contributor>Carinna Torgerson</dc:Contributor>
		<dc:Date>2011-06-27 14:39:10</dc:Date>
		<dc:Format>text/rdf</dc:Format>
		<dc:Language>en</dc:Language>
		<skos:editorialNote>Generated by testgenall.php on Thu Mar 29 10:24:08 PDT 2012.</skos:editorialNote>
		<skos:historyNote>Revision 2: 1 previous definitions.</skos:historyNote>
		<skos:changeNote>See http://www.cognitiveatlas.org/id/tsk_4a57abb949de3 for complete revision history.</skos:changeNote>
		<skos:scopeNote>http://www.w3.org/2004/02/skos/core#Concept</skos:scopeNote>
		<skos:Note>SKOS properties defined in http://www.w3.org/TR/skos-primer/#secrel</skos:Note>
		<skos:inScheme rdf:resource="http://www.cognitiveatlas.org/tasks/"/>
		<skos:definition>Participants are given sequences to recall that exceed their working memory span, usually by about 2 items, however the sequence contains a smaller repeating sequence(s) among the non-repeating items.</skos:definition>
		<skos:prefLabel>Span/Supra-Span Test</skos:prefLabel>
		<skos:altLabel></skos:altLabel>
		<skos:related rdf:resource="http://www.cognitiveatlas.org/id/trm_4a3fd79d09cae"/>
		<skos:related rdf:resource="http://www.cognitiveatlas.org/id/trm_4a3fd79d0b0a6"/>
		<skos:related rdf:resource="http://www.cognitiveatlas.org/id/trm_4a3fd79d09d64"/>
		<skos:related rdf:resource="http://www.cognitiveatlas.org/id/trm_4a3fd79d0b5a7"/>
		<skos:related rdf:resource="http://www.cognitiveatlas.org/id/tsk_4a57abb949a0d"/>
		<skos:related rdf:resource="http://www.cognitiveatlas.org/id/trm_4da881dace79c"/>
		<skos:example>Span/Supra-Span Test is related to Digit span task</skos:example>
		<skos:example>Span/Supra-Span Test is related to Corsi Blocks</skos:example>
		<skos:example>chunking is measured by the contrast of supra-span minus span trials in the Span/Supra-Span Test</skos:example>
		<skos:example>sequence learning is measured by the contrast of supra-span minus span trials in the Span/Supra-Span Test</skos:example>
		<skos:example>cognitive load is measured by the contrast of supra-span minus span trials in the Span/Supra-Span Test</skos:example>
		<skos:example>working memory is measured by the contrast of supra-span minus span trials in the Span/Supra-Span Test</skos:example>
		<cito:citesForInformation rdf:resource="http://www.cognitiveatlas.org/citation/id/cit_4dfa97d8ba519"/>
		<cito:citesForInformation rdf:resource="http://www.cognitiveatlas.org/citation/id/cit_4e08fb6c66845"/>
</skos:Concept><skos:Concept rdf:about="http://www.cognitiveatlas.org/id/tsk_4a57abb949df1"> <dc:identifier>tsk_4a57abb949df1</dc:identifier>
		<dc:Title>Cognitive Atlas : Lexicon : spatial n-back task</dc:Title>
		<dc:Description>RDF output for 'spatial n-back task'</dc:Description>
		<dc:Type>InteractiveResource</dc:Type>
		<dc:Publisher>Cognitive Atlas</dc:Publisher>
		<dc:Creator>Cognitive Atlas RDF Generator</dc:Creator>
		<dc:Contributor>Carinna Torgerson</dc:Contributor>
		<dc:Date>2011-06-17 11:08:47</dc:Date>
		<dc:Format>text/rdf</dc:Format>
		<dc:Language>en</dc:Language>
		<skos:editorialNote>Generated by testgenall.php on Thu Mar 29 10:24:08 PDT 2012.</skos:editorialNote>
		<skos:historyNote>Revision 2: 1 previous definitions.</skos:historyNote>
		<skos:changeNote>See http://www.cognitiveatlas.org/id/tsk_4a57abb949df1 for complete revision history.</skos:changeNote>
		<skos:scopeNote>http://www.w3.org/2004/02/skos/core#Concept</skos:scopeNote>
		<skos:Note>SKOS properties defined in http://www.w3.org/TR/skos-primer/#secrel</skos:Note>
		<skos:inScheme rdf:resource="http://www.cognitiveatlas.org/tasks/"/>
		<skos:definition>Participants view a configuration of dots and must indicate whether the dot is in the same position as the dot in the picture presented n previously (0,1,2,or 3). In some variations, participants are asked to identify the location of the dot n pictures back, rather than indicating if the current dot matches.</skos:definition>
		<skos:prefLabel>spatial n-back task</skos:prefLabel>
		<skos:altLabel></skos:altLabel>
		<skos:related rdf:resource="http://www.cognitiveatlas.org/id/tsk_4a57abb949a6a"/>
		<skos:related rdf:resource="http://www.cognitiveatlas.org/id/trm_4a3fd79d0b1e0"/>
		<skos:related rdf:resource="http://www.cognitiveatlas.org/id/trm_4a3fd79d0b1a6"/>
		<skos:related rdf:resource="http://www.cognitiveatlas.org/id/tsk_4a57abb949bcd"/>
		<skos:example>spatial n-back task is descended from n-back task</skos:example>
		<skos:example>face n-back task is related to spatial n-back task</skos:example>
		<skos:example>spatial working memory is measured by the contrast of 3-back minus 0-back trials in the spatial n-back task</skos:example>
		<skos:example>spatial ability is measured by the contrast of 0-back trials in the spatial n-back task</skos:example>
		<cito:citesForInformation rdf:resource="http://www.cognitiveatlas.org/citation/id/cit_4dfb954b627ed"/>
		<cito:citesForInformation rdf:resource="http://www.cognitiveatlas.org/citation/id/cit_4dfb986b0c680"/>
		<cito:citesForInformation rdf:resource="http://www.cognitiveatlas.org/citation/id/cit_4dfb99fe9d289"/>
</skos:Concept><skos:Concept rdf:about="http://www.cognitiveatlas.org/id/tsk_4a57abb949dfe"> <dc:identifier>tsk_4a57abb949dfe</dc:identifier>
		<dc:Title>Cognitive Atlas : Lexicon : Spielberger's State-Trait Anxiety Questionnaire</dc:Title>
		<dc:Description>RDF output for 'Spielberger's State-Trait Anxiety Questionnaire'</dc:Description>
		<dc:Type>InteractiveResource</dc:Type>
		<dc:Publisher>Cognitive Atlas</dc:Publisher>
		<dc:Creator>Cognitive Atlas RDF Generator</dc:Creator>
		<dc:Contributor>Brenda Gregory</dc:Contributor>
		<dc:Date>2011-04-28 16:17:36</dc:Date>
		<dc:Format>text/rdf</dc:Format>
		<dc:Language>en</dc:Language>
		<skos:editorialNote>Generated by testgenall.php on Thu Mar 29 10:24:08 PDT 2012.</skos:editorialNote>
		<skos:historyNote>Revision 4: 3 previous definitions.</skos:historyNote>
		<skos:changeNote>See http://www.cognitiveatlas.org/id/tsk_4a57abb949dfe for complete revision history.</skos:changeNote>
		<skos:scopeNote>http://www.w3.org/2004/02/skos/core#Concept</skos:scopeNote>
		<skos:Note>SKOS properties defined in http://www.w3.org/TR/skos-primer/#secrel</skos:Note>
		<skos:inScheme rdf:resource="http://www.cognitiveatlas.org/tasks/"/>
		<skos:definition>instrument used to measure trait (chronic) anxiety, a general propensity to be anxious, and state (temporary) anxiety, a temporary state varying in intensity, in adults.</skos:definition>
		<skos:prefLabel>Spielberger's State-Trait Anxiety Questionnaire</skos:prefLabel>
		<skos:altLabel></skos:altLabel>
		<cito:citesForInformation rdf:resource="http://www.cognitiveatlas.org/citation/id/cit_4dfba7127f5b1"/>
		<cito:citesForInformation rdf:resource="http://www.cognitiveatlas.org/citation/id/cit_4dfba7312ee0b"/>
</skos:Concept><skos:Concept rdf:about="http://www.cognitiveatlas.org/id/tsk_4a57abb949e0c"> <dc:identifier>tsk_4a57abb949e0c</dc:identifier>
		<dc:Title>Cognitive Atlas : Lexicon : Sternberg delayed recognition task</dc:Title>
		<dc:Description>RDF output for 'Sternberg delayed recognition task'</dc:Description>
		<dc:Type>InteractiveResource</dc:Type>
		<dc:Publisher>Cognitive Atlas</dc:Publisher>
		<dc:Creator>Cognitive Atlas RDF Generator</dc:Creator>
		<dc:Contributor>Russ Poldrack</dc:Contributor>
		<dc:Date>2012-01-28 11:58:44</dc:Date>
		<dc:Format>text/rdf</dc:Format>
		<dc:Language>en</dc:Language>
		<skos:editorialNote>Generated by testgenall.php on Thu Mar 29 10:24:08 PDT 2012.</skos:editorialNote>
		<skos:historyNote>Revision 5: 4 previous definitions.</skos:historyNote>
		<skos:changeNote>See http://www.cognitiveatlas.org/id/tsk_4a57abb949e0c for complete revision history.</skos:changeNote>
		<skos:scopeNote>http://www.w3.org/2004/02/skos/core#Concept</skos:scopeNote>
		<skos:Note>SKOS properties defined in http://www.w3.org/TR/skos-primer/#secrel</skos:Note>
		<skos:inScheme rdf:resource="http://www.cognitiveatlas.org/tasks/"/>
		<skos:definition>Subjects view a string of letters.  After a delay, a probe letter is presented and subjects indicate if the presented letter was in the previously viewed group. </skos:definition>
		<skos:prefLabel>Sternberg delayed recognition task</skos:prefLabel>
		<skos:altLabel>Sternberg task, delayed recognition task, Sternberg item recognition task</skos:altLabel>
		<skos:related rdf:resource="http://www.cognitiveatlas.org/id/tsk_4a57abb9499e3"/>
		<skos:related rdf:resource="http://www.cognitiveatlas.org/id/trm_4a3fd79d0b0c8"/>
		<skos:related rdf:resource="http://www.cognitiveatlas.org/id/trm_4a3fd79d0ba30"/>
		<skos:related rdf:resource="http://www.cognitiveatlas.org/id/trm_4a3fd79d0ba6c"/>
		<skos:example>delayed match to sample task is a broader synonym of Sternberg delayed recognition task</skos:example>
		<skos:example>serial search is measured by the contrast of average response time trials in the Sternberg delayed recognition task</skos:example>
		<skos:example>maintenance is measured by the contrast of accuracy of immediate recognition test minus accuracy of delayed test trials in the Sternberg delayed recognition task</skos:example>
		<skos:example>working memory retrieval is measured by the contrast of accuracy of participant minus average accuracy of controls trials in the Sternberg delayed recognition task</skos:example>
		<cito:citesForInformation rdf:resource="http://www.cognitiveatlas.org/citation/id/cit_4dfbabe06f0df"/>
		<cito:citesForInformation rdf:resource="http://www.cognitiveatlas.org/citation/id/cit_4dfbae6fb4de4"/>
		<cito:citesForInformation rdf:resource="http://www.cognitiveatlas.org/citation/id/cit_4dfbaeb9095e2"/>
</skos:Concept><skos:Concept rdf:about="http://www.cognitiveatlas.org/id/tsk_4a57abb949e1a"> <dc:identifier>tsk_4a57abb949e1a</dc:identifier>
		<dc:Title>Cognitive Atlas : Lexicon : stop signal task</dc:Title>
		<dc:Description>RDF output for 'stop signal task'</dc:Description>
		<dc:Type>InteractiveResource</dc:Type>
		<dc:Publisher>Cognitive Atlas</dc:Publisher>
		<dc:Creator>Cognitive Atlas RDF Generator</dc:Creator>
		<dc:Contributor>Russ Poldrack</dc:Contributor>
		<dc:Date>2012-01-28 08:20:47</dc:Date>
		<dc:Format>text/rdf</dc:Format>
		<dc:Language>en</dc:Language>
		<skos:editorialNote>Generated by testgenall.php on Thu Mar 29 10:24:08 PDT 2012.</skos:editorialNote>
		<skos:historyNote>Revision 3: 2 previous definitions.</skos:historyNote>
		<skos:changeNote>See http://www.cognitiveatlas.org/id/tsk_4a57abb949e1a for complete revision history.</skos:changeNote>
		<skos:scopeNote>http://www.w3.org/2004/02/skos/core#Concept</skos:scopeNote>
		<skos:Note>SKOS properties defined in http://www.w3.org/TR/skos-primer/#secrel</skos:Note>
		<skos:inScheme rdf:resource="http://www.cognitiveatlas.org/tasks/"/>
		<skos:definition>A task in which an external stimulus signals the participant to interrupt an already-initiated motor response.</skos:definition>
		<skos:prefLabel>stop signal task</skos:prefLabel>
		<skos:altLabel>stop task</skos:altLabel>
		<skos:related rdf:resource="http://www.cognitiveatlas.org/id/trm_4a3fd79d0af66"/>
		<skos:related rdf:resource="http://www.cognitiveatlas.org/id/trm_4da4b203ad5ae"/>
		<skos:example>response inhibition is measured by the contrast of Stop Signal Reaction Time trials in the stop signal task</skos:example>
		<skos:example>selective stop signal task is descended from stop signal task</skos:example>
		<cito:citesForInformation rdf:resource="http://www.cognitiveatlas.org/citation/id/cit_4b44a76c5485b"/>
		<cito:citesForInformation rdf:resource="http://www.cognitiveatlas.org/citation/id/cit_4c6b6036b8b88"/>
</skos:Concept><skos:Concept rdf:about="http://www.cognitiveatlas.org/id/tsk_4a57abb949e27"> <dc:identifier>tsk_4a57abb949e27</dc:identifier>
		<dc:Title>Cognitive Atlas : Lexicon : Stroop task</dc:Title>
		<dc:Description>RDF output for 'Stroop task'</dc:Description>
		<dc:Type>InteractiveResource</dc:Type>
		<dc:Publisher>Cognitive Atlas</dc:Publisher>
		<dc:Creator>Cognitive Atlas RDF Generator</dc:Creator>
		<dc:Contributor>Russ Poldrack</dc:Contributor>
		<dc:Date>2011-12-12 15:39:16</dc:Date>
		<dc:Format>text/rdf</dc:Format>
		<dc:Language>en</dc:Language>
		<skos:editorialNote>Generated by testgenall.php on Thu Mar 29 10:24:08 PDT 2012.</skos:editorialNote>
		<skos:historyNote>Revision 6: 5 previous definitions.</skos:historyNote>
		<skos:changeNote>See http://www.cognitiveatlas.org/id/tsk_4a57abb949e27 for complete revision history.</skos:changeNote>
		<skos:scopeNote>http://www.w3.org/2004/02/skos/core#Concept</skos:scopeNote>
		<skos:Note>SKOS properties defined in http://www.w3.org/TR/skos-primer/#secrel</skos:Note>
		<skos:inScheme rdf:resource="http://www.cognitiveatlas.org/tasks/"/>
		<skos:definition>Subjects view color names presented in various ink colors and are instructed to name the color of the ink.  In incongruent stimuli, color names and ink colors are non-matching. </skos:definition>
		<skos:prefLabel>Stroop task</skos:prefLabel>
		<skos:altLabel></skos:altLabel>
		<skos:related rdf:resource="http://www.cognitiveatlas.org/id/trm_4dadbfd771a54"/>
		<skos:related rdf:resource="http://www.cognitiveatlas.org/id/trm_4b843655d5d75"/>
		<skos:related rdf:resource="http://www.cognitiveatlas.org/id/trm_4b1968619b00b"/>
		<skos:related rdf:resource="http://www.cognitiveatlas.org/id/trm_4b1968619b00b"/>
		<skos:related rdf:resource="http://www.cognitiveatlas.org/id/tsk_4a57abb949d76"/>
		<skos:related rdf:resource="http://www.cognitiveatlas.org/id/trm_4a3fd79d0af66"/>
		<skos:related rdf:resource="http://www.cognitiveatlas.org/id/"/>
		<skos:related rdf:resource="http://www.cognitiveatlas.org/id/"/>
		<skos:example>Stroop task is descended from </skos:example>
		<skos:example>Picture-word Stroop task is descended from Stroop task</skos:example>
		<skos:example>Chimeric Animal Stroop Task is descended from Stroop task</skos:example>
		<skos:example>Color-word Stroop Task is descended from Stroop task</skos:example>
		<skos:example>Color-word Stroop Task is a narrower synonym of Stroop task</skos:example>
		<skos:example>selective attention task is a broader synonym of Stroop task</skos:example>
		<skos:example>response inhibition is measured by the contrast of incongruent minus congruent trials in the Stroop task</skos:example>
		<skos:example> is descended from Stroop task</skos:example>
		<cito:citesForInformation rdf:resource="http://www.cognitiveatlas.org/citation/id/cit_4dfbb9673b971"/>
		<cito:citesForInformation rdf:resource="http://www.cognitiveatlas.org/citation/id/cit_4dfbb9adefd8b"/>
		<cito:citesForInformation rdf:resource="http://www.cognitiveatlas.org/citation/id/cit_4e417140627ac"/>
</skos:Concept><skos:Concept rdf:about="http://www.cognitiveatlas.org/id/tsk_4a57abb949e35"> <dc:identifier>tsk_4a57abb949e35</dc:identifier>
		<dc:Title>Cognitive Atlas : Lexicon : Structured Clinical Interview for Diagnostic and Statistical Manual of Mental Disorders (DSM-IV) Axis I Disorder</dc:Title>
		<dc:Description>RDF output for 'Structured Clinical Interview for Diagnostic and Statistical Manual of Mental Disorders (DSM-IV) Axis I Disorder'</dc:Description>
		<dc:Type>InteractiveResource</dc:Type>
		<dc:Publisher>Cognitive Atlas</dc:Publisher>
		<dc:Creator>Cognitive Atlas RDF Generator</dc:Creator>
		<dc:Contributor>Carinna Torgerson</dc:Contributor>
		<dc:Date>2011-06-17 14:06:53</dc:Date>
		<dc:Format>text/rdf</dc:Format>
		<dc:Language>en</dc:Language>
		<skos:editorialNote>Generated by testgenall.php on Thu Mar 29 10:24:08 PDT 2012.</skos:editorialNote>
		<skos:historyNote>Revision 5: 4 previous definitions.</skos:historyNote>
		<skos:changeNote>See http://www.cognitiveatlas.org/id/tsk_4a57abb949e35 for complete revision history.</skos:changeNote>
		<skos:scopeNote>http://www.w3.org/2004/02/skos/core#Concept</skos:scopeNote>
		<skos:Note>SKOS properties defined in http://www.w3.org/TR/skos-primer/#secrel</skos:Note>
		<skos:inScheme rdf:resource="http://www.cognitiveatlas.org/tasks/"/>
		<skos:definition>a diagnostic exam used to determine DSM-IV Axis I disorders (mental health disorders). It covers 6 diagnostic categories, and is often used in conjunction with an unstructured interview. The exam includes an administration booklet of questions for the examiner to ask and a scoresheet. Scores are not determined by &#34;right&#34; or &#34;wrong&#34; answers, but by number of questions that adhere to diagnostic criteria.</skos:definition>
		<skos:prefLabel>Structured Clinical Interview for Diagnostic and Statistical Manual of Mental Disorders (DSM-IV) Axis I Disorder</skos:prefLabel>
		<skos:altLabel></skos:altLabel>
		<skos:related rdf:resource="http://www.cognitiveatlas.org/id/tsk_4a57abb949e5b"/>
		<skos:related rdf:resource="http://www.cognitiveatlas.org/id/trm_4a3fd79d0a95a"/>
		<skos:example>Symptom Checklist-90-Revised  is related to Structured Clinical Interview for Diagnostic and Statistical Manual of Mental Disorders (DSM-IV) Axis I Disorder</skos:example>
		<skos:example>mood is measured by the contrast of the examiner&#39;s evaluation trials in the Structured Clinical Interview for Diagnostic and Statistical Manual of Mental Disorders (DSM-IV) Axis I Disorder</skos:example>
		<cito:citesForInformation rdf:resource="http://www.cognitiveatlas.org/citation/id/cit_4dfbc155af64d"/>
		<cito:citesForInformation rdf:resource="http://www.cognitiveatlas.org/citation/id/cit_4dfbc29d81a87"/>
		<cito:citesForInformation rdf:resource="http://www.cognitiveatlas.org/citation/id/cit_4dfbc38a59e9a"/>
</skos:Concept><skos:Concept rdf:about="http://www.cognitiveatlas.org/id/tsk_4a57abb949e44"> <dc:identifier>tsk_4a57abb949e44</dc:identifier>
		<dc:Title>Cognitive Atlas : Lexicon : symbol-digit substitution</dc:Title>
		<dc:Description>RDF output for 'symbol-digit substitution'</dc:Description>
		<dc:Type>InteractiveResource</dc:Type>
		<dc:Publisher>Cognitive Atlas</dc:Publisher>
		<dc:Creator>Cognitive Atlas RDF Generator</dc:Creator>
		<dc:Contributor>Natalie Picchetti</dc:Contributor>
		<dc:Date>2011-04-07 11:03:43</dc:Date>
		<dc:Format>text/rdf</dc:Format>
		<dc:Language>en</dc:Language>
		<skos:editorialNote>Generated by testgenall.php on Thu Mar 29 10:24:08 PDT 2012.</skos:editorialNote>
		<skos:historyNote>Revision 3: 2 previous definitions.</skos:historyNote>
		<skos:changeNote>See http://www.cognitiveatlas.org/id/tsk_4a57abb949e44 for complete revision history.</skos:changeNote>
		<skos:scopeNote>http://www.w3.org/2004/02/skos/core#Concept</skos:scopeNote>
		<skos:Note>SKOS properties defined in http://www.w3.org/TR/skos-primer/#secrel</skos:Note>
		<skos:inScheme rdf:resource="http://www.cognitiveatlas.org/tasks/"/>
		<skos:definition>DSST is a neuropsychological test sensitive to brain damage, dementia, age and depression. It isn’t sensitive to the location of brain-damage (except for damage comprising part of the visual field). It consists of (e.g. nine) digit-symbol pairs (e.g. 1/-,2/┴ ... 7/Λ,8/X,9/=) followed by a list of digits. Under each digit the subject should write down the corresponding symbol as fast as possible. The number of correct symbols within the allowed time (e.g. 90 or 120 sec) is measured.
</skos:definition>
		<skos:prefLabel>symbol-digit substitution</skos:prefLabel>
		<skos:altLabel></skos:altLabel>
		<skos:related rdf:resource="http://www.cognitiveatlas.org/id/tsk_4a57abb949a25"/>
		<skos:related rdf:resource="http://www.cognitiveatlas.org/id/tsk_4a57abb949f12"/>
		<skos:example>symbol-digit substitution is an exact synonym of Digit/Symbol Coding test</skos:example>
		<skos:example>symbol-digit substitution is descended from Wechsler Adult Intelligence Scale - Revised</skos:example>
		<cito:citesForInformation rdf:resource="http://www.cognitiveatlas.org/citation/id/cit_4dfbd438bf052"/>
</skos:Concept><skos:Concept rdf:about="http://www.cognitiveatlas.org/id/tsk_4a57abb949e5b"> <dc:identifier>tsk_4a57abb949e5b</dc:identifier>
		<dc:Title>Cognitive Atlas : Lexicon : Symptom Checklist-90-Revised </dc:Title>
		<dc:Description>RDF output for 'Symptom Checklist-90-Revised '</dc:Description>
		<dc:Type>InteractiveResource</dc:Type>
		<dc:Publisher>Cognitive Atlas</dc:Publisher>
		<dc:Creator>Cognitive Atlas RDF Generator</dc:Creator>
		<dc:Contributor>Brenda Gregory</dc:Contributor>
		<dc:Date>2011-05-18 14:02:21</dc:Date>
		<dc:Format>text/rdf</dc:Format>
		<dc:Language>en</dc:Language>
		<skos:editorialNote>Generated by testgenall.php on Thu Mar 29 10:24:08 PDT 2012.</skos:editorialNote>
		<skos:historyNote>Revision 3: 2 previous definitions.</skos:historyNote>
		<skos:changeNote>See http://www.cognitiveatlas.org/id/tsk_4a57abb949e5b for complete revision history.</skos:changeNote>
		<skos:scopeNote>http://www.w3.org/2004/02/skos/core#Concept</skos:scopeNote>
		<skos:Note>SKOS properties defined in http://www.w3.org/TR/skos-primer/#secrel</skos:Note>
		<skos:inScheme rdf:resource="http://www.cognitiveatlas.org/tasks/"/>
		<skos:definition>a relatively brief self-report psychometric instrument designed to evaluate a broad range of psychological problems and symptoms of psychopathology. It is also useful in measuring the progress and outcome of psychiatric and psychological treatments or for research purposes.</skos:definition>
		<skos:prefLabel>Symptom Checklist-90-Revised </skos:prefLabel>
		<skos:altLabel></skos:altLabel>
		<skos:related rdf:resource="http://www.cognitiveatlas.org/id/trm_4a3fd79d0a95a"/>
		<skos:related rdf:resource="http://www.cognitiveatlas.org/id/tsk_4a57abb949e35"/>
		<skos:example>Symptom Checklist-90-Revised  is related to Structured Clinical Interview for Diagnostic and Statistical Manual of Mental Disorders (DSM-IV) Axis I Disorder</skos:example>
		<skos:example>mood is measured by the contrast of standard deviation from the mean score trials in the Symptom Checklist-90-Revised </skos:example>
		<cito:citesForInformation rdf:resource="http://www.cognitiveatlas.org/citation/id/cit_4dfbd9816083b"/>
		<cito:citesForInformation rdf:resource="http://www.cognitiveatlas.org/citation/id/cit_4dfbd9d7d1b33"/>
</skos:Concept><skos:Concept rdf:about="http://www.cognitiveatlas.org/id/tsk_4a57abb949e7c"> <dc:identifier>tsk_4a57abb949e7c</dc:identifier>
		<dc:Title>Cognitive Atlas : Lexicon : syntactic acceptability judgement task</dc:Title>
		<dc:Description>RDF output for 'syntactic acceptability judgement task'</dc:Description>
		<dc:Type>InteractiveResource</dc:Type>
		<dc:Publisher>Cognitive Atlas</dc:Publisher>
		<dc:Creator>Cognitive Atlas RDF Generator</dc:Creator>
		<dc:Contributor>Carinna Torgerson</dc:Contributor>
		<dc:Date>2011-06-17 16:16:45</dc:Date>
		<dc:Format>text/rdf</dc:Format>
		<dc:Language>en</dc:Language>
		<skos:editorialNote>Generated by testgenall.php on Thu Mar 29 10:24:08 PDT 2012.</skos:editorialNote>
		<skos:historyNote>Revision 2: 1 previous definitions.</skos:historyNote>
		<skos:changeNote>See http://www.cognitiveatlas.org/id/tsk_4a57abb949e7c for complete revision history.</skos:changeNote>
		<skos:scopeNote>http://www.w3.org/2004/02/skos/core#Concept</skos:scopeNote>
		<skos:Note>SKOS properties defined in http://www.w3.org/TR/skos-primer/#secrel</skos:Note>
		<skos:inScheme rdf:resource="http://www.cognitiveatlas.org/tasks/"/>
		<skos:definition>Also called the syntactic plausibility judgment task, this task asks participants to read sentences and indicate whether or not they are gramatically correct. </skos:definition>
		<skos:prefLabel>syntactic acceptability judgement task</skos:prefLabel>
		<skos:altLabel></skos:altLabel>
		<skos:related rdf:resource="http://www.cognitiveatlas.org/id/trm_4a3fd79d0b340"/>
		<skos:related rdf:resource="http://www.cognitiveatlas.org/id/trm_4a3fd79d0b756"/>
		<skos:related rdf:resource="http://www.cognitiveatlas.org/id/trm_4a3fd79d0a7f8"/>
		<skos:related rdf:resource="http://www.cognitiveatlas.org/id/trm_4c8a842512a33"/>
		<skos:example>syntactic parsing is measured by the contrast of accuracy of participant minus average accuracy of controls trials in the syntactic acceptability judgement task</skos:example>
		<skos:example>grammatical encoding is measured by the contrast of accuracy of participant minus average accuracy of controls trials in the syntactic acceptability judgement task</skos:example>
		<skos:example>linguistic competence is measured by the contrast of accuracy of participant minus average accuracy of controls trials in the syntactic acceptability judgement task</skos:example>
		<skos:example>Syntactic Discrimination is related to syntactic acceptability judgement task</skos:example>
		<cito:citesForInformation rdf:resource="http://www.cognitiveatlas.org/citation/id/cit_4dfbde055ce41"/>
		<cito:citesForInformation rdf:resource="http://www.cognitiveatlas.org/citation/id/cit_4dfbe00812089"/>
</skos:Concept><skos:Concept rdf:about="http://www.cognitiveatlas.org/id/tsk_4a57abb949e8a"> <dc:identifier>tsk_4a57abb949e8a</dc:identifier>
		<dc:Title>Cognitive Atlas : Lexicon : task-switching </dc:Title>
		<dc:Description>RDF output for 'task-switching '</dc:Description>
		<dc:Type>InteractiveResource</dc:Type>
		<dc:Publisher>Cognitive Atlas</dc:Publisher>
		<dc:Creator>Cognitive Atlas RDF Generator</dc:Creator>
		<dc:Contributor>Agatha Lenartowicz</dc:Contributor>
		<dc:Date>2009-07-10 14:06:33</dc:Date>
		<dc:Format>text/rdf</dc:Format>
		<dc:Language>en</dc:Language>
		<skos:editorialNote>Generated by testgenall.php on Thu Mar 29 10:24:08 PDT 2012.</skos:editorialNote>
		<skos:historyNote>No previous definition revisions.</skos:historyNote>
		<skos:changeNote>This is the first and only definition provided.</skos:changeNote>
		<skos:scopeNote>http://www.w3.org/2004/02/skos/core#Concept</skos:scopeNote>
		<skos:Note>SKOS properties defined in http://www.w3.org/TR/skos-primer/#secrel</skos:Note>
		<skos:inScheme rdf:resource="http://www.cognitiveatlas.org/tasks/"/>
		<skos:definition>A task in which participants alternate between two or more judgments typically regarding the same set of stimuli. Accuracy and reaction time are measured for each judgment.</skos:definition>
		<skos:prefLabel>task-switching </skos:prefLabel>
		<skos:altLabel></skos:altLabel>
		<skos:related rdf:resource="http://www.cognitiveatlas.org/id/trm_4a3fd79d0b5fb"/>
		<skos:related rdf:resource="http://www.cognitiveatlas.org/id/trm_4b45f56827e93"/>
		<skos:related rdf:resource="http://www.cognitiveatlas.org/id/tsk_4a57abb949dad"/>
		<skos:example>task-switching  is related to Set-shifting task</skos:example>
		<skos:example>attention shifting is measured by the contrast of switch trial - repeat trial = switch cost trials in the task-switching </skos:example>
		<skos:example>Task set reconfiguration is measured by the contrast of switch trial - repeat trial = switch cost trials in the task-switching </skos:example>
		<cito:citesForInformation rdf:resource="http://www.cognitiveatlas.org/citation/id/cit_4dff89080d63d"/>
		<cito:citesForInformation rdf:resource="http://www.cognitiveatlas.org/citation/id/cit_4dff89ac0c8cb"/>
</skos:Concept><skos:Concept rdf:about="http://www.cognitiveatlas.org/id/tsk_4a57abb949e98"> <dc:identifier>tsk_4a57abb949e98</dc:identifier>
		<dc:Title>Cognitive Atlas : Lexicon : Temporal discounting task</dc:Title>
		<dc:Description>RDF output for 'Temporal discounting task'</dc:Description>
		<dc:Type>InteractiveResource</dc:Type>
		<dc:Publisher>Cognitive Atlas</dc:Publisher>
		<dc:Creator>Cognitive Atlas RDF Generator</dc:Creator>
		<dc:Contributor>Natalie Picchetti</dc:Contributor>
		<dc:Date>2011-05-20 14:51:31</dc:Date>
		<dc:Format>text/rdf</dc:Format>
		<dc:Language>en</dc:Language>
		<skos:editorialNote>Generated by testgenall.php on Thu Mar 29 10:24:08 PDT 2012.</skos:editorialNote>
		<skos:historyNote>Revision 2: 1 previous definitions.</skos:historyNote>
		<skos:changeNote>See http://www.cognitiveatlas.org/id/tsk_4a57abb949e98 for complete revision history.</skos:changeNote>
		<skos:scopeNote>http://www.w3.org/2004/02/skos/core#Concept</skos:scopeNote>
		<skos:Note>SKOS properties defined in http://www.w3.org/TR/skos-primer/#secrel</skos:Note>
		<skos:inScheme rdf:resource="http://www.cognitiveatlas.org/tasks/"/>
		<skos:definition>refers to the tendency of people to discount rewards as they approach a temporal horizon in the future or the past (i.e., become so distant in time that they cease to be valuable or to have additive effects). To put it another way, it is a tendency to give greater value to rewards as they move away from their temporal horizons and towards the &#34;now&#34;. For instance, a nicotine deprived smoker may highly value a cigarette available any time in the next 6 hours but assign little or no value to a cigarette available in 6 months.</skos:definition>
		<skos:prefLabel>Temporal discounting task</skos:prefLabel>
		<skos:altLabel></skos:altLabel>
		<skos:related rdf:resource="http://www.cognitiveatlas.org/id/trm_4a3fd79d0ae7b"/>
		<skos:related rdf:resource="http://www.cognitiveatlas.org/id/trm_4a3fd79d0ae7b"/>
		<skos:related rdf:resource="http://www.cognitiveatlas.org/id/trm_4a3fd79d09877"/>
		<skos:example>prospective planning is measured by the contrast of areas of activation during task minus baseline trials in the Temporal discounting task</skos:example>
		<skos:example>prospective planning is measured by the contrast of standard deviation of k (discounting) trials in the Temporal discounting task</skos:example>
		<skos:example>appetitive motivation is measured by the contrast of standard deviation of k (discounting) trials in the Temporal discounting task</skos:example>
		<cito:citesForInformation rdf:resource="http://www.cognitiveatlas.org/citation/id/cit_4dff8d090fbb8"/>
		<cito:citesForInformation rdf:resource="http://www.cognitiveatlas.org/citation/id/cit_4dff8d6494764"/>
		<cito:citesForInformation rdf:resource="http://www.cognitiveatlas.org/citation/id/cit_4dff8eda29de4"/>
</skos:Concept><skos:Concept rdf:about="http://www.cognitiveatlas.org/id/tsk_4a57abb949ea5"> <dc:identifier>tsk_4a57abb949ea5</dc:identifier>
		<dc:Title>Cognitive Atlas : Lexicon : Test of Word Reading Efficiency</dc:Title>
		<dc:Description>RDF output for 'Test of Word Reading Efficiency'</dc:Description>
		<dc:Type>InteractiveResource</dc:Type>
		<dc:Publisher>Cognitive Atlas</dc:Publisher>
		<dc:Creator>Cognitive Atlas RDF Generator</dc:Creator>
		<dc:Contributor>Brenda Gregory</dc:Contributor>
		<dc:Date>2011-04-28 17:27:36</dc:Date>
		<dc:Format>text/rdf</dc:Format>
		<dc:Language>en</dc:Language>
		<skos:editorialNote>Generated by testgenall.php on Thu Mar 29 10:24:08 PDT 2012.</skos:editorialNote>
		<skos:historyNote>Revision 3: 2 previous definitions.</skos:historyNote>
		<skos:changeNote>See http://www.cognitiveatlas.org/id/tsk_4a57abb949ea5 for complete revision history.</skos:changeNote>
		<skos:scopeNote>http://www.w3.org/2004/02/skos/core#Concept</skos:scopeNote>
		<skos:Note>SKOS properties defined in http://www.w3.org/TR/skos-primer/#secrel</skos:Note>
		<skos:inScheme rdf:resource="http://www.cognitiveatlas.org/tasks/"/>
		<skos:definition>a nationally normed measure of word reading accuracy and fluency that provides an efficient means of monitoring the growth of two kinds of word reading skills that are critical in the development of overall reading ability: the ability to accurately recognize familiar words as whole units or “sight words” and the ability to “sound out” words quickly. </skos:definition>
		<skos:prefLabel>Test of Word Reading Efficiency</skos:prefLabel>
		<skos:altLabel></skos:altLabel>
		<skos:related rdf:resource="http://www.cognitiveatlas.org/id/trm_4a3fd79d0a775"/>
		<skos:related rdf:resource="http://www.cognitiveatlas.org/id/trm_4a3fd79d0b826"/>
		<skos:example>language comprehension is measured by the contrast of standard deviation from the mean score trials in the Test of Word Reading Efficiency</skos:example>
		<skos:example>lexical processing is measured by the contrast of standard deviation from the mean score trials in the Test of Word Reading Efficiency</skos:example>
		<cito:citesForInformation rdf:resource="http://www.cognitiveatlas.org/citation/id/cit_4dff9a90e6c01"/>
		<cito:citesForInformation rdf:resource="http://www.cognitiveatlas.org/citation/id/cit_4dff9b2baa37b"/>
</skos:Concept><skos:Concept rdf:about="http://www.cognitiveatlas.org/id/tsk_4a57abb949eb3"> <dc:identifier>tsk_4a57abb949eb3</dc:identifier>
		<dc:Title>Cognitive Atlas : Lexicon : Tobacco Craving Questionnaire</dc:Title>
		<dc:Description>RDF output for 'Tobacco Craving Questionnaire'</dc:Description>
		<dc:Type>InteractiveResource</dc:Type>
		<dc:Publisher>Cognitive Atlas</dc:Publisher>
		<dc:Creator>Cognitive Atlas RDF Generator</dc:Creator>
		<dc:Contributor>Natalie Picchetti</dc:Contributor>
		<dc:Date>2011-04-11 15:21:30</dc:Date>
		<dc:Format>text/rdf</dc:Format>
		<dc:Language>en</dc:Language>
		<skos:editorialNote>Generated by testgenall.php on Thu Mar 29 10:24:08 PDT 2012.</skos:editorialNote>
		<skos:historyNote>Revision 3: 2 previous definitions.</skos:historyNote>
		<skos:changeNote>See http://www.cognitiveatlas.org/id/tsk_4a57abb949eb3 for complete revision history.</skos:changeNote>
		<skos:scopeNote>http://www.w3.org/2004/02/skos/core#Concept</skos:scopeNote>
		<skos:Note>SKOS properties defined in http://www.w3.org/TR/skos-primer/#secrel</skos:Note>
		<skos:inScheme rdf:resource="http://www.cognitiveatlas.org/tasks/"/>
		<skos:definition>a multidimensional questionnaire to assess tobacco craving.  It consists of a 47-item TCQ and other forms assessing demographics, tobacco and other drug use history, quit attempts, and current mood.  It represents four specific constructs that characterize craving for tobacco: (a) Emotionality, or smoking in anticipation of relief from withdrawal symptoms or negative mood, (b) expectancy, or anticipation of positive outcomes from smoking, (c) compulsivity, or an inability to control tobacco use, and (d) purposefulness, or intention and planning to smoke for positive outcomes.  It is an instrument for assessing tobacco craving in individuals not attempting to reduce or quit smoking.
</skos:definition>
		<skos:prefLabel>Tobacco Craving Questionnaire</skos:prefLabel>
		<skos:altLabel></skos:altLabel>
		<skos:related rdf:resource="http://www.cognitiveatlas.org/id/tsk_4a57abb949a78"/>
		<skos:example>Tobacco Craving Questionnaire is related to Fagerstrom Test for Nicotine Dependence</skos:example>
		<cito:citesForInformation rdf:resource="http://www.cognitiveatlas.org/citation/id/cit_4da37ea20ce3d"/>
		<cito:citesForInformation rdf:resource="http://www.cognitiveatlas.org/citation/id/cit_4da37ea20ce3d"/>
		<cito:citesForInformation rdf:resource="http://www.cognitiveatlas.org/citation/id/cit_4dffb2683ce1b"/>
</skos:Concept><skos:Concept rdf:about="http://www.cognitiveatlas.org/id/tsk_4a57abb949ec0"> <dc:identifier>tsk_4a57abb949ec0</dc:identifier>
		<dc:Title>Cognitive Atlas : Lexicon : Trail Making Test A and B</dc:Title>
		<dc:Description>RDF output for 'Trail Making Test A and B'</dc:Description>
		<dc:Type>InteractiveResource</dc:Type>
		<dc:Publisher>Cognitive Atlas</dc:Publisher>
		<dc:Creator>Cognitive Atlas RDF Generator</dc:Creator>
		<dc:Contributor>Agatha Lenartowicz</dc:Contributor>
		<dc:Date>2009-07-10 14:06:33</dc:Date>
		<dc:Format>text/rdf</dc:Format>
		<dc:Language>en</dc:Language>
		<skos:editorialNote>Generated by testgenall.php on Thu Mar 29 10:24:08 PDT 2012.</skos:editorialNote>
		<skos:historyNote>No previous definition revisions.</skos:historyNote>
		<skos:changeNote>This is the first and only definition provided.</skos:changeNote>
		<skos:scopeNote>http://www.w3.org/2004/02/skos/core#Concept</skos:scopeNote>
		<skos:Note>SKOS properties defined in http://www.w3.org/TR/skos-primer/#secrel</skos:Note>
		<skos:inScheme rdf:resource="http://www.cognitiveatlas.org/tasks/"/>
		<skos:definition>A neuropsychological test in which participants must connect-the-dots (traverse between items) according to some specified order. In Test A these items are numbers (1,2,3 etc.) and the order is determined by increasing magnitude. In Test B these items are both numbers and letters (1,2,3, A,B,C etc.) and the order is determined by a combination of increasing numbers AND letters (e.g., 1 A 2 B 3 C..) requiring participants to alternate between letters and numbers.</skos:definition>
		<skos:prefLabel>Trail Making Test A and B</skos:prefLabel>
		<skos:altLabel></skos:altLabel>
		<skos:related rdf:resource="http://www.cognitiveatlas.org/id/trm_4a3fd79d0b4cd"/>
		<skos:related rdf:resource="http://www.cognitiveatlas.org/id/trm_4a3fd79d0a252"/>
		<skos:related rdf:resource="http://www.cognitiveatlas.org/id/trm_4a3fd79d0b0bd"/>
		<skos:example>visual search is measured by the contrast of ANOVA of time by age group trials in the Trail Making Test A and B</skos:example>
		<skos:example>executive function is measured by the contrast of ANOVA of time by age group trials in the Trail Making Test A and B</skos:example>
		<skos:example>serial processing is measured by the contrast of ANOVA of time by age group trials in the Trail Making Test A and B</skos:example>
		<cito:citesForInformation rdf:resource="http://www.cognitiveatlas.org/citation/id/cit_4dffbaea770a8"/>
</skos:Concept><skos:Concept rdf:about="http://www.cognitiveatlas.org/id/tsk_4a57abb949ece"> <dc:identifier>tsk_4a57abb949ece</dc:identifier>
		<dc:Title>Cognitive Atlas : Lexicon : Unified Parkinson's Disease Rating Scale</dc:Title>
		<dc:Description>RDF output for 'Unified Parkinson's Disease Rating Scale'</dc:Description>
		<dc:Type>InteractiveResource</dc:Type>
		<dc:Publisher>Cognitive Atlas</dc:Publisher>
		<dc:Creator>Cognitive Atlas RDF Generator</dc:Creator>
		<dc:Contributor>Russ Poldrack</dc:Contributor>
		<dc:Date>2011-08-10 07:41:42</dc:Date>
		<dc:Format>text/rdf</dc:Format>
		<dc:Language>en</dc:Language>
		<skos:editorialNote>Generated by testgenall.php on Thu Mar 29 10:24:08 PDT 2012.</skos:editorialNote>
		<skos:historyNote>Revision 4: 3 previous definitions.</skos:historyNote>
		<skos:changeNote>See http://www.cognitiveatlas.org/id/tsk_4a57abb949ece for complete revision history.</skos:changeNote>
		<skos:scopeNote>http://www.w3.org/2004/02/skos/core#Concept</skos:scopeNote>
		<skos:Note>SKOS properties defined in http://www.w3.org/TR/skos-primer/#secrel</skos:Note>
		<skos:inScheme rdf:resource="http://www.cognitiveatlas.org/tasks/"/>
		<skos:definition>a rating scale used to follow the longitudinal course of Parkinson&#39;s disease, made up of the following sections: (1)evaluation of Mentation, behavior, and mood, (2)self evaluation of the activities of daily life (ADLs), (3)clinician-scored motor evaluation, (4)Hoehn and Yahr stating of severity of Parkinson disease, (5)Schwab and England ADL scale; these are evaluated by interview and clinical observation.</skos:definition>
		<skos:prefLabel>Unified Parkinson's Disease Rating Scale</skos:prefLabel>
		<skos:altLabel>UPDRS</skos:altLabel>
		<cito:citesForInformation rdf:resource="http://www.cognitiveatlas.org/citation/id/cit_4dffdb74e8e58"/>
</skos:Concept><skos:Concept rdf:about="http://www.cognitiveatlas.org/id/tsk_4a57abb949edb"> <dc:identifier>tsk_4a57abb949edb</dc:identifier>
		<dc:Title>Cognitive Atlas : Lexicon : visual alignment task </dc:Title>
		<dc:Description>RDF output for 'visual alignment task '</dc:Description>
		<dc:Type>InteractiveResource</dc:Type>
		<dc:Publisher>Cognitive Atlas</dc:Publisher>
		<dc:Creator>Cognitive Atlas RDF Generator</dc:Creator>
		<dc:Contributor>Carinna Torgerson</dc:Contributor>
		<dc:Date>2011-06-21 11:30:32</dc:Date>
		<dc:Format>text/rdf</dc:Format>
		<dc:Language>en</dc:Language>
		<skos:editorialNote>Generated by testgenall.php on Thu Mar 29 10:24:08 PDT 2012.</skos:editorialNote>
		<skos:historyNote>Revision 2: 1 previous definitions.</skos:historyNote>
		<skos:changeNote>See http://www.cognitiveatlas.org/id/tsk_4a57abb949edb for complete revision history.</skos:changeNote>
		<skos:scopeNote>http://www.w3.org/2004/02/skos/core#Concept</skos:scopeNote>
		<skos:Note>SKOS properties defined in http://www.w3.org/TR/skos-primer/#secrel</skos:Note>
		<skos:inScheme rdf:resource="http://www.cognitiveatlas.org/tasks/"/>
		<skos:definition>Participants are shown misaligned lines and asked to indicate which side the top line is offset. Alternatively, participants may be asked to complete an alignment with a pencil or digital pointer.</skos:definition>
		<skos:prefLabel>visual alignment task </skos:prefLabel>
		<skos:altLabel></skos:altLabel>
		<skos:related rdf:resource="http://www.cognitiveatlas.org/id/trm_4a3fd79d0b1a6"/>
		<skos:related rdf:resource="http://www.cognitiveatlas.org/id/trm_4a3fd79d0b4b5"/>
		<skos:example>spatial ability is measured by the contrast of accuracy of participant minus average accuracy of controls trials in the visual alignment task </skos:example>
		<skos:example>visual perception is measured by the contrast of accuracy of participant minus average accuracy of controls trials in the visual alignment task </skos:example>
		<cito:citesForInformation rdf:resource="http://www.cognitiveatlas.org/citation/id/cit_4e00d9078a9fe"/>
		<cito:citesForInformation rdf:resource="http://www.cognitiveatlas.org/citation/id/cit_4e00e1813dd5b"/>
		<cito:citesForInformation rdf:resource="http://www.cognitiveatlas.org/citation/id/cit_4e00e269253d4"/>
</skos:Concept><skos:Concept rdf:about="http://www.cognitiveatlas.org/id/tsk_4a57abb949ee9"> <dc:identifier>tsk_4a57abb949ee9</dc:identifier>
		<dc:Title>Cognitive Atlas : Lexicon : visuospatial cueing task</dc:Title>
		<dc:Description>RDF output for 'visuospatial cueing task'</dc:Description>
		<dc:Type>InteractiveResource</dc:Type>
		<dc:Publisher>Cognitive Atlas</dc:Publisher>
		<dc:Creator>Cognitive Atlas RDF Generator</dc:Creator>
		<dc:Contributor>Carinna Torgerson</dc:Contributor>
		<dc:Date>2011-06-21 14:19:03</dc:Date>
		<dc:Format>text/rdf</dc:Format>
		<dc:Language>en</dc:Language>
		<skos:editorialNote>Generated by testgenall.php on Thu Mar 29 10:24:08 PDT 2012.</skos:editorialNote>
		<skos:historyNote>Revision 2: 1 previous definitions.</skos:historyNote>
		<skos:changeNote>See http://www.cognitiveatlas.org/id/tsk_4a57abb949ee9 for complete revision history.</skos:changeNote>
		<skos:scopeNote>http://www.w3.org/2004/02/skos/core#Concept</skos:scopeNote>
		<skos:Note>SKOS properties defined in http://www.w3.org/TR/skos-primer/#secrel</skos:Note>
		<skos:inScheme rdf:resource="http://www.cognitiveatlas.org/tasks/"/>
		<skos:definition>participants look at a computer screen and press buttons to respond to targets. In some of the trials, a visual cue will appear before the target, but in the same spot as the target.</skos:definition>
		<skos:prefLabel>visuospatial cueing task</skos:prefLabel>
		<skos:altLabel></skos:altLabel>
		<skos:related rdf:resource="http://www.cognitiveatlas.org/id/trm_4a3fd79d0ad58"/>
		<skos:related rdf:resource="http://www.cognitiveatlas.org/id/trm_4a3fd79d0b46f"/>
		<skos:related rdf:resource="http://www.cognitiveatlas.org/id/trm_4a3fd79d0b5fb"/>
		<skos:example> is measured by visuospatial cueing task</skos:example>
		<skos:example>visual attention is measured by the contrast of reaction time to incongruent cues minus reaction time to congruent cues trials in the visuospatial cueing task</skos:example>
		<skos:example>attention shifting is measured by the contrast of reaction time to incongruent cues minus reaction time to congruent cues trials in the visuospatial cueing task</skos:example>
		<cito:citesForInformation rdf:resource="http://www.cognitiveatlas.org/citation/id/cit_4e0108085d833"/>
		<cito:citesForInformation rdf:resource="http://www.cognitiveatlas.org/citation/id/cit_4e0109fcf4154"/>
		<cito:citesForInformation rdf:resource="http://www.cognitiveatlas.org/citation/id/cit_4e010a6c69c95"/>
</skos:Concept><skos:Concept rdf:about="http://www.cognitiveatlas.org/id/tsk_4a57abb949ef7"> <dc:identifier>tsk_4a57abb949ef7</dc:identifier>
		<dc:Title>Cognitive Atlas : Lexicon : Warrington's Face/Word Recognition Test</dc:Title>
		<dc:Description>RDF output for 'Warrington's Face/Word Recognition Test'</dc:Description>
		<dc:Type>InteractiveResource</dc:Type>
		<dc:Publisher>Cognitive Atlas</dc:Publisher>
		<dc:Creator>Cognitive Atlas RDF Generator</dc:Creator>
		<dc:Contributor>Carinna Torgerson</dc:Contributor>
		<dc:Date>2011-06-21 14:33:13</dc:Date>
		<dc:Format>text/rdf</dc:Format>
		<dc:Language>en</dc:Language>
		<skos:editorialNote>Generated by testgenall.php on Thu Mar 29 10:24:08 PDT 2012.</skos:editorialNote>
		<skos:historyNote>Revision 2: 1 previous definitions.</skos:historyNote>
		<skos:changeNote>See http://www.cognitiveatlas.org/id/tsk_4a57abb949ef7 for complete revision history.</skos:changeNote>
		<skos:scopeNote>http://www.w3.org/2004/02/skos/core#Concept</skos:scopeNote>
		<skos:Note>SKOS properties defined in http://www.w3.org/TR/skos-primer/#secrel</skos:Note>
		<skos:inScheme rdf:resource="http://www.cognitiveatlas.org/tasks/"/>
		<skos:definition>Also called the Warrington Recognition Memory Test (RMT), &#34;the RMT consists of the presentation of 50 printed words at the rate of one word every 3 s, and for each word the subject is required to judge the presented stimulus as &#34;pleasant&#34; or &#34;unpleasant&#34; to help ensure that they are attending to the stimulus items. The patient is then presented with a series of word pairs, and the task is to identify which of the two words came from the target list. A series of 50 faces is then presented at the same rate, and the patient is asked to provide the same pleasant versus unpleasant judgments; the patient
is then presented with a series of 50 pairs of faces, and the task is again to identify which of the two faces came from the target list.&#34; - (Hermann, Connell, Barr, &amp; Wyler 1995)</skos:definition>
		<skos:prefLabel>Warrington's Face/Word Recognition Test</skos:prefLabel>
		<skos:altLabel></skos:altLabel>
		<cito:citesForInformation rdf:resource="http://www.cognitiveatlas.org/citation/id/cit_4e010f9a9d874"/>
		<cito:citesForInformation rdf:resource="http://www.cognitiveatlas.org/citation/id/cit_4e01129bb5640"/>
</skos:Concept><skos:Concept rdf:about="http://www.cognitiveatlas.org/id/tsk_4a57abb949f04"> <dc:identifier>tsk_4a57abb949f04</dc:identifier>
		<dc:Title>Cognitive Atlas : Lexicon : Wechsler Adult Intelligence Scale-Revised</dc:Title>
		<dc:Description>RDF output for 'Wechsler Adult Intelligence Scale-Revised'</dc:Description>
		<dc:Type>InteractiveResource</dc:Type>
		<dc:Publisher>Cognitive Atlas</dc:Publisher>
		<dc:Creator>Cognitive Atlas RDF Generator</dc:Creator>
		<dc:Contributor>Brenda Gregory</dc:Contributor>
		<dc:Date>2011-05-16 10:54:51</dc:Date>
		<dc:Format>text/rdf</dc:Format>
		<dc:Language>en</dc:Language>
		<skos:editorialNote>Generated by testgenall.php on Thu Mar 29 10:24:08 PDT 2012.</skos:editorialNote>
		<skos:historyNote>Revision 3: 2 previous definitions.</skos:historyNote>
		<skos:changeNote>See http://www.cognitiveatlas.org/id/tsk_4a57abb949f04 for complete revision history.</skos:changeNote>
		<skos:scopeNote>http://www.w3.org/2004/02/skos/core#Concept</skos:scopeNote>
		<skos:Note>SKOS properties defined in http://www.w3.org/TR/skos-primer/#secrel</skos:Note>
		<skos:inScheme rdf:resource="http://www.cognitiveatlas.org/tasks/"/>
		<skos:definition>a general test of intelligence, which Wechsler defined as, &#34;... the global capacity of the individual to act purposefully, to think rationally, and to deal effectively with his environment.&#34; In keeping with this definition of intelligence as an aggregate of mental aptitudes or abilities, the WAIS-R consists of 11 subtests divided into two parts, verbal and performance.</skos:definition>
		<skos:prefLabel>Wechsler Adult Intelligence Scale-Revised</skos:prefLabel>
		<skos:altLabel></skos:altLabel>
</skos:Concept><skos:Concept rdf:about="http://www.cognitiveatlas.org/id/tsk_4a57abb949f12"> <dc:identifier>tsk_4a57abb949f12</dc:identifier>
		<dc:Title>Cognitive Atlas : Lexicon : Wechsler Adult Intelligence Scale - Revised</dc:Title>
		<dc:Description>RDF output for 'Wechsler Adult Intelligence Scale - Revised'</dc:Description>
		<dc:Type>InteractiveResource</dc:Type>
		<dc:Publisher>Cognitive Atlas</dc:Publisher>
		<dc:Creator>Cognitive Atlas RDF Generator</dc:Creator>
		<dc:Contributor>Brenda Gregory</dc:Contributor>
		<dc:Date>2011-04-29 11:00:03</dc:Date>
		<dc:Format>text/rdf</dc:Format>
		<dc:Language>en</dc:Language>
		<skos:editorialNote>Generated by testgenall.php on Thu Mar 29 10:24:08 PDT 2012.</skos:editorialNote>
		<skos:historyNote>Revision 3: 2 previous definitions.</skos:historyNote>
		<skos:changeNote>See http://www.cognitiveatlas.org/id/tsk_4a57abb949f12 for complete revision history.</skos:changeNote>
		<skos:scopeNote>http://www.w3.org/2004/02/skos/core#Concept</skos:scopeNote>
		<skos:Note>SKOS properties defined in http://www.w3.org/TR/skos-primer/#secrel</skos:Note>
		<skos:inScheme rdf:resource="http://www.cognitiveatlas.org/tasks/"/>
		<skos:definition>used with adults ages 16 to 90 and measures cognitive ability using a core battery of 10 unique subtests that focus on four specific domains of intelligence: verbal comprehension, perceptual reasoning, working memory, and processing speed. </skos:definition>
		<skos:prefLabel>Wechsler Adult Intelligence Scale - Revised</skos:prefLabel>
		<skos:altLabel></skos:altLabel>
		<skos:related rdf:resource="http://www.cognitiveatlas.org/id/tsk_4a57abb94989b"/>
		<skos:related rdf:resource="http://www.cognitiveatlas.org/id/trm_4b7497a289534"/>
		<skos:related rdf:resource="http://www.cognitiveatlas.org/id/tsk_4a57abb949a25"/>
		<skos:related rdf:resource="http://www.cognitiveatlas.org/id/trm_4c3e0a9576c3b"/>
		<skos:related rdf:resource="http://www.cognitiveatlas.org/id/tsk_4a57abb949e44"/>
		<skos:related rdf:resource="http://www.cognitiveatlas.org/id/trm_4b94affc43245"/>
		<skos:related rdf:resource="http://www.cognitiveatlas.org/id/trm_4a3fd79d0a8ed"/>
		<skos:related rdf:resource="http://www.cognitiveatlas.org/id/trm_4a3fd79d0b44c"/>
		<skos:related rdf:resource="http://www.cognitiveatlas.org/id/trm_4a3fd79d0b077"/>
		<skos:related rdf:resource="http://www.cognitiveatlas.org/id/trm_4a3fd79d0b077"/>
		<skos:related rdf:resource="http://www.cognitiveatlas.org/id/trm_4a3fd79d0b077"/>
		<skos:related rdf:resource="http://www.cognitiveatlas.org/id/trm_4a3fd79d0b077"/>
		<skos:related rdf:resource="http://www.cognitiveatlas.org/id/trm_4a3fd79d09f64"/>
		<skos:related rdf:resource="http://www.cognitiveatlas.org/id/trm_4a3fd79d09f64"/>
		<skos:related rdf:resource="http://www.cognitiveatlas.org/id/trm_4a3fd79d0a81b"/>
		<skos:related rdf:resource="http://www.cognitiveatlas.org/id/trm_4a3fd79d0a81b"/>
		<skos:related rdf:resource="http://www.cognitiveatlas.org/id/trm_4a3fd79d09d35"/>
		<skos:related rdf:resource="http://www.cognitiveatlas.org/id/trm_4b94b12bf0eb2"/>
		<skos:example>Backward digit span task is related to Wechsler Adult Intelligence Scale - Revised</skos:example>
		<skos:example>Block Design Test is descended from Wechsler Adult Intelligence Scale - Revised</skos:example>
		<skos:example>Digit/Symbol Coding test is descended from Wechsler Adult Intelligence Scale - Revised</skos:example>
		<skos:example>letter number sequencing is descended from Wechsler Adult Intelligence Scale - Revised</skos:example>
		<skos:example>symbol-digit substitution is descended from Wechsler Adult Intelligence Scale - Revised</skos:example>
		<skos:example>Wechsler Abbreviated Scale of Intelligence is descended from Wechsler Adult Intelligence Scale - Revised</skos:example>
		<skos:example>mental arithmetic is measured by the contrast of Arithmetic trials in the Wechsler Adult Intelligence Scale - Revised</skos:example>
		<skos:example>verbal fluency is measured by the contrast of Vocabulary trials in the Wechsler Adult Intelligence Scale - Revised</skos:example>
		<skos:example>semantic knowledge is measured by the contrast of Information trials in the Wechsler Adult Intelligence Scale - Revised</skos:example>
		<skos:example>semantic knowledge is measured by the contrast of Comprehension trials in the Wechsler Adult Intelligence Scale - Revised</skos:example>
		<skos:example>semantic knowledge is measured by the contrast of Similarities trials in the Wechsler Adult Intelligence Scale - Revised</skos:example>
		<skos:example>semantic knowledge is measured by the contrast of Picture Completion trials in the Wechsler Adult Intelligence Scale - Revised</skos:example>
		<skos:example>crystallized intelligence is measured by the contrast of Arithmetic trials in the Wechsler Adult Intelligence Scale - Revised</skos:example>
		<skos:example>crystallized intelligence is measured by the contrast of Block Design trials in the Wechsler Adult Intelligence Scale - Revised</skos:example>
		<skos:example>logical reasoning is measured by the contrast of Picture Completion trials in the Wechsler Adult Intelligence Scale - Revised</skos:example>
		<skos:example>logical reasoning is measured by the contrast of Picture Arrangement trials in the Wechsler Adult Intelligence Scale - Revised</skos:example>
		<skos:example>cognitive development is measured by the contrast of participant IQ minus average IQ trials in the Wechsler Adult Intelligence Scale - Revised</skos:example>
		<skos:example>Wechsler Memory Scale Fourth Edition is descended from Wechsler Adult Intelligence Scale - Revised</skos:example>
		<cito:citesForInformation rdf:resource="http://www.cognitiveatlas.org/citation/id/cit_4e01239970594"/>
		<cito:citesForInformation rdf:resource="http://www.cognitiveatlas.org/citation/id/cit_4e01295546406"/>
</skos:Concept><skos:Concept rdf:about="http://www.cognitiveatlas.org/id/tsk_4a57abb949f21"> <dc:identifier>tsk_4a57abb949f21</dc:identifier>
		<dc:Title>Cognitive Atlas : Lexicon : Wisconsin Card Sorting test</dc:Title>
		<dc:Description>RDF output for 'Wisconsin Card Sorting test'</dc:Description>
		<dc:Type>InteractiveResource</dc:Type>
		<dc:Publisher>Cognitive Atlas</dc:Publisher>
		<dc:Creator>Cognitive Atlas RDF Generator</dc:Creator>
		<dc:Contributor>Russ Poldrack</dc:Contributor>
		<dc:Date>2012-01-28 11:43:02</dc:Date>
		<dc:Format>text/rdf</dc:Format>
		<dc:Language>en</dc:Language>
		<skos:editorialNote>Generated by testgenall.php on Thu Mar 29 10:24:08 PDT 2012.</skos:editorialNote>
		<skos:historyNote>Revision 4: 3 previous definitions.</skos:historyNote>
		<skos:changeNote>See http://www.cognitiveatlas.org/id/tsk_4a57abb949f21 for complete revision history.</skos:changeNote>
		<skos:scopeNote>http://www.w3.org/2004/02/skos/core#Concept</skos:scopeNote>
		<skos:Note>SKOS properties defined in http://www.w3.org/TR/skos-primer/#secrel</skos:Note>
		<skos:inScheme rdf:resource="http://www.cognitiveatlas.org/tasks/"/>
		<skos:definition>The participant is presented with stimulus cards with shapes on them.  The cards differ in color of the shapes, number of the shapes, and the form of the shapes. The participant is asked to sort these cards into two piles. The participant is not told what stimulus dimension to use in order to sort the cards, but the administrator tells the participant if a particular match is correct. During the test, the sorting rules are changed and the participant must discover the new sorting rule in order to be successful. </skos:definition>
		<skos:prefLabel>Wisconsin Card Sorting test</skos:prefLabel>
		<skos:altLabel>WCST</skos:altLabel>
		<skos:related rdf:resource="http://www.cognitiveatlas.org/id/trm_4a3fd79d0b613"/>
		<skos:related rdf:resource="http://www.cognitiveatlas.org/id/trm_4a3fd79d0b5a7"/>
		<skos:related rdf:resource="http://www.cognitiveatlas.org/id/tsk_4a57abb949ad7"/>
		<skos:related rdf:resource="http://www.cognitiveatlas.org/id/trm_4a3fd79d0b607"/>
		<skos:related rdf:resource="http://www.cognitiveatlas.org/id/trm_4a3fd79d0b607"/>
		<skos:related rdf:resource="http://www.cognitiveatlas.org/id/tsk_4a57abb949dad"/>
		<skos:related rdf:resource="http://www.cognitiveatlas.org/id/trm_4a3fd79d0b607"/>
		<skos:related rdf:resource="http://www.cognitiveatlas.org/id/trm_4a3fd79d0a252"/>
		<skos:related rdf:resource="http://www.cognitiveatlas.org/id/trm_4a3fd79d09df0"/>
		<skos:example>task switching is measured by the contrast of Perseverative errors trials in the Wisconsin Card Sorting test</skos:example>
		<skos:example>working memory is measured by the contrast of Failure to maintain set trials in the Wisconsin Card Sorting test</skos:example>
		<skos:example>Intradimensional shift task is a broader synonym of Wisconsin Card Sorting test</skos:example>
		<skos:example>set shifting is measured by the contrast of Failure to maintain set trials in the Wisconsin Card Sorting test</skos:example>
		<skos:example>set shifting is measured by the contrast of Total number of categories acheived trials in the Wisconsin Card Sorting test</skos:example>
		<skos:example>Set-shifting task is a broader synonym of Wisconsin Card Sorting test</skos:example>
		<skos:example>set shifting is measured by the contrast of Total number of categories acheived trials in the Wisconsin Card Sorting test</skos:example>
		<skos:example>executive function is measured by the contrast of Total number of categories acheived trials in the Wisconsin Card Sorting test</skos:example>
		<skos:example>conceptual skill is measured by the contrast of Total number of categories acheived trials in the Wisconsin Card Sorting test</skos:example>
		<cito:citesForInformation rdf:resource="http://www.cognitiveatlas.org/citation/id/cit_4e021b91b722d"/>
		<cito:citesForInformation rdf:resource="http://www.cognitiveatlas.org/citation/id/cit_4e021ce008918"/>
</skos:Concept><skos:Concept rdf:about="http://www.cognitiveatlas.org/id/tsk_4a57abb949f2f"> <dc:identifier>tsk_4a57abb949f2f</dc:identifier>
		<dc:Title>Cognitive Atlas : Lexicon : word attack</dc:Title>
		<dc:Description>RDF output for 'word attack'</dc:Description>
		<dc:Type>InteractiveResource</dc:Type>
		<dc:Publisher>Cognitive Atlas</dc:Publisher>
		<dc:Creator>Cognitive Atlas RDF Generator</dc:Creator>
		<dc:Contributor>Carinna Torgerson</dc:Contributor>
		<dc:Date>2011-06-22 10:46:39</dc:Date>
		<dc:Format>text/rdf</dc:Format>
		<dc:Language>en</dc:Language>
		<skos:editorialNote>Generated by testgenall.php on Thu Mar 29 10:24:08 PDT 2012.</skos:editorialNote>
		<skos:historyNote>Revision 2: 1 previous definitions.</skos:historyNote>
		<skos:changeNote>See http://www.cognitiveatlas.org/id/tsk_4a57abb949f2f for complete revision history.</skos:changeNote>
		<skos:scopeNote>http://www.w3.org/2004/02/skos/core#Concept</skos:scopeNote>
		<skos:Note>SKOS properties defined in http://www.w3.org/TR/skos-primer/#secrel</skos:Note>
		<skos:inScheme rdf:resource="http://www.cognitiveatlas.org/tasks/"/>
		<skos:definition>Participants must read non-words aloud. Raw scores are converted into a &#34;reading comprehension age,&#34; which is then compared to the participant&#39;s real age to determine if they are a poor or gifted reader.</skos:definition>
		<skos:prefLabel>word attack</skos:prefLabel>
		<skos:altLabel></skos:altLabel>
		<skos:related rdf:resource="http://www.cognitiveatlas.org/id/trm_4a3fd79d0ac87"/>
		<skos:related rdf:resource="http://www.cognitiveatlas.org/id/trm_4a3fd79d0aeb6"/>
		<skos:related rdf:resource="http://www.cognitiveatlas.org/id/trm_4a3fd79d0b832"/>
		<skos:example>phonological encoding is measured by the contrast of reading comprehension age minus real age trials in the word attack</skos:example>
		<skos:example>reading is measured by the contrast of reading comprehension age minus real age trials in the word attack</skos:example>
		<skos:example>morphological processing is measured by the contrast of reading comprehension age minus real age trials in the word attack</skos:example>
		<cito:citesForInformation rdf:resource="http://www.cognitiveatlas.org/citation/id/cit_4e0220f770be9"/>
		<cito:citesForInformation rdf:resource="http://www.cognitiveatlas.org/citation/id/cit_4e02213bc1140"/>
		<cito:citesForInformation rdf:resource="http://www.cognitiveatlas.org/citation/id/cit_4e022a223d2f2"/>
</skos:Concept><skos:Concept rdf:about="http://www.cognitiveatlas.org/id/tsk_4a57abb949f3d"> <dc:identifier>tsk_4a57abb949f3d</dc:identifier>
		<dc:Title>Cognitive Atlas : Lexicon : Word generation task</dc:Title>
		<dc:Description>RDF output for 'Word generation task'</dc:Description>
		<dc:Type>InteractiveResource</dc:Type>
		<dc:Publisher>Cognitive Atlas</dc:Publisher>
		<dc:Creator>Cognitive Atlas RDF Generator</dc:Creator>
		<dc:Contributor>Brenda Gregory</dc:Contributor>
		<dc:Date>2011-04-19 12:06:57</dc:Date>
		<dc:Format>text/rdf</dc:Format>
		<dc:Language>en</dc:Language>
		<skos:editorialNote>Generated by testgenall.php on Thu Mar 29 10:24:08 PDT 2012.</skos:editorialNote>
		<skos:historyNote>Revision 3: 2 previous definitions.</skos:historyNote>
		<skos:changeNote>See http://www.cognitiveatlas.org/id/tsk_4a57abb949f3d for complete revision history.</skos:changeNote>
		<skos:scopeNote>http://www.w3.org/2004/02/skos/core#Concept</skos:scopeNote>
		<skos:Note>SKOS properties defined in http://www.w3.org/TR/skos-primer/#secrel</skos:Note>
		<skos:inScheme rdf:resource="http://www.cognitiveatlas.org/tasks/"/>
		<skos:definition>Covert: Semantic: subjects listen to or view nouns and silently generate an associated verb, or subjects view a category and silently generate as many exemplars as possible; Orthographic: subjects listen to or view a letter and silently generate as many words as possible that start with that letter; Phonologic: subjects listen to or view a word and silently generate words that rhyme. 

Overt: semantic: subjects listen to or view nouns and overtly generate an associated verb, or subjects view a category and overtly generate as many exemplars as possible; Orthographic: subjects listen to or view a letter and overtly generate as many words as possible that start with that letter; Phonologic: subjects listen to or view a word and overtly generate words that rhyme.</skos:definition>
		<skos:prefLabel>Word generation task</skos:prefLabel>
		<skos:altLabel></skos:altLabel>
		<skos:related rdf:resource="http://www.cognitiveatlas.org/id/trm_4a3fd79d0b87a"/>
		<skos:related rdf:resource="http://www.cognitiveatlas.org/id/trm_4a3fd79d0b44c"/>
		<skos:example>semantic processing is measured by the contrast of number of words divided by time trials in the Word generation task</skos:example>
		<skos:example>verbal fluency is measured by the contrast of number of words divided by time trials in the Word generation task</skos:example>
		<cito:citesForInformation rdf:resource="http://www.cognitiveatlas.org/citation/id/cit_4e022c2386f8e"/>
		<cito:citesForInformation rdf:resource="http://www.cognitiveatlas.org/citation/id/cit_4e022e5d93f39"/>
</skos:Concept><skos:Concept rdf:about="http://www.cognitiveatlas.org/id/tsk_4a57abb949f4a"> <dc:identifier>tsk_4a57abb949f4a</dc:identifier>
		<dc:Title>Cognitive Atlas : Lexicon : word identification</dc:Title>
		<dc:Description>RDF output for 'word identification'</dc:Description>
		<dc:Type>InteractiveResource</dc:Type>
		<dc:Publisher>Cognitive Atlas</dc:Publisher>
		<dc:Creator>Cognitive Atlas RDF Generator</dc:Creator>
		<dc:Contributor>Natalie Picchetti</dc:Contributor>
		<dc:Date>2011-04-15 12:01:55</dc:Date>
		<dc:Format>text/rdf</dc:Format>
		<dc:Language>en</dc:Language>
		<skos:editorialNote>Generated by testgenall.php on Thu Mar 29 10:24:08 PDT 2012.</skos:editorialNote>
		<skos:historyNote>Revision 3: 2 previous definitions.</skos:historyNote>
		<skos:changeNote>See http://www.cognitiveatlas.org/id/tsk_4a57abb949f4a for complete revision history.</skos:changeNote>
		<skos:scopeNote>http://www.w3.org/2004/02/skos/core#Concept</skos:scopeNote>
		<skos:Note>SKOS properties defined in http://www.w3.org/TR/skos-primer/#secrel</skos:Note>
		<skos:inScheme rdf:resource="http://www.cognitiveatlas.org/tasks/"/>
		<skos:definition>is the process of determining the pronunciation and some degree of meaning of an unknown word. Note: Word- identification skills commonly taught are phonic analysis, structural analysis, context clues, configuration clues, dictionary skills, and sometimes picture clues.
</skos:definition>
		<skos:prefLabel>word identification</skos:prefLabel>
		<skos:altLabel></skos:altLabel>
		<skos:related rdf:resource="http://www.cognitiveatlas.org/id/trm_4a3fd79d0b80f"/>
		<skos:related rdf:resource="http://www.cognitiveatlas.org/id/trm_4a3fd79d0ad41"/>
		<skos:related rdf:resource="http://www.cognitiveatlas.org/id/trm_4a3fd79d0b5a7"/>
		<skos:related rdf:resource="http://www.cognitiveatlas.org/id/trm_4a3fd79d0a4f9"/>
		<skos:example>lexical access is measured by the contrast of accuracy of participant minus average accuracy of controls trials in the word identification</skos:example>
		<skos:example>preattentive processing is measured by the contrast of primed identification trials in the word identification</skos:example>
		<skos:example>working memory is measured by the contrast of response time to known words minus (or learned words) response time to unknown words trials in the word identification</skos:example>
		<skos:example>iconic memory is measured by the contrast of perceptual identification trials in the word identification</skos:example>
		<cito:citesForInformation rdf:resource="http://www.cognitiveatlas.org/citation/id/cit_4e023c7f94536"/>
</skos:Concept><skos:Concept rdf:about="http://www.cognitiveatlas.org/id/trm_4d54b2cc0f943"> <dc:identifier>trm_4d54b2cc0f943</dc:identifier>
		<dc:Title>Cognitive Atlas : Lexicon : Cambridge Gambling Task</dc:Title>
		<dc:Description>RDF output for 'Cambridge Gambling Task'</dc:Description>
		<dc:Type>InteractiveResource</dc:Type>
		<dc:Publisher>Cognitive Atlas</dc:Publisher>
		<dc:Creator>Cognitive Atlas RDF Generator</dc:Creator>
		<dc:Contributor>Tom Schonberg</dc:Contributor>
		<dc:Date>2011-02-10 19:53:48</dc:Date>
		<dc:Format>text/rdf</dc:Format>
		<dc:Language>en</dc:Language>
		<skos:editorialNote>Generated by testgenall.php on Thu Mar 29 10:24:08 PDT 2012.</skos:editorialNote>
		<skos:historyNote>No previous definition revisions.</skos:historyNote>
		<skos:changeNote>This is the first and only definition provided.</skos:changeNote>
		<skos:scopeNote>http://www.w3.org/2004/02/skos/core#Concept</skos:scopeNote>
		<skos:Note>SKOS properties defined in http://www.w3.org/TR/skos-primer/#secrel</skos:Note>
		<skos:inScheme rdf:resource="http://www.cognitiveatlas.org/tasks/"/>
		<skos:definition>A behavioral task intended to measure risky decision making by subjects.
A token is hidden under one of six boxes that are each one of two colors.Different trials
have different ratios between box colors(3:3,4:2,5:1).On each trial,participants choose a
color on which to bet.The color with the higher probability (more boxes) is associated with
lower potential gains and lower potential losses of points than is the color with lower
probability. </skos:definition>
		<skos:prefLabel>Cambridge Gambling Task</skos:prefLabel>
		<skos:altLabel></skos:altLabel>
		<skos:related rdf:resource="http://www.cognitiveatlas.org/id/trm_4a3fd79d0b64e"/>
		<skos:related rdf:resource="http://www.cognitiveatlas.org/id/trm_4b6525253c63f"/>
		<skos:related rdf:resource="http://www.cognitiveatlas.org/id/trm_4d55a2bbcfdff"/>
		<skos:related rdf:resource="http://www.cognitiveatlas.org/id/tsk_4a57abb949ae5"/>
		<skos:example>Cambridge Gambling Task is a narrower synonym of Choice task between risky and non-risky options</skos:example>
		<skos:example>Cambridge Gambling Task is related to Iowa Gambling Task</skos:example>
		<skos:example>risk seeking is measured by the contrast of correct answers times probability of each color trials in the Cambridge Gambling Task</skos:example>
		<skos:example>reward is measured by the contrast of ratio trials in the Cambridge Gambling Task</skos:example>
		<cito:citesForInformation rdf:resource="http://www.cognitiveatlas.org/citation/id/cit_4d54b48147b06"/>
		<cito:citesForInformation rdf:resource="http://www.cognitiveatlas.org/citation/id/cit_4de6b6e412117"/>
		<cito:citesForInformation rdf:resource="http://www.cognitiveatlas.org/citation/id/cit_4de6b72e283ad"/>
</skos:Concept><skos:Concept rdf:about="http://www.cognitiveatlas.org/id/trm_4d54b61a14a14"> <dc:identifier>trm_4d54b61a14a14</dc:identifier>
		<dc:Title>Cognitive Atlas : Lexicon : Probabilistic gambling task</dc:Title>
		<dc:Description>RDF output for 'Probabilistic gambling task'</dc:Description>
		<dc:Type>InteractiveResource</dc:Type>
		<dc:Publisher>Cognitive Atlas</dc:Publisher>
		<dc:Creator>Cognitive Atlas RDF Generator</dc:Creator>
		<dc:Contributor>Tom Schonberg</dc:Contributor>
		<dc:Date>2011-02-11 13:02:24</dc:Date>
		<dc:Format>text/rdf</dc:Format>
		<dc:Language>en</dc:Language>
		<skos:editorialNote>Generated by testgenall.php on Thu Mar 29 10:24:08 PDT 2012.</skos:editorialNote>
		<skos:historyNote>Revision 2: 1 previous definitions.</skos:historyNote>
		<skos:changeNote>See http://www.cognitiveatlas.org/id/trm_4d54b61a14a14 for complete revision history.</skos:changeNote>
		<skos:scopeNote>http://www.w3.org/2004/02/skos/core#Concept</skos:scopeNote>
		<skos:Note>SKOS properties defined in http://www.w3.org/TR/skos-primer/#secrel</skos:Note>
		<skos:inScheme rdf:resource="http://www.cognitiveatlas.org/tasks/"/>
		<skos:definition>Two cards are drawn without replacement from a deck containing cards numbered from one to ten (one of each). After the first card is presented, participants bet whether the next card will be higher or lower than the first card. Thus there is maximal risk when the first card is five or six, zero risk when it is ten or one. 

In later version of the task participants bet on whether the second card will be higher or lower before seeing the first card.</skos:definition>
		<skos:prefLabel>Probabilistic gambling task</skos:prefLabel>
		<skos:altLabel></skos:altLabel>
		<skos:related rdf:resource="http://www.cognitiveatlas.org/id/trm_4a3fd79d0a585"/>
		<skos:related rdf:resource="http://www.cognitiveatlas.org/id/trm_4a3fd79d0b64e"/>
		<skos:example> is measured by Probabilistic gambling task</skos:example>
		<skos:example>risk seeking is measured by the contrast of accuracy of participant minus average accuracy of controls trials in the Probabilistic gambling task</skos:example>
		<cito:citesForInformation rdf:resource="http://www.cognitiveatlas.org/citation/id/cit_4d54b62d050c7"/>
		<cito:citesForInformation rdf:resource="http://www.cognitiveatlas.org/citation/id/cit_4d54b63f0dcd8"/>
		<cito:citesForInformation rdf:resource="http://www.cognitiveatlas.org/citation/id/cit_4d54b673a9469"/>
		<cito:citesForInformation rdf:resource="http://www.cognitiveatlas.org/citation/id/cit_4df8ef325c153"/>
</skos:Concept><skos:Concept rdf:about="http://www.cognitiveatlas.org/id/trm_4d54b8361e93e"> <dc:identifier>trm_4d54b8361e93e</dc:identifier>
		<dc:Title>Cognitive Atlas : Lexicon : Behavioral Investment allocation strategy (BIAS)</dc:Title>
		<dc:Description>RDF output for 'Behavioral Investment allocation strategy (BIAS)'</dc:Description>
		<dc:Type>InteractiveResource</dc:Type>
		<dc:Publisher>Cognitive Atlas</dc:Publisher>
		<dc:Creator>Cognitive Atlas RDF Generator</dc:Creator>
		<dc:Contributor>Tom Schonberg</dc:Contributor>
		<dc:Date>2011-02-10 20:16:54</dc:Date>
		<dc:Format>text/rdf</dc:Format>
		<dc:Language>en</dc:Language>
		<skos:editorialNote>Generated by testgenall.php on Thu Mar 29 10:24:08 PDT 2012.</skos:editorialNote>
		<skos:historyNote>No previous definition revisions.</skos:historyNote>
		<skos:changeNote>This is the first and only definition provided.</skos:changeNote>
		<skos:scopeNote>http://www.w3.org/2004/02/skos/core#Concept</skos:scopeNote>
		<skos:Note>SKOS properties defined in http://www.w3.org/TR/skos-primer/#secrel</skos:Note>
		<skos:inScheme rdf:resource="http://www.cognitiveatlas.org/tasks/"/>
		<skos:definition>On each trial, participants choose between two stocks (gain/loss gambles, one stochastically dominating the other) and one bond (a sure gain of $1). They must learn through trial-and-error the characteristics of the stocks, which change over blocks of trials. Feedback on payoffs of the forgone options is presented on each trial. </skos:definition>
		<skos:prefLabel>Behavioral Investment allocation strategy (BIAS)</skos:prefLabel>
		<skos:altLabel></skos:altLabel>
		<skos:related rdf:resource="http://www.cognitiveatlas.org/id/trm_4d55a2bbcfdff"/>
		<skos:example>Behavioral Investment allocation strategy (BIAS) is a narrower synonym of Choice task between risky and non-risky options</skos:example>
		<cito:citesForInformation rdf:resource="http://www.cognitiveatlas.org/citation/id/cit_4d54b861dc450"/>
		<cito:citesForInformation rdf:resource="http://www.cognitiveatlas.org/citation/id/cit_4de57c44b29d6"/>
</skos:Concept><skos:Concept rdf:about="http://www.cognitiveatlas.org/id/trm_4d55997cd3edb"> <dc:identifier>trm_4d55997cd3edb</dc:identifier>
		<dc:Title>Cognitive Atlas : Lexicon : Non-choice task to study expected value and uncertainty</dc:Title>
		<dc:Description>RDF output for 'Non-choice task to study expected value and uncertainty'</dc:Description>
		<dc:Type>InteractiveResource</dc:Type>
		<dc:Publisher>Cognitive Atlas</dc:Publisher>
		<dc:Creator>Cognitive Atlas RDF Generator</dc:Creator>
		<dc:Contributor>Tom Schonberg</dc:Contributor>
		<dc:Date>2011-02-11 12:18:04</dc:Date>
		<dc:Format>text/rdf</dc:Format>
		<dc:Language>en</dc:Language>
		<skos:editorialNote>Generated by testgenall.php on Thu Mar 29 10:24:08 PDT 2012.</skos:editorialNote>
		<skos:historyNote>No previous definition revisions.</skos:historyNote>
		<skos:changeNote>This is the first and only definition provided.</skos:changeNote>
		<skos:scopeNote>http://www.w3.org/2004/02/skos/core#Concept</skos:scopeNote>
		<skos:Note>SKOS properties defined in http://www.w3.org/TR/skos-primer/#secrel</skos:Note>
		<skos:inScheme rdf:resource="http://www.cognitiveatlas.org/tasks/"/>
		<skos:definition>Each of 12 stimuli (circles of different colors, numbers and sizes) is associated with a different reward magnitude and probability. These include all combinations of (100 and 200) point rewards with (0, 0.25, 0.5, 0.75 and 1) probabilities, plus 300 and 400 rewards with 0.5 probability. Participants are first trained to learn the probabilities and outcomes associated with each stimulus. Next, on each trial, a stimulus appears in one of four quadrants of the screen, and participants indicate which quadrant using a button press</skos:definition>
		<skos:prefLabel>Non-choice task to study expected value and uncertainty</skos:prefLabel>
		<skos:altLabel></skos:altLabel>
		<skos:related rdf:resource="http://www.cognitiveatlas.org/id/trm_4a3fd79d0b64e"/>
		<skos:related rdf:resource="http://www.cognitiveatlas.org/id/trm_4a3fd79d0b64e"/>
		<skos:example>risk seeking is measured by the contrast of response time to risky choices minus response time to non-risky choices trials in the Non-choice task to study expected value and uncertainty</skos:example>
		<skos:example>risk seeking is measured by the contrast of number of participant&#39;s risky choices minus average number of risky choices trials in the Non-choice task to study expected value and uncertainty</skos:example>
		<cito:citesForInformation rdf:resource="http://www.cognitiveatlas.org/citation/id/cit_4d55999f3f7c9"/>
</skos:Concept><skos:Concept rdf:about="http://www.cognitiveatlas.org/id/trm_4d559bcd67c18"> <dc:identifier>trm_4d559bcd67c18</dc:identifier>
		<dc:Title>Cognitive Atlas : Lexicon : Balloon Analogue Risk Task (BART)</dc:Title>
		<dc:Description>RDF output for 'Balloon Analogue Risk Task (BART)'</dc:Description>
		<dc:Type>InteractiveResource</dc:Type>
		<dc:Publisher>Cognitive Atlas</dc:Publisher>
		<dc:Creator>Cognitive Atlas RDF Generator</dc:Creator>
		<dc:Contributor>Tom Schonberg</dc:Contributor>
		<dc:Date>2011-02-11 12:27:57</dc:Date>
		<dc:Format>text/rdf</dc:Format>
		<dc:Language>en</dc:Language>
		<skos:editorialNote>Generated by testgenall.php on Thu Mar 29 10:24:08 PDT 2012.</skos:editorialNote>
		<skos:historyNote>No previous definition revisions.</skos:historyNote>
		<skos:changeNote>This is the first and only definition provided.</skos:changeNote>
		<skos:scopeNote>http://www.w3.org/2004/02/skos/core#Concept</skos:scopeNote>
		<skos:Note>SKOS properties defined in http://www.w3.org/TR/skos-primer/#secrel</skos:Note>
		<skos:inScheme rdf:resource="http://www.cognitiveatlas.org/tasks/"/>
		<skos:definition>On each trial, participants pump a simulated balloon without knowing when it will explode. Each pump increases the potential reward to be gained but also the probability of explosion, whichwipesoutallpotentialgains for that trial. Inmoststudies,balloonexplosionprobabilities are drawn from a uniform distribution, and participants must learn explosion probabilities through trial-and-error.</skos:definition>
		<skos:prefLabel>Balloon Analogue Risk Task (BART)</skos:prefLabel>
		<skos:altLabel></skos:altLabel>
		<skos:related rdf:resource="http://www.cognitiveatlas.org/id/trm_4a3fd79d0b64e"/>
		<skos:related rdf:resource="http://www.cognitiveatlas.org/id/tsk_4a57abb949d5b"/>
		<skos:example>risk seeking is measured by the contrast of negative feedback trials in the Balloon Analogue Risk Task (BART)</skos:example>
		<skos:example>Risky Gains task is related to Balloon Analogue Risk Task (BART)</skos:example>
		<cito:citesForInformation rdf:resource="http://www.cognitiveatlas.org/citation/id/cit_4d559c4dec264"/>
		<cito:citesForInformation rdf:resource="http://www.cognitiveatlas.org/citation/id/cit_4d559c87f3173"/>
		<cito:citesForInformation rdf:resource="http://www.cognitiveatlas.org/citation/id/cit_4d559cff860c8"/>
		<cito:citesForInformation rdf:resource="http://www.cognitiveatlas.org/citation/id/cit_4de57915b0eac"/>
</skos:Concept><skos:Concept rdf:about="http://www.cognitiveatlas.org/id/trm_4d559d2703bae"> <dc:identifier>trm_4d559d2703bae</dc:identifier>
		<dc:Title>Cognitive Atlas : Lexicon : Devils Task</dc:Title>
		<dc:Description>RDF output for 'Devils Task'</dc:Description>
		<dc:Type>InteractiveResource</dc:Type>
		<dc:Publisher>Cognitive Atlas</dc:Publisher>
		<dc:Creator>Cognitive Atlas RDF Generator</dc:Creator>
		<dc:Contributor>Tom Schonberg</dc:Contributor>
		<dc:Date>2011-02-11 12:33:43</dc:Date>
		<dc:Format>text/rdf</dc:Format>
		<dc:Language>en</dc:Language>
		<skos:editorialNote>Generated by testgenall.php on Thu Mar 29 10:24:08 PDT 2012.</skos:editorialNote>
		<skos:historyNote>No previous definition revisions.</skos:historyNote>
		<skos:changeNote>This is the first and only definition provided.</skos:changeNote>
		<skos:scopeNote>http://www.w3.org/2004/02/skos/core#Concept</skos:scopeNote>
		<skos:Note>SKOS properties defined in http://www.w3.org/TR/skos-primer/#secrel</skos:Note>
		<skos:inScheme rdf:resource="http://www.cognitiveatlas.org/tasks/"/>
		<skos:definition>This task is a forerunner to the BART: on each trial, participants decide howmany of seven treasure chests to open. They are informed that six boxes contain a prize and one box contains a ‘devil’ that will cause themto lose all their potential gains on that trial. Similar to the BART, participants make sequential choices and, after opening each chest, decide whether to continue to the next chest or cash in their earnings to that point.</skos:definition>
		<skos:prefLabel>Devils Task</skos:prefLabel>
		<skos:altLabel></skos:altLabel>
		<skos:related rdf:resource="http://www.cognitiveatlas.org/id/trm_4a3fd79d0b64e"/>
		<skos:example>risk seeking is measured by the contrast of negative feedback trials in the Devils Task</skos:example>
		<cito:citesForInformation rdf:resource="http://www.cognitiveatlas.org/citation/id/cit_4d559d7572d80"/>
		<cito:citesForInformation rdf:resource="http://www.cognitiveatlas.org/citation/id/cit_4d559e9ca6aaf"/>
</skos:Concept><skos:Concept rdf:about="http://www.cognitiveatlas.org/id/trm_4d55a2bbcfdff"> <dc:identifier>trm_4d55a2bbcfdff</dc:identifier>
		<dc:Title>Cognitive Atlas : Lexicon : Choice task between risky and non-risky options</dc:Title>
		<dc:Description>RDF output for 'Choice task between risky and non-risky options'</dc:Description>
		<dc:Type>InteractiveResource</dc:Type>
		<dc:Publisher>Cognitive Atlas</dc:Publisher>
		<dc:Creator>Cognitive Atlas RDF Generator</dc:Creator>
		<dc:Contributor>Carinna Torgerson</dc:Contributor>
		<dc:Date>2011-06-01 16:02:57</dc:Date>
		<dc:Format>text/rdf</dc:Format>
		<dc:Language>en</dc:Language>
		<skos:editorialNote>Generated by testgenall.php on Thu Mar 29 10:24:08 PDT 2012.</skos:editorialNote>
		<skos:historyNote>Revision 3: 2 previous definitions.</skos:historyNote>
		<skos:changeNote>See http://www.cognitiveatlas.org/id/trm_4d55a2bbcfdff for complete revision history.</skos:changeNote>
		<skos:scopeNote>http://www.w3.org/2004/02/skos/core#Concept</skos:scopeNote>
		<skos:Note>SKOS properties defined in http://www.w3.org/TR/skos-primer/#secrel</skos:Note>
		<skos:inScheme rdf:resource="http://www.cognitiveatlas.org/tasks/"/>
		<skos:definition>a choice made between two or more options when one of those options has some probability >0 of producing either a reinforcing or an aversive consequence</skos:definition>
		<skos:prefLabel>Choice task between risky and non-risky options</skos:prefLabel>
		<skos:altLabel></skos:altLabel>
		<skos:related rdf:resource="http://www.cognitiveatlas.org/id/trm_4d54b8361e93e"/>
		<skos:related rdf:resource="http://www.cognitiveatlas.org/id/trm_4a3fd79d0b64e"/>
		<skos:related rdf:resource="http://www.cognitiveatlas.org/id/trm_4d54b2cc0f943"/>
		<skos:related rdf:resource="http://www.cognitiveatlas.org/id/tsk_4a57abb949ae5"/>
		<skos:related rdf:resource="http://www.cognitiveatlas.org/id/tsk_4a57abb949d5b"/>
		<skos:example>Behavioral Investment allocation strategy (BIAS) is a narrower synonym of Choice task between risky and non-risky options</skos:example>
		<skos:example>risk seeking is measured by the contrast of risky option trials in the Choice task between risky and non-risky options</skos:example>
		<skos:example>Cambridge Gambling Task is a narrower synonym of Choice task between risky and non-risky options</skos:example>
		<skos:example>Iowa Gambling Task is a narrower synonym of Choice task between risky and non-risky options</skos:example>
		<skos:example>Risky Gains task is a narrower synonym of Choice task between risky and non-risky options</skos:example>
		<cito:citesForInformation rdf:resource="http://www.cognitiveatlas.org/citation/id/cit_4d55a32988c87"/>
		<cito:citesForInformation rdf:resource="http://www.cognitiveatlas.org/citation/id/cit_4d55a34cc2ddc"/>
</skos:Concept><skos:Concept rdf:about="http://www.cognitiveatlas.org/id/trm_4d8a48e403c78"> <dc:identifier>trm_4d8a48e403c78</dc:identifier>
		<dc:Title>Cognitive Atlas : Lexicon : Inductive reasoning aptitude</dc:Title>
		<dc:Description>RDF output for 'Inductive reasoning aptitude'</dc:Description>
		<dc:Type>InteractiveResource</dc:Type>
		<dc:Publisher>Cognitive Atlas</dc:Publisher>
		<dc:Creator>Cognitive Atlas RDF Generator</dc:Creator>
		<dc:Contributor>Natalie Picchetti</dc:Contributor>
		<dc:Date>2011-04-01 12:54:26</dc:Date>
		<dc:Format>text/rdf</dc:Format>
		<dc:Language>en</dc:Language>
		<skos:editorialNote>Generated by testgenall.php on Thu Mar 29 10:24:08 PDT 2012.</skos:editorialNote>
		<skos:historyNote>Revision 2: 1 previous definitions.</skos:historyNote>
		<skos:changeNote>See http://www.cognitiveatlas.org/id/trm_4d8a48e403c78 for complete revision history.</skos:changeNote>
		<skos:scopeNote>http://www.w3.org/2004/02/skos/core#Concept</skos:scopeNote>
		<skos:Note>SKOS properties defined in http://www.w3.org/TR/skos-primer/#secrel</skos:Note>
		<skos:inScheme rdf:resource="http://www.cognitiveatlas.org/tasks/"/>
		<skos:definition>is a measurable aptitude for how well a person can identify a pattern within a large amount of data. 


</skos:definition>
		<skos:prefLabel>Inductive reasoning aptitude</skos:prefLabel>
		<skos:altLabel></skos:altLabel>
		<skos:related rdf:resource="http://www.cognitiveatlas.org/id/trm_4a3fd79d0a590"/>
		<skos:related rdf:resource="http://www.cognitiveatlas.org/id/trm_4a3fd79d0aec1"/>
		<skos:example>inductive reasoning is measured by the contrast of accuracy of participant minus average accuracy of controls trials in the Inductive reasoning aptitude</skos:example>
		<skos:example>reasoning is measured by the contrast of accuracy of participant minus average accuracy of controls trials in the Inductive reasoning aptitude</skos:example>
		<cito:citesForInformation rdf:resource="http://www.cognitiveatlas.org/citation/id/cit_4dee65850762a"/>
		<cito:citesForInformation rdf:resource="http://www.cognitiveatlas.org/citation/id/cit_4dee7f7b59573"/>
		<cito:citesForInformation rdf:resource="http://www.cognitiveatlas.org/citation/id/cit_4dee7ffa55ee8"/>
</skos:Concept><skos:Concept rdf:about="http://www.cognitiveatlas.org/id/trm_4d949c5b0e380"> <dc:identifier>trm_4d949c5b0e380</dc:identifier>
		<dc:Title>Cognitive Atlas : Lexicon : Rhyme verification task</dc:Title>
		<dc:Description>RDF output for 'Rhyme verification task'</dc:Description>
		<dc:Type>InteractiveResource</dc:Type>
		<dc:Publisher>Cognitive Atlas</dc:Publisher>
		<dc:Creator>Cognitive Atlas RDF Generator</dc:Creator>
		<dc:Contributor>Russ Poldrack</dc:Contributor>
		<dc:Date>2012-01-28 07:38:09</dc:Date>
		<dc:Format>text/rdf</dc:Format>
		<dc:Language>en</dc:Language>
		<skos:editorialNote>Generated by testgenall.php on Thu Mar 29 10:24:08 PDT 2012.</skos:editorialNote>
		<skos:historyNote>Revision 5: 4 previous definitions.</skos:historyNote>
		<skos:changeNote>See http://www.cognitiveatlas.org/id/trm_4d949c5b0e380 for complete revision history.</skos:changeNote>
		<skos:scopeNote>http://www.w3.org/2004/02/skos/core#Concept</skos:scopeNote>
		<skos:Note>SKOS properties defined in http://www.w3.org/TR/skos-primer/#secrel</skos:Note>
		<skos:inScheme rdf:resource="http://www.cognitiveatlas.org/tasks/"/>
		<skos:definition>Stimuli are presented in pairs (either words or pseudowords) and the subject is asked to judge whether the pair of stimuli rhyme with one another.</skos:definition>
		<skos:prefLabel>Rhyme verification task</skos:prefLabel>
		<skos:altLabel>rhyming judgment task, rhyming task, rhyme task, rhyme judgment task, rhyme decision task, rhyming decision task</skos:altLabel>
		<skos:related rdf:resource="http://www.cognitiveatlas.org/id/trm_4a3fd79d0b832"/>
		<skos:related rdf:resource="http://www.cognitiveatlas.org/id/trm_4a3fd79d0b832"/>
		<skos:related rdf:resource="http://www.cognitiveatlas.org/id/trm_4a3fd79d0b2b4"/>
		<skos:related rdf:resource="http://www.cognitiveatlas.org/id/trm_4a3fd79d0b58f"/>
		<skos:related rdf:resource="http://www.cognitiveatlas.org/id/trm_4a3fd79d0ac87"/>
		<skos:related rdf:resource="http://www.cognitiveatlas.org/id/trm_4a3fd79d0ac87"/>
		<skos:example>morphological processing is measured by the contrast of Word - baseline trials in the Rhyme verification task</skos:example>
		<skos:example>morphological processing is measured by the contrast of Pseudoword - baseline trials in the Rhyme verification task</skos:example>
		<skos:example>sublexical route is measured by the contrast of Pseudoword - baseline trials in the Rhyme verification task</skos:example>
		<skos:example>word recognition is measured by the contrast of Pseudoword - word trials in the Rhyme verification task</skos:example>
		<skos:example>phonological encoding is measured by the contrast of Word - baseline trials in the Rhyme verification task</skos:example>
		<skos:example>phonological encoding is measured by the contrast of Pseudoword - baseline trials in the Rhyme verification task</skos:example>
		<cito:citesForInformation rdf:resource="http://www.cognitiveatlas.org/citation/id/cit_4df940ded0659"/>
</skos:Concept><skos:Concept rdf:about="http://www.cognitiveatlas.org/id/trm_4da4b203ad5ae"> <dc:identifier>trm_4da4b203ad5ae</dc:identifier>
		<dc:Title>Cognitive Atlas : Lexicon : selective stop signal task</dc:Title>
		<dc:Description>RDF output for 'selective stop signal task'</dc:Description>
		<dc:Type>InteractiveResource</dc:Type>
		<dc:Publisher>Cognitive Atlas</dc:Publisher>
		<dc:Creator>Cognitive Atlas RDF Generator</dc:Creator>
		<dc:Contributor>Russ Poldrack</dc:Contributor>
		<dc:Date>2011-04-12 13:11:47</dc:Date>
		<dc:Format>text/rdf</dc:Format>
		<dc:Language>en</dc:Language>
		<skos:editorialNote>Generated by testgenall.php on Thu Mar 29 10:24:08 PDT 2012.</skos:editorialNote>
		<skos:historyNote>No previous definition revisions.</skos:historyNote>
		<skos:changeNote>This is the first and only definition provided.</skos:changeNote>
		<skos:scopeNote>http://www.w3.org/2004/02/skos/core#Concept</skos:scopeNote>
		<skos:Note>SKOS properties defined in http://www.w3.org/TR/skos-primer/#secrel</skos:Note>
		<skos:inScheme rdf:resource="http://www.cognitiveatlas.org/tasks/"/>
		<skos:definition>A version of the stop signal task where inhibition is contingent upon both the presence of the stop signal and the particular stimulus.  </skos:definition>
		<skos:prefLabel>selective stop signal task</skos:prefLabel>
		<skos:altLabel></skos:altLabel>
		<skos:related rdf:resource="http://www.cognitiveatlas.org/id/tsk_4a57abb949e1a"/>
		<skos:example>selective stop signal task is descended from stop signal task</skos:example>
</skos:Concept><skos:Concept rdf:about="http://www.cognitiveatlas.org/id/trm_4da6304c9aa23"> <dc:identifier>trm_4da6304c9aa23</dc:identifier>
		<dc:Title>Cognitive Atlas : Lexicon : attention networks test</dc:Title>
		<dc:Description>RDF output for 'attention networks test'</dc:Description>
		<dc:Type>InteractiveResource</dc:Type>
		<dc:Publisher>Cognitive Atlas</dc:Publisher>
		<dc:Creator>Cognitive Atlas RDF Generator</dc:Creator>
		<dc:Contributor>Corey White</dc:Contributor>
		<dc:Date>2011-08-18 07:56:14</dc:Date>
		<dc:Format>text/rdf</dc:Format>
		<dc:Language>en</dc:Language>
		<skos:editorialNote>Generated by testgenall.php on Thu Mar 29 10:24:08 PDT 2012.</skos:editorialNote>
		<skos:historyNote>Revision 4: 3 previous definitions.</skos:historyNote>
		<skos:changeNote>See http://www.cognitiveatlas.org/id/trm_4da6304c9aa23 for complete revision history.</skos:changeNote>
		<skos:scopeNote>http://www.w3.org/2004/02/skos/core#Concept</skos:scopeNote>
		<skos:Note>SKOS properties defined in http://www.w3.org/TR/skos-primer/#secrel</skos:Note>
		<skos:inScheme rdf:resource="http://www.cognitiveatlas.org/tasks/"/>
		<skos:definition>involves presenting participants with flanker stimuli in which a target item (>) is surrounded by congruent (> > > > >), neutral (- - > - -), or incongruent ( > >  >) flankers.  Stimulus presentation is preceded by different cue conditions and the participant is instructed to identify the target stimulus.</skos:definition>
		<skos:prefLabel>attention networks test</skos:prefLabel>
		<skos:altLabel></skos:altLabel>
		<skos:related rdf:resource="http://www.cognitiveatlas.org/id/trm_4a3fd79d0b5fb"/>
		<skos:related rdf:resource="http://www.cognitiveatlas.org/id/trm_4a3fd79d0a246"/>
		<skos:example>attention shifting is measured by the contrast of  trials in the attention networks test</skos:example>
		<skos:example>executive control is measured by the contrast of  trials in the attention networks test</skos:example>
		<cito:citesForInformation rdf:resource="http://www.cognitiveatlas.org/citation/id/cit_4e496a66946fb"/>
</skos:Concept><skos:Concept rdf:about="http://www.cognitiveatlas.org/id/trm_4da630c52c011"> <dc:identifier>trm_4da630c52c011</dc:identifier>
		<dc:Title>Cognitive Atlas : Lexicon : delayed discounting task</dc:Title>
		<dc:Description>RDF output for 'delayed discounting task'</dc:Description>
		<dc:Type>InteractiveResource</dc:Type>
		<dc:Publisher>Cognitive Atlas</dc:Publisher>
		<dc:Creator>Cognitive Atlas RDF Generator</dc:Creator>
		<dc:Contributor>John Clithero</dc:Contributor>
		<dc:Date>2011-05-23 14:09:43</dc:Date>
		<dc:Format>text/rdf</dc:Format>
		<dc:Language>en</dc:Language>
		<skos:editorialNote>Generated by testgenall.php on Thu Mar 29 10:24:08 PDT 2012.</skos:editorialNote>
		<skos:historyNote>Revision 2: 1 previous definitions.</skos:historyNote>
		<skos:changeNote>See http://www.cognitiveatlas.org/id/trm_4da630c52c011 for complete revision history.</skos:changeNote>
		<skos:scopeNote>http://www.w3.org/2004/02/skos/core#Concept</skos:scopeNote>
		<skos:Note>SKOS properties defined in http://www.w3.org/TR/skos-primer/#secrel</skos:Note>
		<skos:inScheme rdf:resource="http://www.cognitiveatlas.org/tasks/"/>
		<skos:definition>A task for identifying preferences over tradeoffs between costs and benefits occurring at different times.</skos:definition>
		<skos:prefLabel>delayed discounting task</skos:prefLabel>
		<skos:altLabel></skos:altLabel>
		<cito:citesForInformation rdf:resource="http://www.cognitiveatlas.org/citation/id/cit_4ddacd3d36e2d"/>
		<cito:citesForInformation rdf:resource="http://www.cognitiveatlas.org/citation/id/cit_4ddacd4fca66f"/>
		<cito:citesForInformation rdf:resource="http://www.cognitiveatlas.org/citation/id/cit_4ddacd68cee59"/>
</skos:Concept><skos:Concept rdf:about="http://www.cognitiveatlas.org/id/trm_4da63146f12d7"> <dc:identifier>trm_4da63146f12d7</dc:identifier>
		<dc:Title>Cognitive Atlas : Lexicon : remember/know task</dc:Title>
		<dc:Description>RDF output for 'remember/know task'</dc:Description>
		<dc:Type>InteractiveResource</dc:Type>
		<dc:Publisher>Cognitive Atlas</dc:Publisher>
		<dc:Creator>Cognitive Atlas RDF Generator</dc:Creator>
		<dc:Contributor>Natalie Picchetti</dc:Contributor>
		<dc:Date>2011-04-13 16:27:02</dc:Date>
		<dc:Format>text/rdf</dc:Format>
		<dc:Language>en</dc:Language>
		<skos:editorialNote>Generated by testgenall.php on Thu Mar 29 10:24:08 PDT 2012.</skos:editorialNote>
		<skos:historyNote>No previous definition revisions.</skos:historyNote>
		<skos:changeNote>This is the first and only definition provided.</skos:changeNote>
		<skos:scopeNote>http://www.w3.org/2004/02/skos/core#Concept</skos:scopeNote>
		<skos:Note>SKOS properties defined in http://www.w3.org/TR/skos-primer/#secrel</skos:Note>
		<skos:inScheme rdf:resource="http://www.cognitiveatlas.org/tasks/"/>
		<skos:definition>No definition submitted yet.</skos:definition>
		<skos:prefLabel>remember/know task</skos:prefLabel>
		<skos:altLabel></skos:altLabel>
</skos:Concept><skos:Concept rdf:about="http://www.cognitiveatlas.org/id/trm_4da6318f7381b"> <dc:identifier>trm_4da6318f7381b</dc:identifier>
		<dc:Title>Cognitive Atlas : Lexicon : probabilistic reversal learning</dc:Title>
		<dc:Description>RDF output for 'probabilistic reversal learning'</dc:Description>
		<dc:Type>InteractiveResource</dc:Type>
		<dc:Publisher>Cognitive Atlas</dc:Publisher>
		<dc:Creator>Cognitive Atlas RDF Generator</dc:Creator>
		<dc:Contributor>Natalie Picchetti</dc:Contributor>
		<dc:Date>2011-04-13 16:28:15</dc:Date>
		<dc:Format>text/rdf</dc:Format>
		<dc:Language>en</dc:Language>
		<skos:editorialNote>Generated by testgenall.php on Thu Mar 29 10:24:08 PDT 2012.</skos:editorialNote>
		<skos:historyNote>No previous definition revisions.</skos:historyNote>
		<skos:changeNote>This is the first and only definition provided.</skos:changeNote>
		<skos:scopeNote>http://www.w3.org/2004/02/skos/core#Concept</skos:scopeNote>
		<skos:Note>SKOS properties defined in http://www.w3.org/TR/skos-primer/#secrel</skos:Note>
		<skos:inScheme rdf:resource="http://www.cognitiveatlas.org/tasks/"/>
		<skos:definition>No definition submitted yet.</skos:definition>
		<skos:prefLabel>probabilistic reversal learning</skos:prefLabel>
		<skos:altLabel></skos:altLabel>
</skos:Concept><skos:Concept rdf:about="http://www.cognitiveatlas.org/id/trm_4da631be60291"> <dc:identifier>trm_4da631be60291</dc:identifier>
		<dc:Title>Cognitive Atlas : Lexicon : Counting Stroop Task</dc:Title>
		<dc:Description>RDF output for 'Counting Stroop Task'</dc:Description>
		<dc:Type>InteractiveResource</dc:Type>
		<dc:Publisher>Cognitive Atlas</dc:Publisher>
		<dc:Creator>Cognitive Atlas RDF Generator</dc:Creator>
		<dc:Contributor>Natalie Picchetti</dc:Contributor>
		<dc:Date>2011-04-13 16:29:02</dc:Date>
		<dc:Format>text/rdf</dc:Format>
		<dc:Language>en</dc:Language>
		<skos:editorialNote>Generated by testgenall.php on Thu Mar 29 10:24:08 PDT 2012.</skos:editorialNote>
		<skos:historyNote>No previous definition revisions.</skos:historyNote>
		<skos:changeNote>This is the first and only definition provided.</skos:changeNote>
		<skos:scopeNote>http://www.w3.org/2004/02/skos/core#Concept</skos:scopeNote>
		<skos:Note>SKOS properties defined in http://www.w3.org/TR/skos-primer/#secrel</skos:Note>
		<skos:inScheme rdf:resource="http://www.cognitiveatlas.org/tasks/"/>
		<skos:definition>No definition submitted yet. </skos:definition>
		<skos:prefLabel>Counting Stroop Task</skos:prefLabel>
		<skos:altLabel></skos:altLabel>
</skos:Concept><skos:Concept rdf:about="http://www.cognitiveatlas.org/id/trm_4da6327154fd4"> <dc:identifier>trm_4da6327154fd4</dc:identifier>
		<dc:Title>Cognitive Atlas : Lexicon : scene recognition task</dc:Title>
		<dc:Description>RDF output for 'scene recognition task'</dc:Description>
		<dc:Type>InteractiveResource</dc:Type>
		<dc:Publisher>Cognitive Atlas</dc:Publisher>
		<dc:Creator>Cognitive Atlas RDF Generator</dc:Creator>
		<dc:Contributor>Natalie Picchetti</dc:Contributor>
		<dc:Date>2011-04-13 16:32:01</dc:Date>
		<dc:Format>text/rdf</dc:Format>
		<dc:Language>en</dc:Language>
		<skos:editorialNote>Generated by testgenall.php on Thu Mar 29 10:24:08 PDT 2012.</skos:editorialNote>
		<skos:historyNote>No previous definition revisions.</skos:historyNote>
		<skos:changeNote>This is the first and only definition provided.</skos:changeNote>
		<skos:scopeNote>http://www.w3.org/2004/02/skos/core#Concept</skos:scopeNote>
		<skos:Note>SKOS properties defined in http://www.w3.org/TR/skos-primer/#secrel</skos:Note>
		<skos:inScheme rdf:resource="http://www.cognitiveatlas.org/tasks/"/>
		<skos:definition>No definition submitted yet.</skos:definition>
		<skos:prefLabel>scene recognition task</skos:prefLabel>
		<skos:altLabel></skos:altLabel>
</skos:Concept><skos:Concept rdf:about="http://www.cognitiveatlas.org/id/trm_4da6331cdeeb5"> <dc:identifier>trm_4da6331cdeeb5</dc:identifier>
		<dc:Title>Cognitive Atlas : Lexicon : California Verbal Learning Test</dc:Title>
		<dc:Description>RDF output for 'California Verbal Learning Test'</dc:Description>
		<dc:Type>InteractiveResource</dc:Type>
		<dc:Publisher>Cognitive Atlas</dc:Publisher>
		<dc:Creator>Cognitive Atlas RDF Generator</dc:Creator>
		<dc:Contributor>Natalie Picchetti</dc:Contributor>
		<dc:Date>2011-04-13 16:34:52</dc:Date>
		<dc:Format>text/rdf</dc:Format>
		<dc:Language>en</dc:Language>
		<skos:editorialNote>Generated by testgenall.php on Thu Mar 29 10:24:08 PDT 2012.</skos:editorialNote>
		<skos:historyNote>No previous definition revisions.</skos:historyNote>
		<skos:changeNote>This is the first and only definition provided.</skos:changeNote>
		<skos:scopeNote>http://www.w3.org/2004/02/skos/core#Concept</skos:scopeNote>
		<skos:Note>SKOS properties defined in http://www.w3.org/TR/skos-primer/#secrel</skos:Note>
		<skos:inScheme rdf:resource="http://www.cognitiveatlas.org/tasks/"/>
		<skos:definition>No definition submitted yet.</skos:definition>
		<skos:prefLabel>California Verbal Learning Test</skos:prefLabel>
		<skos:altLabel></skos:altLabel>
		<skos:related rdf:resource="http://www.cognitiveatlas.org/id/trm_4a3fd79d0b95b"/>
		<skos:example>recall is measured by the contrast of  trials in the California Verbal Learning Test</skos:example>
</skos:Concept><skos:Concept rdf:about="http://www.cognitiveatlas.org/id/trm_4da63357e4999"> <dc:identifier>trm_4da63357e4999</dc:identifier>
		<dc:Title>Cognitive Atlas : Lexicon : Wechsler Memory Scale (revised)</dc:Title>
		<dc:Description>RDF output for 'Wechsler Memory Scale (revised)'</dc:Description>
		<dc:Type>InteractiveResource</dc:Type>
		<dc:Publisher>Cognitive Atlas</dc:Publisher>
		<dc:Creator>Cognitive Atlas RDF Generator</dc:Creator>
		<dc:Contributor>Natalie Picchetti</dc:Contributor>
		<dc:Date>2011-04-13 16:35:51</dc:Date>
		<dc:Format>text/rdf</dc:Format>
		<dc:Language>en</dc:Language>
		<skos:editorialNote>Generated by testgenall.php on Thu Mar 29 10:24:08 PDT 2012.</skos:editorialNote>
		<skos:historyNote>No previous definition revisions.</skos:historyNote>
		<skos:changeNote>This is the first and only definition provided.</skos:changeNote>
		<skos:scopeNote>http://www.w3.org/2004/02/skos/core#Concept</skos:scopeNote>
		<skos:Note>SKOS properties defined in http://www.w3.org/TR/skos-primer/#secrel</skos:Note>
		<skos:inScheme rdf:resource="http://www.cognitiveatlas.org/tasks/"/>
		<skos:definition>No definition submitted yet.</skos:definition>
		<skos:prefLabel>Wechsler Memory Scale (revised)</skos:prefLabel>
		<skos:altLabel></skos:altLabel>
		<skos:related rdf:resource="http://www.cognitiveatlas.org/id/tsk_4a57abb949abc"/>
		<skos:example>immediate recall test is descended from Wechsler Memory Scale (revised)</skos:example>
</skos:Concept><skos:Concept rdf:about="http://www.cognitiveatlas.org/id/trm_4da6338803ed2"> <dc:identifier>trm_4da6338803ed2</dc:identifier>
		<dc:Title>Cognitive Atlas : Lexicon : Wechsler Intelligence Scale for Children - Revised</dc:Title>
		<dc:Description>RDF output for 'Wechsler Intelligence Scale for Children - Revised'</dc:Description>
		<dc:Type>InteractiveResource</dc:Type>
		<dc:Publisher>Cognitive Atlas</dc:Publisher>
		<dc:Creator>Cognitive Atlas RDF Generator</dc:Creator>
		<dc:Contributor>Natalie Picchetti</dc:Contributor>
		<dc:Date>2011-04-13 16:36:40</dc:Date>
		<dc:Format>text/rdf</dc:Format>
		<dc:Language>en</dc:Language>
		<skos:editorialNote>Generated by testgenall.php on Thu Mar 29 10:24:08 PDT 2012.</skos:editorialNote>
		<skos:historyNote>No previous definition revisions.</skos:historyNote>
		<skos:changeNote>This is the first and only definition provided.</skos:changeNote>
		<skos:scopeNote>http://www.w3.org/2004/02/skos/core#Concept</skos:scopeNote>
		<skos:Note>SKOS properties defined in http://www.w3.org/TR/skos-primer/#secrel</skos:Note>
		<skos:inScheme rdf:resource="http://www.cognitiveatlas.org/tasks/"/>
		<skos:definition>No definition submitted yet.</skos:definition>
		<skos:prefLabel>Wechsler Intelligence Scale for Children - Revised</skos:prefLabel>
		<skos:altLabel></skos:altLabel>
</skos:Concept><skos:Concept rdf:about="http://www.cognitiveatlas.org/id/trm_4da633dbb5817"> <dc:identifier>trm_4da633dbb5817</dc:identifier>
		<dc:Title>Cognitive Atlas : Lexicon : word fluency test</dc:Title>
		<dc:Description>RDF output for 'word fluency test'</dc:Description>
		<dc:Type>InteractiveResource</dc:Type>
		<dc:Publisher>Cognitive Atlas</dc:Publisher>
		<dc:Creator>Cognitive Atlas RDF Generator</dc:Creator>
		<dc:Contributor>Natalie Picchetti</dc:Contributor>
		<dc:Date>2011-04-13 16:38:03</dc:Date>
		<dc:Format>text/rdf</dc:Format>
		<dc:Language>en</dc:Language>
		<skos:editorialNote>Generated by testgenall.php on Thu Mar 29 10:24:08 PDT 2012.</skos:editorialNote>
		<skos:historyNote>No previous definition revisions.</skos:historyNote>
		<skos:changeNote>This is the first and only definition provided.</skos:changeNote>
		<skos:scopeNote>http://www.w3.org/2004/02/skos/core#Concept</skos:scopeNote>
		<skos:Note>SKOS properties defined in http://www.w3.org/TR/skos-primer/#secrel</skos:Note>
		<skos:inScheme rdf:resource="http://www.cognitiveatlas.org/tasks/"/>
		<skos:definition>No definition submitted yet.</skos:definition>
		<skos:prefLabel>word fluency test</skos:prefLabel>
		<skos:altLabel></skos:altLabel>
</skos:Concept><skos:Concept rdf:about="http://www.cognitiveatlas.org/id/trm_4da633fe917c4"> <dc:identifier>trm_4da633fe917c4</dc:identifier>
		<dc:Title>Cognitive Atlas : Lexicon : color trails test</dc:Title>
		<dc:Description>RDF output for 'color trails test'</dc:Description>
		<dc:Type>InteractiveResource</dc:Type>
		<dc:Publisher>Cognitive Atlas</dc:Publisher>
		<dc:Creator>Cognitive Atlas RDF Generator</dc:Creator>
		<dc:Contributor>Natalie Picchetti</dc:Contributor>
		<dc:Date>2011-04-13 16:38:38</dc:Date>
		<dc:Format>text/rdf</dc:Format>
		<dc:Language>en</dc:Language>
		<skos:editorialNote>Generated by testgenall.php on Thu Mar 29 10:24:08 PDT 2012.</skos:editorialNote>
		<skos:historyNote>No previous definition revisions.</skos:historyNote>
		<skos:changeNote>This is the first and only definition provided.</skos:changeNote>
		<skos:scopeNote>http://www.w3.org/2004/02/skos/core#Concept</skos:scopeNote>
		<skos:Note>SKOS properties defined in http://www.w3.org/TR/skos-primer/#secrel</skos:Note>
		<skos:inScheme rdf:resource="http://www.cognitiveatlas.org/tasks/"/>
		<skos:definition>No definition submitted yet.</skos:definition>
		<skos:prefLabel>color trails test</skos:prefLabel>
		<skos:altLabel></skos:altLabel>
</skos:Concept><skos:Concept rdf:about="http://www.cognitiveatlas.org/id/trm_4da634216ebbc"> <dc:identifier>trm_4da634216ebbc</dc:identifier>
		<dc:Title>Cognitive Atlas : Lexicon : dual-task paradigm</dc:Title>
		<dc:Description>RDF output for 'dual-task paradigm'</dc:Description>
		<dc:Type>InteractiveResource</dc:Type>
		<dc:Publisher>Cognitive Atlas</dc:Publisher>
		<dc:Creator>Cognitive Atlas RDF Generator</dc:Creator>
		<dc:Contributor>Natalie Picchetti</dc:Contributor>
		<dc:Date>2011-04-13 16:39:13</dc:Date>
		<dc:Format>text/rdf</dc:Format>
		<dc:Language>en</dc:Language>
		<skos:editorialNote>Generated by testgenall.php on Thu Mar 29 10:24:08 PDT 2012.</skos:editorialNote>
		<skos:historyNote>No previous definition revisions.</skos:historyNote>
		<skos:changeNote>This is the first and only definition provided.</skos:changeNote>
		<skos:scopeNote>http://www.w3.org/2004/02/skos/core#Concept</skos:scopeNote>
		<skos:Note>SKOS properties defined in http://www.w3.org/TR/skos-primer/#secrel</skos:Note>
		<skos:inScheme rdf:resource="http://www.cognitiveatlas.org/tasks/"/>
		<skos:definition>NO definition submitted yet.</skos:definition>
		<skos:prefLabel>dual-task paradigm</skos:prefLabel>
		<skos:altLabel></skos:altLabel>
		<skos:related rdf:resource="http://www.cognitiveatlas.org/id/trm_4a3fd79d09b28"/>
		<skos:example>automaticity is measured by the contrast of  trials in the dual-task paradigm</skos:example>
</skos:Concept><skos:Concept rdf:about="http://www.cognitiveatlas.org/id/trm_4da869646e5d1"> <dc:identifier>trm_4da869646e5d1</dc:identifier>
		<dc:Title>Cognitive Atlas : Lexicon : item recognition task</dc:Title>
		<dc:Description>RDF output for 'item recognition task'</dc:Description>
		<dc:Type>InteractiveResource</dc:Type>
		<dc:Publisher>Cognitive Atlas</dc:Publisher>
		<dc:Creator>Cognitive Atlas RDF Generator</dc:Creator>
		<dc:Contributor>Natalie Picchetti</dc:Contributor>
		<dc:Date>2011-04-15 08:51:00</dc:Date>
		<dc:Format>text/rdf</dc:Format>
		<dc:Language>en</dc:Language>
		<skos:editorialNote>Generated by testgenall.php on Thu Mar 29 10:24:08 PDT 2012.</skos:editorialNote>
		<skos:historyNote>No previous definition revisions.</skos:historyNote>
		<skos:changeNote>This is the first and only definition provided.</skos:changeNote>
		<skos:scopeNote>http://www.w3.org/2004/02/skos/core#Concept</skos:scopeNote>
		<skos:Note>SKOS properties defined in http://www.w3.org/TR/skos-primer/#secrel</skos:Note>
		<skos:inScheme rdf:resource="http://www.cognitiveatlas.org/tasks/"/>
		<skos:definition>No definition submitted yet.</skos:definition>
		<skos:prefLabel>item recognition task</skos:prefLabel>
		<skos:altLabel></skos:altLabel>
</skos:Concept><skos:Concept rdf:about="http://www.cognitiveatlas.org/id/trm_4da869e68b5c4"> <dc:identifier>trm_4da869e68b5c4</dc:identifier>
		<dc:Title>Cognitive Atlas : Lexicon : memory span test</dc:Title>
		<dc:Description>RDF output for 'memory span test'</dc:Description>
		<dc:Type>InteractiveResource</dc:Type>
		<dc:Publisher>Cognitive Atlas</dc:Publisher>
		<dc:Creator>Cognitive Atlas RDF Generator</dc:Creator>
		<dc:Contributor>Natalie Picchetti</dc:Contributor>
		<dc:Date>2011-04-15 08:53:10</dc:Date>
		<dc:Format>text/rdf</dc:Format>
		<dc:Language>en</dc:Language>
		<skos:editorialNote>Generated by testgenall.php on Thu Mar 29 10:24:08 PDT 2012.</skos:editorialNote>
		<skos:historyNote>No previous definition revisions.</skos:historyNote>
		<skos:changeNote>This is the first and only definition provided.</skos:changeNote>
		<skos:scopeNote>http://www.w3.org/2004/02/skos/core#Concept</skos:scopeNote>
		<skos:Note>SKOS properties defined in http://www.w3.org/TR/skos-primer/#secrel</skos:Note>
		<skos:inScheme rdf:resource="http://www.cognitiveatlas.org/tasks/"/>
		<skos:definition>No definition submitted yet.</skos:definition>
		<skos:prefLabel>memory span test</skos:prefLabel>
		<skos:altLabel></skos:altLabel>
</skos:Concept><skos:Concept rdf:about="http://www.cognitiveatlas.org/id/trm_4da86ad02b3ea"> <dc:identifier>trm_4da86ad02b3ea</dc:identifier>
		<dc:Title>Cognitive Atlas : Lexicon : complex span test</dc:Title>
		<dc:Description>RDF output for 'complex span test'</dc:Description>
		<dc:Type>InteractiveResource</dc:Type>
		<dc:Publisher>Cognitive Atlas</dc:Publisher>
		<dc:Creator>Cognitive Atlas RDF Generator</dc:Creator>
		<dc:Contributor>Natalie Picchetti</dc:Contributor>
		<dc:Date>2011-04-15 08:57:04</dc:Date>
		<dc:Format>text/rdf</dc:Format>
		<dc:Language>en</dc:Language>
		<skos:editorialNote>Generated by testgenall.php on Thu Mar 29 10:24:08 PDT 2012.</skos:editorialNote>
		<skos:historyNote>No previous definition revisions.</skos:historyNote>
		<skos:changeNote>This is the first and only definition provided.</skos:changeNote>
		<skos:scopeNote>http://www.w3.org/2004/02/skos/core#Concept</skos:scopeNote>
		<skos:Note>SKOS properties defined in http://www.w3.org/TR/skos-primer/#secrel</skos:Note>
		<skos:inScheme rdf:resource="http://www.cognitiveatlas.org/tasks/"/>
		<skos:definition>No definition submitted yet.</skos:definition>
		<skos:prefLabel>complex span test</skos:prefLabel>
		<skos:altLabel></skos:altLabel>
</skos:Concept><skos:Concept rdf:about="http://www.cognitiveatlas.org/id/trm_4da86b539924c"> <dc:identifier>trm_4da86b539924c</dc:identifier>
		<dc:Title>Cognitive Atlas : Lexicon : spatial span test</dc:Title>
		<dc:Description>RDF output for 'spatial span test'</dc:Description>
		<dc:Type>InteractiveResource</dc:Type>
		<dc:Publisher>Cognitive Atlas</dc:Publisher>
		<dc:Creator>Cognitive Atlas RDF Generator</dc:Creator>
		<dc:Contributor>Natalie Picchetti</dc:Contributor>
		<dc:Date>2011-04-15 08:59:15</dc:Date>
		<dc:Format>text/rdf</dc:Format>
		<dc:Language>en</dc:Language>
		<skos:editorialNote>Generated by testgenall.php on Thu Mar 29 10:24:08 PDT 2012.</skos:editorialNote>
		<skos:historyNote>No previous definition revisions.</skos:historyNote>
		<skos:changeNote>This is the first and only definition provided.</skos:changeNote>
		<skos:scopeNote>http://www.w3.org/2004/02/skos/core#Concept</skos:scopeNote>
		<skos:Note>SKOS properties defined in http://www.w3.org/TR/skos-primer/#secrel</skos:Note>
		<skos:inScheme rdf:resource="http://www.cognitiveatlas.org/tasks/"/>
		<skos:definition>No definition submitted yet.</skos:definition>
		<skos:prefLabel>spatial span test</skos:prefLabel>
		<skos:altLabel></skos:altLabel>
</skos:Concept><skos:Concept rdf:about="http://www.cognitiveatlas.org/id/trm_4da86c2a70a7d"> <dc:identifier>trm_4da86c2a70a7d</dc:identifier>
		<dc:Title>Cognitive Atlas : Lexicon : Dot Pattern Expectancy Task</dc:Title>
		<dc:Description>RDF output for 'Dot Pattern Expectancy Task'</dc:Description>
		<dc:Type>InteractiveResource</dc:Type>
		<dc:Publisher>Cognitive Atlas</dc:Publisher>
		<dc:Creator>Cognitive Atlas RDF Generator</dc:Creator>
		<dc:Contributor>Natalie Picchetti</dc:Contributor>
		<dc:Date>2011-04-15 09:02:50</dc:Date>
		<dc:Format>text/rdf</dc:Format>
		<dc:Language>en</dc:Language>
		<skos:editorialNote>Generated by testgenall.php on Thu Mar 29 10:24:08 PDT 2012.</skos:editorialNote>
		<skos:historyNote>No previous definition revisions.</skos:historyNote>
		<skos:changeNote>This is the first and only definition provided.</skos:changeNote>
		<skos:scopeNote>http://www.w3.org/2004/02/skos/core#Concept</skos:scopeNote>
		<skos:Note>SKOS properties defined in http://www.w3.org/TR/skos-primer/#secrel</skos:Note>
		<skos:inScheme rdf:resource="http://www.cognitiveatlas.org/tasks/"/>
		<skos:definition>No definition submitted yet.</skos:definition>
		<skos:prefLabel>Dot Pattern Expectancy Task</skos:prefLabel>
		<skos:altLabel></skos:altLabel>
</skos:Concept><skos:Concept rdf:about="http://www.cognitiveatlas.org/id/trm_4da86c6808ddd"> <dc:identifier>trm_4da86c6808ddd</dc:identifier>
		<dc:Title>Cognitive Atlas : Lexicon : cattell culture fair intelligence test</dc:Title>
		<dc:Description>RDF output for 'cattell culture fair intelligence test'</dc:Description>
		<dc:Type>InteractiveResource</dc:Type>
		<dc:Publisher>Cognitive Atlas</dc:Publisher>
		<dc:Creator>Cognitive Atlas RDF Generator</dc:Creator>
		<dc:Contributor>Natalie Picchetti</dc:Contributor>
		<dc:Date>2011-04-15 09:03:52</dc:Date>
		<dc:Format>text/rdf</dc:Format>
		<dc:Language>en</dc:Language>
		<skos:editorialNote>Generated by testgenall.php on Thu Mar 29 10:24:08 PDT 2012.</skos:editorialNote>
		<skos:historyNote>No previous definition revisions.</skos:historyNote>
		<skos:changeNote>This is the first and only definition provided.</skos:changeNote>
		<skos:scopeNote>http://www.w3.org/2004/02/skos/core#Concept</skos:scopeNote>
		<skos:Note>SKOS properties defined in http://www.w3.org/TR/skos-primer/#secrel</skos:Note>
		<skos:inScheme rdf:resource="http://www.cognitiveatlas.org/tasks/"/>
		<skos:definition>No definition submitted yet.</skos:definition>
		<skos:prefLabel>cattell culture fair intelligence test</skos:prefLabel>
		<skos:altLabel></skos:altLabel>
</skos:Concept><skos:Concept rdf:about="http://www.cognitiveatlas.org/id/trm_4da86c8bb3b04"> <dc:identifier>trm_4da86c8bb3b04</dc:identifier>
		<dc:Title>Cognitive Atlas : Lexicon : letter comparison</dc:Title>
		<dc:Description>RDF output for 'letter comparison'</dc:Description>
		<dc:Type>InteractiveResource</dc:Type>
		<dc:Publisher>Cognitive Atlas</dc:Publisher>
		<dc:Creator>Cognitive Atlas RDF Generator</dc:Creator>
		<dc:Contributor>Natalie Picchetti</dc:Contributor>
		<dc:Date>2011-04-15 09:04:27</dc:Date>
		<dc:Format>text/rdf</dc:Format>
		<dc:Language>en</dc:Language>
		<skos:editorialNote>Generated by testgenall.php on Thu Mar 29 10:24:08 PDT 2012.</skos:editorialNote>
		<skos:historyNote>No previous definition revisions.</skos:historyNote>
		<skos:changeNote>This is the first and only definition provided.</skos:changeNote>
		<skos:scopeNote>http://www.w3.org/2004/02/skos/core#Concept</skos:scopeNote>
		<skos:Note>SKOS properties defined in http://www.w3.org/TR/skos-primer/#secrel</skos:Note>
		<skos:inScheme rdf:resource="http://www.cognitiveatlas.org/tasks/"/>
		<skos:definition>No definition submitted yet.</skos:definition>
		<skos:prefLabel>letter comparison</skos:prefLabel>
		<skos:altLabel></skos:altLabel>
</skos:Concept><skos:Concept rdf:about="http://www.cognitiveatlas.org/id/trm_4da86cb034ff6"> <dc:identifier>trm_4da86cb034ff6</dc:identifier>
		<dc:Title>Cognitive Atlas : Lexicon : pattern comparison</dc:Title>
		<dc:Description>RDF output for 'pattern comparison'</dc:Description>
		<dc:Type>InteractiveResource</dc:Type>
		<dc:Publisher>Cognitive Atlas</dc:Publisher>
		<dc:Creator>Cognitive Atlas RDF Generator</dc:Creator>
		<dc:Contributor>Natalie Picchetti</dc:Contributor>
		<dc:Date>2011-04-15 09:05:04</dc:Date>
		<dc:Format>text/rdf</dc:Format>
		<dc:Language>en</dc:Language>
		<skos:editorialNote>Generated by testgenall.php on Thu Mar 29 10:24:08 PDT 2012.</skos:editorialNote>
		<skos:historyNote>No previous definition revisions.</skos:historyNote>
		<skos:changeNote>This is the first and only definition provided.</skos:changeNote>
		<skos:scopeNote>http://www.w3.org/2004/02/skos/core#Concept</skos:scopeNote>
		<skos:Note>SKOS properties defined in http://www.w3.org/TR/skos-primer/#secrel</skos:Note>
		<skos:inScheme rdf:resource="http://www.cognitiveatlas.org/tasks/"/>
		<skos:definition>No definition submitted yet.</skos:definition>
		<skos:prefLabel>pattern comparison</skos:prefLabel>
		<skos:altLabel></skos:altLabel>
</skos:Concept><skos:Concept rdf:about="http://www.cognitiveatlas.org/id/trm_4da86cdbd9eeb"> <dc:identifier>trm_4da86cdbd9eeb</dc:identifier>
		<dc:Title>Cognitive Atlas : Lexicon : test of variables of attention</dc:Title>
		<dc:Description>RDF output for 'test of variables of attention'</dc:Description>
		<dc:Type>InteractiveResource</dc:Type>
		<dc:Publisher>Cognitive Atlas</dc:Publisher>
		<dc:Creator>Cognitive Atlas RDF Generator</dc:Creator>
		<dc:Contributor>Natalie Picchetti</dc:Contributor>
		<dc:Date>2011-04-15 09:05:47</dc:Date>
		<dc:Format>text/rdf</dc:Format>
		<dc:Language>en</dc:Language>
		<skos:editorialNote>Generated by testgenall.php on Thu Mar 29 10:24:08 PDT 2012.</skos:editorialNote>
		<skos:historyNote>No previous definition revisions.</skos:historyNote>
		<skos:changeNote>This is the first and only definition provided.</skos:changeNote>
		<skos:scopeNote>http://www.w3.org/2004/02/skos/core#Concept</skos:scopeNote>
		<skos:Note>SKOS properties defined in http://www.w3.org/TR/skos-primer/#secrel</skos:Note>
		<skos:inScheme rdf:resource="http://www.cognitiveatlas.org/tasks/"/>
		<skos:definition>No definition submitted yet.</skos:definition>
		<skos:prefLabel>test of variables of attention</skos:prefLabel>
		<skos:altLabel></skos:altLabel>
</skos:Concept><skos:Concept rdf:about="http://www.cognitiveatlas.org/id/trm_4da86cfe8cf1b"> <dc:identifier>trm_4da86cfe8cf1b</dc:identifier>
		<dc:Title>Cognitive Atlas : Lexicon : sustained attention to response task</dc:Title>
		<dc:Description>RDF output for 'sustained attention to response task'</dc:Description>
		<dc:Type>InteractiveResource</dc:Type>
		<dc:Publisher>Cognitive Atlas</dc:Publisher>
		<dc:Creator>Cognitive Atlas RDF Generator</dc:Creator>
		<dc:Contributor>Natalie Picchetti</dc:Contributor>
		<dc:Date>2011-04-15 09:06:22</dc:Date>
		<dc:Format>text/rdf</dc:Format>
		<dc:Language>en</dc:Language>
		<skos:editorialNote>Generated by testgenall.php on Thu Mar 29 10:24:08 PDT 2012.</skos:editorialNote>
		<skos:historyNote>No previous definition revisions.</skos:historyNote>
		<skos:changeNote>This is the first and only definition provided.</skos:changeNote>
		<skos:scopeNote>http://www.w3.org/2004/02/skos/core#Concept</skos:scopeNote>
		<skos:Note>SKOS properties defined in http://www.w3.org/TR/skos-primer/#secrel</skos:Note>
		<skos:inScheme rdf:resource="http://www.cognitiveatlas.org/tasks/"/>
		<skos:definition>No definition submitted yet.</skos:definition>
		<skos:prefLabel>sustained attention to response task</skos:prefLabel>
		<skos:altLabel></skos:altLabel>
</skos:Concept><skos:Concept rdf:about="http://www.cognitiveatlas.org/id/trm_4da87b8bf1511"> <dc:identifier>trm_4da87b8bf1511</dc:identifier>
		<dc:Title>Cognitive Atlas : Lexicon : matching familiar figures test</dc:Title>
		<dc:Description>RDF output for 'matching familiar figures test'</dc:Description>
		<dc:Type>InteractiveResource</dc:Type>
		<dc:Publisher>Cognitive Atlas</dc:Publisher>
		<dc:Creator>Cognitive Atlas RDF Generator</dc:Creator>
		<dc:Contributor>Natalie Picchetti</dc:Contributor>
		<dc:Date>2011-04-15 10:08:27</dc:Date>
		<dc:Format>text/rdf</dc:Format>
		<dc:Language>en</dc:Language>
		<skos:editorialNote>Generated by testgenall.php on Thu Mar 29 10:24:08 PDT 2012.</skos:editorialNote>
		<skos:historyNote>No previous definition revisions.</skos:historyNote>
		<skos:changeNote>This is the first and only definition provided.</skos:changeNote>
		<skos:scopeNote>http://www.w3.org/2004/02/skos/core#Concept</skos:scopeNote>
		<skos:Note>SKOS properties defined in http://www.w3.org/TR/skos-primer/#secrel</skos:Note>
		<skos:inScheme rdf:resource="http://www.cognitiveatlas.org/tasks/"/>
		<skos:definition>No definition submitted yet.</skos:definition>
		<skos:prefLabel>matching familiar figures test</skos:prefLabel>
		<skos:altLabel></skos:altLabel>
</skos:Concept><skos:Concept rdf:about="http://www.cognitiveatlas.org/id/trm_4da87e439c411"> <dc:identifier>trm_4da87e439c411</dc:identifier>
		<dc:Title>Cognitive Atlas : Lexicon : Tower of London</dc:Title>
		<dc:Description>RDF output for 'Tower of London'</dc:Description>
		<dc:Type>InteractiveResource</dc:Type>
		<dc:Publisher>Cognitive Atlas</dc:Publisher>
		<dc:Creator>Cognitive Atlas RDF Generator</dc:Creator>
		<dc:Contributor>Natalie Picchetti</dc:Contributor>
		<dc:Date>2011-04-15 10:20:03</dc:Date>
		<dc:Format>text/rdf</dc:Format>
		<dc:Language>en</dc:Language>
		<skos:editorialNote>Generated by testgenall.php on Thu Mar 29 10:24:08 PDT 2012.</skos:editorialNote>
		<skos:historyNote>No previous definition revisions.</skos:historyNote>
		<skos:changeNote>This is the first and only definition provided.</skos:changeNote>
		<skos:scopeNote>http://www.w3.org/2004/02/skos/core#Concept</skos:scopeNote>
		<skos:Note>SKOS properties defined in http://www.w3.org/TR/skos-primer/#secrel</skos:Note>
		<skos:inScheme rdf:resource="http://www.cognitiveatlas.org/tasks/"/>
		<skos:definition>No definition submitted yet.</skos:definition>
		<skos:prefLabel>Tower of London</skos:prefLabel>
		<skos:altLabel></skos:altLabel>
</skos:Concept><skos:Concept rdf:about="http://www.cognitiveatlas.org/id/trm_4da87e7282f92"> <dc:identifier>trm_4da87e7282f92</dc:identifier>
		<dc:Title>Cognitive Atlas : Lexicon : Tower of Hanoi</dc:Title>
		<dc:Description>RDF output for 'Tower of Hanoi'</dc:Description>
		<dc:Type>InteractiveResource</dc:Type>
		<dc:Publisher>Cognitive Atlas</dc:Publisher>
		<dc:Creator>Cognitive Atlas RDF Generator</dc:Creator>
		<dc:Contributor>Natalie Picchetti</dc:Contributor>
		<dc:Date>2011-04-15 10:20:50</dc:Date>
		<dc:Format>text/rdf</dc:Format>
		<dc:Language>en</dc:Language>
		<skos:editorialNote>Generated by testgenall.php on Thu Mar 29 10:24:08 PDT 2012.</skos:editorialNote>
		<skos:historyNote>No previous definition revisions.</skos:historyNote>
		<skos:changeNote>This is the first and only definition provided.</skos:changeNote>
		<skos:scopeNote>http://www.w3.org/2004/02/skos/core#Concept</skos:scopeNote>
		<skos:Note>SKOS properties defined in http://www.w3.org/TR/skos-primer/#secrel</skos:Note>
		<skos:inScheme rdf:resource="http://www.cognitiveatlas.org/tasks/"/>
		<skos:definition>No definition submitted yet.</skos:definition>
		<skos:prefLabel>Tower of Hanoi</skos:prefLabel>
		<skos:altLabel></skos:altLabel>
</skos:Concept><skos:Concept rdf:about="http://www.cognitiveatlas.org/id/trm_4da87e9c79847"> <dc:identifier>trm_4da87e9c79847</dc:identifier>
		<dc:Title>Cognitive Atlas : Lexicon : dichotic listening task</dc:Title>
		<dc:Description>RDF output for 'dichotic listening task'</dc:Description>
		<dc:Type>InteractiveResource</dc:Type>
		<dc:Publisher>Cognitive Atlas</dc:Publisher>
		<dc:Creator>Cognitive Atlas RDF Generator</dc:Creator>
		<dc:Contributor>Natalie Picchetti</dc:Contributor>
		<dc:Date>2011-04-15 10:21:32</dc:Date>
		<dc:Format>text/rdf</dc:Format>
		<dc:Language>en</dc:Language>
		<skos:editorialNote>Generated by testgenall.php on Thu Mar 29 10:24:08 PDT 2012.</skos:editorialNote>
		<skos:historyNote>No previous definition revisions.</skos:historyNote>
		<skos:changeNote>This is the first and only definition provided.</skos:changeNote>
		<skos:scopeNote>http://www.w3.org/2004/02/skos/core#Concept</skos:scopeNote>
		<skos:Note>SKOS properties defined in http://www.w3.org/TR/skos-primer/#secrel</skos:Note>
		<skos:inScheme rdf:resource="http://www.cognitiveatlas.org/tasks/"/>
		<skos:definition>No definition submitted yet.</skos:definition>
		<skos:prefLabel>dichotic listening task</skos:prefLabel>
		<skos:altLabel></skos:altLabel>
		<skos:related rdf:resource="http://www.cognitiveatlas.org/id/trm_4a3fd79d098eb"/>
		<skos:example>attended channel is measured by the contrast of  trials in the dichotic listening task</skos:example>
</skos:Concept><skos:Concept rdf:about="http://www.cognitiveatlas.org/id/trm_4da87f383435b"> <dc:identifier>trm_4da87f383435b</dc:identifier>
		<dc:Title>Cognitive Atlas : Lexicon : directed forgetting task</dc:Title>
		<dc:Description>RDF output for 'directed forgetting task'</dc:Description>
		<dc:Type>InteractiveResource</dc:Type>
		<dc:Publisher>Cognitive Atlas</dc:Publisher>
		<dc:Creator>Cognitive Atlas RDF Generator</dc:Creator>
		<dc:Contributor>Natalie Picchetti</dc:Contributor>
		<dc:Date>2011-04-15 10:24:08</dc:Date>
		<dc:Format>text/rdf</dc:Format>
		<dc:Language>en</dc:Language>
		<skos:editorialNote>Generated by testgenall.php on Thu Mar 29 10:24:08 PDT 2012.</skos:editorialNote>
		<skos:historyNote>No previous definition revisions.</skos:historyNote>
		<skos:changeNote>This is the first and only definition provided.</skos:changeNote>
		<skos:scopeNote>http://www.w3.org/2004/02/skos/core#Concept</skos:scopeNote>
		<skos:Note>SKOS properties defined in http://www.w3.org/TR/skos-primer/#secrel</skos:Note>
		<skos:inScheme rdf:resource="http://www.cognitiveatlas.org/tasks/"/>
		<skos:definition>No definition submitted yet.</skos:definition>
		<skos:prefLabel>directed forgetting task</skos:prefLabel>
		<skos:altLabel></skos:altLabel>
</skos:Concept><skos:Concept rdf:about="http://www.cognitiveatlas.org/id/trm_4da87f81bc2c8"> <dc:identifier>trm_4da87f81bc2c8</dc:identifier>
		<dc:Title>Cognitive Atlas : Lexicon : retrieval-induced forgetting task</dc:Title>
		<dc:Description>RDF output for 'retrieval-induced forgetting task'</dc:Description>
		<dc:Type>InteractiveResource</dc:Type>
		<dc:Publisher>Cognitive Atlas</dc:Publisher>
		<dc:Creator>Cognitive Atlas RDF Generator</dc:Creator>
		<dc:Contributor>Natalie Picchetti</dc:Contributor>
		<dc:Date>2011-04-15 10:25:21</dc:Date>
		<dc:Format>text/rdf</dc:Format>
		<dc:Language>en</dc:Language>
		<skos:editorialNote>Generated by testgenall.php on Thu Mar 29 10:24:08 PDT 2012.</skos:editorialNote>
		<skos:historyNote>No previous definition revisions.</skos:historyNote>
		<skos:changeNote>This is the first and only definition provided.</skos:changeNote>
		<skos:scopeNote>http://www.w3.org/2004/02/skos/core#Concept</skos:scopeNote>
		<skos:Note>SKOS properties defined in http://www.w3.org/TR/skos-primer/#secrel</skos:Note>
		<skos:inScheme rdf:resource="http://www.cognitiveatlas.org/tasks/"/>
		<skos:definition>No definition submitted yet.</skos:definition>
		<skos:prefLabel>retrieval-induced forgetting task</skos:prefLabel>
		<skos:altLabel></skos:altLabel>
</skos:Concept><skos:Concept rdf:about="http://www.cognitiveatlas.org/id/trm_4da87fb28978e"> <dc:identifier>trm_4da87fb28978e</dc:identifier>
		<dc:Title>Cognitive Atlas : Lexicon : Paced Auditory Serial Addition Test</dc:Title>
		<dc:Description>RDF output for 'Paced Auditory Serial Addition Test'</dc:Description>
		<dc:Type>InteractiveResource</dc:Type>
		<dc:Publisher>Cognitive Atlas</dc:Publisher>
		<dc:Creator>Cognitive Atlas RDF Generator</dc:Creator>
		<dc:Contributor>Russ Poldrack</dc:Contributor>
		<dc:Date>2012-01-28 07:54:23</dc:Date>
		<dc:Format>text/rdf</dc:Format>
		<dc:Language>en</dc:Language>
		<skos:editorialNote>Generated by testgenall.php on Thu Mar 29 10:24:08 PDT 2012.</skos:editorialNote>
		<skos:historyNote>Revision 2: 1 previous definitions.</skos:historyNote>
		<skos:changeNote>See http://www.cognitiveatlas.org/id/trm_4da87fb28978e for complete revision history.</skos:changeNote>
		<skos:scopeNote>http://www.w3.org/2004/02/skos/core#Concept</skos:scopeNote>
		<skos:Note>SKOS properties defined in http://www.w3.org/TR/skos-primer/#secrel</skos:Note>
		<skos:inScheme rdf:resource="http://www.cognitiveatlas.org/tasks/"/>
		<skos:definition>No definition submitted yet.</skos:definition>
		<skos:prefLabel>Paced Auditory Serial Addition Test</skos:prefLabel>
		<skos:altLabel>PASAT</skos:altLabel>
</skos:Concept><skos:Concept rdf:about="http://www.cognitiveatlas.org/id/trm_4da87fdd7820e"> <dc:identifier>trm_4da87fdd7820e</dc:identifier>
		<dc:Title>Cognitive Atlas : Lexicon : Porteus maze test</dc:Title>
		<dc:Description>RDF output for 'Porteus maze test'</dc:Description>
		<dc:Type>InteractiveResource</dc:Type>
		<dc:Publisher>Cognitive Atlas</dc:Publisher>
		<dc:Creator>Cognitive Atlas RDF Generator</dc:Creator>
		<dc:Contributor>Natalie Picchetti</dc:Contributor>
		<dc:Date>2011-04-15 10:26:53</dc:Date>
		<dc:Format>text/rdf</dc:Format>
		<dc:Language>en</dc:Language>
		<skos:editorialNote>Generated by testgenall.php on Thu Mar 29 10:24:08 PDT 2012.</skos:editorialNote>
		<skos:historyNote>No previous definition revisions.</skos:historyNote>
		<skos:changeNote>This is the first and only definition provided.</skos:changeNote>
		<skos:scopeNote>http://www.w3.org/2004/02/skos/core#Concept</skos:scopeNote>
		<skos:Note>SKOS properties defined in http://www.w3.org/TR/skos-primer/#secrel</skos:Note>
		<skos:inScheme rdf:resource="http://www.cognitiveatlas.org/tasks/"/>
		<skos:definition>No definition submitted yet.</skos:definition>
		<skos:prefLabel>Porteus maze test</skos:prefLabel>
		<skos:altLabel></skos:altLabel>
		<skos:related rdf:resource="http://www.cognitiveatlas.org/id/trm_4b86c55f3d5df"/>
		<skos:example>WISC-R Mazes is an exact synonym of Porteus maze test</skos:example>
</skos:Concept><skos:Concept rdf:about="http://www.cognitiveatlas.org/id/trm_4da880396c76b"> <dc:identifier>trm_4da880396c76b</dc:identifier>
		<dc:Title>Cognitive Atlas : Lexicon : Rey-Ostereith Complex Figure Test</dc:Title>
		<dc:Description>RDF output for 'Rey-Ostereith Complex Figure Test'</dc:Description>
		<dc:Type>InteractiveResource</dc:Type>
		<dc:Publisher>Cognitive Atlas</dc:Publisher>
		<dc:Creator>Cognitive Atlas RDF Generator</dc:Creator>
		<dc:Contributor>Natalie Picchetti</dc:Contributor>
		<dc:Date>2011-04-15 10:28:25</dc:Date>
		<dc:Format>text/rdf</dc:Format>
		<dc:Language>en</dc:Language>
		<skos:editorialNote>Generated by testgenall.php on Thu Mar 29 10:24:08 PDT 2012.</skos:editorialNote>
		<skos:historyNote>No previous definition revisions.</skos:historyNote>
		<skos:changeNote>This is the first and only definition provided.</skos:changeNote>
		<skos:scopeNote>http://www.w3.org/2004/02/skos/core#Concept</skos:scopeNote>
		<skos:Note>SKOS properties defined in http://www.w3.org/TR/skos-primer/#secrel</skos:Note>
		<skos:inScheme rdf:resource="http://www.cognitiveatlas.org/tasks/"/>
		<skos:definition>No definition submitted yet.</skos:definition>
		<skos:prefLabel>Rey-Ostereith Complex Figure Test</skos:prefLabel>
		<skos:altLabel></skos:altLabel>
</skos:Concept><skos:Concept rdf:about="http://www.cognitiveatlas.org/id/trm_4da880ff8fd4a"> <dc:identifier>trm_4da880ff8fd4a</dc:identifier>
		<dc:Title>Cognitive Atlas : Lexicon : Cambridge Neuropsychological Test Automated Battery </dc:Title>
		<dc:Description>RDF output for 'Cambridge Neuropsychological Test Automated Battery '</dc:Description>
		<dc:Type>InteractiveResource</dc:Type>
		<dc:Publisher>Cognitive Atlas</dc:Publisher>
		<dc:Creator>Cognitive Atlas RDF Generator</dc:Creator>
		<dc:Contributor>Natalie Picchetti</dc:Contributor>
		<dc:Date>2011-04-15 10:31:43</dc:Date>
		<dc:Format>text/rdf</dc:Format>
		<dc:Language>en</dc:Language>
		<skos:editorialNote>Generated by testgenall.php on Thu Mar 29 10:24:08 PDT 2012.</skos:editorialNote>
		<skos:historyNote>No previous definition revisions.</skos:historyNote>
		<skos:changeNote>This is the first and only definition provided.</skos:changeNote>
		<skos:scopeNote>http://www.w3.org/2004/02/skos/core#Concept</skos:scopeNote>
		<skos:Note>SKOS properties defined in http://www.w3.org/TR/skos-primer/#secrel</skos:Note>
		<skos:inScheme rdf:resource="http://www.cognitiveatlas.org/tasks/"/>
		<skos:definition>is a computer-based cognitive assessment system consisting of a battery of neuropsychological tests, administered to subjects using a touch screen computer. The 22 tests in CANTAB examine various areas of cognitive function, including:

    * general memory and learning,
    * working memory and executive function,
    * visual memory,
    * attention and reaction time (RT),
    * semantic/verbal memory,
    * decision making and response control.

The CANTAB endeavours to import the accuracy and rigour of computerised psychological testing whilst retaining the wide range of ability measures demanded of a neuropsychological battery. It is suitable for young and old subjects, and aims to be culture and language independent through the use of non-verbal stimuli in the majority of the tests.</skos:definition>
		<skos:prefLabel>Cambridge Neuropsychological Test Automated Battery </skos:prefLabel>
		<skos:altLabel></skos:altLabel>
</skos:Concept><skos:Concept rdf:about="http://www.cognitiveatlas.org/id/trm_4da881dace79c"> <dc:identifier>trm_4da881dace79c</dc:identifier>
		<dc:Title>Cognitive Atlas : Lexicon : Corsi Blocks</dc:Title>
		<dc:Description>RDF output for 'Corsi Blocks'</dc:Description>
		<dc:Type>InteractiveResource</dc:Type>
		<dc:Publisher>Cognitive Atlas</dc:Publisher>
		<dc:Creator>Cognitive Atlas RDF Generator</dc:Creator>
		<dc:Contributor>Natalie Picchetti</dc:Contributor>
		<dc:Date>2011-04-15 10:35:51</dc:Date>
		<dc:Format>text/rdf</dc:Format>
		<dc:Language>en</dc:Language>
		<skos:editorialNote>Generated by testgenall.php on Thu Mar 29 10:24:08 PDT 2012.</skos:editorialNote>
		<skos:historyNote>Revision 2: 1 previous definitions.</skos:historyNote>
		<skos:changeNote>See http://www.cognitiveatlas.org/id/trm_4da881dace79c for complete revision history.</skos:changeNote>
		<skos:scopeNote>http://www.w3.org/2004/02/skos/core#Concept</skos:scopeNote>
		<skos:Note>SKOS properties defined in http://www.w3.org/TR/skos-primer/#secrel</skos:Note>
		<skos:inScheme rdf:resource="http://www.cognitiveatlas.org/tasks/"/>
		<skos:definition>was developed in the early 1970s as a visuospatial counterpart to the verbal-memory span task (Milner, 1971). Over the years, it has frequently been used to assess visuospatial short-term memory performance in adults (e.g. Smyth &amp; Scholey, 1992), children (e.g. Orsini, Schiappa, &amp; Grossi, 1981), and patients with neuropsychological deficits (e.g. Vilkki &amp; Holst, 1989). 

The original Corsi apparatus consisted of a set of nine identical blocks (3 X 3 X 3 cm) irregularly positioned on a wooden board (23 X 28 cm). The experimenter points to a series of blocks at a rate of one block per second. Subsequently, the participant is required to point to the same blocks in their order of presentation. The length of the block sequences increases until recall is no longer correct. 

Numerous variations have since been employed in both display characteristics (e.g. colour, number and size of the blocks, block placement, size of the board) and test administration (e.g. presentation rate, block sequences, recall order, scoring technique) (for a review, see Berch, Krikorian, &amp; Huha, 1998).</skos:definition>
		<skos:prefLabel>Corsi Blocks</skos:prefLabel>
		<skos:altLabel></skos:altLabel>
		<skos:related rdf:resource="http://www.cognitiveatlas.org/id/tsk_4a57abb9498df"/>
		<skos:related rdf:resource="http://www.cognitiveatlas.org/id/tsk_4a57abb949de3"/>
		<skos:example>Block Tapping Test is descended from Corsi Blocks</skos:example>
		<skos:example>Span/Supra-Span Test is related to Corsi Blocks</skos:example>
</skos:Concept><skos:Concept rdf:about="http://www.cognitiveatlas.org/id/trm_4da886fc2bc46"> <dc:identifier>trm_4da886fc2bc46</dc:identifier>
		<dc:Title>Cognitive Atlas : Lexicon : Visual Patterns Test</dc:Title>
		<dc:Description>RDF output for 'Visual Patterns Test'</dc:Description>
		<dc:Type>InteractiveResource</dc:Type>
		<dc:Publisher>Cognitive Atlas</dc:Publisher>
		<dc:Creator>Cognitive Atlas RDF Generator</dc:Creator>
		<dc:Contributor>Natalie Picchetti</dc:Contributor>
		<dc:Date>2011-04-15 10:57:16</dc:Date>
		<dc:Format>text/rdf</dc:Format>
		<dc:Language>en</dc:Language>
		<skos:editorialNote>Generated by testgenall.php on Thu Mar 29 10:24:08 PDT 2012.</skos:editorialNote>
		<skos:historyNote>No previous definition revisions.</skos:historyNote>
		<skos:changeNote>This is the first and only definition provided.</skos:changeNote>
		<skos:scopeNote>http://www.w3.org/2004/02/skos/core#Concept</skos:scopeNote>
		<skos:Note>SKOS properties defined in http://www.w3.org/TR/skos-primer/#secrel</skos:Note>
		<skos:inScheme rdf:resource="http://www.cognitiveatlas.org/tasks/"/>
		<skos:definition>is a measure of short term visual memory that has been designed for use both as a clinical tool and a research instrument.  In the VPT, the subject is presented with matrix patterns of black and white squares in grids of varying size and required to memorize a series of black and white checkerboard-like patterns of increasing complexity. Such matrix patterns are virtually impossible to code verbally.</skos:definition>
		<skos:prefLabel>Visual Patterns Test</skos:prefLabel>
		<skos:altLabel></skos:altLabel>
</skos:Concept><skos:Concept rdf:about="http://www.cognitiveatlas.org/id/trm_4da887bdd8908"> <dc:identifier>trm_4da887bdd8908</dc:identifier>
		<dc:Title>Cognitive Atlas : Lexicon : mirror tracing test</dc:Title>
		<dc:Description>RDF output for 'mirror tracing test'</dc:Description>
		<dc:Type>InteractiveResource</dc:Type>
		<dc:Publisher>Cognitive Atlas</dc:Publisher>
		<dc:Creator>Cognitive Atlas RDF Generator</dc:Creator>
		<dc:Contributor>Natalie Picchetti</dc:Contributor>
		<dc:Date>2011-04-15 11:00:29</dc:Date>
		<dc:Format>text/rdf</dc:Format>
		<dc:Language>en</dc:Language>
		<skos:editorialNote>Generated by testgenall.php on Thu Mar 29 10:24:08 PDT 2012.</skos:editorialNote>
		<skos:historyNote>No previous definition revisions.</skos:historyNote>
		<skos:changeNote>This is the first and only definition provided.</skos:changeNote>
		<skos:scopeNote>http://www.w3.org/2004/02/skos/core#Concept</skos:scopeNote>
		<skos:Note>SKOS properties defined in http://www.w3.org/TR/skos-primer/#secrel</skos:Note>
		<skos:inScheme rdf:resource="http://www.cognitiveatlas.org/tasks/"/>
		<skos:definition>No definition submitted yet.</skos:definition>
		<skos:prefLabel>mirror tracing test</skos:prefLabel>
		<skos:altLabel></skos:altLabel>
</skos:Concept><skos:Concept rdf:about="http://www.cognitiveatlas.org/id/trm_4da8885b33375"> <dc:identifier>trm_4da8885b33375</dc:identifier>
		<dc:Title>Cognitive Atlas : Lexicon : Rivermead Behavioural Memory Test</dc:Title>
		<dc:Description>RDF output for 'Rivermead Behavioural Memory Test'</dc:Description>
		<dc:Type>InteractiveResource</dc:Type>
		<dc:Publisher>Cognitive Atlas</dc:Publisher>
		<dc:Creator>Cognitive Atlas RDF Generator</dc:Creator>
		<dc:Contributor>Natalie Picchetti</dc:Contributor>
		<dc:Date>2011-04-15 11:03:07</dc:Date>
		<dc:Format>text/rdf</dc:Format>
		<dc:Language>en</dc:Language>
		<skos:editorialNote>Generated by testgenall.php on Thu Mar 29 10:24:08 PDT 2012.</skos:editorialNote>
		<skos:historyNote>No previous definition revisions.</skos:historyNote>
		<skos:changeNote>This is the first and only definition provided.</skos:changeNote>
		<skos:scopeNote>http://www.w3.org/2004/02/skos/core#Concept</skos:scopeNote>
		<skos:Note>SKOS properties defined in http://www.w3.org/TR/skos-primer/#secrel</skos:Note>
		<skos:inScheme rdf:resource="http://www.cognitiveatlas.org/tasks/"/>
		<skos:definition>comprises a number of subtests focused on providing objective measures of everyday memory performance in people with observed and/or reported memory difficulties.</skos:definition>
		<skos:prefLabel>Rivermead Behavioural Memory Test</skos:prefLabel>
		<skos:altLabel></skos:altLabel>
</skos:Concept><skos:Concept rdf:about="http://www.cognitiveatlas.org/id/trm_4da88a2a63d97"> <dc:identifier>trm_4da88a2a63d97</dc:identifier>
		<dc:Title>Cognitive Atlas : Lexicon : Paired Associate Learning</dc:Title>
		<dc:Description>RDF output for 'Paired Associate Learning'</dc:Description>
		<dc:Type>InteractiveResource</dc:Type>
		<dc:Publisher>Cognitive Atlas</dc:Publisher>
		<dc:Creator>Cognitive Atlas RDF Generator</dc:Creator>
		<dc:Contributor>Russ Poldrack</dc:Contributor>
		<dc:Date>2012-01-28 08:09:44</dc:Date>
		<dc:Format>text/rdf</dc:Format>
		<dc:Language>en</dc:Language>
		<skos:editorialNote>Generated by testgenall.php on Thu Mar 29 10:24:08 PDT 2012.</skos:editorialNote>
		<skos:historyNote>Revision 2: 1 previous definitions.</skos:historyNote>
		<skos:changeNote>See http://www.cognitiveatlas.org/id/trm_4da88a2a63d97 for complete revision history.</skos:changeNote>
		<skos:scopeNote>http://www.w3.org/2004/02/skos/core#Concept</skos:scopeNote>
		<skos:Note>SKOS properties defined in http://www.w3.org/TR/skos-primer/#secrel</skos:Note>
		<skos:inScheme rdf:resource="http://www.cognitiveatlas.org/tasks/"/>
		<skos:definition>was invented by Mary Whiton Calkins in 1894 and involves the pairing of two items (usually words)—a stimulus and a response. For example, words such as calendar (stimulus) and shoe (response) may be paired, and when the learner is prompted with the stimulus, he responds with the appropriate word (shoe).</skos:definition>
		<skos:prefLabel>Paired Associate Learning</skos:prefLabel>
		<skos:altLabel>associative learning task</skos:altLabel>
</skos:Concept><skos:Concept rdf:about="http://www.cognitiveatlas.org/id/trm_4da88a8e13f26"> <dc:identifier>trm_4da88a8e13f26</dc:identifier>
		<dc:Title>Cognitive Atlas : Lexicon : Vigilance</dc:Title>
		<dc:Description>RDF output for 'Vigilance'</dc:Description>
		<dc:Type>InteractiveResource</dc:Type>
		<dc:Publisher>Cognitive Atlas</dc:Publisher>
		<dc:Creator>Cognitive Atlas RDF Generator</dc:Creator>
		<dc:Contributor>Russ Poldrack</dc:Contributor>
		<dc:Date>2012-01-28 08:27:19</dc:Date>
		<dc:Format>text/rdf</dc:Format>
		<dc:Language>en</dc:Language>
		<skos:editorialNote>Generated by testgenall.php on Thu Mar 29 10:24:08 PDT 2012.</skos:editorialNote>
		<skos:historyNote>Revision 2: 1 previous definitions.</skos:historyNote>
		<skos:changeNote>See http://www.cognitiveatlas.org/id/trm_4da88a8e13f26 for complete revision history.</skos:changeNote>
		<skos:scopeNote>http://www.w3.org/2004/02/skos/core#Concept</skos:scopeNote>
		<skos:Note>SKOS properties defined in http://www.w3.org/TR/skos-primer/#secrel</skos:Note>
		<skos:inScheme rdf:resource="http://www.cognitiveatlas.org/tasks/"/>
		<skos:definition>No definition submitted yet.</skos:definition>
		<skos:prefLabel>Vigilance</skos:prefLabel>
		<skos:altLabel>sustained attention task</skos:altLabel>
</skos:Concept><skos:Concept rdf:about="http://www.cognitiveatlas.org/id/trm_4da88ae0f2952"> <dc:identifier>trm_4da88ae0f2952</dc:identifier>
		<dc:Title>Cognitive Atlas : Lexicon : Rey Auditory Verbal Learning Task</dc:Title>
		<dc:Description>RDF output for 'Rey Auditory Verbal Learning Task'</dc:Description>
		<dc:Type>InteractiveResource</dc:Type>
		<dc:Publisher>Cognitive Atlas</dc:Publisher>
		<dc:Creator>Cognitive Atlas RDF Generator</dc:Creator>
		<dc:Contributor>Natalie Picchetti</dc:Contributor>
		<dc:Date>2011-04-15 11:13:52</dc:Date>
		<dc:Format>text/rdf</dc:Format>
		<dc:Language>en</dc:Language>
		<skos:editorialNote>Generated by testgenall.php on Thu Mar 29 10:24:08 PDT 2012.</skos:editorialNote>
		<skos:historyNote>No previous definition revisions.</skos:historyNote>
		<skos:changeNote>This is the first and only definition provided.</skos:changeNote>
		<skos:scopeNote>http://www.w3.org/2004/02/skos/core#Concept</skos:scopeNote>
		<skos:Note>SKOS properties defined in http://www.w3.org/TR/skos-primer/#secrel</skos:Note>
		<skos:inScheme rdf:resource="http://www.cognitiveatlas.org/tasks/"/>
		<skos:definition>No definition submitted yet.</skos:definition>
		<skos:prefLabel>Rey Auditory Verbal Learning Task</skos:prefLabel>
		<skos:altLabel></skos:altLabel>
</skos:Concept><skos:Concept rdf:about="http://www.cognitiveatlas.org/id/trm_4da88b17b985b"> <dc:identifier>trm_4da88b17b985b</dc:identifier>
		<dc:Title>Cognitive Atlas : Lexicon : Nonword Repetition Task</dc:Title>
		<dc:Description>RDF output for 'Nonword Repetition Task'</dc:Description>
		<dc:Type>InteractiveResource</dc:Type>
		<dc:Publisher>Cognitive Atlas</dc:Publisher>
		<dc:Creator>Cognitive Atlas RDF Generator</dc:Creator>
		<dc:Contributor>Natalie Picchetti</dc:Contributor>
		<dc:Date>2011-04-15 11:14:47</dc:Date>
		<dc:Format>text/rdf</dc:Format>
		<dc:Language>en</dc:Language>
		<skos:editorialNote>Generated by testgenall.php on Thu Mar 29 10:24:08 PDT 2012.</skos:editorialNote>
		<skos:historyNote>No previous definition revisions.</skos:historyNote>
		<skos:changeNote>This is the first and only definition provided.</skos:changeNote>
		<skos:scopeNote>http://www.w3.org/2004/02/skos/core#Concept</skos:scopeNote>
		<skos:Note>SKOS properties defined in http://www.w3.org/TR/skos-primer/#secrel</skos:Note>
		<skos:inScheme rdf:resource="http://www.cognitiveatlas.org/tasks/"/>
		<skos:definition>No definition submitted yet.</skos:definition>
		<skos:prefLabel>Nonword Repetition Task</skos:prefLabel>
		<skos:altLabel></skos:altLabel>
</skos:Concept><skos:Concept rdf:about="http://www.cognitiveatlas.org/id/trm_4da88b3b0cbcc"> <dc:identifier>trm_4da88b3b0cbcc</dc:identifier>
		<dc:Title>Cognitive Atlas : Lexicon : Response Mapping Task</dc:Title>
		<dc:Description>RDF output for 'Response Mapping Task'</dc:Description>
		<dc:Type>InteractiveResource</dc:Type>
		<dc:Publisher>Cognitive Atlas</dc:Publisher>
		<dc:Creator>Cognitive Atlas RDF Generator</dc:Creator>
		<dc:Contributor>Natalie Picchetti</dc:Contributor>
		<dc:Date>2011-04-15 11:15:23</dc:Date>
		<dc:Format>text/rdf</dc:Format>
		<dc:Language>en</dc:Language>
		<skos:editorialNote>Generated by testgenall.php on Thu Mar 29 10:24:08 PDT 2012.</skos:editorialNote>
		<skos:historyNote>No previous definition revisions.</skos:historyNote>
		<skos:changeNote>This is the first and only definition provided.</skos:changeNote>
		<skos:scopeNote>http://www.w3.org/2004/02/skos/core#Concept</skos:scopeNote>
		<skos:Note>SKOS properties defined in http://www.w3.org/TR/skos-primer/#secrel</skos:Note>
		<skos:inScheme rdf:resource="http://www.cognitiveatlas.org/tasks/"/>
		<skos:definition>No definition submitted yet.</skos:definition>
		<skos:prefLabel>Response Mapping Task</skos:prefLabel>
		<skos:altLabel></skos:altLabel>
</skos:Concept><skos:Concept rdf:about="http://www.cognitiveatlas.org/id/trm_4da88b63787d6"> <dc:identifier>trm_4da88b63787d6</dc:identifier>
		<dc:Title>Cognitive Atlas : Lexicon : Pursuit Rotor Task</dc:Title>
		<dc:Description>RDF output for 'Pursuit Rotor Task'</dc:Description>
		<dc:Type>InteractiveResource</dc:Type>
		<dc:Publisher>Cognitive Atlas</dc:Publisher>
		<dc:Creator>Cognitive Atlas RDF Generator</dc:Creator>
		<dc:Contributor>Natalie Picchetti</dc:Contributor>
		<dc:Date>2011-05-19 14:20:24</dc:Date>
		<dc:Format>text/rdf</dc:Format>
		<dc:Language>en</dc:Language>
		<skos:editorialNote>Generated by testgenall.php on Thu Mar 29 10:24:08 PDT 2012.</skos:editorialNote>
		<skos:historyNote>Revision 2: 1 previous definitions.</skos:historyNote>
		<skos:changeNote>See http://www.cognitiveatlas.org/id/trm_4da88b63787d6 for complete revision history.</skos:changeNote>
		<skos:scopeNote>http://www.w3.org/2004/02/skos/core#Concept</skos:scopeNote>
		<skos:Note>SKOS properties defined in http://www.w3.org/TR/skos-primer/#secrel</skos:Note>
		<skos:inScheme rdf:resource="http://www.cognitiveatlas.org/tasks/"/>
		<skos:definition>The pursuit rotor task is a task used in common use in the mid 20th century which involved a participant trying to follow (pursue) a small disc on a rotating turntable. Original mechanical versions had typical rotation rates of 60 RPM, which is probably too fast for mouse-controlled versions. The PEBL version offers a simple version with multiple trials and controllable parameters that can be used as a test of hand-eye coordination. </skos:definition>
		<skos:prefLabel>Pursuit Rotor Task</skos:prefLabel>
		<skos:altLabel></skos:altLabel>
</skos:Concept><skos:Concept rdf:about="http://www.cognitiveatlas.org/id/trm_4da88b8b60ffb"> <dc:identifier>trm_4da88b8b60ffb</dc:identifier>
		<dc:Title>Cognitive Atlas : Lexicon : alternating runs paradigm</dc:Title>
		<dc:Description>RDF output for 'alternating runs paradigm'</dc:Description>
		<dc:Type>InteractiveResource</dc:Type>
		<dc:Publisher>Cognitive Atlas</dc:Publisher>
		<dc:Creator>Cognitive Atlas RDF Generator</dc:Creator>
		<dc:Contributor>Corey White</dc:Contributor>
		<dc:Date>2011-08-15 10:58:20</dc:Date>
		<dc:Format>text/rdf</dc:Format>
		<dc:Language>en</dc:Language>
		<skos:editorialNote>Generated by testgenall.php on Thu Mar 29 10:24:08 PDT 2012.</skos:editorialNote>
		<skos:historyNote>Revision 2: 1 previous definitions.</skos:historyNote>
		<skos:changeNote>See http://www.cognitiveatlas.org/id/trm_4da88b8b60ffb for complete revision history.</skos:changeNote>
		<skos:scopeNote>http://www.w3.org/2004/02/skos/core#Concept</skos:scopeNote>
		<skos:Note>SKOS properties defined in http://www.w3.org/TR/skos-primer/#secrel</skos:Note>
		<skos:inScheme rdf:resource="http://www.cognitiveatlas.org/tasks/"/>
		<skos:definition>A type of task-switching paradigm in which two different tasks are presented in alternating runs or blocks</skos:definition>
		<skos:prefLabel>alternating runs paradigm</skos:prefLabel>
		<skos:altLabel></skos:altLabel>
		<skos:related rdf:resource="http://www.cognitiveatlas.org/id/trm_4a3fd79d0a246"/>
		<skos:example>executive control is measured by the contrast of  trials in the alternating runs paradigm</skos:example>
		<cito:citesForInformation rdf:resource="http://www.cognitiveatlas.org/citation/id/cit_4e495eb285c64"/>
		<cito:citesForInformation rdf:resource="http://www.cognitiveatlas.org/citation/id/cit_4e495ed0e80a4"/>
</skos:Concept><skos:Concept rdf:about="http://www.cognitiveatlas.org/id/trm_4da88bb3c2462"> <dc:identifier>trm_4da88bb3c2462</dc:identifier>
		<dc:Title>Cognitive Atlas : Lexicon : object alternation task</dc:Title>
		<dc:Description>RDF output for 'object alternation task'</dc:Description>
		<dc:Type>InteractiveResource</dc:Type>
		<dc:Publisher>Cognitive Atlas</dc:Publisher>
		<dc:Creator>Cognitive Atlas RDF Generator</dc:Creator>
		<dc:Contributor>Natalie Picchetti</dc:Contributor>
		<dc:Date>2011-04-15 11:17:23</dc:Date>
		<dc:Format>text/rdf</dc:Format>
		<dc:Language>en</dc:Language>
		<skos:editorialNote>Generated by testgenall.php on Thu Mar 29 10:24:08 PDT 2012.</skos:editorialNote>
		<skos:historyNote>No previous definition revisions.</skos:historyNote>
		<skos:changeNote>This is the first and only definition provided.</skos:changeNote>
		<skos:scopeNote>http://www.w3.org/2004/02/skos/core#Concept</skos:scopeNote>
		<skos:Note>SKOS properties defined in http://www.w3.org/TR/skos-primer/#secrel</skos:Note>
		<skos:inScheme rdf:resource="http://www.cognitiveatlas.org/tasks/"/>
		<skos:definition>No definition submitted yet.</skos:definition>
		<skos:prefLabel>object alternation task</skos:prefLabel>
		<skos:altLabel></skos:altLabel>
</skos:Concept><skos:Concept rdf:about="http://www.cognitiveatlas.org/id/trm_4da88bd4412da"> <dc:identifier>trm_4da88bd4412da</dc:identifier>
		<dc:Title>Cognitive Atlas : Lexicon : animal naming task</dc:Title>
		<dc:Description>RDF output for 'animal naming task'</dc:Description>
		<dc:Type>InteractiveResource</dc:Type>
		<dc:Publisher>Cognitive Atlas</dc:Publisher>
		<dc:Creator>Cognitive Atlas RDF Generator</dc:Creator>
		<dc:Contributor>Corey White</dc:Contributor>
		<dc:Date>2011-08-15 11:05:39</dc:Date>
		<dc:Format>text/rdf</dc:Format>
		<dc:Language>en</dc:Language>
		<skos:editorialNote>Generated by testgenall.php on Thu Mar 29 10:24:08 PDT 2012.</skos:editorialNote>
		<skos:historyNote>Revision 2: 1 previous definitions.</skos:historyNote>
		<skos:changeNote>See http://www.cognitiveatlas.org/id/trm_4da88bd4412da for complete revision history.</skos:changeNote>
		<skos:scopeNote>http://www.w3.org/2004/02/skos/core#Concept</skos:scopeNote>
		<skos:Note>SKOS properties defined in http://www.w3.org/TR/skos-primer/#secrel</skos:Note>
		<skos:inScheme rdf:resource="http://www.cognitiveatlas.org/tasks/"/>
		<skos:definition>animals are presented, usually pictorially, and participants are asked to name them aloud</skos:definition>
		<skos:prefLabel>animal naming task</skos:prefLabel>
		<skos:altLabel></skos:altLabel>
		<skos:related rdf:resource="http://www.cognitiveatlas.org/id/trm_4a3fd79d0b077"/>
		<skos:related rdf:resource="http://www.cognitiveatlas.org/id/trm_4a3fd79d0b44c"/>
		<skos:example>semantic knowledge is measured by the contrast of  trials in the animal naming task</skos:example>
		<skos:example>verbal fluency is measured by the contrast of  trials in the animal naming task</skos:example>
</skos:Concept><skos:Concept rdf:about="http://www.cognitiveatlas.org/id/trm_4da88bff0507c"> <dc:identifier>trm_4da88bff0507c</dc:identifier>
		<dc:Title>Cognitive Atlas : Lexicon : CatBat task</dc:Title>
		<dc:Description>RDF output for 'CatBat task'</dc:Description>
		<dc:Type>InteractiveResource</dc:Type>
		<dc:Publisher>Cognitive Atlas</dc:Publisher>
		<dc:Creator>Cognitive Atlas RDF Generator</dc:Creator>
		<dc:Contributor>Natalie Picchetti</dc:Contributor>
		<dc:Date>2011-04-15 11:18:39</dc:Date>
		<dc:Format>text/rdf</dc:Format>
		<dc:Language>en</dc:Language>
		<skos:editorialNote>Generated by testgenall.php on Thu Mar 29 10:24:08 PDT 2012.</skos:editorialNote>
		<skos:historyNote>No previous definition revisions.</skos:historyNote>
		<skos:changeNote>This is the first and only definition provided.</skos:changeNote>
		<skos:scopeNote>http://www.w3.org/2004/02/skos/core#Concept</skos:scopeNote>
		<skos:Note>SKOS properties defined in http://www.w3.org/TR/skos-primer/#secrel</skos:Note>
		<skos:inScheme rdf:resource="http://www.cognitiveatlas.org/tasks/"/>
		<skos:definition>No definition submitted yet.</skos:definition>
		<skos:prefLabel>CatBat task</skos:prefLabel>
		<skos:altLabel></skos:altLabel>
</skos:Concept><skos:Concept rdf:about="http://www.cognitiveatlas.org/id/trm_4da88c205b16b"> <dc:identifier>trm_4da88c205b16b</dc:identifier>
		<dc:Title>Cognitive Atlas : Lexicon : Haptic Illusion Task</dc:Title>
		<dc:Description>RDF output for 'Haptic Illusion Task'</dc:Description>
		<dc:Type>InteractiveResource</dc:Type>
		<dc:Publisher>Cognitive Atlas</dc:Publisher>
		<dc:Creator>Cognitive Atlas RDF Generator</dc:Creator>
		<dc:Contributor>Natalie Picchetti</dc:Contributor>
		<dc:Date>2011-04-15 11:19:12</dc:Date>
		<dc:Format>text/rdf</dc:Format>
		<dc:Language>en</dc:Language>
		<skos:editorialNote>Generated by testgenall.php on Thu Mar 29 10:24:08 PDT 2012.</skos:editorialNote>
		<skos:historyNote>No previous definition revisions.</skos:historyNote>
		<skos:changeNote>This is the first and only definition provided.</skos:changeNote>
		<skos:scopeNote>http://www.w3.org/2004/02/skos/core#Concept</skos:scopeNote>
		<skos:Note>SKOS properties defined in http://www.w3.org/TR/skos-primer/#secrel</skos:Note>
		<skos:inScheme rdf:resource="http://www.cognitiveatlas.org/tasks/"/>
		<skos:definition>No definition submitted yet.</skos:definition>
		<skos:prefLabel>Haptic Illusion Task</skos:prefLabel>
		<skos:altLabel></skos:altLabel>
</skos:Concept><skos:Concept rdf:about="http://www.cognitiveatlas.org/id/trm_4da88c5302e06"> <dc:identifier>trm_4da88c5302e06</dc:identifier>
		<dc:Title>Cognitive Atlas : Lexicon : Brixton Spatial Anticipation Test</dc:Title>
		<dc:Description>RDF output for 'Brixton Spatial Anticipation Test'</dc:Description>
		<dc:Type>InteractiveResource</dc:Type>
		<dc:Publisher>Cognitive Atlas</dc:Publisher>
		<dc:Creator>Cognitive Atlas RDF Generator</dc:Creator>
		<dc:Contributor>Natalie Picchetti</dc:Contributor>
		<dc:Date>2011-04-15 11:20:03</dc:Date>
		<dc:Format>text/rdf</dc:Format>
		<dc:Language>en</dc:Language>
		<skos:editorialNote>Generated by testgenall.php on Thu Mar 29 10:24:08 PDT 2012.</skos:editorialNote>
		<skos:historyNote>No previous definition revisions.</skos:historyNote>
		<skos:changeNote>This is the first and only definition provided.</skos:changeNote>
		<skos:scopeNote>http://www.w3.org/2004/02/skos/core#Concept</skos:scopeNote>
		<skos:Note>SKOS properties defined in http://www.w3.org/TR/skos-primer/#secrel</skos:Note>
		<skos:inScheme rdf:resource="http://www.cognitiveatlas.org/tasks/"/>
		<skos:definition>No definition submitted yet.</skos:definition>
		<skos:prefLabel>Brixton Spatial Anticipation Test</skos:prefLabel>
		<skos:altLabel></skos:altLabel>
</skos:Concept><skos:Concept rdf:about="http://www.cognitiveatlas.org/id/trm_4da88c904862b"> <dc:identifier>trm_4da88c904862b</dc:identifier>
		<dc:Title>Cognitive Atlas : Lexicon : Hayling Sentence Completion Test</dc:Title>
		<dc:Description>RDF output for 'Hayling Sentence Completion Test'</dc:Description>
		<dc:Type>InteractiveResource</dc:Type>
		<dc:Publisher>Cognitive Atlas</dc:Publisher>
		<dc:Creator>Cognitive Atlas RDF Generator</dc:Creator>
		<dc:Contributor>Carinna Torgerson</dc:Contributor>
		<dc:Date>2011-06-27 13:47:59</dc:Date>
		<dc:Format>text/rdf</dc:Format>
		<dc:Language>en</dc:Language>
		<skos:editorialNote>Generated by testgenall.php on Thu Mar 29 10:24:08 PDT 2012.</skos:editorialNote>
		<skos:historyNote>Revision 2: 1 previous definitions.</skos:historyNote>
		<skos:changeNote>See http://www.cognitiveatlas.org/id/trm_4da88c904862b for complete revision history.</skos:changeNote>
		<skos:scopeNote>http://www.w3.org/2004/02/skos/core#Concept</skos:scopeNote>
		<skos:Note>SKOS properties defined in http://www.w3.org/TR/skos-primer/#secrel</skos:Note>
		<skos:inScheme rdf:resource="http://www.cognitiveatlas.org/tasks/"/>
		<skos:definition>Participants are given the beginnings of sentences to complete. The sentences appear to have expected answers. In the first condition, participants must complete the sentence with a/the word that makes sense. In the second condition, participants are asked to complete sentences by saying semantically unrelated words, thereby making the sentence nonsensical.</skos:definition>
		<skos:prefLabel>Hayling Sentence Completion Test</skos:prefLabel>
		<skos:altLabel></skos:altLabel>
		<skos:related rdf:resource="http://www.cognitiveatlas.org/id/tsk_4a57abb949d9f"/>
		<skos:related rdf:resource="http://www.cognitiveatlas.org/id/trm_4a3fd79d09f2a"/>
		<skos:related rdf:resource="http://www.cognitiveatlas.org/id/trm_4a3fd79d0af66"/>
		<skos:related rdf:resource="http://www.cognitiveatlas.org/id/trm_4a3fd79d0b892"/>
		<skos:example>sentence completion test is a broader synonym of Hayling Sentence Completion Test</skos:example>
		<skos:example>creative cognition is measured by the contrast of converted A and B error score trials in the Hayling Sentence Completion Test</skos:example>
		<skos:example>response inhibition is measured by the contrast of Initiation minus Inhibition trials in the Hayling Sentence Completion Test</skos:example>
		<skos:example>sentence comprehension is measured by the contrast of Initiation trials in the Hayling Sentence Completion Test</skos:example>
		<cito:citesForInformation rdf:resource="http://www.cognitiveatlas.org/citation/id/cit_4dfa7488e31e4"/>
		<cito:citesForInformation rdf:resource="http://www.cognitiveatlas.org/citation/id/cit_4e08ed2959c6e"/>
</skos:Concept><skos:Concept rdf:about="http://www.cognitiveatlas.org/id/trm_4da88cb222308"> <dc:identifier>trm_4da88cb222308</dc:identifier>
		<dc:Title>Cognitive Atlas : Lexicon : Picture Set Test</dc:Title>
		<dc:Description>RDF output for 'Picture Set Test'</dc:Description>
		<dc:Type>InteractiveResource</dc:Type>
		<dc:Publisher>Cognitive Atlas</dc:Publisher>
		<dc:Creator>Cognitive Atlas RDF Generator</dc:Creator>
		<dc:Contributor>Natalie Picchetti</dc:Contributor>
		<dc:Date>2011-04-15 11:21:38</dc:Date>
		<dc:Format>text/rdf</dc:Format>
		<dc:Language>en</dc:Language>
		<skos:editorialNote>Generated by testgenall.php on Thu Mar 29 10:24:08 PDT 2012.</skos:editorialNote>
		<skos:historyNote>No previous definition revisions.</skos:historyNote>
		<skos:changeNote>This is the first and only definition provided.</skos:changeNote>
		<skos:scopeNote>http://www.w3.org/2004/02/skos/core#Concept</skos:scopeNote>
		<skos:Note>SKOS properties defined in http://www.w3.org/TR/skos-primer/#secrel</skos:Note>
		<skos:inScheme rdf:resource="http://www.cognitiveatlas.org/tasks/"/>
		<skos:definition>No definition submitted yet.</skos:definition>
		<skos:prefLabel>Picture Set Test</skos:prefLabel>
		<skos:altLabel></skos:altLabel>
</skos:Concept><skos:Concept rdf:about="http://www.cognitiveatlas.org/id/trm_4da88ec6735ad"> <dc:identifier>trm_4da88ec6735ad</dc:identifier>
		<dc:Title>Cognitive Atlas : Lexicon : Uznadze Haptic Illusion Task</dc:Title>
		<dc:Description>RDF output for 'Uznadze Haptic Illusion Task'</dc:Description>
		<dc:Type>InteractiveResource</dc:Type>
		<dc:Publisher>Cognitive Atlas</dc:Publisher>
		<dc:Creator>Cognitive Atlas RDF Generator</dc:Creator>
		<dc:Contributor>Natalie Picchetti</dc:Contributor>
		<dc:Date>2011-04-15 11:30:30</dc:Date>
		<dc:Format>text/rdf</dc:Format>
		<dc:Language>en</dc:Language>
		<skos:editorialNote>Generated by testgenall.php on Thu Mar 29 10:24:08 PDT 2012.</skos:editorialNote>
		<skos:historyNote>No previous definition revisions.</skos:historyNote>
		<skos:changeNote>This is the first and only definition provided.</skos:changeNote>
		<skos:scopeNote>http://www.w3.org/2004/02/skos/core#Concept</skos:scopeNote>
		<skos:Note>SKOS properties defined in http://www.w3.org/TR/skos-primer/#secrel</skos:Note>
		<skos:inScheme rdf:resource="http://www.cognitiveatlas.org/tasks/"/>
		<skos:definition>No definition submitted yet.</skos:definition>
		<skos:prefLabel>Uznadze Haptic Illusion Task</skos:prefLabel>
		<skos:altLabel></skos:altLabel>
</skos:Concept><skos:Concept rdf:about="http://www.cognitiveatlas.org/id/trm_4da890594742a"> <dc:identifier>trm_4da890594742a</dc:identifier>
		<dc:Title>Cognitive Atlas : Lexicon : emotional regulation task</dc:Title>
		<dc:Description>RDF output for 'emotional regulation task'</dc:Description>
		<dc:Type>InteractiveResource</dc:Type>
		<dc:Publisher>Cognitive Atlas</dc:Publisher>
		<dc:Creator>Cognitive Atlas RDF Generator</dc:Creator>
		<dc:Contributor>Natalie Picchetti</dc:Contributor>
		<dc:Date>2011-04-15 11:37:13</dc:Date>
		<dc:Format>text/rdf</dc:Format>
		<dc:Language>en</dc:Language>
		<skos:editorialNote>Generated by testgenall.php on Thu Mar 29 10:24:08 PDT 2012.</skos:editorialNote>
		<skos:historyNote>No previous definition revisions.</skos:historyNote>
		<skos:changeNote>This is the first and only definition provided.</skos:changeNote>
		<skos:scopeNote>http://www.w3.org/2004/02/skos/core#Concept</skos:scopeNote>
		<skos:Note>SKOS properties defined in http://www.w3.org/TR/skos-primer/#secrel</skos:Note>
		<skos:inScheme rdf:resource="http://www.cognitiveatlas.org/tasks/"/>
		<skos:definition>No definition submitted yet.</skos:definition>
		<skos:prefLabel>emotional regulation task</skos:prefLabel>
		<skos:altLabel></skos:altLabel>
</skos:Concept><skos:Concept rdf:about="http://www.cognitiveatlas.org/id/trm_4da89077f19ae"> <dc:identifier>trm_4da89077f19ae</dc:identifier>
		<dc:Title>Cognitive Atlas : Lexicon : Digit Cancellation Task</dc:Title>
		<dc:Description>RDF output for 'Digit Cancellation Task'</dc:Description>
		<dc:Type>InteractiveResource</dc:Type>
		<dc:Publisher>Cognitive Atlas</dc:Publisher>
		<dc:Creator>Cognitive Atlas RDF Generator</dc:Creator>
		<dc:Contributor>Natalie Picchetti</dc:Contributor>
		<dc:Date>2011-04-15 11:37:43</dc:Date>
		<dc:Format>text/rdf</dc:Format>
		<dc:Language>en</dc:Language>
		<skos:editorialNote>Generated by testgenall.php on Thu Mar 29 10:24:08 PDT 2012.</skos:editorialNote>
		<skos:historyNote>No previous definition revisions.</skos:historyNote>
		<skos:changeNote>This is the first and only definition provided.</skos:changeNote>
		<skos:scopeNote>http://www.w3.org/2004/02/skos/core#Concept</skos:scopeNote>
		<skos:Note>SKOS properties defined in http://www.w3.org/TR/skos-primer/#secrel</skos:Note>
		<skos:inScheme rdf:resource="http://www.cognitiveatlas.org/tasks/"/>
		<skos:definition>No definition submitted yet.</skos:definition>
		<skos:prefLabel>Digit Cancellation Task</skos:prefLabel>
		<skos:altLabel></skos:altLabel>
</skos:Concept><skos:Concept rdf:about="http://www.cognitiveatlas.org/id/trm_4da89089ce0af"> <dc:identifier>trm_4da89089ce0af</dc:identifier>
		<dc:Title>Cognitive Atlas : Lexicon : Zoo Map Test</dc:Title>
		<dc:Description>RDF output for 'Zoo Map Test'</dc:Description>
		<dc:Type>InteractiveResource</dc:Type>
		<dc:Publisher>Cognitive Atlas</dc:Publisher>
		<dc:Creator>Cognitive Atlas RDF Generator</dc:Creator>
		<dc:Contributor>Natalie Picchetti</dc:Contributor>
		<dc:Date>2011-04-15 11:38:01</dc:Date>
		<dc:Format>text/rdf</dc:Format>
		<dc:Language>en</dc:Language>
		<skos:editorialNote>Generated by testgenall.php on Thu Mar 29 10:24:08 PDT 2012.</skos:editorialNote>
		<skos:historyNote>No previous definition revisions.</skos:historyNote>
		<skos:changeNote>This is the first and only definition provided.</skos:changeNote>
		<skos:scopeNote>http://www.w3.org/2004/02/skos/core#Concept</skos:scopeNote>
		<skos:Note>SKOS properties defined in http://www.w3.org/TR/skos-primer/#secrel</skos:Note>
		<skos:inScheme rdf:resource="http://www.cognitiveatlas.org/tasks/"/>
		<skos:prefLabel>Zoo Map Test</skos:prefLabel>
		<skos:altLabel></skos:altLabel>
</skos:Concept><skos:Concept rdf:about="http://www.cognitiveatlas.org/id/trm_4da890a9bd7a3"> <dc:identifier>trm_4da890a9bd7a3</dc:identifier>
		<dc:Title>Cognitive Atlas : Lexicon : Morris Water Maze</dc:Title>
		<dc:Description>RDF output for 'Morris Water Maze'</dc:Description>
		<dc:Type>InteractiveResource</dc:Type>
		<dc:Publisher>Cognitive Atlas</dc:Publisher>
		<dc:Creator>Cognitive Atlas RDF Generator</dc:Creator>
		<dc:Contributor>Russ Poldrack</dc:Contributor>
		<dc:Date>2012-01-28 07:53:15</dc:Date>
		<dc:Format>text/rdf</dc:Format>
		<dc:Language>en</dc:Language>
		<skos:editorialNote>Generated by testgenall.php on Thu Mar 29 10:24:08 PDT 2012.</skos:editorialNote>
		<skos:historyNote>Revision 2: 1 previous definitions.</skos:historyNote>
		<skos:changeNote>See http://www.cognitiveatlas.org/id/trm_4da890a9bd7a3 for complete revision history.</skos:changeNote>
		<skos:scopeNote>http://www.w3.org/2004/02/skos/core#Concept</skos:scopeNote>
		<skos:Note>SKOS properties defined in http://www.w3.org/TR/skos-primer/#secrel</skos:Note>
		<skos:inScheme rdf:resource="http://www.cognitiveatlas.org/tasks/"/>
		<skos:definition>No definition submitted yet.</skos:definition>
		<skos:prefLabel>Morris Water Maze</skos:prefLabel>
		<skos:altLabel>morris water task</skos:altLabel>
</skos:Concept><skos:Concept rdf:about="http://www.cognitiveatlas.org/id/trm_4da890cf99b9e"> <dc:identifier>trm_4da890cf99b9e</dc:identifier>
		<dc:Title>Cognitive Atlas : Lexicon : Stockings of Cambridge Task</dc:Title>
		<dc:Description>RDF output for 'Stockings of Cambridge Task'</dc:Description>
		<dc:Type>InteractiveResource</dc:Type>
		<dc:Publisher>Cognitive Atlas</dc:Publisher>
		<dc:Creator>Cognitive Atlas RDF Generator</dc:Creator>
		<dc:Contributor>Natalie Picchetti</dc:Contributor>
		<dc:Date>2011-04-15 11:39:11</dc:Date>
		<dc:Format>text/rdf</dc:Format>
		<dc:Language>en</dc:Language>
		<skos:editorialNote>Generated by testgenall.php on Thu Mar 29 10:24:08 PDT 2012.</skos:editorialNote>
		<skos:historyNote>No previous definition revisions.</skos:historyNote>
		<skos:changeNote>This is the first and only definition provided.</skos:changeNote>
		<skos:scopeNote>http://www.w3.org/2004/02/skos/core#Concept</skos:scopeNote>
		<skos:Note>SKOS properties defined in http://www.w3.org/TR/skos-primer/#secrel</skos:Note>
		<skos:inScheme rdf:resource="http://www.cognitiveatlas.org/tasks/"/>
		<skos:definition>No definition submitted yet.</skos:definition>
		<skos:prefLabel>Stockings of Cambridge Task</skos:prefLabel>
		<skos:altLabel></skos:altLabel>
</skos:Concept><skos:Concept rdf:about="http://www.cognitiveatlas.org/id/trm_4da890f978492"> <dc:identifier>trm_4da890f978492</dc:identifier>
		<dc:Title>Cognitive Atlas : Lexicon : Glasgow Coma Scale</dc:Title>
		<dc:Description>RDF output for 'Glasgow Coma Scale'</dc:Description>
		<dc:Type>InteractiveResource</dc:Type>
		<dc:Publisher>Cognitive Atlas</dc:Publisher>
		<dc:Creator>Cognitive Atlas RDF Generator</dc:Creator>
		<dc:Contributor>Natalie Picchetti</dc:Contributor>
		<dc:Date>2011-04-20 16:58:30</dc:Date>
		<dc:Format>text/rdf</dc:Format>
		<dc:Language>en</dc:Language>
		<skos:editorialNote>Generated by testgenall.php on Thu Mar 29 10:24:08 PDT 2012.</skos:editorialNote>
		<skos:historyNote>Revision 2: 1 previous definitions.</skos:historyNote>
		<skos:changeNote>See http://www.cognitiveatlas.org/id/trm_4da890f978492 for complete revision history.</skos:changeNote>
		<skos:scopeNote>http://www.w3.org/2004/02/skos/core#Concept</skos:scopeNote>
		<skos:Note>SKOS properties defined in http://www.w3.org/TR/skos-primer/#secrel</skos:Note>
		<skos:inScheme rdf:resource="http://www.cognitiveatlas.org/tasks/"/>
		<skos:definition>is a neurological scale that aims to give a reliable, objective way of recording the conscious state of a person for initial as well as subsequent assessment. A patient is assessed against the criteria of the scale, and the resulting points give a patient score between 3 (indicating deep unconsciousness) and either 14 (original scale) or 15 (the more widely used modified or revised scale).</skos:definition>
		<skos:prefLabel>Glasgow Coma Scale</skos:prefLabel>
		<skos:altLabel></skos:altLabel>
</skos:Concept><skos:Concept rdf:about="http://www.cognitiveatlas.org/id/trm_4da8911e715e3"> <dc:identifier>trm_4da8911e715e3</dc:identifier>
		<dc:Title>Cognitive Atlas : Lexicon : Early Social Communications Scales</dc:Title>
		<dc:Description>RDF output for 'Early Social Communications Scales'</dc:Description>
		<dc:Type>InteractiveResource</dc:Type>
		<dc:Publisher>Cognitive Atlas</dc:Publisher>
		<dc:Creator>Cognitive Atlas RDF Generator</dc:Creator>
		<dc:Contributor>Natalie Picchetti</dc:Contributor>
		<dc:Date>2011-04-15 11:40:30</dc:Date>
		<dc:Format>text/rdf</dc:Format>
		<dc:Language>en</dc:Language>
		<skos:editorialNote>Generated by testgenall.php on Thu Mar 29 10:24:08 PDT 2012.</skos:editorialNote>
		<skos:historyNote>No previous definition revisions.</skos:historyNote>
		<skos:changeNote>This is the first and only definition provided.</skos:changeNote>
		<skos:scopeNote>http://www.w3.org/2004/02/skos/core#Concept</skos:scopeNote>
		<skos:Note>SKOS properties defined in http://www.w3.org/TR/skos-primer/#secrel</skos:Note>
		<skos:inScheme rdf:resource="http://www.cognitiveatlas.org/tasks/"/>
		<skos:definition>No definition submitted yet.</skos:definition>
		<skos:prefLabel>Early Social Communications Scales</skos:prefLabel>
		<skos:altLabel></skos:altLabel>
</skos:Concept><skos:Concept rdf:about="http://www.cognitiveatlas.org/id/trm_4da8914987ee2"> <dc:identifier>trm_4da8914987ee2</dc:identifier>
		<dc:Title>Cognitive Atlas : Lexicon : Reynell Developmental Language Scales</dc:Title>
		<dc:Description>RDF output for 'Reynell Developmental Language Scales'</dc:Description>
		<dc:Type>InteractiveResource</dc:Type>
		<dc:Publisher>Cognitive Atlas</dc:Publisher>
		<dc:Creator>Cognitive Atlas RDF Generator</dc:Creator>
		<dc:Contributor>Natalie Picchetti</dc:Contributor>
		<dc:Date>2011-04-15 11:41:13</dc:Date>
		<dc:Format>text/rdf</dc:Format>
		<dc:Language>en</dc:Language>
		<skos:editorialNote>Generated by testgenall.php on Thu Mar 29 10:24:08 PDT 2012.</skos:editorialNote>
		<skos:historyNote>No previous definition revisions.</skos:historyNote>
		<skos:changeNote>This is the first and only definition provided.</skos:changeNote>
		<skos:scopeNote>http://www.w3.org/2004/02/skos/core#Concept</skos:scopeNote>
		<skos:Note>SKOS properties defined in http://www.w3.org/TR/skos-primer/#secrel</skos:Note>
		<skos:inScheme rdf:resource="http://www.cognitiveatlas.org/tasks/"/>
		<skos:definition>No definition submitted yet.</skos:definition>
		<skos:prefLabel>Reynell Developmental Language Scales</skos:prefLabel>
		<skos:altLabel></skos:altLabel>
</skos:Concept><skos:Concept rdf:about="http://www.cognitiveatlas.org/id/trm_4da891794859f"> <dc:identifier>trm_4da891794859f</dc:identifier>
		<dc:Title>Cognitive Atlas : Lexicon : MacAuthur Communicative Development Inventory</dc:Title>
		<dc:Description>RDF output for 'MacAuthur Communicative Development Inventory'</dc:Description>
		<dc:Type>InteractiveResource</dc:Type>
		<dc:Publisher>Cognitive Atlas</dc:Publisher>
		<dc:Creator>Cognitive Atlas RDF Generator</dc:Creator>
		<dc:Contributor>Natalie Picchetti</dc:Contributor>
		<dc:Date>2011-04-15 11:42:01</dc:Date>
		<dc:Format>text/rdf</dc:Format>
		<dc:Language>en</dc:Language>
		<skos:editorialNote>Generated by testgenall.php on Thu Mar 29 10:24:08 PDT 2012.</skos:editorialNote>
		<skos:historyNote>No previous definition revisions.</skos:historyNote>
		<skos:changeNote>This is the first and only definition provided.</skos:changeNote>
		<skos:scopeNote>http://www.w3.org/2004/02/skos/core#Concept</skos:scopeNote>
		<skos:Note>SKOS properties defined in http://www.w3.org/TR/skos-primer/#secrel</skos:Note>
		<skos:inScheme rdf:resource="http://www.cognitiveatlas.org/tasks/"/>
		<skos:definition>No definition submitted yet.</skos:definition>
		<skos:prefLabel>MacAuthur Communicative Development Inventory</skos:prefLabel>
		<skos:altLabel></skos:altLabel>
</skos:Concept><skos:Concept rdf:about="http://www.cognitiveatlas.org/id/trm_4da891a546d8c"> <dc:identifier>trm_4da891a546d8c</dc:identifier>
		<dc:Title>Cognitive Atlas : Lexicon : Autism Diagnostic Observation Schedule</dc:Title>
		<dc:Description>RDF output for 'Autism Diagnostic Observation Schedule'</dc:Description>
		<dc:Type>InteractiveResource</dc:Type>
		<dc:Publisher>Cognitive Atlas</dc:Publisher>
		<dc:Creator>Cognitive Atlas RDF Generator</dc:Creator>
		<dc:Contributor>Corey White</dc:Contributor>
		<dc:Date>2011-08-15 12:07:37</dc:Date>
		<dc:Format>text/rdf</dc:Format>
		<dc:Language>en</dc:Language>
		<skos:editorialNote>Generated by testgenall.php on Thu Mar 29 10:24:08 PDT 2012.</skos:editorialNote>
		<skos:historyNote>Revision 2: 1 previous definitions.</skos:historyNote>
		<skos:changeNote>See http://www.cognitiveatlas.org/id/trm_4da891a546d8c for complete revision history.</skos:changeNote>
		<skos:scopeNote>http://www.w3.org/2004/02/skos/core#Concept</skos:scopeNote>
		<skos:Note>SKOS properties defined in http://www.w3.org/TR/skos-primer/#secrel</skos:Note>
		<skos:inScheme rdf:resource="http://www.cognitiveatlas.org/tasks/"/>
		<skos:definition>Series of structured and semi-structured tasks that involve social interaction between the examiner and the subject.  Subject is given opportunities to exhibit social and communication behaviors relevant to Austism</skos:definition>
		<skos:prefLabel>Autism Diagnostic Observation Schedule</skos:prefLabel>
		<skos:altLabel></skos:altLabel>
</skos:Concept><skos:Concept rdf:about="http://www.cognitiveatlas.org/id/trm_4da891d43240c"> <dc:identifier>trm_4da891d43240c</dc:identifier>
		<dc:Title>Cognitive Atlas : Lexicon : Modified Erikson Scale of Communication Attitudes</dc:Title>
		<dc:Description>RDF output for 'Modified Erikson Scale of Communication Attitudes'</dc:Description>
		<dc:Type>InteractiveResource</dc:Type>
		<dc:Publisher>Cognitive Atlas</dc:Publisher>
		<dc:Creator>Cognitive Atlas RDF Generator</dc:Creator>
		<dc:Contributor>Natalie Picchetti</dc:Contributor>
		<dc:Date>2011-04-15 11:43:32</dc:Date>
		<dc:Format>text/rdf</dc:Format>
		<dc:Language>en</dc:Language>
		<skos:editorialNote>Generated by testgenall.php on Thu Mar 29 10:24:08 PDT 2012.</skos:editorialNote>
		<skos:historyNote>No previous definition revisions.</skos:historyNote>
		<skos:changeNote>This is the first and only definition provided.</skos:changeNote>
		<skos:scopeNote>http://www.w3.org/2004/02/skos/core#Concept</skos:scopeNote>
		<skos:Note>SKOS properties defined in http://www.w3.org/TR/skos-primer/#secrel</skos:Note>
		<skos:inScheme rdf:resource="http://www.cognitiveatlas.org/tasks/"/>
		<skos:definition>No definition submitted yet.</skos:definition>
		<skos:prefLabel>Modified Erikson Scale of Communication Attitudes</skos:prefLabel>
		<skos:altLabel></skos:altLabel>
</skos:Concept><skos:Concept rdf:about="http://www.cognitiveatlas.org/id/trm_4dadbdd0b2b8c"> <dc:identifier>trm_4dadbdd0b2b8c</dc:identifier>
		<dc:Title>Cognitive Atlas : Lexicon : delayed response task</dc:Title>
		<dc:Description>RDF output for 'delayed response task'</dc:Description>
		<dc:Type>InteractiveResource</dc:Type>
		<dc:Publisher>Cognitive Atlas</dc:Publisher>
		<dc:Creator>Cognitive Atlas RDF Generator</dc:Creator>
		<dc:Contributor>Natalie Picchetti</dc:Contributor>
		<dc:Date>2011-04-19 09:52:32</dc:Date>
		<dc:Format>text/rdf</dc:Format>
		<dc:Language>en</dc:Language>
		<skos:editorialNote>Generated by testgenall.php on Thu Mar 29 10:24:08 PDT 2012.</skos:editorialNote>
		<skos:historyNote>No previous definition revisions.</skos:historyNote>
		<skos:changeNote>This is the first and only definition provided.</skos:changeNote>
		<skos:scopeNote>http://www.w3.org/2004/02/skos/core#Concept</skos:scopeNote>
		<skos:Note>SKOS properties defined in http://www.w3.org/TR/skos-primer/#secrel</skos:Note>
		<skos:inScheme rdf:resource="http://www.cognitiveatlas.org/tasks/"/>
		<skos:definition>No definition submitted yet.</skos:definition>
		<skos:prefLabel>delayed response task</skos:prefLabel>
		<skos:altLabel></skos:altLabel>
		<skos:related rdf:resource="http://www.cognitiveatlas.org/id/trm_4dadbe225bdf1"/>
		<skos:example>spatial delayed response task is descended from delayed response task</skos:example>
</skos:Concept><skos:Concept rdf:about="http://www.cognitiveatlas.org/id/trm_4dadbe225bdf1"> <dc:identifier>trm_4dadbe225bdf1</dc:identifier>
		<dc:Title>Cognitive Atlas : Lexicon : spatial delayed response task</dc:Title>
		<dc:Description>RDF output for 'spatial delayed response task'</dc:Description>
		<dc:Type>InteractiveResource</dc:Type>
		<dc:Publisher>Cognitive Atlas</dc:Publisher>
		<dc:Creator>Cognitive Atlas RDF Generator</dc:Creator>
		<dc:Contributor>Natalie Picchetti</dc:Contributor>
		<dc:Date>2011-04-19 09:53:54</dc:Date>
		<dc:Format>text/rdf</dc:Format>
		<dc:Language>en</dc:Language>
		<skos:editorialNote>Generated by testgenall.php on Thu Mar 29 10:24:08 PDT 2012.</skos:editorialNote>
		<skos:historyNote>No previous definition revisions.</skos:historyNote>
		<skos:changeNote>This is the first and only definition provided.</skos:changeNote>
		<skos:scopeNote>http://www.w3.org/2004/02/skos/core#Concept</skos:scopeNote>
		<skos:Note>SKOS properties defined in http://www.w3.org/TR/skos-primer/#secrel</skos:Note>
		<skos:inScheme rdf:resource="http://www.cognitiveatlas.org/tasks/"/>
		<skos:definition>No definition submitted yet.</skos:definition>
		<skos:prefLabel>spatial delayed response task</skos:prefLabel>
		<skos:altLabel></skos:altLabel>
		<skos:related rdf:resource="http://www.cognitiveatlas.org/id/trm_4dadbdd0b2b8c"/>
		<skos:example>spatial delayed response task is descended from delayed response task</skos:example>
</skos:Concept><skos:Concept rdf:about="http://www.cognitiveatlas.org/id/trm_4dadbfd771a54"> <dc:identifier>trm_4dadbfd771a54</dc:identifier>
		<dc:Title>Cognitive Atlas : Lexicon : Picture-word Stroop task</dc:Title>
		<dc:Description>RDF output for 'Picture-word Stroop task'</dc:Description>
		<dc:Type>InteractiveResource</dc:Type>
		<dc:Publisher>Cognitive Atlas</dc:Publisher>
		<dc:Creator>Cognitive Atlas RDF Generator</dc:Creator>
		<dc:Contributor>Natalie Picchetti</dc:Contributor>
		<dc:Date>2011-04-19 10:01:11</dc:Date>
		<dc:Format>text/rdf</dc:Format>
		<dc:Language>en</dc:Language>
		<skos:editorialNote>Generated by testgenall.php on Thu Mar 29 10:24:08 PDT 2012.</skos:editorialNote>
		<skos:historyNote>No previous definition revisions.</skos:historyNote>
		<skos:changeNote>This is the first and only definition provided.</skos:changeNote>
		<skos:scopeNote>http://www.w3.org/2004/02/skos/core#Concept</skos:scopeNote>
		<skos:Note>SKOS properties defined in http://www.w3.org/TR/skos-primer/#secrel</skos:Note>
		<skos:inScheme rdf:resource="http://www.cognitiveatlas.org/tasks/"/>
		<skos:definition>No definition submitted yet.</skos:definition>
		<skos:prefLabel>Picture-word Stroop task</skos:prefLabel>
		<skos:altLabel></skos:altLabel>
		<skos:related rdf:resource="http://www.cognitiveatlas.org/id/tsk_4a57abb949e27"/>
		<skos:example>Picture-word Stroop task is descended from Stroop task</skos:example>
</skos:Concept><skos:Concept rdf:about="http://www.cognitiveatlas.org/id/trm_4e31d031bc8c2"> <dc:identifier>trm_4e31d031bc8c2</dc:identifier>
		<dc:Title>Cognitive Atlas : Lexicon : synchrony judgment task</dc:Title>
		<dc:Description>RDF output for 'synchrony judgment task'</dc:Description>
		<dc:Type>InteractiveResource</dc:Type>
		<dc:Publisher>Cognitive Atlas</dc:Publisher>
		<dc:Creator>Cognitive Atlas RDF Generator</dc:Creator>
		<dc:Contributor>Scott Love</dc:Contributor>
		<dc:Date>2011-08-04 21:29:05</dc:Date>
		<dc:Format>text/rdf</dc:Format>
		<dc:Language>en</dc:Language>
		<skos:editorialNote>Generated by testgenall.php on Thu Mar 29 10:24:08 PDT 2012.</skos:editorialNote>
		<skos:historyNote>Revision 3: 2 previous definitions.</skos:historyNote>
		<skos:changeNote>See http://www.cognitiveatlas.org/id/trm_4e31d031bc8c2 for complete revision history.</skos:changeNote>
		<skos:scopeNote>http://www.w3.org/2004/02/skos/core#Concept</skos:scopeNote>
		<skos:Note>SKOS properties defined in http://www.w3.org/TR/skos-primer/#secrel</skos:Note>
		<skos:inScheme rdf:resource="http://www.cognitiveatlas.org/tasks/"/>
		<skos:definition>Participants decide whether the unimodal cues to a crossmodal event (stimulus) were in temporal synchrony or not, i.e., whether they were &#34;in synch&#34; or &#34;out of synch&#34;.</skos:definition>
		<skos:prefLabel>synchrony judgment task</skos:prefLabel>
		<skos:altLabel>simultaneity judgment task, SJ</skos:altLabel>
		<skos:related rdf:resource="http://www.cognitiveatlas.org/id/trm_4e31e6dca01ca"/>
		<skos:example>synchrony perception is measured by the contrast of  trials in the synchrony judgment task</skos:example>
		<cito:citesForInformation rdf:resource="http://www.cognitiveatlas.org/citation/id/cit_4e31e2c5aa6c8"/>
		<cito:citesForInformation rdf:resource="http://www.cognitiveatlas.org/citation/id/cit_4e31e2efbbd6e"/>
		<cito:citesForInformation rdf:resource="http://www.cognitiveatlas.org/citation/id/cit_4e31e31c58c7a"/>
		<cito:citesForInformation rdf:resource="http://www.cognitiveatlas.org/citation/id/cit_4e31e33a09ec9"/>
		<cito:citesForInformation rdf:resource="http://www.cognitiveatlas.org/citation/id/cit_4e31e350bd679"/>
		<cito:citesForInformation rdf:resource="http://www.cognitiveatlas.org/citation/id/cit_4e31e37e17ea2"/>
		<cito:citesForInformation rdf:resource="http://www.cognitiveatlas.org/citation/id/cit_4e31e39927db6"/>
		<cito:citesForInformation rdf:resource="http://www.cognitiveatlas.org/citation/id/cit_4e31e3f827cf5"/>
</skos:Concept><skos:Concept rdf:about="http://www.cognitiveatlas.org/id/trm_4e31d69b7f422"> <dc:identifier>trm_4e31d69b7f422</dc:identifier>
		<dc:Title>Cognitive Atlas : Lexicon : temporal order judgment task</dc:Title>
		<dc:Description>RDF output for 'temporal order judgment task'</dc:Description>
		<dc:Type>InteractiveResource</dc:Type>
		<dc:Publisher>Cognitive Atlas</dc:Publisher>
		<dc:Creator>Cognitive Atlas RDF Generator</dc:Creator>
		<dc:Contributor>Scott Love</dc:Contributor>
		<dc:Date>2011-08-04 21:30:50</dc:Date>
		<dc:Format>text/rdf</dc:Format>
		<dc:Language>en</dc:Language>
		<skos:editorialNote>Generated by testgenall.php on Thu Mar 29 10:24:08 PDT 2012.</skos:editorialNote>
		<skos:historyNote>Revision 3: 2 previous definitions.</skos:historyNote>
		<skos:changeNote>See http://www.cognitiveatlas.org/id/trm_4e31d69b7f422 for complete revision history.</skos:changeNote>
		<skos:scopeNote>http://www.w3.org/2004/02/skos/core#Concept</skos:scopeNote>
		<skos:Note>SKOS properties defined in http://www.w3.org/TR/skos-primer/#secrel</skos:Note>
		<skos:inScheme rdf:resource="http://www.cognitiveatlas.org/tasks/"/>
		<skos:definition>Participants decide which of two (or more) unimodal cues (e.g. audio or video) was presented first (or sometimes second) in a crossmodal stimulus. Alternatively, unimodal (auditory, visual or tactile) temporal order judgments generally involve deciding which of two spatial locations was presented first.</skos:definition>
		<skos:prefLabel>temporal order judgment task</skos:prefLabel>
		<skos:altLabel>TOJ</skos:altLabel>
		<skos:related rdf:resource="http://www.cognitiveatlas.org/id/trm_4e31e6dca01ca"/>
		<skos:example>synchrony perception is measured by the contrast of  trials in the temporal order judgment task</skos:example>
		<cito:citesForInformation rdf:resource="http://www.cognitiveatlas.org/citation/id/cit_4e31e04b44751"/>
		<cito:citesForInformation rdf:resource="http://www.cognitiveatlas.org/citation/id/cit_4e31e1d60f9d4"/>
</skos:Concept><skos:Concept rdf:about="http://www.cognitiveatlas.org/id/trm_4e550887d92de"> <dc:identifier>trm_4e550887d92de</dc:identifier>
		<dc:Title>Cognitive Atlas : Lexicon : heat stimulation</dc:Title>
		<dc:Description>RDF output for 'heat stimulation'</dc:Description>
		<dc:Type>InteractiveResource</dc:Type>
		<dc:Publisher>Cognitive Atlas</dc:Publisher>
		<dc:Creator>Cognitive Atlas RDF Generator</dc:Creator>
		<dc:Contributor>Birgit Nierula</dc:Contributor>
		<dc:Date>2011-08-25 10:32:13</dc:Date>
		<dc:Format>text/rdf</dc:Format>
		<dc:Language>en</dc:Language>
		<skos:editorialNote>Generated by testgenall.php on Thu Mar 29 10:24:08 PDT 2012.</skos:editorialNote>
		<skos:historyNote>Revision 3: 2 previous definitions.</skos:historyNote>
		<skos:changeNote>See http://www.cognitiveatlas.org/id/trm_4e550887d92de for complete revision history.</skos:changeNote>
		<skos:scopeNote>http://www.w3.org/2004/02/skos/core#Concept</skos:scopeNote>
		<skos:Note>SKOS properties defined in http://www.w3.org/TR/skos-primer/#secrel</skos:Note>
		<skos:inScheme rdf:resource="http://www.cognitiveatlas.org/tasks/"/>
		<skos:definition>A heat stimulus is applied to the skin and the participant rates the experienced sensation on a visual analogue scale</skos:definition>
		<skos:prefLabel>heat stimulation</skos:prefLabel>
		<skos:altLabel></skos:altLabel>
		<skos:related rdf:resource="http://www.cognitiveatlas.org/id/trm_4b65259eeee34"/>
		<skos:example>pain is measured by the contrast of  trials in the heat stimulation</skos:example>
</skos:Concept><skos:Concept rdf:about="http://www.cognitiveatlas.org/id/trm_4e5662373bc89"> <dc:identifier>trm_4e5662373bc89</dc:identifier>
		<dc:Title>Cognitive Atlas : Lexicon : heat sensitization/adaptation</dc:Title>
		<dc:Description>RDF output for 'heat sensitization/adaptation'</dc:Description>
		<dc:Type>InteractiveResource</dc:Type>
		<dc:Publisher>Cognitive Atlas</dc:Publisher>
		<dc:Creator>Cognitive Atlas RDF Generator</dc:Creator>
		<dc:Contributor>Birgit Nierula</dc:Contributor>
		<dc:Date>2011-09-09 08:59:15</dc:Date>
		<dc:Format>text/rdf</dc:Format>
		<dc:Language>en</dc:Language>
		<skos:editorialNote>Generated by testgenall.php on Thu Mar 29 10:24:08 PDT 2012.</skos:editorialNote>
		<skos:historyNote>Revision 4: 3 previous definitions.</skos:historyNote>
		<skos:changeNote>See http://www.cognitiveatlas.org/id/trm_4e5662373bc89 for complete revision history.</skos:changeNote>
		<skos:scopeNote>http://www.w3.org/2004/02/skos/core#Concept</skos:scopeNote>
		<skos:Note>SKOS properties defined in http://www.w3.org/TR/skos-primer/#secrel</skos:Note>
		<skos:inScheme rdf:resource="http://www.cognitiveatlas.org/tasks/"/>
		<skos:definition>A long (~ 30 seconds or more) heat stimulus is applied to the skin and the participant rates the experienced sensation continuously on a visual analogue scale</skos:definition>
		<skos:prefLabel>heat sensitization/adaptation</skos:prefLabel>
		<skos:altLabel>heat sensibilization / habituation, tonic stimulation model with continuous visual analogue scale</skos:altLabel>
		<skos:related rdf:resource="http://www.cognitiveatlas.org/id/trm_4e6127bd91be9"/>
		<skos:related rdf:resource="http://www.cognitiveatlas.org/id/trm_4e61264db33d4"/>
		<skos:example>pain habituation is measured by the contrast of  trials in the heat sensitization/adaptation</skos:example>
		<skos:example>pain sensitization  is measured by the contrast of  trials in the heat sensitization/adaptation</skos:example>
</skos:Concept><skos:Concept rdf:about="http://www.cognitiveatlas.org/id/trm_4e5bb14d814a8"> <dc:identifier>trm_4e5bb14d814a8</dc:identifier>
		<dc:Title>Cognitive Atlas : Lexicon : Rubber Hand Illusion</dc:Title>
		<dc:Description>RDF output for 'Rubber Hand Illusion'</dc:Description>
		<dc:Type>InteractiveResource</dc:Type>
		<dc:Publisher>Cognitive Atlas</dc:Publisher>
		<dc:Creator>Cognitive Atlas RDF Generator</dc:Creator>
		<dc:Contributor>Birgit Nierula</dc:Contributor>
		<dc:Date>2011-08-29 09:08:56</dc:Date>
		<dc:Format>text/rdf</dc:Format>
		<dc:Language>en</dc:Language>
		<skos:editorialNote>Generated by testgenall.php on Thu Mar 29 10:24:08 PDT 2012.</skos:editorialNote>
		<skos:historyNote>Revision 3: 2 previous definitions.</skos:historyNote>
		<skos:changeNote>See http://www.cognitiveatlas.org/id/trm_4e5bb14d814a8 for complete revision history.</skos:changeNote>
		<skos:scopeNote>http://www.w3.org/2004/02/skos/core#Concept</skos:scopeNote>
		<skos:Note>SKOS properties defined in http://www.w3.org/TR/skos-primer/#secrel</skos:Note>
		<skos:inScheme rdf:resource="http://www.cognitiveatlas.org/tasks/"/>
		<skos:definition>One hand is occluded from sight and an artificial hand is lying in front of the participant. Synchronious paint brush strokes are applied to the same fingers of the occluded hand and the artificial hand. The participant rates the sense of ownership of the artificial hand on the Ownership Illusion Questionnaire or reports the felt position of his or her own hand against a ruler (proprioceptive drift).</skos:definition>
		<skos:prefLabel>Rubber Hand Illusion</skos:prefLabel>
		<skos:altLabel></skos:altLabel>
		<skos:related rdf:resource="http://www.cognitiveatlas.org/id/trm_4e5badf095692"/>
		<skos:related rdf:resource="http://www.cognitiveatlas.org/id/trm_4e5faabfe8ce3"/>
		<skos:example>Sense of ownership is measured by the contrast of  trials in the Rubber Hand Illusion</skos:example>
		<skos:example>Sense of body ownership is measured by the contrast of  trials in the Rubber Hand Illusion</skos:example>
		<cito:citesForInformation rdf:resource="http://www.cognitiveatlas.org/citation/id/cit_4e5bb38a8c240"/>
</skos:Concept><skos:Concept rdf:about="http://www.cognitiveatlas.org/id/trm_4e5d07565b68e"> <dc:identifier>trm_4e5d07565b68e</dc:identifier>
		<dc:Title>Cognitive Atlas : Lexicon : mechanical stimulation</dc:Title>
		<dc:Description>RDF output for 'mechanical stimulation'</dc:Description>
		<dc:Type>InteractiveResource</dc:Type>
		<dc:Publisher>Cognitive Atlas</dc:Publisher>
		<dc:Creator>Cognitive Atlas RDF Generator</dc:Creator>
		<dc:Contributor>Birgit Nierula</dc:Contributor>
		<dc:Date>2011-08-30 08:52:54</dc:Date>
		<dc:Format>text/rdf</dc:Format>
		<dc:Language>en</dc:Language>
		<skos:editorialNote>Generated by testgenall.php on Thu Mar 29 10:24:08 PDT 2012.</skos:editorialNote>
		<skos:historyNote>No previous definition revisions.</skos:historyNote>
		<skos:changeNote>This is the first and only definition provided.</skos:changeNote>
		<skos:scopeNote>http://www.w3.org/2004/02/skos/core#Concept</skos:scopeNote>
		<skos:Note>SKOS properties defined in http://www.w3.org/TR/skos-primer/#secrel</skos:Note>
		<skos:inScheme rdf:resource="http://www.cognitiveatlas.org/tasks/"/>
		<skos:definition>A mechanical stimulus is applied to the skin and the participant rates the experienced sensation on a visual analogue scale.</skos:definition>
		<skos:prefLabel>mechanical stimulation</skos:prefLabel>
		<skos:altLabel>Pin tip stimulation</skos:altLabel>
		<skos:related rdf:resource="http://www.cognitiveatlas.org/id/trm_4b65259eeee34"/>
		<skos:example>pain is measured by the contrast of  trials in the mechanical stimulation</skos:example>
</skos:Concept><skos:Concept rdf:about="http://www.cognitiveatlas.org/id/trm_4e5e7ac84c2e5"> <dc:identifier>trm_4e5e7ac84c2e5</dc:identifier>
		<dc:Title>Cognitive Atlas : Lexicon : Dual Sensitization</dc:Title>
		<dc:Description>RDF output for 'Dual Sensitization'</dc:Description>
		<dc:Type>InteractiveResource</dc:Type>
		<dc:Publisher>Cognitive Atlas</dc:Publisher>
		<dc:Creator>Cognitive Atlas RDF Generator</dc:Creator>
		<dc:Contributor>Birgit Nierula</dc:Contributor>
		<dc:Date>2011-08-31 11:18:48</dc:Date>
		<dc:Format>text/rdf</dc:Format>
		<dc:Language>en</dc:Language>
		<skos:editorialNote>Generated by testgenall.php on Thu Mar 29 10:24:08 PDT 2012.</skos:editorialNote>
		<skos:historyNote>Revision 2: 1 previous definitions.</skos:historyNote>
		<skos:changeNote>See http://www.cognitiveatlas.org/id/trm_4e5e7ac84c2e5 for complete revision history.</skos:changeNote>
		<skos:scopeNote>http://www.w3.org/2004/02/skos/core#Concept</skos:scopeNote>
		<skos:Note>SKOS properties defined in http://www.w3.org/TR/skos-primer/#secrel</skos:Note>
		<skos:inScheme rdf:resource="http://www.cognitiveatlas.org/tasks/"/>
		<skos:definition>Heat stimuli below, at, and above pain threshold (PT; stimulation interval: 30 – 40 seconds) are applied to the skin and the participant gives continuous pain ratings on a visual analogue scale. </skos:definition>
		<skos:prefLabel>Dual Sensitization</skos:prefLabel>
		<skos:altLabel>tonic heat stimulation model</skos:altLabel>
		<skos:related rdf:resource="http://www.cognitiveatlas.org/id/trm_4e61264db33d4"/>
		<skos:related rdf:resource="http://www.cognitiveatlas.org/id/trm_4e6127bd91be9"/>
		<skos:example>pain sensitization  is measured by the contrast of  trials in the Dual Sensitization</skos:example>
		<skos:example>pain habituation is measured by the contrast of  trials in the Dual Sensitization</skos:example>
		<cito:citesForInformation rdf:resource="http://www.cognitiveatlas.org/citation/id/cit_4e5e7d4ac900d"/>
		<cito:citesForInformation rdf:resource="http://www.cognitiveatlas.org/citation/id/cit_4e612a1a9b692"/>
</skos:Concept><skos:Concept rdf:about="http://www.cognitiveatlas.org/id/trm_4e5fcd75efb58"> <dc:identifier>trm_4e5fcd75efb58</dc:identifier>
		<dc:Title>Cognitive Atlas : Lexicon : Thermal Grill Illusion</dc:Title>
		<dc:Description>RDF output for 'Thermal Grill Illusion'</dc:Description>
		<dc:Type>InteractiveResource</dc:Type>
		<dc:Publisher>Cognitive Atlas</dc:Publisher>
		<dc:Creator>Cognitive Atlas RDF Generator</dc:Creator>
		<dc:Contributor>Birgit Nierula</dc:Contributor>
		<dc:Date>2011-09-01 11:22:45</dc:Date>
		<dc:Format>text/rdf</dc:Format>
		<dc:Language>en</dc:Language>
		<skos:editorialNote>Generated by testgenall.php on Thu Mar 29 10:24:08 PDT 2012.</skos:editorialNote>
		<skos:historyNote>No previous definition revisions.</skos:historyNote>
		<skos:changeNote>This is the first and only definition provided.</skos:changeNote>
		<skos:scopeNote>http://www.w3.org/2004/02/skos/core#Concept</skos:scopeNote>
		<skos:Note>SKOS properties defined in http://www.w3.org/TR/skos-primer/#secrel</skos:Note>
		<skos:inScheme rdf:resource="http://www.cognitiveatlas.org/tasks/"/>
		<skos:definition>Innocuous warm and cool bars that are spatially interlaced are applied together to the skin and produce a painful burning sensation. The participant rates the experienced sensation.</skos:definition>
		<skos:prefLabel>Thermal Grill Illusion</skos:prefLabel>
		<skos:altLabel>Thunberg Illusion</skos:altLabel>
		<cito:citesForInformation rdf:resource="http://www.cognitiveatlas.org/citation/id/cit_4e5fd1557357a"/>
		<cito:citesForInformation rdf:resource="http://www.cognitiveatlas.org/citation/id/cit_4e5fd170b348b"/>
</skos:Concept><skos:Concept rdf:about="http://www.cognitiveatlas.org/id/trm_4e6112759926e"> <dc:identifier>trm_4e6112759926e</dc:identifier>
		<dc:Title>Cognitive Atlas : Lexicon : Tonic pain stimulation</dc:Title>
		<dc:Description>RDF output for 'Tonic pain stimulation'</dc:Description>
		<dc:Type>InteractiveResource</dc:Type>
		<dc:Publisher>Cognitive Atlas</dc:Publisher>
		<dc:Creator>Cognitive Atlas RDF Generator</dc:Creator>
		<dc:Contributor>Birgit Nierula</dc:Contributor>
		<dc:Date>2011-09-02 10:29:25</dc:Date>
		<dc:Format>text/rdf</dc:Format>
		<dc:Language>en</dc:Language>
		<skos:editorialNote>Generated by testgenall.php on Thu Mar 29 10:24:08 PDT 2012.</skos:editorialNote>
		<skos:historyNote>No previous definition revisions.</skos:historyNote>
		<skos:changeNote>This is the first and only definition provided.</skos:changeNote>
		<skos:scopeNote>http://www.w3.org/2004/02/skos/core#Concept</skos:scopeNote>
		<skos:Note>SKOS properties defined in http://www.w3.org/TR/skos-primer/#secrel</skos:Note>
		<skos:inScheme rdf:resource="http://www.cognitiveatlas.org/tasks/"/>
		<skos:definition>A long pain stimulus (usually more than 20 seconds) is applied to the skin and the participant gives continuous ratings on a visual analogue scale. Pain can be induced with thermal (hot/cold), electrical, chemical or mechanical stimuli.</skos:definition>
		<skos:prefLabel>Tonic pain stimulation</skos:prefLabel>
		<skos:altLabel></skos:altLabel>
		<skos:related rdf:resource="http://www.cognitiveatlas.org/id/trm_4b65259eeee34"/>
		<skos:example>pain is measured by the contrast of Pain versus No Pain trials in the Tonic pain stimulation</skos:example>
</skos:Concept><skos:Concept rdf:about="http://www.cognitiveatlas.org/id/trm_4e6114e7b1ff2"> <dc:identifier>trm_4e6114e7b1ff2</dc:identifier>
		<dc:Title>Cognitive Atlas : Lexicon : Phasic pain stimulation</dc:Title>
		<dc:Description>RDF output for 'Phasic pain stimulation'</dc:Description>
		<dc:Type>InteractiveResource</dc:Type>
		<dc:Publisher>Cognitive Atlas</dc:Publisher>
		<dc:Creator>Cognitive Atlas RDF Generator</dc:Creator>
		<dc:Contributor>Birgit Nierula</dc:Contributor>
		<dc:Date>2011-09-02 10:39:51</dc:Date>
		<dc:Format>text/rdf</dc:Format>
		<dc:Language>en</dc:Language>
		<skos:editorialNote>Generated by testgenall.php on Thu Mar 29 10:24:08 PDT 2012.</skos:editorialNote>
		<skos:historyNote>No previous definition revisions.</skos:historyNote>
		<skos:changeNote>This is the first and only definition provided.</skos:changeNote>
		<skos:scopeNote>http://www.w3.org/2004/02/skos/core#Concept</skos:scopeNote>
		<skos:Note>SKOS properties defined in http://www.w3.org/TR/skos-primer/#secrel</skos:Note>
		<skos:inScheme rdf:resource="http://www.cognitiveatlas.org/tasks/"/>
		<skos:definition>A short pain stimulus (usually up to 3 seconds) is applied to the skin and the participant rates the stimulus on a visual analogue scale. Pain can be induced with thermal (hot/cold), electrical or mechanical stimuli.</skos:definition>
		<skos:prefLabel>Phasic pain stimulation</skos:prefLabel>
		<skos:altLabel></skos:altLabel>
		<skos:related rdf:resource="http://www.cognitiveatlas.org/id/trm_4b65259eeee34"/>
		<skos:example>pain is measured by the contrast of  trials in the Phasic pain stimulation</skos:example>
</skos:Concept><skos:Concept rdf:about="http://www.cognitiveatlas.org/id/trm_4e664d3718e1b"> <dc:identifier>trm_4e664d3718e1b</dc:identifier>
		<dc:Title>Cognitive Atlas : Lexicon : cold stimulation </dc:Title>
		<dc:Description>RDF output for 'cold stimulation '</dc:Description>
		<dc:Type>InteractiveResource</dc:Type>
		<dc:Publisher>Cognitive Atlas</dc:Publisher>
		<dc:Creator>Cognitive Atlas RDF Generator</dc:Creator>
		<dc:Contributor>Birgit Nierula</dc:Contributor>
		<dc:Date>2011-09-06 09:41:27</dc:Date>
		<dc:Format>text/rdf</dc:Format>
		<dc:Language>en</dc:Language>
		<skos:editorialNote>Generated by testgenall.php on Thu Mar 29 10:24:08 PDT 2012.</skos:editorialNote>
		<skos:historyNote>No previous definition revisions.</skos:historyNote>
		<skos:changeNote>This is the first and only definition provided.</skos:changeNote>
		<skos:scopeNote>http://www.w3.org/2004/02/skos/core#Concept</skos:scopeNote>
		<skos:Note>SKOS properties defined in http://www.w3.org/TR/skos-primer/#secrel</skos:Note>
		<skos:inScheme rdf:resource="http://www.cognitiveatlas.org/tasks/"/>
		<skos:definition>A noxious cold stimulus is applied to the skin and the participant rates the experienced sensation on a visual analogue scale.</skos:definition>
		<skos:prefLabel>cold stimulation </skos:prefLabel>
		<skos:altLabel></skos:altLabel>
</skos:Concept><skos:Concept rdf:about="http://www.cognitiveatlas.org/id/trm_4e68e08950157"> <dc:identifier>trm_4e68e08950157</dc:identifier>
		<dc:Title>Cognitive Atlas : Lexicon : electric stimulation</dc:Title>
		<dc:Description>RDF output for 'electric stimulation'</dc:Description>
		<dc:Type>InteractiveResource</dc:Type>
		<dc:Publisher>Cognitive Atlas</dc:Publisher>
		<dc:Creator>Cognitive Atlas RDF Generator</dc:Creator>
		<dc:Contributor>Birgit Nierula</dc:Contributor>
		<dc:Date>2011-09-08 08:34:33</dc:Date>
		<dc:Format>text/rdf</dc:Format>
		<dc:Language>en</dc:Language>
		<skos:editorialNote>Generated by testgenall.php on Thu Mar 29 10:24:08 PDT 2012.</skos:editorialNote>
		<skos:historyNote>No previous definition revisions.</skos:historyNote>
		<skos:changeNote>This is the first and only definition provided.</skos:changeNote>
		<skos:scopeNote>http://www.w3.org/2004/02/skos/core#Concept</skos:scopeNote>
		<skos:Note>SKOS properties defined in http://www.w3.org/TR/skos-primer/#secrel</skos:Note>
		<skos:inScheme rdf:resource="http://www.cognitiveatlas.org/tasks/"/>
		<skos:definition>An electric stimulus is applied to the skin and the participant rates the perceived pain on a visual analogue scale.</skos:definition>
		<skos:prefLabel>electric stimulation</skos:prefLabel>
		<skos:altLabel></skos:altLabel>
		<skos:related rdf:resource="http://www.cognitiveatlas.org/id/trm_4b65259eeee34"/>
		<skos:example>pain is measured by the contrast of  trials in the electric stimulation</skos:example>
</skos:Concept><skos:Concept rdf:about="http://www.cognitiveatlas.org/id/trm_4e6a2f61b17b0"> <dc:identifier>trm_4e6a2f61b17b0</dc:identifier>
		<dc:Title>Cognitive Atlas : Lexicon : capsaicin-evoked pain</dc:Title>
		<dc:Description>RDF output for 'capsaicin-evoked pain'</dc:Description>
		<dc:Type>InteractiveResource</dc:Type>
		<dc:Publisher>Cognitive Atlas</dc:Publisher>
		<dc:Creator>Cognitive Atlas RDF Generator</dc:Creator>
		<dc:Contributor>Birgit Nierula</dc:Contributor>
		<dc:Date>2011-09-09 08:23:13</dc:Date>
		<dc:Format>text/rdf</dc:Format>
		<dc:Language>en</dc:Language>
		<skos:editorialNote>Generated by testgenall.php on Thu Mar 29 10:24:08 PDT 2012.</skos:editorialNote>
		<skos:historyNote>No previous definition revisions.</skos:historyNote>
		<skos:changeNote>This is the first and only definition provided.</skos:changeNote>
		<skos:scopeNote>http://www.w3.org/2004/02/skos/core#Concept</skos:scopeNote>
		<skos:Note>SKOS properties defined in http://www.w3.org/TR/skos-primer/#secrel</skos:Note>
		<skos:inScheme rdf:resource="http://www.cognitiveatlas.org/tasks/"/>
		<skos:definition>Capsaicin, the active ingredient of chili peppers, is injected intradermally into the skin and participants rate the experienced sensation on a rating scale.</skos:definition>
		<skos:prefLabel>capsaicin-evoked pain</skos:prefLabel>
		<skos:altLabel></skos:altLabel>
		<skos:related rdf:resource="http://www.cognitiveatlas.org/id/trm_4b65259eeee34"/>
		<skos:example>pain is measured by the contrast of  trials in the capsaicin-evoked pain</skos:example>
</skos:Concept><skos:Concept rdf:about="http://www.cognitiveatlas.org/id/trm_4e6a44ee854f8"> <dc:identifier>trm_4e6a44ee854f8</dc:identifier>
		<dc:Title>Cognitive Atlas : Lexicon : Cold Pressor test</dc:Title>
		<dc:Description>RDF output for 'Cold Pressor test'</dc:Description>
		<dc:Type>InteractiveResource</dc:Type>
		<dc:Publisher>Cognitive Atlas</dc:Publisher>
		<dc:Creator>Cognitive Atlas RDF Generator</dc:Creator>
		<dc:Contributor>Birgit Nierula</dc:Contributor>
		<dc:Date>2011-09-09 09:55:10</dc:Date>
		<dc:Format>text/rdf</dc:Format>
		<dc:Language>en</dc:Language>
		<skos:editorialNote>Generated by testgenall.php on Thu Mar 29 10:24:08 PDT 2012.</skos:editorialNote>
		<skos:historyNote>No previous definition revisions.</skos:historyNote>
		<skos:changeNote>This is the first and only definition provided.</skos:changeNote>
		<skos:scopeNote>http://www.w3.org/2004/02/skos/core#Concept</skos:scopeNote>
		<skos:Note>SKOS properties defined in http://www.w3.org/TR/skos-primer/#secrel</skos:Note>
		<skos:inScheme rdf:resource="http://www.cognitiveatlas.org/tasks/"/>
		<skos:definition>The hand or foot is immersed into a bowl of iced water and participants report their sensation from first clear pain to unbearable pain on a scale.</skos:definition>
		<skos:prefLabel>Cold Pressor test</skos:prefLabel>
		<skos:altLabel></skos:altLabel>
		<skos:related rdf:resource="http://www.cognitiveatlas.org/id/trm_4b65259eeee34"/>
		<skos:example>pain is measured by the contrast of  trials in the Cold Pressor test</skos:example>
</skos:Concept><skos:Concept rdf:about="http://www.cognitiveatlas.org/id/trm_4e8a0dd29ec7b"> <dc:identifier>trm_4e8a0dd29ec7b</dc:identifier>
		<dc:Title>Cognitive Atlas : Lexicon : sequential shape matching</dc:Title>
		<dc:Description>RDF output for 'sequential shape matching'</dc:Description>
		<dc:Type>InteractiveResource</dc:Type>
		<dc:Publisher>Cognitive Atlas</dc:Publisher>
		<dc:Creator>Cognitive Atlas RDF Generator</dc:Creator>
		<dc:Contributor>Matt Craddock</dc:Contributor>
		<dc:Date>2011-10-03 12:32:34</dc:Date>
		<dc:Format>text/rdf</dc:Format>
		<dc:Language>en</dc:Language>
		<skos:editorialNote>Generated by testgenall.php on Thu Mar 29 10:24:08 PDT 2012.</skos:editorialNote>
		<skos:historyNote>No previous definition revisions.</skos:historyNote>
		<skos:changeNote>This is the first and only definition provided.</skos:changeNote>
		<skos:scopeNote>http://www.w3.org/2004/02/skos/core#Concept</skos:scopeNote>
		<skos:Note>SKOS properties defined in http://www.w3.org/TR/skos-primer/#secrel</skos:Note>
		<skos:inScheme rdf:resource="http://www.cognitiveatlas.org/tasks/"/>
		<skos:definition>Participants are shown an object for a fixed period. After an interstimulus interval, typically with no intervening object presentations, a second object is presented. The second object is either the same or a different object. Typically, at least one other factor is manipulated. For example, the object may be presented from different viewpoints at each presentation.</skos:definition>
		<skos:prefLabel>sequential shape matching</skos:prefLabel>
		<skos:altLabel></skos:altLabel>
		<skos:related rdf:resource="http://www.cognitiveatlas.org/id/trm_4a3fd79d0aab0"/>
		<skos:example>object recognition is measured by the contrast of  trials in the sequential shape matching</skos:example>
</skos:Concept><skos:Concept rdf:about="http://www.cognitiveatlas.org/id/trm_4e8dd3831f0cc"> <dc:identifier>trm_4e8dd3831f0cc</dc:identifier>
		<dc:Title>Cognitive Atlas : Lexicon : deterministic classification</dc:Title>
		<dc:Description>RDF output for 'deterministic classification'</dc:Description>
		<dc:Type>InteractiveResource</dc:Type>
		<dc:Publisher>Cognitive Atlas</dc:Publisher>
		<dc:Creator>Cognitive Atlas RDF Generator</dc:Creator>
		<dc:Contributor>Natalie Picchetti</dc:Contributor>
		<dc:Date>2011-11-10 15:51:27</dc:Date>
		<dc:Format>text/rdf</dc:Format>
		<dc:Language>en</dc:Language>
		<skos:editorialNote>Generated by testgenall.php on Thu Mar 29 10:24:08 PDT 2012.</skos:editorialNote>
		<skos:historyNote>Revision 3: 2 previous definitions.</skos:historyNote>
		<skos:changeNote>See http://www.cognitiveatlas.org/id/trm_4e8dd3831f0cc for complete revision history.</skos:changeNote>
		<skos:scopeNote>http://www.w3.org/2004/02/skos/core#Concept</skos:scopeNote>
		<skos:Note>SKOS properties defined in http://www.w3.org/TR/skos-primer/#secrel</skos:Note>
		<skos:inScheme rdf:resource="http://www.cognitiveatlas.org/tasks/"/>
		<skos:definition>Is a feedback-driven learning task in which participants classify stimuli into different categories.  A common version of this task is the &#34;weather prediction task.&#34;
</skos:definition>
		<skos:prefLabel>deterministic classification</skos:prefLabel>
		<skos:altLabel></skos:altLabel>
</skos:Concept><skos:Concept rdf:about="http://www.cognitiveatlas.org/id/trm_4e8dd3dfd9fff"> <dc:identifier>trm_4e8dd3dfd9fff</dc:identifier>
		<dc:Title>Cognitive Atlas : Lexicon : mixed event-related probe</dc:Title>
		<dc:Description>RDF output for 'mixed event-related probe'</dc:Description>
		<dc:Type>InteractiveResource</dc:Type>
		<dc:Publisher>Cognitive Atlas</dc:Publisher>
		<dc:Creator>Cognitive Atlas RDF Generator</dc:Creator>
		<dc:Contributor>Natalie Picchetti</dc:Contributor>
		<dc:Date>2011-11-10 16:31:18</dc:Date>
		<dc:Format>text/rdf</dc:Format>
		<dc:Language>en</dc:Language>
		<skos:editorialNote>Generated by testgenall.php on Thu Mar 29 10:24:08 PDT 2012.</skos:editorialNote>
		<skos:historyNote>Revision 2: 1 previous definitions.</skos:historyNote>
		<skos:changeNote>See http://www.cognitiveatlas.org/id/trm_4e8dd3dfd9fff for complete revision history.</skos:changeNote>
		<skos:scopeNote>http://www.w3.org/2004/02/skos/core#Concept</skos:scopeNote>
		<skos:Note>SKOS properties defined in http://www.w3.org/TR/skos-primer/#secrel</skos:Note>
		<skos:inScheme rdf:resource="http://www.cognitiveatlas.org/tasks/"/>
		<skos:definition>When an experimental run consists of blocks of two or more related behavioral tasks.  For example, a mixed event-related probe in a classification learning experiment can consist of alternating blocks of probabilistic classification trials and deterministic classification trials.</skos:definition>
		<skos:prefLabel>mixed event-related probe</skos:prefLabel>
		<skos:altLabel></skos:altLabel>
</skos:Concept><skos:Concept rdf:about="http://www.cognitiveatlas.org/id/trm_4eb1f3a8ec119"> <dc:identifier>trm_4eb1f3a8ec119</dc:identifier>
		<dc:Title>Cognitive Atlas : Lexicon : Intermodal Preferential Looking Paradigm</dc:Title>
		<dc:Description>RDF output for 'Intermodal Preferential Looking Paradigm'</dc:Description>
		<dc:Type>InteractiveResource</dc:Type>
		<dc:Publisher>Cognitive Atlas</dc:Publisher>
		<dc:Creator>Cognitive Atlas RDF Generator</dc:Creator>
		<dc:Contributor>Antonio Franco</dc:Contributor>
		<dc:Date>2011-11-02 18:51:37</dc:Date>
		<dc:Format>text/rdf</dc:Format>
		<dc:Language>en</dc:Language>
		<skos:editorialNote>Generated by testgenall.php on Thu Mar 29 10:24:08 PDT 2012.</skos:editorialNote>
		<skos:historyNote>No previous definition revisions.</skos:historyNote>
		<skos:changeNote>This is the first and only definition provided.</skos:changeNote>
		<skos:scopeNote>http://www.w3.org/2004/02/skos/core#Concept</skos:scopeNote>
		<skos:Note>SKOS properties defined in http://www.w3.org/TR/skos-primer/#secrel</skos:Note>
		<skos:inScheme rdf:resource="http://www.cognitiveatlas.org/tasks/"/>
		<skos:definition>A paradigm to test infant&#39;s comprehension about linguistic stimuli. The infants are exposed to two visual stimuli at the same time they hear an auditory stimulus corresponding to only one of the seen images . Looking time is the measure to know whether they associate the word to the right image.</skos:definition>
		<skos:prefLabel>Intermodal Preferential Looking Paradigm</skos:prefLabel>
		<skos:altLabel>IPL, IPLP</skos:altLabel>
		<skos:related rdf:resource="http://www.cognitiveatlas.org/id/trm_4a3fd79d0a775"/>
		<skos:example>language comprehension is measured by the contrast of  trials in the Intermodal Preferential Looking Paradigm</skos:example>
		<cito:citesForInformation rdf:resource="http://www.cognitiveatlas.org/citation/id/cit_4eb329d245a86"/>
		<cito:citesForInformation rdf:resource="http://www.cognitiveatlas.org/citation/id/cit_4eb32b17210fb"/>
</skos:Concept><skos:Concept rdf:about="http://www.cognitiveatlas.org/id/trm_4ebc6a6b75ebf"> <dc:identifier>trm_4ebc6a6b75ebf</dc:identifier>
		<dc:Title>Cognitive Atlas : Lexicon : tone counting</dc:Title>
		<dc:Description>RDF output for 'tone counting'</dc:Description>
		<dc:Type>InteractiveResource</dc:Type>
		<dc:Publisher>Cognitive Atlas</dc:Publisher>
		<dc:Creator>Cognitive Atlas RDF Generator</dc:Creator>
		<dc:Contributor>Natalie Picchetti</dc:Contributor>
		<dc:Date>2011-11-11 06:39:09</dc:Date>
		<dc:Format>text/rdf</dc:Format>
		<dc:Language>en</dc:Language>
		<skos:editorialNote>Generated by testgenall.php on Thu Mar 29 10:24:08 PDT 2012.</skos:editorialNote>
		<skos:historyNote>Revision 2: 1 previous definitions.</skos:historyNote>
		<skos:changeNote>See http://www.cognitiveatlas.org/id/trm_4ebc6a6b75ebf for complete revision history.</skos:changeNote>
		<skos:scopeNote>http://www.w3.org/2004/02/skos/core#Concept</skos:scopeNote>
		<skos:Note>SKOS properties defined in http://www.w3.org/TR/skos-primer/#secrel</skos:Note>
		<skos:inScheme rdf:resource="http://www.cognitiveatlas.org/tasks/"/>
		<skos:definition>A task in which a participant needs to count and remember the number of specific tones presented in an experimental run.</skos:definition>
		<skos:prefLabel>tone counting</skos:prefLabel>
		<skos:altLabel>tone-counting</skos:altLabel>
</skos:Concept><skos:Concept rdf:about="http://www.cognitiveatlas.org/id/trm_4ebc728326a13"> <dc:identifier>trm_4ebc728326a13</dc:identifier>
		<dc:Title>Cognitive Atlas : Lexicon : single-task weather prediction </dc:Title>
		<dc:Description>RDF output for 'single-task weather prediction '</dc:Description>
		<dc:Type>InteractiveResource</dc:Type>
		<dc:Publisher>Cognitive Atlas</dc:Publisher>
		<dc:Creator>Cognitive Atlas RDF Generator</dc:Creator>
		<dc:Contributor>Natalie Picchetti</dc:Contributor>
		<dc:Date>2011-11-10 17:11:06</dc:Date>
		<dc:Format>text/rdf</dc:Format>
		<dc:Language>en</dc:Language>
		<skos:editorialNote>Generated by testgenall.php on Thu Mar 29 10:24:08 PDT 2012.</skos:editorialNote>
		<skos:historyNote>Revision 2: 1 previous definitions.</skos:historyNote>
		<skos:changeNote>See http://www.cognitiveatlas.org/id/trm_4ebc728326a13 for complete revision history.</skos:changeNote>
		<skos:scopeNote>http://www.w3.org/2004/02/skos/core#Concept</skos:scopeNote>
		<skos:Note>SKOS properties defined in http://www.w3.org/TR/skos-primer/#secrel</skos:Note>
		<skos:inScheme rdf:resource="http://www.cognitiveatlas.org/tasks/"/>
		<skos:definition>is a feedback driven classification learning task in which a subject is presented with a stimuli (ex-geometric shapes) and has to classify them into one of two categories (ex-rainy or sunny weather), and then receives feedback on if the response was correct or incorrect.  This may or may not be presented with other stimuli (ex-tones of different frequencies), but the goal of the task is to only pay attention the the classification task at hand. 
</skos:definition>
		<skos:prefLabel>single-task weather prediction </skos:prefLabel>
		<skos:altLabel>single task weather prediction </skos:altLabel>
</skos:Concept><skos:Concept rdf:about="http://www.cognitiveatlas.org/id/trm_4ebc98cc77e7b"> <dc:identifier>trm_4ebc98cc77e7b</dc:identifier>
		<dc:Title>Cognitive Atlas : Lexicon : dual-task weather prediction</dc:Title>
		<dc:Description>RDF output for 'dual-task weather prediction'</dc:Description>
		<dc:Type>InteractiveResource</dc:Type>
		<dc:Publisher>Cognitive Atlas</dc:Publisher>
		<dc:Creator>Cognitive Atlas RDF Generator</dc:Creator>
		<dc:Contributor>Natalie Picchetti</dc:Contributor>
		<dc:Date>2011-11-10 20:52:40</dc:Date>
		<dc:Format>text/rdf</dc:Format>
		<dc:Language>en</dc:Language>
		<skos:editorialNote>Generated by testgenall.php on Thu Mar 29 10:24:08 PDT 2012.</skos:editorialNote>
		<skos:historyNote>Revision 2: 1 previous definitions.</skos:historyNote>
		<skos:changeNote>See http://www.cognitiveatlas.org/id/trm_4ebc98cc77e7b for complete revision history.</skos:changeNote>
		<skos:scopeNote>http://www.w3.org/2004/02/skos/core#Concept</skos:scopeNote>
		<skos:Note>SKOS properties defined in http://www.w3.org/TR/skos-primer/#secrel</skos:Note>
		<skos:inScheme rdf:resource="http://www.cognitiveatlas.org/tasks/"/>
		<skos:definition>A task in which a subject must attend and respond to two different tasks contained in one experimental run; one task is a feedback driven classification learning task in which a subject is presented with a stimuli (ex-geometric shapes) and has to classify them into one of two categories (ex-rainy or sunny weather), and then receives feedback on whether the response was correct or incorrect.  The other task requires the subject to listen to different tones and count the number of a specific tone.</skos:definition>
		<skos:prefLabel>dual-task weather prediction</skos:prefLabel>
		<skos:altLabel>dual task weather prediction</skos:altLabel>
</skos:Concept><skos:Concept rdf:about="http://www.cognitiveatlas.org/id/trm_4ebc9d2e397f2"> <dc:identifier>trm_4ebc9d2e397f2</dc:identifier>
		<dc:Title>Cognitive Atlas : Lexicon : classification probe without feedback</dc:Title>
		<dc:Description>RDF output for 'classification probe without feedback'</dc:Description>
		<dc:Type>InteractiveResource</dc:Type>
		<dc:Publisher>Cognitive Atlas</dc:Publisher>
		<dc:Creator>Cognitive Atlas RDF Generator</dc:Creator>
		<dc:Contributor>Natalie Picchetti</dc:Contributor>
		<dc:Date>2011-11-10 19:57:34</dc:Date>
		<dc:Format>text/rdf</dc:Format>
		<dc:Language>en</dc:Language>
		<skos:editorialNote>Generated by testgenall.php on Thu Mar 29 10:24:08 PDT 2012.</skos:editorialNote>
		<skos:historyNote>No previous definition revisions.</skos:historyNote>
		<skos:changeNote>This is the first and only definition provided.</skos:changeNote>
		<skos:scopeNote>http://www.w3.org/2004/02/skos/core#Concept</skos:scopeNote>
		<skos:Note>SKOS properties defined in http://www.w3.org/TR/skos-primer/#secrel</skos:Note>
		<skos:inScheme rdf:resource="http://www.cognitiveatlas.org/tasks/"/>
		<skos:definition>is preformed after receiving training in the classification learning task.  It is similar to the classification learning task but in this task the subject does not receive feedback.</skos:definition>
		<skos:prefLabel>classification probe without feedback</skos:prefLabel>
		<skos:altLabel></skos:altLabel>
</skos:Concept><skos:Concept rdf:about="http://www.cognitiveatlas.org/id/trm_4ebd44cd88360"> <dc:identifier>trm_4ebd44cd88360</dc:identifier>
		<dc:Title>Cognitive Atlas : Lexicon : Abstract/concrete judgment: Bilingual</dc:Title>
		<dc:Description>RDF output for 'Abstract/concrete judgment: Bilingual'</dc:Description>
		<dc:Type>InteractiveResource</dc:Type>
		<dc:Publisher>Cognitive Atlas</dc:Publisher>
		<dc:Creator>Cognitive Atlas RDF Generator</dc:Creator>
		<dc:Contributor>Russ Poldrack</dc:Contributor>
		<dc:Date>2011-11-11 07:52:45</dc:Date>
		<dc:Format>text/rdf</dc:Format>
		<dc:Language>en</dc:Language>
		<skos:editorialNote>Generated by testgenall.php on Thu Mar 29 10:24:08 PDT 2012.</skos:editorialNote>
		<skos:historyNote>No previous definition revisions.</skos:historyNote>
		<skos:changeNote>This is the first and only definition provided.</skos:changeNote>
		<skos:scopeNote>http://www.w3.org/2004/02/skos/core#Concept</skos:scopeNote>
		<skos:Note>SKOS properties defined in http://www.w3.org/TR/skos-primer/#secrel</skos:Note>
		<skos:inScheme rdf:resource="http://www.cognitiveatlas.org/tasks/"/>
		<skos:definition>Task in which subjects are presented with words that are either abstract or concrete nouns, and decide for each term whether it is abstract or concrete.</skos:definition>
		<skos:prefLabel>Abstract/concrete judgment: Bilingual</skos:prefLabel>
		<skos:altLabel></skos:altLabel>
		<skos:related rdf:resource="http://www.cognitiveatlas.org/id/trm_4f24126c22011"/>
		<skos:example>Abstract/concrete judgment: Bilingual is descended from abstract/concrete task</skos:example>
</skos:Concept><skos:Concept rdf:about="http://www.cognitiveatlas.org/id/trm_4ebd477ab5a11"> <dc:identifier>trm_4ebd477ab5a11</dc:identifier>
		<dc:Title>Cognitive Atlas : Lexicon : object n-back</dc:Title>
		<dc:Description>RDF output for 'object n-back'</dc:Description>
		<dc:Type>InteractiveResource</dc:Type>
		<dc:Publisher>Cognitive Atlas</dc:Publisher>
		<dc:Creator>Cognitive Atlas RDF Generator</dc:Creator>
		<dc:Contributor>Russ Poldrack</dc:Contributor>
		<dc:Date>2011-11-11 08:04:10</dc:Date>
		<dc:Format>text/rdf</dc:Format>
		<dc:Language>en</dc:Language>
		<skos:editorialNote>Generated by testgenall.php on Thu Mar 29 10:24:08 PDT 2012.</skos:editorialNote>
		<skos:historyNote>No previous definition revisions.</skos:historyNote>
		<skos:changeNote>This is the first and only definition provided.</skos:changeNote>
		<skos:scopeNote>http://www.w3.org/2004/02/skos/core#Concept</skos:scopeNote>
		<skos:Note>SKOS properties defined in http://www.w3.org/TR/skos-primer/#secrel</skos:Note>
		<skos:inScheme rdf:resource="http://www.cognitiveatlas.org/tasks/"/>
		<skos:definition>An n-back task in which the stimuli are images of visual objects.</skos:definition>
		<skos:prefLabel>object n-back</skos:prefLabel>
		<skos:altLabel></skos:altLabel>
</skos:Concept><skos:Concept rdf:about="http://www.cognitiveatlas.org/id/trm_4ebd47b8bab6b"> <dc:identifier>trm_4ebd47b8bab6b</dc:identifier>
		<dc:Title>Cognitive Atlas : Lexicon : object one-back task</dc:Title>
		<dc:Description>RDF output for 'object one-back task'</dc:Description>
		<dc:Type>InteractiveResource</dc:Type>
		<dc:Publisher>Cognitive Atlas</dc:Publisher>
		<dc:Creator>Cognitive Atlas RDF Generator</dc:Creator>
		<dc:Contributor>Russ Poldrack</dc:Contributor>
		<dc:Date>2011-11-11 08:05:12</dc:Date>
		<dc:Format>text/rdf</dc:Format>
		<dc:Language>en</dc:Language>
		<skos:editorialNote>Generated by testgenall.php on Thu Mar 29 10:24:08 PDT 2012.</skos:editorialNote>
		<skos:historyNote>No previous definition revisions.</skos:historyNote>
		<skos:changeNote>This is the first and only definition provided.</skos:changeNote>
		<skos:scopeNote>http://www.w3.org/2004/02/skos/core#Concept</skos:scopeNote>
		<skos:Note>SKOS properties defined in http://www.w3.org/TR/skos-primer/#secrel</skos:Note>
		<skos:inScheme rdf:resource="http://www.cognitiveatlas.org/tasks/"/>
		<skos:definition>A one-back task in which the stimuli are images of visual objects</skos:definition>
		<skos:prefLabel>object one-back task</skos:prefLabel>
		<skos:altLabel></skos:altLabel>
</skos:Concept><skos:Concept rdf:about="http://www.cognitiveatlas.org/id/trm_4ebd482eba5b1"> <dc:identifier>trm_4ebd482eba5b1</dc:identifier>
		<dc:Title>Cognitive Atlas : Lexicon : word one-back task</dc:Title>
		<dc:Description>RDF output for 'word one-back task'</dc:Description>
		<dc:Type>InteractiveResource</dc:Type>
		<dc:Publisher>Cognitive Atlas</dc:Publisher>
		<dc:Creator>Cognitive Atlas RDF Generator</dc:Creator>
		<dc:Contributor>Russ Poldrack</dc:Contributor>
		<dc:Date>2011-11-11 08:07:10</dc:Date>
		<dc:Format>text/rdf</dc:Format>
		<dc:Language>en</dc:Language>
		<skos:editorialNote>Generated by testgenall.php on Thu Mar 29 10:24:08 PDT 2012.</skos:editorialNote>
		<skos:historyNote>No previous definition revisions.</skos:historyNote>
		<skos:changeNote>This is the first and only definition provided.</skos:changeNote>
		<skos:scopeNote>http://www.w3.org/2004/02/skos/core#Concept</skos:scopeNote>
		<skos:Note>SKOS properties defined in http://www.w3.org/TR/skos-primer/#secrel</skos:Note>
		<skos:inScheme rdf:resource="http://www.cognitiveatlas.org/tasks/"/>
		<skos:definition>A one-back task on which subjects are presented with words or word-like stimuli</skos:definition>
		<skos:prefLabel>word one-back task</skos:prefLabel>
		<skos:altLabel></skos:altLabel>
</skos:Concept><skos:Concept rdf:about="http://www.cognitiveatlas.org/id/trm_4f23fc8c42d28"> <dc:identifier>trm_4f23fc8c42d28</dc:identifier>
		<dc:Title>Cognitive Atlas : Lexicon : Monetary incentive delay task</dc:Title>
		<dc:Description>RDF output for 'Monetary incentive delay task'</dc:Description>
		<dc:Type>InteractiveResource</dc:Type>
		<dc:Publisher>Cognitive Atlas</dc:Publisher>
		<dc:Creator>Cognitive Atlas RDF Generator</dc:Creator>
		<dc:Contributor>Russ Poldrack</dc:Contributor>
		<dc:Date>2012-01-28 08:09:00</dc:Date>
		<dc:Format>text/rdf</dc:Format>
		<dc:Language>en</dc:Language>
		<skos:editorialNote>Generated by testgenall.php on Thu Mar 29 10:24:08 PDT 2012.</skos:editorialNote>
		<skos:historyNote>Revision 2: 1 previous definitions.</skos:historyNote>
		<skos:changeNote>See http://www.cognitiveatlas.org/id/trm_4f23fc8c42d28 for complete revision history.</skos:changeNote>
		<skos:scopeNote>http://www.w3.org/2004/02/skos/core#Concept</skos:scopeNote>
		<skos:Note>SKOS properties defined in http://www.w3.org/TR/skos-primer/#secrel</skos:Note>
		<skos:inScheme rdf:resource="http://www.cognitiveatlas.org/tasks/"/>
		<skos:definition>Task in which subject makes a response within a time window and is potentially rewarded for the response depending on their reaction time.</skos:definition>
		<skos:prefLabel>Monetary incentive delay task</skos:prefLabel>
		<skos:altLabel>MID, monetary incentive delay (mid) task</skos:altLabel>
</skos:Concept><skos:Concept rdf:about="http://www.cognitiveatlas.org/id/trm_4f240cb09f8e5"> <dc:identifier>trm_4f240cb09f8e5</dc:identifier>
		<dc:Title>Cognitive Atlas : Lexicon : semantic decision task</dc:Title>
		<dc:Description>RDF output for 'semantic decision task'</dc:Description>
		<dc:Type>InteractiveResource</dc:Type>
		<dc:Publisher>Cognitive Atlas</dc:Publisher>
		<dc:Creator>Cognitive Atlas RDF Generator</dc:Creator>
		<dc:Contributor>Russ Poldrack</dc:Contributor>
		<dc:Date>2012-01-28 06:56:48</dc:Date>
		<dc:Format>text/rdf</dc:Format>
		<dc:Language>en</dc:Language>
		<skos:editorialNote>Generated by testgenall.php on Thu Mar 29 10:24:08 PDT 2012.</skos:editorialNote>
		<skos:historyNote>No previous definition revisions.</skos:historyNote>
		<skos:changeNote>This is the first and only definition provided.</skos:changeNote>
		<skos:scopeNote>http://www.w3.org/2004/02/skos/core#Concept</skos:scopeNote>
		<skos:Note>SKOS properties defined in http://www.w3.org/TR/skos-primer/#secrel</skos:Note>
		<skos:inScheme rdf:resource="http://www.cognitiveatlas.org/tasks/"/>
		<skos:definition>A task in which a subject makes a decision about the meaning of a stimulus.</skos:definition>
		<skos:prefLabel>semantic decision task</skos:prefLabel>
		<skos:altLabel></skos:altLabel>
</skos:Concept><skos:Concept rdf:about="http://www.cognitiveatlas.org/id/trm_4f240d346320c"> <dc:identifier>trm_4f240d346320c</dc:identifier>
		<dc:Title>Cognitive Atlas : Lexicon : covert naming task</dc:Title>
		<dc:Description>RDF output for 'covert naming task'</dc:Description>
		<dc:Type>InteractiveResource</dc:Type>
		<dc:Publisher>Cognitive Atlas</dc:Publisher>
		<dc:Creator>Cognitive Atlas RDF Generator</dc:Creator>
		<dc:Contributor>Russ Poldrack</dc:Contributor>
		<dc:Date>2012-01-28 07:29:50</dc:Date>
		<dc:Format>text/rdf</dc:Format>
		<dc:Language>en</dc:Language>
		<skos:editorialNote>Generated by testgenall.php on Thu Mar 29 10:24:08 PDT 2012.</skos:editorialNote>
		<skos:historyNote>Revision 2: 1 previous definitions.</skos:historyNote>
		<skos:changeNote>See http://www.cognitiveatlas.org/id/trm_4f240d346320c for complete revision history.</skos:changeNote>
		<skos:scopeNote>http://www.w3.org/2004/02/skos/core#Concept</skos:scopeNote>
		<skos:Note>SKOS properties defined in http://www.w3.org/TR/skos-primer/#secrel</skos:Note>
		<skos:inScheme rdf:resource="http://www.cognitiveatlas.org/tasks/"/>
		<skos:definition>A task in which subjects name a stimulus silently</skos:definition>
		<skos:prefLabel>covert naming task</skos:prefLabel>
		<skos:altLabel>covert production task</skos:altLabel>
</skos:Concept><skos:Concept rdf:about="http://www.cognitiveatlas.org/id/trm_4f240d7664628"> <dc:identifier>trm_4f240d7664628</dc:identifier>
		<dc:Title>Cognitive Atlas : Lexicon : semantic relatedness task</dc:Title>
		<dc:Description>RDF output for 'semantic relatedness task'</dc:Description>
		<dc:Type>InteractiveResource</dc:Type>
		<dc:Publisher>Cognitive Atlas</dc:Publisher>
		<dc:Creator>Cognitive Atlas RDF Generator</dc:Creator>
		<dc:Contributor>Russ Poldrack</dc:Contributor>
		<dc:Date>2012-01-28 07:00:06</dc:Date>
		<dc:Format>text/rdf</dc:Format>
		<dc:Language>en</dc:Language>
		<skos:editorialNote>Generated by testgenall.php on Thu Mar 29 10:24:08 PDT 2012.</skos:editorialNote>
		<skos:historyNote>No previous definition revisions.</skos:historyNote>
		<skos:changeNote>This is the first and only definition provided.</skos:changeNote>
		<skos:scopeNote>http://www.w3.org/2004/02/skos/core#Concept</skos:scopeNote>
		<skos:Note>SKOS properties defined in http://www.w3.org/TR/skos-primer/#secrel</skos:Note>
		<skos:inScheme rdf:resource="http://www.cognitiveatlas.org/tasks/"/>
		<skos:definition>A task in which subjects judge whether a set of stimuli are related by meaning.</skos:definition>
		<skos:prefLabel>semantic relatedness task</skos:prefLabel>
		<skos:altLabel></skos:altLabel>
</skos:Concept><skos:Concept rdf:about="http://www.cognitiveatlas.org/id/trm_4f240e7f989f8"> <dc:identifier>trm_4f240e7f989f8</dc:identifier>
		<dc:Title>Cognitive Atlas : Lexicon : auditory temporal discrimination task</dc:Title>
		<dc:Description>RDF output for 'auditory temporal discrimination task'</dc:Description>
		<dc:Type>InteractiveResource</dc:Type>
		<dc:Publisher>Cognitive Atlas</dc:Publisher>
		<dc:Creator>Cognitive Atlas RDF Generator</dc:Creator>
		<dc:Contributor>Russ Poldrack</dc:Contributor>
		<dc:Date>2012-01-28 07:04:31</dc:Date>
		<dc:Format>text/rdf</dc:Format>
		<dc:Language>en</dc:Language>
		<skos:editorialNote>Generated by testgenall.php on Thu Mar 29 10:24:08 PDT 2012.</skos:editorialNote>
		<skos:historyNote>No previous definition revisions.</skos:historyNote>
		<skos:changeNote>This is the first and only definition provided.</skos:changeNote>
		<skos:scopeNote>http://www.w3.org/2004/02/skos/core#Concept</skos:scopeNote>
		<skos:Note>SKOS properties defined in http://www.w3.org/TR/skos-primer/#secrel</skos:Note>
		<skos:inScheme rdf:resource="http://www.cognitiveatlas.org/tasks/"/>
		<skos:definition>A task in which the subject discriminates auditory stimuli based on temporal characteristics.</skos:definition>
		<skos:prefLabel>auditory temporal discrimination task</skos:prefLabel>
		<skos:altLabel></skos:altLabel>
</skos:Concept><skos:Concept rdf:about="http://www.cognitiveatlas.org/id/trm_4f240edf92865"> <dc:identifier>trm_4f240edf92865</dc:identifier>
		<dc:Title>Cognitive Atlas : Lexicon : Mental imagery task</dc:Title>
		<dc:Description>RDF output for 'Mental imagery task'</dc:Description>
		<dc:Type>InteractiveResource</dc:Type>
		<dc:Publisher>Cognitive Atlas</dc:Publisher>
		<dc:Creator>Cognitive Atlas RDF Generator</dc:Creator>
		<dc:Contributor>Russ Poldrack</dc:Contributor>
		<dc:Date>2012-01-28 07:06:07</dc:Date>
		<dc:Format>text/rdf</dc:Format>
		<dc:Language>en</dc:Language>
		<skos:editorialNote>Generated by testgenall.php on Thu Mar 29 10:24:08 PDT 2012.</skos:editorialNote>
		<skos:historyNote>No previous definition revisions.</skos:historyNote>
		<skos:changeNote>This is the first and only definition provided.</skos:changeNote>
		<skos:scopeNote>http://www.w3.org/2004/02/skos/core#Concept</skos:scopeNote>
		<skos:Note>SKOS properties defined in http://www.w3.org/TR/skos-primer/#secrel</skos:Note>
		<skos:inScheme rdf:resource="http://www.cognitiveatlas.org/tasks/"/>
		<skos:definition>A task in which subjects create mental images</skos:definition>
		<skos:prefLabel>Mental imagery task</skos:prefLabel>
		<skos:altLabel>imagery task</skos:altLabel>
</skos:Concept><skos:Concept rdf:about="http://www.cognitiveatlas.org/id/trm_4f240f1c740da"> <dc:identifier>trm_4f240f1c740da</dc:identifier>
		<dc:Title>Cognitive Atlas : Lexicon : verbal fluency task</dc:Title>
		<dc:Description>RDF output for 'verbal fluency task'</dc:Description>
		<dc:Type>InteractiveResource</dc:Type>
		<dc:Publisher>Cognitive Atlas</dc:Publisher>
		<dc:Creator>Cognitive Atlas RDF Generator</dc:Creator>
		<dc:Contributor>Russ Poldrack</dc:Contributor>
		<dc:Date>2012-01-28 07:07:08</dc:Date>
		<dc:Format>text/rdf</dc:Format>
		<dc:Language>en</dc:Language>
		<skos:editorialNote>Generated by testgenall.php on Thu Mar 29 10:24:08 PDT 2012.</skos:editorialNote>
		<skos:historyNote>No previous definition revisions.</skos:historyNote>
		<skos:changeNote>This is the first and only definition provided.</skos:changeNote>
		<skos:scopeNote>http://www.w3.org/2004/02/skos/core#Concept</skos:scopeNote>
		<skos:Note>SKOS properties defined in http://www.w3.org/TR/skos-primer/#secrel</skos:Note>
		<skos:inScheme rdf:resource="http://www.cognitiveatlas.org/tasks/"/>
		<skos:definition>A test of the ability to verbally produce words.</skos:definition>
		<skos:prefLabel>verbal fluency task</skos:prefLabel>
		<skos:altLabel></skos:altLabel>
</skos:Concept><skos:Concept rdf:about="http://www.cognitiveatlas.org/id/trm_4f240fbdf1601"> <dc:identifier>trm_4f240fbdf1601</dc:identifier>
		<dc:Title>Cognitive Atlas : Lexicon : word comprehension task</dc:Title>
		<dc:Description>RDF output for 'word comprehension task'</dc:Description>
		<dc:Type>InteractiveResource</dc:Type>
		<dc:Publisher>Cognitive Atlas</dc:Publisher>
		<dc:Creator>Cognitive Atlas RDF Generator</dc:Creator>
		<dc:Contributor>Russ Poldrack</dc:Contributor>
		<dc:Date>2012-01-28 07:09:49</dc:Date>
		<dc:Format>text/rdf</dc:Format>
		<dc:Language>en</dc:Language>
		<skos:editorialNote>Generated by testgenall.php on Thu Mar 29 10:24:08 PDT 2012.</skos:editorialNote>
		<skos:historyNote>No previous definition revisions.</skos:historyNote>
		<skos:changeNote>This is the first and only definition provided.</skos:changeNote>
		<skos:scopeNote>http://www.w3.org/2004/02/skos/core#Concept</skos:scopeNote>
		<skos:Note>SKOS properties defined in http://www.w3.org/TR/skos-primer/#secrel</skos:Note>
		<skos:inScheme rdf:resource="http://www.cognitiveatlas.org/tasks/"/>
		<skos:definition>A task that measures the comprehension of word meaning.</skos:definition>
		<skos:prefLabel>word comprehension task</skos:prefLabel>
		<skos:altLabel></skos:altLabel>
</skos:Concept><skos:Concept rdf:about="http://www.cognitiveatlas.org/id/trm_4f241001dfcee"> <dc:identifier>trm_4f241001dfcee</dc:identifier>
		<dc:Title>Cognitive Atlas : Lexicon : Letter case judgment task</dc:Title>
		<dc:Description>RDF output for 'Letter case judgment task'</dc:Description>
		<dc:Type>InteractiveResource</dc:Type>
		<dc:Publisher>Cognitive Atlas</dc:Publisher>
		<dc:Creator>Cognitive Atlas RDF Generator</dc:Creator>
		<dc:Contributor>Russ Poldrack</dc:Contributor>
		<dc:Date>2012-01-28 07:10:57</dc:Date>
		<dc:Format>text/rdf</dc:Format>
		<dc:Language>en</dc:Language>
		<skos:editorialNote>Generated by testgenall.php on Thu Mar 29 10:24:08 PDT 2012.</skos:editorialNote>
		<skos:historyNote>No previous definition revisions.</skos:historyNote>
		<skos:changeNote>This is the first and only definition provided.</skos:changeNote>
		<skos:scopeNote>http://www.w3.org/2004/02/skos/core#Concept</skos:scopeNote>
		<skos:Note>SKOS properties defined in http://www.w3.org/TR/skos-primer/#secrel</skos:Note>
		<skos:inScheme rdf:resource="http://www.cognitiveatlas.org/tasks/"/>
		<skos:definition>A task in which the subject decides whether letters are uppercase or lowercase.</skos:definition>
		<skos:prefLabel>Letter case judgment task</skos:prefLabel>
		<skos:altLabel>case judgment task</skos:altLabel>
</skos:Concept><skos:Concept rdf:about="http://www.cognitiveatlas.org/id/trm_4f24108555294"> <dc:identifier>trm_4f24108555294</dc:identifier>
		<dc:Title>Cognitive Atlas : Lexicon : visually guided saccade task</dc:Title>
		<dc:Description>RDF output for 'visually guided saccade task'</dc:Description>
		<dc:Type>InteractiveResource</dc:Type>
		<dc:Publisher>Cognitive Atlas</dc:Publisher>
		<dc:Creator>Cognitive Atlas RDF Generator</dc:Creator>
		<dc:Contributor>Russ Poldrack</dc:Contributor>
		<dc:Date>2012-01-28 07:13:09</dc:Date>
		<dc:Format>text/rdf</dc:Format>
		<dc:Language>en</dc:Language>
		<skos:editorialNote>Generated by testgenall.php on Thu Mar 29 10:24:08 PDT 2012.</skos:editorialNote>
		<skos:historyNote>No previous definition revisions.</skos:historyNote>
		<skos:changeNote>This is the first and only definition provided.</skos:changeNote>
		<skos:scopeNote>http://www.w3.org/2004/02/skos/core#Concept</skos:scopeNote>
		<skos:Note>SKOS properties defined in http://www.w3.org/TR/skos-primer/#secrel</skos:Note>
		<skos:inScheme rdf:resource="http://www.cognitiveatlas.org/tasks/"/>
		<skos:definition>A task in which subjects make visually guided eye movements.</skos:definition>
		<skos:prefLabel>visually guided saccade task</skos:prefLabel>
		<skos:altLabel></skos:altLabel>
</skos:Concept><skos:Concept rdf:about="http://www.cognitiveatlas.org/id/trm_4f24112057e90"> <dc:identifier>trm_4f24112057e90</dc:identifier>
		<dc:Title>Cognitive Atlas : Lexicon : categorization task</dc:Title>
		<dc:Description>RDF output for 'categorization task'</dc:Description>
		<dc:Type>InteractiveResource</dc:Type>
		<dc:Publisher>Cognitive Atlas</dc:Publisher>
		<dc:Creator>Cognitive Atlas RDF Generator</dc:Creator>
		<dc:Contributor>Russ Poldrack</dc:Contributor>
		<dc:Date>2012-01-28 07:15:44</dc:Date>
		<dc:Format>text/rdf</dc:Format>
		<dc:Language>en</dc:Language>
		<skos:editorialNote>Generated by testgenall.php on Thu Mar 29 10:24:08 PDT 2012.</skos:editorialNote>
		<skos:historyNote>No previous definition revisions.</skos:historyNote>
		<skos:changeNote>This is the first and only definition provided.</skos:changeNote>
		<skos:scopeNote>http://www.w3.org/2004/02/skos/core#Concept</skos:scopeNote>
		<skos:Note>SKOS properties defined in http://www.w3.org/TR/skos-primer/#secrel</skos:Note>
		<skos:inScheme rdf:resource="http://www.cognitiveatlas.org/tasks/"/>
		<skos:definition>Task in which a subject classifies stimuli into one of a set of categories</skos:definition>
		<skos:prefLabel>categorization task</skos:prefLabel>
		<skos:altLabel></skos:altLabel>
</skos:Concept><skos:Concept rdf:about="http://www.cognitiveatlas.org/id/trm_4f241173868a3"> <dc:identifier>trm_4f241173868a3</dc:identifier>
		<dc:Title>Cognitive Atlas : Lexicon : navigation task</dc:Title>
		<dc:Description>RDF output for 'navigation task'</dc:Description>
		<dc:Type>InteractiveResource</dc:Type>
		<dc:Publisher>Cognitive Atlas</dc:Publisher>
		<dc:Creator>Cognitive Atlas RDF Generator</dc:Creator>
		<dc:Contributor>Russ Poldrack</dc:Contributor>
		<dc:Date>2012-01-28 07:17:07</dc:Date>
		<dc:Format>text/rdf</dc:Format>
		<dc:Language>en</dc:Language>
		<skos:editorialNote>Generated by testgenall.php on Thu Mar 29 10:24:08 PDT 2012.</skos:editorialNote>
		<skos:historyNote>No previous definition revisions.</skos:historyNote>
		<skos:changeNote>This is the first and only definition provided.</skos:changeNote>
		<skos:scopeNote>http://www.w3.org/2004/02/skos/core#Concept</skos:scopeNote>
		<skos:Note>SKOS properties defined in http://www.w3.org/TR/skos-primer/#secrel</skos:Note>
		<skos:inScheme rdf:resource="http://www.cognitiveatlas.org/tasks/"/>
		<skos:definition>A task in which the subject navigates a spatial layout.</skos:definition>
		<skos:prefLabel>navigation task</skos:prefLabel>
		<skos:altLabel></skos:altLabel>
</skos:Concept><skos:Concept rdf:about="http://www.cognitiveatlas.org/id/trm_4f2411c91ae5e"> <dc:identifier>trm_4f2411c91ae5e</dc:identifier>
		<dc:Title>Cognitive Atlas : Lexicon : recall test</dc:Title>
		<dc:Description>RDF output for 'recall test'</dc:Description>
		<dc:Type>InteractiveResource</dc:Type>
		<dc:Publisher>Cognitive Atlas</dc:Publisher>
		<dc:Creator>Cognitive Atlas RDF Generator</dc:Creator>
		<dc:Contributor>Russ Poldrack</dc:Contributor>
		<dc:Date>2012-01-28 07:18:33</dc:Date>
		<dc:Format>text/rdf</dc:Format>
		<dc:Language>en</dc:Language>
		<skos:editorialNote>Generated by testgenall.php on Thu Mar 29 10:24:08 PDT 2012.</skos:editorialNote>
		<skos:historyNote>No previous definition revisions.</skos:historyNote>
		<skos:changeNote>This is the first and only definition provided.</skos:changeNote>
		<skos:scopeNote>http://www.w3.org/2004/02/skos/core#Concept</skos:scopeNote>
		<skos:Note>SKOS properties defined in http://www.w3.org/TR/skos-primer/#secrel</skos:Note>
		<skos:inScheme rdf:resource="http://www.cognitiveatlas.org/tasks/"/>
		<skos:definition>A test in which the subject is asked to produce a list of previously studied items.</skos:definition>
		<skos:prefLabel>recall test</skos:prefLabel>
		<skos:altLabel></skos:altLabel>
</skos:Concept><skos:Concept rdf:about="http://www.cognitiveatlas.org/id/trm_4f24126c22011"> <dc:identifier>trm_4f24126c22011</dc:identifier>
		<dc:Title>Cognitive Atlas : Lexicon : abstract/concrete task</dc:Title>
		<dc:Description>RDF output for 'abstract/concrete task'</dc:Description>
		<dc:Type>InteractiveResource</dc:Type>
		<dc:Publisher>Cognitive Atlas</dc:Publisher>
		<dc:Creator>Cognitive Atlas RDF Generator</dc:Creator>
		<dc:Contributor>Russ Poldrack</dc:Contributor>
		<dc:Date>2012-01-28 07:21:16</dc:Date>
		<dc:Format>text/rdf</dc:Format>
		<dc:Language>en</dc:Language>
		<skos:editorialNote>Generated by testgenall.php on Thu Mar 29 10:24:08 PDT 2012.</skos:editorialNote>
		<skos:historyNote>No previous definition revisions.</skos:historyNote>
		<skos:changeNote>This is the first and only definition provided.</skos:changeNote>
		<skos:scopeNote>http://www.w3.org/2004/02/skos/core#Concept</skos:scopeNote>
		<skos:Note>SKOS properties defined in http://www.w3.org/TR/skos-primer/#secrel</skos:Note>
		<skos:inScheme rdf:resource="http://www.cognitiveatlas.org/tasks/"/>
		<skos:definition>A task in which subjects decide whether words are abstract or concrete.</skos:definition>
		<skos:prefLabel>abstract/concrete task</skos:prefLabel>
		<skos:altLabel>abstract/concrete judgment</skos:altLabel>
		<skos:related rdf:resource="http://www.cognitiveatlas.org/id/trm_4ebd44cd88360"/>
		<skos:example>Abstract/concrete judgment: Bilingual is descended from abstract/concrete task</skos:example>
</skos:Concept><skos:Concept rdf:about="http://www.cognitiveatlas.org/id/trm_4f2412d4c3b88"> <dc:identifier>trm_4f2412d4c3b88</dc:identifier>
		<dc:Title>Cognitive Atlas : Lexicon : semantic classification task</dc:Title>
		<dc:Description>RDF output for 'semantic classification task'</dc:Description>
		<dc:Type>InteractiveResource</dc:Type>
		<dc:Publisher>Cognitive Atlas</dc:Publisher>
		<dc:Creator>Cognitive Atlas RDF Generator</dc:Creator>
		<dc:Contributor>Russ Poldrack</dc:Contributor>
		<dc:Date>2012-01-28 07:23:00</dc:Date>
		<dc:Format>text/rdf</dc:Format>
		<dc:Language>en</dc:Language>
		<skos:editorialNote>Generated by testgenall.php on Thu Mar 29 10:24:08 PDT 2012.</skos:editorialNote>
		<skos:historyNote>No previous definition revisions.</skos:historyNote>
		<skos:changeNote>This is the first and only definition provided.</skos:changeNote>
		<skos:scopeNote>http://www.w3.org/2004/02/skos/core#Concept</skos:scopeNote>
		<skos:Note>SKOS properties defined in http://www.w3.org/TR/skos-primer/#secrel</skos:Note>
		<skos:inScheme rdf:resource="http://www.cognitiveatlas.org/tasks/"/>
		<skos:definition>A task in which the subject classifies stimuli based on meaning</skos:definition>
		<skos:prefLabel>semantic classification task</skos:prefLabel>
		<skos:altLabel>semantic categorization task</skos:altLabel>
</skos:Concept><skos:Concept rdf:about="http://www.cognitiveatlas.org/id/trm_4f241325579c6"> <dc:identifier>trm_4f241325579c6</dc:identifier>
		<dc:Title>Cognitive Atlas : Lexicon : problem solving task</dc:Title>
		<dc:Description>RDF output for 'problem solving task'</dc:Description>
		<dc:Type>InteractiveResource</dc:Type>
		<dc:Publisher>Cognitive Atlas</dc:Publisher>
		<dc:Creator>Cognitive Atlas RDF Generator</dc:Creator>
		<dc:Contributor>Russ Poldrack</dc:Contributor>
		<dc:Date>2012-01-28 07:24:21</dc:Date>
		<dc:Format>text/rdf</dc:Format>
		<dc:Language>en</dc:Language>
		<skos:editorialNote>Generated by testgenall.php on Thu Mar 29 10:24:08 PDT 2012.</skos:editorialNote>
		<skos:historyNote>No previous definition revisions.</skos:historyNote>
		<skos:changeNote>This is the first and only definition provided.</skos:changeNote>
		<skos:scopeNote>http://www.w3.org/2004/02/skos/core#Concept</skos:scopeNote>
		<skos:Note>SKOS properties defined in http://www.w3.org/TR/skos-primer/#secrel</skos:Note>
		<skos:inScheme rdf:resource="http://www.cognitiveatlas.org/tasks/"/>
		<skos:definition>A task in which subjects must solve a conceptual problem.</skos:definition>
		<skos:prefLabel>problem solving task</skos:prefLabel>
		<skos:altLabel></skos:altLabel>
</skos:Concept><skos:Concept rdf:about="http://www.cognitiveatlas.org/id/trm_4f24135453d65"> <dc:identifier>trm_4f24135453d65</dc:identifier>
		<dc:Title>Cognitive Atlas : Lexicon : spelling task</dc:Title>
		<dc:Description>RDF output for 'spelling task'</dc:Description>
		<dc:Type>InteractiveResource</dc:Type>
		<dc:Publisher>Cognitive Atlas</dc:Publisher>
		<dc:Creator>Cognitive Atlas RDF Generator</dc:Creator>
		<dc:Contributor>Russ Poldrack</dc:Contributor>
		<dc:Date>2012-01-28 07:25:08</dc:Date>
		<dc:Format>text/rdf</dc:Format>
		<dc:Language>en</dc:Language>
		<skos:editorialNote>Generated by testgenall.php on Thu Mar 29 10:24:08 PDT 2012.</skos:editorialNote>
		<skos:historyNote>No previous definition revisions.</skos:historyNote>
		<skos:changeNote>This is the first and only definition provided.</skos:changeNote>
		<skos:scopeNote>http://www.w3.org/2004/02/skos/core#Concept</skos:scopeNote>
		<skos:Note>SKOS properties defined in http://www.w3.org/TR/skos-primer/#secrel</skos:Note>
		<skos:inScheme rdf:resource="http://www.cognitiveatlas.org/tasks/"/>
		<skos:definition>A task in which subjects are asked to spell words.</skos:definition>
		<skos:prefLabel>spelling task</skos:prefLabel>
		<skos:altLabel></skos:altLabel>
</skos:Concept><skos:Concept rdf:about="http://www.cognitiveatlas.org/id/trm_4f2414059baa8"> <dc:identifier>trm_4f2414059baa8</dc:identifier>
		<dc:Title>Cognitive Atlas : Lexicon : Instrumental learning task</dc:Title>
		<dc:Description>RDF output for 'Instrumental learning task'</dc:Description>
		<dc:Type>InteractiveResource</dc:Type>
		<dc:Publisher>Cognitive Atlas</dc:Publisher>
		<dc:Creator>Cognitive Atlas RDF Generator</dc:Creator>
		<dc:Contributor>Russ Poldrack</dc:Contributor>
		<dc:Date>2012-01-28 07:28:05</dc:Date>
		<dc:Format>text/rdf</dc:Format>
		<dc:Language>en</dc:Language>
		<skos:editorialNote>Generated by testgenall.php on Thu Mar 29 10:24:08 PDT 2012.</skos:editorialNote>
		<skos:historyNote>No previous definition revisions.</skos:historyNote>
		<skos:changeNote>This is the first and only definition provided.</skos:changeNote>
		<skos:scopeNote>http://www.w3.org/2004/02/skos/core#Concept</skos:scopeNote>
		<skos:Note>SKOS properties defined in http://www.w3.org/TR/skos-primer/#secrel</skos:Note>
		<skos:inScheme rdf:resource="http://www.cognitiveatlas.org/tasks/"/>
		<skos:definition>A task in which a subject learns to respond through rewards.</skos:definition>
		<skos:prefLabel>Instrumental learning task</skos:prefLabel>
		<skos:altLabel>instrumental conditioning task</skos:altLabel>
</skos:Concept><skos:Concept rdf:about="http://www.cognitiveatlas.org/id/trm_4f2414a1bab77"> <dc:identifier>trm_4f2414a1bab77</dc:identifier>
		<dc:Title>Cognitive Atlas : Lexicon : phonetic discrimination task</dc:Title>
		<dc:Description>RDF output for 'phonetic discrimination task'</dc:Description>
		<dc:Type>InteractiveResource</dc:Type>
		<dc:Publisher>Cognitive Atlas</dc:Publisher>
		<dc:Creator>Cognitive Atlas RDF Generator</dc:Creator>
		<dc:Contributor>Russ Poldrack</dc:Contributor>
		<dc:Date>2012-01-28 07:30:41</dc:Date>
		<dc:Format>text/rdf</dc:Format>
		<dc:Language>en</dc:Language>
		<skos:editorialNote>Generated by testgenall.php on Thu Mar 29 10:24:08 PDT 2012.</skos:editorialNote>
		<skos:historyNote>No previous definition revisions.</skos:historyNote>
		<skos:changeNote>This is the first and only definition provided.</skos:changeNote>
		<skos:scopeNote>http://www.w3.org/2004/02/skos/core#Concept</skos:scopeNote>
		<skos:Note>SKOS properties defined in http://www.w3.org/TR/skos-primer/#secrel</skos:Note>
		<skos:inScheme rdf:resource="http://www.cognitiveatlas.org/tasks/"/>
		<skos:definition>A task in which the subject discriminates stimuli based on phonetic features.</skos:definition>
		<skos:prefLabel>phonetic discrimination task</skos:prefLabel>
		<skos:altLabel></skos:altLabel>
</skos:Concept><skos:Concept rdf:about="http://www.cognitiveatlas.org/id/trm_4f24154867d84"> <dc:identifier>trm_4f24154867d84</dc:identifier>
		<dc:Title>Cognitive Atlas : Lexicon : logical reasoning task</dc:Title>
		<dc:Description>RDF output for 'logical reasoning task'</dc:Description>
		<dc:Type>InteractiveResource</dc:Type>
		<dc:Publisher>Cognitive Atlas</dc:Publisher>
		<dc:Creator>Cognitive Atlas RDF Generator</dc:Creator>
		<dc:Contributor>Russ Poldrack</dc:Contributor>
		<dc:Date>2012-01-28 07:33:28</dc:Date>
		<dc:Format>text/rdf</dc:Format>
		<dc:Language>en</dc:Language>
		<skos:editorialNote>Generated by testgenall.php on Thu Mar 29 10:24:08 PDT 2012.</skos:editorialNote>
		<skos:historyNote>No previous definition revisions.</skos:historyNote>
		<skos:changeNote>This is the first and only definition provided.</skos:changeNote>
		<skos:scopeNote>http://www.w3.org/2004/02/skos/core#Concept</skos:scopeNote>
		<skos:Note>SKOS properties defined in http://www.w3.org/TR/skos-primer/#secrel</skos:Note>
		<skos:inScheme rdf:resource="http://www.cognitiveatlas.org/tasks/"/>
		<skos:definition>A task that requires the use of logical reasoning.</skos:definition>
		<skos:prefLabel>logical reasoning task</skos:prefLabel>
		<skos:altLabel></skos:altLabel>
</skos:Concept><skos:Concept rdf:about="http://www.cognitiveatlas.org/id/trm_4f241614d4a25"> <dc:identifier>trm_4f241614d4a25</dc:identifier>
		<dc:Title>Cognitive Atlas : Lexicon : switch task</dc:Title>
		<dc:Description>RDF output for 'switch task'</dc:Description>
		<dc:Type>InteractiveResource</dc:Type>
		<dc:Publisher>Cognitive Atlas</dc:Publisher>
		<dc:Creator>Cognitive Atlas RDF Generator</dc:Creator>
		<dc:Contributor>Russ Poldrack</dc:Contributor>
		<dc:Date>2012-01-28 07:36:52</dc:Date>
		<dc:Format>text/rdf</dc:Format>
		<dc:Language>en</dc:Language>
		<skos:editorialNote>Generated by testgenall.php on Thu Mar 29 10:24:08 PDT 2012.</skos:editorialNote>
		<skos:historyNote>No previous definition revisions.</skos:historyNote>
		<skos:changeNote>This is the first and only definition provided.</skos:changeNote>
		<skos:scopeNote>http://www.w3.org/2004/02/skos/core#Concept</skos:scopeNote>
		<skos:Note>SKOS properties defined in http://www.w3.org/TR/skos-primer/#secrel</skos:Note>
		<skos:inScheme rdf:resource="http://www.cognitiveatlas.org/tasks/"/>
		<skos:definition>A paradigm requiring subjects to switch between performing multiple different individual tasks.</skos:definition>
		<skos:prefLabel>switch task</skos:prefLabel>
		<skos:altLabel>switching task</skos:altLabel>
</skos:Concept><skos:Concept rdf:about="http://www.cognitiveatlas.org/id/trm_4f24179122380"> <dc:identifier>trm_4f24179122380</dc:identifier>
		<dc:Title>Cognitive Atlas : Lexicon : mental arithmetic task</dc:Title>
		<dc:Description>RDF output for 'mental arithmetic task'</dc:Description>
		<dc:Type>InteractiveResource</dc:Type>
		<dc:Publisher>Cognitive Atlas</dc:Publisher>
		<dc:Creator>Cognitive Atlas RDF Generator</dc:Creator>
		<dc:Contributor>Russ Poldrack</dc:Contributor>
		<dc:Date>2012-01-28 07:43:13</dc:Date>
		<dc:Format>text/rdf</dc:Format>
		<dc:Language>en</dc:Language>
		<skos:editorialNote>Generated by testgenall.php on Thu Mar 29 10:24:08 PDT 2012.</skos:editorialNote>
		<skos:historyNote>No previous definition revisions.</skos:historyNote>
		<skos:changeNote>This is the first and only definition provided.</skos:changeNote>
		<skos:scopeNote>http://www.w3.org/2004/02/skos/core#Concept</skos:scopeNote>
		<skos:Note>SKOS properties defined in http://www.w3.org/TR/skos-primer/#secrel</skos:Note>
		<skos:inScheme rdf:resource="http://www.cognitiveatlas.org/tasks/"/>
		<skos:definition>A task  in which the subject performs arithmetic computations without an external means of recording their work.</skos:definition>
		<skos:prefLabel>mental arithmetic task</skos:prefLabel>
		<skos:altLabel></skos:altLabel>
</skos:Concept><skos:Concept rdf:about="http://www.cognitiveatlas.org/id/trm_4f2417d4a63ae"> <dc:identifier>trm_4f2417d4a63ae</dc:identifier>
		<dc:Title>Cognitive Atlas : Lexicon : random number generation task</dc:Title>
		<dc:Description>RDF output for 'random number generation task'</dc:Description>
		<dc:Type>InteractiveResource</dc:Type>
		<dc:Publisher>Cognitive Atlas</dc:Publisher>
		<dc:Creator>Cognitive Atlas RDF Generator</dc:Creator>
		<dc:Contributor>Russ Poldrack</dc:Contributor>
		<dc:Date>2012-01-28 07:44:20</dc:Date>
		<dc:Format>text/rdf</dc:Format>
		<dc:Language>en</dc:Language>
		<skos:editorialNote>Generated by testgenall.php on Thu Mar 29 10:24:08 PDT 2012.</skos:editorialNote>
		<skos:historyNote>No previous definition revisions.</skos:historyNote>
		<skos:changeNote>This is the first and only definition provided.</skos:changeNote>
		<skos:scopeNote>http://www.w3.org/2004/02/skos/core#Concept</skos:scopeNote>
		<skos:Note>SKOS properties defined in http://www.w3.org/TR/skos-primer/#secrel</skos:Note>
		<skos:inScheme rdf:resource="http://www.cognitiveatlas.org/tasks/"/>
		<skos:definition>A task in which the subject generates a series of random numbers.</skos:definition>
		<skos:prefLabel>random number generation task</skos:prefLabel>
		<skos:altLabel></skos:altLabel>
</skos:Concept><skos:Concept rdf:about="http://www.cognitiveatlas.org/id/trm_4f24183fe80c6"> <dc:identifier>trm_4f24183fe80c6</dc:identifier>
		<dc:Title>Cognitive Atlas : Lexicon : verb generation task</dc:Title>
		<dc:Description>RDF output for 'verb generation task'</dc:Description>
		<dc:Type>InteractiveResource</dc:Type>
		<dc:Publisher>Cognitive Atlas</dc:Publisher>
		<dc:Creator>Cognitive Atlas RDF Generator</dc:Creator>
		<dc:Contributor>Russ Poldrack</dc:Contributor>
		<dc:Date>2012-01-28 07:46:07</dc:Date>
		<dc:Format>text/rdf</dc:Format>
		<dc:Language>en</dc:Language>
		<skos:editorialNote>Generated by testgenall.php on Thu Mar 29 10:24:08 PDT 2012.</skos:editorialNote>
		<skos:historyNote>No previous definition revisions.</skos:historyNote>
		<skos:changeNote>This is the first and only definition provided.</skos:changeNote>
		<skos:scopeNote>http://www.w3.org/2004/02/skos/core#Concept</skos:scopeNote>
		<skos:Note>SKOS properties defined in http://www.w3.org/TR/skos-primer/#secrel</skos:Note>
		<skos:inScheme rdf:resource="http://www.cognitiveatlas.org/tasks/"/>
		<skos:definition>A task in which subjects are presented with nouns and generate an associated verb.</skos:definition>
		<skos:prefLabel>verb generation task</skos:prefLabel>
		<skos:altLabel></skos:altLabel>
</skos:Concept><skos:Concept rdf:about="http://www.cognitiveatlas.org/id/trm_4f24189031a4a"> <dc:identifier>trm_4f24189031a4a</dc:identifier>
		<dc:Title>Cognitive Atlas : Lexicon : Cyberball task</dc:Title>
		<dc:Description>RDF output for 'Cyberball task'</dc:Description>
		<dc:Type>InteractiveResource</dc:Type>
		<dc:Publisher>Cognitive Atlas</dc:Publisher>
		<dc:Creator>Cognitive Atlas RDF Generator</dc:Creator>
		<dc:Contributor>Russ Poldrack</dc:Contributor>
		<dc:Date>2012-01-28 07:47:57</dc:Date>
		<dc:Format>text/rdf</dc:Format>
		<dc:Language>en</dc:Language>
		<skos:editorialNote>Generated by testgenall.php on Thu Mar 29 10:24:08 PDT 2012.</skos:editorialNote>
		<skos:historyNote>Revision 2: 1 previous definitions.</skos:historyNote>
		<skos:changeNote>See http://www.cognitiveatlas.org/id/trm_4f24189031a4a for complete revision history.</skos:changeNote>
		<skos:scopeNote>http://www.w3.org/2004/02/skos/core#Concept</skos:scopeNote>
		<skos:Note>SKOS properties defined in http://www.w3.org/TR/skos-primer/#secrel</skos:Note>
		<skos:inScheme rdf:resource="http://www.cognitiveatlas.org/tasks/"/>
		<skos:definition>A task in which subjects view a set of balls interacting in game.  At some point one of the balls is excluded from the game, simulating social exclusion.</skos:definition>
		<skos:prefLabel>Cyberball task</skos:prefLabel>
		<skos:altLabel>cyberball social exclusion task</skos:altLabel>
</skos:Concept><skos:Concept rdf:about="http://www.cognitiveatlas.org/id/trm_4f24194bce29f"> <dc:identifier>trm_4f24194bce29f</dc:identifier>
		<dc:Title>Cognitive Atlas : Lexicon : conjunction search task</dc:Title>
		<dc:Description>RDF output for 'conjunction search task'</dc:Description>
		<dc:Type>InteractiveResource</dc:Type>
		<dc:Publisher>Cognitive Atlas</dc:Publisher>
		<dc:Creator>Cognitive Atlas RDF Generator</dc:Creator>
		<dc:Contributor>Russ Poldrack</dc:Contributor>
		<dc:Date>2012-01-28 07:50:35</dc:Date>
		<dc:Format>text/rdf</dc:Format>
		<dc:Language>en</dc:Language>
		<skos:editorialNote>Generated by testgenall.php on Thu Mar 29 10:24:08 PDT 2012.</skos:editorialNote>
		<skos:historyNote>No previous definition revisions.</skos:historyNote>
		<skos:changeNote>This is the first and only definition provided.</skos:changeNote>
		<skos:scopeNote>http://www.w3.org/2004/02/skos/core#Concept</skos:scopeNote>
		<skos:Note>SKOS properties defined in http://www.w3.org/TR/skos-primer/#secrel</skos:Note>
		<skos:inScheme rdf:resource="http://www.cognitiveatlas.org/tasks/"/>
		<skos:definition>A task that requires the subject to search for a stimulus defined by a combination of visual features.</skos:definition>
		<skos:prefLabel>conjunction search task</skos:prefLabel>
		<skos:altLabel></skos:altLabel>
</skos:Concept><skos:Concept rdf:about="http://www.cognitiveatlas.org/id/trm_4f2419c4a1646"> <dc:identifier>trm_4f2419c4a1646</dc:identifier>
		<dc:Title>Cognitive Atlas : Lexicon : Multisource interference task</dc:Title>
		<dc:Description>RDF output for 'Multisource interference task'</dc:Description>
		<dc:Type>InteractiveResource</dc:Type>
		<dc:Publisher>Cognitive Atlas</dc:Publisher>
		<dc:Creator>Cognitive Atlas RDF Generator</dc:Creator>
		<dc:Contributor>Russ Poldrack</dc:Contributor>
		<dc:Date>2012-01-28 07:52:36</dc:Date>
		<dc:Format>text/rdf</dc:Format>
		<dc:Language>en</dc:Language>
		<skos:editorialNote>Generated by testgenall.php on Thu Mar 29 10:24:08 PDT 2012.</skos:editorialNote>
		<skos:historyNote>No previous definition revisions.</skos:historyNote>
		<skos:changeNote>This is the first and only definition provided.</skos:changeNote>
		<skos:scopeNote>http://www.w3.org/2004/02/skos/core#Concept</skos:scopeNote>
		<skos:Note>SKOS properties defined in http://www.w3.org/TR/skos-primer/#secrel</skos:Note>
		<skos:inScheme rdf:resource="http://www.cognitiveatlas.org/tasks/"/>
		<skos:definition>A task in which the subject must resolve multiple sources of interference.</skos:definition>
		<skos:prefLabel>Multisource interference task</skos:prefLabel>
		<skos:altLabel>MSIT</skos:altLabel>
</skos:Concept><skos:Concept rdf:about="http://www.cognitiveatlas.org/id/trm_4f241ab50513b"> <dc:identifier>trm_4f241ab50513b</dc:identifier>
		<dc:Title>Cognitive Atlas : Lexicon : mentalizing task</dc:Title>
		<dc:Description>RDF output for 'mentalizing task'</dc:Description>
		<dc:Type>InteractiveResource</dc:Type>
		<dc:Publisher>Cognitive Atlas</dc:Publisher>
		<dc:Creator>Cognitive Atlas RDF Generator</dc:Creator>
		<dc:Contributor>Russ Poldrack</dc:Contributor>
		<dc:Date>2012-01-28 07:56:37</dc:Date>
		<dc:Format>text/rdf</dc:Format>
		<dc:Language>en</dc:Language>
		<skos:editorialNote>Generated by testgenall.php on Thu Mar 29 10:24:08 PDT 2012.</skos:editorialNote>
		<skos:historyNote>No previous definition revisions.</skos:historyNote>
		<skos:changeNote>This is the first and only definition provided.</skos:changeNote>
		<skos:scopeNote>http://www.w3.org/2004/02/skos/core#Concept</skos:scopeNote>
		<skos:Note>SKOS properties defined in http://www.w3.org/TR/skos-primer/#secrel</skos:Note>
		<skos:inScheme rdf:resource="http://www.cognitiveatlas.org/tasks/"/>
		<skos:prefLabel>mentalizing task</skos:prefLabel>
		<skos:altLabel></skos:altLabel>
</skos:Concept><skos:Concept rdf:about="http://www.cognitiveatlas.org/id/trm_4f241b50caaf7"> <dc:identifier>trm_4f241b50caaf7</dc:identifier>
		<dc:Title>Cognitive Atlas : Lexicon : semantic task</dc:Title>
		<dc:Description>RDF output for 'semantic task'</dc:Description>
		<dc:Type>InteractiveResource</dc:Type>
		<dc:Publisher>Cognitive Atlas</dc:Publisher>
		<dc:Creator>Cognitive Atlas RDF Generator</dc:Creator>
		<dc:Contributor>Russ Poldrack</dc:Contributor>
		<dc:Date>2012-01-28 07:59:12</dc:Date>
		<dc:Format>text/rdf</dc:Format>
		<dc:Language>en</dc:Language>
		<skos:editorialNote>Generated by testgenall.php on Thu Mar 29 10:24:08 PDT 2012.</skos:editorialNote>
		<skos:historyNote>No previous definition revisions.</skos:historyNote>
		<skos:changeNote>This is the first and only definition provided.</skos:changeNote>
		<skos:scopeNote>http://www.w3.org/2004/02/skos/core#Concept</skos:scopeNote>
		<skos:Note>SKOS properties defined in http://www.w3.org/TR/skos-primer/#secrel</skos:Note>
		<skos:inScheme rdf:resource="http://www.cognitiveatlas.org/tasks/"/>
		<skos:definition>Any task that requires subjects to process the meaning of stimuli</skos:definition>
		<skos:prefLabel>semantic task</skos:prefLabel>
		<skos:altLabel></skos:altLabel>
</skos:Concept><skos:Concept rdf:about="http://www.cognitiveatlas.org/id/trm_4f241b751c5a0"> <dc:identifier>trm_4f241b751c5a0</dc:identifier>
		<dc:Title>Cognitive Atlas : Lexicon : phonological task</dc:Title>
		<dc:Description>RDF output for 'phonological task'</dc:Description>
		<dc:Type>InteractiveResource</dc:Type>
		<dc:Publisher>Cognitive Atlas</dc:Publisher>
		<dc:Creator>Cognitive Atlas RDF Generator</dc:Creator>
		<dc:Contributor>Russ Poldrack</dc:Contributor>
		<dc:Date>2012-01-28 07:59:49</dc:Date>
		<dc:Format>text/rdf</dc:Format>
		<dc:Language>en</dc:Language>
		<skos:editorialNote>Generated by testgenall.php on Thu Mar 29 10:24:08 PDT 2012.</skos:editorialNote>
		<skos:historyNote>No previous definition revisions.</skos:historyNote>
		<skos:changeNote>This is the first and only definition provided.</skos:changeNote>
		<skos:scopeNote>http://www.w3.org/2004/02/skos/core#Concept</skos:scopeNote>
		<skos:Note>SKOS properties defined in http://www.w3.org/TR/skos-primer/#secrel</skos:Note>
		<skos:inScheme rdf:resource="http://www.cognitiveatlas.org/tasks/"/>
		<skos:definition>Any task that requires the subject to process the sound structure of words.</skos:definition>
		<skos:prefLabel>phonological task</skos:prefLabel>
		<skos:altLabel></skos:altLabel>
</skos:Concept><skos:Concept rdf:about="http://www.cognitiveatlas.org/id/trm_4f241bd52b509"> <dc:identifier>trm_4f241bd52b509</dc:identifier>
		<dc:Title>Cognitive Atlas : Lexicon : semantic fluency task</dc:Title>
		<dc:Description>RDF output for 'semantic fluency task'</dc:Description>
		<dc:Type>InteractiveResource</dc:Type>
		<dc:Publisher>Cognitive Atlas</dc:Publisher>
		<dc:Creator>Cognitive Atlas RDF Generator</dc:Creator>
		<dc:Contributor>Russ Poldrack</dc:Contributor>
		<dc:Date>2012-01-28 08:01:25</dc:Date>
		<dc:Format>text/rdf</dc:Format>
		<dc:Language>en</dc:Language>
		<skos:editorialNote>Generated by testgenall.php on Thu Mar 29 10:24:08 PDT 2012.</skos:editorialNote>
		<skos:historyNote>No previous definition revisions.</skos:historyNote>
		<skos:changeNote>This is the first and only definition provided.</skos:changeNote>
		<skos:scopeNote>http://www.w3.org/2004/02/skos/core#Concept</skos:scopeNote>
		<skos:Note>SKOS properties defined in http://www.w3.org/TR/skos-primer/#secrel</skos:Note>
		<skos:inScheme rdf:resource="http://www.cognitiveatlas.org/tasks/"/>
		<skos:prefLabel>semantic fluency task</skos:prefLabel>
		<skos:altLabel></skos:altLabel>
</skos:Concept><skos:Concept rdf:about="http://www.cognitiveatlas.org/id/trm_4f241be43458e"> <dc:identifier>trm_4f241be43458e</dc:identifier>
		<dc:Title>Cognitive Atlas : Lexicon : phonemic fluency task</dc:Title>
		<dc:Description>RDF output for 'phonemic fluency task'</dc:Description>
		<dc:Type>InteractiveResource</dc:Type>
		<dc:Publisher>Cognitive Atlas</dc:Publisher>
		<dc:Creator>Cognitive Atlas RDF Generator</dc:Creator>
		<dc:Contributor>Russ Poldrack</dc:Contributor>
		<dc:Date>2012-01-28 08:01:40</dc:Date>
		<dc:Format>text/rdf</dc:Format>
		<dc:Language>en</dc:Language>
		<skos:editorialNote>Generated by testgenall.php on Thu Mar 29 10:24:08 PDT 2012.</skos:editorialNote>
		<skos:historyNote>No previous definition revisions.</skos:historyNote>
		<skos:changeNote>This is the first and only definition provided.</skos:changeNote>
		<skos:scopeNote>http://www.w3.org/2004/02/skos/core#Concept</skos:scopeNote>
		<skos:Note>SKOS properties defined in http://www.w3.org/TR/skos-primer/#secrel</skos:Note>
		<skos:inScheme rdf:resource="http://www.cognitiveatlas.org/tasks/"/>
		<skos:prefLabel>phonemic fluency task</skos:prefLabel>
		<skos:altLabel></skos:altLabel>
</skos:Concept><skos:Concept rdf:about="http://www.cognitiveatlas.org/id/trm_4f241c0737cc0"> <dc:identifier>trm_4f241c0737cc0</dc:identifier>
		<dc:Title>Cognitive Atlas : Lexicon : semantic memory task</dc:Title>
		<dc:Description>RDF output for 'semantic memory task'</dc:Description>
		<dc:Type>InteractiveResource</dc:Type>
		<dc:Publisher>Cognitive Atlas</dc:Publisher>
		<dc:Creator>Cognitive Atlas RDF Generator</dc:Creator>
		<dc:Contributor>Russ Poldrack</dc:Contributor>
		<dc:Date>2012-01-28 08:02:15</dc:Date>
		<dc:Format>text/rdf</dc:Format>
		<dc:Language>en</dc:Language>
		<skos:editorialNote>Generated by testgenall.php on Thu Mar 29 10:24:08 PDT 2012.</skos:editorialNote>
		<skos:historyNote>No previous definition revisions.</skos:historyNote>
		<skos:changeNote>This is the first and only definition provided.</skos:changeNote>
		<skos:scopeNote>http://www.w3.org/2004/02/skos/core#Concept</skos:scopeNote>
		<skos:Note>SKOS properties defined in http://www.w3.org/TR/skos-primer/#secrel</skos:Note>
		<skos:inScheme rdf:resource="http://www.cognitiveatlas.org/tasks/"/>
		<skos:definition>A task requiring the subject to use knowledge retrieved from semantic memory.</skos:definition>
		<skos:prefLabel>semantic memory task</skos:prefLabel>
		<skos:altLabel></skos:altLabel>
</skos:Concept><skos:Concept rdf:about="http://www.cognitiveatlas.org/id/trm_4f241c735e7f6"> <dc:identifier>trm_4f241c735e7f6</dc:identifier>
		<dc:Title>Cognitive Atlas : Lexicon : serial reaction time task</dc:Title>
		<dc:Description>RDF output for 'serial reaction time task'</dc:Description>
		<dc:Type>InteractiveResource</dc:Type>
		<dc:Publisher>Cognitive Atlas</dc:Publisher>
		<dc:Creator>Cognitive Atlas RDF Generator</dc:Creator>
		<dc:Contributor>Russ Poldrack</dc:Contributor>
		<dc:Date>2012-01-28 08:04:03</dc:Date>
		<dc:Format>text/rdf</dc:Format>
		<dc:Language>en</dc:Language>
		<skos:editorialNote>Generated by testgenall.php on Thu Mar 29 10:24:08 PDT 2012.</skos:editorialNote>
		<skos:historyNote>No previous definition revisions.</skos:historyNote>
		<skos:changeNote>This is the first and only definition provided.</skos:changeNote>
		<skos:scopeNote>http://www.w3.org/2004/02/skos/core#Concept</skos:scopeNote>
		<skos:Note>SKOS properties defined in http://www.w3.org/TR/skos-primer/#secrel</skos:Note>
		<skos:inScheme rdf:resource="http://www.cognitiveatlas.org/tasks/"/>
		<skos:prefLabel>serial reaction time task</skos:prefLabel>
		<skos:altLabel>SRT, serial response time task, SRTT</skos:altLabel>
</skos:Concept><skos:Concept rdf:about="http://www.cognitiveatlas.org/id/trm_4f241c8d4a75c"> <dc:identifier>trm_4f241c8d4a75c</dc:identifier>
		<dc:Title>Cognitive Atlas : Lexicon : gender discrimination task</dc:Title>
		<dc:Description>RDF output for 'gender discrimination task'</dc:Description>
		<dc:Type>InteractiveResource</dc:Type>
		<dc:Publisher>Cognitive Atlas</dc:Publisher>
		<dc:Creator>Cognitive Atlas RDF Generator</dc:Creator>
		<dc:Contributor>Russ Poldrack</dc:Contributor>
		<dc:Date>2012-01-28 11:22:48</dc:Date>
		<dc:Format>text/rdf</dc:Format>
		<dc:Language>en</dc:Language>
		<skos:editorialNote>Generated by testgenall.php on Thu Mar 29 10:24:08 PDT 2012.</skos:editorialNote>
		<skos:historyNote>Revision 3: 2 previous definitions.</skos:historyNote>
		<skos:changeNote>See http://www.cognitiveatlas.org/id/trm_4f241c8d4a75c for complete revision history.</skos:changeNote>
		<skos:scopeNote>http://www.w3.org/2004/02/skos/core#Concept</skos:scopeNote>
		<skos:Note>SKOS properties defined in http://www.w3.org/TR/skos-primer/#secrel</skos:Note>
		<skos:inScheme rdf:resource="http://www.cognitiveatlas.org/tasks/"/>
		<skos:prefLabel>gender discrimination task</skos:prefLabel>
		<skos:altLabel>gender judgment task, gender decision task</skos:altLabel>
</skos:Concept><skos:Concept rdf:about="http://www.cognitiveatlas.org/id/trm_4f241d7adf14e"> <dc:identifier>trm_4f241d7adf14e</dc:identifier>
		<dc:Title>Cognitive Atlas : Lexicon : global-local task</dc:Title>
		<dc:Description>RDF output for 'global-local task'</dc:Description>
		<dc:Type>InteractiveResource</dc:Type>
		<dc:Publisher>Cognitive Atlas</dc:Publisher>
		<dc:Creator>Cognitive Atlas RDF Generator</dc:Creator>
		<dc:Contributor>Russ Poldrack</dc:Contributor>
		<dc:Date>2012-01-28 08:08:26</dc:Date>
		<dc:Format>text/rdf</dc:Format>
		<dc:Language>en</dc:Language>
		<skos:editorialNote>Generated by testgenall.php on Thu Mar 29 10:24:08 PDT 2012.</skos:editorialNote>
		<skos:historyNote>No previous definition revisions.</skos:historyNote>
		<skos:changeNote>This is the first and only definition provided.</skos:changeNote>
		<skos:scopeNote>http://www.w3.org/2004/02/skos/core#Concept</skos:scopeNote>
		<skos:Note>SKOS properties defined in http://www.w3.org/TR/skos-primer/#secrel</skos:Note>
		<skos:inScheme rdf:resource="http://www.cognitiveatlas.org/tasks/"/>
		<skos:prefLabel>global-local task</skos:prefLabel>
		<skos:altLabel></skos:altLabel>
</skos:Concept><skos:Concept rdf:about="http://www.cognitiveatlas.org/id/trm_4f241e8a01052"> <dc:identifier>trm_4f241e8a01052</dc:identifier>
		<dc:Title>Cognitive Atlas : Lexicon : sentence comprehension task</dc:Title>
		<dc:Description>RDF output for 'sentence comprehension task'</dc:Description>
		<dc:Type>InteractiveResource</dc:Type>
		<dc:Publisher>Cognitive Atlas</dc:Publisher>
		<dc:Creator>Cognitive Atlas RDF Generator</dc:Creator>
		<dc:Contributor>Russ Poldrack</dc:Contributor>
		<dc:Date>2012-01-28 08:12:58</dc:Date>
		<dc:Format>text/rdf</dc:Format>
		<dc:Language>en</dc:Language>
		<skos:editorialNote>Generated by testgenall.php on Thu Mar 29 10:24:08 PDT 2012.</skos:editorialNote>
		<skos:historyNote>No previous definition revisions.</skos:historyNote>
		<skos:changeNote>This is the first and only definition provided.</skos:changeNote>
		<skos:scopeNote>http://www.w3.org/2004/02/skos/core#Concept</skos:scopeNote>
		<skos:Note>SKOS properties defined in http://www.w3.org/TR/skos-primer/#secrel</skos:Note>
		<skos:inScheme rdf:resource="http://www.cognitiveatlas.org/tasks/"/>
		<skos:prefLabel>sentence comprehension task</skos:prefLabel>
		<skos:altLabel></skos:altLabel>
</skos:Concept><skos:Concept rdf:about="http://www.cognitiveatlas.org/id/trm_4f241ee9c4e37"> <dc:identifier>trm_4f241ee9c4e37</dc:identifier>
		<dc:Title>Cognitive Atlas : Lexicon : word-picture matching task</dc:Title>
		<dc:Description>RDF output for 'word-picture matching task'</dc:Description>
		<dc:Type>InteractiveResource</dc:Type>
		<dc:Publisher>Cognitive Atlas</dc:Publisher>
		<dc:Creator>Cognitive Atlas RDF Generator</dc:Creator>
		<dc:Contributor>Russ Poldrack</dc:Contributor>
		<dc:Date>2012-01-28 08:14:33</dc:Date>
		<dc:Format>text/rdf</dc:Format>
		<dc:Language>en</dc:Language>
		<skos:editorialNote>Generated by testgenall.php on Thu Mar 29 10:24:08 PDT 2012.</skos:editorialNote>
		<skos:historyNote>No previous definition revisions.</skos:historyNote>
		<skos:changeNote>This is the first and only definition provided.</skos:changeNote>
		<skos:scopeNote>http://www.w3.org/2004/02/skos/core#Concept</skos:scopeNote>
		<skos:Note>SKOS properties defined in http://www.w3.org/TR/skos-primer/#secrel</skos:Note>
		<skos:inScheme rdf:resource="http://www.cognitiveatlas.org/tasks/"/>
		<skos:prefLabel>word-picture matching task</skos:prefLabel>
		<skos:altLabel>picture-word matching task</skos:altLabel>
</skos:Concept><skos:Concept rdf:about="http://www.cognitiveatlas.org/id/trm_4f241fb95918f"> <dc:identifier>trm_4f241fb95918f</dc:identifier>
		<dc:Title>Cognitive Atlas : Lexicon : recency judgment task</dc:Title>
		<dc:Description>RDF output for 'recency judgment task'</dc:Description>
		<dc:Type>InteractiveResource</dc:Type>
		<dc:Publisher>Cognitive Atlas</dc:Publisher>
		<dc:Creator>Cognitive Atlas RDF Generator</dc:Creator>
		<dc:Contributor>Russ Poldrack</dc:Contributor>
		<dc:Date>2012-01-28 08:18:01</dc:Date>
		<dc:Format>text/rdf</dc:Format>
		<dc:Language>en</dc:Language>
		<skos:editorialNote>Generated by testgenall.php on Thu Mar 29 10:24:08 PDT 2012.</skos:editorialNote>
		<skos:historyNote>No previous definition revisions.</skos:historyNote>
		<skos:changeNote>This is the first and only definition provided.</skos:changeNote>
		<skos:scopeNote>http://www.w3.org/2004/02/skos/core#Concept</skos:scopeNote>
		<skos:Note>SKOS properties defined in http://www.w3.org/TR/skos-primer/#secrel</skos:Note>
		<skos:inScheme rdf:resource="http://www.cognitiveatlas.org/tasks/"/>
		<skos:prefLabel>recency judgment task</skos:prefLabel>
		<skos:altLabel></skos:altLabel>
</skos:Concept><skos:Concept rdf:about="http://www.cognitiveatlas.org/id/trm_4f241fd47f16b"> <dc:identifier>trm_4f241fd47f16b</dc:identifier>
		<dc:Title>Cognitive Atlas : Lexicon : passive avoidance task</dc:Title>
		<dc:Description>RDF output for 'passive avoidance task'</dc:Description>
		<dc:Type>InteractiveResource</dc:Type>
		<dc:Publisher>Cognitive Atlas</dc:Publisher>
		<dc:Creator>Cognitive Atlas RDF Generator</dc:Creator>
		<dc:Contributor>Russ Poldrack</dc:Contributor>
		<dc:Date>2012-01-28 08:18:28</dc:Date>
		<dc:Format>text/rdf</dc:Format>
		<dc:Language>en</dc:Language>
		<skos:editorialNote>Generated by testgenall.php on Thu Mar 29 10:24:08 PDT 2012.</skos:editorialNote>
		<skos:historyNote>No previous definition revisions.</skos:historyNote>
		<skos:changeNote>This is the first and only definition provided.</skos:changeNote>
		<skos:scopeNote>http://www.w3.org/2004/02/skos/core#Concept</skos:scopeNote>
		<skos:Note>SKOS properties defined in http://www.w3.org/TR/skos-primer/#secrel</skos:Note>
		<skos:inScheme rdf:resource="http://www.cognitiveatlas.org/tasks/"/>
		<skos:prefLabel>passive avoidance task</skos:prefLabel>
		<skos:altLabel></skos:altLabel>
</skos:Concept><skos:Concept rdf:about="http://www.cognitiveatlas.org/id/trm_4f241fe40a950"> <dc:identifier>trm_4f241fe40a950</dc:identifier>
		<dc:Title>Cognitive Atlas : Lexicon : fame judgment task</dc:Title>
		<dc:Description>RDF output for 'fame judgment task'</dc:Description>
		<dc:Type>InteractiveResource</dc:Type>
		<dc:Publisher>Cognitive Atlas</dc:Publisher>
		<dc:Creator>Cognitive Atlas RDF Generator</dc:Creator>
		<dc:Contributor>Russ Poldrack</dc:Contributor>
		<dc:Date>2012-01-28 08:18:44</dc:Date>
		<dc:Format>text/rdf</dc:Format>
		<dc:Language>en</dc:Language>
		<skos:editorialNote>Generated by testgenall.php on Thu Mar 29 10:24:08 PDT 2012.</skos:editorialNote>
		<skos:historyNote>No previous definition revisions.</skos:historyNote>
		<skos:changeNote>This is the first and only definition provided.</skos:changeNote>
		<skos:scopeNote>http://www.w3.org/2004/02/skos/core#Concept</skos:scopeNote>
		<skos:Note>SKOS properties defined in http://www.w3.org/TR/skos-primer/#secrel</skos:Note>
		<skos:inScheme rdf:resource="http://www.cognitiveatlas.org/tasks/"/>
		<skos:prefLabel>fame judgment task</skos:prefLabel>
		<skos:altLabel></skos:altLabel>
</skos:Concept><skos:Concept rdf:about="http://www.cognitiveatlas.org/id/trm_4f242042e5805"> <dc:identifier>trm_4f242042e5805</dc:identifier>
		<dc:Title>Cognitive Atlas : Lexicon : Cambridge risk task</dc:Title>
		<dc:Description>RDF output for 'Cambridge risk task'</dc:Description>
		<dc:Type>InteractiveResource</dc:Type>
		<dc:Publisher>Cognitive Atlas</dc:Publisher>
		<dc:Creator>Cognitive Atlas RDF Generator</dc:Creator>
		<dc:Contributor>Russ Poldrack</dc:Contributor>
		<dc:Date>2012-01-28 08:20:18</dc:Date>
		<dc:Format>text/rdf</dc:Format>
		<dc:Language>en</dc:Language>
		<skos:editorialNote>Generated by testgenall.php on Thu Mar 29 10:24:08 PDT 2012.</skos:editorialNote>
		<skos:historyNote>No previous definition revisions.</skos:historyNote>
		<skos:changeNote>This is the first and only definition provided.</skos:changeNote>
		<skos:scopeNote>http://www.w3.org/2004/02/skos/core#Concept</skos:scopeNote>
		<skos:Note>SKOS properties defined in http://www.w3.org/TR/skos-primer/#secrel</skos:Note>
		<skos:inScheme rdf:resource="http://www.cognitiveatlas.org/tasks/"/>
		<skos:prefLabel>Cambridge risk task</skos:prefLabel>
		<skos:altLabel></skos:altLabel>
</skos:Concept><skos:Concept rdf:about="http://www.cognitiveatlas.org/id/trm_4f2420b042165"> <dc:identifier>trm_4f2420b042165</dc:identifier>
		<dc:Title>Cognitive Atlas : Lexicon : reappraisal task</dc:Title>
		<dc:Description>RDF output for 'reappraisal task'</dc:Description>
		<dc:Type>InteractiveResource</dc:Type>
		<dc:Publisher>Cognitive Atlas</dc:Publisher>
		<dc:Creator>Cognitive Atlas RDF Generator</dc:Creator>
		<dc:Contributor>Russ Poldrack</dc:Contributor>
		<dc:Date>2012-01-28 08:22:08</dc:Date>
		<dc:Format>text/rdf</dc:Format>
		<dc:Language>en</dc:Language>
		<skos:editorialNote>Generated by testgenall.php on Thu Mar 29 10:24:08 PDT 2012.</skos:editorialNote>
		<skos:historyNote>No previous definition revisions.</skos:historyNote>
		<skos:changeNote>This is the first and only definition provided.</skos:changeNote>
		<skos:scopeNote>http://www.w3.org/2004/02/skos/core#Concept</skos:scopeNote>
		<skos:Note>SKOS properties defined in http://www.w3.org/TR/skos-primer/#secrel</skos:Note>
		<skos:inScheme rdf:resource="http://www.cognitiveatlas.org/tasks/"/>
		<skos:prefLabel>reappraisal task</skos:prefLabel>
		<skos:altLabel></skos:altLabel>
</skos:Concept><skos:Concept rdf:about="http://www.cognitiveatlas.org/id/trm_4f24211a03b07"> <dc:identifier>trm_4f24211a03b07</dc:identifier>
		<dc:Title>Cognitive Atlas : Lexicon : Raven&#39;s Advanced Progressive Matrices</dc:Title>
		<dc:Description>RDF output for 'Raven&#39;s Advanced Progressive Matrices'</dc:Description>
		<dc:Type>InteractiveResource</dc:Type>
		<dc:Publisher>Cognitive Atlas</dc:Publisher>
		<dc:Creator>Cognitive Atlas RDF Generator</dc:Creator>
		<dc:Contributor>Russ Poldrack</dc:Contributor>
		<dc:Date>2012-01-28 08:23:54</dc:Date>
		<dc:Format>text/rdf</dc:Format>
		<dc:Language>en</dc:Language>
		<skos:editorialNote>Generated by testgenall.php on Thu Mar 29 10:24:08 PDT 2012.</skos:editorialNote>
		<skos:historyNote>No previous definition revisions.</skos:historyNote>
		<skos:changeNote>This is the first and only definition provided.</skos:changeNote>
		<skos:scopeNote>http://www.w3.org/2004/02/skos/core#Concept</skos:scopeNote>
		<skos:Note>SKOS properties defined in http://www.w3.org/TR/skos-primer/#secrel</skos:Note>
		<skos:inScheme rdf:resource="http://www.cognitiveatlas.org/tasks/"/>
		<skos:prefLabel>Raven&#39;s Advanced Progressive Matrices</skos:prefLabel>
		<skos:altLabel>RAPM</skos:altLabel>
</skos:Concept><skos:Concept rdf:about="http://www.cognitiveatlas.org/id/trm_4f242172aea5d"> <dc:identifier>trm_4f242172aea5d</dc:identifier>
		<dc:Title>Cognitive Atlas : Lexicon : updating task</dc:Title>
		<dc:Description>RDF output for 'updating task'</dc:Description>
		<dc:Type>InteractiveResource</dc:Type>
		<dc:Publisher>Cognitive Atlas</dc:Publisher>
		<dc:Creator>Cognitive Atlas RDF Generator</dc:Creator>
		<dc:Contributor>Russ Poldrack</dc:Contributor>
		<dc:Date>2012-01-28 08:25:22</dc:Date>
		<dc:Format>text/rdf</dc:Format>
		<dc:Language>en</dc:Language>
		<skos:editorialNote>Generated by testgenall.php on Thu Mar 29 10:24:08 PDT 2012.</skos:editorialNote>
		<skos:historyNote>No previous definition revisions.</skos:historyNote>
		<skos:changeNote>This is the first and only definition provided.</skos:changeNote>
		<skos:scopeNote>http://www.w3.org/2004/02/skos/core#Concept</skos:scopeNote>
		<skos:Note>SKOS properties defined in http://www.w3.org/TR/skos-primer/#secrel</skos:Note>
		<skos:inScheme rdf:resource="http://www.cognitiveatlas.org/tasks/"/>
		<skos:prefLabel>updating task</skos:prefLabel>
		<skos:altLabel></skos:altLabel>
</skos:Concept><skos:Concept rdf:about="http://www.cognitiveatlas.org/id/trm_4f2421a62cdf8"> <dc:identifier>trm_4f2421a62cdf8</dc:identifier>
		<dc:Title>Cognitive Atlas : Lexicon : face working memory task</dc:Title>
		<dc:Description>RDF output for 'face working memory task'</dc:Description>
		<dc:Type>InteractiveResource</dc:Type>
		<dc:Publisher>Cognitive Atlas</dc:Publisher>
		<dc:Creator>Cognitive Atlas RDF Generator</dc:Creator>
		<dc:Contributor>Russ Poldrack</dc:Contributor>
		<dc:Date>2012-01-28 08:26:14</dc:Date>
		<dc:Format>text/rdf</dc:Format>
		<dc:Language>en</dc:Language>
		<skos:editorialNote>Generated by testgenall.php on Thu Mar 29 10:24:08 PDT 2012.</skos:editorialNote>
		<skos:historyNote>No previous definition revisions.</skos:historyNote>
		<skos:changeNote>This is the first and only definition provided.</skos:changeNote>
		<skos:scopeNote>http://www.w3.org/2004/02/skos/core#Concept</skos:scopeNote>
		<skos:Note>SKOS properties defined in http://www.w3.org/TR/skos-primer/#secrel</skos:Note>
		<skos:inScheme rdf:resource="http://www.cognitiveatlas.org/tasks/"/>
		<skos:prefLabel>face working memory task</skos:prefLabel>
		<skos:altLabel>face wm task</skos:altLabel>
</skos:Concept><skos:Concept rdf:about="http://www.cognitiveatlas.org/id/trm_4f2421c391b83"> <dc:identifier>trm_4f2421c391b83</dc:identifier>
		<dc:Title>Cognitive Atlas : Lexicon : object working memory task</dc:Title>
		<dc:Description>RDF output for 'object working memory task'</dc:Description>
		<dc:Type>InteractiveResource</dc:Type>
		<dc:Publisher>Cognitive Atlas</dc:Publisher>
		<dc:Creator>Cognitive Atlas RDF Generator</dc:Creator>
		<dc:Contributor>Russ Poldrack</dc:Contributor>
		<dc:Date>2012-01-28 08:26:43</dc:Date>
		<dc:Format>text/rdf</dc:Format>
		<dc:Language>en</dc:Language>
		<skos:editorialNote>Generated by testgenall.php on Thu Mar 29 10:24:08 PDT 2012.</skos:editorialNote>
		<skos:historyNote>No previous definition revisions.</skos:historyNote>
		<skos:changeNote>This is the first and only definition provided.</skos:changeNote>
		<skos:scopeNote>http://www.w3.org/2004/02/skos/core#Concept</skos:scopeNote>
		<skos:Note>SKOS properties defined in http://www.w3.org/TR/skos-primer/#secrel</skos:Note>
		<skos:inScheme rdf:resource="http://www.cognitiveatlas.org/tasks/"/>
		<skos:prefLabel>object working memory task</skos:prefLabel>
		<skos:altLabel>object wm task</skos:altLabel>
</skos:Concept><skos:Concept rdf:about="http://www.cognitiveatlas.org/id/trm_4f24226fa2903"> <dc:identifier>trm_4f24226fa2903</dc:identifier>
		<dc:Title>Cognitive Atlas : Lexicon : Fitts task</dc:Title>
		<dc:Description>RDF output for 'Fitts task'</dc:Description>
		<dc:Type>InteractiveResource</dc:Type>
		<dc:Publisher>Cognitive Atlas</dc:Publisher>
		<dc:Creator>Cognitive Atlas RDF Generator</dc:Creator>
		<dc:Contributor>Russ Poldrack</dc:Contributor>
		<dc:Date>2012-01-28 08:29:35</dc:Date>
		<dc:Format>text/rdf</dc:Format>
		<dc:Language>en</dc:Language>
		<skos:editorialNote>Generated by testgenall.php on Thu Mar 29 10:24:08 PDT 2012.</skos:editorialNote>
		<skos:historyNote>No previous definition revisions.</skos:historyNote>
		<skos:changeNote>This is the first and only definition provided.</skos:changeNote>
		<skos:scopeNote>http://www.w3.org/2004/02/skos/core#Concept</skos:scopeNote>
		<skos:Note>SKOS properties defined in http://www.w3.org/TR/skos-primer/#secrel</skos:Note>
		<skos:inScheme rdf:resource="http://www.cognitiveatlas.org/tasks/"/>
		<skos:prefLabel>Fitts task</skos:prefLabel>
		<skos:altLabel>Fitts tapping task</skos:altLabel>
</skos:Concept><skos:Concept rdf:about="http://www.cognitiveatlas.org/id/trm_4f24237f2ed47"> <dc:identifier>trm_4f24237f2ed47</dc:identifier>
		<dc:Title>Cognitive Atlas : Lexicon : general knowledge task</dc:Title>
		<dc:Description>RDF output for 'general knowledge task'</dc:Description>
		<dc:Type>InteractiveResource</dc:Type>
		<dc:Publisher>Cognitive Atlas</dc:Publisher>
		<dc:Creator>Cognitive Atlas RDF Generator</dc:Creator>
		<dc:Contributor>Russ Poldrack</dc:Contributor>
		<dc:Date>2012-01-28 08:34:07</dc:Date>
		<dc:Format>text/rdf</dc:Format>
		<dc:Language>en</dc:Language>
		<skos:editorialNote>Generated by testgenall.php on Thu Mar 29 10:24:08 PDT 2012.</skos:editorialNote>
		<skos:historyNote>No previous definition revisions.</skos:historyNote>
		<skos:changeNote>This is the first and only definition provided.</skos:changeNote>
		<skos:scopeNote>http://www.w3.org/2004/02/skos/core#Concept</skos:scopeNote>
		<skos:Note>SKOS properties defined in http://www.w3.org/TR/skos-primer/#secrel</skos:Note>
		<skos:inScheme rdf:resource="http://www.cognitiveatlas.org/tasks/"/>
		<skos:prefLabel>general knowledge task</skos:prefLabel>
		<skos:altLabel></skos:altLabel>
</skos:Concept><skos:Concept rdf:about="http://www.cognitiveatlas.org/id/trm_4f24239cc239e"> <dc:identifier>trm_4f24239cc239e</dc:identifier>
		<dc:Title>Cognitive Atlas : Lexicon : short-term memory task</dc:Title>
		<dc:Description>RDF output for 'short-term memory task'</dc:Description>
		<dc:Type>InteractiveResource</dc:Type>
		<dc:Publisher>Cognitive Atlas</dc:Publisher>
		<dc:Creator>Cognitive Atlas RDF Generator</dc:Creator>
		<dc:Contributor>Russ Poldrack</dc:Contributor>
		<dc:Date>2012-01-28 08:34:36</dc:Date>
		<dc:Format>text/rdf</dc:Format>
		<dc:Language>en</dc:Language>
		<skos:editorialNote>Generated by testgenall.php on Thu Mar 29 10:24:08 PDT 2012.</skos:editorialNote>
		<skos:historyNote>No previous definition revisions.</skos:historyNote>
		<skos:changeNote>This is the first and only definition provided.</skos:changeNote>
		<skos:scopeNote>http://www.w3.org/2004/02/skos/core#Concept</skos:scopeNote>
		<skos:Note>SKOS properties defined in http://www.w3.org/TR/skos-primer/#secrel</skos:Note>
		<skos:inScheme rdf:resource="http://www.cognitiveatlas.org/tasks/"/>
		<skos:prefLabel>short-term memory task</skos:prefLabel>
		<skos:altLabel>STM task</skos:altLabel>
</skos:Concept><skos:Concept rdf:about="http://www.cognitiveatlas.org/id/trm_4f24247912761"> <dc:identifier>trm_4f24247912761</dc:identifier>
		<dc:Title>Cognitive Atlas : Lexicon : face matching task</dc:Title>
		<dc:Description>RDF output for 'face matching task'</dc:Description>
		<dc:Type>InteractiveResource</dc:Type>
		<dc:Publisher>Cognitive Atlas</dc:Publisher>
		<dc:Creator>Cognitive Atlas RDF Generator</dc:Creator>
		<dc:Contributor>Russ Poldrack</dc:Contributor>
		<dc:Date>2012-01-28 08:38:17</dc:Date>
		<dc:Format>text/rdf</dc:Format>
		<dc:Language>en</dc:Language>
		<skos:editorialNote>Generated by testgenall.php on Thu Mar 29 10:24:08 PDT 2012.</skos:editorialNote>
		<skos:historyNote>No previous definition revisions.</skos:historyNote>
		<skos:changeNote>This is the first and only definition provided.</skos:changeNote>
		<skos:scopeNote>http://www.w3.org/2004/02/skos/core#Concept</skos:scopeNote>
		<skos:Note>SKOS properties defined in http://www.w3.org/TR/skos-primer/#secrel</skos:Note>
		<skos:inScheme rdf:resource="http://www.cognitiveatlas.org/tasks/"/>
		<skos:prefLabel>face matching task</skos:prefLabel>
		<skos:altLabel></skos:altLabel>
</skos:Concept><skos:Concept rdf:about="http://www.cognitiveatlas.org/id/trm_4f242499b8952"> <dc:identifier>trm_4f242499b8952</dc:identifier>
		<dc:Title>Cognitive Atlas : Lexicon : target detection task</dc:Title>
		<dc:Description>RDF output for 'target detection task'</dc:Description>
		<dc:Type>InteractiveResource</dc:Type>
		<dc:Publisher>Cognitive Atlas</dc:Publisher>
		<dc:Creator>Cognitive Atlas RDF Generator</dc:Creator>
		<dc:Contributor>Russ Poldrack</dc:Contributor>
		<dc:Date>2012-01-28 08:38:49</dc:Date>
		<dc:Format>text/rdf</dc:Format>
		<dc:Language>en</dc:Language>
		<skos:editorialNote>Generated by testgenall.php on Thu Mar 29 10:24:08 PDT 2012.</skos:editorialNote>
		<skos:historyNote>No previous definition revisions.</skos:historyNote>
		<skos:changeNote>This is the first and only definition provided.</skos:changeNote>
		<skos:scopeNote>http://www.w3.org/2004/02/skos/core#Concept</skos:scopeNote>
		<skos:Note>SKOS properties defined in http://www.w3.org/TR/skos-primer/#secrel</skos:Note>
		<skos:inScheme rdf:resource="http://www.cognitiveatlas.org/tasks/"/>
		<skos:prefLabel>target detection task</skos:prefLabel>
		<skos:altLabel></skos:altLabel>
</skos:Concept><skos:Concept rdf:about="http://www.cognitiveatlas.org/id/trm_4f2424cb392fc"> <dc:identifier>trm_4f2424cb392fc</dc:identifier>
		<dc:Title>Cognitive Atlas : Lexicon : face-name association task</dc:Title>
		<dc:Description>RDF output for 'face-name association task'</dc:Description>
		<dc:Type>InteractiveResource</dc:Type>
		<dc:Publisher>Cognitive Atlas</dc:Publisher>
		<dc:Creator>Cognitive Atlas RDF Generator</dc:Creator>
		<dc:Contributor>Russ Poldrack</dc:Contributor>
		<dc:Date>2012-01-28 08:39:39</dc:Date>
		<dc:Format>text/rdf</dc:Format>
		<dc:Language>en</dc:Language>
		<skos:editorialNote>Generated by testgenall.php on Thu Mar 29 10:24:08 PDT 2012.</skos:editorialNote>
		<skos:historyNote>No previous definition revisions.</skos:historyNote>
		<skos:changeNote>This is the first and only definition provided.</skos:changeNote>
		<skos:scopeNote>http://www.w3.org/2004/02/skos/core#Concept</skos:scopeNote>
		<skos:Note>SKOS properties defined in http://www.w3.org/TR/skos-primer/#secrel</skos:Note>
		<skos:inScheme rdf:resource="http://www.cognitiveatlas.org/tasks/"/>
		<skos:prefLabel>face-name association task</skos:prefLabel>
		<skos:altLabel></skos:altLabel>
</skos:Concept><skos:Concept rdf:about="http://www.cognitiveatlas.org/id/trm_4f24250e0137e"> <dc:identifier>trm_4f24250e0137e</dc:identifier>
		<dc:Title>Cognitive Atlas : Lexicon : orthographic task</dc:Title>
		<dc:Description>RDF output for 'orthographic task'</dc:Description>
		<dc:Type>InteractiveResource</dc:Type>
		<dc:Publisher>Cognitive Atlas</dc:Publisher>
		<dc:Creator>Cognitive Atlas RDF Generator</dc:Creator>
		<dc:Contributor>Russ Poldrack</dc:Contributor>
		<dc:Date>2012-01-28 08:40:46</dc:Date>
		<dc:Format>text/rdf</dc:Format>
		<dc:Language>en</dc:Language>
		<skos:editorialNote>Generated by testgenall.php on Thu Mar 29 10:24:08 PDT 2012.</skos:editorialNote>
		<skos:historyNote>No previous definition revisions.</skos:historyNote>
		<skos:changeNote>This is the first and only definition provided.</skos:changeNote>
		<skos:scopeNote>http://www.w3.org/2004/02/skos/core#Concept</skos:scopeNote>
		<skos:Note>SKOS properties defined in http://www.w3.org/TR/skos-primer/#secrel</skos:Note>
		<skos:inScheme rdf:resource="http://www.cognitiveatlas.org/tasks/"/>
		<skos:definition>A task that requires processing of letter structure</skos:definition>
		<skos:prefLabel>orthographic task</skos:prefLabel>
		<skos:altLabel></skos:altLabel>
</skos:Concept><skos:Concept rdf:about="http://www.cognitiveatlas.org/id/trm_4f24258b51e2c"> <dc:identifier>trm_4f24258b51e2c</dc:identifier>
		<dc:Title>Cognitive Atlas : Lexicon : living-nonliving task</dc:Title>
		<dc:Description>RDF output for 'living-nonliving task'</dc:Description>
		<dc:Type>InteractiveResource</dc:Type>
		<dc:Publisher>Cognitive Atlas</dc:Publisher>
		<dc:Creator>Cognitive Atlas RDF Generator</dc:Creator>
		<dc:Contributor>Russ Poldrack</dc:Contributor>
		<dc:Date>2012-01-28 08:42:51</dc:Date>
		<dc:Format>text/rdf</dc:Format>
		<dc:Language>en</dc:Language>
		<skos:editorialNote>Generated by testgenall.php on Thu Mar 29 10:24:08 PDT 2012.</skos:editorialNote>
		<skos:historyNote>No previous definition revisions.</skos:historyNote>
		<skos:changeNote>This is the first and only definition provided.</skos:changeNote>
		<skos:scopeNote>http://www.w3.org/2004/02/skos/core#Concept</skos:scopeNote>
		<skos:Note>SKOS properties defined in http://www.w3.org/TR/skos-primer/#secrel</skos:Note>
		<skos:inScheme rdf:resource="http://www.cognitiveatlas.org/tasks/"/>
		<skos:prefLabel>living-nonliving task</skos:prefLabel>
		<skos:altLabel></skos:altLabel>
</skos:Concept><skos:Concept rdf:about="http://www.cognitiveatlas.org/id/trm_4f24479b0db8f"> <dc:identifier>trm_4f24479b0db8f</dc:identifier>
		<dc:Title>Cognitive Atlas : Lexicon : phoneme detection task</dc:Title>
		<dc:Description>RDF output for 'phoneme detection task'</dc:Description>
		<dc:Type>InteractiveResource</dc:Type>
		<dc:Publisher>Cognitive Atlas</dc:Publisher>
		<dc:Creator>Cognitive Atlas RDF Generator</dc:Creator>
		<dc:Contributor>Russ Poldrack</dc:Contributor>
		<dc:Date>2012-01-28 11:08:11</dc:Date>
		<dc:Format>text/rdf</dc:Format>
		<dc:Language>en</dc:Language>
		<skos:editorialNote>Generated by testgenall.php on Thu Mar 29 10:24:08 PDT 2012.</skos:editorialNote>
		<skos:historyNote>No previous definition revisions.</skos:historyNote>
		<skos:changeNote>This is the first and only definition provided.</skos:changeNote>
		<skos:scopeNote>http://www.w3.org/2004/02/skos/core#Concept</skos:scopeNote>
		<skos:Note>SKOS properties defined in http://www.w3.org/TR/skos-primer/#secrel</skos:Note>
		<skos:inScheme rdf:resource="http://www.cognitiveatlas.org/tasks/"/>
		<skos:prefLabel>phoneme detection task</skos:prefLabel>
		<skos:altLabel></skos:altLabel>
</skos:Concept><skos:Concept rdf:about="http://www.cognitiveatlas.org/id/trm_4f2447dfa5947"> <dc:identifier>trm_4f2447dfa5947</dc:identifier>
		<dc:Title>Cognitive Atlas : Lexicon : stop-change task</dc:Title>
		<dc:Description>RDF output for 'stop-change task'</dc:Description>
		<dc:Type>InteractiveResource</dc:Type>
		<dc:Publisher>Cognitive Atlas</dc:Publisher>
		<dc:Creator>Cognitive Atlas RDF Generator</dc:Creator>
		<dc:Contributor>Russ Poldrack</dc:Contributor>
		<dc:Date>2012-01-28 11:09:19</dc:Date>
		<dc:Format>text/rdf</dc:Format>
		<dc:Language>en</dc:Language>
		<skos:editorialNote>Generated by testgenall.php on Thu Mar 29 10:24:08 PDT 2012.</skos:editorialNote>
		<skos:historyNote>No previous definition revisions.</skos:historyNote>
		<skos:changeNote>This is the first and only definition provided.</skos:changeNote>
		<skos:scopeNote>http://www.w3.org/2004/02/skos/core#Concept</skos:scopeNote>
		<skos:Note>SKOS properties defined in http://www.w3.org/TR/skos-primer/#secrel</skos:Note>
		<skos:inScheme rdf:resource="http://www.cognitiveatlas.org/tasks/"/>
		<skos:definition>A task in which the subject makes a discriminative response by default, but makes a different response upon presentation of a stop signal.</skos:definition>
		<skos:prefLabel>stop-change task</skos:prefLabel>
		<skos:altLabel></skos:altLabel>
</skos:Concept><skos:Concept rdf:about="http://www.cognitiveatlas.org/id/trm_4f2447fe67fb9"> <dc:identifier>trm_4f2447fe67fb9</dc:identifier>
		<dc:Title>Cognitive Atlas : Lexicon : visual search task</dc:Title>
		<dc:Description>RDF output for 'visual search task'</dc:Description>
		<dc:Type>InteractiveResource</dc:Type>
		<dc:Publisher>Cognitive Atlas</dc:Publisher>
		<dc:Creator>Cognitive Atlas RDF Generator</dc:Creator>
		<dc:Contributor>Russ Poldrack</dc:Contributor>
		<dc:Date>2012-01-28 11:09:50</dc:Date>
		<dc:Format>text/rdf</dc:Format>
		<dc:Language>en</dc:Language>
		<skos:editorialNote>Generated by testgenall.php on Thu Mar 29 10:24:08 PDT 2012.</skos:editorialNote>
		<skos:historyNote>No previous definition revisions.</skos:historyNote>
		<skos:changeNote>This is the first and only definition provided.</skos:changeNote>
		<skos:scopeNote>http://www.w3.org/2004/02/skos/core#Concept</skos:scopeNote>
		<skos:Note>SKOS properties defined in http://www.w3.org/TR/skos-primer/#secrel</skos:Note>
		<skos:inScheme rdf:resource="http://www.cognitiveatlas.org/tasks/"/>
		<skos:prefLabel>visual search task</skos:prefLabel>
		<skos:altLabel></skos:altLabel>
</skos:Concept><skos:Concept rdf:about="http://www.cognitiveatlas.org/id/trm_4f244860c702c"> <dc:identifier>trm_4f244860c702c</dc:identifier>
		<dc:Title>Cognitive Atlas : Lexicon : prospective memory task</dc:Title>
		<dc:Description>RDF output for 'prospective memory task'</dc:Description>
		<dc:Type>InteractiveResource</dc:Type>
		<dc:Publisher>Cognitive Atlas</dc:Publisher>
		<dc:Creator>Cognitive Atlas RDF Generator</dc:Creator>
		<dc:Contributor>Russ Poldrack</dc:Contributor>
		<dc:Date>2012-01-28 11:11:28</dc:Date>
		<dc:Format>text/rdf</dc:Format>
		<dc:Language>en</dc:Language>
		<skos:editorialNote>Generated by testgenall.php on Thu Mar 29 10:24:08 PDT 2012.</skos:editorialNote>
		<skos:historyNote>No previous definition revisions.</skos:historyNote>
		<skos:changeNote>This is the first and only definition provided.</skos:changeNote>
		<skos:scopeNote>http://www.w3.org/2004/02/skos/core#Concept</skos:scopeNote>
		<skos:Note>SKOS properties defined in http://www.w3.org/TR/skos-primer/#secrel</skos:Note>
		<skos:inScheme rdf:resource="http://www.cognitiveatlas.org/tasks/"/>
		<skos:prefLabel>prospective memory task</skos:prefLabel>
		<skos:altLabel></skos:altLabel>
</skos:Concept><skos:Concept rdf:about="http://www.cognitiveatlas.org/id/trm_4f2448d02d4d9"> <dc:identifier>trm_4f2448d02d4d9</dc:identifier>
		<dc:Title>Cognitive Atlas : Lexicon : object naming task</dc:Title>
		<dc:Description>RDF output for 'object naming task'</dc:Description>
		<dc:Type>InteractiveResource</dc:Type>
		<dc:Publisher>Cognitive Atlas</dc:Publisher>
		<dc:Creator>Cognitive Atlas RDF Generator</dc:Creator>
		<dc:Contributor>Russ Poldrack</dc:Contributor>
		<dc:Date>2012-01-28 11:13:20</dc:Date>
		<dc:Format>text/rdf</dc:Format>
		<dc:Language>en</dc:Language>
		<skos:editorialNote>Generated by testgenall.php on Thu Mar 29 10:24:08 PDT 2012.</skos:editorialNote>
		<skos:historyNote>No previous definition revisions.</skos:historyNote>
		<skos:changeNote>This is the first and only definition provided.</skos:changeNote>
		<skos:scopeNote>http://www.w3.org/2004/02/skos/core#Concept</skos:scopeNote>
		<skos:Note>SKOS properties defined in http://www.w3.org/TR/skos-primer/#secrel</skos:Note>
		<skos:inScheme rdf:resource="http://www.cognitiveatlas.org/tasks/"/>
		<skos:prefLabel>object naming task</skos:prefLabel>
		<skos:altLabel></skos:altLabel>
</skos:Concept><skos:Concept rdf:about="http://www.cognitiveatlas.org/id/trm_4f24492504ca0"> <dc:identifier>trm_4f24492504ca0</dc:identifier>
		<dc:Title>Cognitive Atlas : Lexicon : contextual cueing task</dc:Title>
		<dc:Description>RDF output for 'contextual cueing task'</dc:Description>
		<dc:Type>InteractiveResource</dc:Type>
		<dc:Publisher>Cognitive Atlas</dc:Publisher>
		<dc:Creator>Cognitive Atlas RDF Generator</dc:Creator>
		<dc:Contributor>Russ Poldrack</dc:Contributor>
		<dc:Date>2012-01-28 11:14:45</dc:Date>
		<dc:Format>text/rdf</dc:Format>
		<dc:Language>en</dc:Language>
		<skos:editorialNote>Generated by testgenall.php on Thu Mar 29 10:24:08 PDT 2012.</skos:editorialNote>
		<skos:historyNote>No previous definition revisions.</skos:historyNote>
		<skos:changeNote>This is the first and only definition provided.</skos:changeNote>
		<skos:scopeNote>http://www.w3.org/2004/02/skos/core#Concept</skos:scopeNote>
		<skos:Note>SKOS properties defined in http://www.w3.org/TR/skos-primer/#secrel</skos:Note>
		<skos:inScheme rdf:resource="http://www.cognitiveatlas.org/tasks/"/>
		<skos:prefLabel>contextual cueing task</skos:prefLabel>
		<skos:altLabel>contextual cuing task</skos:altLabel>
</skos:Concept><skos:Concept rdf:about="http://www.cognitiveatlas.org/id/trm_4f24496a80587"> <dc:identifier>trm_4f24496a80587</dc:identifier>
		<dc:Title>Cognitive Atlas : Lexicon : gambling task</dc:Title>
		<dc:Description>RDF output for 'gambling task'</dc:Description>
		<dc:Type>InteractiveResource</dc:Type>
		<dc:Publisher>Cognitive Atlas</dc:Publisher>
		<dc:Creator>Cognitive Atlas RDF Generator</dc:Creator>
		<dc:Contributor>Russ Poldrack</dc:Contributor>
		<dc:Date>2012-01-28 11:18:37</dc:Date>
		<dc:Format>text/rdf</dc:Format>
		<dc:Language>en</dc:Language>
		<skos:editorialNote>Generated by testgenall.php on Thu Mar 29 10:24:08 PDT 2012.</skos:editorialNote>
		<skos:historyNote>Revision 2: 1 previous definitions.</skos:historyNote>
		<skos:changeNote>See http://www.cognitiveatlas.org/id/trm_4f24496a80587 for complete revision history.</skos:changeNote>
		<skos:scopeNote>http://www.w3.org/2004/02/skos/core#Concept</skos:scopeNote>
		<skos:Note>SKOS properties defined in http://www.w3.org/TR/skos-primer/#secrel</skos:Note>
		<skos:inScheme rdf:resource="http://www.cognitiveatlas.org/tasks/"/>
		<skos:definition>A class of tasks in which subjects make decisions about chance gambles.</skos:definition>
		<skos:prefLabel>gambling task</skos:prefLabel>
		<skos:altLabel>gamble task</skos:altLabel>
</skos:Concept><skos:Concept rdf:about="http://www.cognitiveatlas.org/id/trm_4f2449bdcb0b1"> <dc:identifier>trm_4f2449bdcb0b1</dc:identifier>
		<dc:Title>Cognitive Atlas : Lexicon : Wason card selection task</dc:Title>
		<dc:Description>RDF output for 'Wason card selection task'</dc:Description>
		<dc:Type>InteractiveResource</dc:Type>
		<dc:Publisher>Cognitive Atlas</dc:Publisher>
		<dc:Creator>Cognitive Atlas RDF Generator</dc:Creator>
		<dc:Contributor>Russ Poldrack</dc:Contributor>
		<dc:Date>2012-01-28 11:17:17</dc:Date>
		<dc:Format>text/rdf</dc:Format>
		<dc:Language>en</dc:Language>
		<skos:editorialNote>Generated by testgenall.php on Thu Mar 29 10:24:08 PDT 2012.</skos:editorialNote>
		<skos:historyNote>No previous definition revisions.</skos:historyNote>
		<skos:changeNote>This is the first and only definition provided.</skos:changeNote>
		<skos:scopeNote>http://www.w3.org/2004/02/skos/core#Concept</skos:scopeNote>
		<skos:Note>SKOS properties defined in http://www.w3.org/TR/skos-primer/#secrel</skos:Note>
		<skos:inScheme rdf:resource="http://www.cognitiveatlas.org/tasks/"/>
		<skos:prefLabel>Wason card selection task</skos:prefLabel>
		<skos:altLabel>Wason card task, Wason task</skos:altLabel>
</skos:Concept><skos:Concept rdf:about="http://www.cognitiveatlas.org/id/trm_4f244a453522b"> <dc:identifier>trm_4f244a453522b</dc:identifier>
		<dc:Title>Cognitive Atlas : Lexicon : syntactic task</dc:Title>
		<dc:Description>RDF output for 'syntactic task'</dc:Description>
		<dc:Type>InteractiveResource</dc:Type>
		<dc:Publisher>Cognitive Atlas</dc:Publisher>
		<dc:Creator>Cognitive Atlas RDF Generator</dc:Creator>
		<dc:Contributor>Russ Poldrack</dc:Contributor>
		<dc:Date>2012-01-28 11:19:33</dc:Date>
		<dc:Format>text/rdf</dc:Format>
		<dc:Language>en</dc:Language>
		<skos:editorialNote>Generated by testgenall.php on Thu Mar 29 10:24:08 PDT 2012.</skos:editorialNote>
		<skos:historyNote>No previous definition revisions.</skos:historyNote>
		<skos:changeNote>This is the first and only definition provided.</skos:changeNote>
		<skos:scopeNote>http://www.w3.org/2004/02/skos/core#Concept</skos:scopeNote>
		<skos:Note>SKOS properties defined in http://www.w3.org/TR/skos-primer/#secrel</skos:Note>
		<skos:inScheme rdf:resource="http://www.cognitiveatlas.org/tasks/"/>
		<skos:definition>A class of tasks involving the processing of linguistic syntax.</skos:definition>
		<skos:prefLabel>syntactic task</skos:prefLabel>
		<skos:altLabel></skos:altLabel>
</skos:Concept><skos:Concept rdf:about="http://www.cognitiveatlas.org/id/trm_4f244a67d5b17"> <dc:identifier>trm_4f244a67d5b17</dc:identifier>
		<dc:Title>Cognitive Atlas : Lexicon : mirror reading task</dc:Title>
		<dc:Description>RDF output for 'mirror reading task'</dc:Description>
		<dc:Type>InteractiveResource</dc:Type>
		<dc:Publisher>Cognitive Atlas</dc:Publisher>
		<dc:Creator>Cognitive Atlas RDF Generator</dc:Creator>
		<dc:Contributor>Russ Poldrack</dc:Contributor>
		<dc:Date>2012-01-28 11:20:07</dc:Date>
		<dc:Format>text/rdf</dc:Format>
		<dc:Language>en</dc:Language>
		<skos:editorialNote>Generated by testgenall.php on Thu Mar 29 10:24:08 PDT 2012.</skos:editorialNote>
		<skos:historyNote>No previous definition revisions.</skos:historyNote>
		<skos:changeNote>This is the first and only definition provided.</skos:changeNote>
		<skos:scopeNote>http://www.w3.org/2004/02/skos/core#Concept</skos:scopeNote>
		<skos:Note>SKOS properties defined in http://www.w3.org/TR/skos-primer/#secrel</skos:Note>
		<skos:inScheme rdf:resource="http://www.cognitiveatlas.org/tasks/"/>
		<skos:prefLabel>mirror reading task</skos:prefLabel>
		<skos:altLabel></skos:altLabel>
</skos:Concept><skos:Concept rdf:about="http://www.cognitiveatlas.org/id/trm_4f244a88013ae"> <dc:identifier>trm_4f244a88013ae</dc:identifier>
		<dc:Title>Cognitive Atlas : Lexicon : artificial grammar learning task</dc:Title>
		<dc:Description>RDF output for 'artificial grammar learning task'</dc:Description>
		<dc:Type>InteractiveResource</dc:Type>
		<dc:Publisher>Cognitive Atlas</dc:Publisher>
		<dc:Creator>Cognitive Atlas RDF Generator</dc:Creator>
		<dc:Contributor>Russ Poldrack</dc:Contributor>
		<dc:Date>2012-01-28 11:20:40</dc:Date>
		<dc:Format>text/rdf</dc:Format>
		<dc:Language>en</dc:Language>
		<skos:editorialNote>Generated by testgenall.php on Thu Mar 29 10:24:08 PDT 2012.</skos:editorialNote>
		<skos:historyNote>No previous definition revisions.</skos:historyNote>
		<skos:changeNote>This is the first and only definition provided.</skos:changeNote>
		<skos:scopeNote>http://www.w3.org/2004/02/skos/core#Concept</skos:scopeNote>
		<skos:Note>SKOS properties defined in http://www.w3.org/TR/skos-primer/#secrel</skos:Note>
		<skos:inScheme rdf:resource="http://www.cognitiveatlas.org/tasks/"/>
		<skos:prefLabel>artificial grammar learning task</skos:prefLabel>
		<skos:altLabel></skos:altLabel>
</skos:Concept><skos:Concept rdf:about="http://www.cognitiveatlas.org/id/trm_4f244ad7dcde7"> <dc:identifier>trm_4f244ad7dcde7</dc:identifier>
		<dc:Title>Cognitive Atlas : Lexicon : random-dot motion task</dc:Title>
		<dc:Description>RDF output for 'random-dot motion task'</dc:Description>
		<dc:Type>InteractiveResource</dc:Type>
		<dc:Publisher>Cognitive Atlas</dc:Publisher>
		<dc:Creator>Cognitive Atlas RDF Generator</dc:Creator>
		<dc:Contributor>Russ Poldrack</dc:Contributor>
		<dc:Date>2012-01-28 11:21:59</dc:Date>
		<dc:Format>text/rdf</dc:Format>
		<dc:Language>en</dc:Language>
		<skos:editorialNote>Generated by testgenall.php on Thu Mar 29 10:24:08 PDT 2012.</skos:editorialNote>
		<skos:historyNote>No previous definition revisions.</skos:historyNote>
		<skos:changeNote>This is the first and only definition provided.</skos:changeNote>
		<skos:scopeNote>http://www.w3.org/2004/02/skos/core#Concept</skos:scopeNote>
		<skos:Note>SKOS properties defined in http://www.w3.org/TR/skos-primer/#secrel</skos:Note>
		<skos:inScheme rdf:resource="http://www.cognitiveatlas.org/tasks/"/>
		<skos:prefLabel>random-dot motion task</skos:prefLabel>
		<skos:altLabel>dot-motion task, moving-dot task</skos:altLabel>
</skos:Concept><skos:Concept rdf:about="http://www.cognitiveatlas.org/id/trm_4f244c1f6b53f"> <dc:identifier>trm_4f244c1f6b53f</dc:identifier>
		<dc:Title>Cognitive Atlas : Lexicon : color naming task</dc:Title>
		<dc:Description>RDF output for 'color naming task'</dc:Description>
		<dc:Type>InteractiveResource</dc:Type>
		<dc:Publisher>Cognitive Atlas</dc:Publisher>
		<dc:Creator>Cognitive Atlas RDF Generator</dc:Creator>
		<dc:Contributor>Russ Poldrack</dc:Contributor>
		<dc:Date>2012-01-28 11:27:27</dc:Date>
		<dc:Format>text/rdf</dc:Format>
		<dc:Language>en</dc:Language>
		<skos:editorialNote>Generated by testgenall.php on Thu Mar 29 10:24:08 PDT 2012.</skos:editorialNote>
		<skos:historyNote>No previous definition revisions.</skos:historyNote>
		<skos:changeNote>This is the first and only definition provided.</skos:changeNote>
		<skos:scopeNote>http://www.w3.org/2004/02/skos/core#Concept</skos:scopeNote>
		<skos:Note>SKOS properties defined in http://www.w3.org/TR/skos-primer/#secrel</skos:Note>
		<skos:inScheme rdf:resource="http://www.cognitiveatlas.org/tasks/"/>
		<skos:prefLabel>color naming task</skos:prefLabel>
		<skos:altLabel></skos:altLabel>
</skos:Concept><skos:Concept rdf:about="http://www.cognitiveatlas.org/id/trm_4f244d2a54e27"> <dc:identifier>trm_4f244d2a54e27</dc:identifier>
		<dc:Title>Cognitive Atlas : Lexicon : autobiographical memory task</dc:Title>
		<dc:Description>RDF output for 'autobiographical memory task'</dc:Description>
		<dc:Type>InteractiveResource</dc:Type>
		<dc:Publisher>Cognitive Atlas</dc:Publisher>
		<dc:Creator>Cognitive Atlas RDF Generator</dc:Creator>
		<dc:Contributor>Russ Poldrack</dc:Contributor>
		<dc:Date>2012-01-28 11:31:54</dc:Date>
		<dc:Format>text/rdf</dc:Format>
		<dc:Language>en</dc:Language>
		<skos:editorialNote>Generated by testgenall.php on Thu Mar 29 10:24:08 PDT 2012.</skos:editorialNote>
		<skos:historyNote>No previous definition revisions.</skos:historyNote>
		<skos:changeNote>This is the first and only definition provided.</skos:changeNote>
		<skos:scopeNote>http://www.w3.org/2004/02/skos/core#Concept</skos:scopeNote>
		<skos:Note>SKOS properties defined in http://www.w3.org/TR/skos-primer/#secrel</skos:Note>
		<skos:inScheme rdf:resource="http://www.cognitiveatlas.org/tasks/"/>
		<skos:prefLabel>autobiographical memory task</skos:prefLabel>
		<skos:altLabel></skos:altLabel>
		<skos:related rdf:resource="http://www.cognitiveatlas.org/id/trm_4a3fd79d09b10"/>
		<skos:example>autobiographical memory is measured by the contrast of  trials in the autobiographical memory task</skos:example>
</skos:Concept><skos:Concept rdf:about="http://www.cognitiveatlas.org/id/trm_4f244d64e45bc"> <dc:identifier>trm_4f244d64e45bc</dc:identifier>
		<dc:Title>Cognitive Atlas : Lexicon : negative priming task</dc:Title>
		<dc:Description>RDF output for 'negative priming task'</dc:Description>
		<dc:Type>InteractiveResource</dc:Type>
		<dc:Publisher>Cognitive Atlas</dc:Publisher>
		<dc:Creator>Cognitive Atlas RDF Generator</dc:Creator>
		<dc:Contributor>Russ Poldrack</dc:Contributor>
		<dc:Date>2012-01-28 11:32:52</dc:Date>
		<dc:Format>text/rdf</dc:Format>
		<dc:Language>en</dc:Language>
		<skos:editorialNote>Generated by testgenall.php on Thu Mar 29 10:24:08 PDT 2012.</skos:editorialNote>
		<skos:historyNote>No previous definition revisions.</skos:historyNote>
		<skos:changeNote>This is the first and only definition provided.</skos:changeNote>
		<skos:scopeNote>http://www.w3.org/2004/02/skos/core#Concept</skos:scopeNote>
		<skos:Note>SKOS properties defined in http://www.w3.org/TR/skos-primer/#secrel</skos:Note>
		<skos:inScheme rdf:resource="http://www.cognitiveatlas.org/tasks/"/>
		<skos:prefLabel>negative priming task</skos:prefLabel>
		<skos:altLabel></skos:altLabel>
</skos:Concept><skos:Concept rdf:about="http://www.cognitiveatlas.org/id/trm_4f244f0286947"> <dc:identifier>trm_4f244f0286947</dc:identifier>
		<dc:Title>Cognitive Atlas : Lexicon : analogical reasoning task</dc:Title>
		<dc:Description>RDF output for 'analogical reasoning task'</dc:Description>
		<dc:Type>InteractiveResource</dc:Type>
		<dc:Publisher>Cognitive Atlas</dc:Publisher>
		<dc:Creator>Cognitive Atlas RDF Generator</dc:Creator>
		<dc:Contributor>Russ Poldrack</dc:Contributor>
		<dc:Date>2012-01-28 11:39:46</dc:Date>
		<dc:Format>text/rdf</dc:Format>
		<dc:Language>en</dc:Language>
		<skos:editorialNote>Generated by testgenall.php on Thu Mar 29 10:24:08 PDT 2012.</skos:editorialNote>
		<skos:historyNote>No previous definition revisions.</skos:historyNote>
		<skos:changeNote>This is the first and only definition provided.</skos:changeNote>
		<skos:scopeNote>http://www.w3.org/2004/02/skos/core#Concept</skos:scopeNote>
		<skos:Note>SKOS properties defined in http://www.w3.org/TR/skos-primer/#secrel</skos:Note>
		<skos:inScheme rdf:resource="http://www.cognitiveatlas.org/tasks/"/>
		<skos:prefLabel>analogical reasoning task</skos:prefLabel>
		<skos:altLabel></skos:altLabel>
</skos:Concept><skos:Concept rdf:about="http://www.cognitiveatlas.org/id/trm_4f244f46ebf58"> <dc:identifier>trm_4f244f46ebf58</dc:identifier>
		<dc:Title>Cognitive Atlas : Lexicon : rapid serial visual presentation task</dc:Title>
		<dc:Description>RDF output for 'rapid serial visual presentation task'</dc:Description>
		<dc:Type>InteractiveResource</dc:Type>
		<dc:Publisher>Cognitive Atlas</dc:Publisher>
		<dc:Creator>Cognitive Atlas RDF Generator</dc:Creator>
		<dc:Contributor>Russ Poldrack</dc:Contributor>
		<dc:Date>2012-01-28 11:40:54</dc:Date>
		<dc:Format>text/rdf</dc:Format>
		<dc:Language>en</dc:Language>
		<skos:editorialNote>Generated by testgenall.php on Thu Mar 29 10:24:08 PDT 2012.</skos:editorialNote>
		<skos:historyNote>No previous definition revisions.</skos:historyNote>
		<skos:changeNote>This is the first and only definition provided.</skos:changeNote>
		<skos:scopeNote>http://www.w3.org/2004/02/skos/core#Concept</skos:scopeNote>
		<skos:Note>SKOS properties defined in http://www.w3.org/TR/skos-primer/#secrel</skos:Note>
		<skos:inScheme rdf:resource="http://www.cognitiveatlas.org/tasks/"/>
		<skos:prefLabel>rapid serial visual presentation task</skos:prefLabel>
		<skos:altLabel>RSVP task</skos:altLabel>
</skos:Concept><skos:Concept rdf:about="http://www.cognitiveatlas.org/id/trm_4f244f997615c"> <dc:identifier>trm_4f244f997615c</dc:identifier>
		<dc:Title>Cognitive Atlas : Lexicon : bimanual coordination task</dc:Title>
		<dc:Description>RDF output for 'bimanual coordination task'</dc:Description>
		<dc:Type>InteractiveResource</dc:Type>
		<dc:Publisher>Cognitive Atlas</dc:Publisher>
		<dc:Creator>Cognitive Atlas RDF Generator</dc:Creator>
		<dc:Contributor>Russ Poldrack</dc:Contributor>
		<dc:Date>2012-01-28 11:42:17</dc:Date>
		<dc:Format>text/rdf</dc:Format>
		<dc:Language>en</dc:Language>
		<skos:editorialNote>Generated by testgenall.php on Thu Mar 29 10:24:08 PDT 2012.</skos:editorialNote>
		<skos:historyNote>No previous definition revisions.</skos:historyNote>
		<skos:changeNote>This is the first and only definition provided.</skos:changeNote>
		<skos:scopeNote>http://www.w3.org/2004/02/skos/core#Concept</skos:scopeNote>
		<skos:Note>SKOS properties defined in http://www.w3.org/TR/skos-primer/#secrel</skos:Note>
		<skos:inScheme rdf:resource="http://www.cognitiveatlas.org/tasks/"/>
		<skos:prefLabel>bimanual coordination task</skos:prefLabel>
		<skos:altLabel></skos:altLabel>
</skos:Concept><skos:Concept rdf:about="http://www.cognitiveatlas.org/id/trm_4f244fee7d195"> <dc:identifier>trm_4f244fee7d195</dc:identifier>
		<dc:Title>Cognitive Atlas : Lexicon : multi-attribute decision making task</dc:Title>
		<dc:Description>RDF output for 'multi-attribute decision making task'</dc:Description>
		<dc:Type>InteractiveResource</dc:Type>
		<dc:Publisher>Cognitive Atlas</dc:Publisher>
		<dc:Creator>Cognitive Atlas RDF Generator</dc:Creator>
		<dc:Contributor>Russ Poldrack</dc:Contributor>
		<dc:Date>2012-01-28 11:43:42</dc:Date>
		<dc:Format>text/rdf</dc:Format>
		<dc:Language>en</dc:Language>
		<skos:editorialNote>Generated by testgenall.php on Thu Mar 29 10:24:08 PDT 2012.</skos:editorialNote>
		<skos:historyNote>No previous definition revisions.</skos:historyNote>
		<skos:changeNote>This is the first and only definition provided.</skos:changeNote>
		<skos:scopeNote>http://www.w3.org/2004/02/skos/core#Concept</skos:scopeNote>
		<skos:Note>SKOS properties defined in http://www.w3.org/TR/skos-primer/#secrel</skos:Note>
		<skos:inScheme rdf:resource="http://www.cognitiveatlas.org/tasks/"/>
		<skos:prefLabel>multi-attribute decision making task</skos:prefLabel>
		<skos:altLabel></skos:altLabel>
</skos:Concept><skos:Concept rdf:about="http://www.cognitiveatlas.org/id/trm_4f2452adb7d23"> <dc:identifier>trm_4f2452adb7d23</dc:identifier>
		<dc:Title>Cognitive Atlas : Lexicon : odd-even task</dc:Title>
		<dc:Description>RDF output for 'odd-even task'</dc:Description>
		<dc:Type>InteractiveResource</dc:Type>
		<dc:Publisher>Cognitive Atlas</dc:Publisher>
		<dc:Creator>Cognitive Atlas RDF Generator</dc:Creator>
		<dc:Contributor>Russ Poldrack</dc:Contributor>
		<dc:Date>2012-01-28 11:55:25</dc:Date>
		<dc:Format>text/rdf</dc:Format>
		<dc:Language>en</dc:Language>
		<skos:editorialNote>Generated by testgenall.php on Thu Mar 29 10:24:08 PDT 2012.</skos:editorialNote>
		<skos:historyNote>No previous definition revisions.</skos:historyNote>
		<skos:changeNote>This is the first and only definition provided.</skos:changeNote>
		<skos:scopeNote>http://www.w3.org/2004/02/skos/core#Concept</skos:scopeNote>
		<skos:Note>SKOS properties defined in http://www.w3.org/TR/skos-primer/#secrel</skos:Note>
		<skos:inScheme rdf:resource="http://www.cognitiveatlas.org/tasks/"/>
		<skos:prefLabel>odd-even task</skos:prefLabel>
		<skos:altLabel></skos:altLabel>
</skos:Concept><skos:Concept rdf:about="http://www.cognitiveatlas.org/id/trm_4f245326e2eaf"> <dc:identifier>trm_4f245326e2eaf</dc:identifier>
		<dc:Title>Cognitive Atlas : Lexicon : biological motion task</dc:Title>
		<dc:Description>RDF output for 'biological motion task'</dc:Description>
		<dc:Type>InteractiveResource</dc:Type>
		<dc:Publisher>Cognitive Atlas</dc:Publisher>
		<dc:Creator>Cognitive Atlas RDF Generator</dc:Creator>
		<dc:Contributor>Russ Poldrack</dc:Contributor>
		<dc:Date>2012-01-28 11:57:26</dc:Date>
		<dc:Format>text/rdf</dc:Format>
		<dc:Language>en</dc:Language>
		<skos:editorialNote>Generated by testgenall.php on Thu Mar 29 10:24:08 PDT 2012.</skos:editorialNote>
		<skos:historyNote>No previous definition revisions.</skos:historyNote>
		<skos:changeNote>This is the first and only definition provided.</skos:changeNote>
		<skos:scopeNote>http://www.w3.org/2004/02/skos/core#Concept</skos:scopeNote>
		<skos:Note>SKOS properties defined in http://www.w3.org/TR/skos-primer/#secrel</skos:Note>
		<skos:inScheme rdf:resource="http://www.cognitiveatlas.org/tasks/"/>
		<skos:prefLabel>biological motion task</skos:prefLabel>
		<skos:altLabel></skos:altLabel>
</skos:Concept><skos:Concept rdf:about="http://www.cognitiveatlas.org/id/trm_4f2453b806fe1"> <dc:identifier>trm_4f2453b806fe1</dc:identifier>
		<dc:Title>Cognitive Atlas : Lexicon : spatial working memory task</dc:Title>
		<dc:Description>RDF output for 'spatial working memory task'</dc:Description>
		<dc:Type>InteractiveResource</dc:Type>
		<dc:Publisher>Cognitive Atlas</dc:Publisher>
		<dc:Creator>Cognitive Atlas RDF Generator</dc:Creator>
		<dc:Contributor>Russ Poldrack</dc:Contributor>
		<dc:Date>2012-01-28 11:59:52</dc:Date>
		<dc:Format>text/rdf</dc:Format>
		<dc:Language>en</dc:Language>
		<skos:editorialNote>Generated by testgenall.php on Thu Mar 29 10:24:08 PDT 2012.</skos:editorialNote>
		<skos:historyNote>No previous definition revisions.</skos:historyNote>
		<skos:changeNote>This is the first and only definition provided.</skos:changeNote>
		<skos:scopeNote>http://www.w3.org/2004/02/skos/core#Concept</skos:scopeNote>
		<skos:Note>SKOS properties defined in http://www.w3.org/TR/skos-primer/#secrel</skos:Note>
		<skos:inScheme rdf:resource="http://www.cognitiveatlas.org/tasks/"/>
		<skos:prefLabel>spatial working memory task</skos:prefLabel>
		<skos:altLabel></skos:altLabel>
</skos:Concept><skos:Concept rdf:about="http://www.cognitiveatlas.org/id/trm_4f2453ce33f16"> <dc:identifier>trm_4f2453ce33f16</dc:identifier>
		<dc:Title>Cognitive Atlas : Lexicon : social judgment task</dc:Title>
		<dc:Description>RDF output for 'social judgment task'</dc:Description>
		<dc:Type>InteractiveResource</dc:Type>
		<dc:Publisher>Cognitive Atlas</dc:Publisher>
		<dc:Creator>Cognitive Atlas RDF Generator</dc:Creator>
		<dc:Contributor>Russ Poldrack</dc:Contributor>
		<dc:Date>2012-01-28 12:00:14</dc:Date>
		<dc:Format>text/rdf</dc:Format>
		<dc:Language>en</dc:Language>
		<skos:editorialNote>Generated by testgenall.php on Thu Mar 29 10:24:08 PDT 2012.</skos:editorialNote>
		<skos:historyNote>No previous definition revisions.</skos:historyNote>
		<skos:changeNote>This is the first and only definition provided.</skos:changeNote>
		<skos:scopeNote>http://www.w3.org/2004/02/skos/core#Concept</skos:scopeNote>
		<skos:Note>SKOS properties defined in http://www.w3.org/TR/skos-primer/#secrel</skos:Note>
		<skos:inScheme rdf:resource="http://www.cognitiveatlas.org/tasks/"/>
		<skos:prefLabel>social judgment task</skos:prefLabel>
		<skos:altLabel></skos:altLabel>
</skos:Concept><skos:Concept rdf:about="http://www.cognitiveatlas.org/id/trm_4f2454dfca337"> <dc:identifier>trm_4f2454dfca337</dc:identifier>
		<dc:Title>Cognitive Atlas : Lexicon : relational reasoning task</dc:Title>
		<dc:Description>RDF output for 'relational reasoning task'</dc:Description>
		<dc:Type>InteractiveResource</dc:Type>
		<dc:Publisher>Cognitive Atlas</dc:Publisher>
		<dc:Creator>Cognitive Atlas RDF Generator</dc:Creator>
		<dc:Contributor>Russ Poldrack</dc:Contributor>
		<dc:Date>2012-01-28 12:04:47</dc:Date>
		<dc:Format>text/rdf</dc:Format>
		<dc:Language>en</dc:Language>
		<skos:editorialNote>Generated by testgenall.php on Thu Mar 29 10:24:08 PDT 2012.</skos:editorialNote>
		<skos:historyNote>No previous definition revisions.</skos:historyNote>
		<skos:changeNote>This is the first and only definition provided.</skos:changeNote>
		<skos:scopeNote>http://www.w3.org/2004/02/skos/core#Concept</skos:scopeNote>
		<skos:Note>SKOS properties defined in http://www.w3.org/TR/skos-primer/#secrel</skos:Note>
		<skos:inScheme rdf:resource="http://www.cognitiveatlas.org/tasks/"/>
		<skos:prefLabel>relational reasoning task</skos:prefLabel>
		<skos:altLabel></skos:altLabel>
</skos:Concept><skos:Concept rdf:about="http://www.cognitiveatlas.org/id/trm_4f24550fc5f38"> <dc:identifier>trm_4f24550fc5f38</dc:identifier>
		<dc:Title>Cognitive Atlas : Lexicon : prototype distortion task</dc:Title>
		<dc:Description>RDF output for 'prototype distortion task'</dc:Description>
		<dc:Type>InteractiveResource</dc:Type>
		<dc:Publisher>Cognitive Atlas</dc:Publisher>
		<dc:Creator>Cognitive Atlas RDF Generator</dc:Creator>
		<dc:Contributor>Russ Poldrack</dc:Contributor>
		<dc:Date>2012-01-28 12:05:35</dc:Date>
		<dc:Format>text/rdf</dc:Format>
		<dc:Language>en</dc:Language>
		<skos:editorialNote>Generated by testgenall.php on Thu Mar 29 10:24:08 PDT 2012.</skos:editorialNote>
		<skos:historyNote>No previous definition revisions.</skos:historyNote>
		<skos:changeNote>This is the first and only definition provided.</skos:changeNote>
		<skos:scopeNote>http://www.w3.org/2004/02/skos/core#Concept</skos:scopeNote>
		<skos:Note>SKOS properties defined in http://www.w3.org/TR/skos-primer/#secrel</skos:Note>
		<skos:inScheme rdf:resource="http://www.cognitiveatlas.org/tasks/"/>
		<skos:prefLabel>prototype distortion task</skos:prefLabel>
		<skos:altLabel></skos:altLabel>
</skos:Concept><skos:Concept rdf:about="http://www.cognitiveatlas.org/id/trm_4f2456027809f"> <dc:identifier>trm_4f2456027809f</dc:identifier>
		<dc:Title>Cognitive Atlas : Lexicon : false belief task</dc:Title>
		<dc:Description>RDF output for 'false belief task'</dc:Description>
		<dc:Type>InteractiveResource</dc:Type>
		<dc:Publisher>Cognitive Atlas</dc:Publisher>
		<dc:Creator>Cognitive Atlas RDF Generator</dc:Creator>
		<dc:Contributor>Russ Poldrack</dc:Contributor>
		<dc:Date>2012-01-28 12:09:38</dc:Date>
		<dc:Format>text/rdf</dc:Format>
		<dc:Language>en</dc:Language>
		<skos:editorialNote>Generated by testgenall.php on Thu Mar 29 10:24:08 PDT 2012.</skos:editorialNote>
		<skos:historyNote>No previous definition revisions.</skos:historyNote>
		<skos:changeNote>This is the first and only definition provided.</skos:changeNote>
		<skos:scopeNote>http://www.w3.org/2004/02/skos/core#Concept</skos:scopeNote>
		<skos:Note>SKOS properties defined in http://www.w3.org/TR/skos-primer/#secrel</skos:Note>
		<skos:inScheme rdf:resource="http://www.cognitiveatlas.org/tasks/"/>
		<skos:prefLabel>false belief task</skos:prefLabel>
		<skos:altLabel></skos:altLabel>
</skos:Concept><skos:Concept rdf:about="http://www.cognitiveatlas.org/id/trm_4f2456932f11b"> <dc:identifier>trm_4f2456932f11b</dc:identifier>
		<dc:Title>Cognitive Atlas : Lexicon : shadowing task</dc:Title>
		<dc:Description>RDF output for 'shadowing task'</dc:Description>
		<dc:Type>InteractiveResource</dc:Type>
		<dc:Publisher>Cognitive Atlas</dc:Publisher>
		<dc:Creator>Cognitive Atlas RDF Generator</dc:Creator>
		<dc:Contributor>Russ Poldrack</dc:Contributor>
		<dc:Date>2012-01-28 12:12:03</dc:Date>
		<dc:Format>text/rdf</dc:Format>
		<dc:Language>en</dc:Language>
		<skos:editorialNote>Generated by testgenall.php on Thu Mar 29 10:24:08 PDT 2012.</skos:editorialNote>
		<skos:historyNote>No previous definition revisions.</skos:historyNote>
		<skos:changeNote>This is the first and only definition provided.</skos:changeNote>
		<skos:scopeNote>http://www.w3.org/2004/02/skos/core#Concept</skos:scopeNote>
		<skos:Note>SKOS properties defined in http://www.w3.org/TR/skos-primer/#secrel</skos:Note>
		<skos:inScheme rdf:resource="http://www.cognitiveatlas.org/tasks/"/>
		<skos:prefLabel>shadowing task</skos:prefLabel>
		<skos:altLabel></skos:altLabel>
</skos:Concept><skos:Concept rdf:about="http://www.cognitiveatlas.org/id/trm_4f24572cb42e4"> <dc:identifier>trm_4f24572cb42e4</dc:identifier>
		<dc:Title>Cognitive Atlas : Lexicon : parity judgment task</dc:Title>
		<dc:Description>RDF output for 'parity judgment task'</dc:Description>
		<dc:Type>InteractiveResource</dc:Type>
		<dc:Publisher>Cognitive Atlas</dc:Publisher>
		<dc:Creator>Cognitive Atlas RDF Generator</dc:Creator>
		<dc:Contributor>Russ Poldrack</dc:Contributor>
		<dc:Date>2012-01-28 12:14:36</dc:Date>
		<dc:Format>text/rdf</dc:Format>
		<dc:Language>en</dc:Language>
		<skos:editorialNote>Generated by testgenall.php on Thu Mar 29 10:24:08 PDT 2012.</skos:editorialNote>
		<skos:historyNote>No previous definition revisions.</skos:historyNote>
		<skos:changeNote>This is the first and only definition provided.</skos:changeNote>
		<skos:scopeNote>http://www.w3.org/2004/02/skos/core#Concept</skos:scopeNote>
		<skos:Note>SKOS properties defined in http://www.w3.org/TR/skos-primer/#secrel</skos:Note>
		<skos:inScheme rdf:resource="http://www.cognitiveatlas.org/tasks/"/>
		<skos:prefLabel>parity judgment task</skos:prefLabel>
		<skos:altLabel></skos:altLabel>
</skos:Concept><skos:Concept rdf:about="http://www.cognitiveatlas.org/id/trm_4f2457454e458"> <dc:identifier>trm_4f2457454e458</dc:identifier>
		<dc:Title>Cognitive Atlas : Lexicon : numerosity estimation task</dc:Title>
		<dc:Description>RDF output for 'numerosity estimation task'</dc:Description>
		<dc:Type>InteractiveResource</dc:Type>
		<dc:Publisher>Cognitive Atlas</dc:Publisher>
		<dc:Creator>Cognitive Atlas RDF Generator</dc:Creator>
		<dc:Contributor>Russ Poldrack</dc:Contributor>
		<dc:Date>2012-01-28 12:15:01</dc:Date>
		<dc:Format>text/rdf</dc:Format>
		<dc:Language>en</dc:Language>
		<skos:editorialNote>Generated by testgenall.php on Thu Mar 29 10:24:08 PDT 2012.</skos:editorialNote>
		<skos:historyNote>No previous definition revisions.</skos:historyNote>
		<skos:changeNote>This is the first and only definition provided.</skos:changeNote>
		<skos:scopeNote>http://www.w3.org/2004/02/skos/core#Concept</skos:scopeNote>
		<skos:Note>SKOS properties defined in http://www.w3.org/TR/skos-primer/#secrel</skos:Note>
		<skos:inScheme rdf:resource="http://www.cognitiveatlas.org/tasks/"/>
		<skos:prefLabel>numerosity estimation task</skos:prefLabel>
		<skos:altLabel></skos:altLabel>
</skos:Concept><skos:Concept rdf:about="http://www.cognitiveatlas.org/id/trm_4f2457a8b0bc8"> <dc:identifier>trm_4f2457a8b0bc8</dc:identifier>
		<dc:Title>Cognitive Atlas : Lexicon : verbal working memory task</dc:Title>
		<dc:Description>RDF output for 'verbal working memory task'</dc:Description>
		<dc:Type>InteractiveResource</dc:Type>
		<dc:Publisher>Cognitive Atlas</dc:Publisher>
		<dc:Creator>Cognitive Atlas RDF Generator</dc:Creator>
		<dc:Contributor>Russ Poldrack</dc:Contributor>
		<dc:Date>2012-01-28 12:16:40</dc:Date>
		<dc:Format>text/rdf</dc:Format>
		<dc:Language>en</dc:Language>
		<skos:editorialNote>Generated by testgenall.php on Thu Mar 29 10:24:08 PDT 2012.</skos:editorialNote>
		<skos:historyNote>No previous definition revisions.</skos:historyNote>
		<skos:changeNote>This is the first and only definition provided.</skos:changeNote>
		<skos:scopeNote>http://www.w3.org/2004/02/skos/core#Concept</skos:scopeNote>
		<skos:Note>SKOS properties defined in http://www.w3.org/TR/skos-primer/#secrel</skos:Note>
		<skos:inScheme rdf:resource="http://www.cognitiveatlas.org/tasks/"/>
		<skos:definition>A class of tasks involving the online maintenance and/or manipulation of verbal information.</skos:definition>
		<skos:prefLabel>verbal working memory task</skos:prefLabel>
		<skos:altLabel></skos:altLabel>
</skos:Concept><skos:Concept rdf:about="http://www.cognitiveatlas.org/id/trm_4f2457d94fd93"> <dc:identifier>trm_4f2457d94fd93</dc:identifier>
		<dc:Title>Cognitive Atlas : Lexicon : memory guided saccade task</dc:Title>
		<dc:Description>RDF output for 'memory guided saccade task'</dc:Description>
		<dc:Type>InteractiveResource</dc:Type>
		<dc:Publisher>Cognitive Atlas</dc:Publisher>
		<dc:Creator>Cognitive Atlas RDF Generator</dc:Creator>
		<dc:Contributor>Russ Poldrack</dc:Contributor>
		<dc:Date>2012-01-28 12:17:29</dc:Date>
		<dc:Format>text/rdf</dc:Format>
		<dc:Language>en</dc:Language>
		<skos:editorialNote>Generated by testgenall.php on Thu Mar 29 10:24:08 PDT 2012.</skos:editorialNote>
		<skos:historyNote>No previous definition revisions.</skos:historyNote>
		<skos:changeNote>This is the first and only definition provided.</skos:changeNote>
		<skos:scopeNote>http://www.w3.org/2004/02/skos/core#Concept</skos:scopeNote>
		<skos:Note>SKOS properties defined in http://www.w3.org/TR/skos-primer/#secrel</skos:Note>
		<skos:inScheme rdf:resource="http://www.cognitiveatlas.org/tasks/"/>
		<skos:prefLabel>memory guided saccade task</skos:prefLabel>
		<skos:altLabel></skos:altLabel>
</skos:Concept></rdf:RDF>